# baseURI: <https://w3id.org/osdu#>
# imports: http://topbraid.org/schema/schema-single-range/
# imports: http://www.w3.org/2004/02/skos/core#
# imports: http://www.w3.org/2002/07/owl#
# imports: http://www.w3.org/1999/02/22-rdf-syntax-ns#
# imports: http://www.w3.org/XML/1998/namespace#
# imports: http://www.w3.org/2001/XMLSchema#
# imports: https://w3id.org/osdu#
# imports: http://www.w3.org/2000/01/rdf-schema#
# imports: http://www.w3.org/2004/02/skos/core#
# imports: http://www.w3.org/2006/time#
# imports: http://xmlns.com/foaf/0.1/
# imports: http://www.w3.org/ns/auth/acl#
# imports: https://www.geonames.org/ontology/ontology_v3.3.rdf/
# prefix: osdu


@prefix : <https://w3id.org/osdu#> .
@prefix owl: <http://www.w3.org/2002/07/owl#> .
@prefix rdf: <http://www.w3.org/1999/02/22-rdf-syntax-ns#> .
@prefix dc: <http://purl.org/dc/elements/1.1/> .
@prefix xml: <http://www.w3.org/XML/1998/namespace#> .
@prefix xsd: <http://www.w3.org/2001/XMLSchema#> .
@prefix osdu: <https://w3id.org/osdu#> .
@prefix rdfs: <http://www.w3.org/2000/01/rdf-schema#> .
@prefix skos:<http://www.w3.org/2004/02/skos/core#> .
@prefix time:<http://www.w3.org/2006/time#> .
@prefix foaf:<http://xmlns.com/foaf/0.1/> .
@prefix acl:<http://www.w3.org/ns/auth/acl#> .
@prefix gn:<https://www.geonames.org/ontology/ontology_v3.3.rdf/> .
@base <https://w3id.org/osdu#> .


#################################################################
#    Annotation properties
#################################################################

###  http://purl.org/dc/elements/1.1/creator
dc:creator rdf:type owl:AnnotationProperty .


###  http://purl.org/dc/elements/1.1/title
dc:title rdf:type owl:AnnotationProperty .


###  http://www.w3.org/2001/XMLSchema#pattern
xsd:pattern rdf:type owl:AnnotationProperty .


###  http://www.w3.org/2002/07/owl#minCardinality
owl:minCardinality rdf:type owl:AnnotationProperty .


<https://w3id.org/osdu#> rdf:type owl:Ontology ;
                          <http://purl.org/dc/elements/1.1/creator> "Neda Abolhassani, Ph.D."^^xsd:string ;
                          <http://purl.org/dc/elements/1.1/creator> "Ana Tudor, M.S."^^xsd:string ;
                          <http://purl.org/dc/elements/1.1/title> "OSDU Ontology"^^xsd:string ;
                          owl:imports rdf: ;
                          owl:imports rdfs: ;
                          owl:imports xsd: ;
                          owl:imports owl: ;
                          owl:imports skos: ;
                          owl:imports time: ;
                          owl:imports <http://www.w3.org/XML/1998/namespace#> ;
                          owl:imports <http://www.w3.org/ns/auth/acl#> ;
                          owl:imports <http://xmlns.com/foaf/0.1/> ;
                          owl:imports foaf: ;
                          owl:imports <https://www.geonames.org/ontology/ontology_v3.3.rdf> ;
                          owl:versionInfo "Version 1.0" ;
.


#################################################################
#    Classes
#################################################################

###  https://w3id.org/osdu#ACL
osdu:ACL rdf:type owl:Class ;
	skos:prefLabel "Access Control List" ;
	rdfs:comment "The access control tags associated with this entity. This structure is included by the SystemProperties acl, which is part of all OSDU records. Not extensible. " ;
	rdfs:subClassOf owl:Thing ;
.

###  https://w3id.org/osdu#AbstractAccessControlList
osdu:AbstractAccessControlList rdf:type owl:Class ;
	rdfs:subClassOf owl:Thing ;
	rdfs:subClassOf [
		a owl:Restriction ;
		owl:onProperty osdu:owner ;
		owl:minCardinality "1"^^xsd:nonNegativeInteger ;
	] ;
	rdfs:subClassOf [
		a owl:Restriction ;
		owl:onProperty osdu:viewer ;
		owl:minCardinality "1"^^xsd:nonNegativeInteger ;
	] ;
.

###  https://w3id.org/osdu#AbstractActivityParameter
osdu:AbstractActivityParameter rdf:type owl:Class ;
	rdfs:comment "General parameter value used in one instance of activity. [Without inheritance, combined specializations.] " ;
	rdfs:subClassOf owl:Thing ;
	rdfs:subClassOf [
		a owl:Restriction ;
		owl:onProperty osdu:title ;
		owl:minCardinality "1"^^xsd:nonNegativeInteger ;
	] ;
	rdfs:subClassOf [
		a owl:Restriction ;
		owl:onProperty osdu:parameterKindID ;
		owl:minCardinality "1"^^xsd:nonNegativeInteger ;
	] ;
.

###  https://w3id.org/osdu#AbstractAliasNames
osdu:AbstractAliasNames rdf:type owl:Class ;
	rdfs:comment "A list of alternative names for an object.  The preferred name is in a separate, scalar property.  It may or may not be repeated in the alias list, though a best practice is to include it if the list is present, but to omit the list if there are no other names.  Note that the abstract entity is an array so the $ref to it is a simple property reference. " ;
	rdfs:subClassOf owl:Thing ;
.

###  https://w3id.org/osdu#AbstractAnyCrsFeatureCollection
osdu:AbstractAnyCrsFeatureCollection rdf:type owl:Class ;
	rdfs:comment "A schema like GeoJSON FeatureCollection with a non-WGS 84 CRS context; based on https://geojson.org/schema/FeatureCollection.json. Attention: the coordinate order is fixed: Longitude/Easting/Westing/X first, followed by Latitude/Northing/Southing/Y, optionally height as third coordinate. " ;
	rdfs:subClassOf owl:Thing ;
	rdfs:subClassOf [
		a owl:Restriction ;
		owl:onProperty osdu:hasBBox ;
		owl:minQualifiedCardinality "4"^^xsd:nonNegativeInteger ;
		owl:onDataRange xsd:decimal ;
	] ;
	rdfs:subClassOf [
		a owl:Restriction ;
		owl:onProperty osdu:type ;
		owl:minCardinality "1"^^xsd:nonNegativeInteger ;
	] ;
	rdfs:subClassOf [
		a owl:Restriction ;
		owl:onProperty osdu:persistableReferenceCRS ;
		owl:minCardinality "1"^^xsd:nonNegativeInteger ;
	] ;
	rdfs:subClassOf [
		a owl:Restriction ;
		owl:onProperty osdu:hasFeatures ;
		owl:minCardinality "1"^^xsd:nonNegativeInteger ;
	] ;
.

###  https://w3id.org/osdu#AbstractBinGrid
osdu:AbstractBinGrid rdf:type owl:Class ;
	rdfs:comment "The shared properties for a bin grid. " ;
	rdfs:subClassOf owl:Thing ;
.

###  https://w3id.org/osdu#AbstractBusinessRule
osdu:AbstractBusinessRule rdf:type owl:Class ;
	rdfs:comment "The business rule is a collection of one or more data rule sets with their run status as well as a collection of individual rules with their run status. " ;
	rdfs:subClassOf owl:Thing ;
.

###  https://w3id.org/osdu#AbstractColumnBasedTable
osdu:AbstractColumnBasedTable rdf:type owl:Class ;
	rdfs:comment "The ColumnBasedTable is a set of columns, which have equal length (data.ColumnSize) included by types carrying embedded table properties. Columns have a Property Kind, UnitOfMeasure and Facet. There are KeyColumns (index columns) and Columns (for look-up values). Examples are KrPc, PVT and Facies tables. " ;
	rdfs:subClassOf owl:Thing ;
.

###  https://w3id.org/osdu#AbstractColumnLayerGridPatch
osdu:AbstractColumnLayerGridPatch rdf:type owl:Class ;
	rdfs:comment "The group of elements which all column grid layers (ijk or unstructured) contain " ;
	rdfs:subClassOf owl:Thing ;
.

###  https://w3id.org/osdu#AbstractCommonResources
osdu:AbstractCommonResources rdf:type owl:Class ;
	skos:prefLabel "OSDU Common Resources" ;
	rdfs:comment "Common resources to be injected at root 'data' level for every entity, which is persistable in Storage. The insertion is performed by the OsduSchemaComposer script. " ;
	rdfs:subClassOf owl:Thing ;
.

###  https://w3id.org/osdu#AbstractCompressionInfo
osdu:AbstractCompressionInfo rdf:type owl:Class ;
	rdfs:comment "A schema fragment containing information about the compression applied. This is typically included for types supporting compression in the dataset group-type. " ;
	rdfs:subClassOf owl:Thing ;
.

###  https://w3id.org/osdu#AbstractContact
osdu:AbstractContact rdf:type owl:Class ;
	skos:prefLabel "Abstract Contact" ;
	rdfs:comment "An object with properties that describe a specific person or other point-of-contact (like an email distribution list) that is relevant in this context (like a given data set or business project). The contact specified may be either internal or external to the organisation (something denoted via the Organisation object that is referenced). Note that some properties contain personally identifiable information, so it might not be appropriate to populate all properties in all scenarios. " ;
	rdfs:subClassOf owl:Thing ;
.

###  https://w3id.org/osdu#AbstractCoordinates
osdu:AbstractCoordinates rdf:type owl:Class ;
	rdfs:comment "A geographic position on the surface of the earth. " ;
	rdfs:subClassOf owl:Thing ;
.

###  https://w3id.org/osdu#AbstractDataset
osdu:AbstractDataset rdf:type owl:Class ;
	rdfs:comment "Schema fragment holding properties common for all datasets. " ;
	rdfs:subClassOf owl:Thing ;
	rdfs:subClassOf [
		a owl:Restriction ;
		owl:onProperty osdu:hasDatasetProperties ;
		owl:minCardinality "1"^^xsd:nonNegativeInteger ;
	] ;
.

###  https://w3id.org/osdu#AbstractFacet
osdu:AbstractFacet rdf:type owl:Class ;
	rdfs:comment "A tuple FacetType, FacetRole, both calling specific references  FacetType: Enumeration of the type of additional context about the nature of a property type (it may include conditions, direction, qualifiers, or statistics).   FacetRole: Additional context about the nature of a property type. The purpose of such attribute is to minimize the need to create specialized property types by mutualizing some well known qualifiers such as maximum, minimum which apply to a lot of different property types. " ;
	rdfs:subClassOf owl:Thing ;
	rdfs:subClassOf [
		a owl:Restriction ;
		owl:onProperty osdu:facetTypeID ;
		owl:minCardinality "1"^^xsd:nonNegativeInteger ;
	] ;
	rdfs:subClassOf [
		a owl:Restriction ;
		owl:onProperty osdu:facetRoleID ;
		owl:minCardinality "1"^^xsd:nonNegativeInteger ;
	] ;
.

###  https://w3id.org/osdu#AbstractFacility
osdu:AbstractFacility rdf:type owl:Class ;
	rdfs:comment "The schema fragment included by facilities. A facility is a grouping of equipment that is located within a specific geographic boundary or site and that is used in the context of energy-related activities such as exploration, extraction, generation, storage, processing, disposal, supply, or transfer. Clarifications: (1) A facility may be surface or subsurface located. (2) Usually facility equipment is commonly owned or operated. (3) Industry definitions may vary and differ from this one. This schema fragment is included by Well, Wellbore, Rig, as well as Tank Batteries, Compression Stations, Storage Facilities, Wind Farms, Wind Turbines, Mining Facilities, etc., once these types are included in to the OSDU. " ;
	rdfs:subClassOf owl:Thing ;
.

###  https://w3id.org/osdu#AbstractFacilityEvent
osdu:AbstractFacilityEvent rdf:type owl:Class ;
	rdfs:comment "A significant occurrence in the life of a facility, which often changes its state, or the state of one of its components. It can describe a point-in-time (event) or a time interval of a specific type (FacilityEventType). " ;
	rdfs:subClassOf owl:Thing ;
.

###  https://w3id.org/osdu#AbstractFacilityOperator
osdu:AbstractFacilityOperator rdf:type owl:Class ;
	rdfs:comment "The organisation that was responsible for a facility at some point in time. " ;
	rdfs:subClassOf owl:Thing ;
.

###  https://w3id.org/osdu#AbstractFacilitySpecification
osdu:AbstractFacilitySpecification rdf:type owl:Class ;
	rdfs:comment "A property, characteristic, or attribute about a facility that is not described explicitly elsewhere. " ;
	rdfs:subClassOf owl:Thing ;
.

###  https://w3id.org/osdu#AbstractFacilityState
osdu:AbstractFacilityState rdf:type owl:Class ;
	rdfs:comment "The life cycle status of a facility at some point in time. " ;
	rdfs:subClassOf owl:Thing ;
.

###  https://w3id.org/osdu#AbstractFacilityVerticalMeasurement
osdu:AbstractFacilityVerticalMeasurement rdf:type owl:Class ;
	rdfs:comment "A location along a wellbore, _usually_ associated with some aspect of the drilling of the wellbore, but not with any intersecting _subsurface_ natural surfaces. " ;
	rdfs:subClassOf owl:Thing ;
.

###  https://w3id.org/osdu#AbstractFeatureCollection
osdu:AbstractFeatureCollection rdf:type owl:Class ;
	skos:prefLabel "GeoJSON FeatureCollection" ;
	rdfs:comment "GeoJSON feature collection as originally published in https://geojson.org/schema/FeatureCollection.json. Attention: the coordinate order is fixed: Longitude first, followed by Latitude, optionally height above MSL (EPSG:5714) as third coordinate. " ;
	rdfs:subClassOf owl:Thing ;
	rdfs:subClassOf [
		a owl:Restriction ;
		owl:onProperty osdu:hasBBox ;
		owl:minQualifiedCardinality "4"^^xsd:nonNegativeInteger ;
		owl:onDataRange xsd:decimal ;
	] ;
	rdfs:subClassOf [
		a owl:Restriction ;
		owl:onProperty osdu:type ;
		owl:minCardinality "1"^^xsd:nonNegativeInteger ;
	] ;
	rdfs:subClassOf [
		a owl:Restriction ;
		owl:onProperty osdu:hasFeatures ;
		owl:minCardinality "1"^^xsd:nonNegativeInteger ;
	] ;
.

###  https://w3id.org/osdu#AbstractFile
osdu:AbstractFile rdf:type owl:Class ;
	rdfs:comment "The schema fragment representing single files " ;
	rdfs:subClassOf owl:Thing ;
	rdfs:subClassOf [
		a owl:Restriction ;
		owl:onProperty osdu:hasDatasetProperties ;
		owl:minCardinality "1"^^xsd:nonNegativeInteger ;
	] ;
.

###  https://w3id.org/osdu#AbstractFileCollection
osdu:AbstractFileCollection rdf:type owl:Class ;
	rdfs:comment "The schema fragment representing file collections. " ;
	rdfs:subClassOf owl:Thing ;
	rdfs:subClassOf [
		a owl:Restriction ;
		owl:onProperty osdu:hasDatasetProperties ;
		owl:minCardinality "1"^^xsd:nonNegativeInteger ;
	] ;
.

###  https://w3id.org/osdu#AbstractFileSourceInfo
osdu:AbstractFileSourceInfo rdf:type owl:Class ;
	rdfs:comment "A schema fragment to describe file source information. " ;
	rdfs:subClassOf owl:Thing ;
	rdfs:subClassOf [
		a owl:Restriction ;
		owl:onProperty osdu:fileSource ;
		owl:minCardinality "1"^^xsd:nonNegativeInteger ;
	] ;
.

###  https://w3id.org/osdu#AbstractGeoBasinContext
osdu:AbstractGeoBasinContext rdf:type owl:Class ;
	rdfs:comment "A single, typed basin entity reference, which is 'abstracted' to AbstractGeoContext and then aggregated by GeoContexts properties. " ;
	rdfs:subClassOf osdu:AbstractGeoContext ;
.

###  https://w3id.org/osdu#AbstractGeoContext
osdu:AbstractGeoContext rdf:type owl:Class ;
	rdfs:comment "A geographic context to an entity. It can be either a reference to a GeoPoliticalEntity, Basin, Field, Play or Prospect. " ;
	rdfs:subClassOf owl:Thing ;
.

###  https://w3id.org/osdu#AbstractGeoFieldContext
osdu:AbstractGeoFieldContext rdf:type owl:Class ;
	rdfs:comment "A single, typed field entity reference, which is 'abstracted' to AbstractGeoContext and then aggregated by GeoContexts properties. " ;
	rdfs:subClassOf osdu:AbstractGeoContext ;
.

###  https://w3id.org/osdu#AbstractGeoPlayContext
osdu:AbstractGeoPlayContext rdf:type owl:Class ;
	rdfs:comment "A single, typed Play entity reference, which is 'abstracted' to AbstractGeoContext and then aggregated by GeoContexts properties. " ;
	rdfs:subClassOf osdu:AbstractGeoContext ;
.

###  https://w3id.org/osdu#AbstractGeoPoliticalContext
osdu:AbstractGeoPoliticalContext rdf:type owl:Class ;
	rdfs:comment "A single, typed geo-political entity reference, which is 'abstracted' to AbstractGeoContext and then aggregated by GeoContexts properties. " ;
	rdfs:subClassOf osdu:AbstractGeoContext ;
.

###  https://w3id.org/osdu#AbstractGeoProspectContext
osdu:AbstractGeoProspectContext rdf:type owl:Class ;
	rdfs:comment "A single, typed Prospect entity reference, which is 'abstracted' to AbstractGeoContext and then aggregated by GeoContexts properties. " ;
	rdfs:subClassOf osdu:AbstractGeoContext ;
.

###  https://w3id.org/osdu#AbstractGeologicUnitInterpretation
osdu:AbstractGeologicUnitInterpretation rdf:type owl:Class ;
	rdfs:comment "Common properties for entities describing an opinion of a volume-based geologic feature or unit. " ;
	rdfs:subClassOf owl:Thing ;
.

###  https://w3id.org/osdu#AbstractGridRepresentation
osdu:AbstractGridRepresentation rdf:type owl:Class ;
	rdfs:comment "The group of elements contained by all different kind of grids " ;
	rdfs:subClassOf osdu:AbstractRepresentation ;
.

###  https://w3id.org/osdu#AbstractIjkGridFlowSimulationBoundaryConnection
osdu:AbstractIjkGridFlowSimulationBoundaryConnection rdf:type owl:Class ;
	rdfs:comment "This structure intends to define the reservoir boundary connection in an IJK grid such as aquifer connection. It can be reused in various Ijk Grid flow simulation related representations which need some boundary connections. " ;
	rdfs:subClassOf owl:Thing ;
.

###  https://w3id.org/osdu#AbstractIjkGridPatch
osdu:AbstractIjkGridPatch rdf:type owl:Class ;
	rdfs:comment "Definition of a collection of hexahedra which are organized and indexable by means of 3 (almost orthogonal) directions and called I, J and K. Only an abstract group type in order to be reused in GPGrid. " ;
	rdfs:subClassOf osdu:AbstractColumnLayerGridPatch ;
.

###  https://w3id.org/osdu#AbstractInterpretation
osdu:AbstractInterpretation rdf:type owl:Class ;
	rdfs:comment "The group of properties shared by different kinds of interpretations " ;
	rdfs:subClassOf owl:Thing ;
.

###  https://w3id.org/osdu#AbstractLegalParentList
osdu:AbstractLegalParentList rdf:type owl:Class ;
	skos:prefLabel "Parent List" ;
	rdfs:comment "A list of entity id:version references to record instances recorded in the data platform, from which the current record is derived and from which the legal tags must be derived. This structure is included by the SystemProperties ancestry, which is part of all OSDU records. Not extensible. " ;
	rdfs:subClassOf owl:Thing ;
.

###  https://w3id.org/osdu#AbstractLegalTags
osdu:AbstractLegalTags rdf:type owl:Class ;
	skos:prefLabel "Legal Meta Data" ;
	rdfs:comment "Legal meta data like legal tags, relevant other countries, legal status. This structure is included by the SystemProperties legal, which is part of all OSDU records. Not extensible. " ;
	rdfs:subClassOf owl:Thing ;
	rdfs:subClassOf [
		a owl:Restriction ;
		owl:onProperty osdu:legalTags ;
		owl:minCardinality "1"^^xsd:nonNegativeInteger ;
	] ;
	rdfs:subClassOf [
		a owl:Restriction ;
		owl:onProperty osdu:otherRelevantDataCountries ;
		owl:minCardinality "1"^^xsd:nonNegativeInteger ;
	] ;
.

###  https://w3id.org/osdu#AbstractMaster
osdu:AbstractMaster rdf:type owl:Class ;
	skos:prefLabel "Abstract Master" ;
	rdfs:comment "Properties shared with all master-data schema instances. " ;
	rdfs:subClassOf owl:Thing ;
.

###  https://w3id.org/osdu#AbstractMetaItem
osdu:AbstractMetaItem rdf:type owl:Class ;
	skos:prefLabel "Frame of Reference Meta Data Item" ;
	rdfs:comment "A meta data item, which allows the association of named properties or property values to a Unit/Measurement/CRS/Azimuth/Time context. " ;
	rdfs:subClassOf owl:Thing ;
.

###  https://w3id.org/osdu#AbstractProject
osdu:AbstractProject rdf:type owl:Class ;
	rdfs:comment "A Project is a business activity that consumes financial and human resources and produces (digital) work products. " ;
	rdfs:subClassOf owl:Thing ;
.

###  https://w3id.org/osdu#AbstractProjectActivity
osdu:AbstractProjectActivity rdf:type owl:Class ;
	rdfs:comment "The activity abstraction for projects and surveys (master-data). " ;
	rdfs:subClassOf owl:Thing ;
.

###  https://w3id.org/osdu#AbstractPropertyType
osdu:AbstractPropertyType rdf:type owl:Class ;
	rdfs:comment "A nested object holding the relationship to a PropertyType by id (uuid) and a derived, human-readable name. " ;
	rdfs:subClassOf owl:Thing ;
.

###  https://w3id.org/osdu#AbstractQualityMetric
osdu:AbstractQualityMetric rdf:type owl:Class ;
	rdfs:comment "Generic quality metric schema fragment containing the universal properties for data profiling and data metrics of OSDU objects. " ;
	rdfs:subClassOf owl:Thing ;
.

###  https://w3id.org/osdu#AbstractReferenceLevel
osdu:AbstractReferenceLevel rdf:type owl:Class ;
	rdfs:comment "A reference level or horizontal reference surface definition, which can be used embedded in other schemas. " ;
	rdfs:subClassOf owl:Thing ;
.

###  https://w3id.org/osdu#AbstractReferencePropertyType
osdu:AbstractReferencePropertyType rdf:type owl:Class ;
	rdfs:comment "The purpose of this schema is best understood in the context of a columnar dataset: the AbstractReferencePropertyType describes a column in a columnar dataset by declaring its value type (number, string), a UnitQuantity if the value type is a number, a kind if the string value is actually a relationship to a e.g. reference-data type. " ;
	rdfs:subClassOf owl:Thing ;
.

###  https://w3id.org/osdu#AbstractReferenceType
osdu:AbstractReferenceType rdf:type owl:Class ;
	rdfs:comment "Generic reference object containing the universal properties of reference data, especially the ones commonly thought of as Types " ;
	rdfs:subClassOf owl:Thing ;
.

###  https://w3id.org/osdu#AbstractRepresentation
osdu:AbstractRepresentation rdf:type owl:Class ;
	rdfs:comment "The group of properties shared by all different kinds of representations. " ;
	rdfs:subClassOf owl:Thing ;
.

###  https://w3id.org/osdu#AbstractSpatialLocation
osdu:AbstractSpatialLocation rdf:type owl:Class ;
	rdfs:comment "A geographic object which can be described by a set of points. " ;
	rdfs:subClassOf owl:Thing ;
.

###  https://w3id.org/osdu#AbstractSpatialReference
osdu:AbstractSpatialReference rdf:type owl:Class ;
	rdfs:comment "A schema fragment providing a spatial reference context, i.e. relationship(s) to CoordinateReferenceSystem instances and persistable reference strings (self-contained, engine consumable CRS definitions). " ;
	rdfs:subClassOf owl:Thing ;
.

###  https://w3id.org/osdu#AbstractSpecification
osdu:AbstractSpecification rdf:type owl:Class ;
	rdfs:comment "An array element of an analysis specifying the numeric, text or date-time value associated with a ParameterType. " ;
	rdfs:subClassOf owl:Thing ;
.

###  https://w3id.org/osdu#AbstractStorageLocation
osdu:AbstractStorageLocation rdf:type owl:Class ;
	rdfs:comment "A record about the storage location of an item, e.g. a rock or fluid sample, seismic tape, where (facility), by whom (organisation), when (dates) and how (description). " ;
	rdfs:subClassOf owl:Thing ;
.

###  https://w3id.org/osdu#AbstractSystemProperties
osdu:AbstractSystemProperties rdf:type owl:Class ;
	rdfs:subClassOf owl:Thing ;
	rdfs:subClassOf [
		a owl:Restriction ;
		owl:onProperty osdu:kind ;
		owl:minCardinality "1"^^xsd:nonNegativeInteger ;
	] ;
	rdfs:subClassOf [
		a owl:Restriction ;
		owl:onProperty osdu:acl ;
		owl:minCardinality "1"^^xsd:nonNegativeInteger ;
	] ;
	rdfs:subClassOf [
		a owl:Restriction ;
		owl:onProperty osdu:legal ;
		owl:minCardinality "1"^^xsd:nonNegativeInteger ;
	] ;
.

###  https://w3id.org/osdu#AbstractTechnicalAssurance
osdu:AbstractTechnicalAssurance rdf:type owl:Class ;
	rdfs:comment "Describes a record's overall suitability for general business consumption based on level of trust. " ;
	rdfs:subClassOf owl:Thing ;
	rdfs:subClassOf [
		a owl:Restriction ;
		owl:onProperty osdu:technicalAssuranceTypeID ;
		owl:minCardinality "1"^^xsd:nonNegativeInteger ;
	] ;
.

###  https://w3id.org/osdu#AbstractUnstructuredColumnLayerGridPatch
osdu:AbstractUnstructuredColumnLayerGridPatch rdf:type owl:Class ;
	rdfs:comment "Definition of a collection of polyhedra which are only organized by column. Only an abstract group type in order to be reused in GPGrid. " ;
	rdfs:subClassOf osdu:AbstractColumnLayerGridPatch ;
.

###  https://w3id.org/osdu#AbstractUnstructuredGridPatch
osdu:AbstractUnstructuredGridPatch rdf:type owl:Class ;
	rdfs:comment "Definition of a collection of polyhedra which are not organized in any dimension. Only an abstract group type in order to be reused in GPGrid. " ;
	rdfs:subClassOf owl:Thing ;
.

###  https://w3id.org/osdu#AbstractVectorHeaderMapping
osdu:AbstractVectorHeaderMapping rdf:type owl:Class ;
	rdfs:comment "Array of objects which define the meaning and format of a tabular structure used in a binary file as a header.  The initial use case is the trace headers of a SEG-Y file.  Note that some of this information may be repeated in the SEG-Y EBCDIC header. " ;
	rdfs:subClassOf owl:Thing ;
.

###  https://w3id.org/osdu#AbstractWPCActivity
osdu:AbstractWPCActivity rdf:type owl:Class ;
	rdfs:comment "The activity abstraction included by projects (master-data) and work-product-component group-type specialisations. " ;
	rdfs:subClassOf owl:Thing ;
	rdfs:subClassOf [
		a owl:Restriction ;
		owl:onProperty osdu:parameters ;
		owl:minCardinality "1"^^xsd:nonNegativeInteger ;
	] ;
.

###  https://w3id.org/osdu#AbstractWPCGroupType
osdu:AbstractWPCGroupType rdf:type owl:Class ;
	rdfs:comment "Generic reference object containing the universal group-type properties of a Work Product Component for inclusion in data type specific Work Product Component objects " ;
	rdfs:subClassOf owl:Thing ;
.

###  https://w3id.org/osdu#AbstractWellboreDrillingReason
osdu:AbstractWellboreDrillingReason rdf:type owl:Class ;
	rdfs:comment "Purpose for drilling a wellbore, which often is an indication of the level of risk. " ;
	rdfs:subClassOf owl:Thing ;
.

###  https://w3id.org/osdu#AbstractWorkProductComponent
osdu:AbstractWorkProductComponent rdf:type owl:Class ;
	rdfs:comment "Generic reference object containing the universal properties of a Work Product Component for inclusion in data type specific Work Product Component objects " ;
	rdfs:subClassOf owl:Thing ;
.

###  https://w3id.org/osdu#AcceptableUsage
osdu:AcceptableUsage rdf:type owl:Class ;
	rdfs:comment "Describes the workflows and/or personas that the technical assurance value is valid for (e.g., This data has a technical assurance property of trusted and it is suitable for Seismic Interpretation). " ;
	rdfs:subClassOf owl:Thing ;
.

###  https://w3id.org/osdu#AcquisitionDateRanges
osdu:AcquisitionDateRanges rdf:type owl:Class ;
	skos:prefLabel "Acquisition Date Ranges" ;
	rdfs:comment "Defines the start and end date of the processing completed on the dataset " ;
	rdfs:subClassOf owl:Thing ;
.

###  https://w3id.org/osdu#Activity
osdu:Activity rdf:type owl:Class ;
	rdfs:comment "Instance of a given activity " ;
	rdfs:subClassOf osdu:WorkProductComponent ;
	rdfs:subClassOf osdu:AbstractCommonResources ;
	rdfs:subClassOf osdu:AbstractWPCGroupType ;
	rdfs:subClassOf osdu:AbstractWorkProductComponent ;
	rdfs:subClassOf osdu:AbstractWPCActivity ;
.

###  https://w3id.org/osdu#ActivityCode
osdu:ActivityCode rdf:type owl:Class ;
	rdfs:comment "ActivityCode for Well Construction and Intervention (for L1), Construct well (for L2), Intervene well (for L2), … " ;
	rdfs:subClassOf osdu:ReferenceData ;
	rdfs:subClassOf osdu:AbstractCommonResources ;
	rdfs:subClassOf osdu:AbstractReferenceType ;
.

###  https://w3id.org/osdu#ActivityLevel
osdu:ActivityLevel rdf:type owl:Class ;
	rdfs:comment "Proposed reference values: L1, L2, L3, L4, L5, L6 " ;
	rdfs:subClassOf osdu:ReferenceData ;
	rdfs:subClassOf osdu:AbstractCommonResources ;
	rdfs:subClassOf osdu:AbstractReferenceType ;
.

###  https://w3id.org/osdu#ActivityOutcome
osdu:ActivityOutcome rdf:type owl:Class ;
	rdfs:comment "Possible outcomes from a drilling activity " ;
	rdfs:subClassOf osdu:ReferenceData ;
	rdfs:subClassOf osdu:AbstractCommonResources ;
	rdfs:subClassOf osdu:AbstractReferenceType ;
.

###  https://w3id.org/osdu#ActivityOutcomeDetail
osdu:ActivityOutcomeDetail rdf:type owl:Class ;
	rdfs:comment "Detailed outcomes from a drilling activity " ;
	rdfs:subClassOf osdu:ReferenceData ;
	rdfs:subClassOf osdu:AbstractCommonResources ;
	rdfs:subClassOf osdu:AbstractReferenceType ;
.

###  https://w3id.org/osdu#ActivityPlan
osdu:ActivityPlan rdf:type owl:Class ;
	rdfs:comment "Information about a series of planned activities. " ;
	rdfs:subClassOf osdu:MasterData ;
	rdfs:subClassOf osdu:AbstractCommonResources ;
	rdfs:subClassOf osdu:AbstractMaster ;
	rdfs:subClassOf osdu:AbstractProject ;
.

###  https://w3id.org/osdu#ActivityTemplate
osdu:ActivityTemplate rdf:type owl:Class ;
	rdfs:comment "Description of one type of activity, e.g., a work-step in a workflow. " ;
	rdfs:subClassOf osdu:MasterData ;
	rdfs:subClassOf osdu:AbstractCommonResources ;
	rdfs:subClassOf osdu:AbstractMaster ;
.

###  https://w3id.org/osdu#ActivityTemplateArc
osdu:ActivityTemplateArc rdf:type owl:Class ;
	rdfs:comment "An 'arc' establishing a link between ActivityTemplate output and input parameters. " ;
	rdfs:subClassOf osdu:MasterData ;
	rdfs:subClassOf osdu:AbstractCommonResources ;
	rdfs:subClassOf osdu:AbstractMaster ;
.

###  https://w3id.org/osdu#ActivityType
osdu:ActivityType rdf:type owl:Class ;
	rdfs:comment "Used to describe the type of activity the data results - such as RunActivity, PullActivity,... " ;
	rdfs:subClassOf osdu:ReferenceData ;
	rdfs:subClassOf osdu:AbstractCommonResources ;
	rdfs:subClassOf osdu:AbstractReferenceType ;
.

###  https://w3id.org/osdu#ActualIndicatorType
osdu:ActualIndicatorType rdf:type owl:Class ;
	rdfs:comment "DEPRECATED: (not used anywhere) Object that describes the actual planning status of an object - such as Tubular Assembly - to indicate if it is planned, concrete, prototyped or any other relevant status. " ;
	rdfs:subClassOf osdu:ReferenceData ;
	rdfs:subClassOf osdu:AbstractCommonResources ;
	rdfs:subClassOf osdu:AbstractReferenceType ;
.

###  https://w3id.org/osdu#AdditiveType
osdu:AdditiveType rdf:type owl:Class ;
	rdfs:comment "Items added to cement slurry or cement spacers, washes and fluids " ;
	rdfs:subClassOf osdu:ReferenceData ;
	rdfs:subClassOf osdu:AbstractCommonResources ;
	rdfs:subClassOf osdu:AbstractReferenceType ;
.

###  https://w3id.org/osdu#Agreement
osdu:Agreement rdf:type owl:Class ;
	rdfs:comment "A contract or other covenant between Company and counterparties which is relevant to the data universe because it includes terms governing use of data. " ;
	rdfs:subClassOf osdu:MasterData ;
	rdfs:subClassOf osdu:AbstractCommonResources ;
	rdfs:subClassOf osdu:AbstractMaster ;
.

###  https://w3id.org/osdu#AgreementType
osdu:AgreementType rdf:type owl:Class ;
	rdfs:comment "A kind of document, record or other publication containing the terms of an agreed understanding, undertaking, contract or mutual consent between two or more parties. " ;
	rdfs:subClassOf osdu:ReferenceData ;
	rdfs:subClassOf osdu:AbstractCommonResources ;
	rdfs:subClassOf osdu:AbstractReferenceType ;
.

###  https://w3id.org/osdu#AliasNameType
osdu:AliasNameType rdf:type owl:Class ;
	rdfs:comment "Used to describe the type of name aliases. " ;
	rdfs:subClassOf osdu:ReferenceData ;
	rdfs:subClassOf osdu:AbstractCommonResources ;
	rdfs:subClassOf osdu:AbstractReferenceType ;
.

###  https://w3id.org/osdu#AliasNameTypeClass
osdu:AliasNameTypeClass rdf:type owl:Class ;
	rdfs:comment "Used to describe the type of alias name types. AliasNameTypeClass is intended to be used to categorize alias name types by their general purpose, with values like Standard Identifier, System Identifier, and Moniker. Combined with the AliasNameType, and DefinitionOrganisation one can define a complete context for a particular identifier or name. For example, a standard identifier of type Regulatory ID, from API, is the US standards regulatory ID; a standard identifier of type company ID, from BigOil, is BigOil's Standard ID; System Identifiers would be particular to systems of record, or other systems, and Monikers, things like display names, plot labels, etc. " ;
	rdfs:subClassOf osdu:ReferenceData ;
	rdfs:subClassOf osdu:AbstractCommonResources ;
	rdfs:subClassOf osdu:AbstractReferenceType ;
.

###  https://w3id.org/osdu#AngleRange
osdu:AngleRange rdf:type owl:Class ;
	rdfs:comment "A range container carrying minimum/maximum angle values. " ;
	rdfs:subClassOf owl:Thing ;
.

###  https://w3id.org/osdu#AnisotropyType
osdu:AnisotropyType rdf:type owl:Class ;
	rdfs:comment "Describes the anisotropy model assumed and solved for such as Isotropic, VTI, HTI, TTI, Orthorhombic. " ;
	rdfs:subClassOf osdu:ReferenceData ;
	rdfs:subClassOf osdu:AbstractCommonResources ;
	rdfs:subClassOf osdu:AbstractReferenceType ;
.

###  https://w3id.org/osdu#AnnularFluidType
osdu:AnnularFluidType rdf:type owl:Class ;
	rdfs:comment "Type of fluid in wellbore at time of perforation job. " ;
	rdfs:subClassOf osdu:ReferenceData ;
	rdfs:subClassOf osdu:AbstractCommonResources ;
	rdfs:subClassOf osdu:AbstractReferenceType ;
.

###  https://w3id.org/osdu#AnyCrsGeoJSONFeature
osdu:AnyCrsGeoJSONFeature rdf:type owl:Class ;
	skos:prefLabel "AnyCrsGeoJSON Feature" ;
	rdfs:subClassOf owl:Thing ;
	rdfs:subClassOf [
		a owl:Restriction ;
		owl:onProperty osdu:hasBBox ;
		owl:minQualifiedCardinality "4"^^xsd:nonNegativeInteger ;
		owl:onDataRange xsd:decimal ;
	] ;
	rdfs:subClassOf [
		a owl:Restriction ;
		owl:onProperty osdu:type ;
		owl:minCardinality "1"^^xsd:nonNegativeInteger ;
	] ;
	rdfs:subClassOf [
		a owl:Restriction ;
		owl:onProperty osdu:property ;
		owl:minCardinality "1"^^xsd:nonNegativeInteger ;
	] ;
	rdfs:subClassOf [
		a owl:Restriction ;
		owl:onProperty osdu:geometry ;
		owl:minCardinality "1"^^xsd:nonNegativeInteger ;
	] ;
.

###  https://w3id.org/osdu#AnyCrsGeoJSONGeometryCollection
osdu:AnyCrsGeoJSONGeometryCollection rdf:type owl:Class ;
	skos:prefLabel "AnyCrsGeoJSON GeometryCollection" ;
	rdfs:subClassOf owl:Thing ;
	rdfs:subClassOf [
		a owl:Restriction ;
		owl:onProperty osdu:hasBBox ;
		owl:minQualifiedCardinality "4"^^xsd:nonNegativeInteger ;
		owl:onDataRange xsd:decimal ;
	] ;
	rdfs:subClassOf [
		a owl:Restriction ;
		owl:onProperty osdu:type ;
		owl:minCardinality "1"^^xsd:nonNegativeInteger ;
	] ;
	rdfs:subClassOf [
		a owl:Restriction ;
		owl:onProperty osdu:geometry ;
		owl:minCardinality "1"^^xsd:nonNegativeInteger ;
	] ;
.

###  https://w3id.org/osdu#AnyCrsGeoJSONLineString
osdu:AnyCrsGeoJSONLineString rdf:type owl:Class ;
	skos:prefLabel "AnyCrsGeoJSON LineString" ;
	rdfs:subClassOf osdu:Geometries ;
	rdfs:subClassOf [
		a owl:Restriction ;
		owl:onProperty osdu:coordinate ;
		owl:minQualifiedCardinality "2"^^xsd:nonNegativeInteger ;
		owl:onClass osdu:AnyCrsGeoJSONLineStringCoordinatesArray ;
	] ;
	rdfs:subClassOf [
		a owl:Restriction ;
		owl:onProperty osdu:hasBBox ;
		owl:minQualifiedCardinality "4"^^xsd:nonNegativeInteger ;
		owl:onDataRange xsd:decimal ;
	] ;
	rdfs:subClassOf [
		a owl:Restriction ;
		owl:onProperty osdu:type ;
		owl:minCardinality "1"^^xsd:nonNegativeInteger ;
	] ;
	rdfs:subClassOf [
		a owl:Restriction ;
		owl:onProperty osdu:coordinate ;
		owl:minCardinality "1"^^xsd:nonNegativeInteger ;
	] ;
.

###  https://w3id.org/osdu#AnyCrsGeoJSONLineStringCoordinatesArray
osdu:AnyCrsGeoJSONLineStringCoordinatesArray rdf:type owl:Class ;
	rdfs:subClassOf osdu:Array ;
	rdfs:subClassOf [
		a owl:Restriction ;
		owl:onProperty osdu:item ;
		owl:minQualifiedCardinality "2"^^xsd:nonNegativeInteger ;
		owl:onDataRange xsd:decimal ;
	] ;
.

###  https://w3id.org/osdu#AnyCrsGeoJSONMultiLineString
osdu:AnyCrsGeoJSONMultiLineString rdf:type owl:Class ;
	skos:prefLabel "AnyCrsGeoJSON MultiLineString" ;
	rdfs:subClassOf osdu:Geometries ;
	rdfs:subClassOf [
		a owl:Restriction ;
		owl:onProperty osdu:hasBBox ;
		owl:minQualifiedCardinality "4"^^xsd:nonNegativeInteger ;
		owl:onDataRange xsd:decimal ;
	] ;
	rdfs:subClassOf [
		a owl:Restriction ;
		owl:onProperty osdu:type ;
		owl:minCardinality "1"^^xsd:nonNegativeInteger ;
	] ;
	rdfs:subClassOf [
		a owl:Restriction ;
		owl:onProperty osdu:coordinate ;
		owl:minCardinality "1"^^xsd:nonNegativeInteger ;
	] ;
.

###  https://w3id.org/osdu#AnyCrsGeoJSONMultiLineStringCoordinatesArray
osdu:AnyCrsGeoJSONMultiLineStringCoordinatesArray rdf:type owl:Class ;
	rdfs:subClassOf osdu:Array ;
	rdfs:subClassOf [
		a owl:Restriction ;
		owl:onProperty osdu:item ;
		owl:minQualifiedCardinality "2"^^xsd:nonNegativeInteger ;
		owl:onClass osdu:AnyCrsGeoJSONMultiLineStringCoordinatesArrayItemsArray ;
	] ;
.

###  https://w3id.org/osdu#AnyCrsGeoJSONMultiLineStringCoordinatesArrayItemsArray
osdu:AnyCrsGeoJSONMultiLineStringCoordinatesArrayItemsArray rdf:type owl:Class ;
	rdfs:subClassOf osdu:Array ;
	rdfs:subClassOf [
		a owl:Restriction ;
		owl:onProperty osdu:item ;
		owl:minQualifiedCardinality "2"^^xsd:nonNegativeInteger ;
		owl:onDataRange xsd:decimal ;
	] ;
.

###  https://w3id.org/osdu#AnyCrsGeoJSONMultiPoint
osdu:AnyCrsGeoJSONMultiPoint rdf:type owl:Class ;
	skos:prefLabel "AnyCrsGeoJSON MultiPoint" ;
	rdfs:subClassOf osdu:Geometries ;
	rdfs:subClassOf [
		a owl:Restriction ;
		owl:onProperty osdu:hasBBox ;
		owl:minQualifiedCardinality "4"^^xsd:nonNegativeInteger ;
		owl:onDataRange xsd:decimal ;
	] ;
	rdfs:subClassOf [
		a owl:Restriction ;
		owl:onProperty osdu:type ;
		owl:minCardinality "1"^^xsd:nonNegativeInteger ;
	] ;
	rdfs:subClassOf [
		a owl:Restriction ;
		owl:onProperty osdu:coordinate ;
		owl:minCardinality "1"^^xsd:nonNegativeInteger ;
	] ;
.

###  https://w3id.org/osdu#AnyCrsGeoJSONMultiPointCoordinatesArray
osdu:AnyCrsGeoJSONMultiPointCoordinatesArray rdf:type owl:Class ;
	rdfs:subClassOf osdu:Array ;
	rdfs:subClassOf [
		a owl:Restriction ;
		owl:onProperty osdu:item ;
		owl:minQualifiedCardinality "2"^^xsd:nonNegativeInteger ;
		owl:onDataRange xsd:decimal ;
	] ;
.

###  https://w3id.org/osdu#AnyCrsGeoJSONMultiPolygon
osdu:AnyCrsGeoJSONMultiPolygon rdf:type owl:Class ;
	skos:prefLabel "AnyCrsGeoJSON MultiPolygon" ;
	rdfs:subClassOf osdu:Geometries ;
	rdfs:subClassOf [
		a owl:Restriction ;
		owl:onProperty osdu:hasBBox ;
		owl:minQualifiedCardinality "4"^^xsd:nonNegativeInteger ;
		owl:onDataRange xsd:decimal ;
	] ;
	rdfs:subClassOf [
		a owl:Restriction ;
		owl:onProperty osdu:type ;
		owl:minCardinality "1"^^xsd:nonNegativeInteger ;
	] ;
	rdfs:subClassOf [
		a owl:Restriction ;
		owl:onProperty osdu:coordinate ;
		owl:minCardinality "1"^^xsd:nonNegativeInteger ;
	] ;
.

###  https://w3id.org/osdu#AnyCrsGeoJSONMultiPolygonCoordinatesArray
osdu:AnyCrsGeoJSONMultiPolygonCoordinatesArray rdf:type owl:Class ;
	rdfs:subClassOf osdu:Array ;
.

###  https://w3id.org/osdu#AnyCrsGeoJSONMultiPolygonCoordinatesArrayItemsArray
osdu:AnyCrsGeoJSONMultiPolygonCoordinatesArrayItemsArray rdf:type owl:Class ;
	rdfs:subClassOf osdu:Array ;
	rdfs:subClassOf [
		a owl:Restriction ;
		owl:onProperty osdu:item ;
		owl:minQualifiedCardinality "4"^^xsd:nonNegativeInteger ;
		owl:onClass osdu:AnyCrsGeoJSONMultiPolygonCoordinatesArrayItemsArrayItemsArray ;
	] ;
.

###  https://w3id.org/osdu#AnyCrsGeoJSONMultiPolygonCoordinatesArrayItemsArrayItemsArray
osdu:AnyCrsGeoJSONMultiPolygonCoordinatesArrayItemsArrayItemsArray rdf:type owl:Class ;
	rdfs:subClassOf osdu:Array ;
	rdfs:subClassOf [
		a owl:Restriction ;
		owl:onProperty osdu:item ;
		owl:minQualifiedCardinality "2"^^xsd:nonNegativeInteger ;
		owl:onDataRange xsd:decimal ;
	] ;
.

###  https://w3id.org/osdu#AnyCrsGeoJSONPoint
osdu:AnyCrsGeoJSONPoint rdf:type owl:Class ;
	skos:prefLabel "AnyCrsGeoJSON Point" ;
	rdfs:subClassOf osdu:Geometries ;
	rdfs:subClassOf [
		a owl:Restriction ;
		owl:onProperty osdu:coordinate ;
		owl:minQualifiedCardinality "2"^^xsd:nonNegativeInteger ;
		owl:onDataRange xsd:decimal ;
	] ;
	rdfs:subClassOf [
		a owl:Restriction ;
		owl:onProperty osdu:hasBBox ;
		owl:minQualifiedCardinality "4"^^xsd:nonNegativeInteger ;
		owl:onDataRange xsd:decimal ;
	] ;
	rdfs:subClassOf [
		a owl:Restriction ;
		owl:onProperty osdu:type ;
		owl:minCardinality "1"^^xsd:nonNegativeInteger ;
	] ;
	rdfs:subClassOf [
		a owl:Restriction ;
		owl:onProperty osdu:coordinate ;
		owl:minCardinality "1"^^xsd:nonNegativeInteger ;
	] ;
.

###  https://w3id.org/osdu#AnyCrsGeoJSONPolygon
osdu:AnyCrsGeoJSONPolygon rdf:type owl:Class ;
	skos:prefLabel "AnyCrsGeoJSON Polygon" ;
	rdfs:subClassOf osdu:Geometries ;
	rdfs:subClassOf [
		a owl:Restriction ;
		owl:onProperty osdu:hasBBox ;
		owl:minQualifiedCardinality "4"^^xsd:nonNegativeInteger ;
		owl:onDataRange xsd:decimal ;
	] ;
	rdfs:subClassOf [
		a owl:Restriction ;
		owl:onProperty osdu:type ;
		owl:minCardinality "1"^^xsd:nonNegativeInteger ;
	] ;
	rdfs:subClassOf [
		a owl:Restriction ;
		owl:onProperty osdu:coordinate ;
		owl:minCardinality "1"^^xsd:nonNegativeInteger ;
	] ;
.

###  https://w3id.org/osdu#AnyCrsGeoJSONPolygonCoordinatesArray
osdu:AnyCrsGeoJSONPolygonCoordinatesArray rdf:type owl:Class ;
	rdfs:subClassOf osdu:Array ;
	rdfs:subClassOf [
		a owl:Restriction ;
		owl:onProperty osdu:item ;
		owl:minQualifiedCardinality "4"^^xsd:nonNegativeInteger ;
		owl:onClass osdu:AnyCrsGeoJSONPolygonCoordinatesArrayItemsArray ;
	] ;
.

###  https://w3id.org/osdu#AnyCrsGeoJSONPolygonCoordinatesArrayItemsArray
osdu:AnyCrsGeoJSONPolygonCoordinatesArrayItemsArray rdf:type owl:Class ;
	rdfs:subClassOf osdu:Array ;
	rdfs:subClassOf [
		a owl:Restriction ;
		owl:onProperty osdu:item ;
		owl:minQualifiedCardinality "2"^^xsd:nonNegativeInteger ;
		owl:onDataRange xsd:decimal ;
	] ;
.

###  https://w3id.org/osdu#AquiferInterpretation
osdu:AquiferInterpretation rdf:type owl:Class ;
	rdfs:comment "An interpretation of a RockVolumeFeature as water-bearing rocks " ;
	rdfs:subClassOf osdu:WorkProductComponent ;
	rdfs:subClassOf osdu:AbstractCommonResources ;
	rdfs:subClassOf osdu:AbstractWPCGroupType ;
	rdfs:subClassOf osdu:AbstractWorkProductComponent ;
	rdfs:subClassOf osdu:AbstractInterpretation ;
.

###  https://w3id.org/osdu#Arc
osdu:Arc rdf:type owl:Class ;
	rdfs:comment "An 'arc' establishing a link between a single pair of ActivityTemplate input and output parameters. " ;
	rdfs:subClassOf owl:Thing ;
	rdfs:subClassOf [
		a owl:Restriction ;
		owl:onProperty osdu:producingActivityTemplateID ;
		owl:minCardinality "1"^^xsd:nonNegativeInteger ;
	] ;
	rdfs:subClassOf [
		a owl:Restriction ;
		owl:onProperty osdu:producingParameterTitle ;
		owl:minCardinality "1"^^xsd:nonNegativeInteger ;
	] ;
	rdfs:subClassOf [
		a owl:Restriction ;
		owl:onProperty osdu:consumingActivityTemplateID ;
		owl:minCardinality "1"^^xsd:nonNegativeInteger ;
	] ;
	rdfs:subClassOf [
		a owl:Restriction ;
		owl:onProperty osdu:consumingParameterTitle ;
		owl:minCardinality "1"^^xsd:nonNegativeInteger ;
	] ;
	rdfs:subClassOf [
		a owl:Restriction ;
		owl:onProperty osdu:precedingActivityTemplateID ;
		owl:minCardinality "1"^^xsd:nonNegativeInteger ;
	] ;
	rdfs:subClassOf [
		a owl:Restriction ;
		owl:onProperty osdu:succeedingActivityTemplateID ;
		owl:minCardinality "1"^^xsd:nonNegativeInteger ;
	] ;
.

###  https://w3id.org/osdu#Array
osdu:Array rdf:type owl:Class ;
	rdfs:subClassOf owl:Thing ;
.

###  https://w3id.org/osdu#ArtefactRole
osdu:ArtefactRole rdf:type owl:Class ;
	rdfs:comment "A representation of some or all of an original product adapted to a purpose. " ;
	rdfs:subClassOf osdu:ReferenceData ;
	rdfs:subClassOf osdu:AbstractCommonResources ;
	rdfs:subClassOf osdu:AbstractReferenceType ;
.

###  https://w3id.org/osdu#Artefacts
osdu:Artefacts rdf:type owl:Class ;
	rdfs:comment "An array of Artefacts - each artefact has a Role, Resource tuple. An artefact is distinct from the file, in the sense certain valuable information is generated during loading process (Artefact generation process). Examples include retrieving location data, performing an OCR which may result in the generation of artefacts which need to be preserved distinctly " ;
	rdfs:subClassOf owl:Thing ;
.

###  https://w3id.org/osdu#ArtificialLiftType
osdu:ArtificialLiftType rdf:type owl:Class ;
	rdfs:comment "Used to reflect the type of Artificial Lift the data went out - 'Surface Pump', 'Submersible Pump',... " ;
	rdfs:subClassOf osdu:ReferenceData ;
	rdfs:subClassOf osdu:AbstractCommonResources ;
	rdfs:subClassOf osdu:AbstractReferenceType ;
.

###  https://w3id.org/osdu#AuthorityCode
osdu:AuthorityCode rdf:type owl:Class ;
	skos:prefLabel "Method Authority Code" ;
	rdfs:comment "The authority code corresponding to the ISO19111 ID and 'projjson' id. " ;
	rdfs:subClassOf owl:Thing ;
.

###  https://w3id.org/osdu#AzimuthReferenceType
osdu:AzimuthReferenceType rdf:type owl:Class ;
	rdfs:comment "The definition of north in a spatial reference survey. A reference table identifying valid north references used in surveying to define angular measurements " ;
	rdfs:subClassOf osdu:ReferenceData ;
	rdfs:subClassOf osdu:AbstractCommonResources ;
	rdfs:subClassOf osdu:AbstractReferenceType ;
.

###  https://w3id.org/osdu#BHARun
osdu:BHARun rdf:type owl:Class ;
	rdfs:comment "A single bottom hole assembly run. This represents the period beginning when the BHA enters the hole until it leaves the hole. " ;
	rdfs:subClassOf osdu:MasterData ;
	rdfs:subClassOf osdu:AbstractCommonResources ;
	rdfs:subClassOf osdu:AbstractMaster ;
	rdfs:subClassOf osdu:AbstractProject ;
.

###  https://w3id.org/osdu#BarrelFormulation
osdu:BarrelFormulation rdf:type owl:Class ;
	skos:prefLabel "Barrel Formulation" ;
	rdfs:comment "Description of the formulation of the barrel that will be part of the drilling mud " ;
	rdfs:subClassOf owl:Thing ;
	rdfs:subClassOf [
		a owl:Restriction ;
		owl:onProperty osdu:productName ;
		owl:minCardinality "1"^^xsd:nonNegativeInteger ;
	] ;
.

###  https://w3id.org/osdu#BaseCRS
osdu:BaseCRS rdf:type owl:Class ;
	skos:prefLabel "Base CRS" ;
	rdfs:comment "The base geographic CRS of this projected CRS. Only populated for CoordinateReferenceSystemType==ProjectedCRS. " ;
	rdfs:subClassOf owl:Thing ;
.

###  https://w3id.org/osdu#Basin
osdu:Basin rdf:type owl:Class ;
	rdfs:comment "A natural geographic area covering a single depositional system. " ;
	rdfs:subClassOf osdu:MasterData ;
	rdfs:subClassOf osdu:AbstractCommonResources ;
	rdfs:subClassOf osdu:AbstractMaster ;
.

###  https://w3id.org/osdu#BasinType
osdu:BasinType rdf:type owl:Class ;
	rdfs:comment "A geologic region where an accumulation of deposited sediments has depressed or is preserved within the crust. " ;
	rdfs:subClassOf osdu:ReferenceData ;
	rdfs:subClassOf osdu:AbstractCommonResources ;
	rdfs:subClassOf osdu:AbstractReferenceType ;
.

###  https://w3id.org/osdu#BBox
osdu:BBox rdf:type owl:Class ;
	rdfs:comment "A class for capturing ordered coordinates for a bounded box" ;
	rdfs:subClassOf osdu:Array ;
.

###  https://w3id.org/osdu#BhaStatus
osdu:BhaStatus rdf:type owl:Class ;
	rdfs:comment "The status of the Bottom Hole Assembly. Proposed reference values: final, progress, plan, unknown " ;
	rdfs:subClassOf osdu:ReferenceData ;
	rdfs:subClassOf osdu:AbstractCommonResources ;
	rdfs:subClassOf osdu:AbstractReferenceType ;
.

###  https://w3id.org/osdu#BinGridDefinitionMethodType
osdu:BinGridDefinitionMethodType rdf:type owl:Class ;
	rdfs:comment "Mathematical model describing generation of nodes for a regular grid.  Either 4 corner points using perspective transformation or P6 for origin and direction using affine operation. " ;
	rdfs:subClassOf osdu:ReferenceData ;
	rdfs:subClassOf osdu:AbstractCommonResources ;
	rdfs:subClassOf osdu:AbstractReferenceType ;
.

###  https://w3id.org/osdu#BitDullCode
osdu:BitDullCode rdf:type owl:Class ;
	rdfs:comment "The IADC bit dull codes " ;
	rdfs:subClassOf osdu:ReferenceData ;
	rdfs:subClassOf osdu:AbstractCommonResources ;
	rdfs:subClassOf osdu:AbstractReferenceType ;
.

###  https://w3id.org/osdu#BitReasonPulled
osdu:BitReasonPulled rdf:type owl:Class ;
	rdfs:comment "The IADC list of reasons why a bit might have been pulled " ;
	rdfs:subClassOf osdu:ReferenceData ;
	rdfs:subClassOf osdu:AbstractCommonResources ;
	rdfs:subClassOf osdu:AbstractReferenceType ;
.

###  https://w3id.org/osdu#BitRecord
osdu:BitRecord rdf:type owl:Class ;
	rdfs:comment "Information on the condition of the Drill Bit as recorded during an operations report " ;
	rdfs:subClassOf owl:Thing ;
	rdfs:subClassOf [
		a owl:Restriction ;
		owl:onProperty osdu:numBit ;
		owl:minCardinality "1"^^xsd:nonNegativeInteger ;
	] ;
.

###  https://w3id.org/osdu#BitType
osdu:BitType rdf:type owl:Class ;
	rdfs:comment "The general type of drilling bit used to create a wellbore interval. " ;
	rdfs:subClassOf osdu:ReferenceData ;
	rdfs:subClassOf osdu:AbstractCommonResources ;
	rdfs:subClassOf osdu:AbstractReferenceType ;
.

###  https://w3id.org/osdu#BottomHolePressureType
osdu:BottomHolePressureType rdf:type owl:Class ;
	rdfs:comment "The Method used to calculate or measure bottomhole pressure during perforation job. " ;
	rdfs:subClassOf osdu:ReferenceData ;
	rdfs:subClassOf osdu:AbstractCommonResources ;
	rdfs:subClassOf osdu:AbstractReferenceType ;
.

###  https://w3id.org/osdu#BoundaryFeature
osdu:BoundaryFeature rdf:type owl:Class ;
	rdfs:comment "An interface between two geological objects, such as horizons and faults. It is a surface object. " ;
	rdfs:subClassOf osdu:MasterData ;
	rdfs:subClassOf osdu:AbstractCommonResources ;
	rdfs:subClassOf osdu:AbstractMaster ;
.

###  https://w3id.org/osdu#BoundaryRelationType
osdu:BoundaryRelationType rdf:type owl:Class ;
	rdfs:comment "Describes the boundary relation of a body with surrounding stratigraphic units: unconformable, conformable " ;
	rdfs:subClassOf osdu:ReferenceData ;
	rdfs:subClassOf osdu:AbstractCommonResources ;
	rdfs:subClassOf osdu:AbstractReferenceType ;
.

###  https://w3id.org/osdu#CalculationMethodType
osdu:CalculationMethodType rdf:type owl:Class ;
	rdfs:comment "The method to calculate a wellbore path from the discrete station measurements of a wellbore directional survey. " ;
	rdfs:subClassOf osdu:ReferenceData ;
	rdfs:subClassOf osdu:AbstractCommonResources ;
	rdfs:subClassOf osdu:AbstractReferenceType ;
.

###  https://w3id.org/osdu#CasingDesign
osdu:CasingDesign rdf:type owl:Class ;
	rdfs:comment "The design of the Casing in a wellbore " ;
	rdfs:subClassOf osdu:MasterData ;
	rdfs:subClassOf osdu:AbstractCommonResources ;
	rdfs:subClassOf osdu:AbstractMaster ;
.

###  https://w3id.org/osdu#CatalogMapStateType
osdu:CatalogMapStateType rdf:type owl:Class ;
	rdfs:comment "A qualification of a mapping between catalog items. Mappings can be between 'identical' items, similar but not identical items or not supported. " ;
	rdfs:subClassOf osdu:ReferenceData ;
	rdfs:subClassOf osdu:AbstractCommonResources ;
	rdfs:subClassOf osdu:AbstractReferenceType ;
.

###  https://w3id.org/osdu#CellShapeType
osdu:CellShapeType rdf:type owl:Class ;
	rdfs:comment "An enumeration of cell shape types based on the RESQML model, i.e. tetrahedral, pyramidal, prism, hexahedral, polyhedral. " ;
	rdfs:subClassOf osdu:ReferenceData ;
	rdfs:subClassOf osdu:AbstractCommonResources ;
	rdfs:subClassOf osdu:AbstractReferenceType ;
.

###  https://w3id.org/osdu#CementAdditive
osdu:CementAdditive rdf:type owl:Class ;
	skos:prefLabel "Cement Additive" ;
	rdfs:comment "Additives used during a cement job " ;
	rdfs:subClassOf owl:Thing ;
	rdfs:subClassOf [
		a owl:Restriction ;
		owl:onProperty osdu:additiveName ;
		owl:minCardinality "1"^^xsd:nonNegativeInteger ;
	] ;
	rdfs:subClassOf [
		a owl:Restriction ;
		owl:onProperty osdu:additiveAmount ;
		owl:minCardinality "1"^^xsd:nonNegativeInteger ;
	] ;
	rdfs:subClassOf [
		a owl:Restriction ;
		owl:onProperty osdu:typeConc ;
		owl:minCardinality "1"^^xsd:nonNegativeInteger ;
	] ;
	rdfs:subClassOf [
		a owl:Restriction ;
		owl:onProperty osdu:concentration ;
		owl:minCardinality "1"^^xsd:nonNegativeInteger ;
	] ;
	rdfs:subClassOf [
		a owl:Restriction ;
		owl:onProperty osdu:wtSack ;
		owl:minCardinality "1"^^xsd:nonNegativeInteger ;
	] ;
	rdfs:subClassOf [
		a owl:Restriction ;
		owl:onProperty osdu:volSack ;
		owl:minCardinality "1"^^xsd:nonNegativeInteger ;
	] ;
.

###  https://w3id.org/osdu#CementJobType
osdu:CementJobType rdf:type owl:Class ;
	rdfs:comment "A single cement job. Possible Values: Primary, Plug, Squeeze, Unknown " ;
	rdfs:subClassOf osdu:ReferenceData ;
	rdfs:subClassOf osdu:AbstractCommonResources ;
	rdfs:subClassOf osdu:AbstractReferenceType ;
.

###  https://w3id.org/osdu#CementPumpSchedule
osdu:CementPumpSchedule rdf:type owl:Class ;
	skos:prefLabel "Cement Pump Schedule" ;
	rdfs:comment "Set of (Time / Rate / Back Pressure). " ;
	rdfs:subClassOf owl:Thing ;
.

###  https://w3id.org/osdu#CementStage
osdu:CementStage rdf:type owl:Class ;
	skos:prefLabel "Cement Stage" ;
	rdfs:comment "A single cement job. " ;
	rdfs:subClassOf owl:Thing ;
	rdfs:subClassOf [
		a owl:Restriction ;
		owl:onProperty osdu:stageNumber ;
		owl:minCardinality "1"^^xsd:nonNegativeInteger ;
	] ;
	rdfs:subClassOf [
		a owl:Restriction ;
		owl:onProperty osdu:stageType ;
		owl:minCardinality "1"^^xsd:nonNegativeInteger ;
	] ;
.

###  https://w3id.org/osdu#CementingFluid
osdu:CementingFluid rdf:type owl:Class ;
	skos:prefLabel "Cementing Fluid" ;
	rdfs:comment "Displaced Mud, washes and spacers, cements, displacement mud. " ;
	rdfs:subClassOf owl:Thing ;
.

###  https://w3id.org/osdu#ChronoStratigraphy
osdu:ChronoStratigraphy rdf:type owl:Class ;
	rdfs:comment "The reference value type for Chronostratigraphic classification. The purpose of chronostratigraphic classification is to organize systematically the rocks forming the Earth's crust into named units (chronostratigraphic units) that represent intervals of geologic time (geochronologic units) to serve as references in narratives about Earth history including the evolution of life. Records of this kind represent chronostratigraphic units, i.e., bodies of rocks that include all rocks representative of a specific interval of geologic time, and only this time span. Chronostratigraphic units are bounded by isochronous horizons which mark specific moments of geological time. The rank (via data.ChronostratigraphicHierarchy) and relative magnitude of the units in the chronostratigraphic hierarchy are a function of the durations they represent. " ;
	rdfs:subClassOf osdu:ReferenceData ;
	rdfs:subClassOf osdu:AbstractCommonResources ;
	rdfs:subClassOf osdu:AbstractReferenceType ;
.

###  https://w3id.org/osdu#CollectionPurpose
osdu:CollectionPurpose rdf:type owl:Class ;
	rdfs:comment "A governed purpose code for collections, e.g. 'Flow simulation output properties', 'Study', or similar. " ;
	rdfs:subClassOf osdu:ReferenceData ;
	rdfs:subClassOf osdu:AbstractCommonResources ;
	rdfs:subClassOf osdu:AbstractReferenceType ;
.

###  https://w3id.org/osdu#ColumnBasedTable
osdu:ColumnBasedTable rdf:type owl:Class ;
	rdfs:comment "A ColumnBasedTable is a set of columns, which have equal length (data.ColumnSize). Columns have a Property Kind, UnitOfMeasure and Facet. There are KeyColumns (index columns) and Columns (for look-up values). Examples are KrPc, PVT and Facies tables. " ;
	rdfs:subClassOf osdu:WorkProductComponent ;
	rdfs:subClassOf osdu:AbstractCommonResources ;
	rdfs:subClassOf osdu:AbstractWPCGroupType ;
	rdfs:subClassOf osdu:AbstractWorkProductComponent ;
.

###  https://w3id.org/osdu#ColumnBasedTableType
osdu:ColumnBasedTableType rdf:type owl:Class ;
	rdfs:comment "ColumnBasedTableType holds the values for the various possible and non exhaustive column based table types. " ;
	rdfs:subClassOf osdu:ReferenceData ;
	rdfs:subClassOf osdu:AbstractCommonResources ;
	rdfs:subClassOf osdu:AbstractReferenceType ;
.

###  https://w3id.org/osdu#ColumnShapeType
osdu:ColumnShapeType rdf:type owl:Class ;
	rdfs:comment "An enumeration for column shape types based on RESQML, i.e. triangular, quadrilateral, polygonal. " ;
	rdfs:subClassOf osdu:ReferenceData ;
	rdfs:subClassOf osdu:AbstractCommonResources ;
	rdfs:subClassOf osdu:AbstractReferenceType ;
.

###  https://w3id.org/osdu#ColumnValues
osdu:ColumnValues rdf:type owl:Class ;
	rdfs:comment "Value of the column. Generally only one of the attribute should be instantiated. " ;
	rdfs:subClassOf owl:Thing ;
.

###  https://w3id.org/osdu#Columnvalues
osdu:Columnvalues rdf:type owl:Class ;
	skos:prefLabel "Column values" ;
	rdfs:comment "Value of the column. Generally only one of the attribute should be instantiated. " ;
	rdfs:subClassOf owl:Thing ;
.

###  https://w3id.org/osdu#ComponentVolumesTestSystem
osdu:ComponentVolumesTestSystem rdf:type owl:Class ;
	skos:prefLabel "Component Volumes Test System" ;
	rdfs:comment "Description of the tested component during a singe step. " ;
	rdfs:subClassOf owl:Thing ;
	rdfs:subClassOf [
		a owl:Restriction ;
		owl:onProperty osdu:systemComponentVolume ;
		owl:minCardinality "1"^^xsd:nonNegativeInteger ;
	] ;
.

###  https://w3id.org/osdu#CompressedVectorHeaders
osdu:CompressedVectorHeaders rdf:type owl:Class ;
	skos:prefLabel "File.CompressedVectorHeaders" ;
	rdfs:comment "A File type carrying compression and vector header mapping information. " ;
	rdfs:subClassOf osdu:Dataset ;
	rdfs:subClassOf osdu:AbstractCommonResources ;
	rdfs:subClassOf osdu:AbstractDataset ;
	rdfs:subClassOf osdu:AbstractFile ;
	rdfs:subClassOf osdu:AbstractCompressionInfo ;
	rdfs:subClassOf osdu:AbstractVectorHeaderMapping ;
.

###  https://w3id.org/osdu#CompressionMethodType
osdu:CompressionMethodType rdf:type owl:Class ;
	rdfs:comment "A scheme for packing data into a smaller digital space. " ;
	rdfs:subClassOf osdu:ReferenceData ;
	rdfs:subClassOf osdu:AbstractCommonResources ;
	rdfs:subClassOf osdu:AbstractReferenceType ;
.

###  https://w3id.org/osdu#ConcatenatedTransformation
osdu:ConcatenatedTransformation rdf:type owl:Class ;
	rdfs:subClassOf owl:Thing ;
.

###  https://w3id.org/osdu#Conditions
osdu:Conditions rdf:type owl:Class ;
	rdfs:comment "The conditions under which this analysis has been carried out " ;
	rdfs:subClassOf owl:Thing ;
.

###  https://w3id.org/osdu#Configuration
osdu:Configuration rdf:type owl:Class ;
	rdfs:comment "A configuration for a UnitQuantity offering a sub-set of units and a default unit. " ;
	rdfs:subClassOf owl:Thing ;
	rdfs:subClassOf [
		a owl:Restriction ;
		owl:onProperty osdu:preferredUnitID ;
		owl:minCardinality "1"^^xsd:nonNegativeInteger ;
	] ;
.

###  https://w3id.org/osdu#ConnectedSourceDataJob
osdu:ConnectedSourceDataJob rdf:type owl:Class ;
	rdfs:comment "Scheduling, data fetch, and ingestion configuration for automated jobs against a registered connected data source. " ;
	rdfs:subClassOf osdu:MasterData ;
	rdfs:subClassOf osdu:AbstractCommonResources ;
	rdfs:subClassOf osdu:AbstractMaster ;
.

###  https://w3id.org/osdu#ConnectedSourceRegistryEntry
osdu:ConnectedSourceRegistryEntry rdf:type owl:Class ;
	rdfs:comment "System-level object containing business and technical metadata for an external OSDU-compliant data source, used for registration of that source within the OSDU external data framework. " ;
	rdfs:subClassOf osdu:MasterData ;
	rdfs:subClassOf osdu:AbstractCommonResources ;
	rdfs:subClassOf osdu:AbstractMaster ;
.

###  https://w3id.org/osdu#ContactRoleType
osdu:ContactRoleType rdf:type owl:Class ;
	rdfs:comment "Role of the contact within the associated organisation, such as Account owner, Sales Representative, Technical Support, Project Manager, Party Chief, Client Representative, Senior Observer. " ;
	rdfs:subClassOf osdu:ReferenceData ;
	rdfs:subClassOf osdu:AbstractCommonResources ;
	rdfs:subClassOf osdu:AbstractReferenceType ;
.

###  https://w3id.org/osdu#ContractorType
osdu:ContractorType rdf:type owl:Class ;
	rdfs:comment "The role of a contractor providing services, such as Recording, Line Clearing, Positioning, Data Processing. " ;
	rdfs:subClassOf osdu:ReferenceData ;
	rdfs:subClassOf osdu:AbstractCommonResources ;
	rdfs:subClassOf osdu:AbstractReferenceType ;
.

###  https://w3id.org/osdu#Contractors
osdu:Contractors rdf:type owl:Class ;
	rdfs:comment "References to organisations which supplied services to the Project. " ;
	rdfs:subClassOf owl:Thing ;
.

###  https://w3id.org/osdu#ConventionalCoreType
osdu:ConventionalCoreType rdf:type owl:Class ;
	rdfs:comment "A reference value type for Conventional Cores. " ;
	rdfs:subClassOf osdu:ReferenceData ;
	rdfs:subClassOf osdu:AbstractCommonResources ;
	rdfs:subClassOf osdu:AbstractReferenceType ;
.

###  https://w3id.org/osdu#CoordinateReferenceSystem
osdu:CoordinateReferenceSystem rdf:type owl:Class ;
	rdfs:comment "Used to describe any kind of coordinate reference system. The type is identified by CoordinateReferenceSystemType (used by the system) and Kind facing the end-user. The Code is according to OSDU standard a string, the EPSG standard number is available via the CodeAsNumber property. Description carries EPSG's Remark. AttributionAuthority carries EPSG's DataSource. AliasNames carry the EPSG Alias contents. " ;
	rdfs:subClassOf osdu:ReferenceData ;
	rdfs:subClassOf osdu:AbstractCommonResources ;
	rdfs:subClassOf osdu:AbstractReferenceType ;
.

###  https://w3id.org/osdu#CoordinateSystem
osdu:CoordinateSystem rdf:type owl:Class ;
	skos:prefLabel "Coordinate System" ;
	rdfs:comment "The coordinate system defining the dimension and individual axes used by the CRS. " ;
	rdfs:subClassOf owl:Thing ;
.

###  https://w3id.org/osdu#CoordinateTransformation
osdu:CoordinateTransformation rdf:type owl:Class ;
	rdfs:comment "Used to describe a coordinate operation between two geodetic CRSs. The type is identified by CoordinateTransformationType (used by the system) and Kind facing the end-user. The Code is according to OSDU standard a string, the EPSG standard number is available via the CodeAsNumber property. Description carries EPSG's Remark. AttributionAuthority carries EPSG's DataSource. AliasNames carry the EPSG Alias contents. " ;
	rdfs:subClassOf osdu:ReferenceData ;
	rdfs:subClassOf osdu:AbstractCommonResources ;
	rdfs:subClassOf osdu:AbstractReferenceType ;
.

###  https://w3id.org/osdu#Core
osdu:Core rdf:type owl:Class ;
	rdfs:comment "A rock sample obtained by drilling into the earth with a pipe conveyed hollow bit and core barrel " ;
	rdfs:subClassOf owl:Thing ;
.

###  https://w3id.org/osdu#CorePreservationType
osdu:CorePreservationType rdf:type owl:Class ;
	rdfs:comment "The core preservation classification type, such as Wax-sealed, Resin-coated, Cling-wrap, etc. " ;
	rdfs:subClassOf osdu:ReferenceData ;
	rdfs:subClassOf osdu:AbstractCommonResources ;
	rdfs:subClassOf osdu:AbstractReferenceType ;
.

###  https://w3id.org/osdu#CoreRemark
osdu:CoreRemark rdf:type owl:Class ;
	rdfs:comment "An array contains narrative remarks pertaining to a core. " ;
	rdfs:subClassOf owl:Thing ;
.

###  https://w3id.org/osdu#Coring
osdu:Coring rdf:type owl:Class ;
	rdfs:comment "The activity of acquiring a core from within a wellbore. The two predominant types are by drilling, or by sidewall. In drilling a cylindrical sample of rock is collected using a core bit in conjunction with a core barrel and core catcher. Sidewall cores are taken from the side of the borehole, usually by a wireline tool. Sidewall cores may be taken using percussion or mechanical drilling. " ;
	rdfs:subClassOf osdu:MasterData ;
	rdfs:subClassOf osdu:AbstractCommonResources ;
	rdfs:subClassOf osdu:AbstractMaster ;
	rdfs:subClassOf osdu:AbstractProjectActivity ;
.

###  https://w3id.org/osdu#Cost
osdu:Cost rdf:type owl:Class ;
	rdfs:comment "Cost information captured for a defined time period during operations and/or drilling " ;
	rdfs:subClassOf owl:Thing ;
	rdfs:subClassOf [
		a owl:Restriction ;
		owl:onProperty osdu:totalCostAmount ;
		owl:minCardinality "1"^^xsd:nonNegativeInteger ;
	] ;
	rdfs:subClassOf [
		a owl:Restriction ;
		owl:onProperty osdu:costCurrency ;
		owl:minCardinality "1"^^xsd:nonNegativeInteger ;
	] ;
.

###  https://w3id.org/osdu#Currency
osdu:Currency rdf:type owl:Class ;
	rdfs:comment "Used to describe the type of currencies. " ;
	rdfs:subClassOf osdu:ReferenceData ;
	rdfs:subClassOf osdu:AbstractCommonResources ;
	rdfs:subClassOf osdu:AbstractReferenceType ;
.

###  https://w3id.org/osdu#Curve
osdu:Curve rdf:type owl:Class ;
	rdfs:comment "A set of properties describing a trajectory station property which is available for this instance of a WellboreTrajectory. " ;
	rdfs:subClassOf owl:Thing ;
.

###  https://w3id.org/osdu#CurveIndexDimensionType
osdu:CurveIndexDimensionType rdf:type owl:Class ;
	rdfs:comment "DEPRECATED: (not used anywhere) Describes the physical dimension a curve index is defined from - can be Depth, Time, Counter,... " ;
	rdfs:subClassOf osdu:ReferenceData ;
	rdfs:subClassOf osdu:AbstractCommonResources ;
	rdfs:subClassOf osdu:AbstractReferenceType ;
.

###  https://w3id.org/osdu#CurveSampleType
osdu:CurveSampleType rdf:type owl:Class ;
	rdfs:comment "The value type of well log curve samples, e.g. Float, double, string. " ;
	rdfs:subClassOf osdu:ReferenceData ;
	rdfs:subClassOf osdu:AbstractCommonResources ;
	rdfs:subClassOf osdu:AbstractReferenceType ;
.

###  https://w3id.org/osdu#Curves
osdu:Curves rdf:type owl:Class ;
	rdfs:subClassOf owl:Thing ;
.

###  https://w3id.org/osdu#3DInterpretationSet
osdu:2DInterpretationSet rdf:type owl:Class ;
	rdfs:comment "A seismic 2D interpretation set is a collection of logical processed lines and associated trace datasets that represent an important and uniform set for interpretation.  It does not comprise all of the datasets with a common processing geometry, nor all of the lines/datasets from a processing project, nor all of the lines/datasets from an acquisition project, because some are not suitable for interpretation.  An interpretation survey may include 2D lines and datasets from more than one acquisition or processing project.  Consequently, it is not an acquisition survey nor a processing survey.  It is not an application project, which is a collection of all the various objects an application and user care about for some analysis (seismic, wells, etc.).  It inherits properties shared by project entities because it can serve to capture the archiving of a master or authorized project activity.  Interpretation objects (horizons) are hung from an interpretation project to give context and to derive spatial location based on the processing geometry of the associated 2D lines. Trace datasets and seismic horizons are associated through LineageAssertion, although a master collection of trace datasets and horizons are explicitly related through a child relationship property. " ;
	rdfs:subClassOf osdu:MasterData ;
	rdfs:subClassOf osdu:AbstractCommonResources ;
	rdfs:subClassOf osdu:AbstractMaster ;
	rdfs:subClassOf osdu:AbstractProject ;
	rdfs:subClassOf osdu:AbstractProjectActivity ;
.

###  https://w3id.org/osdu#3DInterpretationSet
osdu:3DInterpretationSet rdf:type owl:Class ;
	skos:prefLabel "Seismic3DInterpretationSet" ;
	rdfs:comment "A seismic 3D interpretation survey is a collection of trace datasets with a common bin grid that are important for interpretation.  It does not comprise all of the datasets with a common bin grid, nor all of the datasets from a processing project, nor all of the datasets from an acquisition project, because some are not suitable for interpretation.  An interpretation survey may include datasets from more than one acquisition or processing project.  Consequently, it is not an acquisition survey nor a processing survey.  It is not an application project, which is a collection of all the various objects an application and user care about for some analysis (seismic, wells, etc.).  It inherits properties shared by project entities because it can serve to capture the archiving of a master or authorized project activity. Interpretation objects (horizons) are hung from an interpretation survey to give context and to derive spatial location based on the common bin grid.  Trace datasets and seismic horizons are associated through LineageAssertion, although a master collection of trace datasets and horizons are explicitly related through a child relationship property. " ;
	rdfs:subClassOf osdu:MasterData ;
	rdfs:subClassOf osdu:AbstractCommonResources ;
	rdfs:subClassOf osdu:AbstractMaster ;
	rdfs:subClassOf osdu:AbstractProject ;
	rdfs:subClassOf osdu:AbstractProjectActivity ;
.


###  https://w3id.org/osdu#DSTRun
osdu:DSTRun rdf:type owl:Class ;
	skos:prefLabel "DST Run" ;
	rdfs:comment "A test performed on a drillstem " ;
	rdfs:subClassOf owl:Thing ;
.

###  https://w3id.org/osdu#DataCollection
osdu:DataCollection rdf:type owl:Class ;
	rdfs:comment "Transient collection of object references used e.g. to exchange context between running applications. DataCollection is not intended to be persisted. " ;
	rdfs:subClassOf owl:Thing ;
	rdfs:subClassOf [
		a owl:Restriction ;
		owl:onProperty osdu:resources ;
		owl:minCardinality "1"^^xsd:nonNegativeInteger ;
	] ;
	rdfs:subClassOf [
		a owl:Restriction ;
		owl:onProperty osdu:name ;
		owl:minCardinality "1"^^xsd:nonNegativeInteger ;
	] ;
	rdfs:subClassOf [
		a owl:Restriction ;
		owl:onProperty osdu:ownerID ;
		owl:minCardinality "1"^^xsd:nonNegativeInteger ;
	] ;
.

###  https://w3id.org/osdu#DataQuality
osdu:DataQuality rdf:type owl:Class ;
	rdfs:comment "This is used to store result from a run of Data Quality Metric Evaluation engine. Captures summary information, such as which Business rule-set(s) and rule(s) have been used, when this was run and by whom. Detailed result (such as which rule failed, for which meta data item and what was offending value causing the rule to fail) is meant to be made available in a file that is linked to this work-product component. Through Lineage Assertion, this can relate to the entities which were used for the run of Evaluation engine, such as a collection of wells whose meta data were inspected by using a set of rules. " ;
	rdfs:subClassOf osdu:WorkProductComponent ;
	rdfs:subClassOf osdu:AbstractCommonResources ;
	rdfs:subClassOf osdu:AbstractWPCGroupType ;
	rdfs:subClassOf osdu:AbstractWorkProductComponent ;
.

###  https://w3id.org/osdu#DataRule
osdu:DataRule rdf:type owl:Class ;
	rdfs:comment "The list of QualityDataRule items that this QualityDataRuleSet consists of. " ;
	rdfs:subClassOf owl:Thing ;
.

###  https://w3id.org/osdu#DataRuleDimensionType
osdu:DataRuleDimensionType rdf:type owl:Class ;
	rdfs:comment "A set of data quality rules to assess a specific aspect in the trustworthiness of data. " ;
	rdfs:subClassOf osdu:ReferenceData ;
	rdfs:subClassOf osdu:AbstractCommonResources ;
	rdfs:subClassOf osdu:AbstractReferenceType ;
.

###  https://w3id.org/osdu#DataRulePurposeType
osdu:DataRulePurposeType rdf:type owl:Class ;
	rdfs:comment "Reference value used by QualityDataRule to indicate the purpose and expected reaction on pass or failure. " ;
	rdfs:subClassOf osdu:ReferenceData ;
	rdfs:subClassOf osdu:AbstractCommonResources ;
	rdfs:subClassOf osdu:AbstractReferenceType ;
.

###  https://w3id.org/osdu#DataRuleSets
osdu:DataRuleSets rdf:type owl:Class ;
	rdfs:comment "The list of data rule sets that is relevant for this business process. Each data rule set reference is associated with a run-status. " ;
	rdfs:subClassOf owl:Thing ;
.

###  https://w3id.org/osdu#DataRules
osdu:DataRules rdf:type owl:Class ;
	rdfs:comment "The list of individual data rules that is relevant for this business process. Each data rule reference is associated with a run-status. " ;
	rdfs:subClassOf owl:Thing ;
.

###  https://w3id.org/osdu#Dataset
osdu:Dataset rdf:type owl:Class ;
	rdfs:subClassOf osdu:System ;
.

###  https://w3id.org/osdu#DatasetProperties
osdu:DatasetProperties rdf:type owl:Class ;
	skos:prefLabel "Dataset Properties" ;
	rdfs:comment "The dataset properties for a file collection, single file, data space, or other source. " ;
	rdfs:subClassOf owl:Thing ;
	rdfs:subClassOf [
		a owl:Restriction ;
		owl:onProperty osdu:fileCollectionPath ;
		owl:minCardinality "1"^^xsd:nonNegativeInteger ;
	] ;
	rdfs:subClassOf [
		a owl:Restriction ;
		owl:onProperty osdu:uri ;
		owl:minCardinality "1"^^xsd:nonNegativeInteger ;
	] ;
	rdfs:subClassOf [
		a owl:Restriction ;
		owl:onProperty osdu:connectedSourceRegistryEntryID ;
		owl:minCardinality "1"^^xsd:nonNegativeInteger ;
	] ;
	rdfs:subClassOf [
		a owl:Restriction ;
		owl:onProperty osdu:connectedSourcedataJobID ;
		owl:minCardinality "1"^^xsd:nonNegativeInteger ;
	] ;
	rdfs:subClassOf [
		a owl:Restriction ;
		owl:onProperty osdu:sourceDataPartitionID ;
		owl:minCardinality "1"^^xsd:nonNegativeInteger ;
	] ;
	rdfs:subClassOf [
		a owl:Restriction ;
		owl:onProperty osdu:sourceRecordID ;
		owl:minCardinality "1"^^xsd:nonNegativeInteger ;
	] ;
.

###  https://w3id.org/osdu#Datum
osdu:Datum rdf:type owl:Class ;
	rdfs:comment "The datum of this CRS. Only populated for CoordinateReferenceSystemType in [GeographicCRS, VerticalCRS, EngineeringCRS]. " ;
	rdfs:subClassOf owl:Thing ;
.

###  https://w3id.org/osdu#DatumEnsemble
osdu:DatumEnsemble rdf:type owl:Class ;
	rdfs:comment "The DatumEnsemble for the CRS's datum. Only populated for GeographicCRS. " ;
	rdfs:subClassOf owl:Thing ;
.

###  https://w3id.org/osdu#DepositionGeometryType
osdu:DepositionGeometryType rdf:type owl:Class ;
	rdfs:comment "The Deposition Geometry classification (corresponding to Energistics RESQML DepositionMode). Examples are parallel to top, parallel to bottom, etc. " ;
	rdfs:subClassOf osdu:ReferenceData ;
	rdfs:subClassOf osdu:AbstractCommonResources ;
	rdfs:subClassOf osdu:AbstractReferenceType ;
.

###  https://w3id.org/osdu#DepthRange
osdu:DepthRange rdf:type owl:Class ;
	skos:prefLabel "Depth Range" ;
	rdfs:comment "The depth range over which the the activity takes place " ;
	rdfs:subClassOf owl:Thing ;
.

###  https://w3id.org/osdu#DimensionType
osdu:DimensionType rdf:type owl:Class ;
	rdfs:comment "Geometry along which a velocity model is defined, such as line (could be checkshot), surface, volume, time series (for 4D/time lapse). Ex. 1D, 2D, 3D, 1D_TL, 2D_TL, and 3D_TL. " ;
	rdfs:subClassOf osdu:ReferenceData ;
	rdfs:subClassOf osdu:AbstractCommonResources ;
	rdfs:subClassOf osdu:AbstractReferenceType ;
.

###  https://w3id.org/osdu#DiscretisationSchemeType
osdu:DiscretisationSchemeType rdf:type owl:Class ;
	rdfs:comment "Describes geometrically where in a discretised cell representation of a velocity number field the value applies, such as vertex, cell center, average across cell. " ;
	rdfs:subClassOf osdu:ReferenceData ;
	rdfs:subClassOf osdu:AbstractCommonResources ;
	rdfs:subClassOf osdu:AbstractReferenceType ;
.

###  https://w3id.org/osdu#Document
osdu:Document rdf:type owl:Class ;
	rdfs:comment "A document can be any document that is required to be stored in an electronic format. Examples of this could be daily drilling reports, drilling schematics, or material quality analysis reports. " ;
	rdfs:subClassOf osdu:WorkProductComponent ;
	rdfs:subClassOf osdu:AbstractCommonResources ;
	rdfs:subClassOf osdu:AbstractWPCGroupType ;
	rdfs:subClassOf osdu:AbstractWorkProductComponent ;
.

###  https://w3id.org/osdu#DocumentType
osdu:DocumentType rdf:type owl:Class ;
	rdfs:comment "A piece of printed or electronic material containing communication or evidence that is intended for persistent or permanent record. " ;
	rdfs:subClassOf osdu:ReferenceData ;
	rdfs:subClassOf osdu:AbstractCommonResources ;
	rdfs:subClassOf osdu:AbstractReferenceType ;
.

###  https://w3id.org/osdu#DomainType
osdu:DomainType rdf:type owl:Class ;
	rdfs:comment "The vertical domain type of models, interpretations and representations. " ;
	rdfs:subClassOf osdu:ReferenceData ;
	rdfs:subClassOf osdu:AbstractCommonResources ;
	rdfs:subClassOf osdu:AbstractReferenceType ;
.

###  https://w3id.org/osdu#DownHoleMaximumRPM
osdu:DownHoleMaximumRPM rdf:type owl:Class ;
	skos:prefLabel "DownHole Maximum RPM" ;
	rdfs:comment "The down-hole planned maximum rotary speed for the run " ;
	rdfs:subClassOf owl:Thing ;
	rdfs:subClassOf [
		a owl:Restriction ;
		owl:onproperty osdu:hasPoint ;
		owl:minCardinality "1"^^xsd:nonNegativeInteger ;
	] ;
.

###  https://w3id.org/osdu#DownHoleMinimumRPM
osdu:DownHoleMinimumRPM rdf:type owl:Class ;
	skos:prefLabel "DownHole Minimum RPM" ;
	rdfs:comment "The down-hole planned minimum rotary speed for the run " ;
	rdfs:subClassOf owl:Thing ;
	rdfs:subClassOf [
		a owl:Restriction ;
		owl:onproperty osdu:hasPoint ;
		owl:minCardinality "1"^^xsd:nonNegativeInteger ;
	] ;
.

###  https://w3id.org/osdu#DownHoleRecommendedRPM
osdu:DownHoleRecommendedRPM rdf:type owl:Class ;
	skos:prefLabel "DownHole Recommended RPM" ;
	rdfs:comment "The down-hole recommended rotary speed for the run " ;
	rdfs:subClassOf owl:Thing ;
	rdfs:subClassOf [
		a owl:Restriction ;
		owl:onproperty osdu:hasPoint;
		owl:minCardinality "1"^^xsd:nonNegativeInteger ;
	] ;
.

###  https://w3id.org/osdu#DrillingActivity
osdu:DrillingActivity rdf:type owl:Class ;
	skos:prefLabel "Drilling Activity" ;
	rdfs:comment "Information regarding an individual activity that is part of the Drilling Report " ;
	rdfs:subClassOf owl:Thing ;
.

###  https://w3id.org/osdu#DrillingActivityClassType
osdu:DrillingActivityClassType rdf:type owl:Class ;
	rdfs:comment "The type of drilling activity classes " ;
	rdfs:subClassOf osdu:ReferenceData ;
	rdfs:subClassOf osdu:AbstractCommonResources ;
	rdfs:subClassOf osdu:AbstractReferenceType ;
.

###  https://w3id.org/osdu#DrillingParameters
osdu:DrillingParameters rdf:type owl:Class ;
	skos:prefLabel "Drilling Parameters" ;
	rdfs:comment "The bottomhole assembly drilling parameters schema, which contains statistical and calculated operations data for the run, related to depths, activities, temperature, pressure, flow rates, torque, etc. " ;
	rdfs:subClassOf owl:Thing ;
.

###  https://w3id.org/osdu#DrillingReasonType
osdu:DrillingReasonType rdf:type owl:Class ;
	rdfs:comment "Used to describe the type of drilling reasons. " ;
	rdfs:subClassOf osdu:ReferenceData ;
	rdfs:subClassOf osdu:AbstractCommonResources ;
	rdfs:subClassOf osdu:AbstractReferenceType ;
.

###  https://w3id.org/osdu#DrillingReportStatusInfo
osdu:DrillingReportStatusInfo rdf:type owl:Class ;
	rdfs:comment "Status information related to a Drilling Report " ;
	rdfs:subClassOf owl:Thing ;
	rdfs:subClassOf [
		a owl:Restriction ;
		owl:onProperty osdu:statusDateTime ;
		owl:minCardinality "1"^^xsd:nonNegativeInteger ;
	] ;
.

###  https://w3id.org/osdu#ETPDataspace
osdu:ETPDataspace rdf:type owl:Class ;
	rdfs:comment "Describes the location and attributes of a Dataspace accessible through ETP (Energistics Transfer Protocol) APIs, for ETP 1.2 and above " ;
	rdfs:subClassOf osdu:Dataset ;
	rdfs:subClassOf osdu:AbstractCommonResources ;
	rdfs:subClassOf osdu:AbstractDataset ;
.

###  https://w3id.org/osdu#EarthModelInterpretation
osdu:EarthModelInterpretation rdf:type owl:Class ;
	rdfs:comment "A single, consistent interpretation of an entire earth model. " ;
	rdfs:subClassOf osdu:WorkProductComponent ;
	rdfs:subClassOf osdu:AbstractCommonResources ;
	rdfs:subClassOf osdu:AbstractWPCGroupType ;
	rdfs:subClassOf osdu:AbstractWorkProductComponent ;
	rdfs:subClassOf osdu:AbstractInterpretation ;
.

###  https://w3id.org/osdu#EncodingFormatType
osdu:EncodingFormatType rdf:type owl:Class ;
	rdfs:comment "Used to describe the type of encoding formats. " ;
	rdfs:subClassOf osdu:ReferenceData ;
	rdfs:subClassOf osdu:AbstractCommonResources ;
	rdfs:subClassOf osdu:AbstractReferenceType ;
.

###  https://w3id.org/osdu#EvaluationPlan
osdu:EvaluationPlan rdf:type owl:Class ;
	rdfs:comment "A planned evaluation on a drilling operation " ;
	rdfs:subClassOf osdu:MasterData ;
	rdfs:subClassOf osdu:AbstractCommonResources ;
	rdfs:subClassOf osdu:AbstractMaster ;
	rdfs:subClassOf osdu:AbstractProject ;
.

###  https://w3id.org/osdu#ExistenceKind
osdu:ExistenceKind rdf:type owl:Class ;
	rdfs:comment "ExistenceKind describes at which stage the instance is in the cradle-to-grave span of its existence. Typical values are: Proposed, Planned, Active, Inactive, Marked for Disposal. " ;
	rdfs:subClassOf osdu:ReferenceData ;
	rdfs:subClassOf osdu:AbstractCommonResources ;
	rdfs:subClassOf osdu:AbstractReferenceType ;
.

###  https://w3id.org/osdu#ExpectedVolume
osdu:ExpectedVolume rdf:type owl:Class ;
	skos:prefLabel "Expected Volume" ;
	rdfs:comment "Individual description, for a given pressure, of the Volume Pumped expectations for a single step of the test. " ;
	rdfs:subClassOf owl:Thing ;
	rdfs:subClassOf [
		a owl:Restriction ;
		owl:onProperty osdu:pressure ;
		owl:minCardinality "1"^^xsd:nonNegativeInteger ;
	] ;
.

###  https://w3id.org/osdu#Extent
osdu:Extent rdf:type owl:Class ;
	rdfs:comment "Extent or area of use information. " ;
	rdfs:subClassOf owl:Thing ;
.

###  https://w3id.org/osdu#ExternalCatalogNamespace
osdu:ExternalCatalogNamespace rdf:type owl:Class ;
	rdfs:comment "A namespace for a group of catalog records. This is used in conjunction with external catalogs to group records of a particular kind belonging together to achieve unique code and name look-ups. " ;
	rdfs:subClassOf osdu:ReferenceData ;
	rdfs:subClassOf osdu:AbstractCommonResources ;
	rdfs:subClassOf osdu:AbstractReferenceType ;
.

###  https://w3id.org/osdu#ExternalUnitOfMeasure
osdu:ExternalUnitOfMeasure rdf:type owl:Class ;
	rdfs:comment "A unit of measure description belonging to an external system, which is intended to be mapped or related to a platform-standard UnitOfMeasure record. Mappings can be exact or not. This is expressed by he MapStatus. MapStatus:identical means that the external unit reference can be swapped out by the platform standard reference. MapStatus:corrected indicates same concept but differences in the conversion parameters. Data must be treated or re-labeled; the decision can only be taken on a case by case basis. Finally  MapStatus:unsupported means that there is no equivalent platform standard reference. An ExternalUnitOfMeasure record can be seen as an 'alias' for the UnitOfMeasureID it refers to. Adding NameAliases to UnitOfMeasure is, however, not recommended because local overrides may be lost when new OSDU updates are shipped. " ;
	rdfs:subClassOf osdu:ReferenceData ;
	rdfs:subClassOf osdu:AbstractCommonResources ;
	rdfs:subClassOf osdu:AbstractReferenceType ;
.

###  https://w3id.org/osdu#ExternalUnitQuantity
osdu:ExternalUnitQuantity rdf:type owl:Class ;
	rdfs:comment "An external unit quantity definition to map to a platform standard UnitQuantity record. An ExternalUnitQuantity record can be seen as an 'alias' for the UnitQuantityID it refers to. Adding NameAliases to UnitQuantity is, however, not recommended because local overrides may be lost when new OSDU updates are shipped. " ;
	rdfs:subClassOf osdu:ReferenceData ;
	rdfs:subClassOf osdu:AbstractCommonResources ;
	rdfs:subClassOf osdu:AbstractReferenceType ;
.

###  https://w3id.org/osdu#FacetRole
osdu:FacetRole rdf:type owl:Class ;
	rdfs:comment "The role of a facet, e.g. maximum threshold, cumulative, surface condition, reservoir condition, oil, water, gas, condensate. " ;
	rdfs:subClassOf osdu:ReferenceData ;
	rdfs:subClassOf osdu:AbstractCommonResources ;
	rdfs:subClassOf osdu:AbstractReferenceType ;
.

###  https://w3id.org/osdu#FacetType
osdu:FacetType rdf:type owl:Class ;
	rdfs:comment "Enumerations of the type of qualifier that applies to a property type to provide additional context about the nature of the property. For example, may include conditions, direction, qualifiers, or statistics. Facets are used in RESQML to provide qualifiers to existing property types, which minimizes the need to create specialized property types. " ;
	rdfs:subClassOf osdu:ReferenceData ;
	rdfs:subClassOf osdu:AbstractCommonResources ;
	rdfs:subClassOf osdu:AbstractReferenceType ;
.

###  https://w3id.org/osdu#FacilityEventType
osdu:FacilityEventType rdf:type owl:Class ;
	rdfs:comment "Used to describe the type of facility events. " ;
	rdfs:subClassOf osdu:ReferenceData ;
	rdfs:subClassOf osdu:AbstractCommonResources ;
	rdfs:subClassOf osdu:AbstractReferenceType ;
.

###  https://w3id.org/osdu#FacilityStateType
osdu:FacilityStateType rdf:type owl:Class ;
	rdfs:comment "Life Cycle [Facility State Type] is a set of major phases that are significant to regulators and/or business stakeholders. Life Cycle may apply to a well or its components [or other facility]. " ;
	rdfs:subClassOf osdu:ReferenceData ;
	rdfs:subClassOf osdu:AbstractCommonResources ;
	rdfs:subClassOf osdu:AbstractReferenceType ;
.

###  https://w3id.org/osdu#FacilityType
osdu:FacilityType rdf:type owl:Class ;
	rdfs:comment "Used to identify and describe the type of facility. A facility is a grouping of equipment that is located within a specific geographic boundary or site and that is used in the context of energy-related activities such as exploration, extraction, generation, storage, processing, disposal, supply, or transfer. Clarifications: (1) A facility may be surface or subsurface located. (2) Usually facility equipment is commonly owned or operated. (3) Industry definitions may vary and differ from this one. " ;
	rdfs:subClassOf osdu:ReferenceData ;
	rdfs:subClassOf osdu:AbstractCommonResources ;
	rdfs:subClassOf osdu:AbstractReferenceType ;
.

###  https://w3id.org/osdu#FaultInterpretation
osdu:FaultInterpretation rdf:type owl:Class ;
	rdfs:comment "Geologic information associated to fault-related objects  (marker, fault sticks, modeled objects like triangulated surface) " ;
	rdfs:subClassOf osdu:WorkProductComponent ;
	rdfs:subClassOf osdu:AbstractCommonResources ;
	rdfs:subClassOf osdu:AbstractWPCGroupType ;
	rdfs:subClassOf osdu:AbstractWorkProductComponent ;
	rdfs:subClassOf osdu:AbstractInterpretation ;
.

###  https://w3id.org/osdu#FaultSystem
osdu:FaultSystem rdf:type owl:Class ;
	rdfs:comment "A set of picked faults. In the earth modeling domain this entity corresponds to a PersistedCollection containing GenericRepresentation or SeismicFault items. " ;
	rdfs:subClassOf osdu:WorkProductComponent ;
	rdfs:subClassOf osdu:AbstractCommonResources ;
	rdfs:subClassOf osdu:AbstractWPCGroupType ;
	rdfs:subClassOf osdu:AbstractWorkProductComponent ;
.

###  https://w3id.org/osdu#FaultThrowDescriptions
osdu:FaultThrowDescriptions rdf:type owl:Class ;
	rdfs:comment "A structure carrying descriptions of fault throw characteristics. " ;
	rdfs:subClassOf owl:Thing ;
.

###  https://w3id.org/osdu#FaultThrowType
osdu:FaultThrowType rdf:type owl:Class ;
	rdfs:comment "Classification of the fault throw type, e.g. reverse, normal etc. " ;
	rdfs:subClassOf osdu:ReferenceData ;
	rdfs:subClassOf osdu:AbstractCommonResources ;
	rdfs:subClassOf osdu:AbstractReferenceType ;
.

###  https://w3id.org/osdu#Faults
osdu:Faults rdf:type owl:Class ;
	rdfs:comment "Array of Faults that comprise the Fault System " ;
	rdfs:subClassOf owl:Thing ;
.

###  https://w3id.org/osdu#FeatureType
osdu:FeatureType rdf:type owl:Class ;
	rdfs:comment "Used to describe the type of features. " ;
	rdfs:subClassOf osdu:ReferenceData ;
	rdfs:subClassOf osdu:AbstractCommonResources ;
	rdfs:subClassOf osdu:AbstractReferenceType ;
.

###  https://w3id.org/osdu#Field
osdu:Field rdf:type owl:Class ;
	rdfs:comment "A mineral deposit that has been exploited for commercial purposes. " ;
	rdfs:subClassOf osdu:MasterData ;
	rdfs:subClassOf osdu:AbstractCommonResources ;
	rdfs:subClassOf osdu:AbstractMaster ;
.

###  https://w3id.org/osdu#FilterSpecification
osdu:FilterSpecification rdf:type owl:Class ;
	rdfs:comment "Collection Filter Specification " ;
	rdfs:subClassOf owl:Thing ;
.

###  https://w3id.org/osdu#FlowType
osdu:FlowType rdf:type owl:Class ;
	skos:prefLabel "OAuth2FlowType" ;
	rdfs:comment "Flows, or grants, supported within the OAuth 2.0 authorization framework. " ;
	rdfs:subClassOf osdu:ReferenceData ;
	rdfs:subClassOf osdu:AbstractCommonResources ;
	rdfs:subClassOf osdu:AbstractReferenceType ;
.

###  https://w3id.org/osdu#FlowratePumpGroup
osdu:FlowratePumpGroup rdf:type owl:Class ;
	skos:prefLabel "Flowrate Pump Group" ;
	rdfs:comment "A group of parameters that refer to flowrate " ;
	rdfs:subClassOf owl:Thing ;
	rdfs:subClassOf [
		a owl:Restriction ;
		owl:onProperty osdu:maximumFlowratePump ;
		owl:minCardinality "1"^^xsd:nonNegativeInteger ;
	] ;
	rdfs:subClassOf [
		a owl:Restriction ;
		owl:onProperty osdu:minimumFlowratePump ;
		owl:minCardinality "1"^^xsd:nonNegativeInteger ;
	] ;
.

###  https://w3id.org/osdu#Fluid
osdu:Fluid rdf:type owl:Class ;
	rdfs:comment "Information regarding an individual fluid that is part of the Drilling Report. " ;
	rdfs:subClassOf owl:Thing ;
.

###  https://w3id.org/osdu#FluidFacet
osdu:FluidFacet rdf:type owl:Class ;
	skos:prefLabel "Fluid Facet" ;
	rdfs:comment "A description of an individual facet composing a fluid " ;
	rdfs:subClassOf owl:Thing ;
	rdfs:subClassOf [
		a owl:Restriction ;
		owl:onProperty osdu:fluidPropertyFacetNameID ;
		owl:minCardinality "1"^^xsd:nonNegativeInteger ;
	] ;
	rdfs:subClassOf [
		a owl:Restriction ;
		owl:onProperty osdu:fluidPropertyValue ;
		owl:minCardinality "1"^^xsd:nonNegativeInteger ;
	] ;
	rdfs:subClassOf [
		a owl:Restriction ;
		owl:onProperty osdu:fluidPropertyUnit ;
		owl:minCardinality "1"^^xsd:nonNegativeInteger ;
	] ;
	rdfs:subClassOf [
		a owl:Restriction ;
		owl:onProperty osdu:measuredPropertyID ;
		owl:minCardinality "1"^^xsd:nonNegativeInteger ;
	] ;
.

###  https://w3id.org/osdu#FluidPhaseType
osdu:FluidPhaseType rdf:type owl:Class ;
	rdfs:comment "The fluid phase present in a geological unit's pore space. Examples: aquifer, gas cap, oil column, etc. " ;
	rdfs:subClassOf osdu:ReferenceData ;
	rdfs:subClassOf osdu:AbstractCommonResources ;
	rdfs:subClassOf osdu:AbstractReferenceType ;
.

###  https://w3id.org/osdu#FluidPropertyFacetName
osdu:FluidPropertyFacetName rdf:type owl:Class ;
	rdfs:comment "Reference list of facet names, includes items such as such as  Minimum, Maximum  and Average " ;
	rdfs:subClassOf osdu:ReferenceData ;
	rdfs:subClassOf osdu:AbstractCommonResources ;
	rdfs:subClassOf osdu:AbstractReferenceType ;
.

###  https://w3id.org/osdu#FluidPropertyName
osdu:FluidPropertyName rdf:type owl:Class ;
	rdfs:comment "Fluid properties such as Ph, Pv, Yp, Oil/Water Ratio " ;
	rdfs:subClassOf osdu:ReferenceData ;
	rdfs:subClassOf osdu:AbstractCommonResources ;
	rdfs:subClassOf osdu:AbstractReferenceType ;
.

###  https://w3id.org/osdu#FluidRheologicalModelType
osdu:FluidRheologicalModelType rdf:type owl:Class ;
	rdfs:comment "Mathematical model used in cement calculations " ;
	rdfs:subClassOf osdu:ReferenceData ;
	rdfs:subClassOf osdu:AbstractCommonResources ;
	rdfs:subClassOf osdu:AbstractReferenceType ;
.

###  https://w3id.org/osdu#FluidRole
osdu:FluidRole rdf:type owl:Class ;
	rdfs:comment "Purpose the fluid will play in the wellbore, such as Cement Displacement, Hole Cleaning, Sweep, Completion Fluid " ;
	rdfs:subClassOf osdu:ReferenceData ;
	rdfs:subClassOf osdu:AbstractCommonResources ;
	rdfs:subClassOf osdu:AbstractReferenceType ;
.

###  https://w3id.org/osdu#FluidType
osdu:FluidType rdf:type owl:Class ;
	rdfs:comment "Type of drilling or completions fluid " ;
	rdfs:subClassOf osdu:ReferenceData ;
	rdfs:subClassOf osdu:AbstractCommonResources ;
	rdfs:subClassOf osdu:AbstractReferenceType ;
.

###  https://w3id.org/osdu#FluidsInterval
osdu:FluidsInterval rdf:type owl:Class ;
	skos:prefLabel "Fluids Interval" ;
	rdfs:comment "A fluid used in the drilling of a wellbore's section " ;
	rdfs:subClassOf owl:Thing ;
	rdfs:subClassOf [
		a owl:Restriction ;
		owl:onProperty osdu:intervalName ;
		owl:minCardinality "1"^^xsd:nonNegativeInteger ;
	] ;
	rdfs:subClassOf [
		a owl:Restriction ;
		owl:onProperty osdu:intervalTopMeasuredDepth ;
		owl:minCardinality "1"^^xsd:nonNegativeInteger ;
	] ;
	rdfs:subClassOf [
		a owl:Restriction ;
		owl:onProperty osdu:intervalBaseMeasuredDepth ;
		owl:minCardinality "1"^^xsd:nonNegativeInteger ;
	] ;
	rdfs:subClassOf [
		a owl:Restriction ;
		owl:onProperty osdu:hasFluidsSystem ;
		owl:minCardinality "1"^^xsd:nonNegativeInteger ;
	] ;
.

###  https://w3id.org/osdu#FluidsProgram
osdu:FluidsProgram rdf:type owl:Class ;
	rdfs:comment "Description of the fluids program design " ;
	rdfs:subClassOf osdu:MasterData ;
	rdfs:subClassOf osdu:AbstractCommonResources ;
	rdfs:subClassOf osdu:AbstractMaster ;
.

###  https://w3id.org/osdu#FluidsProperty
osdu:FluidsProperty rdf:type owl:Class ;
	skos:prefLabel "Fluids Property" ;
	rdfs:comment "A description of fluid used in the drilling of a wellbore " ;
	rdfs:subClassOf owl:Thing ;
	rdfs:subClassOf [
		a owl:Restriction ;
		owl:onProperty osdu:fluidPropertyNameID ;
		owl:minCardinality "1"^^xsd:nonNegativeInteger ;
	] ;
	rdfs:subClassOf [
		a owl:Restriction ;
		owl:onProperty osdu:hasFluidFacets ;
		owl:minCardinality "1"^^xsd:nonNegativeInteger ;
	] ;
.

###  https://w3id.org/osdu#FluidsReport
osdu:FluidsReport rdf:type owl:Class ;
	rdfs:comment "Used to capture an analysis of the drilling mud. " ;
	rdfs:subClassOf osdu:MasterData ;
	rdfs:subClassOf osdu:AbstractCommonResources ;
	rdfs:subClassOf osdu:AbstractMaster ;
.

###  https://w3id.org/osdu#FluidsSystem
osdu:FluidsSystem rdf:type owl:Class ;
	skos:prefLabel "Fluid System" ;
	rdfs:comment "Provides the overall description of the drilling fluids system. " ;
	rdfs:subClassOf owl:Thing ;
	rdfs:subClassOf [
		a owl:Restriction ;
		owl:onProperty osdu:hasFluidProperties ;
		owl:minCardinality "1"^^xsd:nonNegativeInteger ;
	] ;
.

###  https://w3id.org/osdu#FormationIntegrityEvaluation
osdu:FormationIntegrityEvaluation rdf:type owl:Class ;
	skos:prefLabel "Formation Integrity Evaluation" ;
	rdfs:comment "A test performed to determine the integrity of a formation " ;
	rdfs:subClassOf owl:Thing ;
.

###  https://w3id.org/osdu#FormationPressureTestType
osdu:FormationPressureTestType rdf:type owl:Class ;
	rdfs:comment "FIT, LOT, XLOT etc. Proposed reference values: Formation Integrity Test, Leak Off Test, Extended Leak Off Test " ;
	rdfs:subClassOf osdu:ReferenceData ;
	rdfs:subClassOf osdu:AbstractCommonResources ;
	rdfs:subClassOf osdu:AbstractReferenceType ;
.

###  https://w3id.org/osdu#FrameOfReferenceAzimuthReference
osdu:FrameOfReferenceAzimuthReference rdf:type owl:Class ;
	rdfs:subClassOf osdu:AbstractMetaItem ;
	rdfs:subClassOf [
		a owl:Restriction ;
		owl:onProperty osdu:kind ;
		owl:minCardinality "1"^^xsd:nonNegativeInteger ;
	] ;
	rdfs:subClassOf [
		a owl:Restriction ;
		owl:onProperty osdu:persistableReference ;
		owl:minCardinality "1"^^xsd:nonNegativeInteger ;
	] ;
.

###  https://w3id.org/osdu#FrameOfReferenceCRS
osdu:FrameOfReferenceCRS rdf:type owl:Class ;
	rdfs:subClassOf osdu:AbstractMetaItem ;
	rdfs:subClassOf [
		a owl:Restriction ;
		owl:onProperty osdu:kind ;
		owl:minCardinality "1"^^xsd:nonNegativeInteger ;
	] ;
	rdfs:subClassOf [
		a owl:Restriction ;
		owl:onProperty osdu:persistableReference ;
		owl:minCardinality "1"^^xsd:nonNegativeInteger ;
	] ;
.

###  https://w3id.org/osdu#FrameOfReferenceDateTime
osdu:FrameOfReferenceDateTime rdf:type owl:Class ;
	rdfs:subClassOf osdu:AbstractMetaItem ;
	rdfs:subClassOf [
		a owl:Restriction ;
		owl:onProperty osdu:kind ;
		owl:minCardinality "1"^^xsd:nonNegativeInteger ;
	] ;
	rdfs:subClassOf [
		a owl:Restriction ;
		owl:onProperty osdu:persistableReference ;
		owl:minCardinality "1"^^xsd:nonNegativeInteger ;
	] ;
.

###  https://w3id.org/osdu#FrameOfReferenceUOM
osdu:FrameOfReferenceUOM rdf:type owl:Class ;
	rdfs:subClassOf osdu:AbstractMetaItem ;
	rdfs:subClassOf [
		a owl:Restriction ;
		owl:onProperty osdu:kind ;
		owl:minCardinality "1"^^xsd:nonNegativeInteger ;
	] ;
	rdfs:subClassOf [
		a owl:Restriction ;
		owl:onProperty osdu:persistableReference ;
		owl:minCardinality "1"^^xsd:nonNegativeInteger ;
	] ;
.

###  https://w3id.org/osdu#FundsAuthorizations
osdu:FundsAuthorizations rdf:type owl:Class ;
	rdfs:comment "The history of expenditure approvals. " ;
	rdfs:subClassOf owl:Thing ;
.

###  https://w3id.org/osdu#GasReading
osdu:GasReading rdf:type owl:Class ;
	rdfs:comment "General information about a gas reading taken during the drill report period " ;
	rdfs:subClassOf owl:Thing ;
	rdfs:subClassOf [
		a owl:Restriction ;
		owl:onProperty osdu:dateTime ;
		owl:minCardinality "1"^^xsd:nonNegativeInteger ;
	] ;
.

###  https://w3id.org/osdu#GasReadingType
osdu:GasReadingType rdf:type owl:Class ;
	rdfs:comment "Type of gas readings associated with an operations report " ;
	rdfs:subClassOf osdu:ReferenceData ;
	rdfs:subClassOf osdu:AbstractCommonResources ;
	rdfs:subClassOf osdu:AbstractReferenceType ;
.

###  https://w3id.org/osdu#Generic
osdu:Generic rdf:type owl:Class ;
	skos:prefLabel "File.Generic" ;
	rdfs:comment "The generic dataset file collection template. " ;
	rdfs:subClassOf osdu:Dataset ;
	rdfs:subClassOf osdu:AbstractCommonResources ;
	rdfs:subClassOf osdu:AbstractDataset ;
	rdfs:subClassOf osdu:AbstractFile ;
	rdfs:subClassOf osdu:AbstractFileCollection ;
.

###  https://w3id.org/osdu#GenericImage
osdu:GenericImage rdf:type owl:Class ;
	rdfs:comment "A generic image work-product-component, which associates an image dataset, typically a JPEG, PNG or TIFF file to a master-data or work-product-component item. GenericImage should not be used for geo-referenced images or core images, which have their own dedicated types. " ;
	rdfs:subClassOf osdu:WorkProductComponent ;
	rdfs:subClassOf osdu:AbstractCommonResources ;
	rdfs:subClassOf osdu:AbstractWPCGroupType ;
	rdfs:subClassOf osdu:AbstractWorkProductComponent ;
	rdfs:subClassOf foaf:Image ;
.

###  https://w3id.org/osdu#GenericProperty
osdu:GenericProperty rdf:type owl:Class ;
	rdfs:comment "The reservoir property representation record, derived from the RESQML AbstractProperty. In RESQML, all subsurface or surface values tied to specific topological locations (or IndexableElements) in a model are carried by any concrete data object that derives from abstract property (contained in the properties package) attached to one or more representations. A representation can have several properties and provides the indexable elements for these lists of values (for more information see IndexableElement). " ;
	rdfs:subClassOf osdu:WorkProductComponent ;
	rdfs:subClassOf osdu:AbstractCommonResources ;
	rdfs:subClassOf osdu:AbstractWPCGroupType ;
	rdfs:subClassOf osdu:AbstractWorkProductComponent ;
	rdfs:subClassOf osdu:AbstractReferencePropertyType ;
.

###  https://w3id.org/osdu#GenericRepresentation
osdu:GenericRepresentation rdf:type owl:Class ;
	rdfs:comment "1D or 2D representations of Geologic Objects such as fault sticks, horizon surfaces, etc. " ;
	rdfs:subClassOf osdu:WorkProductComponent ;
	rdfs:subClassOf osdu:AbstractCommonResources ;
	rdfs:subClassOf osdu:AbstractWPCGroupType ;
	rdfs:subClassOf osdu:AbstractWorkProductComponent ;
	rdfs:subClassOf osdu:AbstractRepresentation ;
.

###  https://w3id.org/osdu#GeoJSON
osdu:GeoJSON rdf:type owl:Class ;
	skos:prefLabel "File.GeoJSON" ;
	rdfs:comment "GeoJSON is an open standard format designed for representing simple geographical features, optionally along with their non-spatial attributes. It is based on the JSON format; the schema is available via https://geojson.org/schema/FeatureCollection.json. The features include points, line strings, polygons, and multi-part collections of these types. Coordinates are exclusively expressed in EPSG::4326. " ;
	rdfs:subClassOf osdu:Dataset ;
	rdfs:subClassOf osdu:AbstractCommonResources ;
	rdfs:subClassOf osdu:AbstractDataset ;
	rdfs:subClassOf osdu:AbstractFile ;
.

###  https://w3id.org/osdu#GeoJSONFeature
osdu:GeoJSONFeature rdf:type owl:Class ;
	skos:prefLabel "GeoJSON Feature" ;
	rdfs:subClassOf owl:Thing ;
	rdfs:subClassOf [
		a owl:Restriction ;
		owl:onProperty osdu:hasBBox ;
		owl:minQualifiedCardinality "4"^^xsd:nonNegativeInteger ;
		owl:onDataRange xsd:decimal ;
	] ;
	rdfs:subClassOf [
		a owl:Restriction ;
		owl:onProperty osdu:type ;
		owl:minCardinality "1"^^xsd:nonNegativeInteger ;
	] ;
	rdfs:subClassOf [
		a owl:Restriction ;
		owl:onProperty osdu:property ;
		owl:minCardinality "1"^^xsd:nonNegativeInteger ;
	] ;
	rdfs:subClassOf [
		a owl:Restriction ;
		owl:onProperty osdu:geometry ;
		owl:minCardinality "1"^^xsd:nonNegativeInteger ;
	] ;
.

###  https://w3id.org/osdu#GeoJSONGeometryCollection
osdu:GeoJSONGeometryCollection rdf:type owl:Class ;
	skos:prefLabel "GeoJSON GeometryCollection" ;
	rdfs:subClassOf owl:Thing ;
	rdfs:subClassOf [
		a owl:Restriction ;
		owl:onProperty osdu:hasBBox ;
		owl:minQualifiedCardinality "4"^^xsd:nonNegativeInteger ;
		owl:onDataRange xsd:decimal ;
	] ;
	rdfs:subClassOf [
		a owl:Restriction ;
		owl:onProperty osdu:type ;
		owl:minCardinality "1"^^xsd:nonNegativeInteger ;
	] ;
	rdfs:subClassOf [
		a owl:Restriction ;
		owl:onProperty osdu:geometry ;
		owl:minCardinality "1"^^xsd:nonNegativeInteger ;
	] ;
.

###  https://w3id.org/osdu#GeoJSONLineString
osdu:GeoJSONLineString rdf:type owl:Class ;
	skos:prefLabel "GeoJSON LineString" ;
	rdfs:subClassOf osdu:Geometries ;
	rdfs:subClassOf [
		a owl:Restriction ;
		owl:onProperty osdu:coordinate ;
		owl:minQualifiedCardinality "2"^^xsd:nonNegativeInteger ;
		owl:onClass osdu:GeoJSONLineStringCoordinatesArray ;
	] ;
	rdfs:subClassOf [
		a owl:Restriction ;
		owl:onProperty osdu:hasBBox ;
		owl:minQualifiedCardinality "4"^^xsd:nonNegativeInteger ;
		owl:onDataRange xsd:decimal ;
	] ;
	rdfs:subClassOf [
		a owl:Restriction ;
		owl:onProperty osdu:type ;
		owl:minCardinality "1"^^xsd:nonNegativeInteger ;
	] ;
	rdfs:subClassOf [
		a owl:Restriction ;
		owl:onProperty osdu:coordinate ;
		owl:minCardinality "1"^^xsd:nonNegativeInteger ;
	] ;
.

###  https://w3id.org/osdu#GeoJSONLineStringCoordinatesArray
osdu:GeoJSONLineStringCoordinatesArray rdf:type owl:Class ;
	rdfs:subClassOf osdu:Array ;
	rdfs:subClassOf [
		a owl:Restriction ;
		owl:onProperty osdu:item ;
		owl:minQualifiedCardinality "2"^^xsd:nonNegativeInteger ;
		owl:onDataRange xsd:decimal ;
	] ;
.

###  https://w3id.org/osdu#GeoJSONMultiLineString
osdu:GeoJSONMultiLineString rdf:type owl:Class ;
	skos:prefLabel "GeoJSON MultiLineString" ;
	rdfs:subClassOf osdu:Geometries ;
	rdfs:subClassOf [
		a owl:Restriction ;
		owl:onProperty osdu:hasBBox ;
		owl:minQualifiedCardinality "4"^^xsd:nonNegativeInteger ;
		owl:onDataRange xsd:decimal ;
	] ;
	rdfs:subClassOf [
		a owl:Restriction ;
		owl:onProperty osdu:type ;
		owl:minCardinality "1"^^xsd:nonNegativeInteger ;
	] ;
	rdfs:subClassOf [
		a owl:Restriction ;
		owl:onProperty osdu:coordinate ;
		owl:minCardinality "1"^^xsd:nonNegativeInteger ;
	] ;
.

###  https://w3id.org/osdu#GeoJSONMultiLineStringCoordinatesArray
osdu:GeoJSONMultiLineStringCoordinatesArray rdf:type owl:Class ;
	rdfs:subClassOf osdu:Array ;
	rdfs:subClassOf [
		a owl:Restriction ;
		owl:onProperty osdu:item ;
		owl:minQualifiedCardinality "2"^^xsd:nonNegativeInteger ;
		owl:onClass osdu:GeoJSONMultiLineStringCoordinatesArrayItemsArray ;
	] ;
.

###  https://w3id.org/osdu#GeoJSONMultiLineStringCoordinatesArrayItemsArray
osdu:GeoJSONMultiLineStringCoordinatesArrayItemsArray rdf:type owl:Class ;
	rdfs:subClassOf osdu:Array ;
	rdfs:subClassOf [
		a owl:Restriction ;
		owl:onProperty osdu:item ;
		owl:minQualifiedCardinality "2"^^xsd:nonNegativeInteger ;
		owl:onDataRange xsd:decimal ;
	] ;
.

###  https://w3id.org/osdu#GeoJSONMultiPoint
osdu:GeoJSONMultiPoint rdf:type owl:Class ;
	skos:prefLabel "GeoJSON MultiPoint" ;
	rdfs:subClassOf osdu:Geometries ;
	rdfs:subClassOf [
		a owl:Restriction ;
		owl:onProperty osdu:hasBBox ;
		owl:minQualifiedCardinality "4"^^xsd:nonNegativeInteger ;
		owl:onDataRange xsd:decimal ;
	] ;
	rdfs:subClassOf [
		a owl:Restriction ;
		owl:onProperty osdu:type ;
		owl:minCardinality "1"^^xsd:nonNegativeInteger ;
	] ;
	rdfs:subClassOf [
		a owl:Restriction ;
		owl:onProperty osdu:coordinate ;
		owl:minCardinality "1"^^xsd:nonNegativeInteger ;
	] ;
.

###  https://w3id.org/osdu#GeoJSONMultiPointCoordinatesArray
osdu:GeoJSONMultiPointCoordinatesArray rdf:type owl:Class ;
	rdfs:subClassOf osdu:Array ;
	rdfs:subClassOf [
		a owl:Restriction ;
		owl:onProperty osdu:item ;
		owl:minQualifiedCardinality "2"^^xsd:nonNegativeInteger ;
		owl:onDataRange xsd:decimal ;
	] ;
.

###  https://w3id.org/osdu#GeoJSONMultiPolygon
osdu:GeoJSONMultiPolygon rdf:type owl:Class ;
	skos:prefLabel "GeoJSON MultiPolygon" ;
	rdfs:subClassOf osdu:Geometries ;
	rdfs:subClassOf [
		a owl:Restriction ;
		owl:onProperty osdu:hasBBox ;
		owl:minQualifiedCardinality "4"^^xsd:nonNegativeInteger ;
		owl:onDataRange xsd:decimal ;
	] ;
	rdfs:subClassOf [
		a owl:Restriction ;
		owl:onProperty osdu:type ;
		owl:minCardinality "1"^^xsd:nonNegativeInteger ;
	] ;
	rdfs:subClassOf [
		a owl:Restriction ;
		owl:onProperty osdu:coordinate ;
		owl:minCardinality "1"^^xsd:nonNegativeInteger ;
	] ;
.

###  https://w3id.org/osdu#GeoJSONMultiPolygonCoordinatesArray
osdu:GeoJSONMultiPolygonCoordinatesArray rdf:type owl:Class ;
	rdfs:subClassOf osdu:Array ;
.

###  https://w3id.org/osdu#GeoJSONMultiPolygonCoordinatesArrayItemsArray
osdu:GeoJSONMultiPolygonCoordinatesArrayItemsArray rdf:type owl:Class ;
	rdfs:subClassOf osdu:Array ;
	rdfs:subClassOf [
		a owl:Restriction ;
		owl:onProperty osdu:item ;
		owl:minQualifiedCardinality "4"^^xsd:nonNegativeInteger ;
		owl:onClass osdu:GeoJSONMultiPolygonCoordinatesArrayItemsArrayItemsArray ;
	] ;
.

###  https://w3id.org/osdu#GeoJSONMultiPolygonCoordinatesArrayItemsArrayItemsArray
osdu:GeoJSONMultiPolygonCoordinatesArrayItemsArrayItemsArray rdf:type owl:Class ;
	rdfs:subClassOf osdu:Array ;
	rdfs:subClassOf [
		a owl:Restriction ;
		owl:onProperty osdu:item ;
		owl:minQualifiedCardinality "2"^^xsd:nonNegativeInteger ;
		owl:onDataRange xsd:decimal ;
	] ;
.

###  https://w3id.org/osdu#GeoJSONPoint
osdu:GeoJSONPoint rdf:type owl:Class ;
	skos:prefLabel "GeoJSON Point" ;
	rdfs:subClassOf osdu:Geometries ;
	rdfs:subClassOf [
		a owl:Restriction ;
		owl:onProperty osdu:coordinate ;
		owl:minQualifiedCardinality "2"^^xsd:nonNegativeInteger ;
		owl:onDataRange xsd:decimal ;
	] ;
	rdfs:subClassOf [
		a owl:Restriction ;
		owl:onProperty osdu:hasBBox ;
		owl:minQualifiedCardinality "4"^^xsd:nonNegativeInteger ;
		owl:onDataRange xsd:decimal ;
	] ;
	rdfs:subClassOf [
		a owl:Restriction ;
		owl:onProperty osdu:type ;
		owl:minCardinality "1"^^xsd:nonNegativeInteger ;
	] ;
	rdfs:subClassOf [
		a owl:Restriction ;
		owl:onProperty osdu:coordinate ;
		owl:minCardinality "1"^^xsd:nonNegativeInteger ;
	] ;
.

###  https://w3id.org/osdu#GeoJSONPolygon
osdu:GeoJSONPolygon rdf:type owl:Class ;
	skos:prefLabel "GeoJSON Polygon" ;
	rdfs:subClassOf osdu:Geometries ;
	rdfs:subClassOf [
		a owl:Restriction ;
		owl:onProperty osdu:hasBBox ;
		owl:minQualifiedCardinality "4"^^xsd:nonNegativeInteger ;
		owl:onDataRange xsd:decimal ;
	] ;
	rdfs:subClassOf [
		a owl:Restriction ;
		owl:onProperty osdu:type ;
		owl:minCardinality "1"^^xsd:nonNegativeInteger ;
	] ;
	rdfs:subClassOf [
		a owl:Restriction ;
		owl:onProperty osdu:coordinate ;
		owl:minCardinality "1"^^xsd:nonNegativeInteger ;
	] ;
.

###  https://w3id.org/osdu#GeoJSONPolygonCoordinatesArray
osdu:GeoJSONPolygonCoordinatesArray rdf:type owl:Class ;
	rdfs:subClassOf osdu:Array ;
	rdfs:subClassOf [
		a owl:Restriction ;
		owl:onProperty osdu:item ;
		owl:minQualifiedCardinality "4"^^xsd:nonNegativeInteger ;
		owl:onClass osdu:GeoJSONPolygonCoordinatesArrayItemsArray ;
	] ;
.

###  https://w3id.org/osdu#GeoJSONPolygonCoordinatesArrayItemsArray
osdu:GeoJSONPolygonCoordinatesArrayItemsArray rdf:type owl:Class ;
	rdfs:subClassOf osdu:Array ;
	rdfs:subClassOf [
		a owl:Restriction ;
		owl:onProperty osdu:item ;
		owl:minQualifiedCardinality "2"^^xsd:nonNegativeInteger ;
		owl:onDataRange xsd:decimal ;
	] ;
.

###  https://w3id.org/osdu#GeoPoliticalEntity
osdu:GeoPoliticalEntity rdf:type owl:Class ;
	rdfs:comment "A named geographical area which is defined and administered by an official entity. " ;
	rdfs:subClassOf osdu:MasterData ;
	rdfs:subClassOf osdu:AbstractCommonResources ;
	rdfs:subClassOf osdu:AbstractMaster ;
.

###  https://w3id.org/osdu#GeoPoliticalEntityType
osdu:GeoPoliticalEntityType rdf:type owl:Class ;
	rdfs:comment "Used to describe the type of geopolitical entities. " ;
	rdfs:subClassOf osdu:ReferenceData ;
	rdfs:subClassOf osdu:AbstractCommonResources ;
	rdfs:subClassOf osdu:AbstractReferenceType ;
.

###  https://w3id.org/osdu#GeoReferencedImage
osdu:GeoReferencedImage rdf:type owl:Class ;
	rdfs:comment "An image representation which contains a coordinate reference system or relates the image map or aerial photo image to a coordinate reference system. With this reference it is possible to compute world coordinates for each image pixel position. The mapping from pixel to world coordinates is often provided by companion file, a so-called world file, see: https://en.wikipedia.org/wiki/World_file. " ;
	rdfs:subClassOf osdu:WorkProductComponent ;
	rdfs:subClassOf osdu:AbstractCommonResources ;
	rdfs:subClassOf osdu:AbstractWPCGroupType ;
	rdfs:subClassOf osdu:AbstractWorkProductComponent ;
	rdfs:subClassOf foaf:Image ;
.

###  https://w3id.org/osdu#GeoReferencedImageType
osdu:GeoReferencedImageType rdf:type owl:Class ;
	rdfs:comment "The type of a geo-referenced image, like, e.g., horizontal map, vertical curtain. " ;
	rdfs:subClassOf osdu:ReferenceData ;
	rdfs:subClassOf osdu:AbstractCommonResources ;
	rdfs:subClassOf osdu:AbstractReferenceType ;
.

###  https://w3id.org/osdu#GeoTIFF
osdu:GeoTIFF rdf:type owl:Class ;
	skos:prefLabel "File.OGC.GeoTIFF" ;
	rdfs:comment "File.OGC.GeoTIFF represents a standard, tagged image file format defined by the Open Geospatial Consortium. The geospatial metadata are included or 'inlined' in the file. The geospatial information includes map projection, coordinate systems, ellipsoids, datums, and everything else necessary to establish the exact spatial reference for the file. " ;
	rdfs:subClassOf osdu:Dataset ;
	rdfs:subClassOf osdu:AbstractCommonResources ;
	rdfs:subClassOf osdu:AbstractDataset ;
	rdfs:subClassOf osdu:AbstractFile ;
	rdfs:subClassOf foaf:Image ;
.

###  https://w3id.org/osdu#GeobodyBoundaryInterpretation
osdu:GeobodyBoundaryInterpretation rdf:type owl:Class ;
	rdfs:comment "Geologic information associated to geobody boundary-related objects  (marker, seismic picks, modeled objects like triangulated surface) " ;
	rdfs:subClassOf osdu:WorkProductComponent ;
	rdfs:subClassOf osdu:AbstractCommonResources ;
	rdfs:subClassOf osdu:AbstractWPCGroupType ;
	rdfs:subClassOf osdu:AbstractWorkProductComponent ;
	rdfs:subClassOf osdu:AbstractInterpretation ;
.

###  https://w3id.org/osdu#GeobodyInterpretation
osdu:GeobodyInterpretation rdf:type owl:Class ;
	rdfs:comment "One of potentially many geobody interpretations as a single consistent description of a local rock volume feature. An interpretation is subjective and very strongly tied to the intellectual activity of the project team members. " ;
	rdfs:subClassOf osdu:WorkProductComponent ;
	rdfs:subClassOf osdu:AbstractCommonResources ;
	rdfs:subClassOf osdu:AbstractWPCGroupType ;
	rdfs:subClassOf osdu:AbstractWorkProductComponent ;
	rdfs:subClassOf osdu:AbstractGeologicUnitInterpretation ;
	rdfs:subClassOf osdu:AbstractInterpretation ;
.

###  https://w3id.org/osdu#GeologicUnitOccurrenceInterpretation
osdu:GeologicUnitOccurrenceInterpretation rdf:type owl:Class ;
	rdfs:comment "Interpretation of a sequence of geologic units actually observed (interpreted)  along or inside a representation, the representation can be  •	1D such as a well or an arbitrary line •	2D like a cross section •	3D like a entire model or a group of fault blocks It is typically based on a stratigraphic column rank but can include more units (example intrusive bodies), duplicated units (repeated sequence along a well or lines), or less units (Eroded or non-deposited). An ordering criteria indicates the reason for the order (age, apparent depth or measured depth). " ;
	rdfs:subClassOf osdu:WorkProductComponent ;
	rdfs:subClassOf osdu:AbstractCommonResources ;
	rdfs:subClassOf osdu:AbstractWPCGroupType ;
	rdfs:subClassOf osdu:AbstractWorkProductComponent ;
	rdfs:subClassOf osdu:AbstractInterpretation ;
.

###  https://w3id.org/osdu#GeologicUnitShapeType
osdu:GeologicUnitShapeType rdf:type owl:Class ;
	rdfs:comment "GeologicUnitShapeType holds the values for 3D shape classifications corresponding to the Energistics Shape3dExt. " ;
	rdfs:subClassOf osdu:ReferenceData ;
	rdfs:subClassOf osdu:AbstractCommonResources ;
	rdfs:subClassOf osdu:AbstractReferenceType ;
.

###  https://w3id.org/osdu#GeologicalFormation
osdu:GeologicalFormation rdf:type owl:Class ;
	rdfs:comment "The name given to a body of rock having a consistent set of physical (litho-stratigraphic), temporal (chrono-stratigraphic) or fossil (bio-stratigraphic) characteristics that distinguishes it from adjacent bodies of rock, and which occupies a particular position in the layers of rock in a geographical region. " ;
	rdfs:subClassOf osdu:ReferenceData ;
	rdfs:subClassOf osdu:AbstractCommonResources ;
	rdfs:subClassOf osdu:AbstractReferenceType ;
.

###  https://w3id.org/osdu#GeologyInterval
osdu:GeologyInterval rdf:type owl:Class ;
	skos:prefLabel "Geology Interval" ;
	rdfs:comment "Geology Interval Component Schema " ;
	rdfs:subClassOf owl:Thing ;
	rdfs:subClassOf [
		a owl:Restriction ;
		owl:onProperty osdu:intervalTopMeasuredDepth ;
		owl:minCardinality "1"^^xsd:nonNegativeInteger ;
	] ;
	rdfs:subClassOf [
		a owl:Restriction ;
		owl:onProperty osdu:intervalBaseMeasuredDepth ;
		owl:minCardinality "1"^^xsd:nonNegativeInteger ;
	] ;
	rdfs:subClassOf [
		a owl:Restriction ;
		owl:onProperty osdu:lithologyTypeID ;
		owl:minCardinality "1"^^xsd:nonNegativeInteger ;
	] ;
.

###  https://w3id.org/osdu#GeometricTargetSet
osdu:GeometricTargetSet rdf:type owl:Class ;
	rdfs:comment "Targets (in the geometrical point of view) for a drilling plan " ;
	rdfs:subClassOf osdu:MasterData ;
	rdfs:subClassOf osdu:AbstractCommonResources ;
	rdfs:subClassOf osdu:AbstractMaster ;
.

###  https://w3id.org/osdu#Geometries
osdu:Geometries rdf:type owl:Class ;
	rdfs:subClassOf owl:Thing ;
.

###  https://w3id.org/osdu#Geometry
osdu:Geometry rdf:type owl:Class ;
	rdfs:comment "The Geometry of the target. " ;
	rdfs:subClassOf owl:Thing ;
.

###  https://w3id.org/osdu#GeometrySection
osdu:GeometrySection rdf:type owl:Class ;
	skos:prefLabel "Geometry Section" ;
	rdfs:comment "The geometric sections that combine to define the shape of a complex target " ;
	rdfs:subClassOf owl:Thing ;
.

###  https://w3id.org/osdu#GpGridRepresentation
osdu:GpGridRepresentation rdf:type owl:Class ;
	rdfs:comment "General Purpose Grid. This Grid is the only one to be able to mix different grid representations (ijk, unstructured column layer, unstructured) into a single one without having to use grid refinement. " ;
	rdfs:subClassOf osdu:WorkProductComponent ;
	rdfs:subClassOf osdu:AbstractCommonResources ;
	rdfs:subClassOf osdu:AbstractWPCGroupType ;
	rdfs:subClassOf osdu:AbstractWorkProductComponent ;
	rdfs:subClassOf osdu:AbstractGridRepresentation ;
.

###  https://w3id.org/osdu#GrainDensityMeasurementType
osdu:GrainDensityMeasurementType rdf:type owl:Class ;
	rdfs:comment "The kind of grain density measurement, which is applied in, e.g. routine core analysis. " ;
	rdfs:subClassOf osdu:ReferenceData ;
	rdfs:subClassOf osdu:AbstractCommonResources ;
	rdfs:subClassOf osdu:AbstractReferenceType ;
.

###  https://w3id.org/osdu#GridConnectionSetRepresentation
osdu:GridConnectionSetRepresentation rdf:type owl:Class ;
	rdfs:comment "A list of cell (and optionally local face) connections in a grid. " ;
	rdfs:subClassOf osdu:WorkProductComponent ;
	rdfs:subClassOf osdu:AbstractCommonResources ;
	rdfs:subClassOf osdu:AbstractWPCGroupType ;
	rdfs:subClassOf osdu:AbstractWorkProductComponent ;
	rdfs:subClassOf osdu:AbstractRepresentation ;
.

###  https://w3id.org/osdu#HeaderKeyName
osdu:HeaderKeyName rdf:type owl:Class ;
	rdfs:comment "Reference data for header names of standard fields used in storage file formats, such as CDPX, INLINE in SEGY. " ;
	rdfs:subClassOf osdu:ReferenceData ;
	rdfs:subClassOf osdu:AbstractCommonResources ;
	rdfs:subClassOf osdu:AbstractReferenceType ;
.

###  https://w3id.org/osdu#HealthSafetyEnvironment
osdu:HealthSafetyEnvironment rdf:type owl:Class ;
	skos:prefLabel "Health Safety Environment" ;
	rdfs:comment "Health Safety or Environment events that occurred since the last drilling/operation report. Captures data related to HSE events (e.g., tests, inspections, meetings, and drills), test values (e.g., pressure tested to), and/or incidents (e.g., discharges, non-compliance notices received, etc.). " ;
	rdfs:subClassOf owl:Thing ;
.

###  https://w3id.org/osdu#HistoricalInterest
osdu:HistoricalInterest rdf:type owl:Class ;
	rdfs:comment "A 'well interest' at some time period as defined by effective and termination date. " ;
	rdfs:subClassOf owl:Thing ;
.

###  https://w3id.org/osdu#HoleSection
osdu:HoleSection rdf:type owl:Class ;
	rdfs:comment "A section of a wellbore of a constant diameter " ;
	rdfs:subClassOf osdu:MasterData ;
	rdfs:subClassOf osdu:AbstractCommonResources ;
	rdfs:subClassOf osdu:AbstractMaster ;
.

###  https://w3id.org/osdu#HorizonInterpretation
osdu:HorizonInterpretation rdf:type owl:Class ;
	rdfs:comment "Geologic information associated to horizon-related object types (marker, seismic picks, modeled objects etc…) " ;
	rdfs:subClassOf osdu:WorkProductComponent ;
	rdfs:subClassOf osdu:AbstractCommonResources ;
	rdfs:subClassOf osdu:AbstractWPCGroupType ;
	rdfs:subClassOf osdu:AbstractWorkProductComponent ;
	rdfs:subClassOf osdu:AbstractInterpretation ;
.

###  https://w3id.org/osdu#HorizontalCRS
osdu:HorizontalCRS rdf:type owl:Class ;
	skos:prefLabel "Horizontal CRS" ;
	rdfs:comment "The horizontal CRS reference of a CompoundCRS. Only populated for CoordinateReferenceSystemType==CompoundCRS. " ;
	rdfs:subClassOf owl:Thing ;
.

###  https://w3id.org/osdu#IjkCellFace
osdu:IjkCellFace rdf:type owl:Class ;
	rdfs:comment "An enumeration of the face of a cell in an IJK grid. " ;
	rdfs:subClassOf osdu:ReferenceData ;
	rdfs:subClassOf osdu:AbstractCommonResources ;
	rdfs:subClassOf osdu:AbstractReferenceType ;
.

###  https://w3id.org/osdu#IjkGridNumericalAquiferRepresentation
osdu:IjkGridNumericalAquiferRepresentation rdf:type owl:Class ;
	rdfs:comment "A numerical aquifer representation defines the geometry of the aquifer as IJK grid cell indices. " ;
	rdfs:subClassOf osdu:WorkProductComponent ;
	rdfs:subClassOf osdu:AbstractCommonResources ;
	rdfs:subClassOf osdu:AbstractWPCGroupType ;
	rdfs:subClassOf osdu:AbstractWorkProductComponent ;
	rdfs:subClassOf osdu:AbstractRepresentation ;
.

###  https://w3id.org/osdu#IjkGridRepresentation
osdu:IjkGridRepresentation rdf:type owl:Class ;
	rdfs:comment "Definition of a collection of hexahedra which are organized and indexable by means of 3 (almost orthogonal) directions and called I, J and K. " ;
	rdfs:subClassOf osdu:WorkProductComponent ;
	rdfs:subClassOf osdu:AbstractCommonResources ;
	rdfs:subClassOf osdu:AbstractWPCGroupType ;
	rdfs:subClassOf osdu:AbstractWorkProductComponent ;
	rdfs:subClassOf osdu:AbstractGridRepresentation ;
	rdfs:subClassOf osdu:AbstractIjkGridPatch ;
.

###  https://w3id.org/osdu#InSARApplication
osdu:InSARApplication rdf:type owl:Class ;
	rdfs:comment "The primary business application of the InSAR data set " ;
	rdfs:subClassOf osdu:ReferenceData ;
	rdfs:subClassOf osdu:AbstractCommonResources ;
	rdfs:subClassOf osdu:AbstractReferenceType ;
.

###  https://w3id.org/osdu#InSARFrequencyBand
osdu:InSARFrequencyBand rdf:type owl:Class ;
	rdfs:comment "The reference value type defining the frequency band of the radar used for the image acquisition " ;
	rdfs:subClassOf osdu:ReferenceData ;
	rdfs:subClassOf osdu:AbstractCommonResources ;
	rdfs:subClassOf osdu:AbstractReferenceType ;
.

###  https://w3id.org/osdu#InSARImageMode
osdu:InSARImageMode rdf:type owl:Class ;
	rdfs:comment "The reference value type defining the radar imaging mode utilised for image acquisition " ;
	rdfs:subClassOf osdu:ReferenceData ;
	rdfs:subClassOf osdu:AbstractCommonResources ;
	rdfs:subClassOf osdu:AbstractReferenceType ;
.

###  https://w3id.org/osdu#InSARPolarisation
osdu:InSARPolarisation rdf:type owl:Class ;
	rdfs:comment "the reference value type defining the radar polarisation utilised for the image acquisition. The polarisation being the direction of the electromagnetic wave. " ;
	rdfs:subClassOf osdu:ReferenceData ;
	rdfs:subClassOf osdu:AbstractCommonResources ;
	rdfs:subClassOf osdu:AbstractReferenceType ;
.

###  https://w3id.org/osdu#InSARProcessingType
osdu:InSARProcessingType rdf:type owl:Class ;
	rdfs:comment "Describes what main process or workflow manipulated the data before arriving at its current state or that it is as acquired " ;
	rdfs:subClassOf osdu:ReferenceData ;
	rdfs:subClassOf osdu:AbstractCommonResources ;
	rdfs:subClassOf osdu:AbstractReferenceType ;
.

###  https://w3id.org/osdu#Incident
osdu:Incident rdf:type owl:Class ;
	rdfs:comment "Description of incidents that have occurred during the last drilling/operations report " ;
	rdfs:subClassOf owl:Thing ;
	rdfs:subClassOf [
		a owl:Restriction ;
		owl:onProperty osdu:dateTime ;
		owl:minCardinality "1"^^xsd:nonNegativeInteger ;
	] ;
.

###  https://w3id.org/osdu#IndexableElement
osdu:IndexableElement rdf:type owl:Class ;
	rdfs:comment "IndexableElement follows the RESQML pattern. IndexableElement is used to 1) contain geometry within a representation, 2) attach properties to a representation, 3) identify portions of a representation when expressing a representation identity, and 4) construct a sub-representation from an existing representation. Several specialized indexable elements, e.g., hinge node faces, have been included to add higher order geometry to a grid representation, and are not available for other purposes. " ;
	rdfs:subClassOf osdu:ReferenceData ;
	rdfs:subClassOf osdu:AbstractCommonResources ;
	rdfs:subClassOf osdu:AbstractReferenceType ;
.

###  https://w3id.org/osdu#IndexableElementCount
osdu:IndexableElementCount rdf:type owl:Class ;
	rdfs:comment "Defines the count of a particular indexable element in a representation " ;
	rdfs:subClassOf owl:Thing ;
	rdfs:subClassOf [
		a owl:Restriction ;
		owl:onProperty osdu:count ;
		owl:minCardinality "1"^^xsd:nonNegativeInteger ;
	] ;
.

###  https://w3id.org/osdu#InstalledTubular
osdu:InstalledTubular rdf:type owl:Class ;
	skos:prefLabel "Installed Tubular" ;
	rdfs:comment "Geometrical Description of tubular assembly as installed in the wellbore " ;
	rdfs:subClassOf owl:Thing ;
	rdfs:subClassOf [
		a owl:Restriction ;
		owl:onProperty osdu:tubularAssemblyID ;
		owl:minCardinality "1"^^xsd:nonNegativeInteger ;
	] ;
.

###  https://w3id.org/osdu#InterpolationMethod
osdu:InterpolationMethod rdf:type owl:Class ;
	rdfs:comment "Mathematical form of velocity interpolation between discretely sample nodes, such as linear in space, bicubic spline, linear in time, trilinear, horizon-based, constant vertically up, constant vertically down, constant vertically both ways. " ;
	rdfs:subClassOf osdu:ReferenceData ;
	rdfs:subClassOf osdu:AbstractCommonResources ;
	rdfs:subClassOf osdu:AbstractReferenceType ;
.

###  https://w3id.org/osdu#Interval
osdu:Interval rdf:type owl:Class ;
	rdfs:comment "An interval given either by relationships to top/base markers or standalone top/base depths. To avoid confusion about entry and exit depths the naming convention uses Start as the entry point of the well path into the geologic unit and Stop as the exit point. For unfolded geologic units and vertical wellbores Start is Top and Stop is Base. " ;
	rdfs:subClassOf owl:Thing ;
.

###  https://w3id.org/osdu#Inventory
osdu:Inventory rdf:type owl:Class ;
	rdfs:comment "Quantity of items inventoried during drilling and/or operations " ;
	rdfs:subClassOf owl:Thing ;
.

###  https://w3id.org/osdu#JPEG
osdu:JPEG rdf:type owl:Class ;
	skos:prefLabel "File.Image.JPEG" ;
	rdfs:comment "An image file in JPEG format, https://en.wikipedia.org/wiki/JPEG. " ;
	rdfs:subClassOf osdu:Dataset ;
	rdfs:subClassOf osdu:AbstractCommonResources ;
	rdfs:subClassOf osdu:AbstractDataset ;
	rdfs:subClassOf osdu:AbstractFile ;
	rdfs:subClassOf foaf:Image ;
.

###  https://w3id.org/osdu#KDirectionType
osdu:KDirectionType rdf:type owl:Class ;
	rdfs:comment "An enumeration for the K-Direction based on the RESQML model, i.e. up, down, not monotonic. " ;
	rdfs:subClassOf osdu:ReferenceData ;
	rdfs:subClassOf osdu:AbstractCommonResources ;
	rdfs:subClassOf osdu:AbstractReferenceType ;
.

###  https://w3id.org/osdu#LegalStatus
osdu:LegalStatus rdf:type owl:Class ;
	rdfs:comment "The status of a legal status evaluation. Typical values are compliant and incompliant. " ;
	rdfs:subClassOf osdu:ReferenceData ;
	rdfs:subClassOf osdu:AbstractCommonResources ;
	rdfs:subClassOf osdu:AbstractReferenceType ;
.

###  https://w3id.org/osdu#LengthRange
osdu:LengthRange rdf:type owl:Class ;
	rdfs:comment "A range container carrying minimum/maximum angle values. " ;
	rdfs:subClassOf owl:Thing ;
.

###  https://w3id.org/osdu#LicenseState
osdu:LicenseState rdf:type owl:Class ;
	rdfs:comment "The record's license state. Typical values are: Proprietary, Licensed, Unlicensed. " ;
	rdfs:subClassOf osdu:ReferenceData ;
	rdfs:subClassOf osdu:AbstractCommonResources ;
	rdfs:subClassOf osdu:AbstractReferenceType ;
.

###  https://w3id.org/osdu#LineageAssertion
osdu:LineageAssertion rdf:type owl:Class ;
	rdfs:comment "Defines relationships with other objects (any kind of Resource) upon which this work product component depends.  The assertion is directed only from the asserting WPC to ancestor objects, not children.  It should not be used to refer to files or artefacts within the WPC -- the association within the WPC is sufficient and Artefacts are actually children of the main WPC file. They should be recorded in the data.Artefacts[] array. " ;
	rdfs:subClassOf owl:Thing ;
.

###  https://w3id.org/osdu#LineageRelationshipType
osdu:LineageRelationshipType rdf:type owl:Class ;
	rdfs:comment "Used by LineageAssertion to describe the nature of the line of descent of a work product component from a prior Resource, such as DIRECT, INDIRECT, REFERENCE.  It is not for proximity (number of nodes away), it is not to cover all the relationships in a full ontology or graph, and it is not to describe the type of activity that created the asserting Work Product or Work Product Component.  LineageAssertion does not encompass a full provenance, process history, or activity model. " ;
	rdfs:subClassOf osdu:ReferenceData ;
	rdfs:subClassOf osdu:AbstractCommonResources ;
	rdfs:subClassOf osdu:AbstractReferenceType ;
.

###  https://w3id.org/osdu#LinerType
osdu:LinerType rdf:type owl:Class ;
	rdfs:comment "This reference table describes the type of liner used in the borehole. For example, slotted, gravel packed or pre-perforated etc. " ;
	rdfs:subClassOf osdu:ReferenceData ;
	rdfs:subClassOf osdu:AbstractCommonResources ;
	rdfs:subClassOf osdu:AbstractReferenceType ;
.

###  https://w3id.org/osdu#LithoStratigraphy
osdu:LithoStratigraphy rdf:type owl:Class ;
	rdfs:comment "Name of lithostratigraphy, regionally dependent " ;
	rdfs:subClassOf osdu:ReferenceData ;
	rdfs:subClassOf osdu:AbstractCommonResources ;
	rdfs:subClassOf osdu:AbstractReferenceType ;
.

###  https://w3id.org/osdu#LithologyType
osdu:LithologyType rdf:type owl:Class ;
	rdfs:comment "Geological description for the type of lithology " ;
	rdfs:subClassOf osdu:ReferenceData ;
	rdfs:subClassOf osdu:AbstractCommonResources ;
	rdfs:subClassOf osdu:AbstractReferenceType ;
.

###  https://w3id.org/osdu#LocalBoundaryFeature
osdu:LocalBoundaryFeature rdf:type owl:Class ;
	rdfs:comment "An interface between two geological objects, such as horizons and faults in the scope of a model. It is a surface object. The scope can be widened by establishing a relationship to a master-data--BoundaryFeature instance. " ;
	rdfs:subClassOf osdu:WorkProductComponent ;
	rdfs:subClassOf osdu:AbstractCommonResources ;
	rdfs:subClassOf osdu:AbstractWPCGroupType ;
	rdfs:subClassOf osdu:AbstractWorkProductComponent ;
.

###  https://w3id.org/osdu#LocalModelCompoundCrs
osdu:LocalModelCompoundCrs rdf:type owl:Class ;
	rdfs:comment "This WPC intends to be a placeholder for storing metadata about the CRS in a Reservoir study. No attribute is present yet but could be added in next releases. The main intent is for now to be able to reference the same CRS (whatever how it is defined) from several representations. " ;
	rdfs:subClassOf osdu:WorkProductComponent ;
	rdfs:subClassOf osdu:AbstractCommonResources ;
	rdfs:subClassOf osdu:AbstractWPCGroupType ;
	rdfs:subClassOf osdu:AbstractWorkProductComponent ;
.

###  https://w3id.org/osdu#LocalModelFeature
osdu:LocalModelFeature rdf:type owl:Class ;
	rdfs:comment "A LocalModelFeature is an explicit description of the relationships between geologic features such as rock volume features (e.g. stratigraphic units, geobodies, phase unit) and boundary features (e.g., genetic, tectonic, and fluid boundaries). " ;
	rdfs:subClassOf osdu:WorkProductComponent ;
	rdfs:subClassOf osdu:AbstractCommonResources ;
	rdfs:subClassOf osdu:AbstractWPCGroupType ;
	rdfs:subClassOf osdu:AbstractWorkProductComponent ;
.

###  https://w3id.org/osdu#LocalRockVolumeFeature
osdu:LocalRockVolumeFeature rdf:type owl:Class ;
	rdfs:comment "A volume of rock that is identified based on some specific attribute, like its mineral content or other physical characteristic. It exists typically in the scope of a model, can be associated with a master-data--RockVolumeFeature for regional correlations. " ;
	rdfs:subClassOf osdu:WorkProductComponent ;
	rdfs:subClassOf osdu:AbstractCommonResources ;
	rdfs:subClassOf osdu:AbstractWPCGroupType ;
	rdfs:subClassOf osdu:AbstractWorkProductComponent ;
.

###  https://w3id.org/osdu#LogCurveBusinessValue
osdu:LogCurveBusinessValue rdf:type owl:Class ;
	rdfs:comment "Used to describe the log curve business values. " ;
	rdfs:subClassOf osdu:ReferenceData ;
	rdfs:subClassOf osdu:AbstractCommonResources ;
	rdfs:subClassOf osdu:AbstractReferenceType ;
.

###  https://w3id.org/osdu#LogCurveFamily
osdu:LogCurveFamily rdf:type owl:Class ;
	rdfs:comment "LogCurveFamily is the detailed Geological Physical Quantity Measured - such as neutron porosity. " ;
	rdfs:subClassOf osdu:ReferenceData ;
	rdfs:subClassOf osdu:AbstractCommonResources ;
	rdfs:subClassOf osdu:AbstractReferenceType ;
.

###  https://w3id.org/osdu#LogCurveMainFamily
osdu:LogCurveMainFamily rdf:type owl:Class ;
	rdfs:comment "LogCurveMainFamily is the Geological Physical Quantity Measured - such as porosity  " ;
	rdfs:subClassOf osdu:ReferenceData ;
	rdfs:subClassOf osdu:AbstractCommonResources ;
	rdfs:subClassOf osdu:AbstractReferenceType ;
.

###  https://w3id.org/osdu#LogCurveType
osdu:LogCurveType rdf:type owl:Class ;
	rdfs:comment "LogCurveType is the standard mnemonic chosen by the company - OSDU provides an initial list. " ;
	rdfs:subClassOf osdu:ReferenceData ;
	rdfs:subClassOf osdu:AbstractCommonResources ;
	rdfs:subClassOf osdu:AbstractReferenceType ;
.

###  https://w3id.org/osdu#LogServiceDateInterval
osdu:LogServiceDateInterval rdf:type owl:Class ;
	rdfs:comment "An interval built from two nested values : StartDate and EndDate. It applies to the whole log services and may apply to composite logs as [start of the first run job] and [end of the last run job]Log Service Date " ;
	rdfs:subClassOf owl:Thing ;
.

###  https://w3id.org/osdu#LogType
osdu:LogType rdf:type owl:Class ;
	rdfs:comment "Used to describe the type of logs. " ;
	rdfs:subClassOf osdu:ReferenceData ;
	rdfs:subClassOf osdu:AbstractCommonResources ;
	rdfs:subClassOf osdu:AbstractReferenceType ;
.

###  https://w3id.org/osdu#MarkerProperty
osdu:MarkerProperty rdf:type owl:Class ;
	rdfs:comment "A set of properties describing a marker property which is available for this instance of a WellboreMarkerSet. " ;
	rdfs:subClassOf owl:Thing ;
.

###  https://w3id.org/osdu#MarkerPropertyType
osdu:MarkerPropertyType rdf:type owl:Class ;
	rdfs:comment "The wellbore marker property catalog for e.g. WellboreMarkerSet data.AvailableMarkerProperties. Similar to LogCurveType and the TrajectoryStationPropertyType which describes well-known properties (or curves or channels in an array view), which can be accessed via the Wellbore Domain Data Management Services. " ;
	rdfs:subClassOf osdu:ReferenceData ;
	rdfs:subClassOf osdu:AbstractCommonResources ;
	rdfs:subClassOf osdu:AbstractReferenceType ;
	rdfs:subClassOf osdu:AbstractReferencePropertyType ;
.

###  https://w3id.org/osdu#MarkerType
osdu:MarkerType rdf:type owl:Class ;
	rdfs:comment "Used to describe the type of markers. " ;
	rdfs:subClassOf osdu:ReferenceData ;
	rdfs:subClassOf osdu:AbstractCommonResources ;
	rdfs:subClassOf osdu:AbstractReferenceType ;
.

###  https://w3id.org/osdu#Markers
osdu:Markers rdf:type owl:Class ;
	rdfs:comment "The array of marker meta data in this set. " ;
	rdfs:subClassOf owl:Thing ;
.

###  https://w3id.org/osdu#MasterData
osdu:MasterData rdf:type owl:Class ;
	rdfs:subClassOf osdu:System ;
.

###  https://w3id.org/osdu#MaterialType
osdu:MaterialType rdf:type owl:Class ;
	rdfs:comment "DEPRECATED: Used to describe the type of materials. This catalog contains a mixture of very different materials and has been replaced by TubularMaterialType and WellProductType. " ;
	rdfs:subClassOf osdu:ReferenceData ;
	rdfs:subClassOf osdu:AbstractCommonResources ;
	rdfs:subClassOf osdu:AbstractReferenceType ;
.

###  https://w3id.org/osdu#MaximumFlowratePump
osdu:MaximumFlowratePump rdf:type owl:Class ;
	skos:prefLabel "Flowrate Pump Maximum" ;
	rdfs:comment "The planned maximum flowrate for the run " ;
	rdfs:subClassOf owl:Thing ;
	rdfs:subClassOf [
		a owl:Restriction ;
		owl:onproperty osdu:hasPoint;
		owl:minCardinality "1"^^xsd:nonNegativeInteger ;
	] ;
.

###  https://w3id.org/osdu#MaximumROP
osdu:MaximumROP rdf:type owl:Class ;
	skos:prefLabel "Maximum R.O.P." ;
	rdfs:comment "The planned maximum rate of penetration for the run " ;
	rdfs:subClassOf owl:Thing ;
	rdfs:subClassOf [
		a owl:Restriction ;
		owl:onproperty osdu:hasPoint;
		owl:minCardinality "1"^^xsd:nonNegativeInteger ;
	] ;
.

###  https://w3id.org/osdu#MaximumRPM
osdu:MaximumRPM rdf:type owl:Class ;
	skos:prefLabel "Maximum RPM" ;
	rdfs:comment "The planned maximum rotary speed for the run " ;
	rdfs:subClassOf owl:Thing ;
	rdfs:subClassOf [
		a owl:Restriction ;
		owl:onproperty osdu:hasPoint;
		owl:minCardinality "1"^^xsd:nonNegativeInteger ;
	] ;
.

###  https://w3id.org/osdu#MaximumTorqueOnBottom
osdu:MaximumTorqueOnBottom rdf:type owl:Class ;
	skos:prefLabel "Maximum Torque On Bottom" ;
	rdfs:comment "The planned maximum torque while on bottom " ;
	rdfs:subClassOf owl:Thing ;
	rdfs:subClassOf [
		a owl:Restriction ;
		owl:onproperty osdu:hasPoint;
		owl:minCardinality "1"^^xsd:nonNegativeInteger ;
	] ;
.

###  https://w3id.org/osdu#MaximumWOB
osdu:MaximumWOB rdf:type owl:Class ;
	skos:prefLabel "Maximum W.O.B." ;
	rdfs:comment "The planned maximum weight on bit for this run " ;
	rdfs:subClassOf owl:Thing ;
	rdfs:subClassOf [
		a owl:Restriction ;
		owl:onproperty osdu:hasPoint;
		owl:minCardinality "1"^^xsd:nonNegativeInteger ;
	] ;
.

###  https://w3id.org/osdu#Method
osdu:Method rdf:type owl:Class ;
	skos:prefLabel "Transformation Method" ;
	rdfs:comment "The Transformation method; Concatenated for CoordinateTransformationType == ConcatenatedOperation; EPSG method code and name for CoordinateTransformationType == Transformation. " ;
	rdfs:subClassOf owl:Thing ;
.

###  https://w3id.org/osdu#MinimumFlowratePump
osdu:MinimumFlowratePump rdf:type owl:Class ;
	skos:prefLabel "Flowrate Pump Minimum" ;
	rdfs:comment "The planned minimum flowrate for the run " ;
	rdfs:subClassOf owl:Thing ;
	rdfs:subClassOf [
		a owl:Restriction ;
		owl:onproperty osdu:hasPoint;
		owl:minCardinality "1"^^xsd:nonNegativeInteger ;
	] ;
.

###  https://w3id.org/osdu#MinimumROP
osdu:MinimumROP rdf:type owl:Class ;
	skos:prefLabel "Minimum R.O.P." ;
	rdfs:comment "The planned minimum rate of penetration for the run " ;
	rdfs:subClassOf owl:Thing ;
	rdfs:subClassOf [
		a owl:Restriction ;
		owl:onproperty osdu:hasPoint;
		owl:minCardinality "1"^^xsd:nonNegativeInteger ;
	] ;
.

###  https://w3id.org/osdu#MinimumRPM
osdu:MinimumRPM rdf:type owl:Class ;
	skos:prefLabel "Minimum RPM" ;
	rdfs:comment "The planned minimum rotary speed for the run " ;
	rdfs:subClassOf owl:Thing ;
	rdfs:subClassOf [
		a owl:Restriction ;
		owl:onproperty osdu:hasPoint;
		owl:minCardinality "1"^^xsd:nonNegativeInteger ;
	] ;
.

###  https://w3id.org/osdu#MinimumTorqueOnBottom
osdu:MinimumTorqueOnBottom rdf:type owl:Class ;
	skos:prefLabel "Minimum Torque On Bottom" ;
	rdfs:comment "The planned minimum torque while on bottom " ;
	rdfs:subClassOf owl:Thing ;
	rdfs:subClassOf [
		a owl:Restriction ;
		owl:onproperty osdu:hasPoint;
		owl:minCardinality "1"^^xsd:nonNegativeInteger ;
	] ;
.

###  https://w3id.org/osdu#MinimumWOB
osdu:MinimumWOB rdf:type owl:Class ;
	skos:prefLabel "Minimum W.O.B." ;
	rdfs:comment "The planned minimum weight on bit for this run " ;
	rdfs:subClassOf owl:Thing ;
	rdfs:subClassOf [
		a owl:Restriction ;
		owl:onproperty osdu:hasPoint;
		owl:minCardinality "1"^^xsd:nonNegativeInteger ;
	] ;
.

###  https://w3id.org/osdu#ModelFeature
osdu:ModelFeature rdf:type owl:Class ;
	rdfs:comment "A ModelFeature is an explicit description of the relationships between geologic features such as rock volume features (e.g. stratigraphic units, geobodies, phase unit) and boundary features (e.g., genetic, tectonic, and fluid boundaries). " ;
	rdfs:subClassOf osdu:MasterData ;
	rdfs:subClassOf osdu:AbstractCommonResources ;
	rdfs:subClassOf osdu:AbstractMaster ;
.

###  https://w3id.org/osdu#MudClass
osdu:MudClass rdf:type owl:Class ;
	rdfs:comment "The status of the fluid liquid. Proposed reference values: water based, oil based, other, pneumatic, unknown " ;
	rdfs:subClassOf osdu:ReferenceData ;
	rdfs:subClassOf osdu:AbstractCommonResources ;
	rdfs:subClassOf osdu:AbstractReferenceType ;
.

###  https://w3id.org/osdu#MudLosses
osdu:MudLosses rdf:type owl:Class ;
	skos:prefLabel "Mud Losses" ;
	rdfs:comment "Mud that has been lost during drilling / operations " ;
	rdfs:subClassOf owl:Thing ;
	rdfs:subClassOf [
		a owl:Restriction ;
		owl:onProperty osdu:dateTime ;
		owl:minCardinality "1"^^xsd:nonNegativeInteger ;
	] ;
.

###  https://w3id.org/osdu#MudPump
osdu:MudPump rdf:type owl:Class ;
	skos:prefLabel "Mud Pump" ;
	rdfs:comment "Pumps present on the rig " ;
	rdfs:subClassOf owl:Thing ;
.

###  https://w3id.org/osdu#MudVolume
osdu:MudVolume rdf:type owl:Class ;
	rdfs:comment "Information related to mud volumes for drilling/operations report " ;
	rdfs:subClassOf owl:Thing ;
	rdfs:subClassOf [
		a owl:Restriction ;
		owl:onProperty osdu:dateTime ;
		owl:minCardinality "1"^^xsd:nonNegativeInteger ;
	] ;
.

###  https://w3id.org/osdu#NotionalSeismicLine
osdu:NotionalSeismicLine rdf:type owl:Class ;
	rdfs:comment "The set of geometries comprising a full seismic transect (referenced through parent-child relationships).  This entity encompasses the concept of a logical processed line.  The parts comprising it cover things like extensions and boundary crossings.  It is largely a data management object to help collect all the geometries pertaining to a transect.  It is not needed for interpretation.  The universal WPC Name property is essential for describing the principal, preferred line name for the full transect. " ;
	rdfs:subClassOf osdu:WorkProductComponent ;
	rdfs:subClassOf osdu:AbstractCommonResources ;
	rdfs:subClassOf osdu:AbstractWPCGroupType ;
	rdfs:subClassOf osdu:AbstractWorkProductComponent ;
.

###  https://w3id.org/osdu#OAuth2FlowType
osdu:OAuth2FlowType rdf:type owl:Class ;
	rdfs:subClassOf owl:Thing ;
.

###  https://w3id.org/osdu#OSDUJsonExtensions
osdu:OSDUJsonExtensions rdf:type owl:Class ;
	rdfs:comment "These records build the catalog of OSDU JSON extensions tags, which are known to the system. " ;
	rdfs:subClassOf osdu:ReferenceData ;
	rdfs:subClassOf osdu:AbstractCommonResources ;
	rdfs:subClassOf osdu:AbstractReferenceType ;
.

###  https://w3id.org/osdu#OSDURegion
osdu:OSDURegion rdf:type owl:Class ;
	rdfs:comment "Used to describe the OSDU regions. " ;
	rdfs:subClassOf osdu:ReferenceData ;
	rdfs:subClassOf osdu:AbstractCommonResources ;
	rdfs:subClassOf osdu:AbstractReferenceType ;
.

###  https://w3id.org/osdu#ObjectAlias
osdu:ObjectAlias rdf:type owl:Class ;
	skos:prefLabel "Object Alias" ;
	rdfs:comment "Definition of an alias " ;
	rdfs:subClassOf owl:Thing ;
	rdfs:subClassOf [
		a owl:Restriction ;
		owl:onProperty osdu:identifier ;
		owl:minCardinality "1"^^xsd:nonNegativeInteger ;
	] ;
	rdfs:subClassOf [
		a owl:Restriction ;
		owl:onProperty osdu:authority ;
		owl:minCardinality "1"^^xsd:nonNegativeInteger ;
	] ;
.

###  https://w3id.org/osdu#ObjectiveType
osdu:ObjectiveType rdf:type owl:Class ;
	rdfs:comment "Purpose or intended use of a work product component, such as Stacking, Depth Migration, Time Migration, Time-depth Conversion. " ;
	rdfs:subClassOf osdu:ReferenceData ;
	rdfs:subClassOf osdu:AbstractCommonResources ;
	rdfs:subClassOf osdu:AbstractReferenceType ;
.

###  https://w3id.org/osdu#ObligationType
osdu:ObligationType rdf:type owl:Class ;
	rdfs:comment "An article or clause [OSDU calls this Obligation Type] that introduces a condition or term which the fulfillment of an agreement depends (provides operational and/or earning requirements) A kind of commitment or duty that in specific scenarios requires a particular course of action as defined in an agreement. " ;
	rdfs:subClassOf osdu:ReferenceData ;
	rdfs:subClassOf osdu:AbstractCommonResources ;
	rdfs:subClassOf osdu:AbstractReferenceType ;
.

###  https://w3id.org/osdu#OpenVDS
osdu:OpenVDS rdf:type owl:Class ;
	skos:prefLabel "FileCollection.Bluware.OpenVDS" ;
	rdfs:comment "The dataset representation for optimized seismic access using the OpenVDS (Open Volume Data Store) framework. " ;
	rdfs:subClassOf osdu:Dataset ;
	rdfs:subClassOf osdu:AbstractCommonResources ;
	rdfs:subClassOf osdu:AbstractDataset ;
	rdfs:subClassOf osdu:AbstractFileCollection ;
.

###  https://w3id.org/osdu#OpenZGY
osdu:OpenZGY rdf:type owl:Class ;
	skos:prefLabel "FileCollection.Slb.OpenZGY" ;
	rdfs:comment "The dataset representation for optimized seismic access to the OpenZGY framework developed by Schlumberger, storing seismic 3D data for seismic interpretation. " ;
	rdfs:subClassOf osdu:Dataset ;
	rdfs:subClassOf osdu:AbstractCommonResources ;
	rdfs:subClassOf osdu:AbstractDataset ;
	rdfs:subClassOf osdu:AbstractFileCollection ;
.

###  https://w3id.org/osdu#OperatingEnvironment
osdu:OperatingEnvironment rdf:type owl:Class ;
	rdfs:comment "The geographic environment in which operations occur or data is collected. " ;
	rdfs:subClassOf osdu:ReferenceData ;
	rdfs:subClassOf osdu:AbstractCommonResources ;
	rdfs:subClassOf osdu:AbstractReferenceType ;
.

###  https://w3id.org/osdu#OperationParameterPlan
osdu:OperationParameterPlan rdf:type owl:Class ;
	skos:prefLabel "Operation Parameter Plan" ;
	rdfs:comment "A series of operating parameters observed during the run " ;
	rdfs:subClassOf owl:Thing ;
	rdfs:subClassOf [
		a owl:Restriction ;
		owl:onProperty osdu:realizationStrategy ;
		owl:minCardinality "1"^^xsd:nonNegativeInteger ;
	] ;
	rdfs:subClassOf [
		a owl:Restriction ;
		owl:onProperty osdu:hasTorqueOnBottomGroup ;
		owl:minCardinality "1"^^xsd:nonNegativeInteger ;
	] ;
	rdfs:subClassOf [
		a owl:Restriction ;
		owl:onProperty osdu:hasRPMGroup ;
		owl:minCardinality "1"^^xsd:nonNegativeInteger ;
	] ;
	rdfs:subClassOf [
		a owl:Restriction ;
		owl:onProperty osdu:hasROPGroup ;
		owl:minCardinality "1"^^xsd:nonNegativeInteger ;
	] ;
	rdfs:subClassOf [
		a owl:Restriction ;
		owl:onProperty osdu:hasWOBGroup ;
		owl:minCardinality "1"^^xsd:nonNegativeInteger ;
	] ;
	rdfs:subClassOf [
		a owl:Restriction ;
		owl:onProperty osdu:hasFlowratePumpGroup ;
		owl:minCardinality "1"^^xsd:nonNegativeInteger ;
	] ;
.

###  https://w3id.org/osdu#OperationalPeriod
osdu:OperationalPeriod rdf:type owl:Class ;
	rdfs:comment "Defines the start and end year of the satellite mission " ;
	rdfs:subClassOf owl:Thing ;
.

###  https://w3id.org/osdu#OperationsReport
osdu:OperationsReport rdf:type owl:Class ;
	rdfs:comment "Information about a series of drilling activities. " ;
	rdfs:subClassOf osdu:MasterData ;
	rdfs:subClassOf osdu:AbstractCommonResources ;
	rdfs:subClassOf osdu:AbstractMaster ;
.

###  https://w3id.org/osdu#OrderingCriteriaType
osdu:OrderingCriteriaType rdf:type owl:Class ;
	rdfs:comment "Enumeration used to specify the order of  GeologicalUnitOccurrenceInterpretation " ;
	rdfs:subClassOf osdu:ReferenceData ;
	rdfs:subClassOf osdu:AbstractCommonResources ;
	rdfs:subClassOf osdu:AbstractReferenceType ;
.

###  https://w3id.org/osdu#Organisation
osdu:Organisation rdf:type owl:Class ;
	rdfs:comment "A legal or administrative body, institution, or company, or any of its divisions. " ;
	rdfs:subClassOf osdu:MasterData ;
	rdfs:subClassOf osdu:AbstractCommonResources ;
	rdfs:subClassOf osdu:AbstractMaster ;
	owl:sameAs foaf:Organization ;
.

###  https://w3id.org/osdu#OrganisationType
osdu:OrganisationType rdf:type owl:Class ;
	rdfs:comment "A general category of an enterprise,  government or other industrial group. " ;
	rdfs:subClassOf osdu:ReferenceData ;
	rdfs:subClassOf osdu:AbstractCommonResources ;
	rdfs:subClassOf osdu:AbstractReferenceType ;
.

###  https://w3id.org/osdu#PNG
osdu:PNG rdf:type owl:Class ;
	skos:prefLabel "File.Image.PNG" ;
	rdfs:comment "An image file in Portable Network Graphics (PNG) format, https://en.wikipedia.org/wiki/Portable_Network_Graphics. " ;
	rdfs:subClassOf osdu:Dataset ;
	rdfs:subClassOf osdu:AbstractCommonResources ;
	rdfs:subClassOf osdu:AbstractDataset ;
	rdfs:subClassOf osdu:AbstractFile ;
	rdfs:subClassOf foaf:Image ;
.

###  https://w3id.org/osdu#PPFGContextType
osdu:PPFGContextType rdf:type owl:Class ;
	rdfs:comment "Reflects the context of the PPFG acquired data (may be Pre-Drill/Post-Drill...) " ;
	rdfs:subClassOf osdu:ReferenceData ;
	rdfs:subClassOf osdu:AbstractCommonResources ;
	rdfs:subClassOf osdu:AbstractReferenceType ;
.

###  https://w3id.org/osdu#PPFGCurveFamily
osdu:PPFGCurveFamily rdf:type owl:Class ;
	rdfs:comment "The PPFG Curve Family reflects the 'Detailed' Geological Physical Quantity Measured - such Pore Pressure in Shale " ;
	rdfs:subClassOf osdu:ReferenceData ;
	rdfs:subClassOf osdu:AbstractCommonResources ;
	rdfs:subClassOf osdu:AbstractReferenceType ;
.

###  https://w3id.org/osdu#PPFGCurveLithoType
osdu:PPFGCurveLithoType rdf:type owl:Class ;
	rdfs:comment "Reflects the lithological unit a PPFG curve is representing " ;
	rdfs:subClassOf osdu:ReferenceData ;
	rdfs:subClassOf osdu:AbstractCommonResources ;
	rdfs:subClassOf osdu:AbstractReferenceType ;
.

###  https://w3id.org/osdu#PPFGCurveMainFamily
osdu:PPFGCurveMainFamily rdf:type owl:Class ;
	rdfs:comment "Reflects the Geological Physical Quantity measured within the PPFG Curve - can be 'Pore Pressure', 'FractureGradient', 'HorizontalStress'... " ;
	rdfs:subClassOf osdu:ReferenceData ;
	rdfs:subClassOf osdu:AbstractCommonResources ;
	rdfs:subClassOf osdu:AbstractReferenceType ;
.

###  https://w3id.org/osdu#PPFGCurveMnemonic
osdu:PPFGCurveMnemonic rdf:type owl:Class ;
	rdfs:comment "The mnemonic of the PPFG Curve is the value as received either from Raw Providers or from Internal Processing team. " ;
	rdfs:subClassOf osdu:ReferenceData ;
	rdfs:subClassOf osdu:AbstractCommonResources ;
	rdfs:subClassOf osdu:AbstractReferenceType ;
.

###  https://w3id.org/osdu#PPFGCurveProbability
osdu:PPFGCurveProbability rdf:type owl:Class ;
	rdfs:comment "The PPFG Curve Family reflects the level of probability associated to the Curve - defined by any company - could be 'Most Likely', 'Min Case',... " ;
	rdfs:subClassOf osdu:ReferenceData ;
	rdfs:subClassOf osdu:AbstractCommonResources ;
	rdfs:subClassOf osdu:AbstractReferenceType ;
.

###  https://w3id.org/osdu#PPFGCurveProcessingType
osdu:PPFGCurveProcessingType rdf:type owl:Class ;
	rdfs:comment "Describes the level of processing each PPFG curve went through " ;
	rdfs:subClassOf osdu:ReferenceData ;
	rdfs:subClassOf osdu:AbstractCommonResources ;
	rdfs:subClassOf osdu:AbstractReferenceType ;
.

###  https://w3id.org/osdu#PPFGCurveTransformModelType
osdu:PPFGCurveTransformModelType rdf:type owl:Class ;
	rdfs:comment "Name of the empirical calibrated model used for pressure calculation from a petrophysical curve (sonic or resistivity logs) - such as Eaton and  Bowers,...  " ;
	rdfs:subClassOf osdu:ReferenceData ;
	rdfs:subClassOf osdu:AbstractCommonResources ;
	rdfs:subClassOf osdu:AbstractReferenceType ;
.

###  https://w3id.org/osdu#PPFGDataset
osdu:PPFGDataset rdf:type owl:Class ;
	rdfs:comment "Pore Pressure and Fracture (Pressure) Gradient (PPFG) data describes the predicted (Pre-drill) and actual (Post-drill) depth-related variations in overburden stress, pore pressure, fracture pressure and minimum principal stress within a wellbore and conveys the range of uncertainty in these values given various plausible geological scenarios. PPFG predictions are fundamental inputs for well design and construction and estimates of pore and fracture pressure are typically provided to the well planning and execution teams. " ;
	rdfs:subClassOf osdu:WorkProductComponent ;
	rdfs:subClassOf osdu:AbstractCommonResources ;
	rdfs:subClassOf osdu:AbstractWPCGroupType ;
	rdfs:subClassOf osdu:AbstractWorkProductComponent ;
.

###  https://w3id.org/osdu#ParameterKey
osdu:ParameterKey rdf:type owl:Class ;
	skos:prefLabel "Parameter Key" ;
	rdfs:comment "Abstract class describing a key used to identify a parameter value. When multiple values are provided for a given parameter, provides a way to identify the parameter through its association with an object, a time index, an integer...  [Without inheritance, combined specializations.] Note: floating point numbers are not supported as key values; the numbers have to be formatted as strings for robust equality operations, which are necessary for keys. " ;
	rdfs:subClassOf owl:Thing ;
.

###  https://w3id.org/osdu#ParameterKind
osdu:ParameterKind rdf:type owl:Class ;
	rdfs:comment "ParameterKind describes the value type of the parameter. Known values are integer, double, string, timestamp, subActivity, dataObject. " ;
	rdfs:subClassOf osdu:ReferenceData ;
	rdfs:subClassOf osdu:AbstractCommonResources ;
	rdfs:subClassOf osdu:AbstractReferenceType ;
.

###  https://w3id.org/osdu#ParameterRole
osdu:ParameterRole rdf:type owl:Class ;
	rdfs:comment "Reference value type describing how an activity  parameter was used by an activity, such as input, output, control, constraint, agent, predecessor activity, successor activity. " ;
	rdfs:subClassOf osdu:ReferenceData ;
	rdfs:subClassOf osdu:AbstractCommonResources ;
	rdfs:subClassOf osdu:AbstractReferenceType ;
.

###  https://w3id.org/osdu#ParameterTemplate
osdu:ParameterTemplate rdf:type owl:Class ;
	skos:prefLabel "Parameter Template" ;
	rdfs:comment "Description of one parameter that participates in one type of activity. [Without inheritance, combined specializations.] " ;
	rdfs:subClassOf owl:Thing ;
	rdfs:subClassOf [
		a owl:Restriction ;
		owl:onProperty osdu:isInput ;
		owl:minCardinality "1"^^xsd:nonNegativeInteger ;
	] ;
	rdfs:subClassOf [
		a owl:Restriction ;
		owl:onProperty osdu:isOutput ;
		owl:minCardinality "1"^^xsd:nonNegativeInteger ;
	] ;
	rdfs:subClassOf [
		a owl:Restriction ;
		owl:onProperty osdu:title ;
		owl:minCardinality "1"^^xsd:nonNegativeInteger ;
	] ;
	rdfs:subClassOf [
		a owl:Restriction ;
		owl:onProperty osdu:maxOccurs ;
		owl:minCardinality "1"^^xsd:nonNegativeInteger ;
	] ;
	rdfs:subClassOf [
		a owl:Restriction ;
		owl:onProperty osdu:minOccurs ;
		owl:minCardinality "1"^^xsd:nonNegativeInteger ;
	] ;
.

###  https://w3id.org/osdu#ParameterType
osdu:ParameterType rdf:type owl:Class ;
	rdfs:comment "Used to describe the type of parameters. " ;
	rdfs:subClassOf osdu:ReferenceData ;
	rdfs:subClassOf osdu:AbstractCommonResources ;
	rdfs:subClassOf osdu:AbstractReferenceType ;
.

###  https://w3id.org/osdu#PerforationCentralizationMethodType
osdu:PerforationCentralizationMethodType rdf:type owl:Class ;
	rdfs:comment "The Perforating Gun Centralization Method Type used in a perforation interval. " ;
	rdfs:subClassOf osdu:ReferenceData ;
	rdfs:subClassOf osdu:AbstractCommonResources ;
	rdfs:subClassOf osdu:AbstractReferenceType ;
.

###  https://w3id.org/osdu#PerforationConveyedMethod
osdu:PerforationConveyedMethod rdf:type owl:Class ;
	rdfs:comment "Equipment type used to run perforation equipment downhole. " ;
	rdfs:subClassOf osdu:ReferenceData ;
	rdfs:subClassOf osdu:AbstractCommonResources ;
	rdfs:subClassOf osdu:AbstractReferenceType ;
.

###  https://w3id.org/osdu#PerforationGunCarrierCategory
osdu:PerforationGunCarrierCategory rdf:type owl:Class ;
	rdfs:comment "The Perforating Gun Category used in a perforation interval. " ;
	rdfs:subClassOf osdu:ReferenceData ;
	rdfs:subClassOf osdu:AbstractCommonResources ;
	rdfs:subClassOf osdu:AbstractReferenceType ;
.

###  https://w3id.org/osdu#PerforationGunCarrierModel
osdu:PerforationGunCarrierModel rdf:type owl:Class ;
	rdfs:comment "The Perforating Gun Carrier Model used in a perforation interval. " ;
	rdfs:subClassOf osdu:ReferenceData ;
	rdfs:subClassOf osdu:AbstractCommonResources ;
	rdfs:subClassOf osdu:AbstractReferenceType ;
.

###  https://w3id.org/osdu#PerforationGunCarrierType
osdu:PerforationGunCarrierType rdf:type owl:Class ;
	rdfs:comment "The Perforating Gun Carrier Type  used in a perforation interval. " ;
	rdfs:subClassOf osdu:ReferenceData ;
	rdfs:subClassOf osdu:AbstractCommonResources ;
	rdfs:subClassOf osdu:AbstractReferenceType ;
.

###  https://w3id.org/osdu#PerforationGunChargeShape
osdu:PerforationGunChargeShape rdf:type owl:Class ;
	rdfs:comment "The Perforating Gun Charge Shape used in a perforation interval. " ;
	rdfs:subClassOf osdu:ReferenceData ;
	rdfs:subClassOf osdu:AbstractCommonResources ;
	rdfs:subClassOf osdu:AbstractReferenceType ;
.

###  https://w3id.org/osdu#PerforationGunChargeSize
osdu:PerforationGunChargeSize rdf:type owl:Class ;
	rdfs:comment "The Perforating Gun Charge Size used in a perforation interval. The value is a number as string, always measured in grams (g = 0.001 kg). " ;
	rdfs:subClassOf osdu:ReferenceData ;
	rdfs:subClassOf osdu:AbstractCommonResources ;
	rdfs:subClassOf osdu:AbstractReferenceType ;
.

###  https://w3id.org/osdu#PerforationGunChargeType
osdu:PerforationGunChargeType rdf:type owl:Class ;
	rdfs:comment "The Perforating Gun Charge Type used in a perforation interval. " ;
	rdfs:subClassOf osdu:ReferenceData ;
	rdfs:subClassOf osdu:AbstractCommonResources ;
	rdfs:subClassOf osdu:AbstractReferenceType ;
.

###  https://w3id.org/osdu#PerforationGunFiringHeadType
osdu:PerforationGunFiringHeadType rdf:type owl:Class ;
	rdfs:comment "The Perforating Gun Firing Head Type used in a perforation interval. " ;
	rdfs:subClassOf osdu:ReferenceData ;
	rdfs:subClassOf osdu:AbstractCommonResources ;
	rdfs:subClassOf osdu:AbstractReferenceType ;
.

###  https://w3id.org/osdu#PerforationGunMetallurgyType
osdu:PerforationGunMetallurgyType rdf:type owl:Class ;
	rdfs:comment "The Perforating Gun Metallurgy Type used in a perforation interval. " ;
	rdfs:subClassOf osdu:ReferenceData ;
	rdfs:subClassOf osdu:AbstractCommonResources ;
	rdfs:subClassOf osdu:AbstractReferenceType ;
.

###  https://w3id.org/osdu#PerforationGunPhasingType
osdu:PerforationGunPhasingType rdf:type owl:Class ;
	rdfs:comment "The Perforating Gun Phasing (the angle between perforations), always measured in degrees of arc. " ;
	rdfs:subClassOf osdu:ReferenceData ;
	rdfs:subClassOf osdu:AbstractCommonResources ;
	rdfs:subClassOf osdu:AbstractReferenceType ;
.

###  https://w3id.org/osdu#PerforationInterval
osdu:PerforationInterval rdf:type owl:Class ;
	rdfs:comment "A Perforation Interval is associated to a Perforation Job. An interval is the Top & Base depth range that a specific Perforating Gun suite was fired in unison to produce Openings. An interval should be created for each Gun suite fired. A interval should also be created for a specific Tubing Punch firing also. " ;
	rdfs:subClassOf osdu:MasterData ;
	rdfs:subClassOf osdu:AbstractCommonResources ;
	rdfs:subClassOf osdu:AbstractMaster ;
.

###  https://w3id.org/osdu#PerforationIntervalReason
osdu:PerforationIntervalReason rdf:type owl:Class ;
	rdfs:comment "Reason why the perforation interval was constructed. " ;
	rdfs:subClassOf osdu:ReferenceData ;
	rdfs:subClassOf osdu:AbstractCommonResources ;
	rdfs:subClassOf osdu:AbstractReferenceType ;
.

###  https://w3id.org/osdu#PerforationIntervalType
osdu:PerforationIntervalType rdf:type owl:Class ;
	rdfs:comment "The method type used during the perforation of an interval. " ;
	rdfs:subClassOf osdu:ReferenceData ;
	rdfs:subClassOf osdu:AbstractCommonResources ;
	rdfs:subClassOf osdu:AbstractReferenceType ;
.

###  https://w3id.org/osdu#PerforationIntervalWLSize
osdu:PerforationIntervalWLSize rdf:type owl:Class ;
	rdfs:comment "Wireline Diameter as string value, always measured in inches  (=0.0254 m). " ;
	rdfs:subClassOf osdu:ReferenceData ;
	rdfs:subClassOf osdu:AbstractCommonResources ;
	rdfs:subClassOf osdu:AbstractReferenceType ;
.

###  https://w3id.org/osdu#PerforationJob
osdu:PerforationJob rdf:type owl:Class ;
	rdfs:comment "A Perforation Job describes an activity performed on a well for the purpose of firing perforation guns or puncher inside Casing, Liner or Tubing to create a flow path between the reservoir outside the pipe and the production annulus within the pipe. A Squeeze job is a remedial effort performed to create a temporary flow path to allow cement to be pumped outside the casing to repair the annular seal. Perf Intervals result in the creation of equivalent Wellbore Openings where they are managed as part of the Completion. A Squeeze job would not result in creation of Wellbore Openings as these are temporary to better seal that interval. " ;
	rdfs:subClassOf osdu:MasterData ;
	rdfs:subClassOf osdu:AbstractCommonResources ;
	rdfs:subClassOf osdu:AbstractMaster ;
.

###  https://w3id.org/osdu#PerforationPillType
osdu:PerforationPillType rdf:type owl:Class ;
	rdfs:comment "Liquid pill pumped to optimise perforation job, e.g., debris prevention. " ;
	rdfs:subClassOf osdu:ReferenceData ;
	rdfs:subClassOf osdu:AbstractCommonResources ;
	rdfs:subClassOf osdu:AbstractReferenceType ;
.

###  https://w3id.org/osdu#PermeabilityMeasurementType
osdu:PermeabilityMeasurementType rdf:type owl:Class ;
	rdfs:comment "The kind of permeability measurement applied in, e.g., routine core analysis. " ;
	rdfs:subClassOf osdu:ReferenceData ;
	rdfs:subClassOf osdu:AbstractCommonResources ;
	rdfs:subClassOf osdu:AbstractReferenceType ;
.

###  https://w3id.org/osdu#PersistedCollection
osdu:PersistedCollection rdf:type owl:Class ;
	rdfs:comment "A persisted collection of objects ingested in the data platform. The collection can aggregate objects of different nature, including master data, work-product-components and reference data. A PersistedCollection can also contain other PersistedCollection(s). " ;
	rdfs:subClassOf osdu:WorkProductComponent ;
	rdfs:subClassOf osdu:AbstractCommonResources ;
	rdfs:subClassOf osdu:AbstractWPCGroupType ;
	rdfs:subClassOf osdu:AbstractWorkProductComponent ;
.

###  https://w3id.org/osdu#Personnel
osdu:Personnel rdf:type owl:Class ;
	rdfs:comment "List of key individuals supporting a Project." ;
	rdfs:subClassOf foaf:Person ;
	rdfs:subClassOf [
		a owl:Restriction ;
		owl:onProperty osdu:organizationID ;
		owl:minCardinality "1"^^xsd:nonNegativeInteger ;
	] ;
	rdfs:subClassOf [
		a owl:Restriction ;
		owl:onProperty osdu:headCount ;
		owl:minCardinality "1"^^xsd:nonNegativeInteger ;
	] ;
.

###  https://w3id.org/osdu#PersonnelOrganisationRole
osdu:PersonnelOrganisationRole rdf:type owl:Class ;
	rdfs:comment "Type of Organisational Role that a person can perform " ;
	rdfs:subClassOf osdu:ReferenceData ;
	rdfs:subClassOf osdu:AbstractCommonResources ;
	rdfs:subClassOf osdu:AbstractReferenceType ;
.

###  https://w3id.org/osdu#PersonnelServiceType
osdu:PersonnelServiceType rdf:type owl:Class ;
	rdfs:comment "Type of drilling service that a person can perform " ;
	rdfs:subClassOf osdu:ReferenceData ;
	rdfs:subClassOf osdu:AbstractCommonResources ;
	rdfs:subClassOf osdu:AbstractReferenceType ;
.

###  https://w3id.org/osdu#PetroleumSystemElementType
osdu:PetroleumSystemElementType rdf:type owl:Class ;
	rdfs:comment "Petroleum system risk element such as Reservoir, Source, Seal, Structure (geometry). " ;
	rdfs:subClassOf osdu:ReferenceData ;
	rdfs:subClassOf osdu:AbstractCommonResources ;
	rdfs:subClassOf osdu:AbstractReferenceType ;
.

###  https://w3id.org/osdu#Phase
osdu:Phase rdf:type owl:Class ;
	rdfs:comment "Description of an individual phase that compose the WellActivityProgram. A phase describes the key milestones and is usually based on the major sections of the well or non-well-related work. (Such as Acces Well, Suspend , Wellhead Removal ...) " ;
	rdfs:subClassOf owl:Thing ;
	rdfs:subClassOf [
		a owl:Restriction ;
		owl:onProperty osdu:typeID ;
		owl:minCardinality "1"^^xsd:nonNegativeInteger ;
	] ;
	rdfs:subClassOf [
		a owl:Restriction ;
		owl:onProperty osdu:wellActivityPlanID ;
		owl:minCardinality "1"^^xsd:nonNegativeInteger ;
	] ;
	rdfs:subClassOf [
		a owl:Restriction ;
		owl:onProperty osdu:bhaRunID ;
		owl:minCardinality "1"^^xsd:nonNegativeInteger ;
	] ;
.

###  https://w3id.org/osdu#PillarShapeType
osdu:PillarShapeType rdf:type owl:Class ;
	rdfs:comment "An enumeration of the pillar shape type based on the RESQML model, i.e., vertical, straight, curved. " ;
	rdfs:subClassOf osdu:ReferenceData ;
	rdfs:subClassOf osdu:AbstractCommonResources ;
	rdfs:subClassOf osdu:AbstractReferenceType ;
.

###  https://w3id.org/osdu#PlannedCementJob
osdu:PlannedCementJob rdf:type owl:Class ;
	rdfs:comment "A single cement job description for the purpose of planning. " ;
	rdfs:subClassOf osdu:MasterData ;
	rdfs:subClassOf osdu:AbstractCommonResources ;
	rdfs:subClassOf osdu:AbstractMaster ;
.

###  https://w3id.org/osdu#PlannedLithology
osdu:PlannedLithology rdf:type owl:Class ;
	rdfs:comment "Describes the sequence of expected lithologic intervals for the Wellbore " ;
	rdfs:subClassOf osdu:WorkProductComponent ;
	rdfs:subClassOf osdu:AbstractCommonResources ;
	rdfs:subClassOf osdu:AbstractWPCGroupType ;
	rdfs:subClassOf osdu:AbstractWorkProductComponent ;
.

###  https://w3id.org/osdu#Play
osdu:Play rdf:type owl:Class ;
	rdfs:comment "A named area that likely contains a combination of certain geological factors making it prospective for mineral exploration. It is often considered to be a set of prospects with a common set of characteristics. " ;
	rdfs:subClassOf osdu:MasterData ;
	rdfs:subClassOf osdu:AbstractCommonResources ;
	rdfs:subClassOf osdu:AbstractMaster ;
.

###  https://w3id.org/osdu#PlayType
osdu:PlayType rdf:type owl:Class ;
	rdfs:comment "Play Type [Well Play Type] is the focus or area conducive to hydrocarbon discovery and includes the related activities for the development and production of the reservoir. " ;
	rdfs:subClassOf osdu:ReferenceData ;
	rdfs:subClassOf osdu:AbstractCommonResources ;
	rdfs:subClassOf osdu:AbstractReferenceType ;
.

###  https://w3id.org/osdu#PlugType
osdu:PlugType rdf:type owl:Class ;
	rdfs:comment "Purpose of Cement Plug such as wellbore abandonment, side-tracking or kick-off. " ;
	rdfs:subClassOf osdu:ReferenceData ;
	rdfs:subClassOf osdu:AbstractCommonResources ;
	rdfs:subClassOf osdu:AbstractReferenceType ;
.

###  https://w3id.org/osdu#Point
osdu:Point rdf:type owl:Class ;
	rdfs:comment "The definition of the point " ;
	rdfs:subClassOf owl:Thing ;
	rdfs:subClassOf [
		a owl:Restriction ;
		owl:onProperty osdu:observationMeasuredDepth ;
		owl:minCardinality "1"^^xsd:nonNegativeInteger ;
	] ;
	rdfs:subClassOf [
		a owl:Restriction ;
		owl:onProperty osdu:valueUnitID ;
		owl:minCardinality "1"^^xsd:nonNegativeInteger ;
	] ;
	rdfs:subClassOf [
		a owl:Restriction ;
		owl:onProperty osdu:hasPointsSources ;
		owl:minCardinality "1"^^xsd:nonNegativeInteger ;
	] ;
.

###  https://w3id.org/osdu#PointsSource
osdu:PointsSource rdf:type owl:Class ;
	skos:prefLabel "Points Source" ;
	rdfs:comment "The definition of the points used as a source for each individual critical point, resulting from parameters set or observed during a BHA run " ;
	rdfs:subClassOf owl:Thing ;
	rdfs:subClassOf [
		a owl:Restriction ;
		owl:onProperty osdu:name ;
		owl:minCardinality "1"^^xsd:nonNegativeInteger ;
	] ;
	rdfs:subClassOf [
		a owl:Restriction ;
		owl:onproperty osdu:hasPoint;
		owl:minCardinality "1"^^xsd:nonNegativeInteger ;
	] ;
	rdfs:subClassOf [
		a owl:Restriction ;
		owl:onProperty osdu:valueUnitID ;
		owl:minCardinality "1"^^xsd:nonNegativeInteger ;
	] ;
.

###  https://w3id.org/osdu#PorosityMeasurementType
osdu:PorosityMeasurementType rdf:type owl:Class ;
	rdfs:comment "The kind of porosity measurement applied in, e.g., routine core analysis. " ;
	rdfs:subClassOf osdu:ReferenceData ;
	rdfs:subClassOf osdu:AbstractCommonResources ;
	rdfs:subClassOf osdu:AbstractReferenceType ;
.

###  https://w3id.org/osdu#Precision
osdu:Precision rdf:type owl:Class ;
	rdfs:comment "Sample data format in terms of sample value precision 8bit Integer, 16bit Floating Point etc. " ;
	rdfs:subClassOf owl:Thing ;
.

###  https://w3id.org/osdu#PreferredUsage
osdu:PreferredUsage rdf:type owl:Class ;
	skos:prefLabel "Preferred Usage" ;
	rdfs:comment "Scope and extent information." ;
	rdfs:subClassOf owl:Thing ;
.

###  https://w3id.org/osdu#PressureCriteria
osdu:PressureCriteria rdf:type owl:Class ;
	skos:prefLabel "Pressure Criteria" ;
	rdfs:comment "Generic description of an individual pressure criterion for a single step of the test " ;
	rdfs:subClassOf owl:Thing ;
.

###  https://w3id.org/osdu#PressureMeasurementType
osdu:PressureMeasurementType rdf:type owl:Class ;
	rdfs:comment "The enumeration for PressureMeasurement types like Ambient or Overburden. " ;
	rdfs:subClassOf osdu:ReferenceData ;
	rdfs:subClassOf osdu:AbstractCommonResources ;
	rdfs:subClassOf osdu:AbstractReferenceType ;
.

###  https://w3id.org/osdu#ProcessedInSAR
osdu:ProcessedInSAR rdf:type owl:Class ;
	rdfs:comment "Interferometric Synthetic Aperture Radar (InSAR) is a representation of surface or ground deformation from satellite radar image data over time " ;
	rdfs:subClassOf osdu:WorkProductComponent ;
	rdfs:subClassOf osdu:AbstractCommonResources ;
	rdfs:subClassOf osdu:AbstractWPCGroupType ;
	rdfs:subClassOf osdu:AbstractWorkProductComponent ;
.

###  https://w3id.org/osdu#ProcessingParameterType
osdu:ProcessingParameterType rdf:type owl:Class ;
	rdfs:comment "A variable that can be changed independently and often arbitrarily between calculations but which remains constant during any calculation. (SEG) " ;
	rdfs:subClassOf osdu:ReferenceData ;
	rdfs:subClassOf osdu:AbstractCommonResources ;
	rdfs:subClassOf osdu:AbstractReferenceType ;
.

###  https://w3id.org/osdu#ProcessingParameters
osdu:ProcessingParameters rdf:type owl:Class ;
	rdfs:comment "Processing Parameters to simply capture process history until full provenance model can be implemented. " ;
	rdfs:subClassOf owl:Thing ;
.

###  https://w3id.org/osdu#Project
osdu:Project rdf:type owl:Class ;
	rdfs:subClassOf owl:Thing ;
.

###  https://w3id.org/osdu#ProjectRole
osdu:ProjectRole rdf:type owl:Class ;
	rdfs:comment "The role of an individual supporting a Project, such as Project Manager, Party Chief, Client Representative, Senior Observer. " ;
	rdfs:subClassOf osdu:ReferenceData ;
	rdfs:subClassOf osdu:AbstractCommonResources ;
	rdfs:subClassOf osdu:AbstractReferenceType ;
.

###  https://w3id.org/osdu#ProjectSpecifications
osdu:ProjectSpecifications rdf:type owl:Class ;
	rdfs:comment "General parameters defining the configuration of the Project.  In the case of a seismic acquisition project it is like receiver interval, source depth, source type.  In the case of a processing project, it is like replacement velocity, reference datum above mean sea level. " ;
	rdfs:subClassOf owl:Thing ;
.

###  https://w3id.org/osdu#ProjectStateType
osdu:ProjectStateType rdf:type owl:Class ;
	rdfs:comment "The Project life cycle state from planning to completion. " ;
	rdfs:subClassOf osdu:ReferenceData ;
	rdfs:subClassOf osdu:AbstractCommonResources ;
	rdfs:subClassOf osdu:AbstractReferenceType ;
.

###  https://w3id.org/osdu#ProjectStates
osdu:ProjectStates rdf:type owl:Class ;
	rdfs:comment "The history of life cycle states that the Project has been through.. " ;
	rdfs:subClassOf owl:Thing ;
.

###  https://w3id.org/osdu#Projection
osdu:Projection rdf:type owl:Class ;
	rdfs:comment "The projection operation of a ProjectedCRS. Only populated for CoordinateReferenceSystemType==ProjectedCRS. " ;
	rdfs:subClassOf owl:Thing ;
.

###  https://w3id.org/osdu#PropertyFieldRepresentationType
osdu:PropertyFieldRepresentationType rdf:type owl:Class ;
	rdfs:comment "The type of topology used to represent the discrete velocity observations, such as Grid or Mesh. " ;
	rdfs:subClassOf osdu:ReferenceData ;
	rdfs:subClassOf osdu:AbstractCommonResources ;
	rdfs:subClassOf osdu:AbstractReferenceType ;
.

###  https://w3id.org/osdu#PropertyNameType
osdu:PropertyNameType rdf:type owl:Class ;
	rdfs:comment "Name of a measured or observed property, such as Vp, Vs, epsilon, delta, eta. " ;
	rdfs:subClassOf osdu:ReferenceData ;
	rdfs:subClassOf osdu:AbstractCommonResources ;
	rdfs:subClassOf osdu:AbstractReferenceType ;
.

###  https://w3id.org/osdu#PropertyType
osdu:PropertyType rdf:type owl:Class ;
	rdfs:comment "PropertyType is part of Energistics PWLS 3, which defines a detailed hierarchy of properties linked to the Energistics UnitQuantity/UnitOfMeasure. " ;
	rdfs:subClassOf osdu:ReferenceData ;
	rdfs:subClassOf osdu:AbstractCommonResources ;
	rdfs:subClassOf osdu:AbstractReferenceType ;
.

###  https://w3id.org/osdu#Prospect
osdu:Prospect rdf:type owl:Class ;
	rdfs:comment "A named area or location, likely containing commercial deposits of a mineral, that is a candidate for extraction.  This normally means a candidate drilling location.. " ;
	rdfs:subClassOf osdu:MasterData ;
	rdfs:subClassOf osdu:AbstractCommonResources ;
	rdfs:subClassOf osdu:AbstractMaster ;
.

###  https://w3id.org/osdu#ProspectType
osdu:ProspectType rdf:type owl:Class ;
	rdfs:comment "A kind of potential trap that must be evaluated by drilling to determine whether it contains commercial quantities of petroleum. " ;
	rdfs:subClassOf osdu:ReferenceData ;
	rdfs:subClassOf osdu:AbstractCommonResources ;
	rdfs:subClassOf osdu:AbstractReferenceType ;
.

###  https://w3id.org/osdu#PumpOpType
osdu:PumpOpType rdf:type owl:Class ;
	rdfs:comment "Type of pump operations performed in the operations report " ;
	rdfs:subClassOf osdu:ReferenceData ;
	rdfs:subClassOf osdu:AbstractCommonResources ;
	rdfs:subClassOf osdu:AbstractReferenceType ;
.

###  https://w3id.org/osdu#PumpOperations
osdu:PumpOperations rdf:type owl:Class ;
	skos:prefLabel "Pump Operations" ;
	rdfs:comment "Information related to pump operations on a drilling/operations report " ;
	rdfs:subClassOf owl:Thing ;
	rdfs:subClassOf [
		a owl:Restriction ;
		owl:onProperty osdu:dateTime ;
		owl:minCardinality "1"^^xsd:nonNegativeInteger ;
	] ;
.

###  https://w3id.org/osdu#QualitativeSpatialAccuracyType
osdu:QualitativeSpatialAccuracyType rdf:type owl:Class ;
	rdfs:comment "The level of confidence that the spatial feature is correctly located. " ;
	rdfs:subClassOf osdu:ReferenceData ;
	rdfs:subClassOf osdu:AbstractCommonResources ;
	rdfs:subClassOf osdu:AbstractReferenceType ;
.

###  https://w3id.org/osdu#QualityDataRule
osdu:QualityDataRule rdf:type owl:Class ;
	rdfs:comment "Generic reference object quality rule " ;
	rdfs:subClassOf osdu:ReferenceData ;
	rdfs:subClassOf osdu:AbstractCommonResources ;
	rdfs:subClassOf osdu:AbstractReferenceType ;
.

###  https://w3id.org/osdu#QualityDataRuleSet
osdu:QualityDataRuleSet rdf:type owl:Class ;
	rdfs:comment "A set of data quality rules to assess a specific aspect in the trustworthiness of data. " ;
	rdfs:subClassOf osdu:ReferenceData ;
	rdfs:subClassOf osdu:AbstractCommonResources ;
	rdfs:subClassOf osdu:AbstractReferenceType ;
.

###  https://w3id.org/osdu#QuantitativeAccuracyBand
osdu:QuantitativeAccuracyBand rdf:type owl:Class ;
	rdfs:comment "A number to express the proximity of a measurement to the true value. " ;
	rdfs:subClassOf osdu:ReferenceData ;
	rdfs:subClassOf osdu:AbstractCommonResources ;
	rdfs:subClassOf osdu:AbstractReferenceType ;
.

###  https://w3id.org/osdu#RCAMeasurement
osdu:RCAMeasurement rdf:type owl:Class ;
	rdfs:comment "A Routine Core Analysis Measurement. " ;
	rdfs:subClassOf owl:Thing ;
.

###  https://w3id.org/osdu#ROPGroup
osdu:ROPGroup rdf:type owl:Class ;
	skos:prefLabel "R.O.P. Group" ;
	rdfs:comment "A group of parameters that refer to ROP (rate of penetration) " ;
	rdfs:subClassOf owl:Thing ;
	rdfs:subClassOf [
		a owl:Restriction ;
		owl:onProperty osdu:maximumROP ;
		owl:minCardinality "1"^^xsd:nonNegativeInteger ;
	] ;
	rdfs:subClassOf [
		a owl:Restriction ;
		owl:onProperty osdu:minimumROP ;
		owl:minCardinality "1"^^xsd:nonNegativeInteger ;
	] ;
.

###  https://w3id.org/osdu#ROPStatistics
osdu:ROPStatistics rdf:type owl:Class ;
	skos:prefLabel "ROP Statistics" ;
	rdfs:comment "Individual Statistics that define the rate of penetration of an activity " ;
	rdfs:subClassOf owl:Thing ;
	rdfs:subClassOf [
		a owl:Restriction ;
		owl:onProperty osdu:statisticRecord ;
		owl:minCardinality "1"^^xsd:nonNegativeInteger ;
	] ;
	rdfs:subClassOf [
		a owl:Restriction ;
		owl:onProperty osdu:probabilityTypeID ;
		owl:minCardinality "1"^^xsd:nonNegativeInteger ;
	] ;
.

###  https://w3id.org/osdu#RPMGroup
osdu:RPMGroup rdf:type owl:Class ;
	skos:prefLabel "R.P.M. Group" ;
	rdfs:comment "A group of parameters that refer to RPM (rotations per minute) " ;
	rdfs:subClassOf owl:Thing ;
.

###  https://w3id.org/osdu#ReasonTripType
osdu:ReasonTripType rdf:type owl:Class ;
	rdfs:comment "BHA trip reason such as Change Bottomhole Assembly, Downhole Motor Failure, Drill Stem Failure " ;
	rdfs:subClassOf osdu:ReferenceData ;
	rdfs:subClassOf osdu:AbstractCommonResources ;
	rdfs:subClassOf osdu:AbstractReferenceType ;
.

###  https://w3id.org/osdu#RecommendedFlowratePump
osdu:RecommendedFlowratePump rdf:type owl:Class ;
	skos:prefLabel "Flowrate Pump Recommended" ;
	rdfs:comment "The recommended flowrate for the run " ;
	rdfs:subClassOf owl:Thing ;
	rdfs:subClassOf [
		a owl:Restriction ;
		owl:onproperty osdu:hasPoint;
		owl:minCardinality "1"^^xsd:nonNegativeInteger ;
	] ;
.

###  https://w3id.org/osdu#RecommendedROP
osdu:RecommendedROP rdf:type owl:Class ;
	skos:prefLabel "Recommended R.O.P." ;
	rdfs:comment "The recommended rate of penetration for the run " ;
	rdfs:subClassOf owl:Thing ;
	rdfs:subClassOf [
		a owl:Restriction ;
		owl:onproperty osdu:hasPoint;
		owl:minCardinality "1"^^xsd:nonNegativeInteger ;
	] ;
.

###  https://w3id.org/osdu#RecommendedRPM
osdu:RecommendedRPM rdf:type owl:Class ;
	skos:prefLabel "Recommended RPM" ;
	rdfs:comment "The recommended rotary speed for the run " ;
	rdfs:subClassOf owl:Thing ;
	rdfs:subClassOf [
		a owl:Restriction ;
		owl:onproperty osdu:hasPoint;
		owl:minCardinality "1"^^xsd:nonNegativeInteger ;
	] ;
.

###  https://w3id.org/osdu#RecommendedWOB
osdu:RecommendedWOB rdf:type owl:Class ;
	skos:prefLabel "Recommended W.O.B." ;
	rdfs:comment "The recommended weight on bit for this run " ;
	rdfs:subClassOf owl:Thing ;
	rdfs:subClassOf [
		a owl:Restriction ;
		owl:onproperty osdu:hasPoint;
		owl:minCardinality "1"^^xsd:nonNegativeInteger ;
	] ;
.

###  https://w3id.org/osdu#ReferenceData
osdu:ReferenceData rdf:type owl:Class ;
	rdfs:subClassOf osdu:System ;
.

###  https://w3id.org/osdu#ReferenceLevel
osdu:ReferenceLevel rdf:type owl:Class ;
	rdfs:comment "A reference level or horizontal reference surface, which can be re-used by many other entities. The area of use is indicated by data.SpatialLocation - as a polygon or as a point if used in context of a Well or Wellbore. " ;
	rdfs:subClassOf osdu:MasterData ;
	rdfs:subClassOf osdu:AbstractCommonResources ;
	rdfs:subClassOf osdu:AbstractMaster ;
	rdfs:subClassOf osdu:AbstractReferenceLevel ;
.

###  https://w3id.org/osdu#Remark
osdu:Remark rdf:type owl:Class ;
	rdfs:comment "An array containing narrative remarks pertaining to a rock sample analysis. " ;
	rdfs:subClassOf owl:Thing ;
.

###  https://w3id.org/osdu#RepresentationRole
osdu:RepresentationRole rdf:type owl:Class ;
	rdfs:comment "A specification of the role, which the representation in context plays. For example: 'Map', 'Pick', 'FaultCenterLine', 'InnerRing', 'OuterRing'. " ;
	rdfs:subClassOf osdu:ReferenceData ;
	rdfs:subClassOf osdu:AbstractCommonResources ;
	rdfs:subClassOf osdu:AbstractReferenceType ;
.

###  https://w3id.org/osdu#RepresentationType
osdu:RepresentationType rdf:type owl:Class ;
	rdfs:comment "The type of a representation, such as, for example, 'PointSet', 'Polyline', 'PolylineSet', 'TriangulatedSurface', etc. " ;
	rdfs:subClassOf osdu:ReferenceData ;
	rdfs:subClassOf osdu:AbstractCommonResources ;
	rdfs:subClassOf osdu:AbstractReferenceType ;
.

###  https://w3id.org/osdu#RepresentativeDipDirection
osdu:RepresentativeDipDirection rdf:type owl:Class ;
	rdfs:comment "Indicates the representative azimuth value of the fault plane " ;
	rdfs:subClassOf owl:Thing ;
.

###  https://w3id.org/osdu#ReservoirCompartmentInterpretation
osdu:ReservoirCompartmentInterpretation rdf:type owl:Class ;
	rdfs:comment "A portion of a reservoir rock which is differentiated laterally from other portions of the same reservoir stratum. This differentiation could be due to being in a different fault block or a different channel or other stratigraphic or structural aspect. A reservoir compartment may or may not be in contact with other reservoir compartments. " ;
	rdfs:subClassOf osdu:WorkProductComponent ;
	rdfs:subClassOf osdu:AbstractCommonResources ;
	rdfs:subClassOf osdu:AbstractWPCGroupType ;
	rdfs:subClassOf osdu:AbstractWorkProductComponent ;
	rdfs:subClassOf osdu:AbstractInterpretation ;
.

###  https://w3id.org/osdu#ReservoirCompartmentUnit
osdu:ReservoirCompartmentUnit rdf:type owl:Class ;
	rdfs:comment "A subdivision of a reservoir compartment generally corresponding to one geologic unit. " ;
	rdfs:subClassOf owl:Thing ;
.

###  https://w3id.org/osdu#ResourceCurationStatus
osdu:ResourceCurationStatus rdf:type owl:Class ;
	rdfs:comment "Used to describe the resource curation statuses. " ;
	rdfs:subClassOf osdu:ReferenceData ;
	rdfs:subClassOf osdu:AbstractCommonResources ;
	rdfs:subClassOf osdu:AbstractReferenceType ;
.

###  https://w3id.org/osdu#ResourceLifecycleStatus
osdu:ResourceLifecycleStatus rdf:type owl:Class ;
	rdfs:comment "Used to describe the resource lifecycle statuses, where the resource is in the process to ingest and release it. " ;
	rdfs:subClassOf osdu:ReferenceData ;
	rdfs:subClassOf osdu:AbstractCommonResources ;
	rdfs:subClassOf osdu:AbstractReferenceType ;
.

###  https://w3id.org/osdu#ResourceSecurityClassification
osdu:ResourceSecurityClassification rdf:type owl:Class ;
	rdfs:comment "Used to describe the resource security classifications. " ;
	rdfs:subClassOf osdu:ReferenceData ;
	rdfs:subClassOf osdu:AbstractCommonResources ;
	rdfs:subClassOf osdu:AbstractReferenceType ;
.

###  https://w3id.org/osdu#RestrictedResources
osdu:RestrictedResources rdf:type owl:Class ;
	rdfs:subClassOf owl:Thing ;
.

###  https://w3id.org/osdu#Rheometer
osdu:Rheometer rdf:type owl:Class ;
	rdfs:comment "Rheometer values observed " ;
	rdfs:subClassOf owl:Thing ;
	rdfs:subClassOf [
		a owl:Restriction ;
		owl:onProperty osdu:temperatureRheometer ;
		owl:minCardinality "1"^^xsd:nonNegativeInteger ;
	] ;
	rdfs:subClassOf [
		a owl:Restriction ;
		owl:onProperty osdu:pressureRheometer ;
		owl:minCardinality "1"^^xsd:nonNegativeInteger ;
	] ;
.

###  https://w3id.org/osdu#RheometerViscosity
osdu:RheometerViscosity rdf:type owl:Class ;
	skos:prefLabel "Rheometer Viscosity" ;
	rdfs:comment "Viscosity values observed " ;
	rdfs:subClassOf owl:Thing ;
	rdfs:subClassOf [
		a owl:Restriction ;
		owl:onProperty osdu:speed ;
		owl:minCardinality "1"^^xsd:nonNegativeInteger ;
	] ;
	rdfs:subClassOf [
		a owl:Restriction ;
		owl:onProperty osdu:viscosity ;
		owl:minCardinality "1"^^xsd:nonNegativeInteger ;
	] ;
.

###  https://w3id.org/osdu#Rig
osdu:Rig rdf:type owl:Class ;
	rdfs:comment "Definition of a drilling rig. " ;
	rdfs:subClassOf osdu:MasterData ;
	rdfs:subClassOf osdu:AbstractCommonResources ;
	rdfs:subClassOf osdu:AbstractMaster ;
	rdfs:subClassOf osdu:AbstractFacility ;
.

###  https://w3id.org/osdu#RigType
osdu:RigType rdf:type owl:Class ;
	rdfs:comment "Types of Drilling Rigs. Possible reference values: Barge, Coiled Tubing, Floater, Jackup, Land, Platform, Semi_Submersible, Unknown " ;
	rdfs:subClassOf osdu:ReferenceData ;
	rdfs:subClassOf osdu:AbstractCommonResources ;
	rdfs:subClassOf osdu:AbstractReferenceType ;
.

###  https://w3id.org/osdu#RigUtilization
osdu:RigUtilization rdf:type owl:Class ;
	rdfs:comment "The utilization of a rig during the drilling phase of a section " ;
	rdfs:subClassOf osdu:MasterData ;
	rdfs:subClassOf osdu:AbstractCommonResources ;
	rdfs:subClassOf osdu:AbstractMaster ;
	rdfs:subClassOf osdu:AbstractProject ;
.

###  https://w3id.org/osdu#Risk
osdu:Risk rdf:type owl:Class ;
	rdfs:comment "Possible risk potentially encountered during the run of a drilling program or a single string run. " ;
	rdfs:subClassOf osdu:MasterData ;
	rdfs:subClassOf osdu:AbstractCommonResources ;
	rdfs:subClassOf osdu:AbstractMaster ;
.

###  https://w3id.org/osdu#RiskCategory
osdu:RiskCategory rdf:type owl:Class ;
	rdfs:comment "Proposed reference values: hydraulics, mechanical, time related, wellbore stability, directional drilling, bit, equipment failure, completion, casing, other, HSE, unknown " ;
	rdfs:subClassOf osdu:ReferenceData ;
	rdfs:subClassOf osdu:AbstractCommonResources ;
	rdfs:subClassOf osdu:AbstractReferenceType ;
.

###  https://w3id.org/osdu#RiskConsequenceCategory
osdu:RiskConsequenceCategory rdf:type owl:Class ;
	rdfs:comment "Consequence category of the risk for possible effects on Asset, Business & Reputation, Environment, Health & Safety… " ;
	rdfs:subClassOf osdu:ReferenceData ;
	rdfs:subClassOf osdu:AbstractCommonResources ;
	rdfs:subClassOf osdu:AbstractReferenceType ;
.

###  https://w3id.org/osdu#RiskConsequenceSubCategory
osdu:RiskConsequenceSubCategory rdf:type owl:Class ;
	rdfs:comment "References the consequence sub-category of the risk. Possible effects arising were a risk event to occur. " ;
	rdfs:subClassOf osdu:ReferenceData ;
	rdfs:subClassOf osdu:AbstractCommonResources ;
	rdfs:subClassOf osdu:AbstractReferenceType ;
.

###  https://w3id.org/osdu#RiskDiscipline
osdu:RiskDiscipline rdf:type owl:Class ;
	rdfs:comment "Organisational unit accountable for maintaining appropriate focus on a risk and its management and for appropriate consultation with stakeholders " ;
	rdfs:subClassOf osdu:ReferenceData ;
	rdfs:subClassOf osdu:AbstractCommonResources ;
	rdfs:subClassOf osdu:AbstractReferenceType ;
.

###  https://w3id.org/osdu#RiskHierarchyLevel
osdu:RiskHierarchyLevel rdf:type owl:Class ;
	rdfs:comment "Area within organisation where risks will be most applicable, includes Well-level, Field-level, Region-level, Global-level " ;
	rdfs:subClassOf osdu:ReferenceData ;
	rdfs:subClassOf osdu:AbstractCommonResources ;
	rdfs:subClassOf osdu:AbstractReferenceType ;
.

###  https://w3id.org/osdu#RiskResponse
osdu:RiskResponse rdf:type owl:Class ;
	skos:prefLabel "Risk Response" ;
	rdfs:comment "Describe a set of action to prevent for a risk or to mitigate its consequences " ;
	rdfs:subClassOf owl:Thing ;
	rdfs:subClassOf [
		a owl:Restriction ;
		owl:onProperty osdu:name ;
		owl:minCardinality "1"^^xsd:nonNegativeInteger ;
	] ;
	rdfs:subClassOf [
		a owl:Restriction ;
		owl:onProperty osdu:description ;
		owl:minCardinality "1"^^xsd:nonNegativeInteger ;
	] ;
	rdfs:subClassOf [
		a owl:Restriction ;
		owl:onProperty osdu:status ;
		owl:minCardinality "1"^^xsd:nonNegativeInteger ;
	] ;
	rdfs:subClassOf [
		a owl:Restriction ;
		owl:onProperty osdu:responsible ;
		owl:minCardinality "1"^^xsd:nonNegativeInteger ;
	] ;
.

###  https://w3id.org/osdu#RiskResponseStatus
osdu:RiskResponseStatus rdf:type owl:Class ;
	rdfs:comment "Describes the status of the action such as In progress, done, cancelled… " ;
	rdfs:subClassOf osdu:ReferenceData ;
	rdfs:subClassOf osdu:AbstractCommonResources ;
	rdfs:subClassOf osdu:AbstractReferenceType ;
.

###  https://w3id.org/osdu#RiskSubCategory
osdu:RiskSubCategory rdf:type owl:Class ;
	rdfs:comment "The reference values for risk sub-categories following the WITSML standard. " ;
	rdfs:subClassOf osdu:ReferenceData ;
	rdfs:subClassOf osdu:AbstractCommonResources ;
	rdfs:subClassOf osdu:AbstractReferenceType ;
.

###  https://w3id.org/osdu#RiskType
osdu:RiskType rdf:type owl:Class ;
	rdfs:comment "Proposed reference values: risk, event, near miss, best practice, lessons learned, other, unknown " ;
	rdfs:subClassOf osdu:ReferenceData ;
	rdfs:subClassOf osdu:AbstractCommonResources ;
	rdfs:subClassOf osdu:AbstractReferenceType ;
.

###  https://w3id.org/osdu#RockFluidOrganizationInterpretation
osdu:RockFluidOrganizationInterpretation rdf:type owl:Class ;
	rdfs:comment "A collection of RockFluid unit interpretations which are part of a same organization i.e. which are inter related. " ;
	rdfs:subClassOf osdu:WorkProductComponent ;
	rdfs:subClassOf osdu:AbstractCommonResources ;
	rdfs:subClassOf osdu:AbstractWPCGroupType ;
	rdfs:subClassOf osdu:AbstractWorkProductComponent ;
	rdfs:subClassOf osdu:AbstractInterpretation ;
.

###  https://w3id.org/osdu#RockFluidUnitInterpretation
osdu:RockFluidUnitInterpretation rdf:type owl:Class ;
	rdfs:comment "A type of rock fluid feature-interpretation , this class identifies a rock fluid feature by its phase. " ;
	rdfs:subClassOf osdu:WorkProductComponent ;
	rdfs:subClassOf osdu:AbstractCommonResources ;
	rdfs:subClassOf osdu:AbstractWPCGroupType ;
	rdfs:subClassOf osdu:AbstractWorkProductComponent ;
	rdfs:subClassOf osdu:AbstractGeologicUnitInterpretation ;
	rdfs:subClassOf osdu:AbstractInterpretation ;
.

###  https://w3id.org/osdu#RockSample
osdu:RockSample rdf:type owl:Class ;
	rdfs:comment "A rock sample retrieved from an outcrop or Well.  It can be core, sample cut from core, cutting, outcrop, slide etc. " ;
	rdfs:subClassOf osdu:MasterData ;
	rdfs:subClassOf osdu:AbstractCommonResources ;
	rdfs:subClassOf osdu:AbstractMaster ;
.

###  https://w3id.org/osdu#RockSampleAnalysis
osdu:RockSampleAnalysis rdf:type owl:Class ;
	rdfs:comment "The meta-data about a rock sample analysis related to core or outcrop rock samples. " ;
	rdfs:subClassOf osdu:WorkProductComponent ;
	rdfs:subClassOf osdu:AbstractCommonResources ;
	rdfs:subClassOf osdu:AbstractWPCGroupType ;
	rdfs:subClassOf osdu:AbstractWorkProductComponent ;
	rdfs:subClassOf osdu:AbstractWPCActivity ;
.

###  https://w3id.org/osdu#RockSampleType
osdu:RockSampleType rdf:type owl:Class ;
	rdfs:comment "The classification of rock samples. " ;
	rdfs:subClassOf osdu:ReferenceData ;
	rdfs:subClassOf osdu:AbstractCommonResources ;
	rdfs:subClassOf osdu:AbstractReferenceType ;
.

###  https://w3id.org/osdu#RockVolumeFeature
osdu:RockVolumeFeature rdf:type owl:Class ;
	rdfs:comment "A volume of rock that is identified based on some specific attribute, like its mineral content or other physical characteristic. It exists typically in the scope of a model. " ;
	rdfs:subClassOf osdu:MasterData ;
	rdfs:subClassOf osdu:AbstractCommonResources ;
	rdfs:subClassOf osdu:AbstractMaster ;
.

###  https://w3id.org/osdu#RoutineCoreAnalysis
osdu:RoutineCoreAnalysis rdf:type owl:Class ;
	skos:prefLabel "Routine Core Analysis" ;
	rdfs:comment "Conditions and results of a routine core analysis. " ;
	rdfs:subClassOf owl:Thing ;
.

###  https://w3id.org/osdu#RunParameterPlan
osdu:RunParameterPlan rdf:type owl:Class ;
	skos:prefLabel "Run Parameter Plan" ;
	rdfs:comment "Operating parameters of a drill string run " ;
	rdfs:subClassOf owl:Thing ;
.

###  https://w3id.org/osdu#SEGY
osdu:SEGY rdf:type owl:Class ;
	skos:prefLabel "FileCollection.SEGY" ;
	rdfs:comment "A generic representation for  SEGY dataset represented as set of files, e.g. representing original tape reels. " ;
	rdfs:subClassOf osdu:Dataset ;
	rdfs:subClassOf osdu:AbstractCommonResources ;
	rdfs:subClassOf osdu:AbstractDataset ;
	rdfs:subClassOf osdu:AbstractFileCollection ;
	rdfs:subClassOf osdu:AbstractVectorHeaderMapping ;
.

###  https://w3id.org/osdu#SampleOrientationType
osdu:SampleOrientationType rdf:type owl:Class ;
	rdfs:comment "The sample orientation direction, which describes the core sample's relationship to the bedding or drilling direction. " ;
	rdfs:subClassOf osdu:ReferenceData ;
	rdfs:subClassOf osdu:AbstractCommonResources ;
	rdfs:subClassOf osdu:AbstractReferenceType ;
.

###  https://w3id.org/osdu#SampleRemarks
osdu:SampleRemarks rdf:type owl:Class ;
	rdfs:comment "An array containing narrative remarks pertaining to a rock sample. " ;
	rdfs:subClassOf owl:Thing ;
.

###  https://w3id.org/osdu#SatelliteGeometry
osdu:SatelliteGeometry rdf:type owl:Class ;
	rdfs:comment "the reference value type defining the orbit or flight direction of the satellite over the image area " ;
	rdfs:subClassOf osdu:ReferenceData ;
	rdfs:subClassOf osdu:AbstractCommonResources ;
	rdfs:subClassOf osdu:AbstractReferenceType ;
.

###  https://w3id.org/osdu#SatelliteMission
osdu:SatelliteMission rdf:type owl:Class ;
	rdfs:comment "The reference value type defining the satellite mission and the operational period " ;
	rdfs:subClassOf osdu:ReferenceData ;
	rdfs:subClassOf osdu:AbstractCommonResources ;
	rdfs:subClassOf osdu:AbstractReferenceType ;
.

###  https://w3id.org/osdu#SaturationMethodType
osdu:SaturationMethodType rdf:type owl:Class ;
	rdfs:comment "The method used to obtain the saturation measurement values, e.g., Dean Stark, Retort, Karl Fischer. " ;
	rdfs:subClassOf osdu:ReferenceData ;
	rdfs:subClassOf osdu:AbstractCommonResources ;
	rdfs:subClassOf osdu:AbstractReferenceType ;
.

###  https://w3id.org/osdu#SchemaFormatType
osdu:SchemaFormatType rdf:type owl:Class ;
	rdfs:comment "Used to describe the type of schema formats. " ;
	rdfs:subClassOf osdu:ReferenceData ;
	rdfs:subClassOf osdu:AbstractCommonResources ;
	rdfs:subClassOf osdu:AbstractReferenceType ;
.

###  https://w3id.org/osdu#Scope
osdu:Scope rdf:type owl:Class ;
	rdfs:comment "Scope declaration. " ;
	rdfs:subClassOf owl:Thing ;
.

###  https://w3id.org/osdu#SealedSurfaceFramework
osdu:SealedSurfaceFramework rdf:type owl:Class ;
	rdfs:comment "Sealed structural model representations associated to geometric elements such as faults, horizons, and intrusions on a scale of meters to kilometers. " ;
	rdfs:subClassOf osdu:WorkProductComponent ;
	rdfs:subClassOf osdu:AbstractCommonResources ;
	rdfs:subClassOf osdu:AbstractWPCGroupType ;
	rdfs:subClassOf osdu:AbstractWorkProductComponent ;
	rdfs:subClassOf osdu:AbstractRepresentation ;
.

###  https://w3id.org/osdu#SectionType
osdu:SectionType rdf:type owl:Class ;
	rdfs:comment "Used to describe the type of sections. " ;
	rdfs:subClassOf osdu:ReferenceData ;
	rdfs:subClassOf osdu:AbstractCommonResources ;
	rdfs:subClassOf osdu:AbstractReferenceType ;
.

###  https://w3id.org/osdu#SecurityScheme
osdu:SecurityScheme rdf:type owl:Class ;
	rdfs:comment "Metadata used to retrieve or generate credentials needed for authorization. " ;
	rdfs:subClassOf owl:Thing ;
	rdfs:subClassOf [
		a owl:Restriction ;
		owl:onProperty osdu:name ;
		owl:minCardinality "1"^^xsd:nonNegativeInteger ;
	] ;
	rdfs:subClassOf [
		a owl:Restriction ;
		owl:onProperty osdu:typeID ;
		owl:minCardinality "1"^^xsd:nonNegativeInteger ;
	] ;
.

###  https://w3id.org/osdu#SecuritySchemeType
osdu:SecuritySchemeType rdf:type owl:Class ;
	rdfs:comment "A type of security scheme, such as OAuth2, used to generate access credentials to a resource. " ;
	rdfs:subClassOf osdu:ReferenceData ;
	rdfs:subClassOf osdu:AbstractCommonResources ;
	rdfs:subClassOf osdu:AbstractReferenceType ;
.

###  https://w3id.org/osdu#Seismic2DInterpretationSet
osdu:Seismic2DInterpretationSet rdf:type owl:Class ;
	rdfs:subClassOf owl:Thing ;
.

###  https://w3id.org/osdu#Seismic3DInterpretationSet
osdu:Seismic3DInterpretationSet rdf:type owl:Class ;
	rdfs:subClassOf owl:Thing ;
.

###  https://w3id.org/osdu#SeismicAcquisitionSurvey
osdu:SeismicAcquisitionSurvey rdf:type owl:Class ;
	rdfs:comment "A seismic acquisition project is a type of business project that deploys resources to the field to record seismic data.  It may be referred to as a field survey, acquisition survey, or field program.  It is not the same as the geometry of the deployed equipment (nav), which is a work product component. " ;
	rdfs:subClassOf osdu:MasterData ;
	rdfs:subClassOf osdu:AbstractCommonResources ;
	rdfs:subClassOf osdu:AbstractMaster ;
	rdfs:subClassOf osdu:AbstractProject ;
	rdfs:subClassOf osdu:AbstractProjectActivity ;
.

###  https://w3id.org/osdu#SeismicAcquisitionType
osdu:SeismicAcquisitionType rdf:type owl:Class ;
	rdfs:comment "The SeismicAcquisitionType, e.g. Conventional, Wide Azimuth, Multi Azimuth etc. " ;
	rdfs:subClassOf osdu:ReferenceData ;
	rdfs:subClassOf osdu:AbstractCommonResources ;
	rdfs:subClassOf osdu:AbstractReferenceType ;
.

###  https://w3id.org/osdu#SeismicAttributeType
osdu:SeismicAttributeType rdf:type owl:Class ;
	rdfs:comment "Describes the meaning of the seismic sample measurements such as amplitude, phase, dip, azimuth. " ;
	rdfs:subClassOf osdu:ReferenceData ;
	rdfs:subClassOf osdu:AbstractCommonResources ;
	rdfs:subClassOf osdu:AbstractReferenceType ;
.

###  https://w3id.org/osdu#SeismicAttributes
osdu:SeismicAttributes rdf:type owl:Class ;
	rdfs:comment "Summary of measurements included with horizon in addition to depth attribute. " ;
	rdfs:subClassOf owl:Thing ;
.

###  https://w3id.org/osdu#SeismicBinGrid
osdu:SeismicBinGrid rdf:type owl:Class ;
	rdfs:comment "A representation of the surface positions for each subsurface node in a set of processed trace data work product components with common positions.  Different sampling (spacing) and extents (ranges) in the trace data may be handled by the same bin grid. " ;
	rdfs:subClassOf osdu:WorkProductComponent ;
	rdfs:subClassOf osdu:AbstractCommonResources ;
	rdfs:subClassOf osdu:AbstractWPCGroupType ;
	rdfs:subClassOf osdu:AbstractWorkProductComponent ;
	rdfs:subClassOf osdu:AbstractBinGrid ;
.

###  https://w3id.org/osdu#SeismicBinGridType
osdu:SeismicBinGridType rdf:type owl:Class ;
	rdfs:comment "Activity responsible for creating node list such as Acquisition, Processing, Velocity.  Usually Processing. " ;
	rdfs:subClassOf osdu:ReferenceData ;
	rdfs:subClassOf osdu:AbstractCommonResources ;
	rdfs:subClassOf osdu:AbstractReferenceType ;
.

###  https://w3id.org/osdu#SeismicDomainType
osdu:SeismicDomainType rdf:type owl:Class ;
	rdfs:comment "Nature of the vertical axis in the trace data set, usually Depth or Time.  Indicates which pair of start/end values in trace data is the reliable, precise pair. " ;
	rdfs:subClassOf osdu:ReferenceData ;
	rdfs:subClassOf osdu:AbstractCommonResources ;
	rdfs:subClassOf osdu:AbstractReferenceType ;
.

###  https://w3id.org/osdu#SeismicEnergySourceType
osdu:SeismicEnergySourceType rdf:type owl:Class ;
	rdfs:comment "Seismic energy source, such as Airgun, Vibroseis,  Dynamite, Watergun. " ;
	rdfs:subClassOf osdu:ReferenceData ;
	rdfs:subClassOf osdu:AbstractCommonResources ;
	rdfs:subClassOf osdu:AbstractReferenceType ;
.

###  https://w3id.org/osdu#SeismicFault
osdu:SeismicFault rdf:type owl:Class ;
	rdfs:comment "A representation of a single fault picked on the basis of seismic data. The record carries information about the seismic geometry context. It can be part of an UnsealedSurfaceFramework. " ;
	rdfs:subClassOf osdu:WorkProductComponent ;
	rdfs:subClassOf osdu:AbstractCommonResources ;
	rdfs:subClassOf osdu:AbstractWPCGroupType ;
	rdfs:subClassOf osdu:AbstractWorkProductComponent ;
	rdfs:subClassOf osdu:AbstractRepresentation ;
.

###  https://w3id.org/osdu#SeismicFaultType
osdu:SeismicFaultType rdf:type owl:Class ;
	rdfs:comment "Geological type of fault geometry, such as Thrust (thr), Reverse (rev), Normal(norm), Strike-slip. " ;
	rdfs:subClassOf osdu:ReferenceData ;
	rdfs:subClassOf osdu:AbstractCommonResources ;
	rdfs:subClassOf osdu:AbstractReferenceType ;
.

###  https://w3id.org/osdu#SeismicFilteringType
osdu:SeismicFilteringType rdf:type owl:Class ;
	rdfs:comment "Class of final applied filters, for ex. high cut, low cut, spiking deconvolution, multiple elimination. " ;
	rdfs:subClassOf osdu:ReferenceData ;
	rdfs:subClassOf osdu:AbstractCommonResources ;
	rdfs:subClassOf osdu:AbstractReferenceType ;
.

###  https://w3id.org/osdu#SeismicGatherType
osdu:SeismicGatherType rdf:type owl:Class ;
	rdfs:comment "The type of gathers represented in seismic pre-stack datasets. " ;
	rdfs:subClassOf osdu:ReferenceData ;
	rdfs:subClassOf osdu:AbstractCommonResources ;
	rdfs:subClassOf osdu:AbstractReferenceType ;
.

###  https://w3id.org/osdu#SeismicGeometryType
osdu:SeismicGeometryType rdf:type owl:Class ;
	rdfs:comment "Standard values for the general geometrical layout of the seismic acquisition survey.  This is an hierarchical value.  The top value is like 2D, 3D, 4D, Borehole, Passive.  The second value is like NATS, WATS, Brick, Crosswell. " ;
	rdfs:subClassOf osdu:ReferenceData ;
	rdfs:subClassOf osdu:AbstractCommonResources ;
	rdfs:subClassOf osdu:AbstractReferenceType ;
.

###  https://w3id.org/osdu#SeismicHorizon
osdu:SeismicHorizon rdf:type owl:Class ;
	rdfs:comment "A set of picks related to seismic processing geometry which define a surface.  The geometry used is referenced by the Interpretation Project. " ;
	rdfs:subClassOf osdu:WorkProductComponent ;
	rdfs:subClassOf osdu:AbstractCommonResources ;
	rdfs:subClassOf osdu:AbstractWPCGroupType ;
	rdfs:subClassOf osdu:AbstractWorkProductComponent ;
	rdfs:subClassOf osdu:AbstractRepresentation ;
.

###  https://w3id.org/osdu#SeismicHorizonType
osdu:SeismicHorizonType rdf:type owl:Class ;
	rdfs:comment "Position on waveform where horizon is picked such as Peak (pk), Trough (tr), Plus to Minus Zero Crossing, Minus to Plus Zero Crossing, Envelope (env). " ;
	rdfs:subClassOf osdu:ReferenceData ;
	rdfs:subClassOf osdu:AbstractCommonResources ;
	rdfs:subClassOf osdu:AbstractReferenceType ;
.

###  https://w3id.org/osdu#SeismicLineGeometries
osdu:SeismicLineGeometries rdf:type owl:Class ;
	rdfs:comment "A processing geometry comprising the 2D Interpretation Survey (often referred to as survey in the context of an interpretation application but not a survey in the context of acquisition). " ;
	rdfs:subClassOf owl:Thing ;
.

###  https://w3id.org/osdu#SeismicLineGeometry
osdu:SeismicLineGeometry rdf:type owl:Class ;
	rdfs:comment "The 2D processing geometry of a 2D seismic line.  This is not the navigation (acquisition surface geometry). The fully sampled geometry is contained in the work product component's file.  This shows the relationship between CMP, X, Y, and station label. The ends and bends version for mapping purposes is in the work product component's spatial area.  The Name universal property is essential for describing the Line Name. " ;
	rdfs:subClassOf osdu:WorkProductComponent ;
	rdfs:subClassOf osdu:AbstractCommonResources ;
	rdfs:subClassOf osdu:AbstractWPCGroupType ;
	rdfs:subClassOf osdu:AbstractWorkProductComponent ;
.

###  https://w3id.org/osdu#SeismicMigrationType
osdu:SeismicMigrationType rdf:type owl:Class ;
	rdfs:comment "Methods to rearrange seismic information elements so that reflections and diffractions are plotted at their true locations. " ;
	rdfs:subClassOf osdu:ReferenceData ;
	rdfs:subClassOf osdu:AbstractCommonResources ;
	rdfs:subClassOf osdu:AbstractReferenceType ;
.

###  https://w3id.org/osdu#SeismicPickingType
osdu:SeismicPickingType rdf:type owl:Class ;
	rdfs:comment "The method that is used to make the seismic picks. " ;
	rdfs:subClassOf osdu:ReferenceData ;
	rdfs:subClassOf osdu:AbstractCommonResources ;
	rdfs:subClassOf osdu:AbstractReferenceType ;
.

###  https://w3id.org/osdu#SeismicProcessingProject
osdu:SeismicProcessingProject rdf:type owl:Class ;
	rdfs:comment "A seismic processing project is a type of business project which manages the creation of processed seismic work products. It is not the same as the geometry of the processed traces (binning or bin grid), which is a work product component, although it typically defines a single binning.  A processing project may merge data from multiple field surveys, so it is not required to be equated to a single field survey.  Original processing and re-processing activities generate separate and independent processing projects. " ;
	rdfs:subClassOf osdu:MasterData ;
	rdfs:subClassOf osdu:AbstractCommonResources ;
	rdfs:subClassOf osdu:AbstractMaster ;
	rdfs:subClassOf osdu:AbstractProject ;
	rdfs:subClassOf osdu:AbstractProjectActivity ;
.

###  https://w3id.org/osdu#SeismicProcessingStageType
osdu:SeismicProcessingStageType rdf:type owl:Class ;
	rdfs:comment "Describes what main process or workflow manipulated the data before arriving at its current state or that it is as acquired in the field, such as partial processing, migration, modeling result, synthetic model, inversion, phase rotation. " ;
	rdfs:subClassOf osdu:ReferenceData ;
	rdfs:subClassOf osdu:AbstractCommonResources ;
	rdfs:subClassOf osdu:AbstractReferenceType ;
.

###  https://w3id.org/osdu#SeismicReceiverConfiguration
osdu:SeismicReceiverConfiguration rdf:type owl:Class ;
	rdfs:comment "Parameters characterizing the seismic receiver configuration. " ;
	rdfs:subClassOf owl:Thing ;
.

###  https://w3id.org/osdu#SeismicReceiverType
osdu:SeismicReceiverType rdf:type owl:Class ;
	rdfs:comment "A catalog member defining a receiver type in seismic data acquisition. " ;
	rdfs:subClassOf osdu:ReferenceData ;
	rdfs:subClassOf osdu:AbstractCommonResources ;
	rdfs:subClassOf osdu:AbstractReferenceType ;
.

###  https://w3id.org/osdu#SeismicSourceConfiguration
osdu:SeismicSourceConfiguration rdf:type owl:Class ;
	rdfs:comment "Parameters characterizing the seismic source configuration. " ;
	rdfs:subClassOf owl:Thing ;
.

###  https://w3id.org/osdu#SeismicStackingType
osdu:SeismicStackingType rdf:type owl:Class ;
	rdfs:comment "Class of trace stacking state - the dimension stacked along, like partial (offset), full, angle, azimuth.  May be qualified with range indicator such as Near, Mid, Far. " ;
	rdfs:subClassOf osdu:ReferenceData ;
	rdfs:subClassOf osdu:AbstractCommonResources ;
	rdfs:subClassOf osdu:AbstractReferenceType ;
.

###  https://w3id.org/osdu#SeismicTraceData
osdu:SeismicTraceData rdf:type owl:Class ;
	rdfs:comment "A single logical dataset containing seismic samples. " ;
	rdfs:subClassOf osdu:WorkProductComponent ;
	rdfs:subClassOf osdu:AbstractCommonResources ;
	rdfs:subClassOf osdu:AbstractWPCGroupType ;
	rdfs:subClassOf osdu:AbstractWorkProductComponent ;
.

###  https://w3id.org/osdu#SeismicTraceDataDimensionalityType
osdu:SeismicTraceDataDimensionalityType rdf:type owl:Class ;
	rdfs:comment "The dimensionality of trace data sets (not as acquired but as in the dataset), such as 2D, 3D, 4D. " ;
	rdfs:subClassOf osdu:ReferenceData ;
	rdfs:subClassOf osdu:AbstractCommonResources ;
	rdfs:subClassOf osdu:AbstractReferenceType ;
.

###  https://w3id.org/osdu#SeismicTraceSortOrder
osdu:SeismicTraceSortOrder rdf:type owl:Class ;
	rdfs:comment "The types of sorting orders for pre-stack seismic datasets. It describes the trace order of the persisted dataset. " ;
	rdfs:subClassOf osdu:ReferenceData ;
	rdfs:subClassOf osdu:AbstractCommonResources ;
	rdfs:subClassOf osdu:AbstractReferenceType ;
.

###  https://w3id.org/osdu#SeismicWaveType
osdu:SeismicWaveType rdf:type owl:Class ;
	rdfs:comment "The kind of elastic wave resulting from a seismic energy impulse. " ;
	rdfs:subClassOf osdu:ReferenceData ;
	rdfs:subClassOf osdu:AbstractCommonResources ;
	rdfs:subClassOf osdu:AbstractReferenceType ;
.

###  https://w3id.org/osdu#SequenceStratigraphicSchemaType
osdu:SequenceStratigraphicSchemaType rdf:type owl:Class ;
	rdfs:comment "Sequence Stratigraphic Schema type, valid if Stratigraphic Column role type is set to Chronostratigraphic " ;
	rdfs:subClassOf osdu:ReferenceData ;
	rdfs:subClassOf osdu:AbstractCommonResources ;
	rdfs:subClassOf osdu:AbstractReferenceType ;
.

###  https://w3id.org/osdu#SequenceStratigraphySurfaceType
osdu:SequenceStratigraphySurfaceType rdf:type owl:Class ;
	rdfs:comment "Describes the horizon sequence stratigraphic information (flooding, ravinement, maximum flooding, transgressive). " ;
	rdfs:subClassOf osdu:ReferenceData ;
	rdfs:subClassOf osdu:AbstractCommonResources ;
	rdfs:subClassOf osdu:AbstractReferenceType ;
.

###  https://w3id.org/osdu#Shape
osdu:Shape rdf:type owl:Class ;
	skos:prefLabel "FileCollection.Esri.Shape" ;
	rdfs:comment "A dataset representing a shapefile format, i.e. a collection of files with specific extensions. A shapefile is a geospatial vector data format for geographic information system (GIS) software. It is developed and regulated by Esri as a mostly open specification for data interoperability among Esri and other GIS software products. The shapefile format can spatially describe vector features: points, lines, and polygons, representing, for example, water wells, rivers, and lakes. Each item usually has attributes that describe it, such as name or properties. The role of the files in the collection is identified by the standard file extension, e.g. '.dbf', '.shp', '.shx', etc. " ;
	rdfs:subClassOf osdu:Dataset ;
	rdfs:subClassOf osdu:AbstractCommonResources ;
	rdfs:subClassOf osdu:AbstractDataset ;
	rdfs:subClassOf osdu:AbstractFileCollection ;
.

###  https://w3id.org/osdu#SidewallCoreType
osdu:SidewallCoreType rdf:type owl:Class ;
	rdfs:comment "A reference value type for Sidewall Cores. " ;
	rdfs:subClassOf osdu:ReferenceData ;
	rdfs:subClassOf osdu:AbstractCommonResources ;
	rdfs:subClassOf osdu:AbstractReferenceType ;
.

###  https://w3id.org/osdu#SingleCellAquifer
osdu:SingleCellAquifer rdf:type owl:Class ;
	rdfs:comment "Describe a cell which is a part or the whole definition of an aquifer. " ;
	rdfs:subClassOf owl:Thing ;
.

###  https://w3id.org/osdu#Software
osdu:Software rdf:type owl:Class ;
	rdfs:comment "The name and version of the software being executed in the context of this activity " ;
	rdfs:subClassOf owl:Thing ;
.

###  https://w3id.org/osdu#SourceCRS
osdu:SourceCRS rdf:type owl:Class ;
	skos:prefLabel "Source CRS" ;
	rdfs:comment "The source CRS ";
	rdfs:subClassOf owl:Thing ;
.

###  https://w3id.org/osdu#SpatialGeometryType
osdu:SpatialGeometryType rdf:type owl:Class ;
	rdfs:comment "Used to describe the type of spatial geometries. " ;
	rdfs:subClassOf osdu:ReferenceData ;
	rdfs:subClassOf osdu:AbstractCommonResources ;
	rdfs:subClassOf osdu:AbstractReferenceType ;
.

###  https://w3id.org/osdu#SpatialParameterType
osdu:SpatialParameterType rdf:type owl:Class ;
	rdfs:comment "Used to describe the type of spatial parameters. " ;
	rdfs:subClassOf osdu:ReferenceData ;
	rdfs:subClassOf osdu:AbstractCommonResources ;
	rdfs:subClassOf osdu:AbstractReferenceType ;
.

###  https://w3id.org/osdu#StandardsOrganisation
osdu:StandardsOrganisation rdf:type owl:Class ;
	rdfs:comment "The reference-data type holding a StandardsOrganisation, e.g. ISO, IOGP, Energistics, etc. The main purpose is to define organisations, which provide alias names to reference-data. " ;
	rdfs:subClassOf osdu:ReferenceData ;
	rdfs:subClassOf osdu:AbstractCommonResources ;
	rdfs:subClassOf osdu:AbstractReferenceType ;
.

###  https://w3id.org/osdu#Statistics
osdu:Statistics rdf:type owl:Class ;
	rdfs:comment "Structure that describes a individual statistic record of the operations from an activity. " ;
	rdfs:subClassOf owl:Thing ;
	rdfs:subClassOf [
		a owl:Restriction ;
		owl:onProperty osdu:statisticRecord ;
		owl:minCardinality "1"^^xsd:nonNegativeInteger ;
	] ;
	rdfs:subClassOf [
		a owl:Restriction ;
		owl:onProperty osdu:probabilityTypeID ;
		owl:minCardinality "1"^^xsd:nonNegativeInteger ;
	] ;
.

###  https://w3id.org/osdu#StorageFacility
osdu:StorageFacility rdf:type owl:Class ;
	rdfs:comment "A generic storage facility for e.g., core and rock or fluid samples, seismic tapes, etc. " ;
	rdfs:subClassOf osdu:MasterData ;
	rdfs:subClassOf osdu:AbstractCommonResources ;
	rdfs:subClassOf osdu:AbstractMaster ;
	rdfs:subClassOf osdu:AbstractFacility ;
.

###  https://w3id.org/osdu#StratigraphicColumn
osdu:StratigraphicColumn rdf:type owl:Class ;
	rdfs:comment "Representation describing the vertical location of rock units in a particular area " ;
	rdfs:subClassOf osdu:WorkProductComponent ;
	rdfs:subClassOf osdu:AbstractCommonResources ;
	rdfs:subClassOf osdu:AbstractWPCGroupType ;
	rdfs:subClassOf osdu:AbstractWorkProductComponent ;
.

###  https://w3id.org/osdu#StratigraphicColumnRankInterpretation
osdu:StratigraphicColumnRankInterpretation rdf:type owl:Class ;
	rdfs:comment "A global hierarchy containing an ordered list of stratigraphic unit interpretations " ;
	rdfs:subClassOf osdu:WorkProductComponent ;
	rdfs:subClassOf osdu:AbstractCommonResources ;
	rdfs:subClassOf osdu:AbstractWPCGroupType ;
	rdfs:subClassOf osdu:AbstractWorkProductComponent ;
	rdfs:subClassOf osdu:AbstractInterpretation ;
.

###  https://w3id.org/osdu#StratigraphicColumnRankUnitType
osdu:StratigraphicColumnRankUnitType rdf:type owl:Class ;
	rdfs:comment "The reference value type defining a column position in a stratigraphic chart, which is ordered by rank (increasing from left to right). " ;
	rdfs:subClassOf osdu:ReferenceData ;
	rdfs:subClassOf osdu:AbstractCommonResources ;
	rdfs:subClassOf osdu:AbstractReferenceType ;
.

###  https://w3id.org/osdu#StratigraphicColumnValidityAreaType
osdu:StratigraphicColumnValidityAreaType rdf:type owl:Class ;
	rdfs:comment "Member where the custom stratigraphic column has been produced. " ;
	rdfs:subClassOf osdu:ReferenceData ;
	rdfs:subClassOf osdu:AbstractCommonResources ;
	rdfs:subClassOf osdu:AbstractReferenceType ;
.

###  https://w3id.org/osdu#StratigraphicRoleType
osdu:StratigraphicRoleType rdf:type owl:Class ;
	rdfs:comment "The role or type of stratigraphy, e.g., Chronostratigraphic, Lithostratigraphic, etc. " ;
	rdfs:subClassOf osdu:ReferenceData ;
	rdfs:subClassOf osdu:AbstractCommonResources ;
	rdfs:subClassOf osdu:AbstractReferenceType ;
.

###  https://w3id.org/osdu#StratigraphicUnitInterpretation
osdu:StratigraphicUnitInterpretation rdf:type owl:Class ;
	rdfs:comment "One of potentially many boundary interpretations as a single consistent description of a local boundary feature. An interpretation is subjective and very strongly tied to the intellectual activity of the project team members. " ;
	rdfs:subClassOf osdu:WorkProductComponent ;
	rdfs:subClassOf osdu:AbstractCommonResources ;
	rdfs:subClassOf osdu:AbstractWPCGroupType ;
	rdfs:subClassOf osdu:AbstractWorkProductComponent ;
	rdfs:subClassOf osdu:AbstractGeologicUnitInterpretation ;
	rdfs:subClassOf osdu:AbstractInterpretation ;
.

###  https://w3id.org/osdu#StratigraphicUnits
osdu:StratigraphicUnits rdf:type owl:Class ;
	skos:prefLabel "Stratigraphic Units" ;
	rdfs:comment "Allow to link the K layers (or the geologic k property for example in case of K expansion or unstructured grid) of this grid with some stratigraphic units of a stratigraphic organization. " ;
	rdfs:subClassOf owl:Thing ;
	rdfs:subClassOf [
		a owl:Restriction ;
		owl:onProperty osdu:stratigraphicUnitsIndex ;
		owl:minCardinality "1"^^xsd:nonNegativeInteger ;
	] ;
	rdfs:subClassOf [
		a owl:Restriction ;
		owl:onProperty osdu:stratigraphicColumnRankInterpretationID ;
		owl:minCardinality "1"^^xsd:nonNegativeInteger ;
	] ;
.

###  https://w3id.org/osdu#StratigraphicUnitsStratigraphicUnitsIndicesArray
osdu:StratigraphicUnitsStratigraphicUnitsIndicesArray rdf:type owl:Class ;
	rdfs:subClassOf osdu:Array ;
.

###  https://w3id.org/osdu#StringClass
osdu:StringClass rdf:type owl:Class ;
	rdfs:comment "Used to describe the string classes. " ;
	rdfs:subClassOf osdu:ReferenceData ;
	rdfs:subClassOf osdu:AbstractCommonResources ;
	rdfs:subClassOf osdu:AbstractReferenceType ;
.

###  https://w3id.org/osdu#StructuralOrganizationInterpretation
osdu:StructuralOrganizationInterpretation rdf:type owl:Class ;
	rdfs:comment "Structural Model Interpretations related to geometric elements such as faults, horizons, and intrusions on a scale of meters to kilometers. " ;
	rdfs:subClassOf osdu:WorkProductComponent ;
	rdfs:subClassOf osdu:AbstractCommonResources ;
	rdfs:subClassOf osdu:AbstractWPCGroupType ;
	rdfs:subClassOf osdu:AbstractWorkProductComponent ;
	rdfs:subClassOf osdu:AbstractInterpretation ;
.

###  https://w3id.org/osdu#SubRepresentation
osdu:SubRepresentation rdf:type owl:Class ;
	rdfs:comment "An ordered list of indexable elements and/or indexable element pairs of existing representations " ;
	rdfs:subClassOf osdu:WorkProductComponent ;
	rdfs:subClassOf osdu:AbstractCommonResources ;
	rdfs:subClassOf osdu:AbstractWPCGroupType ;
	rdfs:subClassOf osdu:AbstractWorkProductComponent ;
	rdfs:subClassOf osdu:AbstractRepresentation ;
.

###  https://w3id.org/osdu#SurveyProgram
osdu:SurveyProgram rdf:type owl:Class ;
	rdfs:comment "Describes the non-contextual content of an OSDU Survey Program object. " ;
	rdfs:subClassOf osdu:MasterData ;
	rdfs:subClassOf osdu:AbstractCommonResources ;
	rdfs:subClassOf osdu:AbstractMaster ;
	rdfs:subClassOf osdu:AbstractProject ;
.

###  https://w3id.org/osdu#SurveySection
osdu:SurveySection rdf:type owl:Class ;
	skos:prefLabel "Survey Section" ;
	rdfs:comment "Description of the Survey Section Component " ;
	rdfs:subClassOf owl:Thing ;
	rdfs:subClassOf [
		a owl:Restriction ;
		owl:onProperty osdu:sequence ;
		owl:minCardinality "1"^^xsd:nonNegativeInteger ;
	] ;
	rdfs:subClassOf [
		a owl:Restriction ;
		owl:onProperty osdu:surveySectionExistenceKind ;
		owl:minCardinality "1"^^xsd:nonNegativeInteger ;
	] ;
.

###  https://w3id.org/osdu#SurveyToolType
osdu:SurveyToolType rdf:type owl:Class ;
	rdfs:comment "Standardized Type of survey tool used. The content is generally derived from the ISCWSA Set of Generic Tool Codes. " ;
	rdfs:subClassOf osdu:ReferenceData ;
	rdfs:subClassOf osdu:AbstractCommonResources ;
	rdfs:subClassOf osdu:AbstractReferenceType ;
.

###  https://w3id.org/osdu#System
osdu:System rdf:type owl:Class ;
	skos:prefLabel "OSDU System Properties" ;
	rdfs:comment "System properties to be injected at root level by the OsduSchemaComposer script. " ;
	rdfs:subClassOf owl:Thing ;
	rdfs:subClassOf [
		a owl:Restriction ;
		owl:onProperty osdu:kind ;
		owl:minCardinality "1"^^xsd:nonNegativeInteger ;
	] ;
	rdfs:subClassOf [
		a owl:Restriction ;
		owl:onProperty osdu:acl ;
		owl:minCardinality "1"^^xsd:nonNegativeInteger ;
	] ;
	rdfs:subClassOf [
		a owl:Restriction ;
		owl:onProperty osdu:legal ;
		owl:minCardinality "1"^^xsd:nonNegativeInteger ;
	] ;
.

###  https://w3id.org/osdu#TIFF
osdu:TIFF rdf:type owl:Class ;
	skos:prefLabel "File.Image.TIFF" ;
	rdfs:comment "An image file in Tagged Image File Format (TIFF), https://en.wikipedia.org/wiki/TIFF. " ;
	rdfs:subClassOf osdu:Dataset ;
	rdfs:subClassOf osdu:AbstractCommonResources ;
	rdfs:subClassOf osdu:AbstractDataset ;
	rdfs:subClassOf osdu:AbstractFile ;
	rdfs:subClassOf foaf:Image ;
.

###  https://w3id.org/osdu#Target
osdu:Target rdf:type owl:Class ;
	rdfs:comment "This is a geometric body describing a volume in the earth intended to be a target of one or more wellbores. " ;
	rdfs:subClassOf owl:Thing ;
.

###  https://w3id.org/osdu#TargetCRS
osdu:TargetCRS rdf:type owl:Class ;
	skos:prefLabel "Target CRS" ;
	rdfs:comment "The target Coordinate Reference System.";
	rdfs:subClassOf owl:Thing ;
.

###  https://w3id.org/osdu#TargetShape
osdu:TargetShape rdf:type owl:Class ;
	rdfs:comment "Target shape such as point, rectangular etc. " ;
	rdfs:subClassOf osdu:ReferenceData ;
	rdfs:subClassOf osdu:AbstractCommonResources ;
	rdfs:subClassOf osdu:AbstractReferenceType ;
.

###  https://w3id.org/osdu#TargetType
osdu:TargetType rdf:type owl:Class ;
	rdfs:comment "Target Category such as geological target or driller target " ;
	rdfs:subClassOf osdu:ReferenceData ;
	rdfs:subClassOf osdu:AbstractCommonResources ;
	rdfs:subClassOf osdu:AbstractReferenceType ;
.

###  https://w3id.org/osdu#TechnicalAssuranceType
osdu:TechnicalAssuranceType rdf:type owl:Class ;
	rdfs:comment "The reference value type describing a record's overall suitability for general business consumption based on data quality. Clarifications: Since Certified is the highest classification of suitable quality, any further change or versioning of a Certified record should be carefully considered and justified. If a Technical Assurance value is not populated then one can assume the data has not been evaluated or its quality is unknown  (=Unevaluated). Technical Assurance values are not intended to be used for the identification of a single preferred or definitive record by comparison with other records. " ;
	rdfs:subClassOf osdu:ReferenceData ;
	rdfs:subClassOf osdu:AbstractCommonResources ;
	rdfs:subClassOf osdu:AbstractReferenceType ;
.

###  https://w3id.org/osdu#TectonicSettingType
osdu:TectonicSettingType rdf:type owl:Class ;
	rdfs:comment "Reference object to offer a list of values to describe the Tectonic Setting - which is a scenario used for Planning and Pore Pressure Practitioners - such as 'Strike Slip' " ;
	rdfs:subClassOf osdu:ReferenceData ;
	rdfs:subClassOf osdu:AbstractCommonResources ;
	rdfs:subClassOf osdu:AbstractReferenceType ;
.

###  https://w3id.org/osdu#Terms
osdu:Terms rdf:type owl:Class ;
	rdfs:subClassOf owl:Thing ;
.

###  https://w3id.org/osdu#TestFluid
osdu:TestFluid rdf:type owl:Class ;
	skos:prefLabel "Test Fluid" ;
	rdfs:comment "Description, for a given step of the test, of the Fluid System used for this step. " ;
	rdfs:subClassOf owl:Thing ;
.

###  https://w3id.org/osdu#TestSubType
osdu:TestSubType rdf:type owl:Class ;
	rdfs:comment "Well Barrier Element test sub-types for the barrier component being tested such as Subsea BOP interval test, Surface BOP test, Surface PCE test, Wireline PCE Test " ;
	rdfs:subClassOf osdu:ReferenceData ;
	rdfs:subClassOf osdu:AbstractCommonResources ;
	rdfs:subClassOf osdu:AbstractReferenceType ;
.

###  https://w3id.org/osdu#TestType
osdu:TestType rdf:type owl:Class ;
	rdfs:comment "Well Barrier Element test types " ;
	rdfs:subClassOf osdu:ReferenceData ;
	rdfs:subClassOf osdu:AbstractCommonResources ;
	rdfs:subClassOf osdu:AbstractReferenceType ;
.

###  https://w3id.org/osdu#TimeLapse
osdu:TimeLapse rdf:type owl:Class ;
	skos:prefLabel "Time Lapse" ;
	rdfs:comment "The contents positions the SeismicTraceData record in context of a time series. This is to be used for time lapse or 4D SeismicTraceData. This structure is optional and absent for SeismicTraceData not part of a time series. " ;
	rdfs:subClassOf owl:Thing ;
.

###  https://w3id.org/osdu#TimeSeries
osdu:TimeSeries rdf:type owl:Class ;
	rdfs:comment "Stores an ordered list of times, for example used for time-dependent properties (saturation) or geometries (varying reservoir geometry through time). " ;
	rdfs:subClassOf osdu:WorkProductComponent ;
	rdfs:subClassOf osdu:AbstractCommonResources ;
	rdfs:subClassOf osdu:AbstractWPCGroupType ;
	rdfs:subClassOf osdu:AbstractWorkProductComponent ;
	rdfs:subClassOf [
		a owl:Restriction ;
		owl:onProperty osdu:timeIndex ;
		owl:minCardinality "1"^^xsd:nonNegativeInteger ;
	] ;
	rdfs:subClassOf [
		a owl:Restriction ;
		owl:onProperty osdu:timeSeriesID ;
		owl:minCardinality "1"^^xsd:nonNegativeInteger ;
	] ;
.

###  https://w3id.org/osdu#TimedComment
osdu:TimedComment rdf:type owl:Class ;
	skos:prefLabel "Timed Comment" ;
	rdfs:comment "Information about a series of drilling activities. " ;
	rdfs:subClassOf owl:Thing ;
.

###  https://w3id.org/osdu#TorqueOnBottomGroup
osdu:TorqueOnBottomGroup rdf:type owl:Class ;
	skos:prefLabel "Torque On Bottom Group" ;
	rdfs:comment "A group of parameters that refer to Torque on Bottom " ;
	rdfs:subClassOf owl:Thing ;
	rdfs:subClassOf [
		a owl:Restriction ;
		owl:onProperty osdu:hasMaximumTorqueOnBottom ;
		owl:minCardinality "1"^^xsd:nonNegativeInteger ;
	] ;
	rdfs:subClassOf [
		a owl:Restriction ;
		owl:onProperty osdu:hasMinimumTorqueOnBottom ;
		owl:minCardinality "1"^^xsd:nonNegativeInteger ;
	] ;
.

###  https://w3id.org/osdu#TrajectoryStationPropertyType
osdu:TrajectoryStationPropertyType rdf:type owl:Class ;
	rdfs:comment "The trajectory station property catalog for e.g. WellboreTrajectory AvailableTrajectoryStationProperties. Similar to LogCurveType the TrajectoryStationPropertyType describes well-known properties (or curves or channels in an array view), which can be accessed via the Wellbore Domain Data Management Services. " ;
	rdfs:subClassOf osdu:ReferenceData ;
	rdfs:subClassOf osdu:AbstractCommonResources ;
	rdfs:subClassOf osdu:AbstractReferenceType ;
	rdfs:subClassOf osdu:AbstractReferencePropertyType ;
.

###  https://w3id.org/osdu#Transformation
osdu:Transformation rdf:type owl:Class ;
	skos:prefLabel "Bound Transformation" ;
	rdfs:comment "The Transformation bound to the BaseCRS in a BoundCRS. Only populated for CoordinateReferenceSystemType==BoundCRS. " ;
	rdfs:subClassOf owl:Thing ;
.

###  https://w3id.org/osdu#TubularAssembly
osdu:TubularAssembly rdf:type owl:Class ;
	rdfs:comment "Well Tubular data contains information on the tubular assemblies and their components for the well, wellbore, or wellbore completion (as appropriate). The tubulars can be tubing, casing or liners or other related equipment which is installed into the well. Tubulars can also be equipment which is lowered into the well in the context of drilling, which is then pulled back out. " ;
	rdfs:subClassOf osdu:WorkProductComponent ;
	rdfs:subClassOf osdu:AbstractCommonResources ;
	rdfs:subClassOf osdu:AbstractWPCGroupType ;
	rdfs:subClassOf osdu:AbstractWorkProductComponent ;
.

###  https://w3id.org/osdu#TubularAssemblyStatus
osdu:TubularAssemblyStatus rdf:type owl:Class ;
	rdfs:comment "Record that reflects the status of the Assembly - as 'installed', 'pulled', 'planned',... - Applicable to tubing/completions as opposed to drillstrings " ;
	rdfs:subClassOf owl:Thing ;
.

###  https://w3id.org/osdu#TubularAssemblyStatusType
osdu:TubularAssemblyStatusType rdf:type owl:Class ;
	rdfs:comment "Used to describe the status of the Tubular Assembly, such as Pulled, Installed,..... " ;
	rdfs:subClassOf osdu:ReferenceData ;
	rdfs:subClassOf osdu:AbstractCommonResources ;
	rdfs:subClassOf osdu:AbstractReferenceType ;
.

###  https://w3id.org/osdu#TubularAssemblyType
osdu:TubularAssemblyType rdf:type owl:Class ;
	rdfs:comment "Used to describe the type of tubular assemblies. " ;
	rdfs:subClassOf osdu:ReferenceData ;
	rdfs:subClassOf osdu:AbstractCommonResources ;
	rdfs:subClassOf osdu:AbstractReferenceType ;
.

###  https://w3id.org/osdu#TubularComponent
osdu:TubularComponent rdf:type owl:Class ;
	rdfs:comment "Well Tubular data contains information on the tubular assemblies and their components for the well, wellbore, or wellbore completion (as appropriate). The tubulars can be tubing, casing or liners or other related equipment which is installed into the well. Tubulars can also be equipment which is lowered into the well in the context of drilling, which is then pulled back out. " ;
	rdfs:subClassOf osdu:WorkProductComponent ;
	rdfs:subClassOf osdu:AbstractCommonResources ;
	rdfs:subClassOf osdu:AbstractWPCGroupType ;
	rdfs:subClassOf osdu:AbstractWorkProductComponent ;
.

###  https://w3id.org/osdu#TubularComponentConnectionType
osdu:TubularComponentConnectionType rdf:type owl:Class ;
	rdfs:comment "Used to describe the type of tubular component connections. " ;
	rdfs:subClassOf osdu:ReferenceData ;
	rdfs:subClassOf osdu:AbstractCommonResources ;
	rdfs:subClassOf osdu:AbstractReferenceType ;
.

###  https://w3id.org/osdu#TubularComponentGrade
osdu:TubularComponentGrade rdf:type owl:Class ;
	rdfs:comment "Id of tubing grade - eg. the tensile strength of the tubing material. A system of classifying the material specifications for steel alloys used in the manufacture of tubing. " ;
	rdfs:subClassOf osdu:ReferenceData ;
	rdfs:subClassOf osdu:AbstractCommonResources ;
	rdfs:subClassOf osdu:AbstractReferenceType ;
.

###  https://w3id.org/osdu#TubularComponentPinBoxType
osdu:TubularComponentPinBoxType rdf:type owl:Class ;
	rdfs:comment "The type of collar used to couple the tubular with another tubing string. " ;
	rdfs:subClassOf osdu:ReferenceData ;
	rdfs:subClassOf osdu:AbstractCommonResources ;
	rdfs:subClassOf osdu:AbstractReferenceType ;
.

###  https://w3id.org/osdu#TubularComponentType
osdu:TubularComponentType rdf:type owl:Class ;
	rdfs:comment "Specifies the types of components that can be used in a tubular string. These are used to specify the type of component and multiple components are used to define a tubular string (Tubular). " ;
	rdfs:subClassOf osdu:ReferenceData ;
	rdfs:subClassOf osdu:AbstractCommonResources ;
	rdfs:subClassOf osdu:AbstractReferenceType ;
.

###  https://w3id.org/osdu#TubularMaterialType
osdu:TubularMaterialType rdf:type owl:Class ;
	rdfs:comment "The general or specific description of the material used to make tubular goods (casing, pipe, etc.) " ;
	rdfs:subClassOf osdu:ReferenceData ;
	rdfs:subClassOf osdu:AbstractCommonResources ;
	rdfs:subClassOf osdu:AbstractReferenceType ;
.

###  https://w3id.org/osdu#TubularUmbilical
osdu:TubularUmbilical rdf:type owl:Class ;
	rdfs:comment "An umbilical is any control, power or sensor cable or tube run through an outlet on the wellhead down to a particular receptacle on a downhole component (power or hydraulic line) or simply to a specific depth (sensors). Examples include Gas lift injection tube, Subsea valve control line, ESP power cable, iWire for external gauges, external Fiber Optic Sensor cable. Umbilicals are run outside of the casing or completion assembly and are typically attached by clamps. Umbilicals are run in hole same time as the host assembly. Casing Umbilicals may be cemented in place e.g. Fiber Optic. " ;
	rdfs:subClassOf osdu:WorkProductComponent ;
	rdfs:subClassOf osdu:AbstractCommonResources ;
	rdfs:subClassOf osdu:AbstractWPCGroupType ;
	rdfs:subClassOf osdu:AbstractWorkProductComponent ;
.

###  https://w3id.org/osdu#TubularUmbilicalServiceType
osdu:TubularUmbilicalServiceType rdf:type owl:Class ;
	rdfs:comment "Used to describe the service the umbilical is designed for (such as Standard, H2S Sour Service,...). " ;
	rdfs:subClassOf osdu:ReferenceData ;
	rdfs:subClassOf osdu:AbstractCommonResources ;
	rdfs:subClassOf osdu:AbstractReferenceType ;
.

###  https://w3id.org/osdu#TubularUmbilicalType
osdu:TubularUmbilicalType rdf:type owl:Class ;
	rdfs:comment "Used to describe the type of tubular umbilical. " ;
	rdfs:subClassOf osdu:ReferenceData ;
	rdfs:subClassOf osdu:AbstractCommonResources ;
	rdfs:subClassOf osdu:AbstractReferenceType ;
.

###  https://w3id.org/osdu#Type
osdu:Type rdf:type owl:Class ;
	rdfs:comment "The generic type entity. " ;
	rdfs:subClassOf osdu:AbstractCommonResources ;
	rdfs:subClassOf osdu:System ;
.

###  https://w3id.org/osdu#UnacceptableUsage
osdu:UnacceptableUsage rdf:type owl:Class ;
	rdfs:comment "Describes the workflows and/or personas that the technical assurance value is not valid for (e.g., This data has a technical assurance property of trusted, but it is not suitable for Seismic Interpretation). " ;
	rdfs:subClassOf owl:Thing ;
.

###  https://w3id.org/osdu#UnitOfMeasure
osdu:UnitOfMeasure rdf:type owl:Class ;
	rdfs:comment "Used to describe the unit of measures. " ;
	rdfs:subClassOf osdu:ReferenceData ;
	rdfs:subClassOf osdu:AbstractCommonResources ;
	rdfs:subClassOf osdu:AbstractReferenceType ;
.

###  https://w3id.org/osdu#UnitOfMeasureConfiguration
osdu:UnitOfMeasureConfiguration rdf:type owl:Class ;
	rdfs:comment "A UnitOfMeasure configuration allowing to associate preferred units and default units to specific UnitQuantity values. UnitQuantity provides the full list of units, UnitOfMeasureConfiguration scopes the lists to a domain's/app's/user's requirements. " ;
	rdfs:subClassOf osdu:ReferenceData ;
	rdfs:subClassOf osdu:AbstractCommonResources ;
	rdfs:subClassOf osdu:AbstractReferenceType ;
.

###  https://w3id.org/osdu#UnitQuantity
osdu:UnitQuantity rdf:type owl:Class ;
	rdfs:comment "A single unit quantity class representing a superclass of mutually comparable quantity kinds. The class may or may not represent a recognized quantity kind (i.e., it may logically be abstract).  Quantities of the same class will have the same quantity dimension.  However, quantities of the same dimension are not necessarily of the same class. The term unit quantity class is intended to have the same general  meaning as the term kind of quantity as defined by the  International vocabulary of meteorology - Basic and general concepts and associated terms (VIM) (JCGM 200:2008) https://www.bipm.org/utils/common/documents/jcgm/JCGM_200_2012.pdf. " ;
	rdfs:subClassOf osdu:ReferenceData ;
	rdfs:subClassOf osdu:AbstractCommonResources ;
	rdfs:subClassOf osdu:AbstractReferenceType ;
.

###  https://w3id.org/osdu#UnsealedSurfaceFramework
osdu:UnsealedSurfaceFramework rdf:type owl:Class ;
	rdfs:comment "Unsealed structural model representations associated to geometric elements such as faults, horizons, and intrusions on a scale of meters to kilometers. " ;
	rdfs:subClassOf osdu:WorkProductComponent ;
	rdfs:subClassOf osdu:AbstractCommonResources ;
	rdfs:subClassOf osdu:AbstractWPCGroupType ;
	rdfs:subClassOf osdu:AbstractWorkProductComponent ;
	rdfs:subClassOf osdu:AbstractRepresentation ;
.

###  https://w3id.org/osdu#UnstructuredColumnLayerGridRepresentation
osdu:UnstructuredColumnLayerGridRepresentation rdf:type owl:Class ;
	rdfs:comment "Definition of a collection of polyhedra which are only organized by column. " ;
	rdfs:subClassOf osdu:WorkProductComponent ;
	rdfs:subClassOf osdu:AbstractCommonResources ;
	rdfs:subClassOf osdu:AbstractWPCGroupType ;
	rdfs:subClassOf osdu:AbstractWorkProductComponent ;
	rdfs:subClassOf osdu:AbstractGridRepresentation ;
	rdfs:subClassOf osdu:AbstractUnstructuredColumnLayerGridPatch ;
.

###  https://w3id.org/osdu#UnstructuredGridRepresentation
osdu:UnstructuredGridRepresentation rdf:type owl:Class ;
	rdfs:comment "Definition of a collection of polyhedra which are not organized in any dimension. " ;
	rdfs:subClassOf osdu:WorkProductComponent ;
	rdfs:subClassOf osdu:AbstractCommonResources ;
	rdfs:subClassOf osdu:AbstractWPCGroupType ;
	rdfs:subClassOf osdu:AbstractWorkProductComponent ;
	rdfs:subClassOf osdu:AbstractGridRepresentation ;
	rdfs:subClassOf osdu:AbstractUnstructuredGridPatch ;
.

###  https://w3id.org/osdu#Usage
osdu:Usage rdf:type owl:Class ;
	rdfs:comment "Scope and extent information." ;
	rdfs:subClassOf owl:Thing ;
.

###  https://w3id.org/osdu#ValueChainStatusType
osdu:ValueChainStatusType rdf:type owl:Class ;
	rdfs:comment "Phase of the value chain where the custom stratigraphic column has been produced. " ;
	rdfs:subClassOf osdu:ReferenceData ;
	rdfs:subClassOf osdu:AbstractCommonResources ;
	rdfs:subClassOf osdu:AbstractReferenceType ;
.

###  https://w3id.org/osdu#VectorHeaderMapping
osdu:VectorHeaderMapping rdf:type owl:Class ;
	rdfs:comment "Array of objects which define the meaning and format of a tabular structure used in a binary file as a header.  The initial use case is the trace headers of a SEG-Y file.  Note that some of this information may be repeated in the SEG-Y EBCDIC header. " ;
	rdfs:subClassOf owl:Thing ;
.

###  https://w3id.org/osdu#VelocityAnalysisMethod
osdu:VelocityAnalysisMethod rdf:type owl:Class ;
	rdfs:comment "Type of algorithm used to derive velocities such as Stacking NMO, Tomography. " ;
	rdfs:subClassOf osdu:ReferenceData ;
	rdfs:subClassOf osdu:AbstractCommonResources ;
	rdfs:subClassOf osdu:AbstractReferenceType ;
.

###  https://w3id.org/osdu#VelocityDirectionType
osdu:VelocityDirectionType rdf:type owl:Class ;
	rdfs:comment "Direction or orientation associated with the velocity model such as vertical, dip-azimuth. " ;
	rdfs:subClassOf osdu:ReferenceData ;
	rdfs:subClassOf osdu:AbstractCommonResources ;
	rdfs:subClassOf osdu:AbstractReferenceType ;
.

###  https://w3id.org/osdu#VelocityModeling
osdu:VelocityModeling rdf:type owl:Class ;
	rdfs:comment "An earth model describing seismic velocities. " ;
	rdfs:subClassOf osdu:WorkProductComponent ;
	rdfs:subClassOf osdu:AbstractCommonResources ;
	rdfs:subClassOf osdu:AbstractWPCGroupType ;
	rdfs:subClassOf osdu:AbstractWorkProductComponent ;
.

###  https://w3id.org/osdu#VelocityType
osdu:VelocityType rdf:type owl:Class ;
	rdfs:comment "Name describing the statistic represented by the velocity model such as RMS, Average, Interval, Instantaneous. " ;
	rdfs:subClassOf osdu:ReferenceData ;
	rdfs:subClassOf osdu:AbstractCommonResources ;
	rdfs:subClassOf osdu:AbstractReferenceType ;
.

###  https://w3id.org/osdu#VerticalCRS
osdu:VerticalCRS rdf:type owl:Class ;
	skos:prefLabel "Vertical CRS" ;
	rdfs:comment "The vertical CRS reference of a CompoundCRS. Only populated for CoordinateReferenceSystemType==CompoundCRS. " ;
	rdfs:subClassOf owl:Thing ;
.

###  https://w3id.org/osdu#VerticalMeasurementID
osdu:VerticalMeasurementID rdf:type owl:Class ;
	skos:prefLabel "Vertical Measurement ID" ;
	rdfs:subClassOf osdu:AbstractFacilityVerticalMeasurement ;
	rdfs:subClassOf owl:Thing ;
.

###  https://w3id.org/osdu#VerticalMeasurementPath
osdu:VerticalMeasurementPath rdf:type owl:Class ;
	rdfs:comment "The type of vertical distance of a point in a well relative to a defined reference point. " ;
	rdfs:subClassOf osdu:ReferenceData ;
	rdfs:subClassOf osdu:AbstractCommonResources ;
	rdfs:subClassOf osdu:AbstractReferenceType ;
.

###  https://w3id.org/osdu#VerticalMeasurementSource
osdu:VerticalMeasurementSource rdf:type owl:Class ;
	rdfs:comment "Used to describe the type of vertical measurement sources. " ;
	rdfs:subClassOf osdu:ReferenceData ;
	rdfs:subClassOf osdu:AbstractCommonResources ;
	rdfs:subClassOf osdu:AbstractReferenceType ;
.

###  https://w3id.org/osdu#VerticalMeasurementType
osdu:VerticalMeasurementType rdf:type owl:Class ;
	rdfs:comment "The horizontal plane of reference for well depth and elevation measurements, where the measured value is zero. " ;
	rdfs:subClassOf osdu:ReferenceData ;
	rdfs:subClassOf osdu:AbstractCommonResources ;
	rdfs:subClassOf osdu:AbstractReferenceType ;
.

###  https://w3id.org/osdu#VoidageGroupInterpretation
osdu:VoidageGroupInterpretation rdf:type owl:Class ;
	rdfs:comment "A group of several reservoir compartments which can be associated to RockFluidOrganisationInterpretations and/or to GeologicUnitOrganizationInterpretations. " ;
	rdfs:subClassOf osdu:WorkProductComponent ;
	rdfs:subClassOf osdu:AbstractCommonResources ;
	rdfs:subClassOf osdu:AbstractWPCGroupType ;
	rdfs:subClassOf osdu:AbstractWorkProductComponent ;
	rdfs:subClassOf osdu:AbstractInterpretation ;
.

###  https://w3id.org/osdu#WBETestStep
osdu:WBETestStep rdf:type owl:Class ;
	skos:prefLabel "W.B.E. Test Step" ;
	rdfs:comment "Description of an individual step of the overall Well Barrier Element Test " ;
	rdfs:subClassOf owl:Thing ;
	rdfs:subClassOf [
		a owl:Restriction ;
		owl:onProperty osdu:stepNumber ;
		owl:minCardinality "1"^^xsd:nonNegativeInteger ;
	] ;
	rdfs:subClassOf [
		a owl:Restriction ;
		owl:onProperty osdu:hasHighPressureCriteria ;
		owl:minCardinality "1"^^xsd:nonNegativeInteger ;
	] ;
	rdfs:subClassOf [
		a owl:Restriction ;
		owl:onProperty osdu:expectedPressureChangeDueToThermalEffects ;
		owl:minCardinality "1"^^xsd:nonNegativeInteger ;
	] ;
	rdfs:subClassOf [
		a owl:Restriction ;
		owl:onProperty osdu:totalVolumeTestSystem ;
		owl:minCardinality "1"^^xsd:nonNegativeInteger ;
	] ;
.

###  https://w3id.org/osdu#WITSML
osdu:WITSML rdf:type owl:Class ;
	skos:prefLabel "File.WITSML" ;
	rdfs:comment "Schema describing a WITSML file resource. " ;
	rdfs:subClassOf osdu:Dataset ;
	rdfs:subClassOf osdu:AbstractCommonResources ;
	rdfs:subClassOf osdu:AbstractDataset ;
	rdfs:subClassOf osdu:AbstractFile ;
.

###  https://w3id.org/osdu#WOBGroup
osdu:WOBGroup rdf:type owl:Class ;
	skos:prefLabel "W.O.B. Group" ;
	rdfs:comment "A group of parameters that refer to WOB (weight on bit) " ;
	rdfs:subClassOf owl:Thing ;
	rdfs:subClassOf [
		a owl:Restriction ;
		owl:onProperty osdu:maximumWOB ;
		owl:minCardinality "1"^^xsd:nonNegativeInteger ;
	] ;
	rdfs:subClassOf [
		a owl:Restriction ;
		owl:onProperty osdu:minimumWOB ;
		owl:minCardinality "1"^^xsd:nonNegativeInteger ;
	] ;
.

###  https://w3id.org/osdu#Weather
osdu:Weather rdf:type owl:Class ;
	rdfs:comment "Meteorological readings for the defined time period on an operations report " ;
	rdfs:subClassOf owl:Thing ;
	rdfs:subClassOf [
		a owl:Restriction ;
		owl:onProperty osdu:dateTime ;
		owl:minCardinality "1"^^xsd:nonNegativeInteger ;
	] ;
.

###  https://w3id.org/osdu#WeatherType
osdu:WeatherType rdf:type owl:Class ;
	rdfs:comment "Type of weather observed during the operations reporting period " ;
	rdfs:subClassOf osdu:ReferenceData ;
	rdfs:subClassOf osdu:AbstractCommonResources ;
	rdfs:subClassOf osdu:AbstractReferenceType ;
.

###  https://w3id.org/osdu#Well
osdu:Well rdf:type owl:Class ;
	rdfs:comment "The origin of a set of wellbores. " ;
	rdfs:subClassOf osdu:MasterData ;
	rdfs:subClassOf osdu:AbstractCommonResources ;
	rdfs:subClassOf osdu:AbstractMaster ;
	rdfs:subClassOf osdu:AbstractFacility ;
.

###  https://w3id.org/osdu#WellActivityPhaseType
osdu:WellActivityPhaseType rdf:type owl:Class ;
	rdfs:comment "Key milestones in a well activity program, usually based on the major sections of the well or non well-related work " ;
	rdfs:subClassOf osdu:ReferenceData ;
	rdfs:subClassOf osdu:AbstractCommonResources ;
	rdfs:subClassOf osdu:AbstractReferenceType ;
.

###  https://w3id.org/osdu#WellActivityProgram
osdu:WellActivityProgram rdf:type owl:Class ;
	rdfs:comment "A complete description of an Activity Program for a unique or a set of Well(s) and/or Wellbore(s) " ;
	rdfs:subClassOf osdu:MasterData ;
	rdfs:subClassOf osdu:AbstractCommonResources ;
	rdfs:subClassOf osdu:AbstractMaster ;
	rdfs:subClassOf osdu:AbstractProject ;
.

###  https://w3id.org/osdu#WellActivityProgramType
osdu:WellActivityProgramType rdf:type owl:Class ;
	rdfs:comment "Type of well activity program. Can be Primary or Contingency " ;
	rdfs:subClassOf osdu:ReferenceData ;
	rdfs:subClassOf osdu:AbstractCommonResources ;
	rdfs:subClassOf osdu:AbstractReferenceType ;
.

###  https://w3id.org/osdu#WellAlias
osdu:WellAlias rdf:type owl:Class ;
	skos:prefLabel "Well Alias" ;
	rdfs:comment "Local name defined for the Well " ;
	rdfs:subClassOf owl:Thing ;
	rdfs:subClassOf [
		a owl:Restriction ;
		owl:onProperty osdu:identifier ;
		owl:minCardinality "1"^^xsd:nonNegativeInteger ;
	] ;
	rdfs:subClassOf [
		a owl:Restriction ;
		owl:onProperty osdu:authority ;
		owl:minCardinality "1"^^xsd:nonNegativeInteger ;
	] ;
.

###  https://w3id.org/osdu#WellBarrierElementTest
osdu:WellBarrierElementTest rdf:type owl:Class ;
	rdfs:comment "Describes a complete sequence to test for the Well Integrity " ;
	rdfs:subClassOf osdu:MasterData ;
	rdfs:subClassOf osdu:AbstractCommonResources ;
	rdfs:subClassOf osdu:AbstractMaster ;
	rdfs:subClassOf osdu:AbstractProject ;
.

###  https://w3id.org/osdu#WellBusinessIntention
osdu:WellBusinessIntention rdf:type owl:Class ;
	rdfs:comment "Business Intention [Well Business Intention] is the general purpose for which resources are approved for drilling a new well or subsequent wellbore(s). " ;
	rdfs:subClassOf osdu:ReferenceData ;
	rdfs:subClassOf osdu:AbstractCommonResources ;
	rdfs:subClassOf osdu:AbstractReferenceType ;
.

###  https://w3id.org/osdu#WellBusinessIntentionOutcome
osdu:WellBusinessIntentionOutcome rdf:type owl:Class ;
	rdfs:comment "Outcome [Well Business Intention Outcome] is the result of attempting to accomplish the Business Intention [Well Business Intention]. " ;
	rdfs:subClassOf osdu:ReferenceData ;
	rdfs:subClassOf osdu:AbstractCommonResources ;
	rdfs:subClassOf osdu:AbstractReferenceType ;
.

###  https://w3id.org/osdu#WellCondition
osdu:WellCondition rdf:type owl:Class ;
	rdfs:comment "Condition [Well Condition] is the operational state of a well component relative to the Role [Well Role]. " ;
	rdfs:subClassOf osdu:ReferenceData ;
	rdfs:subClassOf osdu:AbstractCommonResources ;
	rdfs:subClassOf osdu:AbstractReferenceType ;
.

###  https://w3id.org/osdu#WellFluidDirection
osdu:WellFluidDirection rdf:type owl:Class ;
	rdfs:comment "Fluid Direction [Well Fluid Direction] is the flow direction of the wellhead stream. The facet value can change over the life of the well. " ;
	rdfs:subClassOf osdu:ReferenceData ;
	rdfs:subClassOf osdu:AbstractCommonResources ;
	rdfs:subClassOf osdu:AbstractReferenceType ;
.

###  https://w3id.org/osdu#WellInterestType
osdu:WellInterestType rdf:type owl:Class ;
	rdfs:comment "Well Business Interest [Well Interest Type] describes whether a company currently considers a well entity or its data to be a real or planned asset, and if so, the nature of and motivation for that company's interest. " ;
	rdfs:subClassOf osdu:ReferenceData ;
	rdfs:subClassOf osdu:AbstractCommonResources ;
	rdfs:subClassOf osdu:AbstractReferenceType ;
.

###  https://w3id.org/osdu#WellLog
osdu:WellLog rdf:type owl:Class ;
	rdfs:comment "A well log is a data type that correlates a particular measurement or multiple measurements in a wellbore against depth and/or time within that wellbore. When plotted visually, well logs are typically long line graphs (called curves) but may sometimes be discrete points or intervals. This schema object is intended for digital well logs, not raster log files or raster calibration files, but may be used for the latter in the absence of a defined OSDU schema for these use cases. " ;
	rdfs:subClassOf osdu:WorkProductComponent ;
	rdfs:subClassOf osdu:AbstractCommonResources ;
	rdfs:subClassOf osdu:AbstractWPCGroupType ;
	rdfs:subClassOf osdu:AbstractWorkProductComponent ;
.

###  https://w3id.org/osdu#WellLogSamplingDomainType
osdu:WellLogSamplingDomainType rdf:type owl:Class ;
	rdfs:comment "The reference type for the well log, e.g. the domain of the reference curve. The most common value is Depth but it can also be calendar time, e.g. TimePast-1970-01-01 or SeismicTwoWayTravelTime. " ;
	rdfs:subClassOf osdu:ReferenceData ;
	rdfs:subClassOf osdu:AbstractCommonResources ;
	rdfs:subClassOf osdu:AbstractReferenceType ;
.

###  https://w3id.org/osdu#WellPlanningActivity
osdu:WellPlanningActivity rdf:type owl:Class ;
	skos:prefLabel "Well Planning Activity" ;
	rdfs:comment "Information regarding an individual activity that is part of the ActivityPlan " ;
	rdfs:subClassOf owl:Thing ;
	rdfs:subClassOf [
		a owl:Restriction ;
		owl:onProperty osdu:activityID ;
		owl:minCardinality "1"^^xsd:nonNegativeInteger ;
	] ;
.

###  https://w3id.org/osdu#WellPlanningWell
osdu:WellPlanningWell rdf:type owl:Class ;
	rdfs:comment "Information about a single well. A well is a unique surface location from which wellbores are drilled into the Earth for the purpose of either (1) finding or producing underground resources; or (2) providing services related to the production of underground resources. " ;
	rdfs:subClassOf osdu:MasterData ;
	rdfs:subClassOf osdu:AbstractCommonResources ;
.

###  https://w3id.org/osdu#WellPlanningWellbore
osdu:WellPlanningWellbore rdf:type owl:Class ;
	rdfs:comment "A hole in the ground extending from a point at the earth's surface to the maximum point of penetration. " ;
	rdfs:subClassOf osdu:MasterData ;
	rdfs:subClassOf osdu:AbstractCommonResources ;
.

###  https://w3id.org/osdu#WellProductType
osdu:WellProductType rdf:type owl:Class ;
	rdfs:comment "Product Type [Well Product Type] is the physical product(s) that can be attributed to any well component. " ;
	rdfs:subClassOf osdu:ReferenceData ;
	rdfs:subClassOf osdu:AbstractCommonResources ;
	rdfs:subClassOf osdu:AbstractReferenceType ;
.

###  https://w3id.org/osdu#WellRole
osdu:WellRole rdf:type owl:Class ;
	rdfs:comment "Role [Well Role] is the current purpose, whether planned or actual. If there are multiple Roles among a well’s components, the well may be assigned the facet value with the highest significance. The value of Role may change over the Life Cycle. " ;
	rdfs:subClassOf osdu:ReferenceData ;
	rdfs:subClassOf osdu:AbstractCommonResources ;
	rdfs:subClassOf osdu:AbstractReferenceType ;
.

###  https://w3id.org/osdu#WellSiteProductType
osdu:WellSiteProductType rdf:type owl:Class ;
	rdfs:comment "Type of product produced in context of the well site. " ;
	rdfs:subClassOf osdu:ReferenceData ;
	rdfs:subClassOf osdu:AbstractCommonResources ;
	rdfs:subClassOf osdu:AbstractReferenceType ;
.

###  https://w3id.org/osdu#WellStatusSummary
osdu:WellStatusSummary rdf:type owl:Class ;
	rdfs:comment "Identifies the status of a well component in a way that may combine and-or summarize concepts found in other status facets. For example, a Well Status Summary of Gas Injector Shut-in, which contains commonly desired business information, combines concepts from Product Type, Fluid Direction, and Condition. " ;
	rdfs:subClassOf osdu:ReferenceData ;
	rdfs:subClassOf osdu:AbstractCommonResources ;
	rdfs:subClassOf osdu:AbstractReferenceType ;
.

###  https://w3id.org/osdu#Wellbore
osdu:Wellbore rdf:type owl:Class ;
	rdfs:comment "A hole in the ground extending from a point at the earth's surface to the maximum point of penetration. " ;
	rdfs:subClassOf osdu:MasterData ;
	rdfs:subClassOf osdu:AbstractCommonResources ;
	rdfs:subClassOf osdu:AbstractMaster ;
	rdfs:subClassOf osdu:AbstractFacility ;
.

###  https://w3id.org/osdu#WellboreArchitecture
osdu:WellboreArchitecture rdf:type owl:Class ;
	rdfs:comment "Describes the physical structures for a borehole " ;
	rdfs:subClassOf osdu:MasterData ;
	rdfs:subClassOf osdu:AbstractCommonResources ;
	rdfs:subClassOf osdu:AbstractMaster ;
.

###  https://w3id.org/osdu#WellboreIntervalSet
osdu:WellboreIntervalSet rdf:type owl:Class ;
	rdfs:comment "Define the geologic unit (including stratigraphic units) or fluid intervals along the wellbore, independent or based on markers  (defined in one or several WellboreMarkerSets). " ;
	rdfs:subClassOf osdu:WorkProductComponent ;
	rdfs:subClassOf osdu:AbstractCommonResources ;
	rdfs:subClassOf osdu:AbstractWPCGroupType ;
	rdfs:subClassOf osdu:AbstractWorkProductComponent ;
.

###  https://w3id.org/osdu#WellboreMarkerSet
osdu:WellboreMarkerSet rdf:type owl:Class ;
	rdfs:comment "Wellbore Markers identify the depth in a wellbore, measured below a reference elevation, at which a person or an automated process identifies a noteworthy observation, which is usually a change in the rock that intersects that wellbore. Formation Marker data includes attributes/properties that put these depths in context. Formation Markers are sometimes known as picks or formation tops. " ;
	rdfs:subClassOf osdu:WorkProductComponent ;
	rdfs:subClassOf osdu:AbstractCommonResources ;
	rdfs:subClassOf osdu:AbstractWPCGroupType ;
	rdfs:subClassOf osdu:AbstractWorkProductComponent ;
.

###  https://w3id.org/osdu#WellboreTrajectory
osdu:WellboreTrajectory rdf:type owl:Class ;
	rdfs:comment "Work Product Component describing an individual instance of a wellbore trajectory data object. Also called a deviation survey, wellbore trajectory is data that is used to calculate the position and spatial uncertainty of a planned or actual wellbore in 2-dimensional and 3-dimensional space. " ;
	rdfs:subClassOf osdu:WorkProductComponent ;
	rdfs:subClassOf osdu:AbstractCommonResources ;
	rdfs:subClassOf osdu:AbstractWPCGroupType ;
	rdfs:subClassOf osdu:AbstractWorkProductComponent ;
.

###  https://w3id.org/osdu#WellboreTrajectoryType
osdu:WellboreTrajectoryType rdf:type owl:Class ;
	rdfs:comment "Profile Type [Well Profile Type, Wellbore Trajectory Type] is the general geometry of the wellbore relative to the vertical plane. The specific criteria may vary by operator or regulator. The facet value may change if conditions encountered during drilling are not what was planned or permitted. " ;
	rdfs:subClassOf osdu:ReferenceData ;
	rdfs:subClassOf osdu:AbstractCommonResources ;
	rdfs:subClassOf osdu:AbstractReferenceType ;
.

###  https://w3id.org/osdu#WordFormatType
osdu:WordFormatType rdf:type owl:Class ;
	rdfs:comment "Reference data for primitive data format types which describe the computer interpretation of a storage word, such as Integer, Float. " ;
	rdfs:subClassOf osdu:ReferenceData ;
	rdfs:subClassOf osdu:AbstractCommonResources ;
	rdfs:subClassOf osdu:AbstractReferenceType ;
.

###  https://w3id.org/osdu#WorkProduct
osdu:WorkProduct rdf:type owl:Class ;
	rdfs:comment "A collection of work product components such as might be produced by a business activity and which is delivered to the data platform for loading. " ;
	rdfs:subClassOf osdu:AbstractCommonResources ;
	rdfs:subClassOf osdu:System ;
.

###  https://w3id.org/osdu#WorkProductComponent
osdu:WorkProductComponent rdf:type owl:Class ;
	rdfs:subClassOf osdu:System ;
.

###  https://w3id.org/osdu#Workflow
osdu:Workflow rdf:type owl:Class ;
	rdfs:comment "A workflow configuration in the context of a scheduled job. " ;
	rdfs:subClassOf owl:Thing ;
	rdfs:subClassOf [
		a owl:Restriction ;
		owl:onProperty osdu:securitySchemeName ;
		owl:minCardinality "1"^^xsd:nonNegativeInteger ;
	] ;
.

###  https://w3id.org/osdu#WorkflowParameter
osdu:WorkflowParameter rdf:type owl:Class ;
	skos:prefLabel "Workflow Parameter" ;
	rdfs:comment "Parameter name value pair. " ;
	rdfs:subClassOf owl:Thing ;
.

###  https://w3id.org/osdu#WorkflowPersonaType
osdu:WorkflowPersonaType rdf:type owl:Class ;
	rdfs:comment "Name of the role or personas that the record is technical assurance value is valid or not valid for. " ;
	rdfs:subClassOf osdu:ReferenceData ;
	rdfs:subClassOf osdu:AbstractCommonResources ;
	rdfs:subClassOf osdu:AbstractReferenceType ;
.

###  https://w3id.org/osdu#WorkflowUsageType
osdu:WorkflowUsageType rdf:type owl:Class ;
	rdfs:comment "Describes the workflows that the technical assurance value is valid or not valid for. " ;
	rdfs:subClassOf osdu:ReferenceData ;
	rdfs:subClassOf osdu:AbstractCommonResources ;
	rdfs:subClassOf osdu:AbstractReferenceType ;
.

###  https://w3id.org/osdu#WorldFile
osdu:WorldFile rdf:type owl:Class ;
	skos:prefLabel "File.Image.WorldFile" ;
	rdfs:comment "A file accompanying a File.Image.JPEG, File.Image.PNG or File.Image.TIFF containing the original pixel to 'world' coordinate transformation instructions. Typical file extensions are .jgw, .j2w, .pgw, .tfw, depending on the image type in context. " ;
	rdfs:subClassOf osdu:Dataset ;
	rdfs:subClassOf osdu:AbstractCommonResources ;
	rdfs:subClassOf osdu:AbstractDataset ;
	rdfs:subClassOf osdu:AbstractFile ;
.


#################################################################
#    Object Properties
#################################################################

###  https://w3id.org/osdu#abcdDBinGridLocalCoordinates
osdu:abcdBinGridLocalCoordinates rdf:type owl:ObjectProperty ;
	rdfs:comment "Reference to the ABCDBinGridLocalCoordinates for the object " ;
	rdfs:domain osdu:AbstractBinGrid ;
	rdfs:range osdu:AbstractCoordinates ;
.

###  https://w3id.org/osdu#basinNameAliases
osdu:basinNameAliases rdf:type owl:ObjectProperty ;
	rdfs:comment "Reference to the BasinNameAliases for the object " ;
	rdfs:domain osdu:Basin ;
	rdfs:range osdu:AbstractAliasNames ;
.

###  https://w3id.org/osdu#columns
osdu:columns rdf:type owl:ObjectProperty ;
	rdfs:comment "Reference to the Columns for the object " ;
	rdfs:domain [
		rdf:type owl:Class ;
		owl:unionOf (
			osdu:AbstractColumnBasedTable
			osdu:ColumnBasedTable
			osdu:ColumnBasedTableType
		) ;
	] ;
	rdfs:range osdu:AbstractReferencePropertyType ;
.

###  https://w3id.org/osdu#connectionSet
osdu:connectionSet rdf:type owl:ObjectProperty ;
	rdfs:comment "Reference to the ConnectionSet for the object " ;
	rdfs:domain osdu:IjkGridNumericalAquiferRepresentation ;
	rdfs:range osdu:AbstractIjkGridFlowSimulationBoundaryConnection ;
.

###  https://w3id.org/osdu#coordinate
osdu:coordinate rdf:type owl:ObjectProperty ;
	rdfs:comment "Reference to the coordinates for the object " ;
	rdfs:domain [
		rdf:type owl:Class ;
		owl:unionOf (
			osdu:AnyCrsGeoJSONPoint
			osdu:AnyCrsGeoJSONLineString
		) ;
	] ;
	 rdfs:range [
		rdf:type owl:Class ;
		owl:unionOf (
			xsd:decimal
			osdu:AnyCrsGeoJSONLineStringCoordinatesArray
		) ;
	] ;
.

###  https://w3id.org/osdu#hasDatasetProperties
osdu:hasDatasetProperties rdf:type owl:ObjectProperty ;
	rdfs:comment "Reference to the DatasetProperties for the object " ;
	rdfs:domain osdu:AbstractDataset ;
	rdfs:range owl:Thing ;
.

###  https://w3id.org/osdu#drillingReasons
osdu:drillingReasons rdf:type owl:ObjectProperty ;
	rdfs:comment "Reference to the DrillingReasons for the object " ;
	rdfs:domain osdu:Wellbore ;
	rdfs:range osdu:AbstractWellboreDrillingReason ;
.

###  https://w3id.org/osdu#extensionProperties
osdu:extensionProperties rdf:type owl:ObjectProperty ;
	rdfs:comment "Reference to the ExtensionProperties for the object " ;
	rdfs:domain osdu:Generic ;
	rdfs:range owl:Thing ;
.

###  https://w3id.org/osdu#facetIDs
osdu:facetIDs rdf:type owl:ObjectProperty ;
	rdfs:comment "Reference to the FacetIDs for the object " ;
	rdfs:domain osdu:AbstractReferencePropertyType ;
	rdfs:range osdu:AbstractFacet ;
.

###  https://w3id.org/osdu#facilityEvents
osdu:facilityEvents rdf:type owl:ObjectProperty ;
	rdfs:comment "Reference to the FacilityEvents for the object " ;
	rdfs:domain osdu:AbstractFacility ;
	rdfs:range osdu:AbstractFacilityEvent ;
.

###  https://w3id.org/osdu#facilityNameAliases
osdu:facilityNameAliases rdf:type owl:ObjectProperty ;
	rdfs:comment "Reference to the FacilityNameAliases for the object " ;
	rdfs:domain osdu:AbstractFacility ;
	rdfs:range osdu:AbstractAliasNames ;
.

###  https://w3id.org/osdu#facilityOperators
osdu:facilityOperators rdf:type owl:ObjectProperty ;
	rdfs:comment "Reference to the FacilityOperators for the object " ;
	rdfs:domain osdu:AbstractFacility ;
	rdfs:range osdu:AbstractFacilityOperator ;
.

###  https://w3id.org/osdu#facilitySpecifications
osdu:facilitySpecifications rdf:type owl:ObjectProperty ;
	rdfs:comment "Reference to the FacilitySpecifications for the object " ;
	rdfs:domain osdu:AbstractFacility ;
	rdfs:range osdu:AbstractFacilitySpecification ;
.

###  https://w3id.org/osdu#facilityStates
osdu:facilityStates rdf:type owl:ObjectProperty ;
	rdfs:comment "Reference to the FacilityStates for the object " ;
	rdfs:domain osdu:AbstractFacility ;
	rdfs:range osdu:AbstractFacilityState ;
.

###  https://w3id.org/osdu#fieldNameAliases
osdu:fieldNameAliases rdf:type owl:ObjectProperty ;
	rdfs:comment "Reference to the FieldNameAliases for the object " ;
	rdfs:domain osdu:Field ;
	rdfs:range osdu:AbstractAliasNames ;
.

###  https://w3id.org/osdu#fileSourceInfos
osdu:fileSourceInfos rdf:type owl:ObjectProperty ;
	rdfs:comment "Reference to the FileSourceInfos for the object " ;
	rdfs:domain osdu:DatasetProperties ;
	rdfs:range osdu:AbstractFileSourceInfo ;
.

###  https://w3id.org/osdu#geoContexts
osdu:geoContexts rdf:type owl:ObjectProperty ;
	rdfs:comment "Reference to the GeoContexts for the object " ;
	rdfs:domain [
		rdf:type owl:Class ;
		owl:unionOf (
			osdu:AbstractMaster
			osdu:AbstractWorkProductComponent
		) ;
	] ;
	rdfs:range osdu:AbstractGeoContext ;
.

###  https://w3id.org/osdu#geoPoliticalEntityNameAliases
osdu:geoPoliticalEntityNameAliases rdf:type owl:ObjectProperty ;
	rdfs:comment "Reference to the GeoPoliticalEntityNameAliases for the object " ;
	rdfs:domain osdu:GeoPoliticalEntity ;
	rdfs:range osdu:AbstractAliasNames ;
.

###  https://w3id.org/osdu#geometry
osdu:geometry rdf:type owl:ObjectProperty ;
	rdfs:domain [
		rdf:type owl:Class ;
		owl:unionOf (
			osdu:AnyCrsGeoJSONFeature
			osdu:GeoJSONFeature
		) ;
	] ;
	 rdfs:range [
		rdf:type owl:Class ;
		owl:unionOf (
			owl:Thing
			osdu:AnyCrsGeoJSONGeometryCollection
			osdu:AnyCrsGeoJSONPoint
			osdu:AnyCrsGeoJSONLineString
			osdu:AnyCrsGeoJSONPolygon
			osdu:AnyCrsGeoJSONMultiPoint
			osdu:AnyCrsGeoJSONMultiLineString
			osdu:AnyCrsGeoJSONMultiPolygon
			osdu:AnyCrsGeoJSONGeometryCollection
			osdu:GeoJSONPoint
			osdu:GeoJSONLineString
			osdu:GeoJSONPolygon
			osdu:GeoJSONMultiPoint
			osdu:GeoJSONMultiLineString
			osdu:GeoJSONMultiPolygon
			osdu:GeoJSONGeometryCollection
		) ;
	] ;
.

###  https://w3id.org/osdu#hasABCDBinGridSpatialLocation
osdu:hasABCDBinGridSpatialLocation rdf:type owl:ObjectProperty ;
	rdfs:comment "Reference to the ABCDBinGridSpatialLocation for the object " ;
	rdfs:domain osdu:AbstractBinGrid ;
	rdfs:range osdu:AbstractSpatialLocation ;
.

###  https://w3id.org/osdu#hasAcceptableUsage
osdu:hasAcceptableUsage rdf:type owl:ObjectProperty ;
	rdfs:comment "Reference to the AcceptableUsage for the object " ;
	rdfs:domain osdu:AbstractTechnicalAssurance ;
	rdfs:range osdu:AcceptableUsage ;
.

###  https://w3id.org/osdu#hasAcl
osdu:hasAcl rdf:type owl:ObjectProperty ;
	rdfs:comment "Reference to the Acl for the object " ;
	rdfs:domain osdu:System ;
	rdfs:range osdu:ACL ;
.

###  https://w3id.org/osdu#hasAcquisitionDateRanges
osdu:hasAcquisitionDateRanges rdf:type owl:ObjectProperty ;
	rdfs:comment "Reference to the AcquisitionDateRanges for the object " ;
	rdfs:domain osdu:ProcessedInSAR ;
	rdfs:range osdu:AcquisitionDateRanges ;
.

###  https://w3id.org/osdu#hasActivityArcs
osdu:hasActivityArcs rdf:type owl:ObjectProperty ;
	rdfs:comment "Reference to the ActivityArcs for the object " ;
	rdfs:domain osdu:ActivityTemplateArc ;
	rdfs:range osdu:Arc ;
.

###  https://w3id.org/osdu#hasActivityCode
osdu:hasActivityCode rdf:type owl:ObjectProperty ;
	rdfs:comment "Reference to the ActivityCode for the object " ;
	rdfs:domain [
		rdf:type owl:Class ;
		owl:unionOf (
			osdu:DrillingActivity
			osdu:WellPlanningActivity
		) ;
	] ;
	rdfs:range osdu:ActivityCode ;
.

###  https://w3id.org/osdu#hasActivityLevel
osdu:hasActivityLevel rdf:type owl:ObjectProperty ;
	rdfs:comment "Reference to the ActivityLevel for the object " ;
	rdfs:domain osdu:ActivityCode ;
	rdfs:range osdu:ActivityLevel ;
.

###  https://w3id.org/osdu#hasActivityOutcome
osdu:hasActivityOutcome rdf:type owl:ObjectProperty ;
	rdfs:comment "Reference to the ActivityOutcome for the object " ;
	rdfs:domain osdu:DrillingActivity ;
	rdfs:range osdu:ActivityOutcome ;
.

###  https://w3id.org/osdu#hasActivityOutcomeDetail
osdu:hasActivityOutcomeDetail rdf:type owl:ObjectProperty ;
	rdfs:comment "Reference to the ActivityOutcomeDetail for the object " ;
	rdfs:domain osdu:DrillingActivity ;
	rdfs:range osdu:ActivityOutcomeDetail ;
.

###  https://w3id.org/osdu#hasActivityPlan
osdu:hasActivityPlan rdf:type owl:ObjectProperty ;
	rdfs:comment "Reference to the ActivityPlan for the object " ;
	rdfs:domain osdu:Phase ;
	rdfs:range osdu:ActivityPlan ;
.

###  https://w3id.org/osdu#hasActivityTemplate
osdu:hasActivityTemplate rdf:type owl:ObjectProperty ;
	rdfs:comment "Reference to the ActivityTemplate for the object " ;
	rdfs:domain [
		rdf:type owl:Class ;
		owl:unionOf (
			osdu:AbstractProjectActivity
			osdu:AbstractWPCActivity
			osdu:Arc
		) ;
	] ;
	rdfs:range osdu:ActivityTemplate ;
.

###  https://w3id.org/osdu#hasActivityType
osdu:hasActivityType rdf:type owl:ObjectProperty ;
	rdfs:comment "Reference to the ActivityType for the object " ;
	rdfs:domain osdu:TubularAssembly ;
	rdfs:range osdu:ActivityType ;
.

###  https://w3id.org/osdu#hasAdditiveType
osdu:hasAdditiveType rdf:type owl:ObjectProperty ;
	rdfs:comment "Reference to the AdditiveType for the object " ;
	rdfs:domain osdu:CementAdditive ;
	rdfs:range osdu:AdditiveType ;
.

###  https://w3id.org/osdu#hasAgreement
osdu:hasAgreement rdf:type owl:ObjectProperty ;
	rdfs:comment "Reference to the Agreement for the object " ;
	rdfs:domain osdu:Agreement ;
	rdfs:range osdu:Agreement ;
.

###  https://w3id.org/osdu#hasAgreementType
osdu:hasAgreementType rdf:type owl:ObjectProperty ;
	rdfs:comment "Reference to the AgreementType for the object " ;
	rdfs:domain osdu:Agreement ;
	rdfs:range osdu:AgreementType ;
.

###  https://w3id.org/osdu#hasAliasNameType
osdu:hasAliasNameType rdf:type owl:ObjectProperty ;
	rdfs:comment "Reference to the AliasNameType for the object " ;
	rdfs:domain osdu:AbstractAliasNames ;
	rdfs:range osdu:AliasNameType ;
.

###  https://w3id.org/osdu#hasAliasNameTypeClass
osdu:hasAliasNameTypeClass rdf:type owl:ObjectProperty ;
	rdfs:comment "Reference to the AliasNameTypeClass for the object " ;
	rdfs:domain osdu:AliasNameType ;
	rdfs:range osdu:AliasNameTypeClass ;
.

###  https://w3id.org/osdu#hasAncestry
osdu:hasAncestry rdf:type owl:ObjectProperty ;
	rdfs:comment "Reference to the Ancestry for the object " ;
	rdfs:domain osdu:System ;
	rdfs:range osdu:AbstractLegalParentList ;
.

###  https://w3id.org/osdu#hasAnnularFluidType
osdu:hasAnnularFluidType rdf:type owl:ObjectProperty ;
	rdfs:comment "Reference to the AnnularFluidType for the object " ;
	rdfs:domain osdu:PerforationJob ;
	rdfs:range osdu:AnnularFluidType ;
.

###  https://w3id.org/osdu#hasAquiferInterpretation
osdu:hasAquiferInterpretation rdf:type owl:ObjectProperty ;
	rdfs:comment "Reference to the AquiferInterpretation for the object " ;
	rdfs:domain osdu:IjkGridNumericalAquiferRepresentation ;
	rdfs:range osdu:AquiferInterpretation ;
.

###  https://w3id.org/osdu#hasArtefactRole
osdu:hasArtefactRole rdf:type owl:ObjectProperty ;
	rdfs:comment "Reference to the ArtefactRole for the object " ;
	rdfs:domain osdu:Artefacts ;
	rdfs:range osdu:ArtefactRole ;
.

###  https://w3id.org/osdu#hasArtefacts
osdu:hasArtefacts rdf:type owl:ObjectProperty ;
	rdfs:comment "Reference to the Artefacts for the object " ;
	rdfs:domain osdu:AbstractWPCGroupType ;
	rdfs:range osdu:Artefacts ;
.

###  https://w3id.org/osdu#hasArtificialLiftType
osdu:hasArtificialLiftType rdf:type owl:ObjectProperty ;
	rdfs:comment "Reference to the ArtificialLiftType for the object " ;
	rdfs:domain osdu:TubularAssembly ;
	rdfs:range osdu:ArtificialLiftType ;
.

###  https://w3id.org/osdu#hasAsIngestedCoordinates
osdu:hasAsIngestedCoordinates rdf:type owl:ObjectProperty ;
	rdfs:comment "Reference to the AsIngestedCoordinates for the object " ;
	rdfs:domain osdu:AbstractSpatialLocation ;
	rdfs:range osdu:AbstractAnyCrsFeatureCollection ;
.

###  https://w3id.org/osdu#hasAuthorityCode
osdu:hasAuthorityCode rdf:type owl:ObjectProperty ;
	rdfs:comment "Reference to the AuthorityCode for the object " ;
	rdfs:domain [
		rdf:type owl:Class ;
		owl:unionOf (
			osdu:Method
			osdu:ConcatenatedTransformation
			osdu:SourceCRS
			osdu:TargetCRS
			osdu:Usage
			osdu:Extent
			osdu:Scope
			osdu:PreferredUsage
			osdu:HorizontalCRS
			osdu:VerticalCRS
			osdu:Transformation
			osdu:Datum
			osdu:DatumEnsemble
			osdu:Projection
			osdu:BaseCRS
			osdu:CoordinateSystem
		) ;
	] ;
	rdfs:range osdu:AuthorityCode ;
.

###  https://w3id.org/osdu#hasAvailableMarkerProperties
osdu:hasAvailableMarkerProperties rdf:type owl:ObjectProperty ;
	rdfs:comment "Reference to the AvailableMarkerProperties for the object " ;
	rdfs:domain osdu:WellboreMarkerSet ;
	rdfs:range osdu:MarkerProperty ;
.

###  https://w3id.org/osdu#hasAvailableTrajectoryStationProperties
osdu:hasAvailableTrajectoryStationProperties rdf:type owl:ObjectProperty ;
	rdfs:comment "Reference to the AvailableTrajectoryStationProperties for the object " ;
	rdfs:domain osdu:WellboreTrajectory ;
	rdfs:range osdu:Curve ;
.

###  https://w3id.org/osdu#hasBarrelFormulation
osdu:hasBarrelFormulation rdf:type owl:ObjectProperty ;
	rdfs:comment "Reference to the BarrelFormulation for the object " ;
	rdfs:domain osdu:FluidsSystem ;
	rdfs:range osdu:BarrelFormulation ;
.

###  https://w3id.org/osdu#hasBaseCRS
osdu:hasBaseCRS rdf:type owl:ObjectProperty ;
	rdfs:comment "Reference to the BaseCRS for the object " ;
	rdfs:domain osdu:CoordinateReferenceSystem ;
	rdfs:range osdu:BaseCRS ;
.

###  https://w3id.org/osdu#hasBasin
osdu:hasBasin rdf:type owl:ObjectProperty ;
	rdfs:comment "Reference to the Basin for the object " ;
	rdfs:domain [
		rdf:type owl:Class ;
		owl:unionOf (
			osdu:AbstractGeoBasinContext
			osdu:Basin
		) ;
	] ;
	rdfs:range osdu:Basin ;
.

###  https://w3id.org/osdu#hasBasinType
osdu:hasBasinType rdf:type owl:ObjectProperty ;
	rdfs:comment "Reference to the BasinType for the object " ;
	rdfs:domain [
		rdf:type owl:Class ;
		owl:unionOf (
			osdu:AbstractGeoBasinContext
			osdu:Basin
		) ;
	] ;
	rdfs:range osdu:BasinType ;
.

###  https://w3id.org/osdu#hasBhaStatus
osdu:hasBhaStatus rdf:type owl:ObjectProperty ;
	rdfs:comment "Reference to the BhaStatus for the object " ;
	rdfs:domain osdu:BHARun ;
	rdfs:range osdu:BhaStatus ;
.

###  https://w3id.org/osdu#hasBinGridDefinitionMethodType
osdu:hasBinGridDefinitionMethodType rdf:type owl:ObjectProperty ;
	rdfs:comment "Reference to the BinGridDefinitionMethodType for the object " ;
	rdfs:domain osdu:AbstractBinGrid ;
	rdfs:range osdu:BinGridDefinitionMethodType ;
.

###  https://w3id.org/osdu#hasBitRecord
osdu:hasBitRecord rdf:type owl:ObjectProperty ;
	rdfs:comment "Reference to the BitRecord for the object " ;
	rdfs:domain osdu:OperationsReport ;
	rdfs:range osdu:BitRecord ;
.

###  https://w3id.org/osdu#hasBottomHolePressureType
osdu:hasBottomHolePressureType rdf:type owl:ObjectProperty ;
	rdfs:comment "Reference to the BottomHolePressureType for the object " ;
	rdfs:domain osdu:PerforationInterval ;
	rdfs:range osdu:BottomHolePressureType ;
.

###  https://w3id.org/osdu#hasBoundaryFeature
osdu:hasBoundaryFeature rdf:type owl:ObjectProperty ;
	rdfs:comment "Reference to the BoundaryFeature for the object " ;
	rdfs:domain [
		rdf:type owl:Class ;
		owl:unionOf (
			osdu:AbstractInterpretation
			osdu:LocalBoundaryFeature
		) ;
	] ;
	rdfs:range osdu:BoundaryFeature ;
.

###  https://w3id.org/osdu#hasBoundaryRelationType
osdu:hasBoundaryRelationType rdf:type owl:ObjectProperty ;
	rdfs:comment "Reference to the BoundaryRelationType for the object " ;
	rdfs:domain osdu:GeobodyBoundaryInterpretation ;
	rdfs:range osdu:BoundaryRelationType ;
.

###  https://w3id.org/osdu#hasBusinessRules
osdu:hasBusinessRules rdf:type owl:ObjectProperty ;
	rdfs:comment "Reference to the BusinessRules for the object " ;
	rdfs:domain osdu:DataQuality ;
	rdfs:range osdu:AbstractBusinessRule ;
.

###  https://w3id.org/osdu#hasCatalogMapStateType
osdu:hasCatalogMapStateType rdf:type owl:ObjectProperty ;
	rdfs:comment "Reference to the CatalogMapStateType for the object " ;
	rdfs:domain [
		rdf:type owl:Class ;
		owl:unionOf (
			osdu:ExternalUnitOfMeasure
			osdu:ExternalUnitQuantity
		) ;
	] ;
	rdfs:range osdu:CatalogMapStateType ;
.

###  https://w3id.org/osdu#hasCellShapeType
osdu:hasCellShapeType rdf:type owl:ObjectProperty ;
	rdfs:comment "Reference to the CellShapeType for the object " ;
	rdfs:domain osdu:AbstractUnstructuredGridPatch ;
	rdfs:range osdu:CellShapeType ;
.

###  https://w3id.org/osdu#hasCementAdditives
osdu:hasCementAdditives rdf:type owl:ObjectProperty ;
	rdfs:comment "Reference to the CementAdditives for the object " ;
	rdfs:domain osdu:CementingFluid ;
	rdfs:range osdu:CementAdditive ;
.

###  https://w3id.org/osdu#hasCementJobType
osdu:hasCementJobType rdf:type owl:ObjectProperty ;
	rdfs:comment "Reference to the CementJobType for the object " ;
	rdfs:domain osdu:PlannedCementJob ;
	rdfs:range osdu:CementJobType ;
.

###  https://w3id.org/osdu#hasCementPumpSchedule
osdu:hasCementPumpSchedule rdf:type owl:ObjectProperty ;
	rdfs:comment "Reference to the CementPumpSchedule for the object " ;
	rdfs:domain osdu:CementingFluid ;
	rdfs:range osdu:CementPumpSchedule ;
.

###  https://w3id.org/osdu#hasCementStages
osdu:hasCementStages rdf:type owl:ObjectProperty ;
	rdfs:comment "Reference to the CementStages for the object " ;
	rdfs:domain osdu:PlannedCementJob ;
	rdfs:range osdu:CementStage ;
.

###  https://w3id.org/osdu#hasCementingFluid
osdu:hasCementingFluid rdf:type owl:ObjectProperty ;
	rdfs:comment "Reference to the CementingFluid for the object " ;
	rdfs:domain osdu:CementStage ;
	rdfs:range osdu:CementingFluid ;
.

###  https://w3id.org/osdu#hasCollectionPurpose
osdu:hasCollectionPurpose rdf:type owl:ObjectProperty ;
	rdfs:comment "Reference to the CollectionPurpose for the object " ;
	rdfs:domain osdu:PersistedCollection ;
	rdfs:range osdu:CollectionPurpose ;
.

###  https://w3id.org/osdu#hasColumnBasedTable
osdu:hasColumnBasedTable rdf:type owl:ObjectProperty ;
	rdfs:comment "Reference to the ColumnBasedTable for the object " ;
	rdfs:domain osdu:GenericProperty ;
	rdfs:range osdu:ColumnBasedTable ;
.

###  https://w3id.org/osdu#hasColumnShapeType
osdu:hasColumnShapeType rdf:type owl:ObjectProperty ;
	rdfs:comment "Reference to the ColumnShapeType for the object " ;
	rdfs:domain osdu:AbstractUnstructuredColumnLayerGridPatch ;
	rdfs:range osdu:ColumnShapeType ;
.

###  https://w3id.org/osdu#hasColumnValues
osdu:hasColumnValues rdf:type owl:ObjectProperty ;
	rdfs:comment "Reference to the ColumnValues for the object " ;
	rdfs:domain [
		rdf:type owl:Class ;
		owl:unionOf (
			osdu:AbstractColumnBasedTable
			osdu:ColumnBasedTable
		) ;
	] ;
	rdfs:range osdu:Columnvalues ;
.

###  https://w3id.org/osdu#hasComponentVolumesTestSystem
osdu:hasComponentVolumesTestSystem rdf:type owl:ObjectProperty ;
	rdfs:comment "Reference to the ComponentVolumesTestSystem for the object " ;
	rdfs:domain osdu:WBETestStep ;
	rdfs:range osdu:ComponentVolumesTestSystem ;
.

###  https://w3id.org/osdu#hasCompressionMethodType
osdu:hasCompressionMethodType rdf:type owl:ObjectProperty ;
	rdfs:comment "Reference to the CompressionMethodType for the object " ;
	rdfs:domain osdu:AbstractCompressionInfo ;
	rdfs:range osdu:CompressionMethodType ;
.

###  https://w3id.org/osdu#hasConcatenatedTransformations
osdu:hasConcatenatedTransformations rdf:type owl:ObjectProperty ;
	rdfs:comment "Reference to the ConcatenatedTransformations for the object " ;
	rdfs:domain osdu:CoordinateTransformation ;
	rdfs:range osdu:ConcatenatedTransformation ;
.

###  https://w3id.org/osdu#hasConditions
osdu:hasConditions rdf:type owl:ObjectProperty ;
	rdfs:comment "Reference to the Conditions for the object " ;
	rdfs:domain osdu:RCAMeasurement ;
	rdfs:range osdu:Conditions ;
.

###  https://w3id.org/osdu#hasConfigurations
osdu:hasConfigurations rdf:type owl:ObjectProperty ;
	rdfs:comment "Reference to the Configurations for the object " ;
	rdfs:domain osdu:UnitOfMeasureConfiguration ;
	rdfs:range osdu:Configuration ;
.

###  https://w3id.org/osdu#hasConnectedSourceDataJob
osdu:hasConnectedSourceDataJob rdf:type owl:ObjectProperty ;
	rdfs:comment "Reference to the ConnectedSourceDataJob for the object " ;
	rdfs:domain osdu:DatasetProperties ;
	rdfs:range osdu:ConnectedSourceDataJob ;
.

###  https://w3id.org/osdu#hasConnectedSourceRegistryEntry
osdu:hasConnectedSourceRegistryEntry rdf:type owl:ObjectProperty ;
	rdfs:comment "Reference to the ConnectedSourceRegistryEntry for the object " ;
	rdfs:domain [
		rdf:type owl:Class ;
		owl:unionOf (
			osdu:DatasetProperties
			osdu:ConnectedSourceDataJob
		) ;
	] ;
	rdfs:range osdu:ConnectedSourceRegistryEntry ;
.

###  https://w3id.org/osdu#hasContactRoleType
osdu:hasContactRoleType rdf:type owl:ObjectProperty ;
	rdfs:comment "Reference to the ContactRoleType for the object " ;
	rdfs:domain osdu:AbstractContact ;
	rdfs:range osdu:ContactRoleType ;
.

###  https://w3id.org/osdu#hasContractorType
osdu:hasContractorType rdf:type owl:ObjectProperty ;
	rdfs:comment "Reference to the ContractorType for the object " ;
	rdfs:domain osdu:Contractors ;
	rdfs:range osdu:ContractorType ;
.

###  https://w3id.org/osdu#hasContractors
osdu:hasContractors rdf:type owl:ObjectProperty ;
	rdfs:comment "Reference to the Contractors for the object " ;
	rdfs:domain osdu:AbstractProject ;
	rdfs:range osdu:Contractors ;
.

###  https://w3id.org/osdu#hasCoordinateReferenceSystem
osdu:hasCoordinateReferenceSystem rdf:type owl:ObjectProperty ;
	rdfs:comment "Reference to the CoordinateReferenceSystem for the object " ;
	rdfs:domain [
		rdf:type owl:Class ;
		owl:unionOf (
			osdu:AbstractReferenceLevel
			osdu:AbstractAnyCrsFeatureCollection
			osdu:FrameOfReferenceCRS
			osdu:AbstractSpatialReference
			osdu:AbstractFacilityVerticalMeasurement
			osdu:GeoTIFF
			osdu:Well
			osdu:VelocityModeling
			osdu:SeismicTraceData
			osdu:WellboreTrajectory
			osdu:FaultSystem
			osdu:SeismicLineGeometry
			osdu:SourceCRS
			osdu:TargetCRS
			osdu:HorizontalCRS
			osdu:VerticalCRS
			osdu:BaseCRS
		) ;
	] ;
	rdfs:range osdu:CoordinateReferenceSystem ;
.

###  https://w3id.org/osdu#hasCoordinateSystem
osdu:hasCoordinateSystem rdf:type owl:ObjectProperty ;
	rdfs:comment "Reference to the CoordinateSystem for the object " ;
	rdfs:domain osdu:CoordinateReferenceSystem ;
	rdfs:range osdu:CoordinateSystem ;
.

###  https://w3id.org/osdu#hasCoordinateTransformation
osdu:hasCoordinateTransformation rdf:type owl:ObjectProperty ;
	rdfs:comment "Reference to the CoordinateTransformation for the object " ;
	rdfs:domain [
		rdf:type owl:Class ;
		owl:unionOf (
			osdu:ConcatenatedTransformation
			osdu:Transformation
		) ;
	] ;
	rdfs:range osdu:CoordinateTransformation ;
.

###  https://w3id.org/osdu#hasCorePreservationType
osdu:hasCorePreservationType rdf:type owl:ObjectProperty ;
	rdfs:comment "Reference to the CorePreservationType for the object " ;
	rdfs:domain [
		rdf:type owl:Class ;
		owl:unionOf (
			osdu:RockSample
			osdu:Coring
		) ;
	] ;
	rdfs:range osdu:CorePreservationType ;
.

###  https://w3id.org/osdu#hasCoreRemarks
osdu:hasCoreRemarks rdf:type owl:ObjectProperty ;
	rdfs:comment "Reference to the CoreRemarks for the object " ;
	rdfs:domain osdu:Coring ;
	rdfs:range osdu:CoreRemark ;
.

###  https://w3id.org/osdu#hasCoring
osdu:hasCoring rdf:type owl:ObjectProperty ;
	rdfs:comment "Reference to the Coring for the object " ;
	rdfs:domain [
		rdf:type owl:Class ;
		owl:unionOf (
			osdu:RockSample
			osdu:RockSampleAnalysis
		) ;
	] ;
	rdfs:range osdu:Coring ;
.

###  https://w3id.org/osdu#hasCost
osdu:hasCost rdf:type owl:ObjectProperty ;
	rdfs:comment "Reference to the Cost for the object " ;
	rdfs:domain osdu:OperationsReport ;
	rdfs:range osdu:Cost ;
.

###  https://w3id.org/osdu#hasCurrency
osdu:hasCurrency rdf:type owl:ObjectProperty ;
	rdfs:comment "Reference to the Currency for the object " ;
	rdfs:domain osdu:FundsAuthorizations ;
	rdfs:range osdu:Currency ;
.

###  https://w3id.org/osdu#hasCurveSampleType
osdu:hasCurveSampleType rdf:type owl:ObjectProperty ;
	rdfs:comment "Reference to the CurveSampleType for the object " ;
	rdfs:domain osdu:Curves ;
	rdfs:range osdu:CurveSampleType ;
.

###  https://w3id.org/osdu#hasCurves
osdu:hasCurves rdf:type owl:ObjectProperty ;
	rdfs:comment "Reference to the Curves for the object " ;
	rdfs:domain [
		rdf:type owl:Class ;
		owl:unionOf (
			osdu:WellLog
			osdu:PPFGDataset
		) ;
	] ;
	rdfs:range osdu:Curves ;
.

###  https://w3id.org/osdu#hasDataRuleDimensionType
osdu:hasDataRuleDimensionType rdf:type owl:ObjectProperty ;
	rdfs:comment "Reference to the DataRuleDimensionType for the object " ;
	rdfs:domain osdu:QualityDataRule ;
	rdfs:range osdu:DataRuleDimensionType ;
.

###  https://w3id.org/osdu#hasDataRuleSets
osdu:hasDataRuleSets rdf:type owl:ObjectProperty ;
	rdfs:comment "Reference to the DataRuleSets for the object " ;
	rdfs:domain osdu:AbstractBusinessRule ;
	rdfs:range osdu:DataRuleSets ;
.

###  https://w3id.org/osdu#hasDataRules
osdu:hasDataRules rdf:type owl:ObjectProperty ;
	rdfs:comment "Reference to the DataRules for the object " ;
	rdfs:domain [
		rdf:type owl:Class ;
		owl:unionOf (
			osdu:AbstractBusinessRule
			osdu:QualityDataRuleSet
		) ;
	] ;
	rdfs:range osdu:DataRule ;
.

###  https://w3id.org/osdu#hasDatasetProperties
osdu:hasDatasetProperties rdf:type owl:ObjectProperty ;
	rdfs:comment "Reference to the DatasetProperties for the object " ;
	rdfs:domain [
		rdf:type owl:Class ;
		owl:unionOf (
			osdu:AbstractFileCollection
			osdu:AbstractFile
			osdu:ETPDataspace
			osdu:Generic
		) ;
	] ;
	rdfs:range osdu:DatasetProperties ;
.

###  https://w3id.org/osdu#hasDatum
osdu:hasDatum rdf:type owl:ObjectProperty ;
	rdfs:comment "Reference to the Datum for the object " ;
	rdfs:domain osdu:CoordinateReferenceSystem ;
	rdfs:range osdu:Datum ;
.

###  https://w3id.org/osdu#hasDatumEnsemble
osdu:hasDatumEnsemble rdf:type owl:ObjectProperty ;
	rdfs:comment "Reference to the DatumEnsemble for the object " ;
	rdfs:domain osdu:CoordinateReferenceSystem ;
	rdfs:range osdu:DatumEnsemble ;
.

###  https://w3id.org/osdu#hasDefaultValue
osdu:hasDefaultValue rdf:type owl:ObjectProperty ;
	rdfs:comment "Reference to the DefaultValue for the object " ;
	rdfs:domain osdu:ParameterTemplate ;
	rdfs:range osdu:AbstractActivityParameter ;
.

###  https://w3id.org/osdu#hasDepositionGeometryType
osdu:hasDepositionGeometryType rdf:type owl:ObjectProperty ;
	rdfs:comment "Reference to the DepositionGeometryType for the object " ;
	rdfs:domain osdu:StratigraphicUnitInterpretation ;
	rdfs:range osdu:DepositionGeometryType ;
.

###  https://w3id.org/osdu#hasDepthRange
osdu:hasDepthRange rdf:type owl:ObjectProperty ;
	rdfs:comment "Reference to the DepthRange for the object " ;
	rdfs:domain osdu:WellPlanningActivity ;
	rdfs:range osdu:DepthRange ;
.

###  https://w3id.org/osdu#hasDocument
osdu:hasDocument rdf:type owl:ObjectProperty ;
	rdfs:comment "Reference to the Document for the object " ;
	rdfs:domain osdu:WBETestStep ;
	rdfs:range osdu:Document ;
.

###  https://w3id.org/osdu#hasDocumentType
osdu:hasDocumentType rdf:type owl:ObjectProperty ;
	rdfs:comment "Reference to the DocumentType for the object " ;
	rdfs:domain osdu:Document ;
	rdfs:range osdu:DocumentType ;
.

###  https://w3id.org/osdu#hasDomainType
osdu:hasDomainType rdf:type owl:ObjectProperty ;
	rdfs:comment "Reference to the DomainType for the object " ;
	rdfs:domain osdu:AbstractInterpretation ;
	rdfs:range osdu:DomainType ;
.

###  https://w3id.org/osdu#hasDownHoleMaximumRPM
osdu:hasDownHoleMaximumRPM rdf:type owl:ObjectProperty ;
	rdfs:comment "Reference to the DownHoleMaximumRPM for the object " ;
	rdfs:domain osdu:RPMGroup ;
	rdfs:range osdu:DownHoleMaximumRPM ;
.

###  https://w3id.org/osdu#hasDownHoleMinimumRPM
osdu:hasDownHoleMinimumRPM rdf:type owl:ObjectProperty ;
	rdfs:comment "Reference to the DownHoleMinimumRPM for the object " ;
	rdfs:domain osdu:RPMGroup ;
	rdfs:range osdu:DownHoleMinimumRPM ;
.

###  https://w3id.org/osdu#hasDownHoleRecommendedRPM
osdu:hasDownHoleRecommendedRPM rdf:type owl:ObjectProperty ;
	rdfs:comment "Reference to the DownHoleRecommendedRPM for the object " ;
	rdfs:domain osdu:RPMGroup ;
	rdfs:range osdu:DownHoleRecommendedRPM ;
.

###  https://w3id.org/osdu#hasDrillActivity
osdu:hasDrillActivity rdf:type owl:ObjectProperty ;
	rdfs:comment "Reference to the DrillActivity for the object " ;
	rdfs:domain osdu:OperationsReport ;
	rdfs:range osdu:DrillingActivity ;
.

###  https://w3id.org/osdu#hasDrillingActivityClassType
osdu:hasDrillingActivityClassType rdf:type owl:ObjectProperty ;
	rdfs:comment "Reference to the DrillingActivityClassType for the object " ;
	rdfs:domain osdu:DrillingActivity ;
	rdfs:range osdu:DrillingActivityClassType ;
.

###  https://w3id.org/osdu#hasDrillingParams
osdu:hasDrillingParams rdf:type owl:ObjectProperty ;
	rdfs:comment "Reference to the DrillingParams for the object " ;
	rdfs:domain osdu:BHARun ;
	rdfs:range osdu:DrillingParameters ;
.

###  https://w3id.org/osdu#hasDrillingReasonType
osdu:hasDrillingReasonType rdf:type owl:ObjectProperty ;
	rdfs:comment "Reference to the DrillingReasonType for the object " ;
	rdfs:domain osdu:AbstractWellboreDrillingReason ;
	rdfs:range osdu:DrillingReasonType ;
.

###  https://w3id.org/osdu#hasEarthModelInterpretation
osdu:hasEarthModelInterpretation rdf:type owl:ObjectProperty ;
	rdfs:comment "Reference to the EarthModelInterpretation for the object " ;
	rdfs:domain [
		rdf:type owl:Class ;
		owl:unionOf (
			osdu:AbstractRepresentation
			osdu:AbstractGridRepresentation
		) ;
	] ;
	rdfs:range osdu:EarthModelInterpretation ;
.

###  https://w3id.org/osdu#hasEmbeddedBinGrid
osdu:hasEmbeddedBinGrid rdf:type owl:ObjectProperty ;
	rdfs:comment "Reference to the EmbeddedBinGrid for the object " ;
	rdfs:domain osdu:GeoReferencedImage ;
	rdfs:range osdu:AbstractBinGrid ;
.

###  https://w3id.org/osdu#hasEmbeddedReferenceLevel
osdu:hasEmbeddedReferenceLevel rdf:type owl:ObjectProperty ;
	rdfs:comment "Reference to the EmbeddedReferenceLevel for the object " ;
	rdfs:domain osdu:GeoReferencedImage ;
	rdfs:range osdu:AbstractReferenceLevel ;
.

###  https://w3id.org/osdu#hasEncodingFormatType
osdu:hasEncodingFormatType rdf:type owl:ObjectProperty ;
	rdfs:comment "Reference to the EncodingFormatType for the object " ;
	rdfs:domain [
		rdf:type owl:Class ;
		owl:unionOf (
			osdu:AbstractDataset
			osdu:AbstractFileSourceInfo
		) ;
	] ;
	rdfs:range osdu:EncodingFormatType ;
.

###  https://w3id.org/osdu#hasEvaluationPlan
osdu:hasEvaluationPlan rdf:type owl:ObjectProperty ;
	rdfs:comment "Reference to the EvaluationPlan for the object " ;
	rdfs:domain osdu:Phase ;
	rdfs:range osdu:EvaluationPlan ;
.

###  https://w3id.org/osdu#hasExpectedVolumesBledBack
osdu:hasExpectedVolumesBledBack rdf:type owl:ObjectProperty ;
	rdfs:comment "Reference to the ExpectedVolumesBledBack for the object " ;
	rdfs:domain osdu:WBETestStep ;
	rdfs:range osdu:ExpectedVolume ;
.

###  https://w3id.org/osdu#hasExpectedVolumesPumped
osdu:hasExpectedVolumesPumped rdf:type owl:ObjectProperty ;
	rdfs:comment "Reference to the ExpectedVolumesPumped for the object " ;
	rdfs:domain osdu:WBETestStep ;
	rdfs:range osdu:ExpectedVolume ;
.

###  https://w3id.org/osdu#hasExtent
osdu:hasExtent rdf:type owl:ObjectProperty ;
	rdfs:comment "Reference to the Extent for the object " ;
	rdfs:domain [
		rdf:type owl:Class ;
		owl:unionOf (
			osdu:Usage
			osdu:PreferredUsage
		) ;
	] ;
	rdfs:range osdu:Extent ;
.

###  https://w3id.org/osdu#hasExternalCatalogNamespace
osdu:hasExternalCatalogNamespace rdf:type owl:ObjectProperty ;
	rdfs:comment "Reference to the ExternalCatalogNamespace for the object " ;
	rdfs:domain [
		rdf:type owl:Class ;
		owl:unionOf (
			osdu:ExternalUnitOfMeasure
			osdu:ExternalUnitQuantity
		) ;
	] ;
	rdfs:range osdu:ExternalCatalogNamespace ;
.

###  https://w3id.org/osdu#hasExternalUnitOfMeasure
osdu:hasExternalUnitOfMeasure rdf:type owl:ObjectProperty ;
	rdfs:comment "Reference to the ExternalUnitOfMeasure for the object " ;
	rdfs:domain osdu:ExternalUnitOfMeasure ;
	rdfs:range osdu:ExternalUnitOfMeasure ;
.

###  https://w3id.org/osdu#hasExternalUnitQuantity
osdu:hasExternalUnitQuantity rdf:type owl:ObjectProperty ;
	rdfs:comment "Reference to the ExternalUnitQuantity for the object " ;
	rdfs:domain osdu:ExternalUnitOfMeasure ;
	rdfs:range osdu:ExternalUnitQuantity ;
.

###  https://w3id.org/osdu#hasFacetRole
osdu:hasFacetRole rdf:type owl:ObjectProperty ;
	rdfs:comment "Reference to the FacetRole for the object " ;
	rdfs:domain osdu:AbstractFacet ;
	rdfs:range osdu:FacetRole ;
.

###  https://w3id.org/osdu#hasFacetType
osdu:hasFacetType rdf:type owl:ObjectProperty ;
	rdfs:comment "Reference to the FacetType for the object " ;
	rdfs:domain osdu:AbstractFacet ;
	rdfs:range osdu:FacetType ;
.

###  https://w3id.org/osdu#hasFacilityEventType
osdu:hasFacilityEventType rdf:type owl:ObjectProperty ;
	rdfs:comment "Reference to the FacilityEventType for the object " ;
	rdfs:domain osdu:AbstractFacilityEvent ;
	rdfs:range osdu:FacilityEventType ;
.

###  https://w3id.org/osdu#hasFacilityStateType
osdu:hasFacilityStateType rdf:type owl:ObjectProperty ;
	rdfs:comment "Reference to the FacilityStateType for the object " ;
	rdfs:domain [
		rdf:type owl:Class ;
		owl:unionOf (
			osdu:AbstractFacilityState
			osdu:WellStatusSummary
		) ;
	] ;
	rdfs:range osdu:FacilityStateType ;
.

###  https://w3id.org/osdu#hasFacilityType
osdu:hasFacilityType rdf:type owl:ObjectProperty ;
	rdfs:comment "Reference to the FacilityType for the object " ;
	rdfs:domain osdu:AbstractFacility ;
	rdfs:range osdu:FacilityType ;
.

###  https://w3id.org/osdu#hasFaultInterpretation
osdu:hasFaultInterpretation rdf:type owl:ObjectProperty ;
	rdfs:comment "Reference to the FaultInterpretation for the object " ;
	rdfs:domain osdu:Faults ;
	rdfs:range osdu:FaultInterpretation ;
.

###  https://w3id.org/osdu#hasFaultSystem
osdu:hasFaultSystem rdf:type owl:ObjectProperty ;
	rdfs:comment "Reference to the FaultSystem for the object " ;
	rdfs:domain osdu:UnsealedSurfaceFramework ;
	rdfs:range osdu:FaultSystem ;
.

###  https://w3id.org/osdu#hasFaultThrowDescriptions
osdu:hasFaultThrowDescriptions rdf:type owl:ObjectProperty ;
	rdfs:comment "Reference to the FaultThrowDescriptions for the object " ;
	rdfs:domain osdu:FaultInterpretation ;
	rdfs:range osdu:FaultThrowDescriptions ;
.

###  https://w3id.org/osdu#hasFaultThrowType
osdu:hasFaultThrowType rdf:type owl:ObjectProperty ;
	rdfs:comment "Reference to the FaultThrowType for the object " ;
	rdfs:domain osdu:FaultThrowDescriptions ;
	rdfs:range osdu:FaultThrowType ;
.

###  https://w3id.org/osdu#hasFaults
osdu:hasFaults rdf:type owl:ObjectProperty ;
	rdfs:comment "Reference to the Faults for the object " ;
	rdfs:domain osdu:FaultSystem ;
	rdfs:range osdu:Faults ;
.

###  https://w3id.org/osdu#hasFeatureType
osdu:hasFeatureType rdf:type owl:ObjectProperty ;
	rdfs:comment "Reference to the FeatureType for the object " ;
	rdfs:domain osdu:Markers ;
	rdfs:range osdu:FeatureType ;
.

###  https://w3id.org/osdu#hasFeatures
osdu:hasFeatures rdf:type owl:ObjectProperty ;
	rdfs:comment "Reference to the Features for the object " ;
	rdfs:domain [
		rdf:type owl:Class ;
		owl:unionOf (
			osdu:AbstractAnyCrsFeatureCollection
			osdu:AbstractFeatureCollection
		) ;
	] ;
	rdfs:range osdu:GeoJSONFeature ;
.

###  https://w3id.org/osdu#hasField
osdu:hasField rdf:type owl:ObjectProperty ;
	rdfs:comment "Reference to the Field for the object " ;
	rdfs:domain osdu:AbstractGeoFieldContext ;
	rdfs:range osdu:Field ;
.

###  https://w3id.org/osdu#hasFileSourceInfo
osdu:hasFileSourceInfo rdf:type owl:ObjectProperty ;
	rdfs:comment "Reference to the FileSourceInfo for the object " ;
	rdfs:domain osdu:DatasetProperties ;
	rdfs:range osdu:AbstractFileSourceInfo ;
.

###  https://w3id.org/osdu#hasFilterSpecification
osdu:hasFilterSpecification rdf:type owl:ObjectProperty ;
	rdfs:comment "Reference to the FilterSpecification for the object " ;
	rdfs:domain osdu:DataCollection ;
	rdfs:range osdu:FilterSpecification ;
.

###  https://w3id.org/osdu#hasFirstLocation
osdu:hasFirstLocation rdf:type owl:ObjectProperty ;
	rdfs:comment "Reference to the FirstLocation for the object " ;
	rdfs:domain osdu:SeismicLineGeometry ;
	rdfs:range osdu:AbstractSpatialLocation ;
.

###  https://w3id.org/osdu#hasFlowratePumpGroup
osdu:hasFlowratePumpGroup rdf:type owl:ObjectProperty ;
	rdfs:comment "Reference to the FlowratePumpGroup for the object " ;
	rdfs:domain osdu:OperationParameterPlan ;
	rdfs:range osdu:FlowratePumpGroup ;
.

###  https://w3id.org/osdu#hasFluid
osdu:hasFluid rdf:type owl:ObjectProperty ;
	rdfs:comment "Reference to the Fluid for the object " ;
	rdfs:domain osdu:FluidsReport ;
	rdfs:range osdu:Fluid ;
.

###  https://w3id.org/osdu#hasFluidFacets
osdu:hasFluidFacets rdf:type owl:ObjectProperty ;
	rdfs:comment "Reference to the FluidFacets for the object " ;
	rdfs:domain osdu:FluidsProperty ;
	rdfs:range osdu:FluidFacet ;
.

###  https://w3id.org/osdu#hasFluidIntervals
osdu:hasFluidIntervals rdf:type owl:ObjectProperty ;
	rdfs:comment "Reference to the FluidIntervals for the object " ;
	rdfs:domain osdu:FluidsProgram ;
	rdfs:range osdu:FluidsInterval ;
.

###  https://w3id.org/osdu#hasFluidPhaseType
osdu:hasFluidPhaseType rdf:type owl:ObjectProperty ;
	rdfs:comment "Reference to the FluidPhaseType for the object " ;
	rdfs:domain osdu:RockFluidUnitInterpretation ;
	rdfs:range osdu:FluidPhaseType ;
.

###  https://w3id.org/osdu#hasFluidProperties
osdu:hasFluidProperties rdf:type owl:ObjectProperty ;
	rdfs:comment "Reference to the FluidProperties for the object " ;
	rdfs:domain osdu:FluidsSystem ;
	rdfs:range osdu:FluidsProperty ;
.

###  https://w3id.org/osdu#hasFluidPropertyFacetName
osdu:hasFluidPropertyFacetName rdf:type owl:ObjectProperty ;
	rdfs:comment "Reference to the FluidPropertyFacetName for the object " ;
	rdfs:domain osdu:FluidFacet ;
	rdfs:range osdu:FluidPropertyFacetName ;
.

###  https://w3id.org/osdu#hasFluidPropertyName
osdu:hasFluidPropertyName rdf:type owl:ObjectProperty ;
	rdfs:comment "Reference to the FluidPropertyName for the object " ;
	rdfs:domain osdu:FluidsProperty ;
	rdfs:range osdu:FluidPropertyName ;
.

###  https://w3id.org/osdu#hasFluidRheologicalModelType
osdu:hasFluidRheologicalModelType rdf:type owl:ObjectProperty ;
	rdfs:comment "Reference to the FluidRheologicalModelType for the object " ;
	rdfs:domain osdu:CementingFluid ;
	rdfs:range osdu:FluidRheologicalModelType ;
.

###  https://w3id.org/osdu#hasFluidRole
osdu:hasFluidRole rdf:type owl:ObjectProperty ;
	rdfs:comment "Reference to the FluidRole for the object " ;
	rdfs:domain osdu:FluidsSystem ;
	rdfs:range osdu:FluidRole ;
.

###  https://w3id.org/osdu#hasFluidType
osdu:hasFluidType rdf:type owl:ObjectProperty ;
	rdfs:comment "Reference to the FluidType for the object " ;
	rdfs:domain [
		rdf:type owl:Class ;
		owl:unionOf (
			osdu:FluidsInterval
			osdu:TestFluid
		) ;
	] ;
	rdfs:range osdu:FluidType ;
.

###  https://w3id.org/osdu#hasFluidsSystem
osdu:hasFluidsSystem rdf:type owl:ObjectProperty ;
	rdfs:comment "Reference to the FluidsSystem for the object " ;
	rdfs:domain osdu:FluidsInterval ;
	rdfs:range osdu:FluidsSystem ;
.

###  https://w3id.org/osdu#hasFormationEvaluationCorings
osdu:hasFormationEvaluationCorings rdf:type owl:ObjectProperty ;
	rdfs:comment "Reference to the FormationEvaluationCorings for the object " ;
	rdfs:domain osdu:EvaluationPlan ;
	rdfs:range osdu:Core ;
.

###  https://w3id.org/osdu#hasFormationIntegrityEvaluations
osdu:hasFormationIntegrityEvaluations rdf:type owl:ObjectProperty ;
	rdfs:comment "Reference to the FormationIntegrityEvaluations for the object " ;
	rdfs:domain osdu:EvaluationPlan ;
	rdfs:range osdu:FormationIntegrityEvaluation ;
.

###  https://w3id.org/osdu#hasFundsAuthorizations
osdu:hasFundsAuthorizations rdf:type owl:ObjectProperty ;
	rdfs:comment "Reference to the FundsAuthorizations for the object " ;
	rdfs:domain osdu:AbstractProject ;
	rdfs:range osdu:FundsAuthorizations ;
.

###  https://w3id.org/osdu#hasGasReading
osdu:hasGasReading rdf:type owl:ObjectProperty ;
	rdfs:comment "Reference to the GasReading for the object " ;
	rdfs:domain osdu:OperationsReport ;
	rdfs:range osdu:GasReading ;
.

###  https://w3id.org/osdu#hasGenericRepresentation
osdu:hasGenericRepresentation rdf:type owl:ObjectProperty ;
	rdfs:comment "Reference to the GenericRepresentation for the object " ;
	rdfs:domain osdu:GenericProperty ;
	rdfs:range osdu:GenericRepresentation ;
.

###  https://w3id.org/osdu#hasGeoPoliticalEntity
osdu:hasGeoPoliticalEntity rdf:type owl:ObjectProperty ;
	rdfs:comment "Reference to the GeoPoliticalEntity for the object " ;
	rdfs:domain [
		rdf:type owl:Class ;
		owl:unionOf (
			osdu:AbstractGeoPoliticalContext
			osdu:GeoPoliticalEntity
			osdu:WellPlanningWell
		) ;
	] ;
	rdfs:range osdu:GeoPoliticalEntity ;
.

###  https://w3id.org/osdu#hasGeoPoliticalEntityType
osdu:hasGeoPoliticalEntityType rdf:type owl:ObjectProperty ;
	rdfs:comment "Reference to the GeoPoliticalEntityType for the object " ;
	rdfs:domain [
		rdf:type owl:Class ;
		owl:unionOf (
			osdu:AbstractGeoPoliticalContext
			osdu:GeoPoliticalEntity
		) ;
	] ;
	rdfs:range osdu:GeoPoliticalEntityType ;
.

###  https://w3id.org/osdu#hasGeoReferencedImageType
osdu:hasGeoReferencedImageType rdf:type owl:ObjectProperty ;
	rdfs:comment "Reference to the GeoReferencedImageType for the object " ;
	rdfs:domain osdu:GeoReferencedImage ;
	rdfs:range osdu:GeoReferencedImageType ;
.

###  https://w3id.org/osdu#hasGeobodyInterpretation
osdu:hasGeobodyInterpretation rdf:type owl:ObjectProperty ;
	rdfs:comment "Reference to the GeobodyInterpretation for the object " ;
	rdfs:domain osdu:ReservoirCompartmentUnit ;
	rdfs:range osdu:GeobodyInterpretation ;
.

###  https://w3id.org/osdu#hasGeographicBottomHoleLocation
osdu:hasGeographicBottomHoleLocation rdf:type owl:ObjectProperty ;
	rdfs:comment "Reference to the GeographicBottomHoleLocation for the object " ;
	rdfs:domain osdu:Wellbore ;
	rdfs:range osdu:AbstractSpatialLocation ;
.

###  https://w3id.org/osdu#hasGeologicUnitShapeType
osdu:hasGeologicUnitShapeType rdf:type owl:ObjectProperty ;
	rdfs:comment "Reference to the GeologicUnitShapeType for the object " ;
	rdfs:domain osdu:AbstractGeologicUnitInterpretation ;
	rdfs:range osdu:GeologicUnitShapeType ;
.

###  https://w3id.org/osdu#hasGeologyIntervals
osdu:hasGeologyIntervals rdf:type owl:ObjectProperty ;
	rdfs:comment "Reference to the GeologyIntervals for the object " ;
	rdfs:domain osdu:PlannedLithology ;
	rdfs:range osdu:GeologyInterval ;
.

###  https://w3id.org/osdu#hasGeometricTargetSet
osdu:hasGeometricTargetSet rdf:type owl:ObjectProperty ;
	rdfs:comment "Reference to the GeometricTargetSet for the object " ;
	rdfs:domain osdu:WellPlanningWellbore ;
	rdfs:range osdu:GeometricTargetSet ;
.

###  https://w3id.org/osdu#hasGeometry
osdu:hasGeometry rdf:type owl:ObjectProperty ;
	rdfs:comment "Reference to the Geometry for the object " ;
	rdfs:domain osdu:Target ;
	rdfs:range osdu:Geometry ;
.

###  https://w3id.org/osdu#hasGeometrySections
osdu:hasGeometrySections rdf:type owl:ObjectProperty ;
	rdfs:comment "Reference to the GeometrySections for the object " ;
	rdfs:domain osdu:Geometry ;
	rdfs:range osdu:GeometrySection ;
.

###  https://w3id.org/osdu#hasGpGridRepresentation
osdu:hasGpGridRepresentation rdf:type owl:ObjectProperty ;
	rdfs:comment "Reference to the GpGridRepresentation for the object " ;
	rdfs:domain osdu:AbstractGridRepresentation ;
	rdfs:range osdu:GpGridRepresentation ;
.

###  https://w3id.org/osdu#hasGrainDensityMeasurementType
osdu:hasGrainDensityMeasurementType rdf:type owl:ObjectProperty ;
	rdfs:comment "Reference to the GrainDensityMeasurementType for the object " ;
	rdfs:domain osdu:RoutineCoreAnalysis ;
	rdfs:range osdu:GrainDensityMeasurementType ;
.

###  https://w3id.org/osdu#hasHSE
osdu:hasHSE rdf:type owl:ObjectProperty ;
	rdfs:comment "Reference to the HSE for the object " ;
	rdfs:domain osdu:OperationsReport ;
	rdfs:range osdu:HealthSafetyEnvironment ;
.

###  https://w3id.org/osdu#hasHighPressureCriteria
osdu:hasHighPressureCriteria rdf:type owl:ObjectProperty ;
	rdfs:comment "Reference to the HighPressureCriteria for the object " ;
	rdfs:domain osdu:WBETestStep ;
	rdfs:range osdu:PressureCriteria ;
.

###  https://w3id.org/osdu#hasHistoricalInterests
osdu:hasHistoricalInterests rdf:type owl:ObjectProperty ;
	rdfs:comment "Reference to the HistoricalInterests for the object " ;
	rdfs:domain [
		rdf:type owl:Class ;
		owl:unionOf (
			osdu:Wellbore
			osdu:Well
		) ;
	] ;
	rdfs:range osdu:HistoricalInterest ;
.

###  https://w3id.org/osdu#hasHoleSection
osdu:hasHoleSection rdf:type owl:ObjectProperty ;
	rdfs:comment "Reference to the HoleSection for the object " ;
	rdfs:domain [
		rdf:type owl:Class ;
		owl:unionOf (
			osdu:FluidsInterval
			osdu:WellPlanningWellbore
			osdu:DSTRun
			osdu:CasingDesign
			osdu:BHARun
		) ;
	] ;
	rdfs:range osdu:HoleSection ;
.

###  https://w3id.org/osdu#hasHorizonInterpretation
osdu:hasHorizonInterpretation rdf:type owl:ObjectProperty ;
	rdfs:comment "Reference to the HorizonInterpretation for the object " ;
	rdfs:domain [
		rdf:type owl:Class ;
		owl:unionOf (
			osdu:Markers
			osdu:StratigraphicUnitInterpretation
			osdu:Interval
		) ;
	] ;
	rdfs:range osdu:HorizonInterpretation ;
.

###  https://w3id.org/osdu#hasHorizontalCRS
osdu:hasHorizontalCRS rdf:type owl:ObjectProperty ;
	rdfs:comment "Reference to the HorizontalCRS for the object " ;
	rdfs:domain osdu:CoordinateReferenceSystem ;
	rdfs:range osdu:HorizontalCRS ;
.

###  https://w3id.org/osdu#hasIjkGridRepresentation
osdu:hasIjkGridRepresentation rdf:type owl:ObjectProperty ;
	rdfs:comment "Reference to the IjkGridRepresentation for the object " ;
	rdfs:domain [
		rdf:type owl:Class ;
		owl:unionOf (
			osdu:AbstractIjkGridFlowSimulationBoundaryConnection
			osdu:SingleCellAquifer
		) ;
	] ;
	rdfs:range osdu:IjkGridRepresentation ;
.

###  https://w3id.org/osdu#hasInSARApplication
osdu:hasInSARApplication rdf:type owl:ObjectProperty ;
	rdfs:comment "Reference to the InSARApplication for the object " ;
	rdfs:domain osdu:ProcessedInSAR ;
	rdfs:range osdu:InSARApplication ;
.

###  https://w3id.org/osdu#hasInSARFrequencyBand
osdu:hasInSARFrequencyBand rdf:type owl:ObjectProperty ;
	rdfs:comment "Reference to the InSARFrequencyBand for the object " ;
	rdfs:domain osdu:ProcessedInSAR ;
	rdfs:range osdu:InSARFrequencyBand ;
.

###  https://w3id.org/osdu#hasInSARImageMode
osdu:hasInSARImageMode rdf:type owl:ObjectProperty ;
	rdfs:comment "Reference to the InSARImageMode for the object " ;
	rdfs:domain osdu:ProcessedInSAR ;
	rdfs:range osdu:InSARImageMode ;
.

###  https://w3id.org/osdu#hasInSARPolarisation
osdu:hasInSARPolarisation rdf:type owl:ObjectProperty ;
	rdfs:comment "Reference to the InSARPolarisation for the object " ;
	rdfs:domain osdu:ProcessedInSAR ;
	rdfs:range osdu:InSARPolarisation ;
.

###  https://w3id.org/osdu#hasInSARProcessingType
osdu:hasInSARProcessingType rdf:type owl:ObjectProperty ;
	rdfs:comment "Reference to the InSARProcessingType for the object " ;
	rdfs:domain osdu:ProcessedInSAR ;
	rdfs:range osdu:InSARProcessingType ;
.

###  https://w3id.org/osdu#hasIncident
osdu:hasIncident rdf:type owl:ObjectProperty ;
	rdfs:comment "Reference to the Incident for the object " ;
	rdfs:domain osdu:OperationsReport ;
	rdfs:range osdu:Incident ;
.

###  https://w3id.org/osdu#hasIndexableElement
osdu:hasIndexableElement rdf:type owl:ObjectProperty ;
	rdfs:comment "Reference to the IndexableElement for the object " ;
	rdfs:domain [
		rdf:type owl:Class ;
		owl:unionOf (
			osdu:IndexableElementCount
			osdu:SubRepresentation
			osdu:GenericProperty
		) ;
	] ;
	rdfs:range osdu:IndexableElement ;
.

###  https://w3id.org/osdu#hasIndexableElementCount
osdu:hasIndexableElementCount rdf:type owl:ObjectProperty ;
	rdfs:comment "Reference to the IndexableElementCount for the object " ;
	rdfs:domain osdu:AbstractRepresentation ;
	rdfs:range osdu:IndexableElementCount ;
.

###  https://w3id.org/osdu#hasInstalledTubulars
osdu:hasInstalledTubulars rdf:type owl:ObjectProperty ;
	rdfs:comment "Reference to the InstalledTubulars for the object " ;
	rdfs:domain osdu:WellboreArchitecture ;
	rdfs:range osdu:InstalledTubular ;
.

###  https://w3id.org/osdu#hasInterpolationMethod
osdu:hasInterpolationMethod rdf:type owl:ObjectProperty ;
	rdfs:comment "Reference to the InterpolationMethod for the object " ;
	rdfs:domain osdu:VelocityModeling ;
	rdfs:range osdu:InterpolationMethod ;
.

###  https://w3id.org/osdu#hasIntervalProperties
osdu:hasIntervalProperties rdf:type owl:ObjectProperty ;
	rdfs:comment "Reference to the IntervalProperties for the object " ;
	rdfs:domain osdu:WellboreIntervalSet ;
	rdfs:range osdu:AbstractColumnBasedTable ;
.

###  https://w3id.org/osdu#hasIntervals
osdu:hasIntervals rdf:type owl:ObjectProperty ;
	rdfs:comment "Reference to the Intervals for the object " ;
	rdfs:domain osdu:WellboreIntervalSet ;
	rdfs:range osdu:Interval ;
.

###  https://w3id.org/osdu#hasInventory
osdu:hasInventory rdf:type owl:ObjectProperty ;
	rdfs:comment "Reference to the Inventory for the object " ;
	rdfs:domain osdu:OperationsReport ;
	rdfs:range osdu:Inventory ;
.

###  https://w3id.org/osdu#hasKDirectionType
osdu:hasKDirectionType rdf:type owl:ObjectProperty ;
	rdfs:comment "Reference to the KDirectionType for the object " ;
	rdfs:domain osdu:AbstractColumnLayerGridPatch ;
	rdfs:range osdu:KDirectionType ;
.

###  https://w3id.org/osdu#hasKeys
osdu:hasKeys rdf:type owl:ObjectProperty ;
	rdfs:comment "Reference to the Keys for the object " ;
	rdfs:domain osdu:AbstractActivityParameter ;
	rdfs:range osdu:ParameterKey ;
.

###  https://w3id.org/osdu#hasLastLocation
osdu:hasLastLocation rdf:type owl:ObjectProperty ;
	rdfs:comment "Reference to the LastLocation for the object " ;
	rdfs:domain osdu:SeismicLineGeometry ;
	rdfs:range osdu:AbstractSpatialLocation ;
.

###  https://w3id.org/osdu#hasLegal
osdu:hasLegal rdf:type owl:ObjectProperty ;
	rdfs:comment "Reference to the Legal for the object " ;
	rdfs:domain osdu:System ;
	rdfs:range osdu:AbstractLegalTags ;
.

###  https://w3id.org/osdu#hasLineageAssertions
osdu:hasLineageAssertions rdf:type owl:ObjectProperty ;
	rdfs:comment "Reference to the LineageAssertions for the object " ;
	rdfs:domain [
		rdf:type owl:Class ;
		owl:unionOf (
			osdu:AbstractWorkProductComponent
			osdu:WorkProduct
		) ;
	] ;
	rdfs:range osdu:LineageAssertion ;
.

###  https://w3id.org/osdu#hasLinerType
osdu:hasLinerType rdf:type owl:ObjectProperty ;
	rdfs:comment "Reference to the LinerType for the object " ;
	rdfs:domain osdu:TubularAssembly ;
	rdfs:range osdu:LinerType ;
.

###  https://w3id.org/osdu#hasLithologyType
osdu:hasLithologyType rdf:type owl:ObjectProperty ;
	rdfs:comment "Reference to the LithologyType for the object " ;
	rdfs:domain [
		rdf:type owl:Class ;
		owl:unionOf (
			osdu:AbstractGeologicUnitInterpretation
			osdu:GeologyInterval
		) ;
	] ;
	rdfs:range osdu:LithologyType ;
.

###  https://w3id.org/osdu#hasLiveTraceOutline
osdu:hasLiveTraceOutline rdf:type owl:ObjectProperty ;
	rdfs:comment "Reference to the LiveTraceOutline for the object " ;
	rdfs:domain osdu:SeismicTraceData ;
	rdfs:range osdu:AbstractSpatialLocation ;
.

###  https://w3id.org/osdu#hasLocalModelCompoundCrs
osdu:hasLocalModelCompoundCrs rdf:type owl:ObjectProperty ;
	rdfs:comment "Reference to the LocalModelCompoundCrs for the object " ;
	rdfs:domain osdu:AbstractRepresentation ;
	rdfs:range osdu:LocalModelCompoundCrs ;
.

###  https://w3id.org/osdu#hasLocation
osdu:hasLocation rdf:type owl:ObjectProperty ;
	rdfs:comment "Reference to the Location for the object " ;
	rdfs:domain [
		rdf:type owl:Class ;
		owl:unionOf (
			osdu:Target
			osdu:GeometrySection
		) ;
	] ;
	rdfs:range osdu:AbstractSpatialLocation ;
.

###  https://w3id.org/osdu#hasLogCurveBusinessValue
osdu:hasLogCurveBusinessValue rdf:type owl:ObjectProperty ;
	rdfs:comment "Reference to the LogCurveBusinessValue for the object " ;
	rdfs:domain osdu:Curves ;
	rdfs:range osdu:LogCurveBusinessValue ;
.

###  https://w3id.org/osdu#hasLogCurveFamily
osdu:hasLogCurveFamily rdf:type owl:ObjectProperty ;
	rdfs:comment "Reference to the LogCurveFamily for the object " ;
	rdfs:domain osdu:Curves ;
	rdfs:range osdu:LogCurveFamily ;
.

###  https://w3id.org/osdu#hasLogCurveMainFamily
osdu:hasLogCurveMainFamily rdf:type owl:ObjectProperty ;
	rdfs:comment "Reference to the LogCurveMainFamily for the object " ;
	rdfs:domain osdu:Curves ;
	rdfs:range osdu:LogCurveMainFamily ;
.

###  https://w3id.org/osdu#hasLogCurveType
osdu:hasLogCurveType rdf:type owl:ObjectProperty ;
	rdfs:comment "Reference to the LogCurveType for the object " ;
	rdfs:domain osdu:Curves ;
	rdfs:range osdu:LogCurveType ;
.

###  https://w3id.org/osdu#hasLogServiceDateInterval
osdu:hasLogServiceDateInterval rdf:type owl:ObjectProperty ;
	rdfs:comment "Reference to the LogServiceDateInterval for the object " ;
	rdfs:domain osdu:WellLog ;
	rdfs:range osdu:LogServiceDateInterval ;
.

###  https://w3id.org/osdu#hasLogType
osdu:hasLogType rdf:type owl:ObjectProperty ;
	rdfs:comment "Reference to the LogType for the object " ;
	rdfs:domain osdu:WellLog ;
	rdfs:range osdu:LogType ;
.

###  https://w3id.org/osdu#hasLowPressureCriteria
osdu:hasLowPressureCriteria rdf:type owl:ObjectProperty ;
	rdfs:comment "Reference to the LowPressureCriteria for the object " ;
	rdfs:domain osdu:WBETestStep ;
	rdfs:range osdu:PressureCriteria ;
.

###  https://w3id.org/osdu#hasMarkerPropertyType
osdu:hasMarkerPropertyType rdf:type owl:ObjectProperty ;
	rdfs:comment "Reference to the MarkerPropertyType for the object " ;
	rdfs:domain osdu:MarkerProperty ;
	rdfs:range osdu:MarkerPropertyType ;
.

###  https://w3id.org/osdu#hasMarkerType
osdu:hasMarkerType rdf:type owl:ObjectProperty ;
	rdfs:comment "Reference to the MarkerType for the object " ;
	rdfs:domain osdu:Markers ;
	rdfs:range osdu:MarkerType ;
.

###  https://w3id.org/osdu#hasMarkers
osdu:hasMarkers rdf:type owl:ObjectProperty ;
	rdfs:comment "Reference to the Markers for the object " ;
	rdfs:domain osdu:WellboreMarkerSet ;
	rdfs:range osdu:Markers ;
.

###  https://w3id.org/osdu#hasMaterialType
osdu:hasMaterialType rdf:type owl:ObjectProperty ;
	rdfs:comment "Reference to the MaterialType for the object " ;
	rdfs:domain osdu:Wellbore ;
	rdfs:range osdu:MaterialType ;
.

###  https://w3id.org/osdu#hasMaximumFlowratePump
osdu:hasMaximumFlowratePump rdf:type owl:ObjectProperty ;
	rdfs:comment "Reference to the MaximumFlowratePump for the object " ;
	rdfs:domain osdu:FlowratePumpGroup ;
	rdfs:range osdu:MaximumFlowratePump ;
.

###  https://w3id.org/osdu#hasMaximumROP
osdu:hasMaximumROP rdf:type owl:ObjectProperty ;
	rdfs:comment "Reference to the MaximumROP for the object " ;
	rdfs:domain osdu:ROPGroup ;
	rdfs:range osdu:MaximumROP ;
.

###  https://w3id.org/osdu#hasMaximumRPM
osdu:hasMaximumRPM rdf:type owl:ObjectProperty ;
	rdfs:comment "Reference to the MaximumRPM for the object " ;
	rdfs:domain osdu:RPMGroup ;
	rdfs:range osdu:MaximumRPM ;
.

###  https://w3id.org/osdu#hasMaximumTorqueOnBottom
osdu:hasMaximumTorqueOnBottom rdf:type owl:ObjectProperty ;
	rdfs:comment "Reference to the MaximumTorqueOnBottom for the object " ;
	rdfs:domain osdu:TorqueOnBottomGroup ;
	rdfs:range osdu:MaximumTorqueOnBottom ;
.

###  https://w3id.org/osdu#hasMaximumWOB
osdu:hasMaximumWOB rdf:type owl:ObjectProperty ;
	rdfs:comment "Reference to the MaximumWOB for the object " ;
	rdfs:domain osdu:WOBGroup ;
	rdfs:range osdu:MaximumWOB ;
.

###  https://w3id.org/osdu#hasMethod
osdu:hasMethod rdf:type owl:ObjectProperty ;
	rdfs:comment "Reference to the Method for the object " ;
	rdfs:domain osdu:CoordinateTransformation ;
	rdfs:range osdu:Method ;
.

###  https://w3id.org/osdu#hasMinimumFlowratePump
osdu:hasMinimumFlowratePump rdf:type owl:ObjectProperty ;
	rdfs:comment "Reference to the MinimumFlowratePump for the object " ;
	rdfs:domain osdu:FlowratePumpGroup ;
	rdfs:range osdu:MinimumFlowratePump ;
.

###  https://w3id.org/osdu#hasMinimumROP
osdu:hasMinimumROP rdf:type owl:ObjectProperty ;
	rdfs:comment "Reference to the MinimumROP for the object " ;
	rdfs:domain osdu:ROPGroup ;
	rdfs:range osdu:MinimumROP ;
.

###  https://w3id.org/osdu#hasMinimumRPM
osdu:hasMinimumRPM rdf:type owl:ObjectProperty ;
	rdfs:comment "Reference to the MinimumRPM for the object " ;
	rdfs:domain osdu:RPMGroup ;
	rdfs:range osdu:MinimumRPM ;
.

###  https://w3id.org/osdu#hasMinimumTorqueOnBottom
osdu:hasMinimumTorqueOnBottom rdf:type owl:ObjectProperty ;
	rdfs:comment "Reference to the MinimumTorqueOnBottom for the object " ;
	rdfs:domain osdu:TorqueOnBottomGroup ;
	rdfs:range osdu:MinimumTorqueOnBottom ;
.

###  https://w3id.org/osdu#hasMinimumWOB
osdu:hasMinimumWOB rdf:type owl:ObjectProperty ;
	rdfs:comment "Reference to the MinimumWOB for the object " ;
	rdfs:domain osdu:WOBGroup ;
	rdfs:range osdu:MinimumWOB ;
.

###  https://w3id.org/osdu#hasMitigations
osdu:hasMitigations rdf:type owl:ObjectProperty ;
	rdfs:comment "Reference to the Mitigations for the object " ;
	rdfs:domain osdu:Risk ;
	rdfs:range osdu:RiskResponse ;
.

###  https://w3id.org/osdu#hasModelFeature
osdu:hasModelFeature rdf:type owl:ObjectProperty ;
	rdfs:comment "Reference to the ModelFeature for the object " ;
	rdfs:domain [
		rdf:type owl:Class ;
		owl:unionOf (
			osdu:EarthModelInterpretation
			osdu:RockFluidOrganizationInterpretation
			osdu:VoidageGroupInterpretation
			osdu:StructuralOrganizationInterpretation
			osdu:LocalModelFeature
			osdu:ReservoirCompartmentInterpretation
		) ;
	] ;
	rdfs:range osdu:ModelFeature ;
.

###  https://w3id.org/osdu#hasMudLosses
osdu:hasMudLosses rdf:type owl:ObjectProperty ;
	rdfs:comment "Reference to the MudLosses for the object " ;
	rdfs:domain osdu:OperationsReport ;
	rdfs:range osdu:MudLosses ;
.

###  https://w3id.org/osdu#hasMudPumps
osdu:hasMudPumps rdf:type owl:ObjectProperty ;
	rdfs:comment "Reference to the MudPumps for the object " ;
	rdfs:domain osdu:RigUtilization ;
	rdfs:range osdu:MudPump ;
.

###  https://w3id.org/osdu#hasMudVolume
osdu:hasMudVolume rdf:type owl:ObjectProperty ;
	rdfs:comment "Reference to the MudVolume for the object " ;
	rdfs:domain osdu:OperationsReport ;
	rdfs:range osdu:MudVolume ;
.

###  https://w3id.org/osdu#hasNonProductiveTimeStatistics
osdu:hasNonProductiveTimeStatistics rdf:type owl:ObjectProperty ;
	rdfs:comment "Reference to the NonProductiveTimeStatistics for the object " ;
	rdfs:domain osdu:WellPlanningActivity ;
	rdfs:range osdu:Statistics ;
.

###  https://w3id.org/osdu#hasNotionalSeismicLine
osdu:hasNotionalSeismicLine rdf:type owl:ObjectProperty ;
	rdfs:comment "Reference to the NotionalSeismicLine for the object " ;
	rdfs:domain osdu:SeismicLineGeometry ;
	rdfs:range osdu:NotionalSeismicLine ;
.

###  https://w3id.org/osdu#hasOAuth2FlowType
osdu:hasOAuth2FlowType rdf:type owl:ObjectProperty ;
	rdfs:comment "Reference to the OAuth2FlowType for the object " ;
	rdfs:domain osdu:SecurityScheme ;
	rdfs:range osdu:OAuth2FlowType ;
.

###  https://w3id.org/osdu#hasOSDURegion
osdu:hasOSDURegion rdf:type owl:ObjectProperty ;
	rdfs:comment "Reference to the OSDURegion for the object " ;
	rdfs:domain osdu:AbstractCommonResources ;
	rdfs:range osdu:OSDURegion ;
.

###  https://w3id.org/osdu#hasObligationType
osdu:hasObligationType rdf:type owl:ObjectProperty ;
	rdfs:comment "Reference to the ObligationType for the object " ;
	rdfs:domain osdu:Terms ;
	rdfs:range osdu:ObligationType ;
.

###  https://w3id.org/osdu#hasOnIngestionAcl
osdu:hasOnIngestionAcl rdf:type owl:ObjectProperty ;
	rdfs:comment "Reference to the OnIngestionAcl for the object " ;
	rdfs:domain osdu:ConnectedSourceDataJob ;
	rdfs:range osdu:ACL ;
.

###  https://w3id.org/osdu#hasOnIngestionLegalTags
osdu:hasOnIngestionLegalTags rdf:type owl:ObjectProperty ;
	rdfs:comment "Reference to the OnIngestionLegalTags for the object " ;
	rdfs:domain osdu:ConnectedSourceDataJob ;
	rdfs:range osdu:AbstractLegalTags ;
.

###  https://w3id.org/osdu#hasOperatingEnvironment
osdu:hasOperatingEnvironment rdf:type owl:ObjectProperty ;
	rdfs:comment "Reference to the OperatingEnvironment for the object " ;
	rdfs:domain [
		rdf:type owl:Class ;
		owl:unionOf (
			osdu:AbstractFacility
			osdu:SeismicAcquisitionSurvey
		) ;
	] ;
	rdfs:range osdu:OperatingEnvironment ;
.

###  https://w3id.org/osdu#hasOperationParameterPlan
osdu:hasOperationParameterPlan rdf:type owl:ObjectProperty ;
	rdfs:comment "Reference to the OperationParameterPlan for the object " ;
	rdfs:domain osdu:RunParameterPlan ;
	rdfs:range osdu:OperationParameterPlan ;
.

###  https://w3id.org/osdu#hasOperationalPeriod
osdu:hasOperationalPeriod rdf:type owl:ObjectProperty ;
	rdfs:comment "Reference to the OperationalPeriod for the object " ;
	rdfs:domain osdu:SatelliteMission ;
	rdfs:range osdu:OperationalPeriod ;
.

###  https://w3id.org/osdu#hasOrderingCriteriaType
osdu:hasOrderingCriteriaType rdf:type owl:ObjectProperty ;
	rdfs:comment "Reference to the OrderingCriteriaType for the object " ;
	rdfs:domain osdu:GeologicUnitOccurrenceInterpretation ;
	rdfs:range osdu:OrderingCriteriaType ;
.

###  https://w3id.org/osdu#hasOrganisation
osdu:hasOrganisation rdf:type owl:ObjectProperty ;
	rdfs:comment "Reference to the Organisation for the object " ;
	rdfs:domain [
		rdf:type owl:Class ;
		owl:unionOf (
			osdu:AbstractContact
			osdu:AbstractStorageLocation
			osdu:AbstractFacilityOperator
			osdu:Contractors
			osdu:Personnel
			osdu:AbstractFacility
			osdu:FluidsProgram
			osdu:Fluid
			osdu:RockSample
			osdu:Organisation
			osdu:SurveySection
			osdu:DrillingActivity
			osdu:OperationsReport
			osdu:Incident
			osdu:PerforationJob
			osdu:PerforationInterval
			osdu:Coring
			osdu:Rig
			osdu:PlannedCementJob
			osdu:ConnectedSourceRegistryEntry
			osdu:WellLog
			osdu:RockSampleAnalysis
			osdu:PPFGDataset
			osdu:WellboreTrajectory
			osdu:TubularComponent
			osdu:ProcessedInSAR
		) ;
	] ;
	rdfs:range osdu:Organisation ;
.

###  https://w3id.org/osdu#hasOrganisationType
osdu:hasOrganisationType rdf:type owl:ObjectProperty ;
	rdfs:comment "Reference to the OrganisationType for the object " ;
	rdfs:domain osdu:Organisation ;
	rdfs:range osdu:OrganisationType ;
.

###  https://w3id.org/osdu#hasOtherMeasurements
osdu:hasOtherMeasurements rdf:type owl:ObjectProperty ;
	rdfs:comment "Reference to the OtherMeasurements for the object " ;
	rdfs:domain osdu:RCAMeasurement ;
	rdfs:range osdu:AbstractSpecification ;
.

###  https://w3id.org/osdu#hasOutputInputArcs
osdu:hasOutputInputArcs rdf:type owl:ObjectProperty ;
	rdfs:comment "Reference to the OutputInputArcs for the object " ;
	rdfs:domain osdu:ActivityTemplateArc ;
	rdfs:range osdu:Arc ;
.

###  https://w3id.org/osdu#hasPPFGContextType
osdu:hasPPFGContextType rdf:type owl:ObjectProperty ;
	rdfs:comment "Reference to the PPFGContextType for the object " ;
	rdfs:domain osdu:PPFGDataset ;
	rdfs:range osdu:PPFGContextType ;
.

###  https://w3id.org/osdu#hasPPFGCurveFamily
osdu:hasPPFGCurveFamily rdf:type owl:ObjectProperty ;
	rdfs:comment "Reference to the PPFGCurveFamily for the object " ;
	rdfs:domain osdu:Curves ;
	rdfs:range osdu:PPFGCurveFamily ;
.

###  https://w3id.org/osdu#hasPPFGCurveLithoType
osdu:hasPPFGCurveLithoType rdf:type owl:ObjectProperty ;
	rdfs:comment "Reference to the PPFGCurveLithoType for the object " ;
	rdfs:domain osdu:Curves ;
	rdfs:range osdu:PPFGCurveLithoType ;
.

###  https://w3id.org/osdu#hasPPFGCurveMainFamily
osdu:hasPPFGCurveMainFamily rdf:type owl:ObjectProperty ;
	rdfs:comment "Reference to the PPFGCurveMainFamily for the object " ;
	rdfs:domain osdu:Curves ;
	rdfs:range osdu:PPFGCurveMainFamily ;
.

###  https://w3id.org/osdu#hasPPFGCurveMnemonic
osdu:hasPPFGCurveMnemonic rdf:type owl:ObjectProperty ;
	rdfs:comment "Reference to the PPFGCurveMnemonic for the object " ;
	rdfs:domain osdu:Curves ;
	rdfs:range osdu:PPFGCurveMnemonic ;
.

###  https://w3id.org/osdu#hasPPFGCurveProbability
osdu:hasPPFGCurveProbability rdf:type owl:ObjectProperty ;
	rdfs:comment "Reference to the PPFGCurveProbability for the object " ;
	rdfs:domain [
		rdf:type owl:Class ;
		owl:unionOf (
			osdu:Statistics
			osdu:ROPStatistics
			osdu:Curves
		) ;
	] ;
	rdfs:range osdu:PPFGCurveProbability ;
.

###  https://w3id.org/osdu#hasPPFGCurveTransformModelType
osdu:hasPPFGCurveTransformModelType rdf:type owl:ObjectProperty ;
	rdfs:comment "Reference to the PPFGCurveTransformModelType for the object " ;
	rdfs:domain osdu:Curves ;
	rdfs:range osdu:PPFGCurveTransformModelType ;
.

###  https://w3id.org/osdu#hasPPFGDataset
osdu:hasPPFGDataset rdf:type owl:ObjectProperty ;
	rdfs:comment "Reference to the PPFGDataset for the object " ;
	rdfs:domain [
		rdf:type owl:Class ;
		owl:unionOf (
			osdu:WellPlanningWellbore
			osdu:CasingDesign
		) ;
	] ;
	rdfs:range osdu:PPFGDataset ;
.

###  https://w3id.org/osdu#hasParameterKind
osdu:hasParameterKind rdf:type owl:ObjectProperty ;
	rdfs:comment "Reference to the ParameterKind for the object " ;
	rdfs:domain osdu:AbstractActivityParameter ;
	rdfs:range osdu:ParameterKind ;
.

###  https://w3id.org/osdu#hasParameterRole
osdu:hasParameterRole rdf:type owl:ObjectProperty ;
	rdfs:comment "Reference to the ParameterRole for the object " ;
	rdfs:domain osdu:AbstractActivityParameter ;
	rdfs:range osdu:ParameterRole ;
.

###  https://w3id.org/osdu#hasParameterType
osdu:hasParameterType rdf:type owl:ObjectProperty ;
	rdfs:comment "Reference to the ParameterType for the object " ;
	rdfs:domain [
		rdf:type owl:Class ;
		owl:unionOf (
			osdu:ProjectSpecifications
			osdu:AbstractFacilitySpecification
			osdu:AbstractSpecification
		) ;
	] ;
	rdfs:range osdu:ParameterType ;
.

###  https://w3id.org/osdu#hasParameters
osdu:hasParameters rdf:type owl:ObjectProperty ;
	rdfs:comment "Reference to the Parameters for the object " ;
	rdfs:domain [
		rdf:type owl:Class ;
		owl:unionOf (
			osdu:ActivityTemplate
			osdu:Workflow
		) ;
	] ;
	rdfs:range osdu:WorkflowParameter ;
.

###  https://w3id.org/osdu#hasPerforationCentralizationMethodType
osdu:hasPerforationCentralizationMethodType rdf:type owl:ObjectProperty ;
	rdfs:comment "Reference to the PerforationCentralizationMethodType for the object " ;
	rdfs:domain osdu:PerforationJob ;
	rdfs:range osdu:PerforationCentralizationMethodType ;
.

###  https://w3id.org/osdu#hasPerforationConveyedMethod
osdu:hasPerforationConveyedMethod rdf:type owl:ObjectProperty ;
	rdfs:comment "Reference to the PerforationConveyedMethod for the object " ;
	rdfs:domain osdu:PerforationJob ;
	rdfs:range osdu:PerforationConveyedMethod ;
.

###  https://w3id.org/osdu#hasPerforationGunCarrierCategory
osdu:hasPerforationGunCarrierCategory rdf:type owl:ObjectProperty ;
	rdfs:comment "Reference to the PerforationGunCarrierCategory for the object " ;
	rdfs:domain osdu:PerforationInterval ;
	rdfs:range osdu:PerforationGunCarrierCategory ;
.

###  https://w3id.org/osdu#hasPerforationGunCarrierModel
osdu:hasPerforationGunCarrierModel rdf:type owl:ObjectProperty ;
	rdfs:comment "Reference to the PerforationGunCarrierModel for the object " ;
	rdfs:domain osdu:PerforationInterval ;
	rdfs:range osdu:PerforationGunCarrierModel ;
.

###  https://w3id.org/osdu#hasPerforationGunCarrierType
osdu:hasPerforationGunCarrierType rdf:type owl:ObjectProperty ;
	rdfs:comment "Reference to the PerforationGunCarrierType for the object " ;
	rdfs:domain osdu:PerforationInterval ;
	rdfs:range osdu:PerforationGunCarrierType ;
.

###  https://w3id.org/osdu#hasPerforationGunChargeShape
osdu:hasPerforationGunChargeShape rdf:type owl:ObjectProperty ;
	rdfs:comment "Reference to the PerforationGunChargeShape for the object " ;
	rdfs:domain osdu:PerforationInterval ;
	rdfs:range osdu:PerforationGunChargeShape ;
.

###  https://w3id.org/osdu#hasPerforationGunChargeType
osdu:hasPerforationGunChargeType rdf:type owl:ObjectProperty ;
	rdfs:comment "Reference to the PerforationGunChargeType for the object " ;
	rdfs:domain osdu:PerforationInterval ;
	rdfs:range osdu:PerforationGunChargeType ;
.

###  https://w3id.org/osdu#hasPerforationGunFiringHeadType
osdu:hasPerforationGunFiringHeadType rdf:type owl:ObjectProperty ;
	rdfs:comment "Reference to the PerforationGunFiringHeadType for the object " ;
	rdfs:domain osdu:PerforationInterval ;
	rdfs:range osdu:PerforationGunFiringHeadType ;
.

###  https://w3id.org/osdu#hasPerforationGunMetallurgyType
osdu:hasPerforationGunMetallurgyType rdf:type owl:ObjectProperty ;
	rdfs:comment "Reference to the PerforationGunMetallurgyType for the object " ;
	rdfs:domain osdu:PerforationInterval ;
	rdfs:range osdu:PerforationGunMetallurgyType ;
.

###  https://w3id.org/osdu#hasPerforationIntervalReason
osdu:hasPerforationIntervalReason rdf:type owl:ObjectProperty ;
	rdfs:comment "Reference to the PerforationIntervalReason for the object " ;
	rdfs:domain osdu:PerforationInterval ;
	rdfs:range osdu:PerforationIntervalReason ;
.

###  https://w3id.org/osdu#hasPerforationIntervalType
osdu:hasPerforationIntervalType rdf:type owl:ObjectProperty ;
	rdfs:comment "Reference to the PerforationIntervalType for the object " ;
	rdfs:domain [
		rdf:type owl:Class ;
		owl:unionOf (
			osdu:PerforationJob
			osdu:PerforationInterval
		) ;
	] ;
	rdfs:range osdu:PerforationIntervalType ;
.

###  https://w3id.org/osdu#hasPerforationIntervalWLSize
osdu:hasPerforationIntervalWLSize rdf:type owl:ObjectProperty ;
	rdfs:comment "Reference to the PerforationIntervalWLSize for the object " ;
	rdfs:domain osdu:PerforationInterval ;
	rdfs:range osdu:PerforationIntervalWLSize ;
.

###  https://w3id.org/osdu#hasPerforationJob
osdu:hasPerforationJob rdf:type owl:ObjectProperty ;
	rdfs:comment "Reference to the PerforationJob for the object " ;
	rdfs:domain osdu:PerforationInterval ;
	rdfs:range osdu:PerforationJob ;
.

###  https://w3id.org/osdu#hasPerforationPillType
osdu:hasPerforationPillType rdf:type owl:ObjectProperty ;
	rdfs:comment "Reference to the PerforationPillType for the object " ;
	rdfs:domain osdu:PerforationJob ;
	rdfs:range osdu:PerforationPillType ;
.

###  https://w3id.org/osdu#hasPermeabilityMeasurementType
osdu:hasPermeabilityMeasurementType rdf:type owl:ObjectProperty ;
	rdfs:comment "Reference to the PermeabilityMeasurementType for the object " ;
	rdfs:domain osdu:RCAMeasurement ;
	rdfs:range osdu:PermeabilityMeasurementType ;
.

###  https://w3id.org/osdu#hasPersistedCollection
osdu:hasPersistedCollection rdf:type owl:ObjectProperty ;
	rdfs:comment "Reference to the PersistedCollection for the object " ;
	rdfs:domain [
		rdf:type owl:Class ;
		owl:unionOf (
			osdu:Risk
			osdu:UnsealedSurfaceFramework
			osdu:PersistedCollection
		) ;
	] ;
	rdfs:range osdu:PersistedCollection ;
.

###  https://w3id.org/osdu#hasPersonnel
osdu:hasPersonnel rdf:type owl:ObjectProperty ;
	rdfs:comment "Reference to the Personnel for the object " ;
	rdfs:domain [
		rdf:type owl:Class ;
		owl:unionOf (
			osdu:AbstractProject
			osdu:OperationsReport
		) ;
	] ;
	rdfs:range osdu:Personnel ;
.

###  https://w3id.org/osdu#hasPetroleumSystemElementType
osdu:hasPetroleumSystemElementType rdf:type owl:ObjectProperty ;
	rdfs:comment "Reference to the PetroleumSystemElementType for the object " ;
	rdfs:domain osdu:SeismicHorizon ;
	rdfs:range osdu:PetroleumSystemElementType ;
.

###  https://w3id.org/osdu#hasPhases
osdu:hasPhases rdf:type owl:ObjectProperty ;
	rdfs:comment "Reference to the Phases for the object " ;
	rdfs:domain osdu:WellActivityProgram ;
	rdfs:range osdu:Phase ;
.

###  https://w3id.org/osdu#hasPillarShapeType
osdu:hasPillarShapeType rdf:type owl:ObjectProperty ;
	rdfs:comment "Reference to the PillarShapeType for the object " ;
	rdfs:domain osdu:AbstractColumnLayerGridPatch ;
	rdfs:range osdu:PillarShapeType ;
.

###  https://w3id.org/osdu#hasPlannedLithology
osdu:hasPlannedLithology rdf:type owl:ObjectProperty ;
	rdfs:comment "Reference to the PlannedLithology for the object " ;
	rdfs:domain osdu:WellPlanningWellbore ;
	rdfs:range osdu:PlannedLithology ;
.

###  https://w3id.org/osdu#hasPlay
osdu:hasPlay rdf:type owl:ObjectProperty ;
	rdfs:comment "Reference to the Play for the object " ;
	rdfs:domain osdu:AbstractGeoPlayContext ;
	rdfs:range osdu:Play ;
.

###  https://w3id.org/osdu#hasPlayType
osdu:hasPlayType rdf:type owl:ObjectProperty ;
	rdfs:comment "Reference to the PlayType for the object " ;
	rdfs:domain [
		rdf:type owl:Class ;
		owl:unionOf (
			osdu:AbstractGeoPlayContext
			osdu:Play
			osdu:WellStatusSummary
		) ;
	] ;
	rdfs:range osdu:PlayType ;
.

###  https://w3id.org/osdu#hasPlugType
osdu:hasPlugType rdf:type owl:ObjectProperty ;
	rdfs:comment "Reference to the PlugType for the object " ;
	rdfs:domain osdu:PlannedCementJob ;
	rdfs:range osdu:PlugType ;
.

###  https://w3id.org/osdu#hasPoint
osdu:hasPoint rdf:type owl:ObjectProperty ;
	rdfs:comment "Reference to the Point for the object " ;
	rdfs:domain [
		rdf:type owl:Class ;
		owl:unionOf (
			osdu:AnyCrsGeoJSONLineStringCoordinatesArray
			osdu:AnyCrsGeoJSONPolygonCoordinatesArray
			osdu:BBox
			osdu:MaximumTorqueOnBottom
			osdu:MinimumTorqueOnBottom
			osdu:MaximumRPM
			osdu:MinimumRPM
			osdu:RecommendedRPM
			osdu:DownHoleMaximumRPM
			osdu:DownHoleMinimumRPM
			osdu:DownHoleRecommendedRPM
			osdu:MaximumROP
			osdu:MinimumROP
			osdu:RecommendedROP
			osdu:MaximumWOB
			osdu:MinimumWOB
			osdu:RecommendedWOB
			osdu:MaximumFlowratePump
			osdu:MinimumFlowratePump
			osdu:RecommendedFlowratePump
		) ;
	] ;
	rdfs:range osdu:Point ;
.

###  https://w3id.org/osdu#hasPointsSources
osdu:hasPointsSources rdf:type owl:ObjectProperty ;
	rdfs:comment "Reference to the PointsSources for the object " ;
	rdfs:domain osdu:Point ;
	rdfs:range osdu:PointsSource ;
.

###  https://w3id.org/osdu#hasPorosityMeasurementType
osdu:hasPorosityMeasurementType rdf:type owl:ObjectProperty ;
	rdfs:comment "Reference to the PorosityMeasurementType for the object " ;
	rdfs:domain osdu:RCAMeasurement ;
	rdfs:range osdu:PorosityMeasurementType ;
.

###  https://w3id.org/osdu#hasPrecision
osdu:hasPrecision rdf:type owl:ObjectProperty ;
	rdfs:comment "Reference to the Precision for the object " ;
	rdfs:domain osdu:SeismicTraceData ;
	rdfs:range osdu:Precision ;
.

###  https://w3id.org/osdu#hasPreferredUsage
osdu:hasPreferredUsage rdf:type owl:ObjectProperty ;
	rdfs:comment "Reference to the PreferredUsage for the object " ;
	rdfs:domain [
		rdf:type owl:Class ;
		owl:unionOf (
			osdu:CoordinateTransformation
			osdu:CoordinateReferenceSystem
		) ;
	] ;
	rdfs:range osdu:PreferredUsage ;
.

###  https://w3id.org/osdu#hasPressureMeasurementType
osdu:hasPressureMeasurementType rdf:type owl:ObjectProperty ;
	rdfs:comment "Reference to the PressureMeasurementType for the object " ;
	rdfs:domain osdu:Conditions ;
	rdfs:range osdu:PressureMeasurementType ;
.

###  https://w3id.org/osdu#hasPreventions
osdu:hasPreventions rdf:type owl:ObjectProperty ;
	rdfs:comment "Reference to the Preventions for the object " ;
	rdfs:domain osdu:Risk ;
	rdfs:range osdu:RiskResponse ;
.

###  https://w3id.org/osdu#hasProcessingParameterType
osdu:hasProcessingParameterType rdf:type owl:ObjectProperty ;
	rdfs:comment "Reference to the ProcessingParameterType for the object " ;
	rdfs:domain osdu:ProcessingParameters ;
	rdfs:range osdu:ProcessingParameterType ;
.

###  https://w3id.org/osdu#hasProcessingParameters
osdu:hasProcessingParameters rdf:type owl:ObjectProperty ;
	rdfs:comment "Reference to the ProcessingParameters for the object " ;
	rdfs:domain osdu:SeismicTraceData ;
	rdfs:range osdu:ProcessingParameters ;
.

###  https://w3id.org/osdu#hasProductiveTimeStatistics
osdu:hasProductiveTimeStatistics rdf:type owl:ObjectProperty ;
	rdfs:comment "Reference to the ProductiveTimeStatistics for the object " ;
	rdfs:domain osdu:WellPlanningActivity ;
	rdfs:range osdu:Statistics ;
.

###  https://w3id.org/osdu#hasProjectRole
osdu:hasProjectRole rdf:type owl:ObjectProperty ;
	rdfs:comment "Reference to the ProjectRole for the object " ;
	rdfs:domain osdu:Personnel ;
	rdfs:range osdu:ProjectRole ;
.

###  https://w3id.org/osdu#hasProjectSpecifications
osdu:hasProjectSpecifications rdf:type owl:ObjectProperty ;
	rdfs:comment "Reference to the ProjectSpecifications for the object " ;
	rdfs:domain osdu:AbstractProject ;
	rdfs:range osdu:ProjectSpecifications ;
.

###  https://w3id.org/osdu#hasProjectStateType
osdu:hasProjectStateType rdf:type owl:ObjectProperty ;
	rdfs:comment "Reference to the ProjectStateType for the object " ;
	rdfs:domain osdu:ProjectStates ;
	rdfs:range osdu:ProjectStateType ;
.

###  https://w3id.org/osdu#hasProjectStates
osdu:hasProjectStates rdf:type owl:ObjectProperty ;
	rdfs:comment "Reference to the ProjectStates for the object " ;
	rdfs:domain osdu:AbstractProject ;
	rdfs:range osdu:ProjectStates ;
.

###  https://w3id.org/osdu#hasProjectedBottomHoleLocation
osdu:hasProjectedBottomHoleLocation rdf:type owl:ObjectProperty ;
	rdfs:comment "Reference to the ProjectedBottomHoleLocation for the object " ;
	rdfs:domain osdu:Wellbore ;
	rdfs:range osdu:AbstractSpatialLocation ;
.

###  https://w3id.org/osdu#hasProjection
osdu:hasProjection rdf:type owl:ObjectProperty ;
	rdfs:comment "Reference to the Projection for the object " ;
	rdfs:domain osdu:CoordinateReferenceSystem ;
	rdfs:range osdu:Projection ;
.

###  https://w3id.org/osdu#hasPropertyType
osdu:hasPropertyType rdf:type owl:ObjectProperty ;
	rdfs:comment "Reference to the PropertyType for the object " ;
	rdfs:domain [
		rdf:type owl:Class ;
		owl:unionOf (
			osdu:AbstractReferencePropertyType
			osdu:AbstractPropertyType
			osdu:ParameterTemplate
			osdu:LogCurveType
			osdu:PropertyType
			osdu:LogCurveFamily
			osdu:Configuration
		) ;
	] ;
	rdfs:range osdu:AbstractPropertyType ;
.

###  https://w3id.org/osdu#hasProprietaryActivityCode
osdu:hasProprietaryActivityCode rdf:type owl:ObjectProperty ;
	rdfs:comment "Reference to the ProprietaryActivityCode for the object " ;
	rdfs:domain osdu:DrillingActivity ;
	rdfs:range osdu:ObjectAlias ;
.

###  https://w3id.org/osdu#hasProspect
osdu:hasProspect rdf:type owl:ObjectProperty ;
	rdfs:comment "Reference to the Prospect for the object " ;
	rdfs:domain osdu:AbstractGeoProspectContext ;
	rdfs:range osdu:Prospect ;
.

###  https://w3id.org/osdu#hasProspectType
osdu:hasProspectType rdf:type owl:ObjectProperty ;
	rdfs:comment "Reference to the ProspectType for the object " ;
	rdfs:domain [
		rdf:type owl:Class ;
		owl:unionOf (
			osdu:AbstractGeoProspectContext
			osdu:Prospect
		) ;
	] ;
	rdfs:range osdu:ProspectType ;
.

###  https://w3id.org/osdu#hasPumpOp
osdu:hasPumpOp rdf:type owl:ObjectProperty ;
	rdfs:comment "Reference to the PumpOp for the object " ;
	rdfs:domain osdu:OperationsReport ;
	rdfs:range osdu:PumpOperations ;
.

###  https://w3id.org/osdu#hasQualitativeSpatialAccuracyType
osdu:hasQualitativeSpatialAccuracyType rdf:type owl:ObjectProperty ;
	rdfs:comment "Reference to the QualitativeSpatialAccuracyType for the object " ;
	rdfs:domain osdu:AbstractSpatialLocation ;
	rdfs:range osdu:QualitativeSpatialAccuracyType ;
.

###  https://w3id.org/osdu#hasQualityDataRule
osdu:hasQualityDataRule rdf:type owl:ObjectProperty ;
	rdfs:comment "Reference to the QualityDataRule for the object " ;
	rdfs:domain [
		rdf:type owl:Class ;
		owl:unionOf (
			osdu:DataRules
			osdu:DataRule
		) ;
	] ;
	rdfs:range osdu:QualityDataRule ;
.

###  https://w3id.org/osdu#hasQualityDataRuleSet
osdu:hasQualityDataRuleSet rdf:type owl:ObjectProperty ;
	rdfs:comment "Reference to the QualityDataRuleSet for the object " ;
	rdfs:domain osdu:DataRuleSets ;
	rdfs:range osdu:QualityDataRuleSet ;
.

###  https://w3id.org/osdu#hasQualityMetric
osdu:hasQualityMetric rdf:type owl:ObjectProperty ;
	rdfs:comment "Reference to the QualityMetric for the object " ;
	rdfs:domain osdu:DataQuality ;
	rdfs:range osdu:AbstractQualityMetric ;
.

###  https://w3id.org/osdu#hasQuantitativeAccuracyBand
osdu:hasQuantitativeAccuracyBand rdf:type owl:ObjectProperty ;
	rdfs:comment "Reference to the QuantitativeAccuracyBand for the object " ;
	rdfs:domain osdu:AbstractSpatialLocation ;
	rdfs:range osdu:QuantitativeAccuracyBand ;
.

###  https://w3id.org/osdu#hasRCAMeasurements
osdu:hasRCAMeasurements rdf:type owl:ObjectProperty ;
	rdfs:comment "Reference to the RCAMeasurements for the object " ;
	rdfs:domain osdu:RoutineCoreAnalysis ;
	rdfs:range osdu:RCAMeasurement ;
.

###  https://w3id.org/osdu#hasROPGroup
osdu:hasROPGroup rdf:type owl:ObjectProperty ;
	rdfs:comment "Reference to the ROPGroup for the object " ;
	rdfs:domain osdu:OperationParameterPlan ;
	rdfs:range osdu:ROPGroup ;
.

###  https://w3id.org/osdu#hasRPMGroup
osdu:hasRPMGroup rdf:type owl:ObjectProperty ;
	rdfs:comment "Reference to the RPMGroup for the object " ;
	rdfs:domain osdu:OperationParameterPlan ;
	rdfs:range osdu:RPMGroup ;
.

###  https://w3id.org/osdu#hasRateOfPenetrationStatistics
osdu:hasRateOfPenetrationStatistics rdf:type owl:ObjectProperty ;
	rdfs:comment "Reference to the RateOfPenetrationStatistics for the object " ;
	rdfs:domain osdu:WellPlanningActivity ;
	rdfs:range osdu:ROPStatistics ;
.

###  https://w3id.org/osdu#hasReasonTripType
osdu:hasReasonTripType rdf:type owl:ObjectProperty ;
	rdfs:comment "Reference to the ReasonTripType for the object " ;
	rdfs:domain osdu:BHARun ;
	rdfs:range osdu:ReasonTripType ;
.

###  https://w3id.org/osdu#hasReceiverConfigurations
osdu:hasReceiverConfigurations rdf:type owl:ObjectProperty ;
	rdfs:comment "Reference to the ReceiverConfigurations for the object " ;
	rdfs:domain osdu:SeismicAcquisitionSurvey ;
	rdfs:range osdu:SeismicReceiverConfiguration ;
.

###  https://w3id.org/osdu#hasRecommendedFlowratePump
osdu:hasRecommendedFlowratePump rdf:type owl:ObjectProperty ;
	rdfs:comment "Reference to the RecommendedFlowratePump for the object " ;
	rdfs:domain osdu:FlowratePumpGroup ;
	rdfs:range osdu:RecommendedFlowratePump ;
.

###  https://w3id.org/osdu#hasRecommendedROP
osdu:hasRecommendedROP rdf:type owl:ObjectProperty ;
	rdfs:comment "Reference to the RecommendedROP for the object " ;
	rdfs:domain osdu:ROPGroup ;
	rdfs:range osdu:RecommendedROP ;
.

###  https://w3id.org/osdu#hasRecommendedRPM
osdu:hasRecommendedRPM rdf:type owl:ObjectProperty ;
	rdfs:comment "Reference to the RecommendedRPM for the object " ;
	rdfs:domain osdu:RPMGroup ;
	rdfs:range osdu:RecommendedRPM ;
.

###  https://w3id.org/osdu#hasRecommendedWOB
osdu:hasRecommendedWOB rdf:type owl:ObjectProperty ;
	rdfs:comment "Reference to the RecommendedWOB for the object " ;
	rdfs:domain osdu:WOBGroup ;
	rdfs:range osdu:RecommendedWOB ;
.

###  https://w3id.org/osdu#hasReferenceLevel
osdu:hasReferenceLevel rdf:type owl:ObjectProperty ;
	rdfs:comment "Reference to the ReferenceLevel for the object " ;
	rdfs:domain osdu:GeoReferencedImage ;
	rdfs:range osdu:ReferenceLevel ;
.

###  https://w3id.org/osdu#hasRemarks
osdu:hasRemarks rdf:type owl:ObjectProperty ;
	rdfs:comment "Reference to the Remarks for the object " ;
	rdfs:domain [
		rdf:type owl:Class ;
		owl:unionOf (
			osdu:RCAMeasurement
			osdu:RockSampleAnalysis
		) ;
	] ;
	rdfs:range osdu:Remark ;
.

###  https://w3id.org/osdu#hasRepresentativeDipDirection
osdu:hasRepresentativeDipDirection rdf:type owl:ObjectProperty ;
	rdfs:comment "Reference to the RepresentativeDipDirection for the object " ;
	rdfs:domain osdu:FaultInterpretation ;
	rdfs:range osdu:RepresentativeDipDirection ;
.

###  https://w3id.org/osdu#hasReservoirCompartmentUnits
osdu:hasReservoirCompartmentUnits rdf:type owl:ObjectProperty ;
	rdfs:comment "Reference to the ReservoirCompartmentUnits for the object " ;
	rdfs:domain osdu:ReservoirCompartmentInterpretation ;
	rdfs:range osdu:ReservoirCompartmentUnit ;
.

###  https://w3id.org/osdu#hasReservoirEvaluations
osdu:hasReservoirEvaluations rdf:type owl:ObjectProperty ;
	rdfs:comment "Reference to the ReservoirEvaluations for the object " ;
	rdfs:domain osdu:EvaluationPlan ;
	rdfs:range osdu:DSTRun ;
.

###  https://w3id.org/osdu#hasRestrictedResources
osdu:hasRestrictedResources rdf:type owl:ObjectProperty ;
	rdfs:comment "Reference to the RestrictedResources for the object " ;
	rdfs:domain osdu:Agreement ;
	rdfs:range osdu:RestrictedResources ;
.

###  https://w3id.org/osdu#hasRheometer
osdu:hasRheometer rdf:type owl:ObjectProperty ;
	rdfs:comment "Reference to the Rheometer for the object " ;
	rdfs:domain osdu:Fluid ;
	rdfs:range osdu:Rheometer ;
.

###  https://w3id.org/osdu#hasRheometerViscosities
osdu:hasRheometerViscosities rdf:type owl:ObjectProperty ;
	rdfs:comment "Reference to the RheometerViscosities for the object " ;
	rdfs:domain osdu:Rheometer ;
	rdfs:range osdu:RheometerViscosity ;
.

###  https://w3id.org/osdu#hasRig
osdu:hasRig rdf:type owl:ObjectProperty ;
	rdfs:comment "Reference to the Rig for the object " ;
	rdfs:domain [
		rdf:type owl:Class ;
		owl:unionOf (
			osdu:VerticalMeasurementID
			osdu:WellActivityProgram
			osdu:RigUtilization
		) ;
	] ;
	rdfs:range osdu:Rig ;
.

###  https://w3id.org/osdu#hasRigUtilization
osdu:hasRigUtilization rdf:type owl:ObjectProperty ;
	rdfs:comment "Reference to the RigUtilization for the object " ;
	rdfs:domain osdu:WellBarrierElementTest ;
	rdfs:range osdu:RigUtilization ;
.

###  https://w3id.org/osdu#hasRiskCategory
osdu:hasRiskCategory rdf:type owl:ObjectProperty ;
	rdfs:comment "Reference to the RiskCategory for the object " ;
	rdfs:domain [
		rdf:type owl:Class ;
		owl:unionOf (
			osdu:Risk
			osdu:RiskSubCategory
		) ;
	] ;
	rdfs:range osdu:RiskCategory ;
.

###  https://w3id.org/osdu#hasRiskConsequenceCategory
osdu:hasRiskConsequenceCategory rdf:type owl:ObjectProperty ;
	rdfs:comment "Reference to the RiskConsequenceCategory for the object " ;
	rdfs:domain [
		rdf:type owl:Class ;
		owl:unionOf (
			osdu:Risk
			osdu:RiskConsequenceSubCategory
		) ;
	] ;
	rdfs:range osdu:RiskConsequenceCategory ;
.

###  https://w3id.org/osdu#hasRiskConsequenceSubCategory
osdu:hasRiskConsequenceSubCategory rdf:type owl:ObjectProperty ;
	rdfs:comment "Reference to the RiskConsequenceSubCategory for the object " ;
	rdfs:domain osdu:Risk ;
	rdfs:range osdu:RiskConsequenceSubCategory ;
.

###  https://w3id.org/osdu#hasRiskDiscipline
osdu:hasRiskDiscipline rdf:type owl:ObjectProperty ;
	rdfs:comment "Reference to the RiskDiscipline for the object " ;
	rdfs:domain osdu:Risk ;
	rdfs:range osdu:RiskDiscipline ;
.

###  https://w3id.org/osdu#hasRiskHierarchyLevel
osdu:hasRiskHierarchyLevel rdf:type owl:ObjectProperty ;
	rdfs:comment "Reference to the RiskHierarchyLevel for the object " ;
	rdfs:domain osdu:Risk ;
	rdfs:range osdu:RiskHierarchyLevel ;
.

###  https://w3id.org/osdu#hasRiskSubCategory
osdu:hasRiskSubCategory rdf:type owl:ObjectProperty ;
	rdfs:comment "Reference to the RiskSubCategory for the object " ;
	rdfs:domain osdu:Risk ;
	rdfs:range osdu:RiskSubCategory ;
.

###  https://w3id.org/osdu#hasRiskType
osdu:hasRiskType rdf:type owl:ObjectProperty ;
	rdfs:comment "Reference to the RiskType for the object " ;
	rdfs:domain osdu:Risk ;
	rdfs:range osdu:RiskType ;
.

###  https://w3id.org/osdu#hasRockSample
osdu:hasRockSample rdf:type owl:ObjectProperty ;
	rdfs:comment "Reference to the RockSample for the object " ;
	rdfs:domain [
		rdf:type owl:Class ;
		owl:unionOf (
			osdu:RockSample
			osdu:RockSampleAnalysis
		) ;
	] ;
	rdfs:range osdu:RockSample ;
.

###  https://w3id.org/osdu#hasRockSampleType
osdu:hasRockSampleType rdf:type owl:ObjectProperty ;
	rdfs:comment "Reference to the RockSampleType for the object " ;
	rdfs:domain osdu:RockSample ;
	rdfs:range osdu:RockSampleType ;
.

###  https://w3id.org/osdu#hasRockVolumeFeature
osdu:hasRockVolumeFeature rdf:type owl:ObjectProperty ;
	rdfs:comment "Reference to the RockVolumeFeature for the object " ;
	rdfs:domain [
		rdf:type owl:Class ;
		owl:unionOf (
			osdu:RockFluidUnitInterpretation
			osdu:AquiferInterpretation
			osdu:StratigraphicUnitInterpretation
			osdu:GeobodyInterpretation
			osdu:LocalRockVolumeFeature
		) ;
	] ;
	rdfs:range osdu:RockVolumeFeature ;
.

###  https://w3id.org/osdu#hasRoutineCoreAnalysis
osdu:hasRoutineCoreAnalysis rdf:type owl:ObjectProperty ;
	rdfs:comment "Reference to the RoutineCoreAnalysis for the object " ;
	rdfs:domain osdu:RockSampleAnalysis ;
	rdfs:range osdu:RoutineCoreAnalysis ;
.

###  https://w3id.org/osdu#hasRunParameterPlans
osdu:hasRunParameterPlans rdf:type owl:ObjectProperty ;
	rdfs:comment "Reference to the RunParameterPlans for the object " ;
	rdfs:domain osdu:BHARun ;
	rdfs:range osdu:RunParameterPlan ;
.

###  https://w3id.org/osdu#hasSampleOrientationType
osdu:hasSampleOrientationType rdf:type owl:ObjectProperty ;
	rdfs:comment "Reference to the SampleOrientationType for the object " ;
	rdfs:domain [
		rdf:type owl:Class ;
		owl:unionOf (
			osdu:RockSample
			osdu:RockSampleAnalysis
		) ;
	] ;
	rdfs:range osdu:SampleOrientationType ;
.

###  https://w3id.org/osdu#hasSampleRemarks
osdu:hasSampleRemarks rdf:type owl:ObjectProperty ;
	rdfs:comment "Reference to the SampleRemarks for the object " ;
	rdfs:domain osdu:RockSample ;
	rdfs:range osdu:SampleRemarks ;
.

###  https://w3id.org/osdu#hasSatelliteGeometry
osdu:hasSatelliteGeometry rdf:type owl:ObjectProperty ;
	rdfs:comment "Reference to the SatelliteGeometry for the object " ;
	rdfs:domain osdu:ProcessedInSAR ;
	rdfs:range osdu:SatelliteGeometry ;
.

###  https://w3id.org/osdu#hasSatelliteMission
osdu:hasSatelliteMission rdf:type owl:ObjectProperty ;
	rdfs:comment "Reference to the SatelliteMission for the object " ;
	rdfs:domain osdu:ProcessedInSAR ;
	rdfs:range osdu:SatelliteMission ;
.

###  https://w3id.org/osdu#hasSaturationMethodType
osdu:hasSaturationMethodType rdf:type owl:ObjectProperty ;
	rdfs:comment "Reference to the SaturationMethodType for the object " ;
	rdfs:domain osdu:RoutineCoreAnalysis ;
	rdfs:range osdu:SaturationMethodType ;
.

###  https://w3id.org/osdu#hasSchemaFormatType
osdu:hasSchemaFormatType rdf:type owl:ObjectProperty ;
	rdfs:comment "Reference to the SchemaFormatType for the object " ;
	rdfs:domain osdu:AbstractDataset ;
	rdfs:range osdu:SchemaFormatType ;
.

###  https://w3id.org/osdu#hasScope
osdu:hasScope rdf:type owl:ObjectProperty ;
	rdfs:comment "Reference to the Scope for the object " ;
	rdfs:domain [
		rdf:type owl:Class ;
		owl:unionOf (
			osdu:Usage
			osdu:PreferredUsage
		) ;
	] ;
	rdfs:range osdu:Scope ;
.

###  https://w3id.org/osdu#hasSectionType
osdu:hasSectionType rdf:type owl:ObjectProperty ;
	rdfs:comment "Reference to the SectionType for the object " ;
	rdfs:domain osdu:TubularComponent ;
	rdfs:range osdu:SectionType ;
.

###  https://w3id.org/osdu#hasSecuritySchemeType
osdu:hasSecuritySchemeType rdf:type owl:ObjectProperty ;
	rdfs:comment "Reference to the SecuritySchemeType for the object " ;
	rdfs:domain osdu:SecurityScheme ;
	rdfs:range osdu:SecuritySchemeType ;
.

###  https://w3id.org/osdu#hasSecuritySchemes
osdu:hasSecuritySchemes rdf:type owl:ObjectProperty ;
	rdfs:comment "Reference to the SecuritySchemes for the object " ;
	rdfs:domain osdu:ConnectedSourceRegistryEntry ;
	rdfs:range osdu:SecurityScheme ;
.

###  https://w3id.org/osdu#hasSeismic2DInterpretationSet
osdu:hasSeismic2DInterpretationSet rdf:type owl:ObjectProperty ;
	rdfs:comment "Reference to the Seismic2DInterpretationSet for the object " ;
	rdfs:domain [
		rdf:type owl:Class ;
		owl:unionOf (
			osdu:SeismicTraceData
			osdu:SeismicHorizon
			osdu:SeismicLineGeometry
		) ;
	] ;
	rdfs:range osdu:Seismic2DInterpretationSet ;
.

###  https://w3id.org/osdu#hasSeismic3DInterpretationSet
osdu:hasSeismic3DInterpretationSet rdf:type owl:ObjectProperty ;
	rdfs:comment "Reference to the Seismic3DInterpretationSet for the object " ;
	rdfs:domain [
		rdf:type owl:Class ;
		owl:unionOf (
			osdu:SeismicTraceData
			osdu:SeismicHorizon
		) ;
	] ;
	rdfs:range osdu:Seismic3DInterpretationSet ;
.

###  https://w3id.org/osdu#hasSeismicAcquisitionSurvey
osdu:hasSeismicAcquisitionSurvey rdf:type owl:ObjectProperty ;
	rdfs:comment "Reference to the SeismicAcquisitionSurvey for the object " ;
	rdfs:domain osdu:SeismicTraceData ;
	rdfs:range osdu:SeismicAcquisitionSurvey ;
.

###  https://w3id.org/osdu#hasSeismicAcquisitionType
osdu:hasSeismicAcquisitionType rdf:type owl:ObjectProperty ;
	rdfs:comment "Reference to the SeismicAcquisitionType for the object " ;
	rdfs:domain osdu:SeismicAcquisitionSurvey ;
	rdfs:range osdu:SeismicAcquisitionType ;
.

###  https://w3id.org/osdu#hasSeismicAttributeType
osdu:hasSeismicAttributeType rdf:type owl:ObjectProperty ;
	rdfs:comment "Reference to the SeismicAttributeType for the object " ;
	rdfs:domain [
		rdf:type owl:Class ;
		owl:unionOf (
			osdu:SeismicTraceData
			osdu:SeismicAttributes
		) ;
	] ;
	rdfs:range osdu:SeismicAttributeType ;
.

###  https://w3id.org/osdu#hasSeismicAttributes
osdu:hasSeismicAttributes rdf:type owl:ObjectProperty ;
	rdfs:comment "Reference to the SeismicAttributes for the object " ;
	rdfs:domain osdu:SeismicHorizon ;
	rdfs:range osdu:SeismicAttributes ;
.

###  https://w3id.org/osdu#hasSeismicBinGrid
osdu:hasSeismicBinGrid rdf:type owl:ObjectProperty ;
	rdfs:comment "Reference to the SeismicBinGrid for the object " ;
	rdfs:domain [
		rdf:type owl:Class ;
		owl:unionOf (
			osdu:DInterpretationSet
			osdu:SeismicProcessingProject
			osdu:VelocityModeling
			osdu:SeismicTraceData
			osdu:GeoReferencedImage
			osdu:FaultSystem
			osdu:SeismicHorizon
			osdu:SeismicFault
		) ;
	] ;
	rdfs:range osdu:SeismicBinGrid ;
.

###  https://w3id.org/osdu#hasSeismicBinGridType
osdu:hasSeismicBinGridType rdf:type owl:ObjectProperty ;
	rdfs:comment "Reference to the SeismicBinGridType for the object " ;
	rdfs:domain osdu:AbstractBinGrid ;
	rdfs:range osdu:SeismicBinGridType ;
.

###  https://w3id.org/osdu#hasSeismicDomainType
osdu:hasSeismicDomainType rdf:type owl:ObjectProperty ;
	rdfs:comment "Reference to the SeismicDomainType for the object " ;
	rdfs:domain [
		rdf:type owl:Class ;
		owl:unionOf (
			osdu:VelocityModeling
			osdu:SeismicTraceData
			osdu:FaultSystem
			osdu:SeismicHorizon
			osdu:SeismicFault
		) ;
	] ;
	rdfs:range osdu:SeismicDomainType ;
.

###  https://w3id.org/osdu#hasSeismicEnergySourceType
osdu:hasSeismicEnergySourceType rdf:type owl:ObjectProperty ;
	rdfs:comment "Reference to the SeismicEnergySourceType for the object " ;
	rdfs:domain [
		rdf:type owl:Class ;
		owl:unionOf (
			osdu:SeismicAcquisitionSurvey
			osdu:SeismicSourceConfiguration
		) ;
	] ;
	rdfs:range osdu:SeismicEnergySourceType ;
.

###  https://w3id.org/osdu#hasSeismicFaultType
osdu:hasSeismicFaultType rdf:type owl:ObjectProperty ;
	rdfs:comment "Reference to the SeismicFaultType for the object " ;
	rdfs:domain [
		rdf:type owl:Class ;
		owl:unionOf (
			osdu:Faults
			osdu:SeismicFault
		) ;
	] ;
	rdfs:range osdu:SeismicFaultType ;
.

###  https://w3id.org/osdu#hasSeismicFilteringType
osdu:hasSeismicFilteringType rdf:type owl:ObjectProperty ;
	rdfs:comment "Reference to the SeismicFilteringType for the object " ;
	rdfs:domain osdu:SeismicTraceData ;
	rdfs:range osdu:SeismicFilteringType ;
.

###  https://w3id.org/osdu#hasSeismicGatherType
osdu:hasSeismicGatherType rdf:type owl:ObjectProperty ;
	rdfs:comment "Reference to the SeismicGatherType for the object " ;
	rdfs:domain osdu:SeismicTraceData ;
	rdfs:range osdu:SeismicGatherType ;
.

###  https://w3id.org/osdu#hasSeismicGeometryType
osdu:hasSeismicGeometryType rdf:type owl:ObjectProperty ;
	rdfs:comment "Reference to the SeismicGeometryType for the object " ;
	rdfs:domain [
		rdf:type owl:Class ;
		owl:unionOf (
			osdu:SeismicAcquisitionSurvey
			osdu:SeismicGeometryType
		) ;
	] ;
	rdfs:range osdu:SeismicGeometryType ;
.

###  https://w3id.org/osdu#hasSeismicHorizonType
osdu:hasSeismicHorizonType rdf:type owl:ObjectProperty ;
	rdfs:comment "Reference to the SeismicHorizonType for the object " ;
	rdfs:domain osdu:SeismicHorizon ;
	rdfs:range osdu:SeismicHorizonType ;
.

###  https://w3id.org/osdu#hasSeismicLineGeometries
osdu:hasSeismicLineGeometries rdf:type owl:ObjectProperty ;
	rdfs:comment "Reference to the SeismicLineGeometries for the object " ;
	rdfs:domain osdu:DInterpretationSet ;
	rdfs:range osdu:SeismicLineGeometries ;
.

###  https://w3id.org/osdu#hasSeismicLineGeometry
osdu:hasSeismicLineGeometry rdf:type owl:ObjectProperty ;
	rdfs:comment "Reference to the SeismicLineGeometry for the object " ;
	rdfs:domain [
		rdf:type owl:Class ;
		owl:unionOf (
			osdu:SeismicLineGeometries
			osdu:SeismicTraceData
		) ;
	] ;
	rdfs:range osdu:SeismicLineGeometry ;
.

###  https://w3id.org/osdu#hasSeismicMigrationType
osdu:hasSeismicMigrationType rdf:type owl:ObjectProperty ;
	rdfs:comment "Reference to the SeismicMigrationType for the object " ;
	rdfs:domain osdu:SeismicTraceData ;
	rdfs:range osdu:SeismicMigrationType ;
.

###  https://w3id.org/osdu#hasSeismicPickingType
osdu:hasSeismicPickingType rdf:type owl:ObjectProperty ;
	rdfs:comment "Reference to the SeismicPickingType for the object " ;
	rdfs:domain [
		rdf:type owl:Class ;
		owl:unionOf (
			osdu:FaultSystem
			osdu:Faults
			osdu:SeismicHorizon
			osdu:SeismicFault
		) ;
	] ;
	rdfs:range osdu:SeismicPickingType ;
.

###  https://w3id.org/osdu#hasSeismicProcessingProject
osdu:hasSeismicProcessingProject rdf:type owl:ObjectProperty ;
	rdfs:comment "Reference to the SeismicProcessingProject for the object " ;
	rdfs:domain osdu:SeismicTraceData ;
	rdfs:range osdu:SeismicProcessingProject ;
.

###  https://w3id.org/osdu#hasSeismicProcessingStageType
osdu:hasSeismicProcessingStageType rdf:type owl:ObjectProperty ;
	rdfs:comment "Reference to the SeismicProcessingStageType for the object " ;
	rdfs:domain osdu:SeismicTraceData ;
	rdfs:range osdu:SeismicProcessingStageType ;
.

###  https://w3id.org/osdu#hasSeismicReceiverType
osdu:hasSeismicReceiverType rdf:type owl:ObjectProperty ;
	rdfs:comment "Reference to the SeismicReceiverType for the object " ;
	rdfs:domain osdu:SeismicReceiverConfiguration ;
	rdfs:range osdu:SeismicReceiverType ;
.

###  https://w3id.org/osdu#hasSeismicReferenceElevation
osdu:hasSeismicReferenceElevation rdf:type owl:ObjectProperty ;
	rdfs:comment "Reference to the SeismicReferenceElevation for the object " ;
	rdfs:domain osdu:WellLog ;
	rdfs:range osdu:AbstractFacilityVerticalMeasurement ;
.

###  https://w3id.org/osdu#hasSeismicStackingType
osdu:hasSeismicStackingType rdf:type owl:ObjectProperty ;
	rdfs:comment "Reference to the SeismicStackingType for the object " ;
	rdfs:domain osdu:SeismicTraceData ;
	rdfs:range osdu:SeismicStackingType ;
.

###  https://w3id.org/osdu#hasSeismicTraceDataDimensionalityType
osdu:hasSeismicTraceDataDimensionalityType rdf:type owl:ObjectProperty ;
	rdfs:comment "Reference to the SeismicTraceDataDimensionalityType for the object " ;
	rdfs:domain osdu:SeismicTraceData ;
	rdfs:range osdu:SeismicTraceDataDimensionalityType ;
.

###  https://w3id.org/osdu#hasSeismicTraceSortOrder
osdu:hasSeismicTraceSortOrder rdf:type owl:ObjectProperty ;
	rdfs:comment "Reference to the SeismicTraceSortOrder for the object " ;
	rdfs:domain osdu:SeismicTraceData ;
	rdfs:range osdu:SeismicTraceSortOrder ;
.

###  https://w3id.org/osdu#hasSeismicWaveType
osdu:hasSeismicWaveType rdf:type owl:ObjectProperty ;
	rdfs:comment "Reference to the SeismicWaveType for the object " ;
	rdfs:domain osdu:SeismicTraceData ;
	rdfs:range osdu:SeismicWaveType ;
.

###  https://w3id.org/osdu#hasSequenceStratigraphySurfaceType
osdu:hasSequenceStratigraphySurfaceType rdf:type owl:ObjectProperty ;
	rdfs:comment "Reference to the SequenceStratigraphySurfaceType for the object " ;
	rdfs:domain osdu:HorizonInterpretation ;
	rdfs:range osdu:SequenceStratigraphySurfaceType ;
.

###  https://w3id.org/osdu#hasSingleCellAquiferSet
osdu:hasSingleCellAquiferSet rdf:type owl:ObjectProperty ;
	rdfs:comment "Reference to the SingleCellAquiferSet for the object " ;
	rdfs:domain osdu:IjkGridNumericalAquiferRepresentation ;
	rdfs:range osdu:SingleCellAquifer ;
.

###  https://w3id.org/osdu#hasSoftwareSpecifications
osdu:hasSoftwareSpecifications rdf:type owl:ObjectProperty ;
	rdfs:comment "Reference to the SoftwareSpecifications for the object " ;
	rdfs:domain osdu:AbstractWPCActivity ;
	rdfs:range osdu:Software ;
.

###  https://w3id.org/osdu#hasSourceCRS
osdu:hasSourceCRS rdf:type owl:ObjectProperty ;
	rdfs:comment "Reference to the SourceCRS for the object " ;
	rdfs:domain [
		rdf:type owl:Class ;
		owl:unionOf (
			osdu:CoordinateTransformation
			osdu:CoordinateReferenceSystem
		) ;
	] ;
	rdfs:range osdu:SourceCRS ;
.

###  https://w3id.org/osdu#hasSourceConfigurations
osdu:hasSourceConfigurations rdf:type owl:ObjectProperty ;
	rdfs:comment "Reference to the SourceConfigurations for the object " ;
	rdfs:domain osdu:SeismicAcquisitionSurvey ;
	rdfs:range osdu:SeismicSourceConfiguration ;
.

###  https://w3id.org/osdu#hasSpatialArea
osdu:hasSpatialArea rdf:type owl:ObjectProperty ;
	rdfs:comment "Reference to the SpatialArea for the object " ;
	rdfs:domain [
		rdf:type owl:Class ;
		owl:unionOf (
			osdu:AbstractWorkProductComponent
			osdu:WorkProduct
		) ;
	] ;
	rdfs:range osdu:AbstractSpatialLocation ;
.

###  https://w3id.org/osdu#hasSpatialGeometryType
osdu:hasSpatialGeometryType rdf:type owl:ObjectProperty ;
	rdfs:comment "Reference to the SpatialGeometryType for the object " ;
	rdfs:domain osdu:AbstractSpatialLocation ;
	rdfs:range osdu:SpatialGeometryType ;
.

###  https://w3id.org/osdu#hasSpatialLocation
osdu:hasSpatialLocation rdf:type owl:ObjectProperty ;
	rdfs:comment "Reference to the SpatialLocation for the object " ;
	rdfs:domain osdu:AbstractMaster ;
	rdfs:range osdu:AbstractSpatialLocation ;
.

###  https://w3id.org/osdu#hasSpatialParameterType
osdu:hasSpatialParameterType rdf:type owl:ObjectProperty ;
	rdfs:comment "Reference to the SpatialParameterType for the object " ;
	rdfs:domain osdu:AbstractSpatialLocation ;
	rdfs:range osdu:SpatialParameterType ;
.

###  https://w3id.org/osdu#hasSpatialPoint
osdu:hasSpatialPoint rdf:type owl:ObjectProperty ;
	rdfs:comment "Reference to the SpatialPoint for the object " ;
	rdfs:domain [
		rdf:type owl:Class ;
		owl:unionOf (
			osdu:AbstractWorkProductComponent
			osdu:WorkProduct
		) ;
	] ;
	rdfs:range osdu:AbstractSpatialLocation ;
.

###  https://w3id.org/osdu#hasSpatialReference
osdu:hasSpatialReference rdf:type owl:ObjectProperty ;
	rdfs:comment "Reference to the SpatialReference for the object " ;
	rdfs:domain [
		rdf:type owl:Class ;
		owl:unionOf (
			osdu:Shape
			osdu:WorldFile
		) ;
	] ;
	rdfs:range osdu:AbstractSpatialReference ;
.

###  https://w3id.org/osdu#hasStackAngleRanges
osdu:hasStackAngleRanges rdf:type owl:ObjectProperty ;
	rdfs:comment "Reference to the StackAngleRanges for the object " ;
	rdfs:domain osdu:SeismicTraceData ;
	rdfs:range osdu:AngleRange ;
.

###  https://w3id.org/osdu#hasStackAzimuthRanges
osdu:hasStackAzimuthRanges rdf:type owl:ObjectProperty ;
	rdfs:comment "Reference to the StackAzimuthRanges for the object " ;
	rdfs:domain osdu:SeismicTraceData ;
	rdfs:range osdu:AngleRange ;
.

###  https://w3id.org/osdu#hasStackOffsetRanges
osdu:hasStackOffsetRanges rdf:type owl:ObjectProperty ;
	rdfs:comment "Reference to the StackOffsetRanges for the object " ;
	rdfs:domain osdu:SeismicTraceData ;
	rdfs:range osdu:LengthRange ;
.

###  https://w3id.org/osdu#hasStandardsOrganisation
osdu:hasStandardsOrganisation rdf:type owl:ObjectProperty ;
	rdfs:comment "Reference to the StandardsOrganisation for the object " ;
	rdfs:domain [
		rdf:type owl:Class ;
		owl:unionOf (
			osdu:AbstractAliasNames
			osdu:LogCurveType
		) ;
	] ;
	rdfs:range osdu:StandardsOrganisation ;
.

###  https://w3id.org/osdu#hasStatusInfo
osdu:hasStatusInfo rdf:type owl:ObjectProperty ;
	rdfs:comment "Reference to the StatusInfo for the object " ;
	rdfs:domain osdu:OperationsReport ;
	rdfs:range osdu:DrillingReportStatusInfo ;
.

###  https://w3id.org/osdu#hasStorageFacility
osdu:hasStorageFacility rdf:type owl:ObjectProperty ;
	rdfs:comment "Reference to the StorageFacility for the object " ;
	rdfs:domain osdu:AbstractStorageLocation ;
	rdfs:range osdu:StorageFacility ;
.

###  https://w3id.org/osdu#hasStratigraphicColumn
osdu:hasStratigraphicColumn rdf:type owl:ObjectProperty ;
	rdfs:comment "Reference to the StratigraphicColumn for the object " ;
	rdfs:domain [
		rdf:type owl:Class ;
		owl:unionOf (
			osdu:EarthModelInterpretation
			osdu:WellboreMarkerSet
			osdu:WellboreIntervalSet
		) ;
	] ;
	rdfs:range osdu:StratigraphicColumn ;
.

###  https://w3id.org/osdu#hasStratigraphicColumnRankInterpretation
osdu:hasStratigraphicColumnRankInterpretation rdf:type owl:ObjectProperty ;
	rdfs:comment "Reference to the StratigraphicColumnRankInterpretation for the object " ;
	rdfs:domain [
		rdf:type owl:Class ;
		owl:unionOf (
			osdu:StratigraphicUnits
			osdu:WellboreMarkerSet
			osdu:GeologicUnitOccurrenceInterpretation
			osdu:WellboreIntervalSet
		) ;
	] ;
	rdfs:range osdu:StratigraphicColumnRankInterpretation ;
.

###  https://w3id.org/osdu#hasStratigraphicColumnRankUnitType
osdu:hasStratigraphicColumnRankUnitType rdf:type owl:ObjectProperty ;
	rdfs:comment "Reference to the StratigraphicColumnRankUnitType for the object " ;
	rdfs:domain osdu:ChronoStratigraphy ;
	rdfs:range osdu:StratigraphicColumnRankUnitType ;
.

###  https://w3id.org/osdu#hasStratigraphicRoleType
osdu:hasStratigraphicRoleType rdf:type owl:ObjectProperty ;
	rdfs:comment "Reference to the StratigraphicRoleType for the object " ;
	rdfs:domain [
		rdf:type owl:Class ;
		owl:unionOf (
			osdu:HorizonInterpretation
			osdu:StratigraphicUnitInterpretation
			osdu:StratigraphicColumnRankUnitType
		) ;
	] ;
	rdfs:range osdu:StratigraphicRoleType ;
.

###  https://w3id.org/osdu#hasStratigraphicUnits
osdu:hasStratigraphicUnits rdf:type owl:ObjectProperty ;
	rdfs:comment "Reference to the StratigraphicUnits for the object " ;
	rdfs:domain osdu:AbstractGridRepresentation ;
	rdfs:range osdu:StratigraphicUnits ;
.

###  https://w3id.org/osdu#hasStringClass
osdu:hasStringClass rdf:type owl:ObjectProperty ;
	rdfs:comment "Reference to the StringClass for the object " ;
	rdfs:domain osdu:TubularAssembly ;
	rdfs:range osdu:StringClass ;
.

###  https://w3id.org/osdu#hasStructuralOrganizationInterpretation
osdu:hasStructuralOrganizationInterpretation rdf:type owl:ObjectProperty ;
	rdfs:comment "Reference to the StructuralOrganizationInterpretation for the object " ;
	rdfs:domain [
		rdf:type owl:Class ;
		owl:unionOf (
			osdu:SealedSurfaceFramework
			osdu:UnsealedSurfaceFramework
		) ;
	] ;
	rdfs:range osdu:StructuralOrganizationInterpretation ;
.

###  https://w3id.org/osdu#hasSurveySections
osdu:hasSurveySections rdf:type owl:ObjectProperty ;
	rdfs:comment "Reference to the SurveySections for the object " ;
	rdfs:domain osdu:SurveyProgram ;
	rdfs:range osdu:SurveySection ;
.

###  https://w3id.org/osdu#hasSurveyToolType
osdu:hasSurveyToolType rdf:type owl:ObjectProperty ;
	rdfs:comment "Reference to the SurveyToolType for the object " ;
	rdfs:domain [
		rdf:type owl:Class ;
		owl:unionOf (
			osdu:SurveySection
			osdu:WellboreTrajectory
		) ;
	] ;
	rdfs:range osdu:SurveyToolType ;
.

###  https://w3id.org/osdu#hasTargetCRS
osdu:hasTargetCRS rdf:type owl:ObjectProperty ;
	rdfs:comment "Reference to the TargetCRS for the object " ;
	rdfs:domain [
		rdf:type owl:Class ;
		owl:unionOf (
			osdu:CoordinateTransformation
			osdu:CoordinateReferenceSystem
		) ;
	] ;
	rdfs:range osdu:TargetCRS ;
.

###  https://w3id.org/osdu#hasTargets
osdu:hasTargets rdf:type owl:ObjectProperty ;
	rdfs:comment "Reference to the Targets for the object " ;
	rdfs:domain osdu:GeometricTargetSet ;
	rdfs:range osdu:Target ;
.

###  https://w3id.org/osdu#hasTechnicalAssuranceType
osdu:hasTechnicalAssuranceType rdf:type owl:ObjectProperty ;
	rdfs:comment "Reference to the TechnicalAssuranceType for the object " ;
	rdfs:domain [
		rdf:type owl:Class ;
		owl:unionOf (
			osdu:AbstractTechnicalAssurance
			osdu:AbstractMaster
			osdu:AbstractCommonResources
		) ;
	] ;
	rdfs:range osdu:TechnicalAssuranceType ;
.

###  https://w3id.org/osdu#hasTectonicSettingType
osdu:hasTectonicSettingType rdf:type owl:ObjectProperty ;
	rdfs:comment "Reference to the TectonicSettingType for the object " ;
	rdfs:domain osdu:StructuralOrganizationInterpretation ;
	rdfs:range osdu:TectonicSettingType ;
.

###  https://w3id.org/osdu#hasTerms
osdu:hasTerms rdf:type owl:ObjectProperty ;
	rdfs:comment "Reference to the Terms for the object " ;
	rdfs:domain osdu:Agreement ;
	rdfs:range osdu:Terms ;
.

###  https://w3id.org/osdu#hasTestFluids
osdu:hasTestFluids rdf:type owl:ObjectProperty ;
	rdfs:comment "Reference to the TestFluids for the object " ;
	rdfs:domain osdu:WBETestStep ;
	rdfs:range osdu:TestFluid ;
.

###  https://w3id.org/osdu#hasTestSteps
osdu:hasTestSteps rdf:type owl:ObjectProperty ;
	rdfs:comment "Reference to the TestSteps for the object " ;
	rdfs:domain osdu:WellBarrierElementTest ;
	rdfs:range osdu:WBETestStep ;
.

###  https://w3id.org/osdu#hasTestSubType
osdu:hasTestSubType rdf:type owl:ObjectProperty ;
	rdfs:comment "Reference to the TestSubType for the object " ;
	rdfs:domain osdu:WellBarrierElementTest ;
	rdfs:range osdu:TestSubType ;
.

###  https://w3id.org/osdu#hasTestType
osdu:hasTestType rdf:type owl:ObjectProperty ;
	rdfs:comment "Reference to the TestType for the object " ;
	rdfs:domain osdu:WellBarrierElementTest ;
	rdfs:range osdu:TestType ;
.

###  https://w3id.org/osdu#hasTimeLapse
osdu:hasTimeLapse rdf:type owl:ObjectProperty ;
	rdfs:comment "Reference to the TimeLapse for the object " ;
	rdfs:domain osdu:SeismicTraceData ;
	rdfs:range osdu:TimeLapse ;
.

###  https://w3id.org/osdu#hasTimeSeries
osdu:hasTimeSeries rdf:type owl:ObjectProperty ;
	rdfs:comment "Reference to the TimeSeries for the object " ;
	rdfs:domain [
		rdf:type owl:Class ;
		owl:unionOf (
			osdu:AbstractRepresentation
			osdu:TimeSeries
			osdu:TimeLapse
			osdu:GenericProperty
		) ;
	] ;
	rdfs:range osdu:TimeSeries ;
.

###  https://w3id.org/osdu#hasTimedComments
osdu:hasTimedComments rdf:type owl:ObjectProperty ;
	rdfs:comment "Reference to the TimedComments for the object " ;
	rdfs:domain osdu:OperationsReport ;
	rdfs:range osdu:TimedComment ;
.

###  https://w3id.org/osdu#hasTorqueOnBottomGroup
osdu:hasTorqueOnBottomGroup rdf:type owl:ObjectProperty ;
	rdfs:comment "Reference to the TorqueOnBottomGroup for the object " ;
	rdfs:domain osdu:OperationParameterPlan ;
	rdfs:range osdu:TorqueOnBottomGroup ;
.

###  https://w3id.org/osdu#hasTrajectoryStationPropertyType
osdu:hasTrajectoryStationPropertyType rdf:type owl:ObjectProperty ;
	rdfs:comment "Reference to the TrajectoryStationPropertyType for the object " ;
	rdfs:domain osdu:Curve ;
	rdfs:range osdu:TrajectoryStationPropertyType ;
.

###  https://w3id.org/osdu#hasTransformation
osdu:hasTransformation rdf:type owl:ObjectProperty ;
	rdfs:comment "Reference to the Transformation for the object " ;
	rdfs:domain osdu:CoordinateReferenceSystem ;
	rdfs:range osdu:Transformation ;
.

###  https://w3id.org/osdu#hasTubularAssembly
osdu:hasTubularAssembly rdf:type owl:ObjectProperty ;
	rdfs:comment "Reference to the TubularAssembly for the object " ;
	rdfs:domain [
		rdf:type owl:Class ;
		owl:unionOf (
			osdu:FluidsInterval
			osdu:InstalledTubular
			osdu:CasingDesign
			osdu:DrillingActivity
			osdu:BHARun
			osdu:PerforationJob
			osdu:PlannedCementJob
			osdu:TubularAssembly
			osdu:TubularUmbilical
			osdu:TubularComponent
		) ;
	] ;
	rdfs:range osdu:TubularAssembly ;
.

###  https://w3id.org/osdu#hasTubularAssemblyStatus
osdu:hasTubularAssemblyStatus rdf:type owl:ObjectProperty ;
	rdfs:comment "Reference to the TubularAssemblyStatus for the object " ;
	rdfs:domain osdu:TubularAssembly ;
	rdfs:range osdu:TubularAssemblyStatus ;
.

###  https://w3id.org/osdu#hasTubularAssemblyStatusType
osdu:hasTubularAssemblyStatusType rdf:type owl:ObjectProperty ;
	rdfs:comment "Reference to the TubularAssemblyStatusType for the object " ;
	rdfs:domain osdu:TubularAssemblyStatus ;
	rdfs:range osdu:TubularAssemblyStatusType ;
.

###  https://w3id.org/osdu#hasTubularAssemblyType
osdu:hasTubularAssemblyType rdf:type owl:ObjectProperty ;
	rdfs:comment "Reference to the TubularAssemblyType for the object " ;
	rdfs:domain osdu:TubularAssembly ;
	rdfs:range osdu:TubularAssemblyType ;
.

###  https://w3id.org/osdu#hasTubularComponent
osdu:hasTubularComponent rdf:type owl:ObjectProperty ;
	rdfs:comment "Reference to the TubularComponent for the object " ;
	rdfs:domain [
		rdf:type owl:Class ;
		owl:unionOf (
			osdu:PlannedCementJob
			osdu:TubularUmbilical
		) ;
	] ;
	rdfs:range osdu:TubularComponent ;
.

###  https://w3id.org/osdu#hasTubularComponentConnectionType
osdu:hasTubularComponentConnectionType rdf:type owl:ObjectProperty ;
	rdfs:comment "Reference to the TubularComponentConnectionType for the object " ;
	rdfs:domain osdu:TubularComponent ;
	rdfs:range osdu:TubularComponentConnectionType ;
.

###  https://w3id.org/osdu#hasTubularComponentGrade
osdu:hasTubularComponentGrade rdf:type owl:ObjectProperty ;
	rdfs:comment "Reference to the TubularComponentGrade for the object " ;
	rdfs:domain osdu:TubularComponent ;
	rdfs:range osdu:TubularComponentGrade ;
.

###  https://w3id.org/osdu#hasTubularComponentPinBoxType
osdu:hasTubularComponentPinBoxType rdf:type owl:ObjectProperty ;
	rdfs:comment "Reference to the TubularComponentPinBoxType for the object " ;
	rdfs:domain osdu:TubularComponent ;
	rdfs:range osdu:TubularComponentPinBoxType ;
.

###  https://w3id.org/osdu#hasTubularComponentType
osdu:hasTubularComponentType rdf:type owl:ObjectProperty ;
	rdfs:comment "Reference to the TubularComponentType for the object " ;
	rdfs:domain osdu:TubularComponent ;
	rdfs:range osdu:TubularComponentType ;
.

###  https://w3id.org/osdu#hasTubularMaterialType
osdu:hasTubularMaterialType rdf:type owl:ObjectProperty ;
	rdfs:comment "Reference to the TubularMaterialType for the object " ;
	rdfs:domain osdu:TubularComponent ;
	rdfs:range osdu:TubularMaterialType ;
.

###  https://w3id.org/osdu#hasTubularUmbilicalServiceType
osdu:hasTubularUmbilicalServiceType rdf:type owl:ObjectProperty ;
	rdfs:comment "Reference to the TubularUmbilicalServiceType for the object " ;
	rdfs:domain osdu:TubularUmbilical ;
	rdfs:range osdu:TubularUmbilicalServiceType ;
.

###  https://w3id.org/osdu#hasTubularUmbilicalType
osdu:hasTubularUmbilicalType rdf:type owl:ObjectProperty ;
	rdfs:comment "Reference to the TubularUmbilicalType for the object " ;
	rdfs:domain osdu:TubularUmbilical ;
	rdfs:range osdu:TubularUmbilicalType ;
.

###  https://w3id.org/osdu#hasUnacceptableUsage
osdu:hasUnacceptableUsage rdf:type owl:ObjectProperty ;
	rdfs:comment "Reference to the UnacceptableUsage for the object " ;
	rdfs:domain osdu:AbstractTechnicalAssurance ;
	rdfs:range osdu:UnacceptableUsage ;
.

###  https://w3id.org/osdu#hasUnitOfMeasure
osdu:hasUnitOfMeasure rdf:type owl:ObjectProperty ;
	rdfs:comment "Reference to the UnitOfMeasure for the object " ;
	rdfs:domain [
		rdf:type owl:Class ;
		owl:unionOf (
			osdu:AbstractAnyCrsFeatureCollection
			osdu:FrameOfReferenceUOM
			osdu:AbstractActivityParameter
			osdu:ProjectSpecifications
			osdu:AbstractFacilitySpecification
			osdu:AbstractFacilityVerticalMeasurement
			osdu:Point
			osdu:PointsSource
			osdu:MarkerProperty
			osdu:AbstractSpecification
			osdu:Curve
			osdu:GenericProperty
			osdu:ExternalUnitOfMeasure
			osdu:CoordinateSystem
			osdu:ParameterType
			osdu:Configuration
		) ;
	] ;
	rdfs:range osdu:UnitOfMeasure ;
.

###  https://w3id.org/osdu#hasUnitOfMeasureConfiguration
osdu:hasUnitOfMeasureConfiguration rdf:type owl:ObjectProperty ;
	rdfs:comment "Reference to the UnitOfMeasureConfiguration for the object " ;
	rdfs:domain osdu:UnitOfMeasureConfiguration ;
	rdfs:range osdu:UnitOfMeasureConfiguration ;
.

###  https://w3id.org/osdu#hasUnitQuantity
osdu:hasUnitQuantity rdf:type owl:ObjectProperty ;
	rdfs:comment "Reference to the UnitQuantity for the object " ;
	rdfs:domain [
		rdf:type owl:Class ;
		owl:unionOf (
			osdu:AbstractReferencePropertyType
			osdu:FluidFacet
			osdu:ParameterTemplate
			osdu:UnitOfMeasure
			osdu:ExternalUnitOfMeasure
			osdu:LogCurveType
			osdu:PropertyType
			osdu:LogCurveFamily
			osdu:ExternalUnitQuantity
			osdu:ParameterType
			osdu:Configuration
		) ;
	] ;
	rdfs:range osdu:UnitQuantity ;
.

###  https://w3id.org/osdu#hasUsages
osdu:hasUsages rdf:type owl:ObjectProperty ;
	rdfs:comment "Reference to the Usages for the object " ;
	rdfs:domain [
		rdf:type owl:Class ;
		owl:unionOf (
			osdu:CoordinateTransformation
			osdu:CoordinateReferenceSystem
		) ;
	] ;
	rdfs:range osdu:Usage ;
.

###  https://w3id.org/osdu#hasVectorHeaderMapping
osdu:hasVectorHeaderMapping rdf:type owl:ObjectProperty ;
	rdfs:comment "Reference to the VectorHeaderMapping for the object " ;
	rdfs:domain osdu:AbstractVectorHeaderMapping ;
	rdfs:range osdu:VectorHeaderMapping ;
.

###  https://w3id.org/osdu#hasVelocityAnalysisMethod
osdu:hasVelocityAnalysisMethod rdf:type owl:ObjectProperty ;
	rdfs:comment "Reference to the VelocityAnalysisMethod for the object " ;
	rdfs:domain osdu:VelocityModeling ;
	rdfs:range osdu:VelocityAnalysisMethod ;
.

###  https://w3id.org/osdu#hasVelocityModeling
osdu:hasVelocityModeling rdf:type owl:ObjectProperty ;
	rdfs:comment "Reference to the VelocityModeling for the object " ;
	rdfs:domain osdu:SeismicHorizon ;
	rdfs:range osdu:VelocityModeling ;
.

###  https://w3id.org/osdu#hasVerticalCRS
osdu:hasVerticalCRS rdf:type owl:ObjectProperty ;
	rdfs:comment "Reference to the VerticalCRS for the object " ;
	rdfs:domain osdu:CoordinateReferenceSystem ;
	rdfs:range osdu:VerticalCRS ;
.

###  https://w3id.org/osdu#hasVerticalMeasurement
osdu:hasVerticalMeasurement rdf:type owl:ObjectProperty ;
	rdfs:comment "Reference to the VerticalMeasurement for the object " ;
	rdfs:domain [
		rdf:type owl:Class ;
		owl:unionOf (
			osdu:WellPlanningWellbore
			osdu:RockSample
			osdu:SeismicAcquisitionSurvey
			osdu:PerforationJob
			osdu:PerforationInterval
			osdu:Coring
			osdu:WellLog
			osdu:WellboreMarkerSet
			osdu:RockSampleAnalysis
			osdu:PPFGDataset
			osdu:WellboreTrajectory
			osdu:WellboreIntervalSet
		) ;
	] ;
	rdfs:range osdu:AbstractFacilityVerticalMeasurement ;
.

###  https://w3id.org/osdu#hasVerticalMeasurementPath
osdu:hasVerticalMeasurementPath rdf:type owl:ObjectProperty ;
	rdfs:comment "Reference to the VerticalMeasurementPath for the object " ;
	rdfs:domain [
		rdf:type owl:Class ;
		owl:unionOf (
			osdu:AbstractReferenceLevel
			osdu:AbstractFacilityVerticalMeasurement
		) ;
	] ;
	rdfs:range osdu:VerticalMeasurementPath ;
.

###  https://w3id.org/osdu#hasVerticalMeasurementSource
osdu:hasVerticalMeasurementSource rdf:type owl:ObjectProperty ;
	rdfs:comment "Reference to the VerticalMeasurementSource for the object " ;
	rdfs:domain [
		rdf:type owl:Class ;
		owl:unionOf (
			osdu:AbstractReferenceLevel
			osdu:AbstractFacilityVerticalMeasurement
		) ;
	] ;
	rdfs:range osdu:VerticalMeasurementSource ;
.

###  https://w3id.org/osdu#hasVerticalMeasurementType
osdu:hasVerticalMeasurementType rdf:type owl:ObjectProperty ;
	rdfs:comment "Reference to the VerticalMeasurementType for the object " ;
	rdfs:domain [
		rdf:type owl:Class ;
		owl:unionOf (
			osdu:AbstractReferenceLevel
			osdu:AbstractFacilityVerticalMeasurement
			osdu:VelocityModeling
			osdu:SeismicTraceData
			osdu:FaultSystem
			osdu:SeismicHorizon
			osdu:SeismicFault
		) ;
	] ;
	rdfs:range osdu:VerticalMeasurementType ;
.

###  https://w3id.org/osdu#hasVerticalMeasurements
osdu:hasVerticalMeasurements rdf:type owl:ObjectProperty ;
	rdfs:domain osdu:Wellbore ;
	rdfs:range osdu:VerticalMeasurementID ;
.

###  https://w3id.org/osdu#hasWOBGroup
osdu:hasWOBGroup rdf:type owl:ObjectProperty ;
	rdfs:comment "Reference to the WOBGroup for the object " ;
	rdfs:domain osdu:OperationParameterPlan ;
	rdfs:range osdu:WOBGroup ;
.

###  https://w3id.org/osdu#hasWeather
osdu:hasWeather rdf:type owl:ObjectProperty ;
	rdfs:comment "Reference to the Weather for the object " ;
	rdfs:domain osdu:OperationsReport ;
	rdfs:range osdu:Weather ;
.

###  https://w3id.org/osdu#hasWell
osdu:hasWell rdf:type owl:ObjectProperty ;
	rdfs:comment "Reference to the Well for the object " ;
	rdfs:domain [
		rdf:type owl:Class ;
		owl:unionOf (
			osdu:WellPlanningWell
			osdu:Wellbore
			osdu:PPFGDataset
		) ;
	] ;
	rdfs:range osdu:Well ;
.

###  https://w3id.org/osdu#hasWellActivityPhaseType
osdu:hasWellActivityPhaseType rdf:type owl:ObjectProperty ;
	rdfs:comment "Reference to the WellActivityPhaseType for the object " ;
	rdfs:domain [
		rdf:type owl:Class ;
		owl:unionOf (
			osdu:Phase
			osdu:Cost
		) ;
	] ;
	rdfs:range osdu:WellActivityPhaseType ;
.

###  https://w3id.org/osdu#hasWellActivityProgram
osdu:hasWellActivityProgram rdf:type owl:ObjectProperty ;
	rdfs:comment "Reference to the WellActivityProgram for the object " ;
	rdfs:domain osdu:WellBarrierElementTest ;
	rdfs:range osdu:WellActivityProgram ;
.

###  https://w3id.org/osdu#hasWellActivityProgramType
osdu:hasWellActivityProgramType rdf:type owl:ObjectProperty ;
	rdfs:comment "Reference to the WellActivityProgramType for the object " ;
	rdfs:domain osdu:WellActivityProgram ;
	rdfs:range osdu:WellActivityProgramType ;
.

###  https://w3id.org/osdu#hasWellAlias
osdu:hasWellAlias rdf:type owl:ObjectProperty ;
	rdfs:comment "Reference to the WellAlias for the object " ;
	rdfs:domain osdu:OperationsReport ;
	rdfs:range osdu:WellAlias ;
.

###  https://w3id.org/osdu#hasWellBarrierElementTest
osdu:hasWellBarrierElementTest rdf:type owl:ObjectProperty ;
	rdfs:comment "Reference to the WellBarrierElementTest for the object " ;
	rdfs:domain osdu:Phase ;
	rdfs:range osdu:WellBarrierElementTest ;
.

###  https://w3id.org/osdu#hasWellBusinessIntention
osdu:hasWellBusinessIntention rdf:type owl:ObjectProperty ;
	rdfs:comment "Reference to the WellBusinessIntention for the object " ;
	rdfs:domain [
		rdf:type owl:Class ;
		owl:unionOf (
			osdu:Wellbore
			osdu:Well
			osdu:WellStatusSummary
		) ;
	] ;
	rdfs:range osdu:WellBusinessIntention ;
.

###  https://w3id.org/osdu#hasWellBusinessIntentionOutcome
osdu:hasWellBusinessIntentionOutcome rdf:type owl:ObjectProperty ;
	rdfs:comment "Reference to the WellBusinessIntentionOutcome for the object " ;
	rdfs:domain [
		rdf:type owl:Class ;
		owl:unionOf (
			osdu:Wellbore
			osdu:Well
		) ;
	] ;
	rdfs:range osdu:WellBusinessIntentionOutcome ;
.

###  https://w3id.org/osdu#hasWellCondition
osdu:hasWellCondition rdf:type owl:ObjectProperty ;
	rdfs:comment "Reference to the WellCondition for the object " ;
	rdfs:domain [
		rdf:type owl:Class ;
		owl:unionOf (
			osdu:Wellbore
			osdu:Well
			osdu:WellStatusSummary
		) ;
	] ;
	rdfs:range osdu:WellCondition ;
.

###  https://w3id.org/osdu#hasWellFluidDirection
osdu:hasWellFluidDirection rdf:type owl:ObjectProperty ;
	rdfs:comment "Reference to the WellFluidDirection for the object " ;
	rdfs:domain [
		rdf:type owl:Class ;
		owl:unionOf (
			osdu:Wellbore
			osdu:WellStatusSummary
		) ;
	] ;
	rdfs:range osdu:WellFluidDirection ;
.

###  https://w3id.org/osdu#hasWellInterestType
osdu:hasWellInterestType rdf:type owl:ObjectProperty ;
	rdfs:comment "Reference to the WellInterestType for the object " ;
	rdfs:domain [
		rdf:type owl:Class ;
		owl:unionOf (
			osdu:Wellbore
			osdu:HistoricalInterest
			osdu:Well
		) ;
	] ;
	rdfs:range osdu:WellInterestType ;
.

###  https://w3id.org/osdu#hasWellLog
osdu:hasWellLog rdf:type owl:ObjectProperty ;
	rdfs:comment "Reference to the WellLog for the object " ;
	rdfs:domain [
		rdf:type owl:Class ;
		owl:unionOf (
			osdu:PerforationJob
			osdu:Coring
			osdu:RockSampleAnalysis
		) ;
	] ;
	rdfs:range osdu:WellLog ;
.

###  https://w3id.org/osdu#hasWellLogSamplingDomainType
osdu:hasWellLogSamplingDomainType rdf:type owl:ObjectProperty ;
	rdfs:comment "Reference to the WellLogSamplingDomainType for the object " ;
	rdfs:domain osdu:WellLog ;
	rdfs:range osdu:WellLogSamplingDomainType ;
.

###  https://w3id.org/osdu#hasWellPlanningActivities
osdu:hasWellPlanningActivities rdf:type owl:ObjectProperty ;
	rdfs:comment "Reference to the WellPlanningActivities for the object " ;
	rdfs:domain osdu:ActivityPlan ;
	rdfs:range osdu:WellPlanningActivity ;
.

###  https://w3id.org/osdu#hasWellPlanningWell
osdu:hasWellPlanningWell rdf:type owl:ObjectProperty ;
	rdfs:comment "Reference to the WellPlanningWell for the object " ;
	rdfs:domain [
		rdf:type owl:Class ;
		owl:unionOf (
			osdu:WellPlanningWellbore
			osdu:PlannedLithology
		) ;
	] ;
	rdfs:range osdu:WellPlanningWell ;
.

###  https://w3id.org/osdu#hasWellPlanningWellbore
osdu:hasWellPlanningWellbore rdf:type owl:ObjectProperty ;
	rdfs:comment "Reference to the WellPlanningWellbore for the object " ;
	rdfs:domain [
		rdf:type owl:Class ;
		owl:unionOf (
			osdu:WellBarrierElementTest
			osdu:PlannedCementJob
			osdu:PlannedLithology
		) ;
	] ;
	rdfs:range osdu:WellPlanningWellbore ;
.

###  https://w3id.org/osdu#hasWellProductType
osdu:hasWellProductType rdf:type owl:ObjectProperty ;
	rdfs:comment "Reference to the WellProductType for the object " ;
	rdfs:domain [
		rdf:type owl:Class ;
		owl:unionOf (
			osdu:Wellbore
			osdu:WellStatusSummary
		) ;
	] ;
	rdfs:range osdu:WellProductType ;
.

###  https://w3id.org/osdu#hasWellRole
osdu:hasWellRole rdf:type owl:ObjectProperty ;
	rdfs:comment "Reference to the WellRole for the object " ;
	rdfs:domain [
		rdf:type owl:Class ;
		owl:unionOf (
			osdu:Wellbore
			osdu:Well
			osdu:WellStatusSummary
		) ;
	] ;
	rdfs:range osdu:WellRole ;
.

###  https://w3id.org/osdu#hasWellStatusSummary
osdu:hasWellStatusSummary rdf:type owl:ObjectProperty ;
	rdfs:comment "Reference to the WellStatusSummary for the object " ;
	rdfs:domain [
		rdf:type owl:Class ;
		owl:unionOf (
			osdu:Wellbore
			osdu:Well
		) ;
	] ;
	rdfs:range osdu:WellStatusSummary ;
.

###  https://w3id.org/osdu#hasWellbore
osdu:hasWellbore rdf:type owl:ObjectProperty ;
	rdfs:comment "Reference to the Wellbore for the object " ;
	rdfs:domain [
		rdf:type owl:Class ;
		owl:unionOf (
			osdu:AbstractFacilityVerticalMeasurement
			osdu:FluidsProgram
			osdu:WellPlanningWellbore
			osdu:FluidsReport
			osdu:RockSample
			osdu:Risk
			osdu:Phase
			osdu:EvaluationPlan
			osdu:SeismicSourceConfiguration
			osdu:SeismicReceiverConfiguration
			osdu:GeometricTargetSet
			osdu:SurveyProgram
			osdu:WellboreArchitecture
			osdu:CasingDesign
			osdu:OperationsReport
			osdu:BHARun
			osdu:PerforationJob
			osdu:ActivityPlan
			osdu:PerforationInterval
			osdu:Coring
			osdu:HoleSection
			osdu:TubularAssembly
			osdu:WellLog
			osdu:WellboreMarkerSet
			osdu:TubularUmbilical
			osdu:RockSampleAnalysis
			osdu:PPFGDataset
			osdu:WellboreTrajectory
			osdu:TubularComponent
			osdu:WellboreIntervalSet
		) ;
	] ;
	rdfs:range osdu:Wellbore ;
.

###  https://w3id.org/osdu#hasWellboreAlias
osdu:hasWellboreAlias rdf:type owl:ObjectProperty ;
	rdfs:comment "Reference to the WellboreAlias for the object " ;
	rdfs:domain osdu:OperationsReport ;
	rdfs:range osdu:ObjectAlias ;
.

###  https://w3id.org/osdu#hasWellboreArchitecture
osdu:hasWellboreArchitecture rdf:type owl:ObjectProperty ;
	rdfs:comment "Reference to the WellboreArchitecture for the object " ;
	rdfs:domain [
		rdf:type owl:Class ;
		owl:unionOf (
			osdu:Phase
			osdu:WellBarrierElementTest
			osdu:PlannedCementJob
		) ;
	] ;
	rdfs:range osdu:WellboreArchitecture ;
.

###  https://w3id.org/osdu#hasWellboreMarkerSet
osdu:hasWellboreMarkerSet rdf:type owl:ObjectProperty ;
	rdfs:comment "Reference to the WellboreMarkerSet for the object " ;
	rdfs:domain [
		rdf:type owl:Class ;
		owl:unionOf (
			osdu:WellPlanningWellbore
			osdu:Interval
		) ;
	] ;
	rdfs:range osdu:WellboreMarkerSet ;
.

###  https://w3id.org/osdu#hasWellboreTrajectory
osdu:hasWellboreTrajectory rdf:type owl:ObjectProperty ;
	rdfs:comment "Reference to the WellboreTrajectory for the object " ;
	rdfs:domain [
		rdf:type owl:Class ;
		owl:unionOf (
			osdu:AbstractReferenceLevel
			osdu:AbstractFacilityVerticalMeasurement
			osdu:Wellbore
			osdu:CasingDesign
			osdu:PPFGDataset
			osdu:GeologyInterval
		) ;
	] ;
	rdfs:range osdu:WellboreTrajectory ;
.

###  https://w3id.org/osdu#hasWellboreTrajectoryType
osdu:hasWellboreTrajectoryType rdf:type owl:ObjectProperty ;
	rdfs:comment "Reference to the WellboreTrajectoryType for the object " ;
	rdfs:domain osdu:Wellbore ;
	rdfs:range osdu:WellboreTrajectoryType ;
.

###  https://w3id.org/osdu#hasWgs84Coordinates
osdu:hasWgs84Coordinates rdf:type owl:ObjectProperty ;
	rdfs:comment "Reference to the Wgs84Coordinates for the object " ;
	rdfs:domain [
		rdf:type owl:Class ;
		owl:unionOf (
			osdu:AbstractSpatialLocation
			osdu:CoordinateTransformation
			osdu:CoordinateReferenceSystem
		) ;
	] ;
	rdfs:range osdu:AbstractFeatureCollection ;
.

###  https://w3id.org/osdu#hasWorkflows
osdu:hasWorkflows rdf:type owl:ObjectProperty ;
	rdfs:comment "Reference to the Workflows for the object " ;
	rdfs:domain osdu:ConnectedSourceDataJob ;
	rdfs:range osdu:Workflow ;
.

###  https://w3id.org/osdu#ijkGridPatches
osdu:ijkGridPatches rdf:type owl:ObjectProperty ;
	rdfs:comment "Reference to the IjkGridPatches for the object " ;
	rdfs:domain osdu:GpGridRepresentation ;
	rdfs:range osdu:AbstractIjkGridPatch ;
.

###  https://w3id.org/osdu#item
osdu:item rdf:type owl:ObjectProperty ;
	rdfs:comment "Reference to one of possibly multiple items for the object " ;
	rdfs:domain [
		rdf:type owl:Class ;
		owl:unionOf (
			osdu:AnyCrsGeoJSONLineStringCoordinatesArray
			osdu:AnyCrsGeoJSONPolygonCoordinatesArray
		) ;
	] ;
	 rdfs:range [
		rdf:type owl:Class ;
		owl:unionOf (
			xsd:decimal
			osdu:AnyCrsGeoJSONPolygonCoordinatesArrayItemsArray
		) ;
	] ;
.

###  https://w3id.org/osdu#jobContact
osdu:jobContact rdf:type owl:ObjectProperty ;
	rdfs:comment "Reference to the JobContact for the object " ;
	rdfs:domain osdu:OperationsReport ;
	rdfs:range osdu:AbstractContact ;
.

###  https://w3id.org/osdu#keyColumns
osdu:keyColumns rdf:type owl:ObjectProperty ;
	rdfs:comment "Reference to the KeyColumns for the object " ;
	rdfs:domain [
		rdf:type owl:Class ;
		owl:unionOf (
			osdu:AbstractColumnBasedTable
			osdu:ColumnBasedTable
			osdu:ColumnBasedTableType
		) ;
	] ;
	rdfs:range osdu:AbstractReferencePropertyType ;
.

###  https://w3id.org/osdu#meta
osdu:meta rdf:type owl:ObjectProperty ;
	rdfs:comment "Reference to the meta for the object " ;
	rdfs:domain osdu:System ;
	rdfs:range osdu:AbstractMetaItem ;
.

###  https://w3id.org/osdu#nameAlias
osdu:nameAlias rdf:type owl:ObjectProperty ;
	rdfs:comment "Reference to the NameAlias for the object " ;
	rdfs:domain osdu:AbstractReferenceType ;
	rdfs:range osdu:AbstractAliasNames ;
.

###  https://w3id.org/osdu#nameAliases
osdu:nameAliases rdf:type owl:ObjectProperty ;
	rdfs:comment "Reference to the NameAliases for the object " ;
	rdfs:domain osdu:AbstractMaster ;
	rdfs:range osdu:AbstractAliasNames ;
.

###  https://w3id.org/osdu#organisationNameAliases
osdu:organisationNameAliases rdf:type owl:ObjectProperty ;
	rdfs:comment "Reference to the OrganisationNameAliases for the object " ;
	rdfs:domain osdu:Organisation ;
	rdfs:range osdu:AbstractAliasNames ;
.

###  https://w3id.org/osdu#parameters
osdu:parameters rdf:type owl:ObjectProperty ;
	rdfs:comment "Reference to the Parameters for the object " ;
	rdfs:domain [
		rdf:type owl:Class ;
		owl:unionOf (
			osdu:AbstractProjectActivity
			osdu:AbstractWPCActivity
		) ;
	] ;
	rdfs:range osdu:AbstractActivityParameter ;
.

###  https://w3id.org/osdu#playNameAliases
osdu:playNameAliases rdf:type owl:ObjectProperty ;
	rdfs:comment "Reference to the PlayNameAliases for the object " ;
	rdfs:domain osdu:Play ;
	rdfs:range osdu:AbstractAliasNames ;
.

###  https://w3id.org/osdu#projectNames
osdu:projectNames rdf:type owl:ObjectProperty ;
	rdfs:comment "Reference to the ProjectNames for the object " ;
	rdfs:domain osdu:AbstractProject ;
	rdfs:range osdu:AbstractAliasNames ;
.

###  https://w3id.org/osdu#property
osdu:property rdf:type owl:ObjectProperty ;
	rdfs:domain [
		rdf:type owl:Class ;
		owl:unionOf (
			osdu:AnyCrsGeoJSONFeature
			osdu:GeoJSONFeature
		) ;
	] ;
	rdfs:range owl:Thing ;
.

###  https://w3id.org/osdu#prospectNameAliases
osdu:prospectNameAliases rdf:type owl:ObjectProperty ;
	rdfs:comment "Reference to the ProspectNameAliases for the object " ;
	rdfs:domain osdu:Prospect ;
	rdfs:range osdu:AbstractAliasNames ;
.

###  https://w3id.org/osdu#responsible
osdu:responsible rdf:type owl:ObjectProperty ;
	rdfs:comment "Reference to the Responsibles for the object " ;
	rdfs:domain osdu:RiskResponse ;
	rdfs:range osdu:AbstractContact ;
.

###  https://w3id.org/osdu#reviewers
osdu:reviewers rdf:type owl:ObjectProperty ;
	rdfs:comment "Reference to the Reviewers for the object " ;
	rdfs:domain osdu:AbstractTechnicalAssurance ;
	rdfs:range osdu:AbstractContact ;
.

###  https://w3id.org/osdu#riskResponsibles
osdu:riskResponsibles rdf:type owl:ObjectProperty ;
	rdfs:comment "Reference to the RiskResponsibles for the object " ;
	rdfs:domain osdu:Risk ;
	rdfs:range osdu:AbstractContact ;
.

###  https://w3id.org/osdu#sampleStorageLocations
osdu:sampleStorageLocations rdf:type owl:ObjectProperty ;
	rdfs:comment "Reference to the SampleStorageLocations for the object " ;
	rdfs:domain osdu:RockSample ;
	rdfs:range osdu:AbstractStorageLocation ;
.

###  https://w3id.org/osdu#stratigraphicUnitsIndex
osdu:stratigraphicUnitsIndex rdf:type owl:ObjectProperty ;
	rdfs:domain osdu:StratigraphicUnits ;
	rdfs:range osdu:StratigraphicUnitsStratigraphicUnitsIndicesArray ;
.

###  https://w3id.org/osdu#tags
osdu:tags rdf:type owl:ObjectProperty ;
	rdfs:comment "Reference to the tags for the object " ;
	rdfs:domain osdu:System ;
	rdfs:range owl:Thing ;
.

###  https://w3id.org/osdu#technicalAssurances
osdu:technicalAssurances rdf:type owl:ObjectProperty ;
	rdfs:comment "Reference to the TechnicalAssurances for the object " ;
	rdfs:domain osdu:AbstractWPCGroupType ;
	rdfs:range osdu:AbstractTechnicalAssurance ;
.

###  https://w3id.org/osdu#unstructuredColumnLayerGridPatches
osdu:unstructuredColumnLayerGridPatches rdf:type owl:ObjectProperty ;
	rdfs:comment "Reference to the UnstructuredColumnLayerGridPatches for the object " ;
	rdfs:domain osdu:GpGridRepresentation ;
	rdfs:range osdu:AbstractUnstructuredColumnLayerGridPatch ;
.

###  https://w3id.org/osdu#unstructuredGridPatches
osdu:unstructuredGridPatches rdf:type owl:ObjectProperty ;
	rdfs:comment "Reference to the UnstructuredGridPatches for the object " ;
	rdfs:domain osdu:GpGridRepresentation ;
	rdfs:range osdu:AbstractUnstructuredGridPatch ;
.


#################################################################
#    Data properties
#################################################################

###  https://w3id.org/osdu#afeNumber
osdu:afeNumber rdf:type owl:DatatypeProperty ;
	rdfs:comment "AFE number that this cost item applies to. " ;
	rdfs:domain osdu:Cost ;
	rdfs:range xsd:string ;
.

###  https://w3id.org/osdu#apiKeyKeyName
osdu:apiKeyKeyName rdf:type owl:DatatypeProperty ;
	rdfs:comment "Key for obtaining an API key from the secret repository " ;
	rdfs:domain osdu:SecurityScheme ;
	rdfs:range xsd:string ;
.

###  https://w3id.org/osdu#absentValueCharacters
osdu:absentValueCharacters rdf:type owl:DatatypeProperty ;
	rdfs:comment "The characters that represent absent curve values in this data set, for example  '-999', 'NULL', '0', etc. Typically for legacy data  " ;
	rdfs:domain osdu:PPFGDataset ;
	rdfs:range xsd:string ;
.

###  https://w3id.org/osdu#accessTokenKeyName
osdu:accessTokenKeyName rdf:type owl:DatatypeProperty ;
	rdfs:comment "Key for obtaining an access token from the secret repository " ;
	rdfs:domain osdu:SecurityScheme ;
	rdfs:range xsd:string ;
.

###  https://w3id.org/osdu#accidentDescription
osdu:accidentDescription rdf:type owl:DatatypeProperty ;
	rdfs:comment "Accident description. " ;
	rdfs:domain osdu:Incident ;
	rdfs:range xsd:string ;
.

###  https://w3id.org/osdu#accuracy
osdu:accuracy rdf:type owl:DatatypeProperty ;
	rdfs:comment "The accuracy of the transformation expressed in meters. " ;
	rdfs:domain osdu:CoordinateTransformation ;
	rdfs:range xsd:decimal ;
.

###  https://w3id.org/osdu#acquisitionCompanyID
osdu:acquisitionCompanyID rdf:type owl:DatatypeProperty ;
	rdfs:comment "The relationship to data acquisition company defining the LogCurveType. Log curve codes are ambiguous, the acquisition company association disambiguates them. " ;
	rdfs:domain osdu:LogCurveType ;
	xsd:pattern "^[\\\\w\\\\-\\\\.]+:reference-data\\\\-\\\\-StandardsOrganisation:[\\\\w\\\\-\\\\.\\\\:\\\\%]+:[0-9]*$" ;
	rdfs:range xsd:string ;
.

###  https://w3id.org/osdu#acquisitionDate
osdu:acquisitionDate rdf:type owl:DatatypeProperty ;
	rdfs:comment "The date that the survey data was acquired on the field. " ;
	rdfs:domain osdu:WellboreTrajectory ;
	rdfs:range time:DateTimeDescription ;
.

###  https://w3id.org/osdu#acquisitionRemark
osdu:acquisitionRemark rdf:type owl:DatatypeProperty ;
	rdfs:comment "Remarks related to acquisition context which is not the same as Description which is a summary of the work-product-component. " ;
	rdfs:domain osdu:WellboreTrajectory ;
	rdfs:range xsd:string ;
.

###  https://w3id.org/osdu#acquisitionSite
osdu:acquisitionSite rdf:type owl:DatatypeProperty ;
	rdfs:comment "Acquisition site for the data capture area which is not any of the Country, Field or Basin properties which are all captured within the Geocontext for a work product component. The site should be used as an additional identifier for items such as prominent landmarks, facilities, processing plant or structures that identify the area of interest. " ;
	rdfs:domain osdu:ProcessedInSAR ;
	rdfs:range xsd:string ;
.

###  https://w3id.org/osdu#acquisitionTypeID
osdu:acquisitionTypeID rdf:type owl:DatatypeProperty ;
	rdfs:comment "Acquisition approach used Conventional, Wide Azimuth, Multi Azimuth etc. " ;
	rdfs:domain osdu:SeismicAcquisitionSurvey ;
	xsd:pattern "^[\\\\w\\\\-\\\\.]+:reference-data\\\\-\\\\-SeismicAcquisitionType:[\\\\w\\\\-\\\\.\\\\:\\\\%]+:[0-9]*$" ;
	rdfs:range xsd:string ;
.

###  https://w3id.org/osdu#activeCellCount
osdu:activeCellCount rdf:type owl:DatatypeProperty ;
	rdfs:comment "Total count of active cells in the grid. It is an approximation since the real count of active cells can be modified with some properties. " ;
	rdfs:domain osdu:AbstractGridRepresentation ;
	rdfs:range xsd:integer ;
.

###  https://w3id.org/osdu#activeIndicator
osdu:activeIndicator rdf:type owl:DatatypeProperty ;
	rdfs:comment "A flag indicating if the object is currently active or valid within its lifecycle stage. " ;
	rdfs:domain [
		rdf:type owl:Class ;
		owl:unionOf (
			osdu:ConnectedSourceDataJob
			osdu:TubularAssembly
			osdu:WellboreTrajectory
		) ;
	] ;
	rdfs:range xsd:boolean ;
.

###  https://w3id.org/osdu#activityCodeCatalogVersion
osdu:activityCodeCatalogVersion rdf:type owl:DatatypeProperty ;
	rdfs:comment "The catalog version of this activity " ;
	rdfs:domain osdu:WellPlanningActivity ;
	rdfs:range xsd:string ;
.

###  https://w3id.org/osdu#activityCodeID
osdu:activityCodeID rdf:type owl:DatatypeProperty ;
	rdfs:comment "The activity code of the activity " ;
	rdfs:domain [
		rdf:type owl:Class ;
		owl:unionOf (
			osdu:DrillingActivity
			osdu:WellPlanningActivity
		) ;
	] ;
	xsd:pattern "^[\\\\w\\\\-\\\\.]+:reference-data\\\\-\\\\-ActivityCode:[\\\\w\\\\-\\\\.\\\\:\\\\%]+:[0-9]*$" ;
	rdfs:range xsd:string ;
.

###  https://w3id.org/osdu#activityDepthEnd
osdu:activityDepthEnd rdf:type owl:DatatypeProperty ;
	rdfs:comment "The end depth of the activity. Depth relative to Planned wellbore ZDP. Navigate via WellboreID to the side-car WellPlanningWellbore, which holds the depth reference in data.VerticalMeasurement. " ;
	rdfs:domain osdu:DepthRange ;
	rdfs:range xsd:decimal ;
.

###  https://w3id.org/osdu#activityDepthStart
osdu:activityDepthStart rdf:type owl:DatatypeProperty ;
	rdfs:comment "The start depth of the activity. Depth relative to Planned wellbore ZDP. Navigate via WellboreID to the side-car WellPlanningWellbore, which holds the depth reference in data.VerticalMeasurement. " ;
	rdfs:domain osdu:DepthRange ;
	rdfs:range xsd:decimal ;
.

###  https://w3id.org/osdu#activityID
osdu:activityID rdf:type owl:DatatypeProperty ;
	rdfs:comment "Identifier of the activity " ;
	rdfs:domain [
		rdf:type owl:Class ;
		owl:unionOf (
			osdu:DrillingActivity
			osdu:WellPlanningActivity
		) ;
	] ;
	rdfs:range xsd:string ;
.

###  https://w3id.org/osdu#activityLevel
osdu:activityLevel rdf:type owl:DatatypeProperty ;
	rdfs:comment "The activity level of this activity. Levels go from L1 to L6 " ;
	rdfs:domain osdu:WellPlanningActivity ;
	xsd:pattern "^[\\\\w\\\\-\\\\.]+:reference-data\\\\-\\\\-ActivityLevel:[\\\\w\\\\-\\\\.\\\\:\\\\%]+:[0-9]*$" ;
	rdfs:range xsd:string ;
.

###  https://w3id.org/osdu#activityLevelID
osdu:activityLevelID rdf:type owl:DatatypeProperty ;
	rdfs:comment "The relationship to the ActivityLevel record describing the ActivityCode's position in the hierarchy. " ;
	rdfs:domain osdu:ActivityCode ;
	xsd:pattern "^[\\\\w\\\\-\\\\.]+:reference-data\\\\-\\\\-ActivityLevel:[\\\\w\\\\-\\\\.\\\\:\\\\%]+:[0-9]*$" ;
	rdfs:range xsd:string ;
.

###  https://w3id.org/osdu#activityMDBase
osdu:activityMDBase rdf:type owl:DatatypeProperty ;
	rdfs:comment "Measured depth at the base of interval over which the activity was conducted. " ;
	rdfs:domain osdu:DrillingActivity ;
	rdfs:range xsd:decimal ;
.

###  https://w3id.org/osdu#activityMDTop
osdu:activityMDTop rdf:type owl:DatatypeProperty ;
	rdfs:comment "Measured depth at the top of interval over which the activity was conducted. " ;
	rdfs:domain osdu:DrillingActivity ;
	rdfs:range xsd:decimal ;
.

###  https://w3id.org/osdu#activityOutcomeDetailID
osdu:activityOutcomeDetailID rdf:type owl:DatatypeProperty ;
	rdfs:comment "More detail on the outcome of the activity. For Example Injury, Operation Failed, Kick, Circulation Loss, Mud Loss " ;
	rdfs:domain osdu:DrillingActivity ;
	xsd:pattern "^[\\\\w\\\\-\\\\.]+:reference-data\\\\-\\\\-ActivityOutcomeDetail:[\\\\w\\\\-\\\\.\\\\:\\\\%]+:[0-9]*$" ;
	rdfs:range xsd:string ;
.

###  https://w3id.org/osdu#activityOutcomeID
osdu:activityOutcomeID rdf:type owl:DatatypeProperty ;
	rdfs:comment "OK, Finish, interrupted, failed, etc. " ;
	rdfs:domain osdu:DrillingActivity ;
	xsd:pattern "^[\\\\w\\\\-\\\\.]+:reference-data\\\\-\\\\-ActivityOutcome:[\\\\w\\\\-\\\\.\\\\:\\\\%]+:[0-9]*$" ;
	rdfs:range xsd:string ;
.

###  https://w3id.org/osdu#activityPhaseID
osdu:activityPhaseID rdf:type owl:DatatypeProperty ;
	rdfs:comment "Activity code classification describing higher level steps in the Well Activity " ;
	rdfs:domain osdu:Cost ;
	xsd:pattern "^[\\\\w\\\\-\\\\.]+:reference-data\\\\-\\\\-WellActivityPhaseType:[\\\\w\\\\-\\\\.\\\\:\\\\%]+:[0-9]*$" ;
	rdfs:range xsd:string ;
.

###  https://w3id.org/osdu#activityStartDateTime
osdu:activityStartDateTime rdf:type owl:DatatypeProperty ;
	rdfs:comment "Date and time that activities started. " ;
	rdfs:domain osdu:BHARun ;
	rdfs:range time:DateTimeDescription ;
.

###  https://w3id.org/osdu#activityStopDateTime
osdu:activityStopDateTime rdf:type owl:DatatypeProperty ;
	rdfs:comment "Date and time that activities stopped. " ;
	rdfs:domain osdu:BHARun ;
	rdfs:range time:DateTimeDescription ;
.

###  https://w3id.org/osdu#activityTVDBase
osdu:activityTVDBase rdf:type owl:DatatypeProperty ;
	rdfs:comment "TVD at the base of interval over which the activity was conducted. " ;
	rdfs:domain osdu:DrillingActivity ;
	rdfs:range xsd:decimal ;
.

###  https://w3id.org/osdu#activityTVDTop
osdu:activityTVDTop rdf:type owl:DatatypeProperty ;
	rdfs:comment "TVD at the top of interval over which the activity was conducted. " ;
	rdfs:domain osdu:DrillingActivity ;
	rdfs:range xsd:decimal ;
.

###  https://w3id.org/osdu#activityTemplateID
osdu:activityTemplateID rdf:type owl:DatatypeProperty ;
	rdfs:comment "The relation to the ActivityTemplate carrying expected parameter definitions and default values. " ;
	rdfs:domain [
		rdf:type owl:Class ;
		owl:unionOf (
			osdu:AbstractProjectActivity
			osdu:AbstractWPCActivity
		) ;
	] ;
	xsd:pattern "^[\\\\w\\\\-\\\\.]+:master-data\\\\-\\\\-ActivityTemplate:[\\\\w\\\\-\\\\.\\\\:\\\\%]+:[0-9]*$" ;
	rdfs:range xsd:string ;
.

###  https://w3id.org/osdu#activityType
osdu:activityType rdf:type owl:DatatypeProperty ;
	rdfs:comment "General method or circumstance of logging - MWD, completion, ... " ;
	rdfs:domain osdu:WellLog ;
	rdfs:range xsd:string ;
.

###  https://w3id.org/osdu#activityTypeID
osdu:activityTypeID rdf:type owl:DatatypeProperty ;
	rdfs:comment "Used to describe if it belongs to a RunActivity or to a PullActivity " ;
	rdfs:domain osdu:TubularAssembly ;
	xsd:pattern "^[\\\\w\\\\-\\\\.]+:reference-data\\\\-\\\\-ActivityType:[\\\\w\\\\-\\\\.\\\\:\\\\%]+:[0-9]*$" ;
	rdfs:range xsd:string ;
.

###  https://w3id.org/osdu#activityTypeReasonDescription
osdu:activityTypeReasonDescription rdf:type owl:DatatypeProperty ;
	rdfs:comment "Used to describe the reason of Activity - such as cut/pull, pulling,… " ;
	rdfs:domain osdu:TubularAssembly ;
	rdfs:range xsd:string ;
.

###  https://w3id.org/osdu#additiveAmount
osdu:additiveAmount rdf:type owl:DatatypeProperty ;
	rdfs:comment "Additive Amount. " ;
	rdfs:domain osdu:CementAdditive ;
	rdfs:range xsd:decimal ;
.

###  https://w3id.org/osdu#additiveDensity
osdu:additiveDensity rdf:type owl:DatatypeProperty ;
	rdfs:comment "Additive density. " ;
	rdfs:domain osdu:CementAdditive ;
	rdfs:range xsd:decimal ;
.

###  https://w3id.org/osdu#additiveFormulation
osdu:additiveFormulation rdf:type owl:DatatypeProperty ;
	rdfs:comment "Wet or Dry. " ;
	rdfs:domain osdu:CementAdditive ;
	rdfs:range xsd:string ;
.

###  https://w3id.org/osdu#additiveName
osdu:additiveName rdf:type owl:DatatypeProperty ;
	rdfs:comment "Additive name. " ;
	rdfs:domain osdu:CementAdditive ;
	rdfs:range xsd:string ;
.

###  https://w3id.org/osdu#additiveTypeID
osdu:additiveTypeID rdf:type owl:DatatypeProperty ;
	rdfs:comment "Identifier of additive type or Function (Retarder, Viscosifier, Weighting agent). " ;
	rdfs:domain osdu:CementAdditive ;
	xsd:pattern "^[\\\\w\\\\-\\\\.]+:reference-data\\\\-\\\\-AdditiveType:[\\\\w\\\\-\\\\.\\\\:\\\\%]+:[0-9]*$" ;
	rdfs:range xsd:string ;
.

###  https://w3id.org/osdu#address
osdu:address rdf:type owl:DatatypeProperty ;
	rdfs:comment "A string holding the complete address. " ;
	rdfs:domain osdu:StorageFacility ;
	rdfs:range xsd:string ;
.

###  https://w3id.org/osdu#affectedPersonnel
osdu:affectedPersonnel rdf:type owl:DatatypeProperty ;
	rdfs:comment "Describes the entity that may be affected by the risk " ;
	rdfs:domain osdu:Risk ;
	xsd:pattern "^[\\\\w\\\\-\\\\.]+:master-data\\\\-\\\\-Organisation:[\\\\w\\\\-\\\\.\\\\:\\\\%]+:[0-9]*$" ;
	rdfs:range xsd:string ;
.

###  https://w3id.org/osdu#afterPillFluidLossRate
osdu:afterPillFluidLossRate rdf:type owl:DatatypeProperty ;
	rdfs:comment "Post pill fluid loss rate " ;
	rdfs:domain osdu:PerforationJob ;
	rdfs:range xsd:decimal ;
.

###  https://w3id.org/osdu#ageBegin
osdu:ageBegin rdf:type owl:DatatypeProperty ;
	rdfs:comment "The age in million years at the beginning of the geochronologic interval. " ;
	rdfs:domain osdu:ChronoStratigraphy ;
	rdfs:range xsd:decimal ;
.

###  https://w3id.org/osdu#ageEnd
osdu:ageEnd rdf:type owl:DatatypeProperty ;
	rdfs:comment "The age in million years at the end of the geochronologic interval. " ;
	rdfs:domain osdu:ChronoStratigraphy ;
	rdfs:range xsd:decimal ;
.

###  https://w3id.org/osdu#agency
osdu:agency rdf:type owl:DatatypeProperty ;
	rdfs:comment "Name of company that supplied the weather data. " ;
	rdfs:domain osdu:Weather ;
	rdfs:range xsd:string ;
.

###  https://w3id.org/osdu#agreementExternalID
osdu:agreementExternalID rdf:type owl:DatatypeProperty ;
	rdfs:comment "Unique identifier of agreement in Company contracts system of record. " ;
	rdfs:domain osdu:Agreement ;
	rdfs:range xsd:string ;
.

###  https://w3id.org/osdu#agreementExternalSystem
osdu:agreementExternalSystem rdf:type owl:DatatypeProperty ;
	rdfs:comment "Name of Company contracts system of record containing authorized version of agreement. " ;
	rdfs:domain osdu:Agreement ;
	rdfs:range xsd:string ;
.

###  https://w3id.org/osdu#agreementIDs
osdu:agreementIDs rdf:type owl:DatatypeProperty ;
	rdfs:comment "References to applicable agreements governing the use of the data source " ;
	rdfs:domain osdu:ConnectedSourceRegistryEntry ;
	xsd:pattern "^[\\\\w\\\\-\\\\.]+:master-data\\\\-\\\\-Agreement:[\\\\w\\\\-\\\\.\\\\:\\\\%]+:[0-9]*$" ;
	rdfs:range xsd:string ;
.

###  https://w3id.org/osdu#agreementIdentifier
osdu:agreementIdentifier rdf:type owl:DatatypeProperty ;
	rdfs:comment "Natural unique identifier of an agreement. " ;
	rdfs:domain osdu:Agreement ;
	rdfs:range xsd:string ;
.

###  https://w3id.org/osdu#agreementName
osdu:agreementName rdf:type owl:DatatypeProperty ;
	rdfs:comment "Familiar name of agreement.  May be a code name for highly restricted agreements. " ;
	rdfs:domain osdu:Agreement ;
	rdfs:range xsd:string ;
.

###  https://w3id.org/osdu#agreementParentID
osdu:agreementParentID rdf:type owl:DatatypeProperty ;
	rdfs:comment "Reference to master agreement or other parental agreement in a hierarchy of related agreements. " ;
	rdfs:domain osdu:Agreement ;
	xsd:pattern "^[\\\\w\\\\-\\\\.]+:master-data\\\\-\\\\-Agreement:[\\\\w\\\\-\\\\.\\\\:\\\\%]+:[0-9]*$" ;
	rdfs:range xsd:string ;
.

###  https://w3id.org/osdu#agreementTypeID
osdu:agreementTypeID rdf:type owl:DatatypeProperty ;
	rdfs:comment "General purpose of agreement, such as license, purchase, trade, NDA. " ;
	rdfs:domain osdu:Agreement ;
	xsd:pattern "^[\\\\w\\\\-\\\\.]+:reference-data\\\\-\\\\-AgreementType:[\\\\w\\\\-\\\\.\\\\:\\\\%]+:[0-9]*$" ;
	rdfs:range xsd:string ;
.

###  https://w3id.org/osdu#aliasName
osdu:aliasName rdf:type owl:DatatypeProperty ;
	rdfs:comment "Alternative Name value of defined name type for an object. " ;
	rdfs:domain osdu:AbstractAliasNames ;
	rdfs:range xsd:string ;
.

###  https://w3id.org/osdu#aliasNameTypeClassID
osdu:aliasNameTypeClassID rdf:type owl:DatatypeProperty ;
	rdfs:comment "This supports the type of AliasName (such as Standard Identifier, System Identifier, and so on). AliasNameTypeClass is intended to be used to categorize alias name types by their general purpose, with values like Standard Identifier, System Identifier, and Moniker. Combined with the AliasNameType, and DefinitionOrganisation one can define a complete context for a particular identifier or name. For example, a standard identifier of type Regulatory ID, from API, is the US standards regulatory ID; a standard identifier of type company ID, from BigOil, is BigOil's Standard ID; System Identifiers would be particular to systems of record, or other systems, and Monikers, things like display names, plot labels, etc. " ;
	rdfs:domain osdu:AliasNameType ;
	xsd:pattern "^[\\\\w\\\\-\\\\.]+:reference-data\\\\-\\\\-AliasNameTypeClass:[\\\\w\\\\-\\\\.\\\\:\\\\%]+:[0-9]*$" ;
	rdfs:range xsd:string ;
.

###  https://w3id.org/osdu#aliasNameTypeID
osdu:aliasNameTypeID rdf:type owl:DatatypeProperty ;
	rdfs:comment "A classification of alias names such as by role played or type of source, such as regulatory name, regulatory code, company code, international standard name, etc. " ;
	rdfs:domain osdu:AbstractAliasNames ;
	xsd:pattern "^[\\\\w\\\\-\\\\.]+:reference-data\\\\-\\\\-AliasNameType:[\\\\w\\\\-\\\\.\\\\:\\\\%]+:[0-9]*$" ;
	rdfs:range xsd:string ;
.

###  https://w3id.org/osdu#aliasNameUniqueValueIndicator
osdu:aliasNameUniqueValueIndicator rdf:type owl:DatatypeProperty ;
	rdfs:comment "Indicates whether the value for alias names of a given alias name type must be universally unique. 'Y' indicates that there is a requirement for unique values. 'N' indicates that there is no requirement for unique values. " ;
	rdfs:domain osdu:AliasNameType ;
	rdfs:range xsd:boolean ;
.

###  https://w3id.org/osdu#alkalinityP1
osdu:alkalinityP1 rdf:type owl:DatatypeProperty ;
	rdfs:comment "Mud alkalinity P1 from alternate alkalinity method (volume in ml of 0.02N acid  to reach the phenolphthalein endpoint). " ;
	rdfs:domain osdu:Fluid ;
	rdfs:range xsd:decimal ;
.

###  https://w3id.org/osdu#alkalinityP2
osdu:alkalinityP2 rdf:type owl:DatatypeProperty ;
	rdfs:comment "Mud alkalinity P2 from alternate alkalinity method (volume in ml of 0.02N acid to titrate, the reagent mixture to the phenolphthalein endpoint). " ;
	rdfs:domain osdu:Fluid ;
	rdfs:range xsd:decimal ;
.

###  https://w3id.org/osdu#allowedParameterKind
osdu:allowedParameterKind rdf:type owl:DatatypeProperty ;
	rdfs:comment "If no allowed kind is given, then all kind of data types are allowed. " ;
	rdfs:domain osdu:ParameterTemplate ;
	xsd:pattern "^[\\\\w\\\\-\\\\.]+:reference-data\\\\-\\\\-ParameterKind:[\\\\w\\\\-\\\\.\\\\:\\\\%]+:[0-9]*$" ;
	rdfs:range xsd:string ;
.

###  https://w3id.org/osdu#ambientTemperature
osdu:ambientTemperature rdf:type owl:DatatypeProperty ;
	rdfs:comment "Ambient temperate value " ;
	rdfs:domain osdu:TestFluid ;
	rdfs:range xsd:decimal ;
.

###  https://w3id.org/osdu#analysisDate
osdu:analysisDate rdf:type owl:DatatypeProperty ;
	rdfs:comment "The date the batch of rock sample analysis was performed. " ;
	rdfs:domain osdu:RockSampleAnalysis ;
	rdfs:range time:DateTimeDescription ;
.

###  https://w3id.org/osdu#analysisOrganisationID
osdu:analysisOrganisationID rdf:type owl:DatatypeProperty ;
	rdfs:comment "Identifies the Organisation that produces/produced this analysis. " ;
	rdfs:domain osdu:RockSampleAnalysis ;
	xsd:pattern "^[\\\\w\\\\-\\\\.]+:master-data\\\\-\\\\-Organisation:[\\\\w\\\\-\\\\.\\\\:\\\\%]+:[0-9]*$" ;
	rdfs:range xsd:string ;
.

###  https://w3id.org/osdu#angleArc
osdu:angleArc rdf:type owl:DatatypeProperty ;
	rdfs:comment "Direction of straight line section or radius of arc for continuous curve section. " ;
	rdfs:domain osdu:GeometrySection ;
	rdfs:range xsd:decimal ;
.

###  https://w3id.org/osdu#anisotropyType
osdu:anisotropyType rdf:type owl:DatatypeProperty ;
	rdfs:comment "Type of anisotropy used in the velocity model " ;
	rdfs:domain osdu:VelocityModeling ;
	xsd:pattern "^[\\\\w\\\\-\\\\.]+:reference-data\\\\-\\\\-AnisotropyType:[\\\\w\\\\-\\\\.\\\\:\\\\%]+:[0-9]*$" ;
	rdfs:range xsd:string ;
.

###  https://w3id.org/osdu#annotations
osdu:annotations rdf:type owl:DatatypeProperty ;
	rdfs:comment "Array of Annotations " ;
	rdfs:domain osdu:WorkProduct ;
	rdfs:range xsd:string ;
.

###  https://w3id.org/osdu#annularShapeRatio
osdu:annularShapeRatio rdf:type owl:DatatypeProperty ;
	rdfs:comment "Cleaning coefficient of drilling fluid " ;
	rdfs:domain osdu:Fluid ;
	rdfs:range xsd:decimal ;
.

###  https://w3id.org/osdu#annulusFluidDensity
osdu:annulusFluidDensity rdf:type owl:DatatypeProperty ;
	rdfs:comment "Annulus Fluid Density used to calculate hydrostatic pressure " ;
	rdfs:domain osdu:PerforationJob ;
	rdfs:range xsd:decimal ;
.

###  https://w3id.org/osdu#annulusFluidTopTVD
osdu:annulusFluidTopTVD rdf:type owl:DatatypeProperty ;
	rdfs:comment "TVD of annulus fluid top used to calculate Hydrostatic pressure prior to first gun run " ;
	rdfs:domain osdu:PerforationJob ;
	rdfs:range xsd:decimal ;
.

###  https://w3id.org/osdu#annulusFluidTypeID
osdu:annulusFluidTypeID rdf:type owl:DatatypeProperty ;
	rdfs:comment "Annulus Fluid Type " ;
	rdfs:domain osdu:PerforationJob ;
	xsd:pattern "^[\\\\w\\\\-\\\\.]+:reference-data\\\\-\\\\-AnnularFluidType:[\\\\w\\\\-\\\\.\\\\:\\\\%]+:[0-9]*$" ;
	rdfs:range xsd:string ;
.

###  https://w3id.org/osdu#anticipatedReservoirPressure
osdu:anticipatedReservoirPressure rdf:type owl:DatatypeProperty ;
	rdfs:comment "Hydrostatic pressure at Reservoir / perforated intervals top " ;
	rdfs:domain osdu:PerforationJob ;
	rdfs:range xsd:decimal ;
.

###  https://w3id.org/osdu#applicationID
osdu:applicationID rdf:type owl:DatatypeProperty ;
	rdfs:comment "Use or purpose of data acquisition. For example: Biomass estimation, Ship Detection, Vegetation monitoring, Geomorphology, CCS Storage monitoring, Oil & Gas field injection, Wellbore Casing Failure " ;
	rdfs:domain osdu:ProcessedInSAR ;
	xsd:pattern "^[\\\\w\\\\-\\\\.]+:reference-data\\\\-\\\\-InSARApplication:[\\\\w\\\\-\\\\.\\\\:\\\\%]+:[0-9]*$" ;
	rdfs:range xsd:string ;
.

###  https://w3id.org/osdu#appliedOperations
osdu:appliedOperations rdf:type owl:DatatypeProperty ;
	rdfs:comment "The audit trail of operations applied to the coordinates from the original state to the current state. The list may contain operations applied prior to ingestion as well as the operations applied to produce the Wgs84Coordinates. The text elements refer to ESRI style CRS and Transformation names, which may have to be translated to EPSG standard names. " ;
	rdfs:domain [
		rdf:type owl:Class ;
		owl:unionOf (
			osdu:AbstractSpatialLocation
			osdu:WellboreTrajectory
		) ;
	] ;
	rdfs:range xsd:string ;
.

###  https://w3id.org/osdu#areCuttingsWashedAndDried
osdu:areCuttingsWashedAndDried rdf:type owl:DatatypeProperty ;
	rdfs:comment "For cuttings: a flag indication whether the cuttings were washed and dried. More details in the associated RockSampleAnalysis. " ;
	rdfs:domain osdu:RockSample ;
	rdfs:range xsd:boolean ;
.

###  https://w3id.org/osdu#area
osdu:area rdf:type owl:DatatypeProperty ;
	rdfs:comment "Area of the aquifer. " ;
	rdfs:domain osdu:SingleCellAquifer ;
	rdfs:range xsd:decimal ;
.

###  https://w3id.org/osdu#areaCalculated
osdu:areaCalculated rdf:type owl:DatatypeProperty ;
	rdfs:comment "The calculated are covered by the survey. This value is calculated during the loading of the survey. " ;
	rdfs:domain osdu:SeismicAcquisitionSurvey ;
	rdfs:range xsd:decimal ;
.

###  https://w3id.org/osdu#areaNominal
osdu:areaNominal rdf:type owl:DatatypeProperty ;
	rdfs:comment "The nominal area covered by the survey. This value is usually entered by the end user. " ;
	rdfs:domain osdu:SeismicAcquisitionSurvey ;
	rdfs:range xsd:decimal ;
.

###  https://w3id.org/osdu#artificialLiftTypeID
osdu:artificialLiftTypeID rdf:type owl:DatatypeProperty ;
	rdfs:comment "Type of Artificial Lift used (could be Surface Pump / Submersible Pump / Gas Lift….) " ;
	rdfs:domain osdu:TubularAssembly ;
	xsd:pattern "^[\\\\w\\\\-\\\\.]+:reference-data\\\\-\\\\-ArtificialLiftType:[\\\\w\\\\-\\\\.\\\\:\\\\%]+:[0-9]*$" ;
	rdfs:range xsd:string ;
.

###  https://w3id.org/osdu#asg
osdu:asg rdf:type owl:DatatypeProperty ;
	rdfs:comment "Average specific gravity of solids. " ;
	rdfs:domain osdu:Fluid ;
	rdfs:range xsd:decimal ;
.

###  https://w3id.org/osdu#assemblyBaseMD
osdu:assemblyBaseMD rdf:type owl:DatatypeProperty ;
	rdfs:comment "The measured depth of the base from the whole assembly " ;
	rdfs:domain osdu:TubularAssembly ;
	rdfs:range xsd:decimal ;
.

###  https://w3id.org/osdu#assemblyBaseReportedTVD
osdu:assemblyBaseReportedTVD rdf:type owl:DatatypeProperty ;
	rdfs:comment "Depth of the base of the Assembly measured from the Well-Head " ;
	rdfs:domain osdu:TubularAssembly ;
	rdfs:range xsd:decimal ;
.

###  https://w3id.org/osdu#assemblyTopMD
osdu:assemblyTopMD rdf:type owl:DatatypeProperty ;
	rdfs:comment "The measured depth of the top from the whole assembly " ;
	rdfs:domain osdu:TubularAssembly ;
	rdfs:range xsd:decimal ;
.

###  https://w3id.org/osdu#assemblyTopReportedTVD
osdu:assemblyTopReportedTVD rdf:type owl:DatatypeProperty ;
	rdfs:comment "Depth of the top of the Assembly measured from the Well-Head " ;
	rdfs:domain osdu:TubularAssembly ;
	rdfs:range xsd:decimal ;
.

###  https://w3id.org/osdu#associatedObjectID
osdu:associatedObjectID rdf:type owl:DatatypeProperty ;
	rdfs:comment "The ID of the object (master-data, reference-data, work-product-component or work-product), to which this generic image has been associated. " ;
	rdfs:domain [
		rdf:type owl:Class ;
		owl:unionOf (
			osdu:GeoReferencedImage
			osdu:GenericImage
		) ;
	] ;
	xsd:pattern "^[\\\\w\\\\-\\\\.]+:(master-data\\\\-\\\\-[\\\\w\\\\-\\\\.]+|reference-data\\\\-\\\\-[\\\\w\\\\-\\\\.]+|work-product-component\\\\-\\\\-[\\\\w\\\\-\\\\.]+|work-product\\\\-\\\\-[\\\\w\\\\-\\\\.]+):[\\\\w\\\\-\\\\.\\\\:\\\\%]+:[0-9]*$" ;
	rdfs:range xsd:string ;
.

###  https://w3id.org/osdu#attachmentID
osdu:attachmentID rdf:type owl:DatatypeProperty ;
	rdfs:comment "Attachments associated with the activity " ;
	rdfs:domain osdu:DrillingActivity ;
	xsd:pattern "^[\\\\w\\\\-\\\\.]+:work-product-component\\\\-\\\\-Document:[\\\\w\\\\-\\\\.\\\\:\\\\%]+:[0-9]*$" ;
	rdfs:range xsd:string ;
.

###  https://w3id.org/osdu#attributionAuthority
osdu:attributionAuthority rdf:type owl:DatatypeProperty ;
	rdfs:comment "Name of the authority, or organisation, which governs the entity value and from which it is sourced. " ;
	rdfs:domain osdu:AbstractReferenceType ;
	rdfs:range xsd:string ;
.

###  https://w3id.org/osdu#attributionPublication
osdu:attributionPublication rdf:type owl:DatatypeProperty ;
	rdfs:comment "Name, URL, or other identifier of the publication, or repository, of the attribution source organisation from which the entity value is sourced. " ;
	rdfs:domain osdu:AbstractReferenceType ;
	rdfs:range xsd:string ;
.

###  https://w3id.org/osdu#attributionRevision
osdu:attributionRevision rdf:type owl:DatatypeProperty ;
	rdfs:comment "The distinct instance of the attribution publication, by version number, sequence number, date of publication, etc., that was used for the entity value. " ;
	rdfs:domain osdu:AbstractReferenceType ;
	rdfs:range xsd:string ;
.

###  https://w3id.org/osdu#audience
osdu:audience rdf:type owl:DatatypeProperty ;
	rdfs:comment "Audience used in OAuth2 flows " ;
	rdfs:domain osdu:SecurityScheme ;
	rdfs:range xsd:string ;
.

###  https://w3id.org/osdu#author
osdu:author rdf:type owl:DatatypeProperty ;
	rdfs:comment "The author responsible to the collection content. " ;
	rdfs:domain osdu:PersistedCollection ;
	rdfs:range xsd:string ;
.

###  https://w3id.org/osdu#authorID
osdu:authorID rdf:type owl:DatatypeProperty ;
	rdfs:comment "Array of Authors' IDs of the object.  Could be a person or company entity. " ;
	rdfs:domain [
		rdf:type owl:Class ;
		owl:unionOf (
			osdu:AbstractWorkProductComponent
			osdu:DataCollection
			osdu:WorkProduct
		) ;
	] ;
	rdfs:range xsd:string ;
.

###  https://w3id.org/osdu#authority
osdu:authority rdf:type owl:DatatypeProperty ;
	rdfs:comment "The authority governing the 'Code'. " ;
	rdfs:domain [
		rdf:type owl:Class ;
		owl:unionOf (
			osdu:ObjectAlias
			osdu:WellAlias
			osdu:AuthorityCode
		) ;
	] ;
	rdfs:range xsd:string ;
.

###  https://w3id.org/osdu#authorizationID
osdu:authorizationID rdf:type owl:DatatypeProperty ;
	rdfs:comment "Internal Company control number which identifies the allocation of funds to the Project. " ;
	rdfs:domain osdu:FundsAuthorizations ;
	rdfs:range xsd:string ;
.

###  https://w3id.org/osdu#authorizationUrl
osdu:authorizationUrl rdf:type owl:DatatypeProperty ;
	rdfs:comment "Authorization endpoint of the identity provider used in OAuth2 flows " ;
	rdfs:domain osdu:SecurityScheme ;
	rdfs:range xsd:string ;
.

###  https://w3id.org/osdu#averageBitFlowrate
osdu:averageBitFlowrate rdf:type owl:DatatypeProperty ;
	rdfs:comment "The average flowrate at the bit during the run " ;
	rdfs:domain osdu:DrillingParameters ;
	rdfs:range xsd:decimal ;
.

###  https://w3id.org/osdu#averageCuttingSize
osdu:averageCuttingSize rdf:type owl:DatatypeProperty ;
	rdfs:comment "Average size of the drill cuttings. " ;
	rdfs:domain osdu:Fluid ;
	rdfs:range xsd:decimal ;
.

###  https://w3id.org/osdu#averageFlowratePump
osdu:averageFlowratePump rdf:type owl:DatatypeProperty ;
	rdfs:comment "Average mud pump flow rate. " ;
	rdfs:domain osdu:DrillingParameters ;
	rdfs:range xsd:decimal ;
.

###  https://w3id.org/osdu#averageNodeSpacings
osdu:averageNodeSpacings rdf:type owl:DatatypeProperty ;
	rdfs:comment "The average distance between grid nodes or mesh vertices in each direction (i,j,k).  Note that vertical case is equivalent to sample interval. " ;
	rdfs:domain osdu:VelocityModeling ;
	rdfs:range xsd:decimal ;
.

###  https://w3id.org/osdu#averagePumpPressure
osdu:averagePumpPressure rdf:type owl:DatatypeProperty ;
	rdfs:comment "The average pump pressure used during the run " ;
	rdfs:domain osdu:DrillingParameters ;
	rdfs:range xsd:decimal ;
.

###  https://w3id.org/osdu#averageROP
osdu:averageROP rdf:type owl:DatatypeProperty ;
	rdfs:comment "Average rate of penetration through Interval. " ;
	rdfs:domain osdu:DrillingParameters ;
	rdfs:range xsd:decimal ;
.

###  https://w3id.org/osdu#averageRpm
osdu:averageRpm rdf:type owl:DatatypeProperty ;
	rdfs:comment "Average surface turn rate (commonly in rpm) through Interval. " ;
	rdfs:domain osdu:DrillingParameters ;
	rdfs:range xsd:decimal ;
.

###  https://w3id.org/osdu#averageRpmDownhole
osdu:averageRpmDownhole rdf:type owl:DatatypeProperty ;
	rdfs:comment "Average turn rate (commonly in rpm) downhole. " ;
	rdfs:domain osdu:DrillingParameters ;
	rdfs:range xsd:decimal ;
.

###  https://w3id.org/osdu#averageTorqueDownhole
osdu:averageTorqueDownhole rdf:type owl:DatatypeProperty ;
	rdfs:comment "Average torque: downhole. " ;
	rdfs:domain osdu:DrillingParameters ;
	rdfs:range xsd:decimal ;
.

###  https://w3id.org/osdu#averageTorqueOffBottom
osdu:averageTorqueOffBottom rdf:type owl:DatatypeProperty ;
	rdfs:comment "Average torque: off bottom. " ;
	rdfs:domain osdu:DrillingParameters ;
	rdfs:range xsd:decimal ;
.

###  https://w3id.org/osdu#averageTorqueOnBottom
osdu:averageTorqueOnBottom rdf:type owl:DatatypeProperty ;
	rdfs:comment "Average Torque: on bottom. " ;
	rdfs:domain osdu:DrillingParameters ;
	rdfs:range xsd:decimal ;
.

###  https://w3id.org/osdu#averageVelocityBitNozzle
osdu:averageVelocityBitNozzle rdf:type owl:DatatypeProperty ;
	rdfs:comment "Bit nozzle average velocity. " ;
	rdfs:domain osdu:DrillingParameters ;
	rdfs:range xsd:decimal ;
.

###  https://w3id.org/osdu#averageWOB
osdu:averageWOB rdf:type owl:DatatypeProperty ;
	rdfs:comment "Surface weight on bit - average through interval. " ;
	rdfs:domain osdu:DrillingParameters ;
	rdfs:range xsd:decimal ;
.

###  https://w3id.org/osdu#averageWOBDownhole
osdu:averageWOBDownhole rdf:type owl:DatatypeProperty ;
	rdfs:comment "Weight on bit - average downhole. " ;
	rdfs:domain osdu:DrillingParameters ;
	rdfs:range xsd:decimal ;
.

###  https://w3id.org/osdu#azimuthBottom
osdu:azimuthBottom rdf:type owl:DatatypeProperty ;
	rdfs:comment "Azimuth at stop measured depth. " ;
	rdfs:domain osdu:DrillingParameters ;
	rdfs:range xsd:decimal ;
.

###  https://w3id.org/osdu#azimuthReferenceType
osdu:azimuthReferenceType rdf:type owl:DatatypeProperty ;
	rdfs:comment "The North reference of the trajectory used to define the azimuth angular measurement values. For example, True North, Grid North, Magnetic North. " ;
	rdfs:domain osdu:WellboreTrajectory ;
	xsd:pattern "^[\\\\w\\\\-\\\\.]+:reference-data\\\\-\\\\-AzimuthReferenceType:[\\\\w\\\\-\\\\.\\\\:\\\\%]+:[0-9]*$" ;
	rdfs:range xsd:string ;
.

###  https://w3id.org/osdu#azimuthTop
osdu:azimuthTop rdf:type owl:DatatypeProperty ;
	rdfs:comment "Azimuth at start measured depth. " ;
	rdfs:domain osdu:DrillingParameters ;
	rdfs:range xsd:decimal ;
.

###  https://w3id.org/osdu#bhaRunID
osdu:bhaRunID rdf:type owl:DatatypeProperty ;
	rdfs:comment "Reference to the different BHA runs " ;
	rdfs:domain osdu:Phase ;
	xsd:pattern "^[\\\\w\\\\-\\\\.]+:master-data\\\\-\\\\-BHARun:[\\\\w\\\\-\\\\.\\\\:\\\\%]+:[0-9]*$" ;
	rdfs:range xsd:string ;
.

###  https://w3id.org/osdu#bhPressureTypeID
osdu:bhPressureTypeID rdf:type owl:DatatypeProperty ;
	rdfs:comment "How was the bottom hole pressure determined?  Measured, estimated, etc. " ;
	rdfs:domain osdu:PerforationInterval ;
	xsd:pattern "^[\\\\w\\\\-\\\\.]+:reference-data\\\\-\\\\-BottomHolePressureType:[\\\\w\\\\-\\\\.\\\\:\\\\%]+:[0-9]*$" ;
	rdfs:range xsd:string ;
.

###  https://w3id.org/osdu#backPressure
osdu:backPressure rdf:type owl:DatatypeProperty ;
	rdfs:comment "Back pressure applied during pumping stage. " ;
	rdfs:domain osdu:CementPumpSchedule ;
	rdfs:range xsd:decimal ;
.

###  https://w3id.org/osdu#baritePc
osdu:baritePc rdf:type owl:DatatypeProperty ;
	rdfs:comment "Barite content percent. " ;
	rdfs:domain osdu:Fluid ;
	rdfs:range xsd:decimal ;
.

###  https://w3id.org/osdu#barometricPressure
osdu:barometricPressure rdf:type owl:DatatypeProperty ;
	rdfs:comment "Atmospheric pressure. " ;
	rdfs:domain osdu:Weather ;
	rdfs:range xsd:decimal ;
.

###  https://w3id.org/osdu#baseCRSID
osdu:baseCRSID rdf:type owl:DatatypeProperty ;
	rdfs:comment "The relationship to the BaseCRS. " ;
	rdfs:domain osdu:BaseCRS ;
	xsd:pattern "^[\\\\w\\\\-\\\\.]+:reference-data\\\\-\\\\-CoordinateReferenceSystem:[\\\\w\\\\-\\\\.\\\\:\\\\%]+:[0-9]*$" ;
	rdfs:range xsd:string ;
.

###  https://w3id.org/osdu#baseDepth
osdu:baseDepth rdf:type owl:DatatypeProperty ;
	rdfs:comment "The curve's maximum 'depth' i.e., the reference value at which the curve has its last non-absent value. The curve may contain further absent values in between TopDepth and BaseDepth. Note that the SamplingDomainType may not be a depth as the property name indicates. " ;
	rdfs:domain osdu:Curves ;
	rdfs:range xsd:decimal ;
.

###  https://w3id.org/osdu#baseDepthMeasuredDepth
osdu:baseDepthMeasuredDepth rdf:type owl:DatatypeProperty ;
	rdfs:comment "Measured depth within the wellbore of the LAST surveyed station with recorded data.  If a stored survey has been extrapolated to a deeper depth than the last surveyed station then that is the extrapolated measured depth and not the survey base depth. " ;
	rdfs:domain osdu:WellboreTrajectory ;
	rdfs:range xsd:decimal ;
.

###  https://w3id.org/osdu#baseFluidDensity
osdu:baseFluidDensity rdf:type owl:DatatypeProperty ;
	rdfs:comment "Density of base fluid. " ;
	rdfs:domain osdu:CementingFluid ;
	rdfs:range xsd:decimal ;
.

###  https://w3id.org/osdu#baseFluidType
osdu:baseFluidType rdf:type owl:DatatypeProperty ;
	rdfs:comment "Type of base fluid: Fresh water, Sea water, Brine, Brackish water. " ;
	rdfs:domain osdu:CementingFluid ;
	rdfs:range xsd:string ;
.

###  https://w3id.org/osdu#baseForConversion
osdu:baseForConversion rdf:type owl:DatatypeProperty ;
	rdfs:comment "The base unit for unit conversion. The symbol of the unit which is used for conversion for of all members of this class. The corresponding baseForConversion must be a member of this class. To convert from one member to another member, you logically convert from the source member to the base and then convert from the base to the target member. " ;
	rdfs:domain [
		rdf:type owl:Class ;
		owl:unionOf (
			osdu:UnitQuantity
			osdu:ExternalUnitQuantity
		) ;
	] ;
	rdfs:range xsd:string ;
.

###  https://w3id.org/osdu#basinDescription
osdu:basinDescription rdf:type owl:DatatypeProperty ;
	rdfs:comment "A textual description of the Basin. " ;
	rdfs:domain osdu:Basin ;
	rdfs:range xsd:string ;
.

###  https://w3id.org/osdu#basinID
osdu:basinID rdf:type owl:DatatypeProperty ;
	rdfs:comment "Native identifier from a Master Data Management System or other trusted source external to OSDU - stored here in order to allow for multi-system connection and synchronization. If used, the Source property should identify that source system. " ;
	rdfs:domain [
		rdf:type owl:Class ;
		owl:unionOf (
			osdu:AbstractGeoBasinContext
			osdu:Basin
		) ;
	] ;
	xsd:pattern "^[\\\\w\\\\-\\\\.]+:master-data\\\\-\\\\-Basin:[\\\\w\\\\-\\\\.\\\\:\\\\%]+:[0-9]*$" ;
	rdfs:range xsd:string ;
.

###  https://w3id.org/osdu#basinName
osdu:basinName rdf:type owl:DatatypeProperty ;
	rdfs:comment "Name of the Basin. " ;
	rdfs:domain osdu:Basin ;
	rdfs:range xsd:string ;
.

###  https://w3id.org/osdu#basinTypeID
osdu:basinTypeID rdf:type owl:DatatypeProperty ;
	rdfs:comment "High level classification of the geological characteristics of the Basin; for example, Foothills, Active Margin, Passive Margin, etc. " ;
	rdfs:domain osdu:Basin ;
	xsd:pattern "^[\\\\w\\\\-\\\\.]+:reference-data\\\\-\\\\-BasinType:[\\\\w\\\\-\\\\.\\\\:\\\\%]+:[0-9]*$" ;
	rdfs:range xsd:string ;
.

###  https://w3id.org/osdu#hasBBox
osdu:hasBBox rdf:type owl:DatatypeProperty ;
	rdfs:domain [
		rdf:type owl:Class ;
		owl:unionOf (
			osdu:AnyCrsGeoJSONPoint
			osdu:AnyCrsGeoJSONLineString
			osdu:AnyCrsGeoJSONPolygon
			osdu:AnyCrsGeoJSONMultiPoint
			osdu:AnyCrsGeoJSONMultiLineString
			osdu:AnyCrsGeoJSONMultiPolygon
			osdu:AnyCrsGeoJSONGeometryCollection
			osdu:AnyCrsGeoJSONFeature
			osdu:AbstractAnyCrsFeatureCollection
			osdu:GeoJSONPoint
			osdu:GeoJSONLineString
			osdu:GeoJSONPolygon
			osdu:GeoJSONMultiPoint
			osdu:GeoJSONMultiLineString
			osdu:GeoJSONMultiPolygon
			osdu:GeoJSONGeometryCollection
			osdu:GeoJSONFeature
			osdu:AbstractFeatureCollection
		) ;
	] ;
	rdfs:range osdu:BBox ;
.

###  https://w3id.org/osdu#beaufortScaleNumber
osdu:beaufortScaleNumber rdf:type owl:DatatypeProperty ;
	rdfs:comment "The Beaufort wind force scale is a system used to estimate and report wind speeds when no measuring apparatus is available. It was invented in the early 19th century by Admiral Sir Francis Beaufort of the British Navy as a way to interpret winds from conditions. Values range from 0 (calm) to 12 (hurricane force). " ;
	rdfs:domain osdu:Weather ;
	rdfs:range xsd:decimal ;
.

###  https://w3id.org/osdu#binGridCoveragePercent
osdu:binGridCoveragePercent rdf:type owl:DatatypeProperty ;
	rdfs:comment "Portion of bin grid covered by picked surface expressed in percent. " ;
	rdfs:domain osdu:SeismicHorizon ;
	rdfs:range xsd:decimal ;
.

###  https://w3id.org/osdu#binGridDefinitionMethodTypeID
osdu:binGridDefinitionMethodTypeID rdf:type owl:DatatypeProperty ;
	rdfs:comment "This identifies how the Bin Grid is defined:  4=ABCD four-points method was used to define the grid (P6 parameters are optional and can contain derived values; P6BinNodeIncrementOnIAxis and P6BinNodeIncrementOnJaxis can be used as part of four-point method).  Use a perspective transformation to map between map coordinates and bin coordinates. Note point order.  6=P6 definition method was used to define the bin grid (ABCD points are optional and can contain derived values; ABCDBinGridSpatialLocation must specify the projected CRS).  Use an affine transformation to map between map coordinates and bin coordinates. " ;
	rdfs:domain osdu:AbstractBinGrid ;
	xsd:pattern "^[\\\\w\\\\-\\\\.]+:reference-data\\\\-\\\\-BinGridDefinitionMethodType:[\\\\w\\\\-\\\\.\\\\:\\\\%]+:[0-9]*$" ;
	rdfs:range xsd:string ;
.

###  https://w3id.org/osdu#binGridID
osdu:binGridID rdf:type owl:DatatypeProperty ;
	rdfs:comment "For 3D projects, BinGridID relates to the primary bin grid geometry for the processing; for 3D merge projects, it relates to the final (re-)projection and re-binning geometry. " ;
	rdfs:domain [
		rdf:type owl:Class ;
		owl:unionOf (
			osdu:SeismicProcessingProject
			osdu:VelocityModeling
			osdu:SeismicTraceData
			osdu:FaultSystem
			osdu:SeismicHorizon
			osdu:SeismicFault
		) ;
	] ;
	xsd:pattern "^[\\\\w\\\\-\\\\.]+:work-product-component\\\\-\\\\-SeismicBinGrid:[\\\\w\\\\-\\\\.\\\\:\\\\%]+:[0-9]*$" ;
	rdfs:range xsd:string ;
.

###  https://w3id.org/osdu#binGridName
osdu:binGridName rdf:type owl:DatatypeProperty ;
	rdfs:comment "Name of bin grid (e.g., GEOCO_GREENCYN_PHV_2012).  Probably the name as it exists in a separate corporate store if OSDU is not main system. " ;
	rdfs:domain osdu:AbstractBinGrid ;
	rdfs:range xsd:string ;
.

###  https://w3id.org/osdu#binGridTypeID
osdu:binGridTypeID rdf:type owl:DatatypeProperty ;
	rdfs:comment "Type of bin grid (Acquisition, Processing, Velocity, MagGrav, Magnetics, Gravity, GeologicModel, Reprojected, etc.) " ;
	rdfs:domain osdu:AbstractBinGrid ;
	xsd:pattern "^[\\\\w\\\\-\\\\.]+:reference-data\\\\-\\\\-SeismicBinGridType:[\\\\w\\\\-\\\\.\\\\:\\\\%]+:[0-9]*$" ;
	rdfs:range xsd:string ;
.

###  https://w3id.org/osdu#bitClass
osdu:bitClass rdf:type owl:DatatypeProperty ;
	rdfs:comment "N = new, U = used. " ;
	rdfs:domain osdu:BitRecord ;
	rdfs:range xsd:string ;
.

###  https://w3id.org/osdu#bitMDBase
osdu:bitMDBase rdf:type owl:DatatypeProperty ;
	rdfs:comment "Measured depth of the bit at the ase of interval over which the activity was conducted. " ;
	rdfs:domain osdu:DrillingActivity ;
	rdfs:range xsd:decimal ;
.

###  https://w3id.org/osdu#bitMDTop
osdu:bitMDTop rdf:type owl:DatatypeProperty ;
	rdfs:comment "Measured depth of the bit at the top of interval over which the activity was conducted. " ;
	rdfs:domain osdu:DrillingActivity ;
	rdfs:range xsd:decimal ;
.

###  https://w3id.org/osdu#bitRunNumber
osdu:bitRunNumber rdf:type owl:DatatypeProperty ;
	rdfs:comment "Bit run number. " ;
	rdfs:domain osdu:BHARun ;
	rdfs:range xsd:string ;
.

###  https://w3id.org/osdu#bitRunTIme
osdu:bitRunTIme rdf:type owl:DatatypeProperty ;
	rdfs:comment "Operating time spent by bit for run.  BUSINESS RULE: When reporting an actual as opposed to design, this is required. " ;
	rdfs:domain osdu:DrillingParameters ;
	rdfs:range time:TemporalDuration ;
.

###  https://w3id.org/osdu#blockID
osdu:blockID rdf:type owl:DatatypeProperty ;
	rdfs:comment "Identifier of the Geopolitical Entity that describes the Block associated to the Licence " ;
	rdfs:domain osdu:WellPlanningWell ;
	xsd:pattern "^[\\\\w\\\\-\\\\.]+:master-data\\\\-\\\\-GeoPoliticalEntity:[\\\\w\\\\-\\\\.\\\\:\\\\%]+:[0-9]*$" ;
	rdfs:range xsd:string ;
.

###  https://w3id.org/osdu#booleanColumn
osdu:booleanColumn rdf:type owl:DatatypeProperty ;
	rdfs:comment "A column of only boolean values " ;
	rdfs:domain [
		rdf:type owl:Class ;
		owl:unionOf (
			osdu:ColumnValues
			osdu:Columnvalues
		) ;
	] ;
	rdfs:range xsd:boolean ;
.

###  https://w3id.org/osdu#bottomDepth
osdu:bottomDepth rdf:type owl:DatatypeProperty ;
	rdfs:comment "The depth of the base of the rock sample, core, or analysis result. For point measurements (slides, sidewall cores), the same value is assigned to TopDepth and BottomDepth. " ;
	rdfs:domain [
		rdf:type owl:Class ;
		owl:unionOf (
			osdu:RockSample
			osdu:Coring
			osdu:RockSampleAnalysis
		) ;
	] ;
	rdfs:range xsd:decimal ;
.

###  https://w3id.org/osdu#bottomHoleTemperature
osdu:bottomHoleTemperature rdf:type owl:DatatypeProperty ;
	rdfs:comment "Downhole temperature at mid-point of perforation intervals " ;
	rdfs:domain osdu:PerforationJob ;
	rdfs:range xsd:decimal ;
.

###  https://w3id.org/osdu#bottomMeasuredDepth
osdu:bottomMeasuredDepth rdf:type owl:DatatypeProperty ;
	rdfs:comment "Informational Bottom Measured Depth of the Well Log. Always populate SamplingStart and SamplingStop, which represents the real sampling of the WellLog, including  non-depth sampling. " ;
	rdfs:domain osdu:WellLog ;
	rdfs:range xsd:decimal ;
.

###  https://w3id.org/osdu#boundaryFeatureID
osdu:boundaryFeatureID rdf:type owl:DatatypeProperty ;
	rdfs:comment "When populated, the boundary feature has a wider scope and allows boundary feature correlations across models. " ;
	rdfs:domain osdu:LocalBoundaryFeature ;
	xsd:pattern "^[\\\\w\\\\-\\\\.]+:master-data\\\\-\\\\-BoundaryFeature:[\\\\w\\\\-\\\\.\\\\:\\\\%]+:[0-9]*$" ;
	rdfs:range xsd:string ;
.

###  https://w3id.org/osdu#boundaryIDs
osdu:boundaryIDs rdf:type owl:DatatypeProperty ;
	rdfs:comment "References to the surfaces which delimit the reservoir compartment. " ;
	rdfs:domain osdu:ReservoirCompartmentInterpretation ;
	xsd:pattern "^[\\\\w\\\\-\\\\.]+:(work-product-component\\\\-\\\\-HorizonInterpretation|work-product-component\\\\-\\\\-FaultInterpretation|work-product-component\\\\-\\\\-GeobodyBoundaryInterpretation):[\\\\w\\\\-\\\\.\\\\:\\\\%]+:[0-9]*$" ;
	rdfs:range xsd:string ;
.

###  https://w3id.org/osdu#boundaryRelationTypeID
osdu:boundaryRelationTypeID rdf:type owl:DatatypeProperty ;
	rdfs:comment "Describes the geobody boundary relation with surrounding stratigraphic units: unconformable, conformable " ;
	rdfs:domain osdu:GeobodyBoundaryInterpretation ;
	xsd:pattern "^[\\\\w\\\\-\\\\.]+:reference-data\\\\-\\\\-BoundaryRelationType:[\\\\w\\\\-\\\\.\\\\:\\\\%]+:[0-9]*$" ;
	rdfs:range xsd:string ;
.

###  https://w3id.org/osdu#boundingBoxEastBoundLongitude
osdu:boundingBoxEastBoundLongitude rdf:type owl:DatatypeProperty ;
	rdfs:comment "Eastern longitude limit of the bounding box in degrees based on WGS 84 " ;
	rdfs:domain osdu:Extent ;
	rdfs:range xsd:decimal ;
	rdfs:subPropertyOf gn:longitude ;
.

###  https://w3id.org/osdu#boundingBoxNorthBoundLatitude
osdu:boundingBoxNorthBoundLatitude rdf:type owl:DatatypeProperty ;
	rdfs:comment "Northern latitude limit of the bounding box in degrees based on WGS 84 " ;
	rdfs:domain osdu:Extent ;
	rdfs:range xsd:decimal ;
	rdfs:subPropertyOf gn:latitude ;
.

###  https://w3id.org/osdu#boundingBoxSouthBoundLatitude
osdu:boundingBoxSouthBoundLatitude rdf:type owl:DatatypeProperty ;
	rdfs:comment "Southern latitude limit of the bounding box in degrees based on WGS 84 " ;
	rdfs:domain osdu:Extent ;
	rdfs:range xsd:decimal ;
	rdfs:subPropertyOf gn:latitude ;
.

###  https://w3id.org/osdu#boundingBoxWestBoundLongitude
osdu:boundingBoxWestBoundLongitude rdf:type owl:DatatypeProperty ;
	rdfs:comment "Western longitude limit of the bounding box in degrees based on WGS 84 " ;
	rdfs:domain osdu:Extent ;
	rdfs:range xsd:decimal ;
	rdfs:subPropertyOf gn:longitude ;
.

###  https://w3id.org/osdu#brandName
osdu:brandName rdf:type owl:DatatypeProperty ;
	rdfs:comment "The name of the fluid as given by the supplier " ;
	rdfs:domain osdu:Fluid ;
	rdfs:range xsd:string ;
.

###  https://w3id.org/osdu#brineDensity
osdu:brineDensity rdf:type owl:DatatypeProperty ;
	rdfs:comment "Density of water phase of NAF. " ;
	rdfs:domain osdu:Fluid ;
	rdfs:range xsd:decimal ;
.

###  https://w3id.org/osdu#brinePc
osdu:brinePc rdf:type owl:DatatypeProperty ;
	rdfs:comment "Percent brine content. " ;
	rdfs:domain osdu:Fluid ;
	rdfs:range xsd:decimal ;
.

###  https://w3id.org/osdu#businessActivities
osdu:businessActivities rdf:type owl:DatatypeProperty ;
	rdfs:comment "Array of business processes/workflows that the work product or component has been through (ex. well planning, exploration). " ;
	rdfs:domain [
		rdf:type owl:Class ;
		owl:unionOf (
			osdu:AbstractWorkProductComponent
			osdu:WorkProduct
		) ;
	] ;
	rdfs:range xsd:string ;
.

###  https://w3id.org/osdu#businessIntentionID
osdu:businessIntentionID rdf:type owl:DatatypeProperty ;
	rdfs:comment "Business Intention [Well Business Intention] is the general purpose for which resources are approved for drilling a new well or subsequent wellbore(s). " ;
	rdfs:domain [
		rdf:type owl:Class ;
		owl:unionOf (
			osdu:Wellbore
			osdu:Well
			osdu:WellStatusSummary
		) ;
	] ;
	xsd:pattern "^[\\\\w\\\\-\\\\.]+:reference-data\\\\-\\\\-WellBusinessIntention:[\\\\w\\\\-\\\\.\\\\:\\\\%]+:[0-9]*$" ;
	rdfs:range xsd:string ;
.

###  https://w3id.org/osdu#cclTopShotDistance
osdu:cclTopShotDistance rdf:type owl:DatatypeProperty ;
	rdfs:comment "Distance from CCL to Interval Top " ;
	rdfs:domain osdu:PerforationInterval ;
	rdfs:range xsd:decimal ;
.

###  https://w3id.org/osdu#cableCount
osdu:cableCount rdf:type owl:DatatypeProperty ;
	rdfs:comment "Number of receiver arrays (lines). " ;
	rdfs:domain [
		rdf:type owl:Class ;
		owl:unionOf (
			osdu:SeismicAcquisitionSurvey
			osdu:SeismicReceiverConfiguration
		) ;
	] ;
	rdfs:range xsd:integer ;
.

###  https://w3id.org/osdu#cableDepth
osdu:cableDepth rdf:type owl:DatatypeProperty ;
	rdfs:comment "Marine seismic cable towing depth below sea surface  (Positive Down). " ;
	rdfs:domain osdu:SeismicReceiverConfiguration ;
	rdfs:range xsd:decimal ;
.

###  https://w3id.org/osdu#cableLength
osdu:cableLength rdf:type owl:DatatypeProperty ;
	rdfs:comment "Total length of receiver array. " ;
	rdfs:domain [
		rdf:type owl:Class ;
		owl:unionOf (
			osdu:SeismicAcquisitionSurvey
			osdu:SeismicReceiverConfiguration
		) ;
	] ;
	rdfs:range xsd:decimal ;
.

###  https://w3id.org/osdu#cableSpacing
osdu:cableSpacing rdf:type owl:DatatypeProperty ;
	rdfs:comment "Horizontal distance between receiver arrays. " ;
	rdfs:domain osdu:SeismicReceiverConfiguration ;
	rdfs:range xsd:decimal ;
.

###  https://w3id.org/osdu#cableSpacingDistance
osdu:cableSpacingDistance rdf:type owl:DatatypeProperty ;
	rdfs:comment "DEPRECATED: Use ReceiverConfigurations[].CableSpacing. Horizontal distance between receiver arrays. " ;
	rdfs:domain osdu:SeismicAcquisitionSurvey ;
	rdfs:range xsd:decimal ;
.

###  https://w3id.org/osdu#calcium
osdu:calcium rdf:type owl:DatatypeProperty ;
	rdfs:comment "Calcium content. " ;
	rdfs:domain osdu:Fluid ;
	rdfs:range xsd:decimal ;
.

###  https://w3id.org/osdu#calciumChloride
osdu:calciumChloride rdf:type owl:DatatypeProperty ;
	rdfs:comment "Calcium chloride content. " ;
	rdfs:domain osdu:Fluid ;
	rdfs:range xsd:decimal ;
.

###  https://w3id.org/osdu#calciumChloridePc
osdu:calciumChloridePc rdf:type owl:DatatypeProperty ;
	rdfs:comment "Calcium chloride percent. " ;
	rdfs:domain osdu:Fluid ;
	rdfs:range xsd:decimal ;
.

###  https://w3id.org/osdu#calculationMethodType
osdu:calculationMethodType rdf:type owl:DatatypeProperty ;
	rdfs:comment "Calculation Method Type used to compute the TVD, X OFFSET, Y OFFSET and DOG LEG SEVERITY values for this Directional Survey. For example, Radius of Curvature, Minimum Curvature, Balanced Tangential, etc. " ;
	rdfs:domain osdu:WellboreTrajectory ;
	xsd:pattern "^[\\\\w\\\\-\\\\.]+:reference-data\\\\-\\\\-CalculationMethodType:[\\\\w\\\\-\\\\.\\\\:\\\\%]+:[0-9]*$" ;
	rdfs:range xsd:string ;
.

###  https://w3id.org/osdu#callbackUrl
osdu:callbackUrl rdf:type owl:DatatypeProperty ;
	rdfs:comment "Url the identity provider will send the token to in OAuth2 authorization code flows " ;
	rdfs:domain osdu:SecurityScheme ;
	rdfs:range xsd:string ;
.

###  https://w3id.org/osdu#candidateReferenceCurveIDs
osdu:candidateReferenceCurveIDs rdf:type owl:DatatypeProperty ;
	rdfs:comment "Secondary index curves, which are alternative candidates to act as ReferenceCurveID. Generally not populated, except in the cases where multiple reference curves are present, e.g. measured depth and time. " ;
	rdfs:domain osdu:WellLog ;
	rdfs:range xsd:string ;
.

###  https://w3id.org/osdu#carbonate
osdu:carbonate rdf:type owl:DatatypeProperty ;
	rdfs:comment "Carbonate content. " ;
	rdfs:domain osdu:Fluid ;
	rdfs:range xsd:decimal ;
.

###  https://w3id.org/osdu#casingCollarLocatorMD
osdu:casingCollarLocatorMD rdf:type owl:DatatypeProperty ;
	rdfs:comment "Measured Depth of the Casing Collar Locator used to align perforating guns on depth " ;
	rdfs:domain osdu:PerforationInterval ;
	rdfs:range xsd:decimal ;
.

###  https://w3id.org/osdu#casingDiameterLast
osdu:casingDiameterLast rdf:type owl:DatatypeProperty ;
	rdfs:comment "Diameter of the last casing joint. " ;
	rdfs:domain osdu:DrillingReportStatusInfo ;
	rdfs:range xsd:decimal ;
.

###  https://w3id.org/osdu#casingMDLast
osdu:casingMDLast rdf:type owl:DatatypeProperty ;
	rdfs:comment "Measured depth of the last casing joint. " ;
	rdfs:domain osdu:DrillingReportStatusInfo ;
	rdfs:range xsd:decimal ;
.

###  https://w3id.org/osdu#casingTVDLast
osdu:casingTVDLast rdf:type owl:DatatypeProperty ;
	rdfs:comment "True vertical depth of last casing joint. " ;
	rdfs:domain osdu:DrillingReportStatusInfo ;
	rdfs:range xsd:decimal ;
.

###  https://w3id.org/osdu#cause
osdu:cause rdf:type owl:DatatypeProperty ;
	rdfs:comment "A textual description of the cause of this risk " ;
	rdfs:domain osdu:Risk ;
	rdfs:range xsd:string ;
.

###  https://w3id.org/osdu#causeDescription
osdu:causeDescription rdf:type owl:DatatypeProperty ;
	rdfs:comment "Cause description. " ;
	rdfs:domain osdu:Incident ;
	rdfs:range xsd:string ;
.

###  https://w3id.org/osdu#cellShapeID
osdu:cellShapeID rdf:type owl:DatatypeProperty ;
	rdfs:comment "Indicates the uniform shape of all cells in this grid : tetrahedral, pyramidal, prism, hexahedral, polyhedral " ;
	rdfs:domain osdu:AbstractUnstructuredGridPatch ;
	xsd:pattern "^[\\\\w\\\\-\\\\.]+:reference-data\\\\-\\\\-CellShapeType:[\\\\w\\\\-\\\\.\\\\:\\\\%]+:[0-9]*$" ;
	rdfs:range xsd:string ;
.

###  https://w3id.org/osdu#cellValueTypes
osdu:cellValueTypes rdf:type owl:DatatypeProperty ;
	rdfs:comment "The type of numerical value(s) stored in each grid cell, such as Float or Double. " ;
	rdfs:domain osdu:VelocityModeling ;
	rdfs:range xsd:string ;
.

###  https://w3id.org/osdu#cementBaseMeasuredDepth
osdu:cementBaseMeasuredDepth rdf:type owl:DatatypeProperty ;
	rdfs:comment "Measured depth of base of cement. Depth relative to Planned wellbore ZDP. Navigate via WellboreID to the side-car WellPlanningWellbore, which holds the depth reference in data.VerticalMeasurement. " ;
	rdfs:domain osdu:CementStage ;
	rdfs:range xsd:decimal ;
.

###  https://w3id.org/osdu#cementToolTubularComponentID
osdu:cementToolTubularComponentID rdf:type owl:DatatypeProperty ;
	rdfs:comment "The identifier of the TubularComponent used for Cementing the wellbore " ;
	rdfs:domain osdu:PlannedCementJob ;
	xsd:pattern "^[\\\\w\\\\-\\\\.]+:work-product-component\\\\-\\\\-TubularComponent:[\\\\w\\\\-\\\\.\\\\:\\\\%]+:[0-9]*$" ;
	rdfs:range xsd:string ;
.

###  https://w3id.org/osdu#cementVolume
osdu:cementVolume rdf:type owl:DatatypeProperty ;
	rdfs:comment "Volume of cement. " ;
	rdfs:domain osdu:CementingFluid ;
	rdfs:range xsd:decimal ;
.

###  https://w3id.org/osdu#centralizationMethodID
osdu:centralizationMethodID rdf:type owl:DatatypeProperty ;
	rdfs:comment "Centralization Method " ;
	rdfs:domain osdu:PerforationJob ;
	xsd:pattern "^[\\\\w\\\\-\\\\.]+:reference-data\\\\-\\\\-PerforationCentralizationMethodType:[\\\\w\\\\-\\\\.\\\\:\\\\%]+:[0-9]*$" ;
	rdfs:range xsd:string ;
.

###  https://w3id.org/osdu#chargeManufacturerID
osdu:chargeManufacturerID rdf:type owl:DatatypeProperty ;
	rdfs:comment "Charge Make/Manufacturer " ;
	rdfs:domain osdu:PerforationInterval ;
	xsd:pattern "^[\\\\w\\\\-\\\\.]+:master-data\\\\-\\\\-Organisation:[\\\\w\\\\-\\\\.\\\\:\\\\%]+:[0-9]*$" ;
	rdfs:range xsd:string ;
.

###  https://w3id.org/osdu#chargeShapeID
osdu:chargeShapeID rdf:type owl:DatatypeProperty ;
	rdfs:comment "Charge Shape " ;
	rdfs:domain osdu:PerforationInterval ;
	xsd:pattern "^[\\\\w\\\\-\\\\.]+:reference-data\\\\-\\\\-PerforationGunChargeShape:[\\\\w\\\\-\\\\.\\\\:\\\\%]+:[0-9]*$" ;
	rdfs:range xsd:string ;
.

###  https://w3id.org/osdu#chargeSize
osdu:chargeSize rdf:type owl:DatatypeProperty ;
	rdfs:comment "Charge Size " ;
	rdfs:domain osdu:PerforationInterval ;
	xsd:pattern "^[\\\\w\\\\-\\\\.]+:reference-data\\\\-\\\\-PerforationGunChargeSize:[\\\\w\\\\-\\\\.\\\\:\\\\%]+:[0-9]*$" ;
	rdfs:range xsd:string ;
.

###  https://w3id.org/osdu#chargeTypeID
osdu:chargeTypeID rdf:type owl:DatatypeProperty ;
	rdfs:comment "Charge Type " ;
	rdfs:domain osdu:PerforationInterval ;
	xsd:pattern "^[\\\\w\\\\-\\\\.]+:reference-data\\\\-\\\\-PerforationGunChargeType:[\\\\w\\\\-\\\\.\\\\:\\\\%]+:[0-9]*$" ;
	rdfs:range xsd:string ;
.

###  https://w3id.org/osdu#checksum
osdu:checksum rdf:type owl:DatatypeProperty ;
	rdfs:comment "Checksum of file bytes - a hexadecimal number with even number of bytes. " ;
	rdfs:domain [
		rdf:type owl:Class ;
		owl:unionOf (
			osdu:DatasetProperties
			osdu:AbstractFileSourceInfo
			osdu:AbstractFile
		) ;
	] ;
	xsd:pattern "^([0-9a-fA-F]{2})+$" ;
	rdfs:range xsd:string ;
.

###  https://w3id.org/osdu#checksumAlgorithm
osdu:checksumAlgorithm rdf:type owl:DatatypeProperty ;
	rdfs:comment "The name of the checksum algorithm e.g. MD5, SHA-256. " ;
	rdfs:domain osdu:AbstractFileSourceInfo ;
	rdfs:range xsd:string ;
.

###  https://w3id.org/osdu#childCodes
osdu:childCodes rdf:type owl:DatatypeProperty ;
	rdfs:comment "The narrower interval codes which are contained in or overlapping with this geochronologic interval. " ;
	rdfs:domain osdu:ChronoStratigraphy ;
	rdfs:range xsd:string ;
.

###  https://w3id.org/osdu#chloride
osdu:chloride rdf:type owl:DatatypeProperty ;
	rdfs:comment "Chloride content. " ;
	rdfs:domain osdu:Fluid ;
	rdfs:range xsd:decimal ;
.

###  https://w3id.org/osdu#chronoStratigraphySet
osdu:chronoStratigraphySet rdf:type owl:DatatypeProperty ;
	rdfs:comment "A set of references to ChronoStratigraphy reference data, which belong to the same StratigraphicColumnRankUnitType, e.g. namespace:reference-data--StratigraphicColumnRankUnitType:Chronostratigraphic.System: Only one of ChronoStratigraphySet or StratigraphicUnitInterpretationSet must be populated, never both. " ;
	rdfs:domain osdu:StratigraphicColumnRankInterpretation ;
	xsd:pattern "^[\\\\w\\\\-\\\\.]+:reference-data\\\\-\\\\-ChronoStratigraphy:[\\\\w\\\\-\\\\.\\\\:\\\\%]+:[0-9]*$" ;
	rdfs:range xsd:string ;
.

###  https://w3id.org/osdu#chronostratigraphicIDs
osdu:chronostratigraphicIDs rdf:type owl:DatatypeProperty ;
	rdfs:comment "Chronostratigraphic classification. " ;
	rdfs:domain osdu:GeologyInterval ;
	xsd:pattern "^[\\\\w\\\\-\\\\.]+:reference-data\\\\-\\\\-ChronoStratigraphy:[\\\\w\\\\-\\\\.\\\\:\\\\%]+:[0-9]*$" ;
	rdfs:range xsd:string ;
.

###  https://w3id.org/osdu#classRig
osdu:classRig rdf:type owl:DatatypeProperty ;
	rdfs:comment "Classification of the rig. " ;
	rdfs:domain osdu:Rig ;
	rdfs:range xsd:string ;
.

###  https://w3id.org/osdu#classSlurryDryBlend
osdu:classSlurryDryBlend rdf:type owl:DatatypeProperty ;
	rdfs:comment "Slurry class. " ;
	rdfs:domain osdu:CementingFluid ;
	rdfs:range xsd:string ;
.

###  https://w3id.org/osdu#classificationTableID
osdu:classificationTableID rdf:type owl:DatatypeProperty ;
	rdfs:comment "The srn of the Column Based Table associated to a categorical property. Can be based on a defined dictionary of rock types " ;
	rdfs:domain osdu:GenericProperty ;
	xsd:pattern "^[\\\\w\\\\-\\\\.]+:work-product-component\\\\-\\\\-ColumnBasedTable:[\\\\w\\\\-\\\\.\\\\:\\\\%]+:[0-9]*$" ;
	rdfs:range xsd:string ;
.

###  https://w3id.org/osdu#clientID
osdu:clientID rdf:type owl:DatatypeProperty ;
	rdfs:comment "Client ID " ;
	rdfs:domain osdu:SecurityScheme ;
	rdfs:range xsd:string ;
.

###  https://w3id.org/osdu#clientSecretKeyName
osdu:clientSecretKeyName rdf:type owl:DatatypeProperty ;
	rdfs:comment "Key for obtaining the client secret for use in OAuth2 flows from the secret repository " ;
	rdfs:domain osdu:SecurityScheme ;
	rdfs:range xsd:string ;
.

###  https://w3id.org/osdu#cloudCeiling
osdu:cloudCeiling rdf:type owl:DatatypeProperty ;
	rdfs:comment "Height of cloud cover. " ;
	rdfs:domain osdu:Weather ;
	rdfs:range xsd:decimal ;
.

###  https://w3id.org/osdu#cloudCover
osdu:cloudCover rdf:type owl:DatatypeProperty ;
	rdfs:comment "Description of cloud cover. " ;
	rdfs:domain osdu:Weather ;
	rdfs:range xsd:string ;
.

###  https://w3id.org/osdu#clusterRefNo
osdu:clusterRefNo rdf:type owl:DatatypeProperty ;
	rdfs:comment "Cluster reference number " ;
	rdfs:domain osdu:PerforationInterval ;
	rdfs:range xsd:decimal ;
.

###  https://w3id.org/osdu#code
osdu:code rdf:type owl:DatatypeProperty ;
	rdfs:comment "A descriptive code for the object" ;
	rdfs:domain [
		rdf:type owl:Class ;
		owl:unionOf (
			osdu:AbstractReferenceType
			osdu:AuthorityCode
		) ;
	] ;
	rdfs:range xsd:integer ;
.

###  https://w3id.org/osdu#codeAsNumber
osdu:codeAsNumber rdf:type owl:DatatypeProperty ;
	rdfs:comment "The code as number as opposed to the Code defined as a string. " ;
	rdfs:domain [
		rdf:type owl:Class ;
		owl:unionOf (
			osdu:CoordinateTransformation
			osdu:CoordinateReferenceSystem
		) ;
	] ;
	rdfs:range xsd:integer ;
.

###  https://w3id.org/osdu#codeSpace
osdu:codeSpace rdf:type owl:DatatypeProperty ;
	rdfs:comment "The namespace or authority name governing this object, e.g. EPSG for contents from the EPSG Geodetic Parameter Dataset. " ;
	rdfs:domain [
		rdf:type owl:Class ;
		owl:unionOf (
			osdu:CoordinateTransformation
			osdu:CoordinateReferenceSystem
		) ;
	] ;
	rdfs:range xsd:string ;
.

###  https://w3id.org/osdu#coefficientA
osdu:coefficientA rdf:type owl:DatatypeProperty ;
	rdfs:comment "The A parameter; formula: y = (A+B*x)/(C+D*x) " ;
	rdfs:domain [
		rdf:type owl:Class ;
		owl:unionOf (
			osdu:UnitOfMeasure
			osdu:ExternalUnitOfMeasure
		) ;
	] ;
	rdfs:range xsd:decimal ;
.

###  https://w3id.org/osdu#coefficientB
osdu:coefficientB rdf:type owl:DatatypeProperty ;
	rdfs:comment "The B parameter; formula: y = (A+B*x)/(C+D*x) " ;
	rdfs:domain [
		rdf:type owl:Class ;
		owl:unionOf (
			osdu:UnitOfMeasure
			osdu:ExternalUnitOfMeasure
		) ;
	] ;
	rdfs:range xsd:decimal ;
.

###  https://w3id.org/osdu#coefficientC
osdu:coefficientC rdf:type owl:DatatypeProperty ;
	rdfs:comment "The C parameter; formula: y = (A+B*x)/(C+D*x) " ;
	rdfs:domain [
		rdf:type owl:Class ;
		owl:unionOf (
			osdu:UnitOfMeasure
			osdu:ExternalUnitOfMeasure
		) ;
	] ;
	rdfs:range xsd:decimal ;
.

###  https://w3id.org/osdu#coefficientD
osdu:coefficientD rdf:type owl:DatatypeProperty ;
	rdfs:comment "The D parameter; formula: y = (A+B*x)/(C+D*x) " ;
	rdfs:domain [
		rdf:type owl:Class ;
		owl:unionOf (
			osdu:UnitOfMeasure
			osdu:ExternalUnitOfMeasure
		) ;
	] ;
	rdfs:range xsd:decimal ;
.

###  https://w3id.org/osdu#coilTubingMeasuredDepth
osdu:coilTubingMeasuredDepth rdf:type owl:DatatypeProperty ;
	rdfs:comment "Measured depth of CoilTubing (multi-stage cement job. Depth relative to Planned wellbore ZDP. Navigate via WellboreID to the side-car WellPlanningWellbore, which holds the depth reference in data.VerticalMeasurement. " ;
	rdfs:domain osdu:CementStage ;
	rdfs:range xsd:decimal ;
.

###  https://w3id.org/osdu#colour
osdu:colour rdf:type owl:DatatypeProperty ;
	rdfs:comment "Colour assigned to the geochronologic interval by the ICS (https://stratigraphy.org). The format is #RRGGBB where the colours are expressed as hex codes. " ;
	rdfs:domain osdu:ChronoStratigraphy ;
	rdfs:range xsd:string ;
.

###  https://w3id.org/osdu#columnBasedTableType
osdu:columnBasedTableType rdf:type owl:DatatypeProperty ;
	rdfs:comment "Quickly indicate the type of the column based table (KrPc, PVT, Facies, ...) and its standard columns definition. It is supposed to be used when you don't use KeyColumns neither Columns as attributes of this WPC. " ;
	rdfs:domain [
		rdf:type owl:Class ;
		owl:unionOf (
			osdu:AbstractColumnBasedTable
			osdu:ColumnBasedTable
		) ;
	] ;
	xsd:pattern "^[\\\\w\\\\-\\\\.]+:reference-data\\\\-\\\\-ColumnBasedTableType:[\\\\w\\\\-\\\\.\\\\:\\\\%]+:[0-9]*$" ;
	rdfs:range xsd:string ;
.

###  https://w3id.org/osdu#columnShapeID
osdu:columnShapeID rdf:type owl:DatatypeProperty ;
	rdfs:comment "Indicates the common shape of all columns in this grid : triangular, quadrilateral, polygonal " ;
	rdfs:domain osdu:AbstractUnstructuredColumnLayerGridPatch ;
	xsd:pattern "^[\\\\w\\\\-\\\\.]+:reference-data\\\\-\\\\-ColumnShapeType:[\\\\w\\\\-\\\\.\\\\:\\\\%]+:[0-9]*$" ;
	rdfs:range xsd:string ;
.

###  https://w3id.org/osdu#columnSize
osdu:columnSize rdf:type owl:DatatypeProperty ;
	rdfs:comment "The count of elements in each column " ;
	rdfs:domain [
		rdf:type owl:Class ;
		owl:unionOf (
			osdu:AbstractColumnBasedTable
			osdu:ColumnBasedTable
		) ;
	] ;
	rdfs:range xsd:integer ;
.

###  https://w3id.org/osdu#columnStratigraphicHorizonBaseID
osdu:columnStratigraphicHorizonBaseID rdf:type owl:DatatypeProperty ;
	rdfs:comment "Base Stratigraphic Horizon bounding the stratigraphic unit  in a context of a stratigraphic column (Denormalized information) and not in an context of a model which can have several interpretations. Expecting one single horizon. " ;
	rdfs:domain osdu:StratigraphicUnitInterpretation ;
	xsd:pattern "^[\\\\w\\\\-\\\\.]+:work-product-component\\\\-\\\\-HorizonInterpretation:[\\\\w\\\\-\\\\.\\\\:\\\\%]+:[0-9]*$" ;
	rdfs:range xsd:string ;
.

###  https://w3id.org/osdu#columnStratigraphicHorizonTopID
osdu:columnStratigraphicHorizonTopID rdf:type owl:DatatypeProperty ;
	rdfs:comment "Top Stratigraphic Horizon bounding the stratigraphic unit in a context of a reference stratigraphic column (Denormalized information) and not in an context of a model which can have several interpretations. Expecting one single horizon. " ;
	rdfs:domain osdu:StratigraphicUnitInterpretation ;
	xsd:pattern "^[\\\\w\\\\-\\\\.]+:work-product-component\\\\-\\\\-HorizonInterpretation:[\\\\w\\\\-\\\\.\\\\:\\\\%]+:[0-9]*$" ;
	rdfs:range xsd:string ;
.

###  https://w3id.org/osdu#comment
osdu:comment rdf:type owl:DatatypeProperty ;
	rdfs:comment "A comment or description associated with the object " ;
	owl:sameAs rdfs:comment ;
.

###  https://w3id.org/osdu#commentTime
osdu:commentTime rdf:type owl:DatatypeProperty ;
	rdfs:comment "The time that the comment was made " ;
	rdfs:domain osdu:TimedComment ;
	rdfs:range time:DateTimeDescription ;
.

###  https://w3id.org/osdu#comments
osdu:comments rdf:type owl:DatatypeProperty ;
	rdfs:comment "Comments and remarks. " ;
	owl:sameAs rdfs:comment ;
.

###  https://w3id.org/osdu#commitDate
osdu:commitDate rdf:type owl:DatatypeProperty ;
	rdfs:comment "For reference values published and governed by OSDU: The date and time the record was committed into the OSDU member GitLab reference-values repository. The sole purpose of this date is to optimise the OSDU milestone upgrades. It allows the upgrade code to figure out whether or not the record must be PUT into reference value storage. " ;
	rdfs:domain osdu:AbstractReferenceType ;
	rdfs:range time:DateTimeDescription ;
.

###  https://w3id.org/osdu#companyID
osdu:companyID rdf:type owl:DatatypeProperty ;
	rdfs:comment "ID of a Company" ;
	rdfs:domain [
		rdf:type owl:Class ;
		owl:unionOf (
			osdu:Fluid
			osdu:WellLog
			osdu:WellboreTrajectory
		) ;
	] ;
	xsd:pattern "^[\\\\w\\\\-\\\\.]+:master-data\\\\-\\\\-Organisation:[\\\\w\\\\-\\\\.\\\\:\\\\%]+:[0-9]*$" ;
	rdfs:range xsd:string ;
.

###  https://w3id.org/osdu#companyOrganisationID
osdu:companyOrganisationID rdf:type owl:DatatypeProperty ;
	rdfs:comment "Reference to the company which employs Personnel. " ;
	rdfs:domain osdu:Personnel ;
	xsd:pattern "^[\\\\w\\\\-\\\\.]+:master-data\\\\-\\\\-Organisation:[\\\\w\\\\-\\\\.\\\\:\\\\%]+:[0-9]*$" ;
	rdfs:range xsd:string ;
.

###  https://w3id.org/osdu#components
osdu:components rdf:type owl:DatatypeProperty ;
	rdfs:domain osdu:WorkProduct ;
	xsd:pattern "^[\\\\w\\\\-\\\\.]+:work-product-component\\\\-\\\\-[\\\\w\\\\-\\\\.]+:[\\\\w\\\\-\\\\.\\\\:\\\\%]+:[0-9]*$" ;
	rdfs:range xsd:string ;
.

###  https://w3id.org/osdu#componentsTested
osdu:componentsTested rdf:type owl:DatatypeProperty ;
	rdfs:comment "Text string for noting the components tested " ;
	rdfs:domain osdu:WBETestStep ;
	rdfs:range xsd:string ;
.

###  https://w3id.org/osdu#compressionLevel
osdu:compressionLevel rdf:type owl:DatatypeProperty ;
	rdfs:comment "Number indicating degree of fidelity present in bulk data resulting from compression.  Meaning of number depends on algorithm. " ;
	rdfs:domain osdu:AbstractCompressionInfo ;
	rdfs:range xsd:decimal ;
.

###  https://w3id.org/osdu#compressionMethodTypeID
osdu:compressionMethodTypeID rdf:type owl:DatatypeProperty ;
	rdfs:comment "Name of a compression algorithm applied to the data as stored. " ;
	rdfs:domain osdu:AbstractCompressionInfo ;
	xsd:pattern "^[\\\\w\\\\-\\\\.]+:reference-data\\\\-\\\\-CompressionMethodType:[\\\\w\\\\-\\\\.\\\\:\\\\%]+:[0-9]*$" ;
	rdfs:range xsd:string ;
.

###  https://w3id.org/osdu#concentration
osdu:concentration rdf:type owl:DatatypeProperty ;
	rdfs:comment "Concentration Amount: unit type depends of typeConc. " ;
	rdfs:domain osdu:CementAdditive ;
	rdfs:range xsd:decimal ;
.

###  https://w3id.org/osdu#concentrationUnitOfMeasure
osdu:concentrationUnitOfMeasure rdf:type owl:DatatypeProperty ;
	rdfs:comment "The unit of measure of the planned product concentration " ;
	rdfs:domain osdu:BarrelFormulation ;
	xsd:pattern "^[\\\\w\\\\-\\\\.]+:reference-data\\\\-\\\\-UnitOfMeasure:[\\\\w\\\\-\\\\.\\\\:\\\\%]+:[0-9]*$" ;
	rdfs:range xsd:string ;
.

###  https://w3id.org/osdu#concentrationValue
osdu:concentrationValue rdf:type owl:DatatypeProperty ;
	rdfs:comment "The actual value of the planned product concentration " ;
	rdfs:domain osdu:BarrelFormulation ;
	rdfs:range xsd:decimal ;
.

###  https://w3id.org/osdu#conditionHole
osdu:conditionHole rdf:type owl:DatatypeProperty ;
	rdfs:comment "Hole condition description. " ;
	rdfs:domain [
		rdf:type owl:Class ;
		owl:unionOf (
			osdu:DrillingReportStatusInfo
			osdu:OperationsReport
		) ;
	] ;
	rdfs:range xsd:string ;
.

###  https://w3id.org/osdu#conditionID
osdu:conditionID rdf:type owl:DatatypeProperty ;
	rdfs:comment "Condition [Well Condition] is the operational state of a component relative to the Role [Well Role]. " ;
	rdfs:domain [
		rdf:type owl:Class ;
		owl:unionOf (
			osdu:Wellbore
			osdu:Well
			osdu:WellStatusSummary
		) ;
	] ;
	xsd:pattern "^[\\\\w\\\\-\\\\.]+:reference-data\\\\-\\\\-WellCondition:[\\\\w\\\\-\\\\.\\\\:\\\\%]+:[0-9]*$" ;
	rdfs:range xsd:string ;
.

###  https://w3id.org/osdu#connectedSourceDataJobID
osdu:connectedSourceDataJobID rdf:type owl:DatatypeProperty ;
	rdfs:comment "The relationship to the scheduling, fetch and ingestion configuration. " ;
	rdfs:domain osdu:DatasetProperties ;
	xsd:pattern "^[\\\\w\\\\-\\\\.]+:master-data\\\\-\\\\-ConnectedSourceDataJob:[\\\\w\\\\-\\\\.\\\\:\\\\%]+:[0-9]*$" ;
	rdfs:range xsd:string ;
.

###  https://w3id.org/osdu#connectedSourceDataPartitionID
osdu:connectedSourceDataPartitionID rdf:type owl:DatatypeProperty ;
	rdfs:comment "ID of the external partition containing the desired data " ;
	rdfs:domain osdu:ConnectedSourceDataJob ;
	rdfs:range xsd:string ;
.

###  https://w3id.org/osdu#connectedSourceRegistryEntryID
osdu:connectedSourceRegistryEntryID rdf:type owl:DatatypeProperty ;
	rdfs:comment "The relationship to the OSDU -compliant external, connected data source. " ;
	rdfs:domain [
		rdf:type owl:Class ;
		owl:unionOf (
			osdu:DatasetProperties
			osdu:ConnectedSourceDataJob
		) ;
	] ;
	xsd:pattern "^[\\\\w\\\\-\\\\.]+:master-data\\\\-\\\\-ConnectedSourceRegistryEntry:[\\\\w\\\\-\\\\.\\\\:\\\\%]+:[0-9]*$" ;
	rdfs:range xsd:string ;
.

###  https://w3id.org/osdu#connectedTubularComponentID
osdu:connectedTubularComponentID rdf:type owl:DatatypeProperty ;
	rdfs:comment "Identifier of the Wellhead Outlet the Umbilical is connected to " ;
	rdfs:domain osdu:TubularUmbilical ;
	xsd:pattern "^[\\\\w\\\\-\\\\.]+:work-product-component\\\\-\\\\-TubularComponent:[\\\\w\\\\-\\\\.\\\\:\\\\%]+:[0-9]*$" ;
	rdfs:range xsd:string ;
.

###  https://w3id.org/osdu#connectionCount
osdu:connectionCount rdf:type owl:DatatypeProperty ;
	rdfs:comment "The count of connections between cells. " ;
	rdfs:domain osdu:GridConnectionSetRepresentation ;
	rdfs:range xsd:integer ;
.

###  https://w3id.org/osdu#consequence
osdu:consequence rdf:type owl:DatatypeProperty ;
	rdfs:comment "A textual description of the consequence of this risk occurring " ;
	rdfs:domain osdu:Risk ;
	rdfs:range xsd:string ;
.

###  https://w3id.org/osdu#consequenceCategoryID
osdu:consequenceCategoryID rdf:type owl:DatatypeProperty ;
	rdfs:comment "Reference to the name of the category of the loss - equivalent to the ConsequenceCategory as defined in Bow Tie. " ;
	rdfs:domain osdu:Risk ;
	xsd:pattern "^[\\\\w\\\\-\\\\.]+:reference-data\\\\-\\\\-RiskConsequenceCategory:[\\\\w\\\\-\\\\.\\\\:\\\\%]+:[0-9]*$" ;
	rdfs:range xsd:string ;
.

###  https://w3id.org/osdu#consequenceSubCategoryID
osdu:consequenceSubCategoryID rdf:type owl:DatatypeProperty ;
	rdfs:comment "References the consequence sub-category of the risk. Possible effects arising were a risk event to occur. " ;
	rdfs:domain osdu:Risk ;
	xsd:pattern "^[\\\\w\\\\-\\\\.]+:reference-data\\\\-\\\\-RiskConsequenceSubCategory:[\\\\w\\\\-\\\\.\\\\:\\\\%]+:[0-9]*$" ;
	rdfs:range xsd:string ;
.

###  https://w3id.org/osdu#constraint
osdu:constraint rdf:type owl:DatatypeProperty ;
	rdfs:comment "Textual description of additional constraint associated with the parameter. (note that it will be better to have a formal description of the constraint) " ;
	rdfs:domain osdu:ParameterTemplate ;
	rdfs:range xsd:string ;
.

###  https://w3id.org/osdu#consumingActivityTemplateID
osdu:consumingActivityTemplateID rdf:type owl:DatatypeProperty ;
	rdfs:comment "The relationship to the consuming ActivityTemplate. " ;
	rdfs:domain osdu:Arc ;
	xsd:pattern "^[\\\\w\\\\-\\\\.]+:master-data\\\\-\\\\-ActivityTemplate:[\\\\w\\\\-\\\\.\\\\:\\\\%]+:[0-9]*$" ;
	rdfs:range xsd:string ;
.

###  https://w3id.org/osdu#consumingParameterTitle
osdu:consumingParameterTitle rdf:type owl:DatatypeProperty ;
	rdfs:comment "The Title of the consuming ActivityTemplate Parameter array element. " ;
	rdfs:domain osdu:Arc ;
	rdfs:range xsd:string ;
.

###  https://w3id.org/osdu#contextTypeID
osdu:contextTypeID rdf:type owl:DatatypeProperty ;
	rdfs:comment "ID that reflects the context of the PPFG  data set, for example 'Pre-Drill' or 'Post-Drill' " ;
	rdfs:domain osdu:PPFGDataset ;
	xsd:pattern "^[\\\\w\\\\-\\\\.]+:reference-data\\\\-\\\\-PPFGContextType:[\\\\w\\\\-\\\\.\\\\:\\\\%]+:[0-9]*$" ;
	rdfs:range xsd:string ;
.

###  https://w3id.org/osdu#contractIDs
osdu:contractIDs rdf:type owl:DatatypeProperty ;
	rdfs:comment "References to applicable agreements in external contract database system of record. " ;
	rdfs:domain osdu:AbstractProject ;
	xsd:pattern "^[\\\\w\\\\-\\\\.]+:master-data\\\\-\\\\-Agreement:[\\\\w\\\\-\\\\.\\\\:\\\\%]+:[0-9]*$" ;
	rdfs:range xsd:string ;
.

###  https://w3id.org/osdu#contractorCrew
osdu:contractorCrew rdf:type owl:DatatypeProperty ;
	rdfs:comment "Name of the team, unit, crew, party, or other subdivision of the Contractor that provided services. " ;
	rdfs:domain osdu:Contractors ;
	rdfs:range xsd:string ;
.

###  https://w3id.org/osdu#contractorID
osdu:contractorID rdf:type owl:DatatypeProperty ;
	rdfs:comment "Identifier of the contractor organization. " ;
	rdfs:domain [
		rdf:type owl:Class ;
		owl:unionOf (
			osdu:PerforationJob
			osdu:PlannedCementJob
		) ;
	] ;
	xsd:pattern "^[\\\\w\\\\-\\\\.]+:master-data\\\\-\\\\-Organisation:[\\\\w\\\\-\\\\.\\\\:\\\\%]+:[0-9]*$" ;
	rdfs:range xsd:string ;
.

###  https://w3id.org/osdu#contractorOrganisationID
osdu:contractorOrganisationID rdf:type owl:DatatypeProperty ;
	rdfs:comment "Reference to a company that provided services. " ;
	rdfs:domain osdu:Contractors ;
	xsd:pattern "^[\\\\w\\\\-\\\\.]+:master-data\\\\-\\\\-Organisation:[\\\\w\\\\-\\\\.\\\\:\\\\%]+:[0-9]*$" ;
	rdfs:range xsd:string ;
.

###  https://w3id.org/osdu#contractorSupervisor
osdu:contractorSupervisor rdf:type owl:DatatypeProperty ;
	rdfs:comment "Name of contractor supervisor overseeing the job " ;
	rdfs:domain osdu:PerforationJob ;
	rdfs:range xsd:string ;
.

###  https://w3id.org/osdu#contractorTypeID
osdu:contractorTypeID rdf:type owl:DatatypeProperty ;
	rdfs:comment "The identifier of a reference value for the role of a contractor providing services, such as Recording, Line Clearing, Positioning, Data Processing. " ;
	rdfs:domain osdu:Contractors ;
	xsd:pattern "^[\\\\w\\\\-\\\\.]+:reference-data\\\\-\\\\-ContractorType:[\\\\w\\\\-\\\\.\\\\:\\\\%]+:[0-9]*$" ;
	rdfs:range xsd:string ;
.

###  https://w3id.org/osdu#conveyedMethodID
osdu:conveyedMethodID rdf:type owl:DatatypeProperty ;
	rdfs:comment "How guns are conveyed " ;
	rdfs:domain osdu:PerforationJob ;
	xsd:pattern "^[\\\\w\\\\-\\\\.]+:reference-data\\\\-\\\\-PerforationConveyedMethod:[\\\\w\\\\-\\\\.\\\\:\\\\%]+:[0-9]*$" ;
	rdfs:range xsd:string ;
.

###  https://w3id.org/osdu#coordTfmVersion
osdu:coordTfmVersion rdf:type owl:DatatypeProperty ;
	rdfs:comment "The name of the transformation version or variant " ;
	rdfs:domain osdu:CoordinateTransformation ;
	rdfs:range xsd:string ;
.

###  https://w3id.org/osdu#coordinateQualityCheckDateTime
osdu:coordinateQualityCheckDateTime rdf:type owl:DatatypeProperty ;
	rdfs:comment "The date of the Quality Check. " ;
	rdfs:domain osdu:AbstractSpatialLocation ;
	rdfs:range time:DateTimeDescription ;
.

###  https://w3id.org/osdu#coordinateQualityCheckPerformedBy
osdu:coordinateQualityCheckPerformedBy rdf:type owl:DatatypeProperty ;
	rdfs:comment "The user who performed the Quality Check. " ;
	rdfs:domain osdu:AbstractSpatialLocation ;
	rdfs:range acl:AuthenticatedAgent ;
.

###  https://w3id.org/osdu#coordinateQualityCheckRemarks
osdu:coordinateQualityCheckRemarks rdf:type owl:DatatypeProperty ;
	rdfs:comment "Freetext remarks on Quality Check. " ;
	rdfs:domain osdu:AbstractSpatialLocation ;
	rdfs:range xsd:string ;
.

###  https://w3id.org/osdu#coordinateReferenceSystemID
osdu:coordinateReferenceSystemID rdf:type owl:DatatypeProperty ;
	rdfs:comment "The CRS reference into the CoordinateReferenceSystem reference list. " ;
	rdfs:domain [
		rdf:type owl:Class ;
		owl:unionOf (
			osdu:AbstractAnyCrsFeatureCollection
			osdu:FrameOfReferenceCRS
			osdu:AbstractSpatialReference
			osdu:GeoTIFF
		) ;
	] ;
	xsd:pattern "^[\\\\w\\\\-\\\\.]+:reference-data\\\\-\\\\-CoordinateReferenceSystem:[\\\\w\\\\-\\\\.\\\\:\\\\%]+:[0-9]*$" ;
	rdfs:range xsd:string ;
.

###  https://w3id.org/osdu#coordinateReferenceSystemType
osdu:coordinateReferenceSystemType rdf:type owl:DatatypeProperty ;
	rdfs:comment "The type of coordinate reference system. This is an enumeration of concrete sub-types. " ;
	rdfs:domain osdu:CoordinateReferenceSystem ;
	rdfs:range xsd:string ;
.

###  https://w3id.org/osdu#coordinateTransformationType
osdu:coordinateTransformationType rdf:type owl:DatatypeProperty ;
	rdfs:comment "The type of coordinate transformation. This is an enumeration of concrete sub-types. Transformation is a single operation between a source and a target geodetic CRS; ConcatenatedOperation is a chained set of Transformations. " ;
	rdfs:domain osdu:CoordinateTransformation ;
	rdfs:range xsd:string ;
.

###  https://w3id.org/osdu#coreDiameter
osdu:coreDiameter rdf:type owl:DatatypeProperty ;
	rdfs:comment "A measurement that represents the diameter of the core. " ;
	rdfs:domain [
		rdf:type owl:Class ;
		owl:unionOf (
			osdu:Core
			osdu:Coring
		) ;
	] ;
	rdfs:range xsd:decimal ;
.

###  https://w3id.org/osdu#coreIdentifier
osdu:coreIdentifier rdf:type owl:DatatypeProperty ;
	rdfs:comment "Native identifier from a Master Data Management System or other trusted source external to OSDU - stored here in order to allow for multi-system connection and synchronization. If used, the Source property should identify that source system. i.e. this item is optional. " ;
	rdfs:domain osdu:Coring ;
	rdfs:range xsd:string ;
.

###  https://w3id.org/osdu#coreNumber
osdu:coreNumber rdf:type owl:DatatypeProperty ;
	rdfs:comment "An identifier, assigned by the well operator, that uniquely identifies the core. " ;
	rdfs:domain [
		rdf:type owl:Class ;
		owl:unionOf (
			osdu:Core
			osdu:Coring
		) ;
	] ;
	rdfs:range xsd:string ;
.

###  https://w3id.org/osdu#coreRecoveredDate
osdu:coreRecoveredDate rdf:type owl:DatatypeProperty ;
	rdfs:comment "The date the core returned to surface. " ;
	rdfs:domain osdu:Coring ;
	rdfs:range time:DateTimeDescription ;
.

###  https://w3id.org/osdu#coringID
osdu:coringID rdf:type owl:DatatypeProperty ;
	rdfs:comment "Identifies the Core from which this sample or analysis is derived. " ;
	rdfs:domain [
		rdf:type owl:Class ;
		owl:unionOf (
			osdu:RockSample
			osdu:RockSampleAnalysis
		) ;
	] ;
	xsd:pattern "^[\\\\w\\\\-\\\\.]+:master-data\\\\-\\\\-Coring:[\\\\w\\\\-\\\\.\\\\:\\\\%]+:[0-9]*$" ;
	rdfs:range xsd:string ;
.

###  https://w3id.org/osdu#coringOperationDate
osdu:coringOperationDate rdf:type owl:DatatypeProperty ;
	rdfs:comment "The date of the coring operation. " ;
	rdfs:domain osdu:Coring ;
	rdfs:range time:DateTimeDescription ;
.

###  https://w3id.org/osdu#correctToExternalUnitOfMeasureID
osdu:correctToExternalUnitOfMeasureID rdf:type owl:DatatypeProperty ;
	rdfs:comment "For CatalogMapStateType:Corrected or CatalogMapStateType:Convert, use a conversion to this intermediate unit before swapping the reference to the platform standard UnitOfMeasure. Absent for other map states. " ;
	rdfs:domain osdu:ExternalUnitOfMeasure ;
	xsd:pattern "^[\\\\w\\\\-\\\\.]+:reference-data\\\\-\\\\-ExternalUnitOfMeasure:[\\\\w\\\\-\\\\.\\\\:\\\\%]+:[0-9]*$" ;
	rdfs:range xsd:string ;
.

###  https://w3id.org/osdu#cost
osdu:cost rdf:type owl:DatatypeProperty ;
	rdfs:comment "Bit cost in local currency. " ;
	rdfs:domain osdu:BitRecord ;
	rdfs:range xsd:decimal ;
.

###  https://w3id.org/osdu#costClass
osdu:costClass rdf:type owl:DatatypeProperty ;
	rdfs:comment "Cost class code. " ;
	rdfs:domain osdu:Cost ;
	rdfs:range xsd:string ;
.

###  https://w3id.org/osdu#costCode
osdu:costCode rdf:type owl:DatatypeProperty ;
	rdfs:comment "Cost code. " ;
	rdfs:domain osdu:Cost ;
	rdfs:range xsd:string ;
.

###  https://w3id.org/osdu#costCurrency
osdu:costCurrency rdf:type owl:DatatypeProperty ;
	rdfs:comment "Currency used for Cost Amount " ;
	rdfs:domain [
		rdf:type owl:Class ;
		owl:unionOf (
			osdu:BitRecord
			osdu:Cost
		) ;
	] ;
	rdfs:range xsd:string ;
.

###  https://w3id.org/osdu#costDay
osdu:costDay rdf:type owl:DatatypeProperty ;
	rdfs:comment "Daily cost. " ;
	rdfs:domain osdu:OperationsReport ;
	rdfs:range xsd:decimal ;
.

###  https://w3id.org/osdu#costDayMud
osdu:costDayMud rdf:type owl:DatatypeProperty ;
	rdfs:comment "Daily mud cost. " ;
	rdfs:domain [
		rdf:type owl:Class ;
		owl:unionOf (
			osdu:DrillingReportStatusInfo
			osdu:OperationsReport
		) ;
	] ;
	rdfs:range xsd:decimal ;
.

###  https://w3id.org/osdu#costGroup
osdu:costGroup rdf:type owl:DatatypeProperty ;
	rdfs:comment "Cost group code. " ;
	rdfs:domain osdu:Cost ;
	rdfs:range xsd:string ;
.

###  https://w3id.org/osdu#costItem
osdu:costItem rdf:type owl:DatatypeProperty ;
	rdfs:comment "Cost for the product for the report interval. " ;
	rdfs:domain osdu:Inventory ;
	rdfs:range xsd:string ;
.

###  https://w3id.org/osdu#costLossEstimate
osdu:costLossEstimate rdf:type owl:DatatypeProperty ;
	rdfs:comment "Gross estimate of the cost incurred due to the incident. " ;
	rdfs:domain osdu:Incident ;
	rdfs:range xsd:decimal ;
.

###  https://w3id.org/osdu#costPoolName
osdu:costPoolName rdf:type owl:DatatypeProperty ;
	rdfs:comment "Name of pool/reservoir that this cost item can be accounted to. " ;
	rdfs:domain osdu:Cost ;
	rdfs:range xsd:string ;
.

###  https://w3id.org/osdu#costSubCode
osdu:costSubCode rdf:type owl:DatatypeProperty ;
	rdfs:comment "Cost subcode. " ;
	rdfs:domain osdu:Cost ;
	rdfs:range xsd:string ;
.

###  https://w3id.org/osdu#count
osdu:count rdf:type owl:DatatypeProperty ;
	rdfs:comment "The count of indexable element " ;
	rdfs:domain osdu:IndexableElementCount ;
	rdfs:range xsd:integer ;
.

###  https://w3id.org/osdu#counterparties
osdu:counterparties rdf:type owl:DatatypeProperty ;
	rdfs:comment "A list of references to legal entities which are party to the agreement in addition to Company. " ;
	rdfs:domain osdu:Agreement ;
	xsd:pattern "^[\\\\w\\\\-\\\\.]+:master-data\\\\-\\\\-Organisation:[\\\\w\\\\-\\\\.\\\\:\\\\%]+:[0-9]*$" ;
	rdfs:range xsd:string ;
.

###  https://w3id.org/osdu#coveragePercent
osdu:coveragePercent rdf:type owl:DatatypeProperty ;
	rdfs:comment "Nominal design fold, expressed as the mode in percentage points (60 fold = 6000%). " ;
	rdfs:domain [
		rdf:type owl:Class ;
		owl:unionOf (
			osdu:AbstractBinGrid
			osdu:SeismicTraceData
		) ;
	] ;
	rdfs:range xsd:decimal ;
.

###  https://w3id.org/osdu#createTime
osdu:createTime rdf:type owl:DatatypeProperty ;
	rdfs:comment "Timestamp of the time at which initial version of this OSDU resource object was created. Set by the System. The value is a combined date-time string in ISO-8601 given in UTC. " ;
	rdfs:domain osdu:System ;
	rdfs:range time:DateTimeDescription ;
.

###  https://w3id.org/osdu#createUser
osdu:createUser rdf:type owl:DatatypeProperty ;
	rdfs:comment "The user reference, which created the first version of this resource object. Set by the System. " ;
	rdfs:domain osdu:System ;
	rdfs:range acl:AuthenticatedAgent ;
.

###  https://w3id.org/osdu#creationDateTime
osdu:creationDateTime rdf:type owl:DatatypeProperty ;
	rdfs:comment "Creation DateTime " ;
	rdfs:domain [
		rdf:type owl:Class ;
		owl:unionOf (
			osdu:AbstractWorkProductComponent
			osdu:DataCollection
			osdu:WorkProduct
		) ;
	] ;
	rdfs:range time:DateTimeDescription ;
.

###  https://w3id.org/osdu#criteriaTemplateName
osdu:criteriaTemplateName rdf:type owl:DatatypeProperty ;
	rdfs:comment "The name of a pass/fail or acceptance criteria template that applies for the step " ;
	rdfs:domain osdu:WBETestStep ;
	rdfs:range xsd:string ;
.

###  https://w3id.org/osdu#crosslineIncrement
osdu:crosslineIncrement rdf:type owl:DatatypeProperty ;
	rdfs:comment "Sampling interval of crosslines in this dataset (difference in labels between neighboring crosslines). " ;
	rdfs:domain osdu:SeismicTraceData ;
	rdfs:range xsd:decimal ;
.

###  https://w3id.org/osdu#crosslineMax
osdu:crosslineMax rdf:type owl:DatatypeProperty ;
	rdfs:comment "Largest Xline/Cross line/Bin Value " ;
	rdfs:domain [
		rdf:type owl:Class ;
		owl:unionOf (
			osdu:SeismicTraceData
			osdu:SeismicHorizon
		) ;
	] ;
	rdfs:range xsd:decimal ;
.

###  https://w3id.org/osdu#crosslineMin
osdu:crosslineMin rdf:type owl:DatatypeProperty ;
	rdfs:comment "Smallest Xline/Cross line/Bin Value " ;
	rdfs:domain [
		rdf:type owl:Class ;
		owl:unionOf (
			osdu:SeismicTraceData
			osdu:SeismicHorizon
		) ;
	] ;
	rdfs:range xsd:decimal ;
.

###  https://w3id.org/osdu#crushDamageRatio
osdu:crushDamageRatio rdf:type owl:DatatypeProperty ;
	rdfs:comment "Crush Damage Ratio " ;
	rdfs:domain osdu:PerforationInterval ;
	rdfs:range xsd:decimal ;
.

###  https://w3id.org/osdu#crushZoneDiameter
osdu:crushZoneDiameter rdf:type owl:DatatypeProperty ;
	rdfs:comment "Crush Zone Diameter " ;
	rdfs:domain osdu:PerforationInterval ;
	rdfs:range xsd:decimal ;
.

###  https://w3id.org/osdu#currencyCodeNumericNumber
osdu:currencyCodeNumericNumber rdf:type owl:DatatypeProperty ;
	rdfs:comment "Standard numeric number assigned to a currency " ;
	rdfs:domain osdu:Currency ;
	rdfs:range xsd:integer ;
.

###  https://w3id.org/osdu#currencyID
osdu:currencyID rdf:type owl:DatatypeProperty ;
	rdfs:comment "Type of currency for the authorized expenditure. " ;
	rdfs:domain osdu:FundsAuthorizations ;
	xsd:pattern "^[\\\\w\\\\-\\\\.]+:reference-data\\\\-\\\\-Currency:[\\\\w\\\\-\\\\.\\\\:\\\\%]+:[0-9]*$" ;
	rdfs:range xsd:string ;
.

###  https://w3id.org/osdu#currencySymbolText
osdu:currencySymbolText rdf:type owl:DatatypeProperty ;
	rdfs:comment "The symbol for the currency. " ;
	rdfs:domain osdu:Currency ;
	rdfs:range xsd:string ;
.

###  https://w3id.org/osdu#currentOperatorID
osdu:currentOperatorID rdf:type owl:DatatypeProperty ;
	rdfs:comment "The current operator organization ID; the organization ID may also be found in the FacilityOperatorOrganisationID of the FacilityOperator array providing the actual dates. " ;
	rdfs:domain osdu:AbstractFacility ;
	xsd:pattern "^[\\\\w\\\\-\\\\.]+:master-data\\\\-\\\\-Organisation:[\\\\w\\\\-\\\\.\\\\:\\\\%]+:[0-9]*$" ;
	rdfs:range xsd:string ;
.

###  https://w3id.org/osdu#currentSeaSpeed
osdu:currentSeaSpeed rdf:type owl:DatatypeProperty ;
	rdfs:comment "The speed of the ocean current. " ;
	rdfs:domain osdu:Weather ;
	rdfs:range xsd:decimal ;
.

###  https://w3id.org/osdu#curveDataProcessingTypeIDs
osdu:curveDataProcessingTypeIDs rdf:type owl:DatatypeProperty ;
	rdfs:comment "IDs of the type and level of processing that has been applied to the curve. An array of curve processing operations that have been applied, for example 'Smoothed', 'Calibrated', etc " ;
	rdfs:domain osdu:Curves ;
	xsd:pattern "^[\\\\w\\\\-\\\\.]+:reference-data\\\\-\\\\-PPFGCurveProcessingType:[\\\\w\\\\-\\\\.\\\\:\\\\%]+:[0-9]*$" ;
	rdfs:range xsd:string ;
.

###  https://w3id.org/osdu#curveDescription
osdu:curveDescription rdf:type owl:DatatypeProperty ;
	rdfs:comment "Mnemonic-level curve description is used during parsing or reading and ingesting LAS or DLIS files, to explain the type of measurement being looked at, specifically for that moment. Curve description is specific to that single (log) mnemonic and for the entire log (acquisition run) interval. In essence, curve description defines the internal factors such as what the curve or measurement ideally is representing, how is it calculated, what are the assumptions and the constants. " ;
	rdfs:domain osdu:Curves ;
	rdfs:range xsd:string ;
.

###  https://w3id.org/osdu#curveFamilyID
osdu:curveFamilyID rdf:type owl:DatatypeProperty ;
	rdfs:comment "ID of the PPFG Curve Family of the PPFG quantity measured, for example 'Pore Pressure from Corrected Drilling Exponent'. An individual curve that belongs to a Main Family " ;
	rdfs:domain osdu:Curves ;
	xsd:pattern "^[\\\\w\\\\-\\\\.]+:reference-data\\\\-\\\\-PPFGCurveFamily:[\\\\w\\\\-\\\\.\\\\:\\\\%]+:[0-9]*$" ;
	rdfs:range xsd:string ;
.

###  https://w3id.org/osdu#curveFamilyMnemonicID
osdu:curveFamilyMnemonicID rdf:type owl:DatatypeProperty ;
	rdfs:comment "ID of the mnemonic of the Curve Family which is the value as received either from external providers or from internal processing team, for example 'PP DxC' " ;
	rdfs:domain osdu:Curves ;
	xsd:pattern "^[\\\\w\\\\-\\\\.]+:reference-data\\\\-\\\\-PPFGCurveMnemonic:[\\\\w\\\\-\\\\.\\\\:\\\\%]+:[0-9]*$" ;
	rdfs:range xsd:string ;
.

###  https://w3id.org/osdu#curveID
osdu:curveID rdf:type owl:DatatypeProperty ;
	rdfs:comment "The ID of the Curve " ;
	rdfs:domain osdu:Curves ;
	rdfs:range xsd:string ;
.

###  https://w3id.org/osdu#curveLithologyID
osdu:curveLithologyID rdf:type owl:DatatypeProperty ;
	rdfs:comment "ID of the lithological unit represented by the curve " ;
	rdfs:domain osdu:Curves ;
	xsd:pattern "^[\\\\w\\\\-\\\\.]+:reference-data\\\\-\\\\-PPFGCurveLithoType:[\\\\w\\\\-\\\\.\\\\:\\\\%]+:[0-9]*$" ;
	rdfs:range xsd:string ;
.

###  https://w3id.org/osdu#curveMainFamilyID
osdu:curveMainFamilyID rdf:type owl:DatatypeProperty ;
	rdfs:comment "ID of the Main Family Type of the PPFG quantity measured, for example 'Pore Pressure'. Primarily used for high level curve classification " ;
	rdfs:domain osdu:Curves ;
	xsd:pattern "^[\\\\w\\\\-\\\\.]+:reference-data\\\\-\\\\-PPFGCurveMainFamily:[\\\\w\\\\-\\\\.\\\\:\\\\%]+:[0-9]*$" ;
	rdfs:range xsd:string ;
.

###  https://w3id.org/osdu#curveName
osdu:curveName rdf:type owl:DatatypeProperty ;
	rdfs:comment "The original or as supplied PPFG curve name. Intended to hold historical or legacy information " ;
	rdfs:domain osdu:Curves ;
	rdfs:range xsd:string ;
.

###  https://w3id.org/osdu#curveProbabilityID
osdu:curveProbabilityID rdf:type owl:DatatypeProperty ;
	rdfs:comment "ID of the PPFG Curve probability, for example 'Most Likely Case' and 'P50' " ;
	rdfs:domain osdu:Curves ;
	xsd:pattern "^[\\\\w\\\\-\\\\.]+:reference-data\\\\-\\\\-PPFGCurveProbability:[\\\\w\\\\-\\\\.\\\\:\\\\%]+:[0-9]*$" ;
	rdfs:range xsd:string ;
.

###  https://w3id.org/osdu#curveQuality
osdu:curveQuality rdf:type owl:DatatypeProperty ;
	rdfs:comment "The Quality of the Log Curve. " ;
	rdfs:domain osdu:Curves ;
	rdfs:range xsd:string ;
.

###  https://w3id.org/osdu#curveSampleTypeID
osdu:curveSampleTypeID rdf:type owl:DatatypeProperty ;
	rdfs:comment "The value type to be expected as curve sample values. " ;
	rdfs:domain osdu:Curves ;
	xsd:pattern "^[\\\\w\\\\-\\\\.]+:reference-data\\\\-\\\\-CurveSampleType:[\\\\w\\\\-\\\\.\\\\:\\\\%]+:[0-9]*$" ;
	rdfs:range xsd:string ;
.

###  https://w3id.org/osdu#curveTransformModelTypeID
osdu:curveTransformModelTypeID rdf:type owl:DatatypeProperty ;
	rdfs:comment "ID of the empirical calibrated model used for pressure calculations from a petrophysical curve (sonic or resistivity logs), for example 'Eaton' and  'Bowers',...  " ;
	rdfs:domain osdu:Curves ;
	xsd:pattern "^[\\\\w\\\\-\\\\.]+:reference-data\\\\-\\\\-PPFGCurveTransformModelType:[\\\\w\\\\-\\\\.\\\\:\\\\%]+:[0-9]*$" ;
	rdfs:range xsd:string ;
.

###  https://w3id.org/osdu#curveUOM
osdu:curveUOM rdf:type owl:DatatypeProperty ;
	rdfs:comment "Unit of Measure of the Physical Quantity Measured by the curve. An ID to relevant unit of measure reference " ;
	rdfs:domain osdu:Curves ;
	xsd:pattern "^[\\\\w\\\\-\\\\.]+:reference-data\\\\-\\\\-UnitOfMeasure:[\\\\w\\\\-\\\\.\\\\:\\\\%]+:[0-9]*$" ;
	rdfs:range xsd:string ;
.

###  https://w3id.org/osdu#curveUnit
osdu:curveUnit rdf:type owl:DatatypeProperty ;
	rdfs:comment "Unit of Measure for the Log Curve " ;
	rdfs:domain osdu:Curves ;
	xsd:pattern "^[\\\\w\\\\-\\\\.]+:reference-data\\\\-\\\\-UnitOfMeasure:[\\\\w\\\\-\\\\.\\\\:\\\\%]+:[0-9]*$" ;
	rdfs:range xsd:string ;
.

###  https://w3id.org/osdu#curveVersion
osdu:curveVersion rdf:type owl:DatatypeProperty ;
	rdfs:comment "The Version of the Log Curve. " ;
	rdfs:domain osdu:Curves ;
	rdfs:range xsd:string ;
.

###  https://w3id.org/osdu#customer
osdu:customer rdf:type owl:DatatypeProperty ;
	rdfs:comment "Individual, company, or corporate division that work is being executed on behalf of " ;
	rdfs:domain osdu:OperationsReport ;
	rdfs:range xsd:string ;
.

###  https://w3id.org/osdu#customerId
osdu:customerId rdf:type owl:DatatypeProperty ;
	rdfs:comment "Reference to the Organisation that represents the Customer " ;
	rdfs:domain osdu:OperationsReport ;
	xsd:pattern "^[\\\\w\\\\-\\\\.]+:master-data\\\\-\\\\-Organisation:[\\\\w\\\\-\\\\.\\\\:\\\\%]+:[0-9]*$" ;
	rdfs:range xsd:string ;
.

###  https://w3id.org/osdu#cut
osdu:cut rdf:type owl:DatatypeProperty ;
	rdfs:comment "Flag describing the existence of a cut (accidentally or intentionally) in the line " ;
	rdfs:domain osdu:TubularUmbilical ;
	rdfs:range xsd:boolean ;
.

###  https://w3id.org/osdu#cutDate
osdu:cutDate rdf:type owl:DatatypeProperty ;
	rdfs:comment "The date the cut has happened " ;
	rdfs:domain osdu:TubularUmbilical ;
	rdfs:range time:DateTimeDescription ;
.

###  https://w3id.org/osdu#cutMD
osdu:cutMD rdf:type owl:DatatypeProperty ;
	rdfs:comment "Measured Depth at which the cut has happened " ;
	rdfs:domain osdu:TubularUmbilical ;
	rdfs:range xsd:decimal ;
.

###  https://w3id.org/osdu#dataObjectContentType
osdu:dataObjectContentType rdf:type owl:DatatypeProperty ;
	rdfs:comment "When parameter is limited to data object of given types, describe the allowed types. Used only when ParameterType is dataObject.  String is an OSDU kind of work product component. " ;
	rdfs:domain osdu:ParameterTemplate ;
	rdfs:range xsd:string ;
.

###  https://w3id.org/osdu#dataObjectParameter
osdu:dataObjectParameter rdf:type owl:DatatypeProperty ;
	rdfs:comment "Parameter referencing to a top level object. " ;
	rdfs:domain osdu:AbstractActivityParameter ;
	xsd:pattern "^[\\\\w\\\\-\\\\.]+:[\\\\w\\\\-\\\\.]+:[\\\\w\\\\-\\\\.\\\\:\\\\%]+:[0-9]*$" ;
	rdfs:range xsd:string ;
.

###  https://w3id.org/osdu#dataQuantityParameter
osdu:dataQuantityParameter rdf:type owl:DatatypeProperty ;
	rdfs:comment "Parameter containing a double value. " ;
	rdfs:domain osdu:AbstractActivityParameter ;
	rdfs:range xsd:decimal ;
.

###  https://w3id.org/osdu#dataQuantityParameterUOMID
osdu:dataQuantityParameterUOMID rdf:type owl:DatatypeProperty ;
	rdfs:comment "Identifies unit of measure for floating point value. " ;
	rdfs:domain osdu:AbstractActivityParameter ;
	xsd:pattern "^[\\\\w\\\\-\\\\.]+:reference-data\\\\-\\\\-UnitOfMeasure:[\\\\w\\\\-\\\\.\\\\:\\\\%]+:[0-9]*$" ;
	rdfs:range xsd:string ;
.

###  https://w3id.org/osdu#dataRuleCreatedBy
osdu:dataRuleCreatedBy rdf:type owl:DatatypeProperty ;
	rdfs:comment "User that created the rule independent of OSDU " ;
	rdfs:domain osdu:QualityDataRule ;
	rdfs:range xsd:string ;
.

###  https://w3id.org/osdu#dataRuleCreatedOn
osdu:dataRuleCreatedOn rdf:type owl:DatatypeProperty ;
	rdfs:comment "Date of creation of data rule independent of OSDU " ;
	rdfs:domain osdu:QualityDataRule ;
	rdfs:range time:DateTimeDescription ;
.

###  https://w3id.org/osdu#dataRuleDimensionTypeID
osdu:dataRuleDimensionTypeID rdf:type owl:DatatypeProperty ;
	rdfs:comment "Dimension of the Rule indicating the rule purpose like completeness, validity etc. " ;
	rdfs:domain osdu:QualityDataRule ;
	xsd:pattern "^[\\\\w\\\\-\\\\.]+:reference-data\\\\-\\\\-DataRuleDimensionType:[\\\\w\\\\-\\\\.\\\\:\\\\%]+:[0-9]*$" ;
	rdfs:range xsd:string ;
.

###  https://w3id.org/osdu#dataRuleID
osdu:dataRuleID rdf:type owl:DatatypeProperty ;
	rdfs:comment "The relationship to the individual QualityDataRule. " ;
	rdfs:domain [
		rdf:type owl:Class ;
		owl:unionOf (
			osdu:DataRules
			osdu:DataRule
		) ;
	] ;
	xsd:pattern "^[\\\\w\\\\-\\\\.]+:reference-data\\\\-\\\\-QualityDataRule:[\\\\w\\\\-\\\\.\\\\:\\\\%]+:[0-9]*$" ;
	rdfs:range xsd:string ;
.

###  https://w3id.org/osdu#dataRulePublishedOn
osdu:dataRulePublishedOn rdf:type owl:DatatypeProperty ;
	rdfs:comment "Timestamp of the time when the data rule was published independent of OSDU. " ;
	rdfs:domain osdu:QualityDataRule ;
	rdfs:range time:DateTimeDescription ;
.

###  https://w3id.org/osdu#dataRulePurposeClass
osdu:dataRulePurposeClass rdf:type owl:DatatypeProperty ;
	rdfs:comment "Indicated if the QualityDataRule is required to pass or for information. " ;
	rdfs:domain osdu:DataRule ;
	xsd:pattern "^[\\\\w\\\\-\\\\.]+:reference-data\\\\-\\\\-DataRulePurposeType:[\\\\w\\\\-\\\\.\\\\:\\\\%]+:[0-9]*$" ;
	rdfs:range xsd:string ;
.

###  https://w3id.org/osdu#dataRuleRevision
osdu:dataRuleRevision rdf:type owl:DatatypeProperty ;
	rdfs:comment "Revision version number " ;
	rdfs:domain osdu:QualityDataRule ;
	rdfs:range xsd:string ;
.

###  https://w3id.org/osdu#dataRuleRunStatus
osdu:dataRuleRunStatus rdf:type owl:DatatypeProperty ;
	rdfs:comment "True if data rule has passed, False if data rule did not pass. " ;
	rdfs:domain osdu:DataRules ;
	rdfs:range xsd:boolean ;
.

###  https://w3id.org/osdu#dataRuleSetID
osdu:dataRuleSetID rdf:type owl:DatatypeProperty ;
	rdfs:comment "The relationship to the QualityDataRuleSet. " ;
	rdfs:domain osdu:DataRuleSets ;
	xsd:pattern "^[\\\\w\\\\-\\\\.]+:reference-data\\\\-\\\\-QualityDataRuleSet:[\\\\w\\\\-\\\\.\\\\:\\\\%]+:[0-9]*$" ;
	rdfs:range xsd:string ;
.

###  https://w3id.org/osdu#dataRuleSetRunStatus
osdu:dataRuleSetRunStatus rdf:type owl:DatatypeProperty ;
	rdfs:comment "True if data ruleset rule has passed, False if data ruleset rule dit not pass. " ;
	rdfs:domain osdu:DataRuleSets ;
	rdfs:range xsd:boolean ;
.

###  https://w3id.org/osdu#dataRuleStatement
osdu:dataRuleStatement rdf:type owl:DatatypeProperty ;
	rdfs:comment "Expression of data rule " ;
	rdfs:domain osdu:QualityDataRule ;
	rdfs:range xsd:string ;
.

###  https://w3id.org/osdu#dataRuleStatus
osdu:dataRuleStatus rdf:type owl:DatatypeProperty ;
	rdfs:comment "status of the business rule such as Published " ;
	rdfs:domain osdu:QualityDataRule ;
	rdfs:range xsd:string ;
.

###  https://w3id.org/osdu#dataRuleUpdatedOn
osdu:dataRuleUpdatedOn rdf:type owl:DatatypeProperty ;
	rdfs:comment "Timestamp of the time when the data rule was updated independent of OSDU. " ;
	rdfs:domain osdu:QualityDataRule ;
	rdfs:range time:DateTimeDescription ;
.

###  https://w3id.org/osdu#dataSource
osdu:dataSource rdf:type owl:DatatypeProperty ;
	rdfs:comment "The person, vendor or other provider of this information. " ;
	rdfs:domain osdu:RockSample ;
	rdfs:range xsd:string ;
.

###  https://w3id.org/osdu#dataSourceOrganisationID
osdu:dataSourceOrganisationID rdf:type owl:DatatypeProperty ;
	rdfs:comment "The main source of the header information. " ;
	rdfs:domain osdu:AbstractFacility ;
	xsd:pattern "^[\\\\w\\\\-\\\\.]+:master-data\\\\-\\\\-Organisation:[\\\\w\\\\-\\\\.\\\\:\\\\%]+:[0-9]*$" ;
	rdfs:range xsd:string ;
.

###  https://w3id.org/osdu#dataSourceReferenceKeys
osdu:dataSourceReferenceKeys rdf:type owl:DatatypeProperty ;
	rdfs:comment "Reference to history in source system, for example Jobpro jobset id, dataset id, workflow id " ;
	rdfs:domain osdu:VelocityModeling ;
	rdfs:range xsd:integer ;
.

###  https://w3id.org/osdu#dataSourceSystem
osdu:dataSourceSystem rdf:type owl:DatatypeProperty ;
	rdfs:comment "System providing data source history, eg. Jobpro, etc. " ;
	rdfs:domain osdu:VelocityModeling ;
	rdfs:range xsd:string ;
.

###  https://w3id.org/osdu#datasets
osdu:datasets rdf:type owl:DatatypeProperty ;
	rdfs:comment "The record id, which identifies this OSDU File or dataset resource. " ;
	rdfs:domain osdu:AbstractWPCGroupType ;
	xsd:pattern "^[\\\\w\\\\-\\\\.]+:dataset\\\\-\\\\-[\\\\w\\\\-\\\\.]+:[\\\\w\\\\-\\\\.\\\\:\\\\%]+:[0-9]*$" ;
	rdfs:range xsd:string ;
.

###  https://w3id.org/osdu#date
osdu:date rdf:type owl:DatatypeProperty ;
	rdfs:comment "Date the status has been established " ;
	rdfs:domain osdu:TubularAssemblyStatus ;
	rdfs:range time:DateTimeDescription ;
.

###  https://w3id.org/osdu#dateModified
osdu:dateModified rdf:type owl:DatatypeProperty ;
	rdfs:comment "The UTC date time and date of the document when it was last modified " ;
	rdfs:domain osdu:Document ;
	rdfs:range time:DateTimeDescription ;
.

###  https://w3id.org/osdu#datePublished
osdu:datePublished rdf:type owl:DatatypeProperty ;
	rdfs:comment "The UTC date time and date of the document publication " ;
	rdfs:domain osdu:Document ;
	rdfs:range time:DateTimeDescription ;
.

###  https://w3id.org/osdu#dateStamp
osdu:dateStamp rdf:type owl:DatatypeProperty ;
	rdfs:comment "Date curve was created in the database " ;
	rdfs:domain osdu:Curves ;
	rdfs:range time:DateTimeDescription ;
.

###  https://w3id.org/osdu#dateTime
osdu:dateTime rdf:type owl:DatatypeProperty ;
	rdfs:comment "Date and time that event occurred " ;
	rdfs:domain [
		rdf:type owl:Class ;
		owl:unionOf (
			osdu:Weather
			osdu:PumpOperations
			osdu:MudVolume
			osdu:Incident
			osdu:MudLosses
			osdu:GasReading
		) ;
	] ;
	rdfs:range time:DateTimeDescription ;
.

###  https://w3id.org/osdu#daylightSavingTimeEndDate
osdu:daylightSavingTimeEndDate rdf:type owl:DatatypeProperty ;
	rdfs:comment "Day light saving end date. " ;
	rdfs:domain osdu:GeoPoliticalEntity ;
	rdfs:range time:DateTimeDescription ;
.

###  https://w3id.org/osdu#daylightSavingTimeStartDate
osdu:daylightSavingTimeStartDate rdf:type owl:DatatypeProperty ;
	rdfs:comment "Day light saving start date. " ;
	rdfs:domain osdu:GeoPoliticalEntity ;
	rdfs:range time:DateTimeDescription ;
.

###  https://w3id.org/osdu#daysIncidentFree
osdu:daysIncidentFree rdf:type owl:DatatypeProperty ;
	rdfs:comment "Incident free duration (commonly in days). " ;
	rdfs:domain osdu:HealthSafetyEnvironment ;
	rdfs:range xsd:integer ;
.

###  https://w3id.org/osdu#deadline
osdu:deadline rdf:type owl:DatatypeProperty ;
	rdfs:comment "Date the response must be completed " ;
	rdfs:domain osdu:RiskResponse ;
	rdfs:range time:DateTimeDescription ;
.

###  https://w3id.org/osdu#defaultUnitID
osdu:defaultUnitID rdf:type owl:DatatypeProperty ;
	rdfs:comment "The default UnitOfMeasure to be used for this measurement name. If empty, the first element of the mandatory PreferredUnitIDs array should be taken. The DefaultUnitID should be member of the PreferredUnitIDs array. " ;
	rdfs:domain osdu:Configuration ;
	xsd:pattern "^[\\\\w\\\\-\\\\.]+:reference-data\\\\-\\\\-UnitOfMeasure:[\\\\w\\\\-\\\\.\\\\:\\\\%]+:[0-9]*$" ;
	rdfs:range xsd:string ;
.

###  https://w3id.org/osdu#defaultUnitOfMeasureID
osdu:defaultUnitOfMeasureID rdf:type owl:DatatypeProperty ;
	rdfs:comment "The unit of measure for quantity. " ;
	rdfs:domain osdu:ParameterType ;
	xsd:pattern "^[\\\\w\\\\-\\\\.]+:reference-data\\\\-\\\\-UnitOfMeasure:[\\\\w\\\\-\\\\.\\\\:\\\\%]+:[0-9]*$" ;
	rdfs:range xsd:string ;
.

###  https://w3id.org/osdu#defaultVerticalCRSID
osdu:defaultVerticalCRSID rdf:type owl:DatatypeProperty ;
	rdfs:comment "The default vertical coordinate reference system used in the vertical measurements for a well or wellbore if absent from input vertical measurements and there is no other recourse for obtaining a valid CRS. " ;
	rdfs:domain osdu:Well ;
	xsd:pattern "^[\\\\w\\\\-\\\\.]+:reference-data\\\\-\\\\-CoordinateReferenceSystem:[\\\\w\\\\-\\\\.\\\\:\\\\%]+:[0-9]*$" ;
	rdfs:range xsd:string ;
.

###  https://w3id.org/osdu#defaultVerticalMeasurementID
osdu:defaultVerticalMeasurementID rdf:type owl:DatatypeProperty ;
	rdfs:comment "The default datum reference point, or zero depth point, used to determine other points vertically in a well.  References an entry in the VerticalMeasurements array. " ;
	rdfs:domain [
		rdf:type owl:Class ;
		owl:unionOf (
			osdu:Wellbore
			osdu:Well
		) ;
	] ;
	rdfs:range xsd:string ;
.

###  https://w3id.org/osdu#definitionOrganisationID
osdu:definitionOrganisationID rdf:type owl:DatatypeProperty ;
	rdfs:comment "The StandardsOrganisation (reference-data) or Organisation (master-data) that provided the name (the source). " ;
	rdfs:domain osdu:AbstractAliasNames ;
	xsd:pattern "^[\\\\w\\\\-\\\\.]+:(reference-data\\\\-\\\\-StandardsOrganisation|master-data\\\\-\\\\-Organisation):[\\\\w\\\\-\\\\.\\\\:\\\\%]+:[0-9]*$" ;
	rdfs:range xsd:string ;
.

###  https://w3id.org/osdu#definitiveTrajectoryID
osdu:definitiveTrajectoryID rdf:type owl:DatatypeProperty ;
	rdfs:comment "SRN of Wellbore Trajectory which is considered the authoritative or preferred version. " ;
	rdfs:domain osdu:Wellbore ;
	xsd:pattern "^[\\\\w\\\\-\\\\.]+:work-product-component\\\\-\\\\-WellboreTrajectory:[\\\\w\\\\-\\\\.\\\\:\\\\%]+:[0-9]*$" ;
	rdfs:range xsd:string ;
.

###  https://w3id.org/osdu#densAtPres
osdu:densAtPres rdf:type owl:DatatypeProperty ;
	rdfs:comment "Slurry density at pressure. " ;
	rdfs:domain osdu:CementingFluid ;
	rdfs:range xsd:decimal ;
.

###  https://w3id.org/osdu#densDisplaceFluid
osdu:densDisplaceFluid rdf:type owl:DatatypeProperty ;
	rdfs:comment "Density of displacement fluid. " ;
	rdfs:domain osdu:CementStage ;
	rdfs:range xsd:decimal ;
.

###  https://w3id.org/osdu#density
osdu:density rdf:type owl:DatatypeProperty ;
	rdfs:comment "Fluid density. " ;
	rdfs:domain [
		rdf:type owl:Class ;
		owl:unionOf (
			osdu:Fluid
			osdu:CementingFluid
		) ;
	] ;
	rdfs:range xsd:decimal ;
.

###  https://w3id.org/osdu#depositionGeometryTypeID
osdu:depositionGeometryTypeID rdf:type owl:DatatypeProperty ;
	rdfs:comment "The reference to the deposition geometry type (Energistics RESQML DepositionMode) of this StratigraphicUnitInterpretation. RESQML BUSINESS RULE: The deposition mode for a geological unit MUST be consistent with the boundary relations of a genetic boundary. If it is not, then the boundary relation declaration is retained. " ;
	rdfs:domain osdu:StratigraphicUnitInterpretation ;
	xsd:pattern "^[\\\\w\\\\-\\\\.]+:reference-data\\\\-\\\\-DepositionGeometryType:[\\\\w\\\\-\\\\.\\\\:\\\\%]+:[0-9]*$" ;
	rdfs:range xsd:string ;
.

###  https://w3id.org/osdu#depth
osdu:depth rdf:type owl:DatatypeProperty ;
	rdfs:comment "Depth of the aquifer " ;
	rdfs:domain osdu:SingleCellAquifer ;
	rdfs:range xsd:decimal ;
.

###  https://w3id.org/osdu#depthCoding
osdu:depthCoding rdf:type owl:DatatypeProperty ;
	rdfs:comment "DEPRECATED: Replaced by boolean data.IsRegular. The Coding of the depth. " ;
	rdfs:domain osdu:Curves ;
	xsd:pattern "^REGULAR|DISCRETE$" ;
	rdfs:range xsd:string ;
.

###  https://w3id.org/osdu#depthPerforationBase
osdu:depthPerforationBase rdf:type owl:DatatypeProperty ;
	rdfs:comment "Perforation Base Depth for the DST to run through. Depth relative to Planned wellbore ZDP. Navigate via WellboreID to the side-car WellPlanningWellbore, which holds the depth reference in data.VerticalMeasurement. " ;
	rdfs:domain osdu:DSTRun ;
	rdfs:range xsd:decimal ;
.

###  https://w3id.org/osdu#depthPerforationTop
osdu:depthPerforationTop rdf:type owl:DatatypeProperty ;
	rdfs:comment "Perforation Top Depth for the DST to run through. Depth relative to Planned wellbore ZDP. Navigate via WellboreID to the side-car WellPlanningWellbore, which holds the depth reference in data.VerticalMeasurement. " ;
	rdfs:domain osdu:DSTRun ;
	rdfs:range xsd:decimal ;
.

###  https://w3id.org/osdu#depthShiftsID
osdu:depthShiftsID rdf:type owl:DatatypeProperty ;
	rdfs:comment "The WellLog representation carrying the core-depth to logging-depth correction or mapping used or to be used with this analysis. " ;
	rdfs:domain osdu:RockSampleAnalysis ;
	xsd:pattern "^[\\\\w\\\\-\\\\.]+:work-product-component\\\\-\\\\-WellLog:[\\\\w\\\\-\\\\.\\\\:\\\\%]+:[0-9]*$" ;
	rdfs:range xsd:string ;
.

###  https://w3id.org/osdu#depthUnit
osdu:depthUnit rdf:type owl:DatatypeProperty ;
	rdfs:comment "Unit of Measure for TopDepth and BaseDepth. " ;
	rdfs:domain osdu:Curves ;
	xsd:pattern "^[\\\\w\\\\-\\\\.]+:reference-data\\\\-\\\\-UnitOfMeasure:[\\\\w\\\\-\\\\.\\\\:\\\\%]+:[0-9]*$" ;
	rdfs:range xsd:string ;
.

###  https://w3id.org/osdu#description
osdu:description rdf:type owl:DatatypeProperty ;
	rdfs:comment "A general description of the object." ;
	rdfs:domain [
		rdf:type owl:Class ;
		owl:unionOf (
			osdu:AbstractDataset
			osdu:AbstractWorkProductComponent
			osdu:AbstractReferenceType
			osdu:DataCollection
			osdu:RiskResponse
			osdu:Risk
			osdu:ReferenceLevel
			osdu:ActivityTemplateArc
			osdu:ActivityTemplate
			osdu:ObjectAlias
			osdu:WellAlias
			osdu:PointsSource
			osdu:ConnectedSourceRegistryEntry
			osdu:Type
			osdu:TubularAssemblyStatus
			osdu:GeologyInterval
			osdu:PersistedCollection
			osdu:QualityDataRuleSet
			osdu:Extent
			osdu:WorkProduct
		) ;
	] ;
	rdfs:range xsd:string ;
.

###  https://w3id.org/osdu#designKickTolerance
osdu:designKickTolerance rdf:type owl:DatatypeProperty ;
	rdfs:comment "The designed maximum gas volume for a given degree of underbalance which the circulation can be performed without exceeding the weakest formation in the wellbore " ;
	rdfs:domain osdu:FormationIntegrityEvaluation ;
	rdfs:range xsd:decimal ;
.

###  https://w3id.org/osdu#detailActivity
osdu:detailActivity rdf:type owl:DatatypeProperty ;
	rdfs:comment "Custom string to further define an activity. " ;
	rdfs:domain osdu:DrillingActivity ;
	rdfs:range xsd:string ;
.

###  https://w3id.org/osdu#diameterBit
osdu:diameterBit rdf:type owl:DatatypeProperty ;
	rdfs:comment "Diameter of drilled hole. " ;
	rdfs:domain osdu:BitRecord ;
	rdfs:range xsd:decimal ;
.

###  https://w3id.org/osdu#diameterHole
osdu:diameterHole rdf:type owl:DatatypeProperty ;
	rdfs:comment "Hole nominal inside diameter. " ;
	rdfs:domain osdu:DrillingReportStatusInfo ;
	rdfs:range xsd:decimal ;
.

###  https://w3id.org/osdu#diameterHoleStartMD
osdu:diameterHoleStartMD rdf:type owl:DatatypeProperty ;
	rdfs:comment "Measured depth to the start of the current hole diameter. " ;
	rdfs:domain osdu:DrillingReportStatusInfo ;
	rdfs:range xsd:decimal ;
.

###  https://w3id.org/osdu#diameterPassThrough
osdu:diameterPassThrough rdf:type owl:DatatypeProperty ;
	rdfs:comment "Minimum hole or tubing which bit will pass through (for bi-center bits). " ;
	rdfs:domain osdu:BitRecord ;
	rdfs:range xsd:decimal ;
.

###  https://w3id.org/osdu#diameterPilot
osdu:diameterPilot rdf:type owl:DatatypeProperty ;
	rdfs:comment "Pilot hole nominal inside diameter. " ;
	rdfs:domain [
		rdf:type owl:Class ;
		owl:unionOf (
			osdu:BitRecord
			osdu:DrillingReportStatusInfo
		) ;
	] ;
	rdfs:range xsd:decimal ;
.

###  https://w3id.org/osdu#diameterPilotPlanMD
osdu:diameterPilotPlanMD rdf:type owl:DatatypeProperty ;
	rdfs:comment "The planned measured depth of the pilot hole. " ;
	rdfs:domain osdu:DrillingReportStatusInfo ;
	rdfs:range xsd:decimal ;
.

###  https://w3id.org/osdu#diameterPilotPlanTVD
osdu:diameterPilotPlanTVD rdf:type owl:DatatypeProperty ;
	rdfs:comment "The planned true vertical depth of the pilot hole. " ;
	rdfs:domain osdu:DrillingReportStatusInfo ;
	rdfs:range xsd:decimal ;
.

###  https://w3id.org/osdu#difference
osdu:difference rdf:type owl:DatatypeProperty ;
	rdfs:comment "Indicates if the volume is a product of the difference between 4D surveys " ;
	rdfs:domain osdu:SeismicTraceData ;
	rdfs:range xsd:boolean ;
.

###  https://w3id.org/osdu#dimensionNodeCounts
osdu:dimensionNodeCounts rdf:type owl:DatatypeProperty ;
	rdfs:comment "The number of grid nodes in each direction (i,j,k) " ;
	rdfs:domain osdu:VelocityModeling ;
	rdfs:range xsd:integer ;
.

###  https://w3id.org/osdu#dimensionType
osdu:dimensionType rdf:type owl:DatatypeProperty ;
	rdfs:comment "Is this model defined along a line, on a surface, for a volume, for a time series? " ;
	rdfs:domain osdu:VelocityModeling ;
	xsd:pattern "^[\\\\w\\\\-\\\\.]+:reference-data\\\\-\\\\-DimensionType:[\\\\w\\\\-\\\\.\\\\:\\\\%]+:[0-9]*$" ;
	rdfs:range xsd:string ;
.

###  https://w3id.org/osdu#dip
osdu:dip rdf:type owl:DatatypeProperty ;
	rdfs:comment "Angle of dip of target reference plane with respect to horizontal " ;
	rdfs:domain osdu:Geometry ;
	rdfs:range xsd:decimal ;
.

###  https://w3id.org/osdu#dipAzimuth
osdu:dipAzimuth rdf:type owl:DatatypeProperty ;
	rdfs:comment "Direction of dip of target reference plane with respect to north azimuth reference " ;
	rdfs:domain osdu:Geometry ;
	rdfs:range xsd:decimal ;
.

###  https://w3id.org/osdu#dischargeCoefficient
osdu:dischargeCoefficient rdf:type owl:DatatypeProperty ;
	rdfs:comment "Initial discharge coefficient after perforating but prior to hydraulic fracturing.  A coefficient used in the equation for calculation of pressure drop across a perforation set. " ;
	rdfs:domain osdu:PerforationInterval ;
	rdfs:range xsd:decimal ;
.

###  https://w3id.org/osdu#discretisationSchemeType
osdu:discretisationSchemeType rdf:type owl:DatatypeProperty ;
	rdfs:comment "Given a discretisation of a property field (e.g. a  mesh), the value of a property may refer to a vertex, the center of a cell, or the region covered by a cell.  When vertical interpolation is constant, this also includes an indication of Z Grid Registration, which whether the sample value pertains to the top, center, of bottom of grid. " ;
	rdfs:domain osdu:VelocityModeling ;
	xsd:pattern "^[\\\\w\\\\-\\\\.]+:reference-data\\\\-\\\\-DiscretisationSchemeType:[\\\\w\\\\-\\\\.\\\\:\\\\%]+:[0-9]*$" ;
	rdfs:range xsd:string ;
.

###  https://w3id.org/osdu#disputedIndicator
osdu:disputedIndicator rdf:type owl:DatatypeProperty ;
	rdfs:comment "Indicates whether the GeoPolitical entity has a disputed status. " ;
	rdfs:domain osdu:GeoPoliticalEntity ;
	rdfs:range xsd:boolean ;
.

###  https://w3id.org/osdu#distDrillRot
osdu:distDrillRot rdf:type owl:DatatypeProperty ;
	rdfs:comment "Distance drilled: rotating. " ;
	rdfs:domain osdu:DrillingReportStatusInfo ;
	rdfs:range xsd:decimal ;
.

###  https://w3id.org/osdu#distDrillSlid
osdu:distDrillSlid rdf:type owl:DatatypeProperty ;
	rdfs:comment "Distance drilled: sliding. " ;
	rdfs:domain osdu:DrillingReportStatusInfo ;
	rdfs:range xsd:decimal ;
.

###  https://w3id.org/osdu#distHold
osdu:distHold rdf:type owl:DatatypeProperty ;
	rdfs:comment "Distance covered while holding angle with a steerable drilling assembly. " ;
	rdfs:domain osdu:DrillingReportStatusInfo ;
	rdfs:range xsd:decimal ;
.

###  https://w3id.org/osdu#distReam
osdu:distReam rdf:type owl:DatatypeProperty ;
	rdfs:comment "Distance reamed. " ;
	rdfs:domain osdu:DrillingReportStatusInfo ;
	rdfs:range xsd:decimal ;
.

###  https://w3id.org/osdu#distSteering
osdu:distSteering rdf:type owl:DatatypeProperty ;
	rdfs:comment "Distance covered while actively steering with a steerable drilling assembly. " ;
	rdfs:domain osdu:DrillingReportStatusInfo ;
	rdfs:range xsd:decimal ;
.

###  https://w3id.org/osdu#distanceDrilledRotating
osdu:distanceDrilledRotating rdf:type owl:DatatypeProperty ;
	rdfs:comment "Distance drilled - rotating. " ;
	rdfs:domain osdu:DrillingParameters ;
	rdfs:range xsd:decimal ;
.

###  https://w3id.org/osdu#distanceDrilledSliding
osdu:distanceDrilledSliding rdf:type owl:DatatypeProperty ;
	rdfs:comment "Distance drilled - sliding " ;
	rdfs:domain osdu:DrillingParameters ;
	rdfs:range xsd:decimal ;
.

###  https://w3id.org/osdu#distanceHolding
osdu:distanceHolding rdf:type owl:DatatypeProperty ;
	rdfs:comment "Distance covered while holding angle with a steerable drilling assembly. " ;
	rdfs:domain osdu:DrillingParameters ;
	rdfs:range xsd:decimal ;
.

###  https://w3id.org/osdu#distanceReamed
osdu:distanceReamed rdf:type owl:DatatypeProperty ;
	rdfs:comment "Distance reamed. " ;
	rdfs:domain osdu:DrillingParameters ;
	rdfs:range xsd:decimal ;
.

###  https://w3id.org/osdu#distanceSteering
osdu:distanceSteering rdf:type owl:DatatypeProperty ;
	rdfs:comment "Distance covered while actively steering with a steerable drilling assembly. " ;
	rdfs:domain osdu:DrillingParameters ;
	rdfs:range xsd:decimal ;
.

###  https://w3id.org/osdu#documentLanguage
osdu:documentLanguage rdf:type owl:DatatypeProperty ;
	rdfs:comment "Document language as listed in the ISO 639-3 https://en.wikipedia.org/wiki/ISO_639, https://en.wikipedia.org/wiki/List_of_ISO_639-3_codes " ;
	rdfs:domain osdu:Document ;
	rdfs:range xsd:string ;
.

###  https://w3id.org/osdu#documentSubject
osdu:documentSubject rdf:type owl:DatatypeProperty ;
	rdfs:comment "A description text or an array of subjects covered by the document. If present this information must compliment the Tag and SubTitle " ;
	rdfs:domain osdu:Document ;
	rdfs:range xsd:string ;
.

###  https://w3id.org/osdu#documentTypeID
osdu:documentTypeID rdf:type owl:DatatypeProperty ;
	rdfs:comment "The kind of document--from a business standpoint, e.g., seismic processing report, etc. " ;
	rdfs:domain osdu:Document ;
	xsd:pattern "^[\\\\w\\\\-\\\\.]+:reference-data\\\\-\\\\-DocumentType:[\\\\w\\\\-\\\\.\\\\:\\\\%]+:[0-9]*$" ;
	rdfs:range xsd:string ;
.

###  https://w3id.org/osdu#dogleg
osdu:dogleg rdf:type owl:DatatypeProperty ;
	rdfs:comment "Dogleg severity. " ;
	rdfs:domain osdu:BHARun ;
	rdfs:range xsd:decimal ;
.

###  https://w3id.org/osdu#domainTypeID
osdu:domainTypeID rdf:type owl:DatatypeProperty ;
	rdfs:comment "Describes the domain of the interpretation: Depth, Time, Mixed " ;
	rdfs:domain osdu:AbstractInterpretation ;
	xsd:pattern "^[\\\\w\\\\-\\\\.]+:reference-data\\\\-\\\\-DomainType:[\\\\w\\\\-\\\\.\\\\:\\\\%]+:[0-9]*$" ;
	rdfs:range xsd:string ;
.

###  https://w3id.org/osdu#downholeTemperature
osdu:downholeTemperature rdf:type owl:DatatypeProperty ;
	rdfs:comment "Downhole temperature value " ;
	rdfs:domain osdu:TestFluid ;
	rdfs:range xsd:decimal ;
.

###  https://w3id.org/osdu#driftDiameter
osdu:driftDiameter rdf:type owl:DatatypeProperty ;
	rdfs:comment "The drift diameter is the inside diameter (ID) that the pipe manufacturer guarantees per specifications. Note that the nominal inside diameter is not the same as the drift diameter but is always slightly larger. The drift diameter is used by the well planner to determine what size tools or casing strings can later be run through the casing, whereas the nominal inside diameter is used for fluid volume calculations such as mud circulating times and cement slurry placement calculations. " ;
	rdfs:domain [
		rdf:type owl:Class ;
		owl:unionOf (
			osdu:TubularAssembly
			osdu:TubularComponent
		) ;
	] ;
	rdfs:range xsd:decimal ;
.

###  https://w3id.org/osdu#drilledDistance
osdu:drilledDistance rdf:type owl:DatatypeProperty ;
	rdfs:comment "Distance drilled.  This should be measured along the centerline of the wellbore. " ;
	rdfs:domain osdu:DrillingReportStatusInfo ;
	rdfs:range xsd:decimal ;
.

###  https://w3id.org/osdu#drilledIntervalBeforeTest
osdu:drilledIntervalBeforeTest rdf:type owl:DatatypeProperty ;
	rdfs:comment "The depth of the interval drilled before the integrity test. Depth relative to Planned wellbore ZDP. Navigate via WellboreID to the side-car WellPlanningWellbore, which holds the depth reference in data.VerticalMeasurement. " ;
	rdfs:domain osdu:FormationIntegrityEvaluation ;
	rdfs:range xsd:decimal ;
.

###  https://w3id.org/osdu#drillingFluidProperty
osdu:drillingFluidProperty rdf:type owl:DatatypeProperty ;
	rdfs:comment "Type of mud at time of logging (oil, water based,...) " ;
	rdfs:domain osdu:WellLog ;
	rdfs:range xsd:string ;
.

###  https://w3id.org/osdu#drillingReasonTypeID
osdu:drillingReasonTypeID rdf:type owl:DatatypeProperty ;
	rdfs:comment "Identifier of the drilling reason type for the corresponding time period. " ;
	rdfs:domain osdu:AbstractWellboreDrillingReason ;
	xsd:pattern "^[\\\\w\\\\-\\\\.]+:reference-data\\\\-\\\\-DrillingReasonType:[\\\\w\\\\-\\\\.\\\\:\\\\%]+:[0-9]*$" ;
	rdfs:range xsd:string ;
.

###  https://w3id.org/osdu#drillingStartDateTime
osdu:drillingStartDateTime rdf:type owl:DatatypeProperty ;
	rdfs:comment "Start on bottom - date and time. " ;
	rdfs:domain osdu:BHARun ;
	rdfs:range time:DateTimeDescription ;
.

###  https://w3id.org/osdu#drillingStopDateTime
osdu:drillingStopDateTime rdf:type owl:DatatypeProperty ;
	rdfs:comment "Start off bottom - date and time. " ;
	rdfs:domain osdu:BHARun ;
	rdfs:range time:DateTimeDescription ;
.

###  https://w3id.org/osdu#driveType
osdu:driveType rdf:type owl:DatatypeProperty ;
	rdfs:comment "Bit drive type (Motor, rotary table etc). " ;
	rdfs:domain osdu:BitRecord ;
	rdfs:range xsd:string ;
.

###  https://w3id.org/osdu#dryBlendDensity
osdu:dryBlendDensity rdf:type owl:DatatypeProperty ;
	rdfs:comment "Density of Dry blend. " ;
	rdfs:domain osdu:CementingFluid ;
	rdfs:range xsd:decimal ;
.

###  https://w3id.org/osdu#dryBlendDescription
osdu:dryBlendDescription rdf:type owl:DatatypeProperty ;
	rdfs:comment "Description of dry blend. " ;
	rdfs:domain osdu:CementingFluid ;
	rdfs:range xsd:string ;
.

###  https://w3id.org/osdu#dryBlendMass
osdu:dryBlendMass rdf:type owl:DatatypeProperty ;
	rdfs:comment "Mass of dry blend: the blend is made of different solid additives: the volume is not constant. " ;
	rdfs:domain osdu:CementingFluid ;
	rdfs:range xsd:decimal ;
.

###  https://w3id.org/osdu#dryBlendMassSack
osdu:dryBlendMassSack rdf:type owl:DatatypeProperty ;
	rdfs:comment "Weight of a sack of dry blend. " ;
	rdfs:domain osdu:CementingFluid ;
	rdfs:range xsd:decimal ;
.

###  https://w3id.org/osdu#dryBlendName
osdu:dryBlendName rdf:type owl:DatatypeProperty ;
	rdfs:comment "Name of dry blend. " ;
	rdfs:domain osdu:CementingFluid ;
	rdfs:range xsd:string ;
.

###  https://w3id.org/osdu#duration
osdu:duration rdf:type owl:DatatypeProperty ;
	rdfs:comment "The activity duration (commonly in hours). " ;
	rdfs:domain osdu:DrillingActivity ;
	rdfs:range xsd:string ;
.

###  https://w3id.org/osdu#duringPerfGaugePressure
osdu:duringPerfGaugePressure rdf:type owl:DatatypeProperty ;
	rdfs:comment "Pressure during perforation " ;
	rdfs:domain osdu:PerforationInterval ;
	rdfs:range xsd:decimal ;
.

###  https://w3id.org/osdu#effectiveDate
osdu:effectiveDate rdf:type owl:DatatypeProperty ;
	rdfs:comment "Date when an action goes into effect. " ;
	rdfs:domain [
		rdf:type owl:Class ;
		owl:unionOf (
			osdu:AbstractTechnicalAssurance
			osdu:Play
			osdu:GeoPoliticalEntity
			osdu:Field
			osdu:Organisation
			osdu:Agreement
			osdu:Prospect
		) ;
	] ;
	rdfs:range time:DateTimeDescription ;
.

###  https://w3id.org/osdu#effectiveDateTime
osdu:effectiveDateTime rdf:type owl:DatatypeProperty ;
	rdfs:comment "Date and time that activities started. " ;
	rdfs:domain [
		rdf:type owl:Class ;
		owl:unionOf (
			osdu:AbstractFacilityState
			osdu:AbstractReferenceLevel
			osdu:AbstractStorageLocation
			osdu:AbstractFacilityOperator
			osdu:FundsAuthorizations
			osdu:ProjectSpecifications
			osdu:ProjectStates
			osdu:AbstractWellboreDrillingReason
			osdu:AbstractAliasNames
			osdu:AbstractFacilitySpecification
			osdu:AbstractFacilityVerticalMeasurement
			osdu:AbstractFacilityEvent
			osdu:Risk
			osdu:HistoricalInterest
			osdu:AbstractSpecification
		) ;
	] ;
	rdfs:range time:DateTimeDescription ;
.

###  https://w3id.org/osdu#elapsedTimeCirc
osdu:elapsedTimeCirc rdf:type owl:DatatypeProperty ;
	rdfs:comment "Time spent circulating from the start of the bit run. " ;
	rdfs:domain osdu:DrillingReportStatusInfo ;
	rdfs:range time:TemporalDuration ;
.

###  https://w3id.org/osdu#elapsedTimeDrill
osdu:elapsedTimeDrill rdf:type owl:DatatypeProperty ;
	rdfs:comment "Drilling time. " ;
	rdfs:domain osdu:DrillingReportStatusInfo ;
	rdfs:range time:TemporalDuration ;
.

###  https://w3id.org/osdu#elapsedTimeDrillRot
osdu:elapsedTimeDrillRot rdf:type owl:DatatypeProperty ;
	rdfs:comment "Time spent rotary drilling. " ;
	rdfs:domain osdu:DrillingReportStatusInfo ;
	rdfs:range time:TemporalDuration ;
.

###  https://w3id.org/osdu#elapsedTimeDrillSlid
osdu:elapsedTimeDrillSlid rdf:type owl:DatatypeProperty ;
	rdfs:comment "Time spent slide drilling from the start of the bit run. " ;
	rdfs:domain osdu:DrillingReportStatusInfo ;
	rdfs:range time:TemporalDuration ;
.

###  https://w3id.org/osdu#elapsedTimeHold
osdu:elapsedTimeHold rdf:type owl:DatatypeProperty ;
	rdfs:comment "Time spent with no directional drilling work (commonly in hours). " ;
	rdfs:domain osdu:DrillingReportStatusInfo ;
	rdfs:range time:TemporalDuration ;
.

###  https://w3id.org/osdu#elapsedTimeLoc
osdu:elapsedTimeLoc rdf:type owl:DatatypeProperty ;
	rdfs:comment "Time the rig has been on location (commonly in days). " ;
	rdfs:domain osdu:DrillingReportStatusInfo ;
	rdfs:range time:TemporalDuration ;
.

###  https://w3id.org/osdu#elapsedTimeReam
osdu:elapsedTimeReam rdf:type owl:DatatypeProperty ;
	rdfs:comment "Time spent reaming from the start of the bit run. " ;
	rdfs:domain osdu:DrillingReportStatusInfo ;
	rdfs:range time:TemporalDuration ;
.

###  https://w3id.org/osdu#elapsedTimeSpud
osdu:elapsedTimeSpud rdf:type owl:DatatypeProperty ;
	rdfs:comment "Time since the bit broke ground (commonly in days). " ;
	rdfs:domain osdu:DrillingReportStatusInfo ;
	rdfs:range time:TemporalDuration ;
.

###  https://w3id.org/osdu#elapsedTimeStart
osdu:elapsedTimeStart rdf:type owl:DatatypeProperty ;
	rdfs:comment "Time from the start of operations (commonly in days). " ;
	rdfs:domain osdu:DrillingReportStatusInfo ;
	rdfs:range time:TemporalDuration ;
.

###  https://w3id.org/osdu#elapsedTimeSteering
osdu:elapsedTimeSteering rdf:type owl:DatatypeProperty ;
	rdfs:comment "Time spent steering the bottomhole assembly (commonly in hours). " ;
	rdfs:domain osdu:DrillingReportStatusInfo ;
	rdfs:range time:TemporalDuration ;
.

###  https://w3id.org/osdu#electStab
osdu:electStab rdf:type owl:DatatypeProperty ;
	rdfs:comment "Measurement of the emulsion stability and oil-wetting capability in oil-based muds. " ;
	rdfs:domain osdu:Fluid ;
	rdfs:range xsd:decimal ;
.

###  https://w3id.org/osdu#elementCount
osdu:elementCount rdf:type owl:DatatypeProperty ;
	rdfs:comment "The count of elements in this subrepresentation " ;
	rdfs:domain osdu:SubRepresentation ;
	rdfs:range xsd:integer ;
.

###  https://w3id.org/osdu#emailAddress
osdu:emailAddress rdf:type owl:DatatypeProperty ;
	rdfs:comment "Contact email address. Property may be left empty where it is inappropriate to provide personally identifiable information. " ;
	rdfs:domain osdu:AbstractContact ;
	rdfs:range xsd:string ;
.

###  https://w3id.org/osdu#encodingFormatTypeID
osdu:encodingFormatTypeID rdf:type owl:DatatypeProperty ;
	rdfs:comment "EncodingFormatType ID reference value relationship. It can be a mime-type or media-type. " ;
	rdfs:domain [
		rdf:type owl:Class ;
		owl:unionOf (
			osdu:AbstractDataset
			osdu:AbstractFileSourceInfo
		) ;
	] ;
	xsd:pattern "^[\\\\w\\\\-\\\\.]+:reference-data\\\\-\\\\-EncodingFormatType:[\\\\w\\\\-\\\\.\\\\:\\\\%]+:[0-9]*$" ;
	rdfs:range xsd:string ;
.

###  https://w3id.org/osdu#endDate
osdu:endDate rdf:type owl:DatatypeProperty ;
	rdfs:comment "The Date at which activities ended " ;
	rdfs:domain [
		rdf:type owl:Class ;
		owl:unionOf (
			osdu:Terms
			osdu:LogServiceDateInterval
			osdu:AcquisitionDateRanges
		) ;
	] ;
	rdfs:range time:DateTimeDescription ;
.

###  https://w3id.org/osdu#endDateActivity
osdu:endDateActivity rdf:type owl:DatatypeProperty ;
	rdfs:comment "The end date and time for the activity that this rig was utilized for " ;
	rdfs:domain osdu:RigUtilization ;
	rdfs:range time:DateTimeDescription ;
.

###  https://w3id.org/osdu#endDateTime
osdu:endDateTime rdf:type owl:DatatypeProperty ;
	rdfs:comment "Date and time that activities ended. " ;
	rdfs:domain [
		rdf:type owl:Class ;
		owl:unionOf (
			osdu:FluidsReport
			osdu:OperationsReport
			osdu:DrillingActivity
		) ;
	] ;
	rdfs:range time:DateTimeDescription ;
.

###  https://w3id.org/osdu#endDepth
osdu:endDepth rdf:type owl:DatatypeProperty ;
	rdfs:comment "The sample axis value in the vertical dimension at which Depth formatted data ends. Use SeismicDomainType to know which of time or depth pairs is the actual range vs. what is estimated. " ;
	rdfs:domain osdu:SeismicTraceData ;
	rdfs:range xsd:decimal ;
.

###  https://w3id.org/osdu#endHoleDepth
osdu:endHoleDepth rdf:type owl:DatatypeProperty ;
	rdfs:comment "Measured depth of the wellbore when operations performed with this rig ended. Depth relative to Planned wellbore ZDP. Navigate via HoleSectionId and WellboreID to the side-car WellPlanningWellbore, which holds the depth reference in data.VerticalMeasurement. " ;
	rdfs:domain osdu:RigUtilization ;
	rdfs:range xsd:decimal ;
.

###  https://w3id.org/osdu#endMeasuredDepth
osdu:endMeasuredDepth rdf:type owl:DatatypeProperty ;
	rdfs:comment "Hole measured depth at which the survey run will end/ended. Depth relative to Planned wellbore ZDP. Navigate via WellboreID to the side-car WellPlanningWellbore, which holds the depth reference in data.VerticalMeasurement. " ;
	rdfs:domain osdu:SurveySection ;
	rdfs:range xsd:decimal ;
.

###  https://w3id.org/osdu#endTime
osdu:endTime rdf:type owl:DatatypeProperty ;
	rdfs:comment "The sample axis value in the vertical dimension at which Time formatted data starts. Use SeismicDomainType to know which of time or depth pairs is the actual range vs. what is estimated. " ;
	rdfs:domain osdu:SeismicTraceData ;
	rdfs:range xsd:decimal ;
.

###  https://w3id.org/osdu#endYear
osdu:endYear rdf:type owl:DatatypeProperty ;
	rdfs:comment "The year that the satellite mission ceased or ended. Leave blank if the mission is still active. " ;
	rdfs:domain osdu:OperationalPeriod ;
	rdfs:range xsd:integer ;
.

###  https://w3id.org/osdu#endian
osdu:endian rdf:type owl:DatatypeProperty ;
	rdfs:comment "Endianness of binary value.  Enumeration: BIG, LITTLE.  If absent, applications will need to interpret from context indicators. " ;
	rdfs:domain osdu:AbstractDataset ;
	rdfs:range xsd:string ;
.

###  https://w3id.org/osdu#energySourceTypeID
osdu:energySourceTypeID rdf:type owl:DatatypeProperty ;
	rdfs:comment "Seismic Source type. E.g.: Airgun, Vibroseis, Dynamite,Watergun. " ;
	rdfs:domain [
		rdf:type owl:Class ;
		owl:unionOf (
			osdu:SeismicAcquisitionSurvey
			osdu:SeismicSourceConfiguration
		) ;
	] ;
	xsd:pattern "^[\\\\w\\\\-\\\\.]+:reference-data\\\\-\\\\-SeismicEnergySourceType:[\\\\w\\\\-\\\\.\\\\:\\\\%]+:[0-9]*$" ;
	rdfs:range xsd:string ;
.

###  https://w3id.org/osdu#engineer
osdu:engineer rdf:type owl:DatatypeProperty ;
	rdfs:comment "Name of engineer. " ;
	rdfs:domain [
		rdf:type owl:Class ;
		owl:unionOf (
			osdu:SurveyProgram
			osdu:DrillingReportStatusInfo
		) ;
	] ;
	rdfs:range xsd:string ;
.

###  https://w3id.org/osdu#entranceHoleDiameter
osdu:entranceHoleDiameter rdf:type owl:DatatypeProperty ;
	rdfs:comment "Perforation Entrance Hole Diameter " ;
	rdfs:domain osdu:PerforationInterval ;
	rdfs:range xsd:decimal ;
.

###  https://w3id.org/osdu#equivalentCirculatingDensity
osdu:equivalentCirculatingDensity rdf:type owl:DatatypeProperty ;
	rdfs:comment "Equivalent circulating density where fluid reading was recorded or calculated/simulated " ;
	rdfs:domain osdu:Fluid ;
	rdfs:range xsd:decimal ;
.

###  https://w3id.org/osdu#equivalentMudWeightEstimated
osdu:equivalentMudWeightEstimated rdf:type owl:DatatypeProperty ;
	rdfs:comment "The total amount of pressure exerted at a true vertical depth which is denoted in the mud density. " ;
	rdfs:domain osdu:FormationIntegrityEvaluation ;
	rdfs:range xsd:decimal ;
.

###  https://w3id.org/osdu#equivalentStaticDensity
osdu:equivalentStaticDensity rdf:type owl:DatatypeProperty ;
	rdfs:comment "Equivalent static density where fluid reading was recorded or calculated/simulated " ;
	rdfs:domain osdu:Fluid ;
	rdfs:range xsd:decimal ;
.

###  https://w3id.org/osdu#errorModel
osdu:errorModel rdf:type owl:DatatypeProperty ;
	rdfs:comment "Error model used to calculate ellipses of uncertainty. " ;
	rdfs:domain osdu:SurveySection ;
	rdfs:range xsd:string ;
.

###  https://w3id.org/osdu#estimateHoursLost
osdu:estimateHoursLost rdf:type owl:DatatypeProperty ;
	rdfs:comment "Number of hours lost due to the incident. " ;
	rdfs:domain osdu:Incident ;
	rdfs:range xsd:decimal ;
.

###  https://w3id.org/osdu#estimatedCementTopMeasuredDepth
osdu:estimatedCementTopMeasuredDepth rdf:type owl:DatatypeProperty ;
	rdfs:comment "The estimated Measured depth of the Top of Cement. Depth relative to Planned wellbore ZDP. Navigate via WellboreID to the side-car WellPlanningWellbore, which holds the depth reference in data.VerticalMeasurement. " ;
	rdfs:domain osdu:PlannedCementJob ;
	rdfs:range xsd:decimal ;
.

###  https://w3id.org/osdu#estimatedHoleMeasuredDepth
osdu:estimatedHoleMeasuredDepth rdf:type owl:DatatypeProperty ;
	rdfs:comment "Estimated measured depth at bottom of hole. Depth relative to Planned wellbore ZDP. Navigate via WellboreID to the side-car WellPlanningWellbore, which holds the depth reference in data.VerticalMeasurement. " ;
	rdfs:domain osdu:PlannedCementJob ;
	rdfs:range xsd:decimal ;
.

###  https://w3id.org/osdu#estimatedPluggedBaseMeasuredDepth
osdu:estimatedPluggedBaseMeasuredDepth rdf:type owl:DatatypeProperty ;
	rdfs:comment "If Plug,  estimated measured depth of bottom of plug. Depth relative to Planned wellbore ZDP. Navigate via WellboreID to the side-car WellPlanningWellbore, which holds the depth reference in data.VerticalMeasurement. " ;
	rdfs:domain osdu:PlannedCementJob ;
	rdfs:range xsd:decimal ;
.

###  https://w3id.org/osdu#estimatedPluggedTopMeasuredDepth
osdu:estimatedPluggedTopMeasuredDepth rdf:type owl:DatatypeProperty ;
	rdfs:comment "If Plug, estimated measured depth of top of plug. Depth relative to Planned wellbore ZDP. Navigate via WellboreID to the side-car WellPlanningWellbore, which holds the depth reference in data.VerticalMeasurement. " ;
	rdfs:domain osdu:PlannedCementJob ;
	rdfs:range xsd:decimal ;
.

###  https://w3id.org/osdu#estimatedPreviousShoeMeasuredDepth
osdu:estimatedPreviousShoeMeasuredDepth rdf:type owl:DatatypeProperty ;
	rdfs:comment "Estimated measured depth of previous shoe. Depth relative to Planned wellbore ZDP. Navigate via WellboreID to the side-car WellPlanningWellbore, which holds the depth reference in data.VerticalMeasurement. " ;
	rdfs:domain osdu:PlannedCementJob ;
	rdfs:range xsd:decimal ;
.

###  https://w3id.org/osdu#estimatedPreviousShoeTrueVerticalDepth
osdu:estimatedPreviousShoeTrueVerticalDepth rdf:type owl:DatatypeProperty ;
	rdfs:comment "Estimated True Vertical Depth of previous shoe. Depth relative to Planned wellbore ZDP. Navigate via WellboreID to the side-car WellPlanningWellbore, which holds the depth reference in data.VerticalMeasurement. " ;
	rdfs:domain osdu:PlannedCementJob ;
	rdfs:range xsd:decimal ;
.

###  https://w3id.org/osdu#estimatedStringSetMeasuredDepth
osdu:estimatedStringSetMeasuredDepth rdf:type owl:DatatypeProperty ;
	rdfs:comment "Estimated measured depth of cement string shoe. Depth relative to Planned wellbore ZDP. Navigate via WellboreID to the side-car WellPlanningWellbore, which holds the depth reference in data.VerticalMeasurement. " ;
	rdfs:domain osdu:PlannedCementJob ;
	rdfs:range xsd:decimal ;
.

###  https://w3id.org/osdu#estimatedStringSetTrueVerticalDepth
osdu:estimatedStringSetTrueVerticalDepth rdf:type owl:DatatypeProperty ;
	rdfs:comment "Estimated True vertical depth of cement string shoe. Depth relative to Planned wellbore ZDP. Navigate via WellboreID to the side-car WellPlanningWellbore, which holds the depth reference in data.VerticalMeasurement. " ;
	rdfs:domain osdu:PlannedCementJob ;
	rdfs:range xsd:decimal ;
.

###  https://w3id.org/osdu#estimatedWaitingOnCement
osdu:estimatedWaitingOnCement rdf:type owl:DatatypeProperty ;
	rdfs:comment "Estimated duration for waiting on cement to set. " ;
	rdfs:domain osdu:PlannedCementJob ;
	rdfs:range xsd:string ;
.

###  https://w3id.org/osdu#ethane
osdu:ethane rdf:type owl:DatatypeProperty ;
	rdfs:comment "Ethane (C2) concentration. " ;
	rdfs:domain osdu:GasReading ;
	rdfs:range xsd:decimal ;
.

###  https://w3id.org/osdu#evaluatedKind
osdu:evaluatedKind rdf:type owl:DatatypeProperty ;
	rdfs:comment "The kind of the data this ruleset applies to. Version-specific and non-version-specific kind can be defined. For example, osdu:wks:master-data--Well:1 (requiring only the major version and permits any minor and patch version); osdu:wks:master-data--Wellbore:1.0.0 (this is version-specific); osdu:wks:work-product-component--WellLog (this is unspecific accepting any version). Also note: a total wildcard would have to end with a :  like this: osdu:wks:group-type--EntityType:. " ;
	rdfs:domain osdu:QualityDataRuleSet ;
	xsd:pattern "^[\\\\w\\\\-\\\\.]+:[\\\\w\\\\-\\\\.]+:[\\\\w\\\\-\\\\.]+:([0-9]+)?(\\\\.)?([0-9]+)?(\\\\.)?([0-9]+)?$" ;
	rdfs:range xsd:string ;
.

###  https://w3id.org/osdu#evaluatedRecordID
osdu:evaluatedRecordID rdf:type owl:DatatypeProperty ;
	rdfs:comment "The reference to the evaluated data record. The record version number is required. " ;
	rdfs:domain osdu:DataQuality ;
	xsd:pattern "^[\\\\w\\\\-\\\\.]+:(master-data\\\\-\\\\-[\\\\w\\\\-\\\\.]+|work-product\\\\-\\\\-[\\\\w\\\\-\\\\.]+|work-product-component\\\\-\\\\-[\\\\w\\\\-\\\\.]+):[\\\\w\\\\-\\\\.\\\\:\\\\%]+:[0-9]*$" ;
	rdfs:range xsd:string ;
.

###  https://w3id.org/osdu#evaluationPlanID
osdu:evaluationPlanID rdf:type owl:DatatypeProperty ;
	rdfs:comment "A reference to the object that holds the evaluation information about the drilling program for this phase. " ;
	rdfs:domain osdu:Phase ;
	xsd:pattern "^[\\\\w\\\\-\\\\.]+:master-data\\\\-\\\\-EvaluationPlan:[\\\\w\\\\-\\\\.\\\\:\\\\%]+:[0-9]*$" ;
	rdfs:range xsd:string ;
.

###  https://w3id.org/osdu#excessPercent
osdu:excessPercent rdf:type owl:DatatypeProperty ;
	rdfs:comment "Excess Percent. " ;
	rdfs:domain osdu:CementingFluid ;
	rdfs:range xsd:decimal ;
.

###  https://w3id.org/osdu#excessVolume
osdu:excessVolume rdf:type owl:DatatypeProperty ;
	rdfs:comment "Excess volume. " ;
	rdfs:domain osdu:CementStage ;
	rdfs:range xsd:decimal ;
.

###  https://w3id.org/osdu#existenceKind
osdu:existenceKind rdf:type owl:DatatypeProperty ;
	rdfs:comment "Where does this data resource sit in the cradle-to-grave span of its existence? " ;
	rdfs:domain osdu:AbstractCommonResources ;
	xsd:pattern "^[\\\\w\\\\-\\\\.]+:reference-data\\\\-\\\\-ExistenceKind:[\\\\w\\\\-\\\\.\\\\:\\\\%]+:[0-9]*$" ;
	rdfs:range xsd:string ;
.

###  https://w3id.org/osdu#expansionInDirection
osdu:expansionInDirection rdf:type owl:DatatypeProperty ;
	rdfs:comment "Indicate if a grid has been topologically expanded in a particular dimension (K expansion, J expansion, I expansion) " ;
	rdfs:domain osdu:AbstractColumnLayerGridPatch ;
	rdfs:range xsd:string ;
.

###  https://w3id.org/osdu#expectedMudVolume
osdu:expectedMudVolume rdf:type owl:DatatypeProperty ;
	rdfs:comment "Total mud volume that was expected " ;
	rdfs:domain osdu:MudVolume ;
	rdfs:range xsd:decimal ;
.

###  https://w3id.org/osdu#expectedPressureChangeDueToThermalEffects
osdu:expectedPressureChangeDueToThermalEffects rdf:type owl:DatatypeProperty ;
	rdfs:comment "The expected pressure change due to thermal effects " ;
	rdfs:domain osdu:WBETestStep ;
	rdfs:range xsd:decimal ;
.

###  https://w3id.org/osdu#expectedPressureChangeDueToThermalEffectsComments
osdu:expectedPressureChangeDueToThermalEffectsComments rdf:type owl:DatatypeProperty ;
	rdfs:comment "Comments on the expected pressure change due to thermal effects. Can be used to provide an explanation as to why a value was not entered (e.g. expansion not expected to impact test results) " ;
	rdfs:domain osdu:WBETestStep ;
	rdfs:range xsd:string ;
.

###  https://w3id.org/osdu#extendedRiskCategory
osdu:extendedRiskCategory rdf:type owl:DatatypeProperty ;
	rdfs:comment "Custom string to further extend the risk categorization " ;
	rdfs:domain osdu:Risk ;
	rdfs:range xsd:string ;
.

###  https://w3id.org/osdu#externalRuleID
osdu:externalRuleID rdf:type owl:DatatypeProperty ;
	rdfs:comment "Unique identifier to an external data rule, e.g. PPDM rule ID number. " ;
	rdfs:domain osdu:QualityDataRule ;
	rdfs:range xsd:string ;
.

###  https://w3id.org/osdu#externalUnitQuantityID
osdu:externalUnitQuantityID rdf:type owl:DatatypeProperty ;
	rdfs:comment "The External Unit Quantity is a semantic description of the quantity this ExternalUnitOfMeasure is describing ('Length' for instance). " ;
	rdfs:domain osdu:ExternalUnitOfMeasure ;
	xsd:pattern "^[\\\\w\\\\-\\\\.]+:reference-data\\\\-\\\\-ExternalUnitQuantity:[\\\\w\\\\-\\\\.\\\\:\\\\%]+:[0-9]*$" ;
	rdfs:range xsd:string ;
.

###  https://w3id.org/osdu#extrapolatedMeasuredDepth
osdu:extrapolatedMeasuredDepth rdf:type owl:DatatypeProperty ;
	rdfs:comment "The measured depth to which the survey segment was extrapolated. " ;
	rdfs:domain osdu:WellboreTrajectory ;
	rdfs:range xsd:decimal ;
.

###  https://w3id.org/osdu#face
osdu:face rdf:type owl:DatatypeProperty ;
	rdfs:comment "The faces of the box of the grid which are in connection " ;
	rdfs:domain osdu:AbstractIjkGridFlowSimulationBoundaryConnection ;
	xsd:pattern "^[\\\\w\\\\-\\\\.]+:reference-data\\\\-\\\\-IjkCellFace:[\\\\w\\\\-\\\\.\\\\:\\\\%]+:[0-9]*$" ;
	rdfs:range xsd:string ;
.

###  https://w3id.org/osdu#faceCount
osdu:faceCount rdf:type owl:DatatypeProperty ;
	rdfs:comment "The count of faces in this grid " ;
	rdfs:domain osdu:AbstractUnstructuredGridPatch ;
	rdfs:range xsd:integer ;
.

###  https://w3id.org/osdu#facetRoleID
osdu:facetRoleID rdf:type owl:DatatypeProperty ;
	rdfs:comment "Additional context about the nature of a property type. The purpose of such attribute is to minimize the need to create specialized property types by mutualizing some well known qualifiers such as maximum, minimum which apply to a lot of different property types. " ;
	rdfs:domain osdu:AbstractFacet ;
	xsd:pattern "^[\\\\w\\\\-\\\\.]+:reference-data\\\\-\\\\-FacetRole:[\\\\w\\\\-\\\\.\\\\:\\\\%]+:[0-9]*$" ;
	rdfs:range xsd:string ;
.

###  https://w3id.org/osdu#facetTypeID
osdu:facetTypeID rdf:type owl:DatatypeProperty ;
	rdfs:comment "FacetType: An 'enumeration' of the type of additional context about the nature of a property type (it may include conditions, direction, qualifiers, or statistics). " ;
	rdfs:domain osdu:AbstractFacet ;
	xsd:pattern "^[\\\\w\\\\-\\\\.]+:reference-data\\\\-\\\\-FacetType:[\\\\w\\\\-\\\\.\\\\:\\\\%]+:[0-9]*$" ;
	rdfs:range xsd:string ;
.

###  https://w3id.org/osdu#facilityEventTypeID
osdu:facilityEventTypeID rdf:type owl:DatatypeProperty ;
	rdfs:comment "The facility event type is a picklist. Examples: 'Permit', 'Spud', 'Abandon', etc. " ;
	rdfs:domain osdu:AbstractFacilityEvent ;
	xsd:pattern "^[\\\\w\\\\-\\\\.]+:reference-data\\\\-\\\\-FacilityEventType:[\\\\w\\\\-\\\\.\\\\:\\\\%]+:[0-9]*$" ;
	rdfs:range xsd:string ;
.

###  https://w3id.org/osdu#facilityID
osdu:facilityID rdf:type owl:DatatypeProperty ;
	rdfs:comment "Native identifier from a Master Data Management System or other trusted source external to OSDU - stored here in order to allow for multi-system connection and synchronization. If used, the Source property should identify that source system. " ;
	rdfs:domain osdu:AbstractFacility ;
	rdfs:range xsd:string ;
.

###  https://w3id.org/osdu#facilityName
osdu:facilityName rdf:type owl:DatatypeProperty ;
	rdfs:comment "Name of the Facility. " ;
	rdfs:domain osdu:AbstractFacility ;
	rdfs:range xsd:string ;
.

###  https://w3id.org/osdu#facilityOperatorID
osdu:facilityOperatorID rdf:type owl:DatatypeProperty ;
	rdfs:comment "Internal, unique identifier for an item 'AbstractFacilityOperator'. This identifier is used by 'AbstractFacility.CurrentOperatorID' and 'AbstractFacility.InitialOperatorID'. " ;
	rdfs:domain osdu:AbstractFacilityOperator ;
	rdfs:range xsd:string ;
.

###  https://w3id.org/osdu#facilityOperatorOrganisationID
osdu:facilityOperatorOrganisationID rdf:type owl:DatatypeProperty ;
	rdfs:comment "The company that currently operates, or previously operated the facility " ;
	rdfs:domain osdu:AbstractFacilityOperator ;
	xsd:pattern "^[\\\\w\\\\-\\\\.]+:master-data\\\\-\\\\-Organisation:[\\\\w\\\\-\\\\.\\\\:\\\\%]+:[0-9]*$" ;
	rdfs:range xsd:string ;
.

###  https://w3id.org/osdu#facilitySpecificationDateTime
osdu:facilitySpecificationDateTime rdf:type owl:DatatypeProperty ;
	rdfs:comment "The actual date and time value of the parameter. " ;
	rdfs:domain osdu:AbstractFacilitySpecification ;
	rdfs:range time:DateTimeDescription ;
.

###  https://w3id.org/osdu#facilitySpecificationIndicator
osdu:facilitySpecificationIndicator rdf:type owl:DatatypeProperty ;
	rdfs:comment "The actual indicator value of the parameter. " ;
	rdfs:domain osdu:AbstractFacilitySpecification ;
	rdfs:range xsd:boolean ;
.

###  https://w3id.org/osdu#facilitySpecificationQuantity
osdu:facilitySpecificationQuantity rdf:type owl:DatatypeProperty ;
	rdfs:comment "The value for the specified parameter type. " ;
	rdfs:domain osdu:AbstractFacilitySpecification ;
	rdfs:range xsd:decimal ;
.

###  https://w3id.org/osdu#facilitySpecificationText
osdu:facilitySpecificationText rdf:type owl:DatatypeProperty ;
	rdfs:comment "The actual text value of the parameter. " ;
	rdfs:domain osdu:AbstractFacilitySpecification ;
	rdfs:range xsd:string ;
.

###  https://w3id.org/osdu#facilityStateTypeID
osdu:facilityStateTypeID rdf:type owl:DatatypeProperty ;
	rdfs:comment "Life Cycle [Facility State Type] is a set of major phases that are significant to regulators and/or business stakeholders. Life Cycle may apply to a well or its components [or other facility]. " ;
	rdfs:domain osdu:AbstractFacilityState ;
	xsd:pattern "^[\\\\w\\\\-\\\\.]+:reference-data\\\\-\\\\-FacilityStateType:[\\\\w\\\\-\\\\.\\\\:\\\\%]+:[0-9]*$" ;
	rdfs:range xsd:string ;
.

###  https://w3id.org/osdu#facilityTypeID
osdu:facilityTypeID rdf:type owl:DatatypeProperty ;
	rdfs:comment "The definition of a kind of capability to perform a business function or a service. " ;
	rdfs:domain osdu:AbstractFacility ;
	xsd:pattern "^[\\\\w\\\\-\\\\.]+:reference-data\\\\-\\\\-FacilityType:[\\\\w\\\\-\\\\.\\\\:\\\\%]+:[0-9]*$" ;
	rdfs:range xsd:string ;
.

###  https://w3id.org/osdu#faultHeaveNumber
osdu:faultHeaveNumber rdf:type owl:DatatypeProperty ;
	rdfs:comment "Maximum stratigraphic heave, the apparent horizontal component of the net-slip. " ;
	rdfs:domain [
		rdf:type owl:Class ;
		owl:unionOf (
			osdu:Faults
			osdu:SeismicFault
		) ;
	] ;
	rdfs:range xsd:decimal ;
.

###  https://w3id.org/osdu#faultHeaveNumberUOM
osdu:faultHeaveNumberUOM rdf:type owl:DatatypeProperty ;
	rdfs:comment "ID of the Unit of Measure of the FaultHeaveNumber " ;
	rdfs:domain osdu:Faults ;
	xsd:pattern "^[\\\\w\\\\-\\\\.]+:reference-data\\\\-\\\\-UnitOfMeasure:[\\\\w\\\\-\\\\.\\\\:\\\\%]+:[0-9]*$" ;
	rdfs:range xsd:string ;
.

###  https://w3id.org/osdu#faultInterpretationID
osdu:faultInterpretationID rdf:type owl:DatatypeProperty ;
	rdfs:comment "The related FaultInterpretation for collaborating with Earth Modeling. " ;
	rdfs:domain osdu:Faults ;
	xsd:pattern "^[\\\\w\\\\-\\\\.]+:work-product-component\\\\-\\\\-FaultInterpretation:[\\\\w\\\\-\\\\.\\\\:\\\\%]+:[0-9]*$" ;
	rdfs:range xsd:string ;
.

###  https://w3id.org/osdu#faultInterpretationIDs
osdu:faultInterpretationIDs rdf:type owl:DatatypeProperty ;
	rdfs:comment "Lists the fault interpretation IDs belonging to the structural model " ;
	rdfs:domain osdu:StructuralOrganizationInterpretation ;
	xsd:pattern "^[\\\\w\\\\-\\\\.]+:work-product-component\\\\-\\\\-FaultInterpretation:[\\\\w\\\\-\\\\.\\\\:\\\\%]+:[0-9]*$" ;
	rdfs:range xsd:string ;
.

###  https://w3id.org/osdu#faultNetSlipNumber
osdu:faultNetSlipNumber rdf:type owl:DatatypeProperty ;
	rdfs:comment "Net (average) Slip " ;
	rdfs:domain [
		rdf:type owl:Class ;
		owl:unionOf (
			osdu:Faults
			osdu:SeismicFault
		) ;
	] ;
	rdfs:range xsd:decimal ;
.

###  https://w3id.org/osdu#faultNetSlipNumberUOM
osdu:faultNetSlipNumberUOM rdf:type owl:DatatypeProperty ;
	rdfs:comment "ID of the Unit of Measure of the FaultNetSlipNumber " ;
	rdfs:domain osdu:Faults ;
	xsd:pattern "^[\\\\w\\\\-\\\\.]+:reference-data\\\\-\\\\-UnitOfMeasure:[\\\\w\\\\-\\\\.\\\\:\\\\%]+:[0-9]*$" ;
	rdfs:range xsd:string ;
.

###  https://w3id.org/osdu#faultSystemID
osdu:faultSystemID rdf:type owl:DatatypeProperty ;
	rdfs:comment "An alternative, coherent set of fault representations under one work-product-component. Only one property is expected to be populated, either FaultSystem or SeismicFaultIDs. " ;
	rdfs:domain osdu:UnsealedSurfaceFramework ;
	xsd:pattern "^[\\\\w\\\\-\\\\.]+:work-product-component\\\\-\\\\-FaultSystem:[\\\\w\\\\-\\\\.\\\\:\\\\%]+:[0-9]*$" ;
	rdfs:range xsd:string ;
.

###  https://w3id.org/osdu#faultThrowTypeID
osdu:faultThrowTypeID rdf:type owl:DatatypeProperty ;
	rdfs:comment "Specifies the fault throw type (reverse, normal etc…) " ;
	rdfs:domain osdu:FaultThrowDescriptions ;
	xsd:pattern "^[\\\\w\\\\-\\\\.]+:reference-data\\\\-\\\\-FaultThrowType:[\\\\w\\\\-\\\\.\\\\:\\\\%]+:[0-9]*$" ;
	rdfs:range xsd:string ;
.

###  https://w3id.org/osdu#featureID
osdu:featureID rdf:type owl:DatatypeProperty ;
	rdfs:comment "ID of the Feature of this object. " ;
	rdfs:domain [
		rdf:type owl:Class ;
		owl:unionOf (
			osdu:AbstractInterpretation
			osdu:RockFluidUnitInterpretation
			osdu:EarthModelInterpretation
			osdu:AquiferInterpretation
			osdu:RockFluidOrganizationInterpretation
			osdu:VoidageGroupInterpretation
			osdu:StratigraphicUnitInterpretation
			osdu:GeobodyInterpretation
			osdu:StructuralOrganizationInterpretation
			osdu:ReservoirCompartmentInterpretation
		) ;
	] ;
	xsd:pattern "^[\\\\w\\\\-\\\\.]+:(master-data\\\\-\\\\-BoundaryFeature|master-data\\\\-\\\\-ModelFeature|master-data\\\\-\\\\-RockVolumeFeature|work-product-component\\\\-\\\\-LocalBoundaryFeature|work-product-component\\\\-\\\\-LocalModelFeature|work-product-component\\\\-\\\\-LocalRockVolumeFeature):[\\\\w\\\\-\\\\.\\\\:\\\\%]+:[0-9]*$" ;
	xsd:pattern "^[\\\\w\\\\-\\\\.]+:(master-data\\\\-\\\\-RockVolumeFeature|work-product-component\\\\-\\\\-LocalRockVolumeFeature):[\\\\w\\\\-\\\\.\\\\:\\\\%]+:[0-9]*$" ;
	xsd:pattern "^[\\\\w\\\\-\\\\.]+:(master-data\\\\-\\\\-ModelFeature|work-product-component\\\\-\\\\-LocalModelFeature):[\\\\w\\\\-\\\\.\\\\:\\\\%]+:[0-9]*$" ;
	xsd:pattern "^[\\\\w\\\\-\\\\.]+:(master-data\\\\-\\\\-ModelFeature|master-data\\\\-\\\\-RockVolumeFeature|work-product-component\\\\-\\\\-LocalModelFeature|work-product-component\\\\-\\\\-LocalRockVolumeFeature):[\\\\w\\\\-\\\\.\\\\:\\\\%]+:[0-9]*$" ;
	rdfs:range xsd:string ;
.

###  https://w3id.org/osdu#featureName
osdu:featureName rdf:type owl:DatatypeProperty ;
	rdfs:comment "Name of the feature this object refers to " ;
	rdfs:domain [
		rdf:type owl:Class ;
		owl:unionOf (
			osdu:AbstractInterpretation
			osdu:Markers
			osdu:RockFluidOrganizationInterpretation
		) ;
	] ;
	rdfs:range xsd:string ;
.

###  https://w3id.org/osdu#featureTypeID
osdu:featureTypeID rdf:type owl:DatatypeProperty ;
	rdfs:comment "Feature Type Reference Type. Possible values - Base, top, fault, salt, reef, sea floor " ;
	rdfs:domain osdu:Markers ;
	xsd:pattern "^[\\\\w\\\\-\\\\.]+:reference-data\\\\-\\\\-FeatureType:[\\\\w\\\\-\\\\.\\\\:\\\\%]+:[0-9]*$" ;
	rdfs:range xsd:string ;
.

###  https://w3id.org/osdu#fetchKind
osdu:fetchKind rdf:type owl:DatatypeProperty ;
	rdfs:comment "The data type/schema/kind of data being retrieved form the external source. The returned value should validate against the corresponding registered schema in the OSDU schema service. " ;
	rdfs:domain osdu:ConnectedSourceDataJob ;
	rdfs:range xsd:string ;
.

###  https://w3id.org/osdu#fieldDescription
osdu:fieldDescription rdf:type owl:DatatypeProperty ;
	rdfs:comment "A textual description of the field. " ;
	rdfs:domain osdu:Field ;
	rdfs:range xsd:string ;
.

###  https://w3id.org/osdu#fieldID
osdu:fieldID rdf:type owl:DatatypeProperty ;
	rdfs:comment "Native identifier from a Master Data Management System or other trusted source external to OSDU - stored here in order to allow for multi-system connection and synchronization. " ;
	rdfs:domain [
		rdf:type owl:Class ;
		owl:unionOf (
			osdu:AbstractGeoFieldContext
			osdu:Field
		) ;
	] ;
	xsd:pattern "^[\\\\w\\\\-\\\\.]+:master-data\\\\-\\\\-Field:[\\\\w\\\\-\\\\.\\\\:\\\\%]+:[0-9]*$" ;
	rdfs:range xsd:string ;
.

###  https://w3id.org/osdu#fieldName
osdu:fieldName rdf:type owl:DatatypeProperty ;
	rdfs:comment "The name of the field, which may or may not coincide with a hydrocarbon field. " ;
	rdfs:domain osdu:Field ;
	rdfs:range xsd:string ;
.

###  https://w3id.org/osdu#fileCollectionPath
osdu:fileCollectionPath rdf:type owl:DatatypeProperty ;
	rdfs:comment "The mandatory path to the file collection. A FileCollectionPath should represent folder level access to a set of files. " ;
	rdfs:domain osdu:DatasetProperties ;
	rdfs:range xsd:string ;
.

###  https://w3id.org/osdu#fileSize
osdu:fileSize rdf:type owl:DatatypeProperty ;
	rdfs:comment "Length of file in bytes. Implemented as string. The value must be convertible to a long integer (sizes can become very large). " ;
	rdfs:domain osdu:AbstractFileSourceInfo ;
	xsd:pattern "^[0-9]+$" ;
	rdfs:range xsd:string ;
.

###  https://w3id.org/osdu#fileSource
osdu:fileSource rdf:type owl:DatatypeProperty ;
	rdfs:comment "The location of the file. It can be a relative path. The actual access is provided via the File Service. When used in context of a FileCollection (dataset--FileCollection*) FileSource is a relative path from the FileCollectionPath. It can be used by consumers to pull an individual file if they so choose by concatenating the FileCollectionPath with the FileSource. This property is required. " ;
	rdfs:domain osdu:AbstractFileSourceInfo ;
	rdfs:range xsd:string ;
.

###  https://w3id.org/osdu#filter
osdu:filter rdf:type owl:DatatypeProperty ;
	rdfs:comment "Filter applied to the data fetch request, using data members in the FetchKind schema. " ;
	rdfs:domain osdu:ConnectedSourceDataJob ;
	rdfs:range xsd:string ;
.

###  https://w3id.org/osdu#filterCakeHthp
osdu:filterCakeHthp rdf:type owl:DatatypeProperty ;
	rdfs:comment "High temperature high pressure (HTHP) filter cake thickness. " ;
	rdfs:domain osdu:Fluid ;
	rdfs:range xsd:decimal ;
.

###  https://w3id.org/osdu#filterCakeLtlp
osdu:filterCakeLtlp rdf:type owl:DatatypeProperty ;
	rdfs:comment "Filter cake thickness at low (normal) temperature and pressure. " ;
	rdfs:domain osdu:Fluid ;
	rdfs:range xsd:decimal ;
.

###  https://w3id.org/osdu#filtrateHthp
osdu:filtrateHthp rdf:type owl:DatatypeProperty ;
	rdfs:comment "High temperature high pressure (HTHP) filtrate (volume per 30 min). " ;
	rdfs:domain osdu:Fluid ;
	rdfs:range xsd:decimal ;
.

###  https://w3id.org/osdu#filtrateLtlp
osdu:filtrateLtlp rdf:type owl:DatatypeProperty ;
	rdfs:comment "API water loss (low temperature and pressure mud filtrate measurement) (volume per 30 min). " ;
	rdfs:domain osdu:Fluid ;
	rdfs:range xsd:decimal ;
.

###  https://w3id.org/osdu#filtratePressureHthp
osdu:filtratePressureHthp rdf:type owl:DatatypeProperty ;
	rdfs:comment "High temperature high pressure (HTHP) pressure. " ;
	rdfs:domain osdu:Fluid ;
	rdfs:range xsd:decimal ;
.

###  https://w3id.org/osdu#filtrateTemperatureHthp
osdu:filtrateTemperatureHthp rdf:type owl:DatatypeProperty ;
	rdfs:comment "High temperature high pressure (HTHP) temperature. " ;
	rdfs:domain osdu:Fluid ;
	rdfs:range xsd:decimal ;
.

###  https://w3id.org/osdu#finalConditionBearing
osdu:finalConditionBearing rdf:type owl:DatatypeProperty ;
	rdfs:comment "Condition of bit bearings (integer 0-8 or E, F, N or X). " ;
	rdfs:domain osdu:BitRecord ;
	rdfs:range xsd:string ;
.

###  https://w3id.org/osdu#finalConditionDull
osdu:finalConditionDull rdf:type owl:DatatypeProperty ;
	rdfs:comment "Overall dull condition from IADC bit wear 2 character codes. " ;
	rdfs:domain osdu:BitRecord ;
	xsd:pattern "^[\\\\w\\\\-\\\\.]+:reference-data\\\\-\\\\-BitDullCode:[\\\\w\\\\-\\\\.\\\\:\\\\%]+:[0-9]*$" ;
	rdfs:range xsd:string ;
.

###  https://w3id.org/osdu#finalConditionGauge
osdu:finalConditionGauge rdf:type owl:DatatypeProperty ;
	rdfs:comment "Condition of bit gauge in 1/16 of a inch. I = in gauge, else number of 16ths out of gauge. " ;
	rdfs:domain osdu:BitRecord ;
	rdfs:range xsd:string ;
.

###  https://w3id.org/osdu#finalConditionInner
osdu:finalConditionInner rdf:type owl:DatatypeProperty ;
	rdfs:comment "Condition of inner tooth rows (inner 2/3 of bit) (0-8). " ;
	rdfs:domain osdu:BitRecord ;
	rdfs:range xsd:decimal ;
.

###  https://w3id.org/osdu#finalConditionLocation
osdu:finalConditionLocation rdf:type owl:DatatypeProperty ;
	rdfs:comment "Row and cone numbers for items which need location information (e.g. Cracked Cone, Lost Cone etc). " ;
	rdfs:domain osdu:BitRecord ;
	rdfs:range xsd:string ;
.

###  https://w3id.org/osdu#finalConditionOther
osdu:finalConditionOther rdf:type owl:DatatypeProperty ;
	rdfs:comment "Other comments on bit condition from IADC list (BitDullCode in Standard LISTS). " ;
	rdfs:domain osdu:BitRecord ;
	rdfs:range xsd:string ;
.

###  https://w3id.org/osdu#finalConditionOuter
osdu:finalConditionOuter rdf:type owl:DatatypeProperty ;
	rdfs:comment "Condition of outer tooth rows (outer 1/3 of bit) (0-8). " ;
	rdfs:domain osdu:BitRecord ;
	rdfs:range xsd:decimal ;
.

###  https://w3id.org/osdu#finalConditionReason
osdu:finalConditionReason rdf:type owl:DatatypeProperty ;
	rdfs:comment "Reason bit was pulled from IADC codes. " ;
	rdfs:domain osdu:BitRecord ;
	xsd:pattern "^[\\\\w\\\\-\\\\.]+:reference-data\\\\-\\\\-BitReasonPulled:[\\\\w\\\\-\\\\.\\\\:\\\\%]+:[0-9]*$" ;
	rdfs:range xsd:string ;
.

###  https://w3id.org/osdu#finalSurfPressure
osdu:finalSurfPressure rdf:type owl:DatatypeProperty ;
	rdfs:comment "Final surface pressure " ;
	rdfs:domain osdu:PerforationInterval ;
	rdfs:range xsd:decimal ;
.

###  https://w3id.org/osdu#finalSurfacePressure
osdu:finalSurfacePressure rdf:type owl:DatatypeProperty ;
	rdfs:comment "Pressure at Surface at end of Job " ;
	rdfs:domain osdu:PerforationJob ;
	rdfs:range xsd:decimal ;
.

###  https://w3id.org/osdu#firstCMP
osdu:firstCMP rdf:type owl:DatatypeProperty ;
	rdfs:comment "First Common Mid Point " ;
	rdfs:domain [
		rdf:type owl:Class ;
		owl:unionOf (
			osdu:SeismicTraceData
			osdu:SeismicLineGeometry
		) ;
	] ;
	rdfs:range xsd:decimal ;
.

###  https://w3id.org/osdu#firstShotPoint
osdu:firstShotPoint rdf:type owl:DatatypeProperty ;
	rdfs:comment "The shotpoint that came before all others " ;
	rdfs:domain osdu:SeismicTraceData ;
	rdfs:range xsd:decimal ;
.

###  https://w3id.org/osdu#firstStationLabel
osdu:firstStationLabel rdf:type owl:DatatypeProperty ;
	rdfs:comment "Station label (such as shot point name) corresponding to FirstCMP " ;
	rdfs:domain osdu:SeismicLineGeometry ;
	rdfs:range xsd:string ;
.

###  https://w3id.org/osdu#floatingDatumIndicator
osdu:floatingDatumIndicator rdf:type owl:DatatypeProperty ;
	rdfs:comment "Boolean to show that datum reference is not a constant.  Any description or horizon information must be described in model file(s). " ;
	rdfs:domain osdu:VelocityModeling ;
	rdfs:range xsd:boolean ;
.

###  https://w3id.org/osdu#flowTypeID
osdu:flowTypeID rdf:type owl:DatatypeProperty ;
	rdfs:comment "OAuth2 flow, or grant type " ;
	rdfs:domain osdu:SecurityScheme ;
	xsd:pattern "^[\\\\w\\\\-\\\\.]+:reference-data\\\\-\\\\-OAuth2FlowType:[\\\\w\\\\-\\\\.\\\\:\\\\%]+:[0-9]*$" ;
	rdfs:range xsd:string ;
.

###  https://w3id.org/osdu#flowrateDisplaceAv
osdu:flowrateDisplaceAv rdf:type owl:DatatypeProperty ;
	rdfs:comment "Average displacement rate. " ;
	rdfs:domain osdu:CementStage ;
	rdfs:range xsd:decimal ;
.

###  https://w3id.org/osdu#flowrateDisplaceMx
osdu:flowrateDisplaceMx rdf:type owl:DatatypeProperty ;
	rdfs:comment "Maximum displacement rate. " ;
	rdfs:domain osdu:CementStage ;
	rdfs:range xsd:decimal ;
.

###  https://w3id.org/osdu#flowrateEnd
osdu:flowrateEnd rdf:type owl:DatatypeProperty ;
	rdfs:comment "Final displacement pump rate. " ;
	rdfs:domain osdu:CementStage ;
	rdfs:range xsd:decimal ;
.

###  https://w3id.org/osdu#flowrateMudCirc
osdu:flowrateMudCirc rdf:type owl:DatatypeProperty ;
	rdfs:comment "Rate mud circulated during stage. " ;
	rdfs:domain osdu:CementStage ;
	rdfs:range xsd:decimal ;
.

###  https://w3id.org/osdu#fluidAfterMD
osdu:fluidAfterMD rdf:type owl:DatatypeProperty ;
	rdfs:comment "Static fluid level after perforating " ;
	rdfs:domain osdu:PerforationInterval ;
	rdfs:range xsd:decimal ;
.

###  https://w3id.org/osdu#fluidBaseMeasuredDepth
osdu:fluidBaseMeasuredDepth rdf:type owl:DatatypeProperty ;
	rdfs:comment "Measured depth at bottom of slurry placement. " ;
	rdfs:domain osdu:CementingFluid ;
	rdfs:range xsd:decimal ;
.

###  https://w3id.org/osdu#fluidBeforeMD
osdu:fluidBeforeMD rdf:type owl:DatatypeProperty ;
	rdfs:comment "Static fluid level before perforating " ;
	rdfs:domain osdu:PerforationInterval ;
	rdfs:range xsd:decimal ;
.

###  https://w3id.org/osdu#fluidDensitySystem
osdu:fluidDensitySystem rdf:type owl:DatatypeProperty ;
	rdfs:comment "Density value for the system fluid " ;
	rdfs:domain osdu:TestFluid ;
	rdfs:range xsd:decimal ;
.

###  https://w3id.org/osdu#fluidDensityTest
osdu:fluidDensityTest rdf:type owl:DatatypeProperty ;
	rdfs:comment "Density value for the test fluid " ;
	rdfs:domain osdu:TestFluid ;
	rdfs:range xsd:decimal ;
.

###  https://w3id.org/osdu#fluidDescription
osdu:fluidDescription rdf:type owl:DatatypeProperty ;
	rdfs:comment "Fluid description. " ;
	rdfs:domain osdu:CementingFluid ;
	rdfs:range xsd:string ;
.

###  https://w3id.org/osdu#fluidDirectionID
osdu:fluidDirectionID rdf:type owl:DatatypeProperty ;
	rdfs:comment "Fluid Direction [Well Fluid Direction] is the flow direction of the wellhead stream. The facet value can change over the life of the well or wellbore. " ;
	rdfs:domain [
		rdf:type owl:Class ;
		owl:unionOf (
			osdu:Wellbore
			osdu:WellStatusSummary
		) ;
	] ;
	xsd:pattern "^[\\\\w\\\\-\\\\.]+:reference-data\\\\-\\\\-WellFluidDirection:[\\\\w\\\\-\\\\.\\\\:\\\\%]+:[0-9]*$" ;
	rdfs:range xsd:string ;
.

###  https://w3id.org/osdu#fluidDisplace
osdu:fluidDisplace rdf:type owl:DatatypeProperty ;
	rdfs:comment "Displacement fluid name. " ;
	rdfs:domain osdu:CementStage ;
	rdfs:range xsd:string ;
.

###  https://w3id.org/osdu#fluidIndex
osdu:fluidIndex rdf:type owl:DatatypeProperty ;
	rdfs:comment "Fluid Index: 1: first fluid pumped (=original mud),  					(last-1)=Tail cement, last= displacement mud " ;
	rdfs:domain osdu:CementingFluid ;
	rdfs:range xsd:decimal ;
.

###  https://w3id.org/osdu#fluidLossAfterRate
osdu:fluidLossAfterRate rdf:type owl:DatatypeProperty ;
	rdfs:comment "Fluid lossrate after perforating " ;
	rdfs:domain osdu:PerforationInterval ;
	rdfs:range xsd:decimal ;
.

###  https://w3id.org/osdu#fluidLossBeforeRate
osdu:fluidLossBeforeRate rdf:type owl:DatatypeProperty ;
	rdfs:comment "Fluid loss rate  before perforating " ;
	rdfs:domain osdu:PerforationInterval ;
	rdfs:range xsd:decimal ;
.

###  https://w3id.org/osdu#fluidPhaseTypeID
osdu:fluidPhaseTypeID rdf:type owl:DatatypeProperty ;
	rdfs:comment "The reference to the fluid phase type " ;
	rdfs:domain osdu:RockFluidUnitInterpretation ;
	xsd:pattern "^[\\\\w\\\\-\\\\.]+:reference-data\\\\-\\\\-FluidPhaseType:[\\\\w\\\\-\\\\.\\\\:\\\\%]+:[0-9]*$" ;
	rdfs:range xsd:string ;
.

###  https://w3id.org/osdu#fluidPropertyFacetNameID
osdu:fluidPropertyFacetNameID rdf:type owl:DatatypeProperty ;
	rdfs:comment "Identifier to the list of potential types of Fluid Property Facet (e.g. Measured, Range (Min), Range (Max) " ;
	rdfs:domain osdu:FluidFacet ;
	xsd:pattern "^[\\\\w\\\\-\\\\.]+:reference-data\\\\-\\\\-FluidPropertyFacetName:[\\\\w\\\\-\\\\.\\\\:\\\\%]+:[0-9]*$" ;
	rdfs:range xsd:string ;
.

###  https://w3id.org/osdu#fluidPropertyNameID
osdu:fluidPropertyNameID rdf:type owl:DatatypeProperty ;
	rdfs:comment "An open reference list of fluid properties " ;
	rdfs:domain osdu:FluidsProperty ;
	xsd:pattern "^[\\\\w\\\\-\\\\.]+:reference-data\\\\-\\\\-FluidPropertyName:[\\\\w\\\\-\\\\.\\\\:\\\\%]+:[0-9]*$" ;
	rdfs:range xsd:string ;
.

###  https://w3id.org/osdu#fluidPropertyUnit
osdu:fluidPropertyUnit rdf:type owl:DatatypeProperty ;
	rdfs:comment "The measurement unit of the Fluid Property Value " ;
	rdfs:domain osdu:FluidFacet ;
	xsd:pattern "^[\\\\w\\\\-\\\\.]+:reference-data\\\\-\\\\-UnitOfMeasure:[\\\\w\\\\-\\\\.\\\\:\\\\%]+:[0-9]*$" ;
	rdfs:range xsd:string ;
.

###  https://w3id.org/osdu#fluidPropertyValue
osdu:fluidPropertyValue rdf:type owl:DatatypeProperty ;
	rdfs:comment "The actual value of the property " ;
	rdfs:domain osdu:FluidFacet ;
	rdfs:range xsd:decimal ;
.

###  https://w3id.org/osdu#fluidPurposeID
osdu:fluidPurposeID rdf:type owl:DatatypeProperty ;
	rdfs:comment "The purpose the mud will play in this hole section (can be Sweep, Displacement Mud). " ;
	rdfs:domain osdu:FluidsSystem ;
	xsd:pattern "^[\\\\w\\\\-\\\\.]+:reference-data\\\\-\\\\-FluidRole:[\\\\w\\\\-\\\\.\\\\:\\\\%]+:[0-9]*$" ;
	rdfs:range xsd:string ;
.

###  https://w3id.org/osdu#fluidRheologicalModelID
osdu:fluidRheologicalModelID rdf:type owl:DatatypeProperty ;
	rdfs:comment "Newtonian/Bingham/Power Law/Herschel Bulkley. " ;
	rdfs:domain osdu:CementingFluid ;
	xsd:pattern "^[\\\\w\\\\-\\\\.]+:reference-data\\\\-\\\\-FluidRheologicalModelType:[\\\\w\\\\-\\\\.\\\\:\\\\%]+:[0-9]*$" ;
	rdfs:range xsd:string ;
.

###  https://w3id.org/osdu#fluidSystemName
osdu:fluidSystemName rdf:type owl:DatatypeProperty ;
	rdfs:comment "Free text string of the common name or product name of the drilling mud. " ;
	rdfs:domain osdu:FluidsSystem ;
	rdfs:range xsd:string ;
.

###  https://w3id.org/osdu#fluidTopMeasuredDepth
osdu:fluidTopMeasuredDepth rdf:type owl:DatatypeProperty ;
	rdfs:comment "Estimated Measured depth at top of slurry placement. " ;
	rdfs:domain osdu:CementingFluid ;
	rdfs:range xsd:decimal ;
.

###  https://w3id.org/osdu#fluidTypeID
osdu:fluidTypeID rdf:type owl:DatatypeProperty ;
	rdfs:comment "A fixed list of reference values describing the high level type of the drilling fluid " ;
	rdfs:domain osdu:FluidsInterval ;
	xsd:pattern "^[\\\\w\\\\-\\\\.]+:reference-data\\\\-\\\\-FluidType:[\\\\w\\\\-\\\\.\\\\:\\\\%]+:[0-9]*$" ;
	rdfs:range xsd:string ;
.

###  https://w3id.org/osdu#fluidVolume
osdu:fluidVolume rdf:type owl:DatatypeProperty ;
	rdfs:comment "Fluid/Slurry Volume. " ;
	rdfs:domain osdu:CementingFluid ;
	rdfs:range xsd:decimal ;
.

###  https://w3id.org/osdu#fluidsIDs
osdu:fluidsIDs rdf:type owl:DatatypeProperty ;
	rdfs:comment "References to the Fluids Reports generated during this reporting period. " ;
	rdfs:domain osdu:OperationsReport ;
	xsd:pattern "^[\\\\w\\\\-\\\\.]+:master-data\\\\-\\\\-FluidsReport:[\\\\w\\\\-\\\\.\\\\:\\\\%]+:[0-9]*$" ;
	rdfs:range xsd:string ;
.

###  https://w3id.org/osdu#fluidsSupplierID
osdu:fluidsSupplierID rdf:type owl:DatatypeProperty ;
	rdfs:comment "Identifier of the fluids supplier company " ;
	rdfs:domain osdu:FluidsProgram ;
	xsd:pattern "^[\\\\w\\\\-\\\\.]+:master-data\\\\-\\\\-Organisation:[\\\\w\\\\-\\\\.\\\\:\\\\%]+:[0-9]*$" ;
	rdfs:range xsd:string ;
.

###  https://w3id.org/osdu#foldCount
osdu:foldCount rdf:type owl:DatatypeProperty ;
	rdfs:comment "The number of times a point in the subsurface is sampled.  It measures of the redundancy of common midpoint seismic data. " ;
	rdfs:domain osdu:SeismicAcquisitionSurvey ;
	rdfs:range xsd:integer ;
.

###  https://w3id.org/osdu#forecast24Hr
osdu:forecast24Hr rdf:type owl:DatatypeProperty ;
	rdfs:comment "Forecast of activities for the next 24 hrs. " ;
	rdfs:domain [
		rdf:type owl:Class ;
		owl:unionOf (
			osdu:DrillingReportStatusInfo
			osdu:OperationsReport
		) ;
	] ;
	rdfs:range xsd:string ;
.

###  https://w3id.org/osdu#formationName
osdu:formationName rdf:type owl:DatatypeProperty ;
	rdfs:comment "The name of the relevant formation." ;
	rdfs:domain [
		rdf:type owl:Class ;
		owl:unionOf (
			osdu:FormationIntegrityEvaluation
			osdu:Core
			osdu:DSTRun
		) ;
	] ;
	rdfs:range xsd:string ;
.

###  https://w3id.org/osdu#formationStrength
osdu:formationStrength rdf:type owl:DatatypeProperty ;
	rdfs:comment "The measured formation strength. This should be the final measurement before the end of the report period. " ;
	rdfs:domain osdu:DrillingReportStatusInfo ;
	rdfs:range xsd:decimal ;
.

###  https://w3id.org/osdu#formationStrengthMD
osdu:formationStrengthMD rdf:type owl:DatatypeProperty ;
	rdfs:comment "The measured depth of the formation strength measurement. " ;
	rdfs:domain osdu:DrillingReportStatusInfo ;
	rdfs:range xsd:decimal ;
.

###  https://w3id.org/osdu#formationStrengthTVD
osdu:formationStrengthTVD rdf:type owl:DatatypeProperty ;
	rdfs:comment "The true vertical depth of the formation strength measurement. " ;
	rdfs:domain osdu:DrillingReportStatusInfo ;
	rdfs:range xsd:decimal ;
.

###  https://w3id.org/osdu#frameIdentifier
osdu:frameIdentifier rdf:type owl:DatatypeProperty ;
	rdfs:comment "For multi-frame or multi-section files, this identifier defines the source frame in the file. If the identifier is an index number the index starts with zero and is converted to a string for this property. " ;
	rdfs:domain osdu:WellLog ;
	rdfs:range xsd:string ;
.

###  https://w3id.org/osdu#frequencyBandID
osdu:frequencyBandID rdf:type owl:DatatypeProperty ;
	rdfs:comment "Image frequency band or resolution. For example: C / X / L / P. This is related to the wavelength. (See data.WavelengthID.) " ;
	rdfs:domain osdu:ProcessedInSAR ;
	xsd:pattern "^[\\\\w\\\\-\\\\.]+:reference-data\\\\-\\\\-InSARFrequencyBand:[\\\\w\\\\-\\\\.\\\\:\\\\%]+:[0-9]*$" ;
	rdfs:range xsd:string ;
.

###  https://w3id.org/osdu#frequencyMx
osdu:frequencyMx rdf:type owl:DatatypeProperty ;
	rdfs:comment "Maximum allowable depth frequency for survey stations for this survey run. " ;
	rdfs:domain osdu:SurveySection ;
	rdfs:range xsd:decimal ;
.

###  https://w3id.org/osdu#frictionFactor
osdu:frictionFactor rdf:type owl:DatatypeProperty ;
	rdfs:comment "Friction Factor " ;
	rdfs:domain osdu:PerforationInterval ;
	rdfs:range xsd:decimal ;
.

###  https://w3id.org/osdu#frictionPressure
osdu:frictionPressure rdf:type owl:DatatypeProperty ;
	rdfs:comment "Friction Pressure " ;
	rdfs:domain osdu:PerforationInterval ;
	rdfs:range xsd:decimal ;
.

###  https://w3id.org/osdu#fullOSDUImplementationIndicator
osdu:fullOSDUImplementationIndicator rdf:type owl:DatatypeProperty ;
	rdfs:comment "Flag that determines whether the external source has a full OSDU implementation (true) or a wrapper facade over proprietary APIs (false) " ;
	rdfs:domain osdu:ConnectedSourceRegistryEntry ;
	rdfs:range xsd:boolean ;
.

###  https://w3id.org/osdu#fundsAmount
osdu:fundsAmount rdf:type owl:DatatypeProperty ;
	rdfs:comment "The level of expenditure approved. " ;
	rdfs:domain osdu:FundsAuthorizations ;
	rdfs:range xsd:decimal ;
.

###  https://w3id.org/osdu#gasFoamType
osdu:gasFoamType rdf:type owl:DatatypeProperty ;
	rdfs:comment "Gas type used for foam job. " ;
	rdfs:domain osdu:CementingFluid ;
	rdfs:range xsd:string ;
.

###  https://w3id.org/osdu#gasFoamVol
osdu:gasFoamVol rdf:type owl:DatatypeProperty ;
	rdfs:comment "Volume of gas used for foam job. " ;
	rdfs:domain osdu:CementingFluid ;
	rdfs:range xsd:decimal ;
.

###  https://w3id.org/osdu#gasReadingMeasureDepthTop
osdu:gasReadingMeasureDepthTop rdf:type owl:DatatypeProperty ;
	rdfs:comment "Top measured depth for which the gas reading was conducted " ;
	rdfs:domain osdu:GasReading ;
	rdfs:range xsd:decimal ;
.

###  https://w3id.org/osdu#gasReadingTvdBase
osdu:gasReadingTvdBase rdf:type owl:DatatypeProperty ;
	rdfs:comment "Bottom true vertical depth interval over which the gas reading was conducted. " ;
	rdfs:domain osdu:GasReading ;
	rdfs:range xsd:decimal ;
.

###  https://w3id.org/osdu#gatherTypeID
osdu:gatherTypeID rdf:type owl:DatatypeProperty ;
	rdfs:comment "Pre-stack: the type of gathers in this dataset. " ;
	rdfs:domain osdu:SeismicTraceData ;
	xsd:pattern "^[\\\\w\\\\-\\\\.]+:reference-data\\\\-\\\\-SeismicGatherType:[\\\\w\\\\-\\\\.\\\\:\\\\%]+:[0-9]*$" ;
	rdfs:range xsd:string ;
.

###  https://w3id.org/osdu#gaugeMD
osdu:gaugeMD rdf:type owl:DatatypeProperty ;
	rdfs:comment "Depth of gauge(s) run while perforating. " ;
	rdfs:domain osdu:PerforationInterval ;
	rdfs:range xsd:decimal ;
.

###  https://w3id.org/osdu#gaugeType
osdu:gaugeType rdf:type owl:DatatypeProperty ;
	rdfs:comment "Free text to describe the type of gauge used for the pressure measurement " ;
	rdfs:domain osdu:PPFGDataset ;
	rdfs:range xsd:string ;
.

###  https://w3id.org/osdu#gel0Sec
osdu:gel0Sec rdf:type owl:DatatypeProperty ;
	rdfs:comment "Zero-second gels. " ;
	rdfs:domain osdu:Fluid ;
	rdfs:range xsd:decimal ;
.

###  https://w3id.org/osdu#gel10Min
osdu:gel10Min rdf:type owl:DatatypeProperty ;
	rdfs:comment "Ten-minute gels. " ;
	rdfs:domain [
		rdf:type owl:Class ;
		owl:unionOf (
			osdu:Fluid
			osdu:CementStage
		) ;
	] ;
	rdfs:range xsd:decimal ;
.

###  https://w3id.org/osdu#gel10MinReading
osdu:gel10MinReading rdf:type owl:DatatypeProperty ;
	rdfs:comment "Gel reading after 10 minutes. " ;
	rdfs:domain osdu:CementingFluid ;
	rdfs:range xsd:decimal ;
.

###  https://w3id.org/osdu#gel10MinStrength
osdu:gel10MinStrength rdf:type owl:DatatypeProperty ;
	rdfs:comment "Gel strength after 10 minutes. " ;
	rdfs:domain osdu:CementingFluid ;
	rdfs:range xsd:decimal ;
.

###  https://w3id.org/osdu#gel10Sec
osdu:gel10Sec rdf:type owl:DatatypeProperty ;
	rdfs:comment "Ten-second gels. " ;
	rdfs:domain [
		rdf:type owl:Class ;
		owl:unionOf (
			osdu:Fluid
			osdu:CementStage
		) ;
	] ;
	rdfs:range xsd:decimal ;
.

###  https://w3id.org/osdu#gel10SecReading
osdu:gel10SecReading rdf:type owl:DatatypeProperty ;
	rdfs:comment "Gel reading after 10 seconds. " ;
	rdfs:domain osdu:CementingFluid ;
	rdfs:range xsd:decimal ;
.

###  https://w3id.org/osdu#gel10SecStrength
osdu:gel10SecStrength rdf:type owl:DatatypeProperty ;
	rdfs:comment "Gel strength after 10 seconds. " ;
	rdfs:domain osdu:CementingFluid ;
	rdfs:range xsd:decimal ;
.

###  https://w3id.org/osdu#gel1MinReading
osdu:gel1MinReading rdf:type owl:DatatypeProperty ;
	rdfs:comment "Gel reading after 1 minute. " ;
	rdfs:domain osdu:CementingFluid ;
	rdfs:range xsd:decimal ;
.

###  https://w3id.org/osdu#gel1MinStrength
osdu:gel1MinStrength rdf:type owl:DatatypeProperty ;
	rdfs:comment "Gel strength after 1 minute. " ;
	rdfs:domain osdu:CementingFluid ;
	rdfs:range xsd:decimal ;
.

###  https://w3id.org/osdu#gel30Min
osdu:gel30Min rdf:type owl:DatatypeProperty ;
	rdfs:comment "Thirty-minute gels. " ;
	rdfs:domain osdu:Fluid ;
	rdfs:range xsd:decimal ;
.

###  https://w3id.org/osdu#genericRepresentationIDs
osdu:genericRepresentationIDs rdf:type owl:DatatypeProperty ;
	rdfs:comment "List of Generic Representations linked to structural model inputs and outputs, for example fault sticks and triangulated surfaces, Horizon data points and triangulated surfaces, geobody boundary triangulated surfaces. " ;
	rdfs:domain [
		rdf:type owl:Class ;
		owl:unionOf (
			osdu:SealedSurfaceFramework
			osdu:UnsealedSurfaceFramework
		) ;
	] ;
	xsd:pattern "^[\\\\w\\\\-\\\\.]+:work-product-component\\\\-\\\\-GenericRepresentation:[\\\\w\\\\-\\\\.\\\\:\\\\%]+:[0-9]*$" ;
	rdfs:range xsd:string ;
.

###  https://w3id.org/osdu#geoPoliticalEntityID
osdu:geoPoliticalEntityID rdf:type owl:DatatypeProperty ;
	rdfs:comment "ID of a GeoPoliticalEntity. " ;
	rdfs:domain [
		rdf:type owl:Class ;
		owl:unionOf (
			osdu:AbstractGeoPoliticalContext
			osdu:GeoPoliticalEntity
		) ;
	] ;
	xsd:pattern "^[\\\\w\\\\-\\\\.]+:master-data\\\\-\\\\-GeoPoliticalEntity:[\\\\w\\\\-\\\\.\\\\:\\\\%]+:[0-9]*$" ;
	rdfs:range xsd:string ;
.

###  https://w3id.org/osdu#geoPoliticalEntityName
osdu:geoPoliticalEntityName rdf:type owl:DatatypeProperty ;
	rdfs:comment "Name of the geopolitical entity. " ;
	rdfs:domain osdu:GeoPoliticalEntity ;
	rdfs:range xsd:string ;
.

###  https://w3id.org/osdu#geoPoliticalEntityTypeID
osdu:geoPoliticalEntityTypeID rdf:type owl:DatatypeProperty ;
	rdfs:comment "Type of geopolitical entity. " ;
	rdfs:domain osdu:GeoPoliticalEntity ;
	xsd:pattern "^[\\\\w\\\\-\\\\.]+:reference-data\\\\-\\\\-GeoPoliticalEntityType:[\\\\w\\\\-\\\\.\\\\:\\\\%]+:[0-9]*$" ;
	rdfs:range xsd:string ;
.

###  https://w3id.org/osdu#geoTypeID
osdu:geoTypeID rdf:type owl:DatatypeProperty ;
	rdfs:comment "The fixed geographical type for this object. " ;
	rdfs:domain [
		rdf:type owl:Class ;
		owl:unionOf (
			osdu:AbstractGeoPlayContext
			osdu:AbstractGeoFieldContext
			osdu:AbstractGeoBasinContext
			osdu:AbstractGeoProspectContext
			osdu:AbstractGeoPoliticalContext
		) ;
	] ;
	xsd:pattern "^[\\\\w\\\\-\\\\.]+:reference-data\\\\-\\\\-PlayType:[\\\\w\\\\-\\\\.\\\\:\\\\%]+:[0-9]*$" ;
	xsd:pattern "^[\\\\w\\\\-\\\\.]+:reference-data\\\\-\\\\-BasinType:[\\\\w\\\\-\\\\.\\\\:\\\\%]+:[0-9]*$" ;
	xsd:pattern "^[\\\\w\\\\-\\\\.]+:reference-data\\\\-\\\\-ProspectType:[\\\\w\\\\-\\\\.\\\\:\\\\%]+:[0-9]*$" ;
	xsd:pattern "^[\\\\w\\\\-\\\\.]+:reference-data\\\\-\\\\-GeoPoliticalEntityType:[\\\\w\\\\-\\\\.\\\\:\\\\%]+:[0-9]*$" ;
	rdfs:range xsd:string ;
.

###  https://w3id.org/osdu#geobodyBoundaryInterpretationIDs
osdu:geobodyBoundaryInterpretationIDs rdf:type owl:DatatypeProperty ;
	rdfs:comment "Lists the geobody interpretation IDs belonging to the structural model " ;
	rdfs:domain osdu:StructuralOrganizationInterpretation ;
	xsd:pattern "^[\\\\w\\\\-\\\\.]+:work-product-component\\\\-\\\\-GeobodyBoundaryInterpretation:[\\\\w\\\\-\\\\.\\\\:\\\\%]+:[0-9]*$" ;
	rdfs:range xsd:string ;
.

###  https://w3id.org/osdu#geographicCRSID
osdu:geographicCRSID rdf:type owl:DatatypeProperty ;
	rdfs:comment "Coordinate Reference System defining the Geodetic Datum of the station LATITUDE and LONGITUDE values. If LATITUDE and LONGITUDE attributes are stored, clearly identifying their Datum is required. " ;
	rdfs:domain osdu:WellboreTrajectory ;
	xsd:pattern "^[\\\\w\\\\-\\\\.]+:reference-data\\\\-\\\\-CoordinateReferenceSystem:[\\\\w\\\\-\\\\.\\\\:\\\\%]+:[0-9]*$" ;
	rdfs:range xsd:string ;
.

###  https://w3id.org/osdu#geologicTimeValues
osdu:geologicTimeValues rdf:type owl:DatatypeProperty ;
	rdfs:comment "Array of geologic time values in Year (annums). This value must be positive if it represents a Geological Event in the past. Must be negative if it represents a geological event in the future. " ;
	rdfs:domain osdu:TimeSeries ;
	rdfs:range xsd:decimal ;
.

###  https://w3id.org/osdu#geologicUnitID
osdu:geologicUnitID rdf:type owl:DatatypeProperty ;
	rdfs:comment "The stratigraphic or the geobody associated to this Reservoir compartment unit. " ;
	rdfs:domain osdu:ReservoirCompartmentUnit ;
	xsd:pattern "^[\\\\w\\\\-\\\\.]+:(work-product-component\\\\-\\\\-GeobodyInterpretation|work-product-component\\\\-\\\\-StratigraphicUnitInterpretation):[\\\\w\\\\-\\\\.\\\\:\\\\%]+:[0-9]*$" ;
	rdfs:range xsd:string ;
.

###  https://w3id.org/osdu#geologicUnitInterpretationIDs
osdu:geologicUnitInterpretationIDs rdf:type owl:DatatypeProperty ;
	rdfs:comment "An array of StratigraphicUnitInterpretation, GeobodyInterpretation or RockFluidUnitInterpretation record Ids associated to this interval. " ;
	rdfs:domain [
		rdf:type owl:Class ;
		owl:unionOf (
			osdu:GeologicUnitOccurrenceInterpretation
			osdu:Interval
		) ;
	] ;
	xsd:pattern "^[\\\\w\\\\-\\\\.]+:(work-product-component\\\\-\\\\-RockFluidUnitInterpretation|work-product-component\\\\-\\\\-StratigraphicUnitInterpretation):[\\\\w\\\\-\\\\.\\\\:\\\\%]+:[0-9]*$" ;
	xsd:pattern "^[\\\\w\\\\-\\\\.]+:(work-product-component\\\\-\\\\-StratigraphicUnitInterpretation|work-product-component\\\\-\\\\-GeobodyInterpretation|work-product-component\\\\-\\\\-RockFluidUnitInterpretation):[\\\\w\\\\-\\\\.\\\\:\\\\%]+:[0-9]*$" ;
	rdfs:range xsd:string ;
.

###  https://w3id.org/osdu#geologicUnitOccurrenceInterpretationIDs
osdu:geologicUnitOccurrenceInterpretationIDs rdf:type owl:DatatypeProperty ;
	rdfs:comment "References to Geologic Unit Occurrence Interpretations belonging to this model. " ;
	rdfs:domain osdu:EarthModelInterpretation ;
	xsd:pattern "^[\\\\w\\\\-\\\\.]+:work-product-component\\\\-\\\\-GeologicUnitOccurrenceInterpretation:[\\\\w\\\\-\\\\.\\\\:\\\\%]+:[0-9]*$" ;
	rdfs:range xsd:string ;
.

###  https://w3id.org/osdu#geologicUnitOrganizationInterpretationIDs
osdu:geologicUnitOrganizationInterpretationIDs rdf:type owl:DatatypeProperty ;
	rdfs:comment "Reference to the GeologicUnitOrganizationInterpretations associated to this voidage group. " ;
	rdfs:domain osdu:VoidageGroupInterpretation ;
	xsd:pattern "^[\\\\w\\\\-\\\\.]+:work-product-component\\\\-\\\\-StratigraphicColumnRankInterpretation:[\\\\w\\\\-\\\\.\\\\:\\\\%]+:[0-9]*$" ;
	rdfs:range xsd:string ;
.

###  https://w3id.org/osdu#geologicUnitShapeTypeID
osdu:geologicUnitShapeTypeID rdf:type owl:DatatypeProperty ;
	rdfs:comment "The relationship to a GeologicUnitShapeType like sheet, dyke, dome, mushroom, channel and more. " ;
	rdfs:domain osdu:AbstractGeologicUnitInterpretation ;
	xsd:pattern "^[\\\\w\\\\-\\\\.]+:reference-data\\\\-\\\\-GeologicUnitShapeType:[\\\\w\\\\-\\\\.\\\\:\\\\%]+:[0-9]*$" ;
	rdfs:range xsd:string ;
.

###  https://w3id.org/osdu#geologicalAge
osdu:geologicalAge rdf:type owl:DatatypeProperty ;
	rdfs:comment "Associated geological age " ;
	rdfs:domain osdu:Markers ;
	rdfs:range xsd:string ;
.

###  https://w3id.org/osdu#geologicalUnitAgePeriod
osdu:geologicalUnitAgePeriod rdf:type owl:DatatypeProperty ;
	rdfs:comment "Age period of geologic unit (geochronological name of stage, etc.) " ;
	rdfs:domain osdu:SeismicHorizon ;
	rdfs:range xsd:string ;
.

###  https://w3id.org/osdu#geologicalUnitAgeYear
osdu:geologicalUnitAgeYear rdf:type owl:DatatypeProperty ;
	rdfs:comment "Age of Geologic unit (geochronological).  Number expected but is a string type to be consistent with wellbore marker. " ;
	rdfs:domain osdu:SeismicHorizon ;
	rdfs:range xsd:string ;
.

###  https://w3id.org/osdu#geologicalUnitName
osdu:geologicalUnitName rdf:type owl:DatatypeProperty ;
	rdfs:comment "Geological Unit (formation, bioevent, etc.) Name " ;
	rdfs:domain osdu:SeismicHorizon ;
	rdfs:range xsd:string ;
.

###  https://w3id.org/osdu#geologist
osdu:geologist rdf:type owl:DatatypeProperty ;
	rdfs:comment "Name of operator's wellsite geologist. " ;
	rdfs:domain osdu:DrillingReportStatusInfo ;
	rdfs:range xsd:string ;
.

###  https://w3id.org/osdu#governanceAuthorities
osdu:governanceAuthorities rdf:type owl:DatatypeProperty ;
	rdfs:comment "The Authorities governing the contents. " ;
	rdfs:domain osdu:Type ;
	rdfs:range xsd:string ;
.

###  https://w3id.org/osdu#governanceModel
osdu:governanceModel rdf:type owl:DatatypeProperty ;
	rdfs:comment "The style of governance (only relevant for IsReferenceValueType==true) - it can be FIXED (content must not be augmented), OPEN (additions and changes allowed) or LOCAL (content is exclusively governed by operator). " ;
	rdfs:domain osdu:Type ;
	rdfs:range xsd:string ;
.

###  https://w3id.org/osdu#grainDensity
osdu:grainDensity rdf:type owl:DatatypeProperty ;
	rdfs:comment "Th measured grain density " ;
	rdfs:domain osdu:RoutineCoreAnalysis ;
	rdfs:range xsd:decimal ;
.

###  https://w3id.org/osdu#grainDensityMeasurementTypeID
osdu:grainDensityMeasurementTypeID rdf:type owl:DatatypeProperty ;
	rdfs:comment "The measurement type used to obtain the GrainDensity value. " ;
	rdfs:domain osdu:RoutineCoreAnalysis ;
	xsd:pattern "^[\\\\w\\\\-\\\\.]+:reference-data\\\\-\\\\-GrainDensityMeasurementType:[\\\\w\\\\-\\\\.\\\\:\\\\%]+:[0-9]*$" ;
	rdfs:range xsd:string ;
.

###  https://w3id.org/osdu#gridID
osdu:gridID rdf:type owl:DatatypeProperty ;
	rdfs:comment "The grid which is in connection " ;
	rdfs:domain osdu:AbstractIjkGridFlowSimulationBoundaryConnection ;
	xsd:pattern "^[\\\\w\\\\-\\\\.]+:work-product-component\\\\-\\\\-IjkGridRepresentation:[\\\\w\\\\-\\\\.\\\\:\\\\%]+:[0-9]*$" ;
	rdfs:range xsd:string ;
.

###  https://w3id.org/osdu#gridRepresentationIDs
osdu:gridRepresentationIDs rdf:type owl:DatatypeProperty ;
	rdfs:comment "References to the grid representations which the connections are based on. " ;
	rdfs:domain osdu:GridConnectionSetRepresentation ;
	xsd:pattern "^[\\\\w\\\\-\\\\.]+:(work-product-component\\\\-\\\\-GpGridRepresentation|work-product-component\\\\-\\\\-IjkGridRepresentation|work-product-component\\\\-\\\\-UnstructuredColumnLayerGridRepresentation|work-product-component\\\\-\\\\-UnstructuredGridRepresentation):[\\\\w\\\\-\\\\.\\\\:\\\\%]+:[0-9]*$" ;
	rdfs:range xsd:string ;
.

###  https://w3id.org/osdu#groundResolution
osdu:groundResolution rdf:type owl:DatatypeProperty ;
	rdfs:comment "Horizontal resolution of the image. For example 1 metre or 10 meters " ;
	rdfs:domain osdu:ProcessedInSAR ;
	rdfs:range xsd:decimal ;
.

###  https://w3id.org/osdu#gunCarrierCategoryTypeID
osdu:gunCarrierCategoryTypeID rdf:type owl:DatatypeProperty ;
	rdfs:comment "Gun Carrier Category " ;
	rdfs:domain osdu:PerforationInterval ;
	xsd:pattern "^[\\\\w\\\\-\\\\.]+:reference-data\\\\-\\\\-PerforationGunCarrierCategory:[\\\\w\\\\-\\\\.\\\\:\\\\%]+:[0-9]*$" ;
	rdfs:range xsd:string ;
.

###  https://w3id.org/osdu#gunCarrierManufacturerID
osdu:gunCarrierManufacturerID rdf:type owl:DatatypeProperty ;
	rdfs:comment "Gun Carrier Manufacturer " ;
	rdfs:domain osdu:PerforationInterval ;
	xsd:pattern "^[\\\\w\\\\-\\\\.]+:master-data\\\\-\\\\-Organisation:[\\\\w\\\\-\\\\.\\\\:\\\\%]+:[0-9]*$" ;
	rdfs:range xsd:string ;
.

###  https://w3id.org/osdu#gunCarrierModelID
osdu:gunCarrierModelID rdf:type owl:DatatypeProperty ;
	rdfs:comment "Gun Carrier Model " ;
	rdfs:domain osdu:PerforationInterval ;
	xsd:pattern "^[\\\\w\\\\-\\\\.]+:reference-data\\\\-\\\\-PerforationGunCarrierModel:[\\\\w\\\\-\\\\.\\\\:\\\\%]+:[0-9]*$" ;
	rdfs:range xsd:string ;
.

###  https://w3id.org/osdu#gunCarrierPhasing
osdu:gunCarrierPhasing rdf:type owl:DatatypeProperty ;
	rdfs:comment "Gun Carrier Phasing (angle between perfs). Implemented via a reference list in order to standardize the values. " ;
	rdfs:domain osdu:PerforationInterval ;
	xsd:pattern "^[\\\\w\\\\-\\\\.]+:reference-data\\\\-\\\\-PerforationGunPhasingType:[\\\\w\\\\-\\\\.\\\\:\\\\%]+:[0-9]*$" ;
	rdfs:range xsd:string ;
.

###  https://w3id.org/osdu#gunCarrierTypeID
osdu:gunCarrierTypeID rdf:type owl:DatatypeProperty ;
	rdfs:comment "Gun Carrier Type " ;
	rdfs:domain osdu:PerforationInterval ;
	xsd:pattern "^[\\\\w\\\\-\\\\.]+:reference-data\\\\-\\\\-PerforationGunCarrierType:[\\\\w\\\\-\\\\.\\\\:\\\\%]+:[0-9]*$" ;
	rdfs:range xsd:string ;
.

###  https://w3id.org/osdu#gunDiameter
osdu:gunDiameter rdf:type owl:DatatypeProperty ;
	rdfs:comment "Gun diameter " ;
	rdfs:domain osdu:PerforationInterval ;
	rdfs:range xsd:decimal ;
.

###  https://w3id.org/osdu#gunFiringHeadTypeID
osdu:gunFiringHeadTypeID rdf:type owl:DatatypeProperty ;
	rdfs:comment "Gun Firing Head Type " ;
	rdfs:domain osdu:PerforationInterval ;
	xsd:pattern "^[\\\\w\\\\-\\\\.]+:reference-data\\\\-\\\\-PerforationGunFiringHeadType:[\\\\w\\\\-\\\\.\\\\:\\\\%]+:[0-9]*$" ;
	rdfs:range xsd:string ;
.

###  https://w3id.org/osdu#gunMetallurgyTypeID
osdu:gunMetallurgyTypeID rdf:type owl:DatatypeProperty ;
	rdfs:comment "Metallurgy of the gun " ;
	rdfs:domain osdu:PerforationInterval ;
	xsd:pattern "^[\\\\w\\\\-\\\\.]+:reference-data\\\\-\\\\-PerforationGunMetallurgyType:[\\\\w\\\\-\\\\.\\\\:\\\\%]+:[0-9]*$" ;
	rdfs:range xsd:string ;
.

###  https://w3id.org/osdu#gunSwellDiameter
osdu:gunSwellDiameter rdf:type owl:DatatypeProperty ;
	rdfs:comment "Gun Swell Diameter " ;
	rdfs:domain osdu:PerforationInterval ;
	rdfs:range xsd:decimal ;
.

###  https://w3id.org/osdu#handler
osdu:handler rdf:type owl:DatatypeProperty ;
	rdfs:comment "Allows creation of a specific handler DAG for the source type " ;
	rdfs:domain osdu:Workflow ;
	rdfs:range xsd:string ;
.

###  https://w3id.org/osdu#hardnessCa
osdu:hardnessCa rdf:type owl:DatatypeProperty ;
	rdfs:comment "Total calcium hardness. " ;
	rdfs:domain osdu:Fluid ;
	rdfs:range xsd:decimal ;
.

###  https://w3id.org/osdu#hasCMPIncreaseByOne
osdu:hasCMPIncreaseByOne rdf:type owl:DatatypeProperty ;
	rdfs:comment "Indicates that CMP numbering increases regularly by 1. " ;
	rdfs:domain osdu:SeismicLineGeometry ;
	rdfs:range xsd:boolean ;
.

###  https://w3id.org/osdu#hasCollocatedNodeInKDirection
osdu:hasCollocatedNodeInKDirection rdf:type owl:DatatypeProperty ;
	rdfs:comment "Indicate if at least two adjacent nodes in K Direction are collocated. Also known as pinched node. Usually occur in erosional context. " ;
	rdfs:domain osdu:AbstractColumnLayerGridPatch ;
	rdfs:range xsd:boolean ;
.

###  https://w3id.org/osdu#hasFiniteElementSubnodes
osdu:hasFiniteElementSubnodes rdf:type owl:DatatypeProperty ;
	rdfs:comment "Indicate if the grid has got some finite element subnodes for defining higher order grid geometry and properties. This is mainly used in geomechanical context. " ;
	rdfs:domain osdu:AbstractGridRepresentation ;
	rdfs:range xsd:boolean ;
.

###  https://w3id.org/osdu#hasKGaps
osdu:hasKGaps rdf:type owl:DatatypeProperty ;
	rdfs:comment "Indicate that it exists at least one gap in the whole K direction of the grid. A gap is really a hole, it is not a layer of dead cells. " ;
	rdfs:domain osdu:AbstractColumnLayerGridPatch ;
	rdfs:range xsd:boolean ;
.

###  https://w3id.org/osdu#hasLateralGaps
osdu:hasLateralGaps rdf:type owl:DatatypeProperty ;
	rdfs:comment "Indicate that it exists at least one gap in the lateral direction of the grid. A gap is really a hole, it is not a slice of dead cells. " ;
	rdfs:domain osdu:AbstractColumnLayerGridPatch ;
	rdfs:range xsd:boolean ;
.

###  https://w3id.org/osdu#hasLeakOffOccurred
osdu:hasLeakOffOccurred rdf:type owl:DatatypeProperty ;
	rdfs:comment "Indicates if a leak off has occurred during the test " ;
	rdfs:domain osdu:FormationIntegrityEvaluation ;
	rdfs:range xsd:boolean ;
.

###  https://w3id.org/osdu#hasMonotonicLabelling
osdu:hasMonotonicLabelling rdf:type owl:DatatypeProperty ;
	rdfs:comment "Indicates that the station label (SP name) changes monotonically with respect to CMP. " ;
	rdfs:domain osdu:SeismicLineGeometry ;
	rdfs:range xsd:boolean ;
.

###  https://w3id.org/osdu#hasNaNGeometry
osdu:hasNaNGeometry rdf:type owl:DatatypeProperty ;
	rdfs:comment "Indicate that at least on coordinate of one node of the grid is NaN. It is different than a dead cell which may have a geometry while it is disabled. " ;
	rdfs:domain osdu:AbstractGridRepresentation ;
	rdfs:range xsd:boolean ;
.

###  https://w3id.org/osdu#hasNoGeometry
osdu:hasNoGeometry rdf:type owl:DatatypeProperty ;
	rdfs:comment "Indicate that the grid has no geometry. It is common when one wants a grid only as a collection of cell connections (i.e. pipe network). " ;
	rdfs:domain osdu:AbstractGridRepresentation ;
	rdfs:range xsd:boolean ;
.

###  https://w3id.org/osdu#hasParametricGeometry
osdu:hasParametricGeometry rdf:type owl:DatatypeProperty ;
	rdfs:comment "Indicate that the nodes of the grid are given by means of a parameter along the pillar. Otherwise nodes of the grid are explicitly given by means of an XYZ triplet. " ;
	rdfs:domain osdu:AbstractColumnLayerGridPatch ;
	rdfs:range xsd:boolean ;
.

###  https://w3id.org/osdu#hasSplitNode
osdu:hasSplitNode rdf:type owl:DatatypeProperty ;
	rdfs:comment "Indicate that the grid contains some split nodes i.e some node which are not on a pillar. " ;
	rdfs:domain osdu:AbstractColumnLayerGridPatch ;
	rdfs:range xsd:boolean ;
.

###  https://w3id.org/osdu#hasTrippingSchedule
osdu:hasTrippingSchedule rdf:type owl:DatatypeProperty ;
	rdfs:comment "Flag indicating whether a detailed tripping schedule is available. Available tripping schedules are usually a sign of controlled coring sample quality. " ;
	rdfs:domain osdu:Coring ;
	rdfs:range xsd:boolean ;
.

###  https://w3id.org/osdu#hasTruncations
osdu:hasTruncations rdf:type owl:DatatypeProperty ;
	rdfs:comment "Indicate that some of the pillars of the grid are truncated (Fault contact in Y shape for example) " ;
	rdfs:domain osdu:AbstractColumnLayerGridPatch ;
	rdfs:range xsd:boolean ;
.

###  https://w3id.org/osdu#headCount
osdu:headCount rdf:type owl:DatatypeProperty ;
	rdfs:comment "Number of people on board for that company. " ;
	rdfs:domain osdu:Personnel ;
	rdfs:range xsd:decimal ;
.

###  https://w3id.org/osdu#height
osdu:height rdf:type owl:DatatypeProperty ;
	rdfs:comment "The height above the reference surface defined by the VerticalCoordinateReferenceSystemID positive upwards. " ;
	rdfs:domain osdu:AbstractReferenceLevel ;
	rdfs:range xsd:decimal ;
.

###  https://w3id.org/osdu#holeDepthEnd
osdu:holeDepthEnd rdf:type owl:DatatypeProperty ;
	rdfs:comment "The depth of the hole at the end of the activity. Depth relative to Planned wellbore ZDP. Navigate via WellboreID to the side-car WellPlanningWellbore, which holds the depth reference in data.VerticalMeasurement. " ;
	rdfs:domain osdu:DepthRange ;
	rdfs:range xsd:decimal ;
.

###  https://w3id.org/osdu#holeDepthStart
osdu:holeDepthStart rdf:type owl:DatatypeProperty ;
	rdfs:comment "The depth of the hole at the start of the activity. Depth relative to Planned wellbore ZDP. Navigate via WellboreID to the side-car WellPlanningWellbore, which holds the depth reference in data.VerticalMeasurement. " ;
	rdfs:domain osdu:DepthRange ;
	rdfs:range xsd:decimal ;
.

###  https://w3id.org/osdu#holeDiameter
osdu:holeDiameter rdf:type owl:DatatypeProperty ;
	rdfs:comment "Diameter of the hole " ;
	rdfs:domain osdu:BHARun ;
	rdfs:range xsd:decimal ;
.

###  https://w3id.org/osdu#holeSectionID
osdu:holeSectionID rdf:type owl:DatatypeProperty ;
	rdfs:comment "Description of the Hole Section to which this object relates " ;
	rdfs:domain [
		rdf:type owl:Class ;
		owl:unionOf (
			osdu:FluidsInterval
			osdu:WellPlanningWellbore
			osdu:DSTRun
			osdu:CasingDesign
			osdu:BHARun
		) ;
	] ;
	xsd:pattern "^[\\\\w\\\\-\\\\.]+:master-data\\\\-\\\\-HoleSection:[\\\\w\\\\-\\\\.\\\\:\\\\%]+:[0-9]*$" ;
	rdfs:range xsd:string ;
.

###  https://w3id.org/osdu#holeSectionIDs
osdu:holeSectionIDs rdf:type owl:DatatypeProperty ;
	rdfs:comment "Description of the Hole Sections for this architecture " ;
	rdfs:domain osdu:WellboreArchitecture ;
	xsd:pattern "^[\\\\w\\\\-\\\\.]+:master-data\\\\-\\\\-HoleSection:[\\\\w\\\\-\\\\.\\\\:\\\\%]+:[0-9]*$" ;
	rdfs:range xsd:string ;
.

###  https://w3id.org/osdu#holeSectionId
osdu:holeSectionId rdf:type owl:DatatypeProperty ;
	rdfs:comment "Identifier of the Hole Section that is being drilled " ;
	rdfs:domain osdu:RigUtilization ;
	xsd:pattern "^[\\\\w\\\\-\\\\.]+:master-data\\\\-\\\\-HoleSection:[\\\\w\\\\-\\\\.\\\\:\\\\%]+:[0-9]*$" ;
	rdfs:range xsd:string ;
.

###  https://w3id.org/osdu#holeType
osdu:holeType rdf:type owl:DatatypeProperty ;
	rdfs:comment "Free text describing the type of the hole the DST is running through (such as Cased, OpenHole,…) " ;
	rdfs:domain osdu:DSTRun ;
	rdfs:range xsd:string ;
.

###  https://w3id.org/osdu#holeTypeLogging
osdu:holeTypeLogging rdf:type owl:DatatypeProperty ;
	rdfs:comment "Description of the hole related type of logging - POSSIBLE VALUE : OpenHole / CasedHole / CementedHole " ;
	rdfs:domain osdu:WellLog ;
	xsd:pattern "^OPENHOLE|CASEDHOLE|CEMENTEDHOLE$" ;
	rdfs:range xsd:string ;
.

###  https://w3id.org/osdu#homogeneousMemberKind
osdu:homogeneousMemberKind rdf:type owl:DatatypeProperty ;
	rdfs:comment "If the Collection is homogeneous, this indicates the single data schema Kind within the collection (without the semantic version number). If the collection is heterogeneous (collecting multiple data types) leave this property empty. " ;
	rdfs:domain osdu:PersistedCollection ;
	rdfs:range xsd:string ;
.

###  https://w3id.org/osdu#hookloadDown
osdu:hookloadDown rdf:type owl:DatatypeProperty ;
	rdfs:comment "Hookload when the string is moving down. " ;
	rdfs:domain osdu:DrillingParameters ;
	rdfs:range xsd:decimal ;
.

###  https://w3id.org/osdu#hookloadUp
osdu:hookloadUp rdf:type owl:DatatypeProperty ;
	rdfs:comment "Hookload when the string is moving up. " ;
	rdfs:domain osdu:DrillingParameters ;
	rdfs:range xsd:decimal ;
.

###  https://w3id.org/osdu#horizonInterpretationIDs
osdu:horizonInterpretationIDs rdf:type owl:DatatypeProperty ;
	rdfs:comment "Lists the horizon interpretation IDs belonging to the structural model " ;
	rdfs:domain osdu:StructuralOrganizationInterpretation ;
	xsd:pattern "^[\\\\w\\\\-\\\\.]+:work-product-component\\\\-\\\\-HorizonInterpretation:[\\\\w\\\\-\\\\.\\\\:\\\\%]+:[0-9]*$" ;
	rdfs:range xsd:string ;
.

###  https://w3id.org/osdu#horizontalAxisUnitID
osdu:horizontalAxisUnitID rdf:type owl:DatatypeProperty ;
	rdfs:comment "The horizontal unit for 2-dimensional or 3-dimensional coordinate systems. This property is not populated for 1-dimensional coordinate systems (Vertical CRSs). " ;
	rdfs:domain osdu:CoordinateSystem ;
	xsd:pattern "^[\\\\w\\\\-\\\\.]+:reference-data\\\\-\\\\-UnitOfMeasure:[\\\\w\\\\-\\\\.\\\\:\\\\%]+:[0-9]*$" ;
	rdfs:range xsd:string ;
.

###  https://w3id.org/osdu#horizontalCRSID
osdu:horizontalCRSID rdf:type owl:DatatypeProperty ;
	rdfs:comment "The ID of the HorizontalCrs. " ;
	rdfs:domain [
		rdf:type owl:Class ;
		owl:unionOf (
			osdu:VelocityModeling
			osdu:SeismicTraceData
			osdu:FaultSystem
			osdu:SeismicLineGeometry
			osdu:HorizontalCRS
		) ;
	] ;
	xsd:pattern "^[\\\\w\\\\-\\\\.]+:reference-data\\\\-\\\\-CoordinateReferenceSystem:[\\\\w\\\\-\\\\.\\\\:\\\\%]+:[0-9]*$" ;
	rdfs:range xsd:string ;
.

###  https://w3id.org/osdu#hydrostaticReservoirPressureDifference
osdu:hydrostaticReservoirPressureDifference rdf:type owl:DatatypeProperty ;
	rdfs:comment "Difference between Reservoir Pressure and Hydrostatic pressure. Negative number indicates underbalanced " ;
	rdfs:domain osdu:PerforationJob ;
	rdfs:range xsd:decimal ;
.

###  https://w3id.org/osdu#i
osdu:i rdf:type owl:DatatypeProperty ;
	rdfs:comment "I index of the cell " ;
	rdfs:domain osdu:SingleCellAquifer ;
	rdfs:range xsd:integer ;
.

###  https://w3id.org/osdu#iadcCode
osdu:iadcCode rdf:type owl:DatatypeProperty ;
	rdfs:comment "IADC bit code. " ;
	rdfs:domain osdu:BitRecord ;
	rdfs:range xsd:string ;
.

###  https://w3id.org/osdu#id
osdu:id rdf:type owl:DatatypeProperty ;
	rdfs:comment "The object reference identifying the DIRECT, INDIRECT, REFERENCE dependency. " ;
	rdfs:domain [
		rdf:type owl:Class ;
		owl:unionOf (
			osdu:LineageAssertion
			osdu:AbstractReferenceType
			osdu:System
		) ;
	] ;
	xsd:pattern "^[\\\\w\\\\-\\\\.]+:[\\\\w\\\\-\\\\.]+:[\\\\w\\\\-\\\\.\\\\:\\\\%]+:[0-9]*$" ;
	rdfs:range xsd:string ;
.

###  https://w3id.org/osdu#identifier
osdu:identifier rdf:type owl:DatatypeProperty ;
	rdfs:comment "Identifier property " ;
	rdfs:domain [
		rdf:type owl:Class ;
		owl:unionOf (
			osdu:ObjectAlias
			osdu:WellAlias
			osdu:ReservoirCompartmentUnit
		) ;
	] ;
	rdfs:range xsd:string ;
.

###  https://w3id.org/osdu#imageArea
osdu:imageArea rdf:type owl:DatatypeProperty ;
	rdfs:comment "The area as unit of measure covered by the images which are input for the processing. Must be the same unit as the Measure point Density. Interdependent with number of measured points and  measure point density " ;
	rdfs:domain osdu:ProcessedInSAR ;
	rdfs:range xsd:decimal ;
.

###  https://w3id.org/osdu#imageTypeID
osdu:imageTypeID rdf:type owl:DatatypeProperty ;
	rdfs:comment "The relationship to a GeoReferencedImageType record, which classifies this GeoReferencedImage, e.g., as horizontal map, vertical curtain. " ;
	rdfs:domain osdu:GeoReferencedImage ;
	xsd:pattern "^[\\\\w\\\\-\\\\.]+:reference-data\\\\-\\\\-GeoReferencedImageType:[\\\\w\\\\-\\\\.\\\\:\\\\%]+:[0-9]*$" ;
	rdfs:range xsd:string ;
.

###  https://w3id.org/osdu#imagingModeID
osdu:imagingModeID rdf:type owl:DatatypeProperty ;
	rdfs:comment "Imaging mode utilised. For example: Stripmap, Spotlight, ScanSAR, etc " ;
	rdfs:domain osdu:ProcessedInSAR ;
	xsd:pattern "^[\\\\w\\\\-\\\\.]+:reference-data\\\\-\\\\-InSARImageMode:[\\\\w\\\\-\\\\.\\\\:\\\\%]+:[0-9]*$" ;
	rdfs:range xsd:string ;
.

###  https://w3id.org/osdu#importTimeStamp
osdu:importTimeStamp rdf:type owl:DatatypeProperty ;
	rdfs:comment "The time in ISO-8601 format when the data was imported to VDS. " ;
	rdfs:domain osdu:OpenVDS ;
	rdfs:range time:DateTimeDescription ;
.

###  https://w3id.org/osdu#inUse
osdu:inUse rdf:type owl:DatatypeProperty ;
	rdfs:comment "Used to indicate if Equipment or Service in scope for the Cost Item is being used. Can drive different Standby/In Use Rental Rates where applicable. " ;
	rdfs:domain osdu:Cost ;
	rdfs:range xsd:boolean ;
.

###  https://w3id.org/osdu#inactiveIndicator
osdu:inactiveIndicator rdf:type owl:DatatypeProperty ;
	rdfs:comment "By default reference values are considered as 'active'. An absent 'InactiveIndicator' property value means the reference value is in active use. When 'InactiveIndicator' is set true the reverence value is no longer in use and should no longer be offered as a choice. " ;
	rdfs:domain osdu:AbstractReferenceType ;
	rdfs:range xsd:boolean ;
.

###  https://w3id.org/osdu#incidenceAngle
osdu:incidenceAngle rdf:type owl:DatatypeProperty ;
	rdfs:comment "The single common angle or line of sight angle of the radiation on a flat horizontal terrain. " ;
	rdfs:domain osdu:ProcessedInSAR ;
	rdfs:range xsd:decimal ;
.

###  https://w3id.org/osdu#incidentReporterName
osdu:incidentReporterName rdf:type owl:DatatypeProperty ;
	rdfs:comment "Name of the person who prepared the incident report. " ;
	rdfs:domain osdu:Incident ;
	rdfs:range xsd:string ;
	owl:sameAs foaf:name ;
.

###  https://w3id.org/osdu#inclinationStart
osdu:inclinationStart rdf:type owl:DatatypeProperty ;
	rdfs:comment "Inclination at start measured depth. " ;
	rdfs:domain osdu:DrillingParameters ;
	rdfs:range xsd:decimal ;
.

###  https://w3id.org/osdu#inclinationStop
osdu:inclinationStop rdf:type owl:DatatypeProperty ;
	rdfs:comment "Inclination at stop measured depth. " ;
	rdfs:domain osdu:DrillingParameters ;
	rdfs:range xsd:decimal ;
.

###  https://w3id.org/osdu#index
osdu:index rdf:type owl:DatatypeProperty ;
	rdfs:comment "When parameter is an array, used to indicate the index in the array. " ;
	rdfs:domain osdu:AbstractActivityParameter ;
	rdfs:range xsd:integer ;
.

###  https://w3id.org/osdu#indexFilePath
osdu:indexFilePath rdf:type owl:DatatypeProperty ;
	rdfs:comment "An optional path to an index file. " ;
	rdfs:domain osdu:DatasetProperties ;
	rdfs:range xsd:string ;
.

###  https://w3id.org/osdu#indexableElementID
osdu:indexableElementID rdf:type owl:DatatypeProperty ;
	rdfs:comment "The indexable element which is considered " ;
	rdfs:domain [
		rdf:type owl:Class ;
		owl:unionOf (
			osdu:IndexableElementCount
			osdu:SubRepresentation
			osdu:GenericProperty
		) ;
	] ;
	xsd:pattern "^[\\\\w\\\\-\\\\.]+:reference-data\\\\-\\\\-IndexableElement:[\\\\w\\\\-\\\\.\\\\:\\\\%]+:[0-9]*$" ;
	rdfs:range xsd:string ;
.

###  https://w3id.org/osdu#informationSource
osdu:informationSource rdf:type owl:DatatypeProperty ;
	rdfs:comment "The InformationSource providing the definition if different from AttributionAuthority. " ;
	rdfs:domain [
		rdf:type owl:Class ;
		owl:unionOf (
			osdu:CoordinateTransformation
			osdu:CoordinateReferenceSystem
		) ;
	] ;
	rdfs:range xsd:string ;
.

###  https://w3id.org/osdu#initialConditionBearing
osdu:initialConditionBearing rdf:type owl:DatatypeProperty ;
	rdfs:comment "Condition of bit bearings (integer 0-8 or E, F, N or X)). " ;
	rdfs:domain osdu:BitRecord ;
	rdfs:range xsd:string ;
.

###  https://w3id.org/osdu#initialConditionDull
osdu:initialConditionDull rdf:type owl:DatatypeProperty ;
	rdfs:comment "Overall dull condition from IADC bit wear 2 character codes. " ;
	rdfs:domain osdu:BitRecord ;
	xsd:pattern "^[\\\\w\\\\-\\\\.]+:reference-data\\\\-\\\\-BitDullCode:[\\\\w\\\\-\\\\.\\\\:\\\\%]+:[0-9]*$" ;
	rdfs:range xsd:string ;
.

###  https://w3id.org/osdu#initialConditionGauge
osdu:initialConditionGauge rdf:type owl:DatatypeProperty ;
	rdfs:comment "Condition of bit gauge in 1/16 of an inch. I = in gauge, else number of 16ths out of gauge. " ;
	rdfs:domain osdu:BitRecord ;
	rdfs:range xsd:string ;
.

###  https://w3id.org/osdu#initialConditionInner
osdu:initialConditionInner rdf:type owl:DatatypeProperty ;
	rdfs:comment "Condition of inner tooth rows (inner 2/3 of bit) (0-8). " ;
	rdfs:domain osdu:BitRecord ;
	rdfs:range xsd:decimal ;
.

###  https://w3id.org/osdu#initialConditionLocation
osdu:initialConditionLocation rdf:type owl:DatatypeProperty ;
	rdfs:comment "Row and cone numbers for items which need location information (e.g. Cracked Cone, Lost Cone etc). " ;
	rdfs:domain osdu:BitRecord ;
	rdfs:range xsd:string ;
.

###  https://w3id.org/osdu#initialConditionOther
osdu:initialConditionOther rdf:type owl:DatatypeProperty ;
	rdfs:comment "Other comments on bit condition from IADC list (BitDullCode in standard list). " ;
	rdfs:domain osdu:BitRecord ;
	rdfs:range xsd:string ;
.

###  https://w3id.org/osdu#initialConditionOuter
osdu:initialConditionOuter rdf:type owl:DatatypeProperty ;
	rdfs:comment "Condition of outer tooth rows (outer 1/3 of bit) (0-8). " ;
	rdfs:domain osdu:BitRecord ;
	rdfs:range xsd:decimal ;
.

###  https://w3id.org/osdu#initialConditionReason
osdu:initialConditionReason rdf:type owl:DatatypeProperty ;
	rdfs:comment "Reason bit was pulled from IADC codes. " ;
	rdfs:domain osdu:BitRecord ;
	xsd:pattern "^[\\\\w\\\\-\\\\.]+:reference-data\\\\-\\\\-BitReasonPulled:[\\\\w\\\\-\\\\.\\\\:\\\\%]+:[0-9]*$" ;
	rdfs:range xsd:string ;
.

###  https://w3id.org/osdu#initialOperatorID
osdu:initialOperatorID rdf:type owl:DatatypeProperty ;
	rdfs:comment "A initial operator organization ID; the organization ID may also be found in the FacilityOperatorOrganisationID of the FacilityOperator array providing the actual dates. " ;
	rdfs:domain osdu:AbstractFacility ;
	xsd:pattern "^[\\\\w\\\\-\\\\.]+:master-data\\\\-\\\\-Organisation:[\\\\w\\\\-\\\\.\\\\:\\\\%]+:[0-9]*$" ;
	rdfs:range xsd:string ;
.

###  https://w3id.org/osdu#initialPressure
osdu:initialPressure rdf:type owl:DatatypeProperty ;
	rdfs:comment "Initial pressure of the aquifer.  Default property, caution if the grid property has got multi realizations. " ;
	rdfs:domain osdu:SingleCellAquifer ;
	rdfs:range xsd:decimal ;
.

###  https://w3id.org/osdu#initialProbability
osdu:initialProbability rdf:type owl:DatatypeProperty ;
	rdfs:comment "Initial Probability Level of the Risk. 					Values of 1 through 5 with 1 being the lowest. " ;
	rdfs:domain osdu:Risk ;
	rdfs:range xsd:decimal ;
.

###  https://w3id.org/osdu#initialRiskScore
osdu:initialRiskScore rdf:type owl:DatatypeProperty ;
	rdfs:comment "Score computed as of Pre-Mitigation which is the combination of :  Initial Severity * Initial Probability  Values of 1 through 25 with 1 being the lowest. " ;
	rdfs:domain osdu:Risk ;
	rdfs:range xsd:decimal ;
.

###  https://w3id.org/osdu#initialSeverity
osdu:initialSeverity rdf:type owl:DatatypeProperty ;
	rdfs:comment "Initial Severity Level of the Risk.  					Values of 1 through 5 with 1 being the lowest. " ;
	rdfs:domain osdu:Risk ;
	rdfs:range xsd:decimal ;
.

###  https://w3id.org/osdu#initialSurfPressure
osdu:initialSurfPressure rdf:type owl:DatatypeProperty ;
	rdfs:comment "Initial surface pressure " ;
	rdfs:domain osdu:PerforationInterval ;
	rdfs:range xsd:decimal ;
.

###  https://w3id.org/osdu#inlineIncrement
osdu:inlineIncrement rdf:type owl:DatatypeProperty ;
	rdfs:comment "Sampling interval of inlines in this dataset (difference in labels between neighboring inlines). " ;
	rdfs:domain osdu:SeismicTraceData ;
	rdfs:range xsd:decimal ;
.

###  https://w3id.org/osdu#inlineMax
osdu:inlineMax rdf:type owl:DatatypeProperty ;
	rdfs:comment "Largest Inline/Line/Track value " ;
	rdfs:domain [
		rdf:type owl:Class ;
		owl:unionOf (
			osdu:SeismicTraceData
			osdu:SeismicHorizon
		) ;
	] ;
	rdfs:range xsd:decimal ;
.

###  https://w3id.org/osdu#inlineMin
osdu:inlineMin rdf:type owl:DatatypeProperty ;
	rdfs:comment "Smallest Inline/Line/Track value " ;
	rdfs:domain [
		rdf:type owl:Class ;
		owl:unionOf (
			osdu:SeismicTraceData
			osdu:SeismicHorizon
		) ;
	] ;
	rdfs:range xsd:decimal ;
.

###  https://w3id.org/osdu#innerDiameter
osdu:innerDiameter rdf:type owl:DatatypeProperty ;
	rdfs:comment "Nominal inner diameter of the component. " ;
	rdfs:domain osdu:TubularComponent ;
	rdfs:range xsd:decimal ;
.

###  https://w3id.org/osdu#insideCasingVolume
osdu:insideCasingVolume rdf:type owl:DatatypeProperty ;
	rdfs:comment "Estimated volume inside casing. " ;
	rdfs:domain osdu:CementStage ;
	rdfs:range xsd:decimal ;
.

###  https://w3id.org/osdu#installedTubularAssemblyID
osdu:installedTubularAssemblyID rdf:type owl:DatatypeProperty ;
	rdfs:comment "The identifier of the tubular to be installed. " ;
	rdfs:domain osdu:FluidsInterval ;
	xsd:pattern "^[\\\\w\\\\-\\\\.]+:work-product-component\\\\-\\\\-TubularAssembly:[\\\\w\\\\-\\\\.\\\\:\\\\%]+:[0-9]*$" ;
	rdfs:range xsd:string ;
.

###  https://w3id.org/osdu#integerColumn
osdu:integerColumn rdf:type owl:DatatypeProperty ;
	rdfs:comment "A column of only integer values " ;
	rdfs:domain [
		rdf:type owl:Class ;
		owl:unionOf (
			osdu:ColumnValues
			osdu:Columnvalues
		) ;
	] ;
	rdfs:range xsd:integer ;
.

###  https://w3id.org/osdu#integerParameterKey
osdu:integerParameterKey rdf:type owl:DatatypeProperty ;
	rdfs:comment "Integer value from ParameterKey parameter, associated with this parameter. Example: {ParameterKey: index, StringParameterKey: 2}. " ;
	rdfs:domain osdu:ParameterKey ;
	rdfs:range xsd:integer ;
.

###  https://w3id.org/osdu#integerQuantityParameter
osdu:integerQuantityParameter rdf:type owl:DatatypeProperty ;
	rdfs:comment "Parameter containing an integer value. " ;
	rdfs:domain osdu:AbstractActivityParameter ;
	rdfs:range xsd:integer ;
.

###  https://w3id.org/osdu#interestTypeID
osdu:interestTypeID rdf:type owl:DatatypeProperty ;
	rdfs:comment "Business Interest [Well Interest Type] describes whether a company currently considers a well/wellbore or its data to be a real or planned asset, and if so, the nature of and motivation for that company's interest. " ;
	rdfs:domain [
		rdf:type owl:Class ;
		owl:unionOf (
			osdu:Wellbore
			osdu:HistoricalInterest
			osdu:Well
		) ;
	] ;
	xsd:pattern "^[\\\\w\\\\-\\\\.]+:reference-data\\\\-\\\\-WellInterestType:[\\\\w\\\\-\\\\.\\\\:\\\\%]+:[0-9]*$" ;
	rdfs:range xsd:string ;
.

###  https://w3id.org/osdu#internalOrganisationIndicator
osdu:internalOrganisationIndicator rdf:type owl:DatatypeProperty ;
	rdfs:comment "Indicates if the organisation is internal to the enterprise. " ;
	rdfs:domain osdu:Organisation ;
	rdfs:range xsd:boolean ;
.

###  https://w3id.org/osdu#interpolate
osdu:interpolate rdf:type owl:DatatypeProperty ;
	rdfs:comment "Whether curve can be interpolated or not " ;
	rdfs:domain osdu:Curves ;
	rdfs:range xsd:boolean ;
.

###  https://w3id.org/osdu#interpolationMethodID
osdu:interpolationMethodID rdf:type owl:DatatypeProperty ;
	rdfs:comment "For discretely sampled models, the mathematical form of interpolation between nodes, such as linear in space, bicubic spline, linear in time, trilinear, horizon-based. " ;
	rdfs:domain osdu:VelocityModeling ;
	xsd:pattern "^[\\\\w\\\\-\\\\.]+:reference-data\\\\-\\\\-InterpolationMethod:[\\\\w\\\\-\\\\.\\\\:\\\\%]+:[0-9]*$" ;
	rdfs:range xsd:string ;
.

###  https://w3id.org/osdu#interpretationID
osdu:interpretationID rdf:type owl:DatatypeProperty ;
	rdfs:comment "Allow to link an interpretation ID with this object " ;
	rdfs:domain [
		rdf:type owl:Class ;
		owl:unionOf (
			osdu:AbstractRepresentation
			osdu:AbstractGridRepresentation
			osdu:Markers
			osdu:SealedSurfaceFramework
			osdu:UnsealedSurfaceFramework
			osdu:IjkGridNumericalAquiferRepresentation
		) ;
	] ;
	xsd:pattern "^[\\\\w\\\\-\\\\.]+:(work-product-component\\\\-\\\\-EarthModelInterpretation|work-product-component\\\\-\\\\-GeobodyBoundaryInterpretation|work-product-component\\\\-\\\\-GeobodyInterpretation|work-product-component\\\\-\\\\-HorizonInterpretation|work-product-component\\\\-\\\\-RockFluidOrganizationInterpretation|work-product-component\\\\-\\\\-RockFluidUnitInterpretation|work-product-component\\\\-\\\\-StratigraphicUnitInterpretation|work-product-component\\\\-\\\\-StructuralOrganizationInterpretation|work-product-component\\\\-\\\\-FaultInterpretation|work-product-component\\\\-\\\\-AquiferInterpretation):[\\\\w\\\\-\\\\.\\\\:\\\\%]+:[0-9]*$" ;
	xsd:pattern "^[\\\\w\\\\-\\\\.]+:work-product-component\\\\-\\\\-EarthModelInterpretation:[\\\\w\\\\-\\\\.\\\\:\\\\%]+:[0-9]*$" ;
	xsd:pattern "^[\\\\w\\\\-\\\\.]+:(work-product-component\\\\-\\\\-HorizonInterpretation|work-product-component\\\\-\\\\-FaultInterpretation|work-product-component\\\\-\\\\-GeobodyBoundaryInterpretation):[\\\\w\\\\-\\\\.\\\\:\\\\%]+:[0-9]*$" ;
	xsd:pattern "^[\\\\w\\\\-\\\\.]+:work-product-component\\\\-\\\\-StructuralOrganizationInterpretation:[\\\\w\\\\-\\\\.\\\\:\\\\%]+:[0-9]*$" ;
	xsd:pattern "^[\\\\w\\\\-\\\\.]+:work-product-component\\\\-\\\\-AquiferInterpretation:[\\\\w\\\\-\\\\.\\\\:\\\\%]+:[0-9]*$" ;
	rdfs:range xsd:string ;
.

###  https://w3id.org/osdu#interpretationIDs
osdu:interpretationIDs rdf:type owl:DatatypeProperty ;
	rdfs:comment "References to the interpretations which some (or all) of the connections represent. " ;
	rdfs:domain osdu:GridConnectionSetRepresentation ;
	xsd:pattern "^[\\\\w\\\\-\\\\.]+:(work-product-component\\\\-\\\\-FaultInterpretation|work-product-component\\\\-\\\\-EarthModelInterpretation|work-product-component\\\\-\\\\-GeobodyBoundaryInterpretation|work-product-component\\\\-\\\\-GeobodyInterpretation|work-product-component\\\\-\\\\-HorizonInterpretation|work-product-component\\\\-\\\\-RockFluidOrganizationInterpretation|work-product-component\\\\-\\\\-RockFluidUnitInterpretation|work-product-component\\\\-\\\\-StratigraphicUnitInterpretation|work-product-component\\\\-\\\\-StructuralOrganizationInterpretation):[\\\\w\\\\-\\\\.\\\\:\\\\%]+:[0-9]*$" ;
	rdfs:range xsd:string ;
.

###  https://w3id.org/osdu#interpretationName
osdu:interpretationName rdf:type owl:DatatypeProperty ;
	rdfs:comment "Name of the interpretation the representation refers to " ;
	rdfs:domain osdu:AbstractRepresentation ;
	rdfs:range xsd:string ;
.

###  https://w3id.org/osdu#interpreter
osdu:interpreter rdf:type owl:DatatypeProperty ;
	rdfs:comment "The person or team who interpreted the fault data. " ;
	rdfs:domain [
		rdf:type owl:Class ;
		owl:unionOf (
			osdu:Faults
			osdu:SeismicHorizon
			osdu:SeismicFault
		) ;
	] ;
	rdfs:range xsd:string ;
.

###  https://w3id.org/osdu#interpreterName
osdu:interpreterName rdf:type owl:DatatypeProperty ;
	rdfs:comment "The name of person who interpreted this Log Curve. " ;
	rdfs:domain osdu:Curves ;
	rdfs:range xsd:string ;
	owl:sameAs foaf:name ;
.

###  https://w3id.org/osdu#intervalBaseMeasuredDepth
osdu:intervalBaseMeasuredDepth rdf:type owl:DatatypeProperty ;
	rdfs:comment "The bottom measured depth of the interval in which the fluid will be used (in many cases, this Measured Depth will be the same than the one provided by WellboreArchitecture.HoleSection content). Depth relative to Planned wellbore ZDP. Navigate via WellboreID to the side-car WellPlanningWellbore, which holds the depth reference in data.VerticalMeasurement. " ;
	rdfs:domain [
		rdf:type owl:Class ;
		owl:unionOf (
			osdu:FluidsInterval
			osdu:PerforationInterval
			osdu:GeologyInterval
		) ;
	] ;
	rdfs:range xsd:decimal ;
.

###  https://w3id.org/osdu#intervalComments
osdu:intervalComments rdf:type owl:DatatypeProperty ;
	rdfs:comment "Interval Comments " ;
	rdfs:domain osdu:PerforationInterval ;
	rdfs:range xsd:string ;
.

###  https://w3id.org/osdu#intervalDateTime
osdu:intervalDateTime rdf:type owl:DatatypeProperty ;
	rdfs:comment "Perforation interval date/time " ;
	rdfs:domain osdu:PerforationInterval ;
	rdfs:range time:DateTimeDescription ;
.

###  https://w3id.org/osdu#intervalID
osdu:intervalID rdf:type owl:DatatypeProperty ;
	rdfs:comment "The unique identifier of the interval array member in the data.Intervals[] array. Ideally a UUID. " ;
	rdfs:domain osdu:Interval ;
	rdfs:range xsd:string ;
.

###  https://w3id.org/osdu#intervalLength
osdu:intervalLength rdf:type owl:DatatypeProperty ;
	rdfs:comment "Distance between MD top and base of interval (net distance) aka 'Top Shot to Bottom Shot' Interval. " ;
	rdfs:domain osdu:PerforationInterval ;
	rdfs:range xsd:decimal ;
.

###  https://w3id.org/osdu#intervalName
osdu:intervalName rdf:type owl:DatatypeProperty ;
	rdfs:comment "The name of an interval in which the fluid will be used " ;
	rdfs:domain osdu:FluidsInterval ;
	rdfs:range xsd:string ;
.

###  https://w3id.org/osdu#intervalReasonTypeID
osdu:intervalReasonTypeID rdf:type owl:DatatypeProperty ;
	rdfs:comment "Interval Reason " ;
	rdfs:domain osdu:PerforationInterval ;
	xsd:pattern "^[\\\\w\\\\-\\\\.]+:reference-data\\\\-\\\\-PerforationIntervalReason:[\\\\w\\\\-\\\\.\\\\:\\\\%]+:[0-9]*$" ;
	rdfs:range xsd:string ;
.

###  https://w3id.org/osdu#intervalTVDBase
osdu:intervalTVDBase rdf:type owl:DatatypeProperty ;
	rdfs:comment "True vertical depth at base of interval. " ;
	rdfs:domain osdu:GeologyInterval ;
	rdfs:range xsd:decimal ;
.

###  https://w3id.org/osdu#intervalTVDTop
osdu:intervalTVDTop rdf:type owl:DatatypeProperty ;
	rdfs:comment "True vertical depth at top of the section. " ;
	rdfs:domain osdu:GeologyInterval ;
	rdfs:range xsd:decimal ;
.


###  https://w3id.org/osdu#intervalTopMeasuredDepth
osdu:intervalTopMeasuredDepth rdf:type owl:DatatypeProperty ;
	rdfs:comment "Measured depth at top of interval. Depth relative to Planned wellbore ZDP. Navigate via WellboreID to the side-car WellPlanningWellbore, which holds the depth reference in data.VerticalMeasurement. " ;
	rdfs:domain [
		rdf:type owl:Class ;
		owl:unionOf (
			osdu:FluidsInterval
			osdu:CementStage
			osdu:PerforationInterval
			osdu:GeologyInterval
		) ;
	] ;
	rdfs:range xsd:decimal ;
.

###  https://w3id.org/osdu#intervalTypeID
osdu:intervalTypeID rdf:type owl:DatatypeProperty ;
	rdfs:comment "Perforated interval type " ;
	rdfs:domain osdu:PerforationInterval ;
	xsd:pattern "^[\\\\w\\\\-\\\\.]+:reference-data\\\\-\\\\-PerforationIntervalType:[\\\\w\\\\-\\\\.\\\\:\\\\%]+:[0-9]*$" ;
	rdfs:range xsd:string ;
.

###  https://w3id.org/osdu#invoiceNumber
osdu:invoiceNumber rdf:type owl:DatatypeProperty ;
	rdfs:comment "Invoice number for cost item; the bill is sent to the operator. " ;
	rdfs:domain osdu:Cost ;
	rdfs:range xsd:string ;
.

###  https://w3id.org/osdu#iron
osdu:iron rdf:type owl:DatatypeProperty ;
	rdfs:comment "Iron content. " ;
	rdfs:domain osdu:Fluid ;
	rdfs:range xsd:decimal ;
.

###  https://w3id.org/osdu#isAdditionalShot
osdu:isAdditionalShot rdf:type owl:DatatypeProperty ;
	rdfs:comment "Additional shot Y/N (+1 to Tot Shots calc) " ;
	rdfs:domain osdu:PerforationInterval ;
	rdfs:range xsd:boolean ;
.

###  https://w3id.org/osdu#isBaseUnit
osdu:isBaseUnit rdf:type owl:DatatypeProperty ;
	rdfs:comment "True if the unit is a base unit for the unit quantity. If the property is absent, it means the unit is not a base unit. " ;
	rdfs:domain [
		rdf:type owl:Class ;
		owl:unionOf (
			osdu:UnitOfMeasure
			osdu:ExternalUnitOfMeasure
		) ;
	] ;
	rdfs:range xsd:boolean ;
.

###  https://w3id.org/osdu#isCarryOver
osdu:isCarryOver rdf:type owl:DatatypeProperty ;
	rdfs:comment "Is this item carried from day to day? " ;
	rdfs:domain osdu:Cost ;
	rdfs:range xsd:boolean ;
.

###  https://w3id.org/osdu#isCoilTubing
osdu:isCoilTubing rdf:type owl:DatatypeProperty ;
	rdfs:comment "Coiled Tubing Used (true=CTU used). Values are true (or 1) and false (or 0). " ;
	rdfs:domain osdu:PlannedCementJob ;
	rdfs:range xsd:boolean ;
.

###  https://w3id.org/osdu#isConformableAbove
osdu:isConformableAbove rdf:type owl:DatatypeProperty ;
	rdfs:comment "Defines whether the stratigraphic unit above the horizon is conformable " ;
	rdfs:domain osdu:HorizonInterpretation ;
	rdfs:range xsd:boolean ;
.

###  https://w3id.org/osdu#isConformableBelow
osdu:isConformableBelow rdf:type owl:DatatypeProperty ;
	rdfs:comment "Defines whether the stratigraphic unit below the horizon is conformable " ;
	rdfs:domain osdu:HorizonInterpretation ;
	rdfs:range xsd:boolean ;
.

###  https://w3id.org/osdu#isCoreSlabbed
osdu:isCoreSlabbed rdf:type owl:DatatypeProperty ;
	rdfs:comment "A flag to denote whether a particular core has been slabbed or not. " ;
	rdfs:domain osdu:RockSample ;
	rdfs:range xsd:boolean ;
.

###  https://w3id.org/osdu#isDiscoverable
osdu:isDiscoverable rdf:type owl:DatatypeProperty ;
	rdfs:comment "A flag that indicates if the work is searchable, which means covered in the search index. " ;
	rdfs:domain [
		rdf:type owl:Class ;
		owl:unionOf (
			osdu:AbstractWPCGroupType
			osdu:WorkProduct
		) ;
	] ;
	rdfs:range xsd:boolean ;
.

###  https://w3id.org/osdu#isEstimated
osdu:isEstimated rdf:type owl:DatatypeProperty ;
	rdfs:comment "Is this an estimated cost? " ;
	rdfs:domain osdu:Cost ;
	rdfs:range xsd:boolean ;
.

###  https://w3id.org/osdu#isExtendedLoad
osdu:isExtendedLoad rdf:type owl:DatatypeProperty ;
	rdfs:comment "A flag that indicates if the work is undergoing an extended load.  It reflects the fact that the work product is in an early stage and may be updated before finalization. " ;
	rdfs:domain [
		rdf:type owl:Class ;
		owl:unionOf (
			osdu:AbstractWPCGroupType
			osdu:WorkProduct
		) ;
	] ;
	rdfs:range xsd:boolean ;
.

###  https://w3id.org/osdu#isFoamUsed
osdu:isFoamUsed rdf:type owl:DatatypeProperty ;
	rdfs:comment "Foam used indicator.  Values are true (or 1) and false (or 0). " ;
	rdfs:domain osdu:CementingFluid ;
	rdfs:range xsd:boolean ;
.

###  https://w3id.org/osdu#isHigh
osdu:isHigh rdf:type owl:DatatypeProperty ;
	rdfs:comment "Boolean that states if the criteria are for the high pressure stage (low pressure stage otherwise) " ;
	rdfs:domain osdu:PressureCriteria ;
	rdfs:range xsd:boolean ;
.

###  https://w3id.org/osdu#isInput
osdu:isInput rdf:type owl:DatatypeProperty ;
	rdfs:comment "Indicates if the parameter is an input of the activity. If the parameter is a data object and is also an output of the activity, it is strongly advised to use two parameters : one for input and one for output. The reason is to be able to give two different versions strings for the input and output data object which has got obviously the same UUID. " ;
	rdfs:domain osdu:ParameterTemplate ;
	rdfs:range xsd:boolean ;
.

###  https://w3id.org/osdu#isIntrusive
osdu:isIntrusive rdf:type owl:DatatypeProperty ;
	rdfs:comment "Corresponding to Energistics GeologicUnitMaterialEmplacement 'intrusive' and 'non-intrusive'. " ;
	rdfs:domain osdu:AbstractGeologicUnitInterpretation ;
	rdfs:range xsd:boolean ;
.

###  https://w3id.org/osdu#isListric
osdu:isListric rdf:type owl:DatatypeProperty ;
	rdfs:comment "Specifies whether the fault is considered listric " ;
	rdfs:domain osdu:FaultInterpretation ;
	rdfs:range xsd:boolean ;
.

###  https://w3id.org/osdu#isNearMiss
osdu:isNearMiss rdf:type owl:DatatypeProperty ;
	rdfs:comment "Near miss incident occurrence? " ;
	rdfs:domain osdu:Incident ;
	rdfs:range xsd:boolean ;
.

###  https://w3id.org/osdu#isOffline
osdu:isOffline rdf:type owl:DatatypeProperty ;
	rdfs:comment "Is the activity an Offline activity, Values are true (or 1) and false (or 0). " ;
	rdfs:domain osdu:DrillingActivity ;
	rdfs:range xsd:boolean ;
.

###  https://w3id.org/osdu#isOffshoreJob
osdu:isOffshoreJob rdf:type owl:DatatypeProperty ;
	rdfs:comment "Offshore job? Values are true (or 1) and false (or 0). " ;
	rdfs:domain osdu:PlannedCementJob ;
	rdfs:range xsd:boolean ;
.

###  https://w3id.org/osdu#isOptimum
osdu:isOptimum rdf:type owl:DatatypeProperty ;
	rdfs:comment "Is the activity optimum? Values are true (or 1) and false (or 0). " ;
	rdfs:domain osdu:DrillingActivity ;
	rdfs:range xsd:boolean ;
.

###  https://w3id.org/osdu#isOptional
osdu:isOptional rdf:type owl:DatatypeProperty ;
	rdfs:comment "Flag used to indicates this particular activity is optional in the plan. " ;
	rdfs:domain osdu:WellPlanningActivity ;
	rdfs:range xsd:boolean ;
.

###  https://w3id.org/osdu#isOriented
osdu:isOriented rdf:type owl:DatatypeProperty ;
	rdfs:comment "Indicates if the core was oriented. " ;
	rdfs:domain osdu:Coring ;
	rdfs:range xsd:boolean ;
.

###  https://w3id.org/osdu#isOutput
osdu:isOutput rdf:type owl:DatatypeProperty ;
	rdfs:comment "Indicates if the parameter is an output of the activity. If the parameter is a data object and is also an input of the activity, it is strongly advised to use two parameters : one for input and one for output. The reason is to be able to give two different versions strings for the input and output data object which has got obviously the same UUID. " ;
	rdfs:domain osdu:ParameterTemplate ;
	rdfs:range xsd:boolean ;
.

###  https://w3id.org/osdu#isOverwrite
osdu:isOverwrite rdf:type owl:DatatypeProperty ;
	rdfs:comment "Normally true, higher index trajectory takes precedence over overlapping section of previous trajectory.  Values are true (or 1) and false (or 0). " ;
	rdfs:domain osdu:SurveySection ;
	rdfs:range xsd:boolean ;
.

###  https://w3id.org/osdu#isPlugCleaned
osdu:isPlugCleaned rdf:type owl:DatatypeProperty ;
	rdfs:comment "For sample plugs: a flag indicating whether the plug has been cleaned. More details in the associated RockSampleAnalysis. " ;
	rdfs:domain osdu:RockSample ;
	rdfs:range xsd:boolean ;
.

###  https://w3id.org/osdu#isProcessed
osdu:isProcessed rdf:type owl:DatatypeProperty ;
	rdfs:comment "Indicates if the curve has been (pre)processed or if it is a raw recording " ;
	rdfs:domain osdu:Curves ;
	rdfs:range xsd:boolean ;
.

###  https://w3id.org/osdu#isProductive
osdu:isProductive rdf:type owl:DatatypeProperty ;
	rdfs:comment "Does activity bring closer to objective?  Values are true (or 1) and false (or 0). " ;
	rdfs:domain osdu:DrillingActivity ;
	rdfs:range xsd:boolean ;
.

###  https://w3id.org/osdu#isRadial
osdu:isRadial rdf:type owl:DatatypeProperty ;
	rdfs:comment "TRUE if the grid is periodic in J, i.e., has the topology of a complete 360 degree circle. " ;
	rdfs:domain osdu:AbstractIjkGridPatch ;
	rdfs:range xsd:boolean ;
.

###  https://w3id.org/osdu#isReciprocating
osdu:isReciprocating rdf:type owl:DatatypeProperty ;
	rdfs:comment "Pipe being reciprocated.  Values are true (or 1) and false (or 0). " ;
	rdfs:domain osdu:PlannedCementJob ;
	rdfs:range xsd:boolean ;
.

###  https://w3id.org/osdu#isReferenceValueType
osdu:isReferenceValueType rdf:type owl:DatatypeProperty ;
	rdfs:comment "The flag indicating that this type is a reference value type. " ;
	rdfs:domain osdu:Type ;
	rdfs:range xsd:boolean ;
.

###  https://w3id.org/osdu#isRegular
osdu:isRegular rdf:type owl:DatatypeProperty ;
	rdfs:comment "Boolean property indicating the sampling mode of the ReferenceCurveID. True means all reference curve values are regularly spaced (see SamplingInterval); false means irregular or discrete sample spacing. " ;
	rdfs:domain osdu:WellLog ;
	rdfs:range xsd:boolean ;
.

###  https://w3id.org/osdu#isRental
osdu:isRental rdf:type owl:DatatypeProperty ;
	rdfs:comment "Is this item a rental? " ;
	rdfs:domain osdu:Cost ;
	rdfs:range xsd:boolean ;
.

###  https://w3id.org/osdu#isReturnsToSeabed
osdu:isReturnsToSeabed rdf:type owl:DatatypeProperty ;
	rdfs:comment "Returns to seabed? Values are true (or 1) and false (or 0). " ;
	rdfs:domain osdu:PlannedCementJob ;
	rdfs:range xsd:boolean ;
.

###  https://w3id.org/osdu#isRightHanded
osdu:isRightHanded rdf:type owl:DatatypeProperty ;
	rdfs:comment "Indicates that the IJK grid is right handed, as determined by the triple product of tangent vectors in the I, J, and K directions. " ;
	rdfs:domain osdu:AbstractIjkGridPatch ;
	rdfs:range xsd:boolean ;
.

###  https://w3id.org/osdu#isSealed
osdu:isSealed rdf:type owl:DatatypeProperty ;
	rdfs:comment "Specifies whether the fault is considered sealed " ;
	rdfs:domain osdu:FaultInterpretation ;
	rdfs:range xsd:boolean ;
.

###  https://w3id.org/osdu#isTractorUsed
osdu:isTractorUsed rdf:type owl:DatatypeProperty ;
	rdfs:comment "Is a tractor used during the job to help convey guns " ;
	rdfs:domain osdu:PerforationJob ;
	rdfs:range xsd:boolean ;
.

###  https://w3id.org/osdu#isobutane
osdu:isobutane rdf:type owl:DatatypeProperty ;
	rdfs:comment "Iso-butane (iC4) concentration. " ;
	rdfs:domain osdu:GasReading ;
	rdfs:range xsd:decimal ;
.

###  https://w3id.org/osdu#isopentane
osdu:isopentane rdf:type owl:DatatypeProperty ;
	rdfs:comment "Iso-pentane (iC5) concentration " ;
	rdfs:domain osdu:GasReading ;
	rdfs:range xsd:decimal ;
.

###  https://w3id.org/osdu#issueDateTime
osdu:issueDateTime rdf:type owl:DatatypeProperty ;
	rdfs:comment "Date and time license was issued " ;
	rdfs:domain osdu:WellPlanningWell ;
	rdfs:range time:DateTimeDescription ;
.

###  https://w3id.org/osdu#itemDescription
osdu:itemDescription rdf:type owl:DatatypeProperty ;
	rdfs:comment "Description of the item " ;
	rdfs:domain [
		rdf:type owl:Class ;
		owl:unionOf (
			osdu:Inventory
			osdu:Cost
		) ;
	] ;
	rdfs:range xsd:string ;
.

###  https://w3id.org/osdu#itemName
osdu:itemName rdf:type owl:DatatypeProperty ;
	rdfs:comment "Name or type of inventory item. " ;
	rdfs:domain osdu:Inventory ;
	rdfs:range xsd:decimal ;
.

###  https://w3id.org/osdu#itemSerialNumber
osdu:itemSerialNumber rdf:type owl:DatatypeProperty ;
	rdfs:comment "Serial number. " ;
	rdfs:domain osdu:Cost ;
	rdfs:range xsd:string ;
.

###  https://w3id.org/osdu#itemState
osdu:itemState rdf:type owl:DatatypeProperty ;
	rdfs:comment "The item state for the data object. (Actual, Planned, Unknown and Modeled) " ;
	rdfs:domain osdu:DrillingActivity ;
	rdfs:range xsd:string ;
.

###  https://w3id.org/osdu#j
osdu:j rdf:type owl:DatatypeProperty ;
	rdfs:comment "J index of the cell " ;
	rdfs:domain osdu:SingleCellAquifer ;
	rdfs:range xsd:integer ;
.

###  https://w3id.org/osdu#jobConfig
osdu:jobConfig rdf:type owl:DatatypeProperty ;
	rdfs:comment "Job configuration. " ;
	rdfs:domain osdu:PlannedCementJob ;
	rdfs:range xsd:string ;
.

###  https://w3id.org/osdu#jobEndDateTime
osdu:jobEndDateTime rdf:type owl:DatatypeProperty ;
	rdfs:comment "Job End Date/time " ;
	rdfs:domain osdu:PerforationJob ;
	rdfs:range time:DateTimeDescription ;
.

###  https://w3id.org/osdu#jobStartDateTime
osdu:jobStartDateTime rdf:type owl:DatatypeProperty ;
	rdfs:comment "Job Start Date/time " ;
	rdfs:domain osdu:PerforationJob ;
	rdfs:range time:DateTimeDescription ;
.

###  https://w3id.org/osdu#jobTypeID
osdu:jobTypeID rdf:type owl:DatatypeProperty ;
	rdfs:comment "Type of cement job. " ;
	rdfs:domain osdu:PlannedCementJob ;
	xsd:pattern "^[\\\\w\\\\-\\\\.]+:reference-data\\\\-\\\\-CementJobType:[\\\\w\\\\-\\\\.\\\\:\\\\%]+:[0-9]*$" ;
	rdfs:range xsd:string ;
.

###  https://w3id.org/osdu#k
osdu:k rdf:type owl:DatatypeProperty ;
	rdfs:comment "Consistency index (Power Law and HB). " ;
	rdfs:domain [
		rdf:type owl:Class ;
		owl:unionOf (
			osdu:CementingFluid
			osdu:SingleCellAquifer
		) ;
	] ;
	rdfs:range xsd:integer ;
.

###  https://w3id.org/osdu#kDirectionID
osdu:kDirectionID rdf:type owl:DatatypeProperty ;
	rdfs:comment "Indicate the K direction of the grid : up, down or not monotonic " ;
	rdfs:domain osdu:AbstractColumnLayerGridPatch ;
	xsd:pattern "^[\\\\w\\\\-\\\\.]+:reference-data\\\\-\\\\-KDirectionType:[\\\\w\\\\-\\\\.\\\\:\\\\%]+:[0-9]*$" ;
	rdfs:range xsd:string ;
.

###  https://w3id.org/osdu#keyConstraints
osdu:keyConstraints rdf:type owl:DatatypeProperty ;
	rdfs:comment "Allows to indicate that, in the same activity, this parameter template must be associated to another parameter template identified by its title. The associated parameter value constrains this parameter. " ;
	rdfs:domain osdu:ParameterTemplate ;
	rdfs:range xsd:string ;
.

###  https://w3id.org/osdu#keyName
osdu:keyName rdf:type owl:DatatypeProperty ;
	rdfs:comment "Relationship to a reference value for a name of a property header such as INLINE, CDPX. " ;
	rdfs:domain osdu:VectorHeaderMapping ;
	xsd:pattern "^[\\\\w\\\\-\\\\.]+:reference-data\\\\-\\\\-HeaderKeyName:[\\\\w\\\\-\\\\.\\\\:\\\\%]+:[0-9]*$" ;
	rdfs:range xsd:string ;
.

###  https://w3id.org/osdu#kickOffWellbore
osdu:kickOffWellbore rdf:type owl:DatatypeProperty ;
	rdfs:comment "This is a pointer to the parent wellbore. The wellbore that starts from top has no parent. " ;
	rdfs:domain osdu:Wellbore ;
	xsd:pattern "^[\\\\w\\\\-\\\\.]+:master-data\\\\-\\\\-Wellbore:[\\\\w\\\\-\\\\.\\\\:\\\\%]+:[0-9]*$" ;
	rdfs:range xsd:string ;
.

###  https://w3id.org/osdu#kickTolerance
osdu:kickTolerance rdf:type owl:DatatypeProperty ;
	rdfs:comment "Volume of a kick that will not cause a pressure exceeding the formation fracture pressure. " ;
	rdfs:domain osdu:Phase ;
	rdfs:range xsd:decimal ;
.

###  https://w3id.org/osdu#kickToleranceIntensity
osdu:kickToleranceIntensity rdf:type owl:DatatypeProperty ;
	rdfs:comment "Assumed kick density for calculation of kick tolerance where the fluid reading was recorded. " ;
	rdfs:domain osdu:Fluid ;
	rdfs:range xsd:decimal ;
.

###  https://w3id.org/osdu#kickToleranceVolume
osdu:kickToleranceVolume rdf:type owl:DatatypeProperty ;
	rdfs:comment "Assumed kick volume for calculation of kick tolerance based on the kick intensity where the fluid reading was recorded. " ;
	rdfs:domain osdu:Fluid ;
	rdfs:range xsd:decimal ;
.

###  https://w3id.org/osdu#kickoffMD
osdu:kickoffMD rdf:type owl:DatatypeProperty ;
	rdfs:comment "Measured depth to the kickoff point of the wellbore. " ;
	rdfs:domain osdu:DrillingReportStatusInfo ;
	rdfs:range xsd:decimal ;
.

###  https://w3id.org/osdu#kickoffTVD
osdu:kickoffTVD rdf:type owl:DatatypeProperty ;
	rdfs:comment "True vertical depth to the kickoff point of the wellbore. " ;
	rdfs:domain osdu:DrillingReportStatusInfo ;
	rdfs:range xsd:decimal ;
.

###  https://w3id.org/osdu#kind
osdu:kind rdf:type owl:DatatypeProperty ;
	rdfs:comment "The kind of resource / object." ;
	rdfs:domain [
		rdf:type owl:Class ;
		owl:unionOf (
			osdu:FrameOfReferenceUOM
			osdu:FrameOfReferenceCRS
			osdu:FrameOfReferenceDateTime
			osdu:FrameOfReferenceAzimuthReference
			osdu:CoordinateTransformation
			osdu:CoordinateReferenceSystem
			osdu:System
		) ;
	] ;
	xsd:pattern "^[\\\\w\\\\-\\\\.]+:[\\\\w\\\\-\\\\.]+:[\\\\w\\\\-\\\\.]+:[0-9]+.[0-9]+.[0-9]+$" ;
	rdfs:range xsd:string ;
.

###  https://w3id.org/osdu#labReferenceNumber
osdu:labReferenceNumber rdf:type owl:DatatypeProperty ;
	rdfs:comment "A reference number allowing traceability back to the analysis of the fluid in a lab " ;
	rdfs:domain osdu:FluidsInterval ;
	rdfs:range xsd:decimal ;
.

###  https://w3id.org/osdu#labSampleIdentifier
osdu:labSampleIdentifier rdf:type owl:DatatypeProperty ;
	rdfs:comment "The data vendor assigned sample ID or number. " ;
	rdfs:domain osdu:RockSample ;
	rdfs:range xsd:string ;
.

###  https://w3id.org/osdu#laboratoryName
osdu:laboratoryName rdf:type owl:DatatypeProperty ;
	rdfs:comment "Name or branch of the laboratory performing the analysis. " ;
	rdfs:domain osdu:RockSampleAnalysis ;
	rdfs:range xsd:string ;
.

###  https://w3id.org/osdu#lastAbandonDrillDate
osdu:lastAbandonDrillDate rdf:type owl:DatatypeProperty ;
	rdfs:comment "Last abandonment drill. " ;
	rdfs:domain osdu:HealthSafetyEnvironment ;
	rdfs:range time:DateTimeDescription ;
.

###  https://w3id.org/osdu#lastBopDrillDate
osdu:lastBopDrillDate rdf:type owl:DatatypeProperty ;
	rdfs:comment "Last blow out preventer drill. " ;
	rdfs:domain osdu:HealthSafetyEnvironment ;
	rdfs:range time:DateTimeDescription ;
.

###  https://w3id.org/osdu#lastBopPressureTestDate
osdu:lastBopPressureTestDate rdf:type owl:DatatypeProperty ;
	rdfs:comment "Last blow out preventer pressure test. " ;
	rdfs:domain osdu:HealthSafetyEnvironment ;
	rdfs:range time:DateTimeDescription ;
.

###  https://w3id.org/osdu#lastCMP
osdu:lastCMP rdf:type owl:DatatypeProperty ;
	rdfs:comment "Last Common Mid Point " ;
	rdfs:domain [
		rdf:type owl:Class ;
		owl:unionOf (
			osdu:SeismicTraceData
			osdu:SeismicLineGeometry
		) ;
	] ;
	rdfs:range xsd:decimal ;
.

###  https://w3id.org/osdu#lastCasingPressureTestDate
osdu:lastCasingPressureTestDate rdf:type owl:DatatypeProperty ;
	rdfs:comment "Last casing pressure test date and time. " ;
	rdfs:domain osdu:HealthSafetyEnvironment ;
	rdfs:range time:DateTimeDescription ;
.

###  https://w3id.org/osdu#lastDiverterDrillDate
osdu:lastDiverterDrillDate rdf:type owl:DatatypeProperty ;
	rdfs:comment "Last diverter drill. " ;
	rdfs:domain osdu:HealthSafetyEnvironment ;
	rdfs:range time:DateTimeDescription ;
.

###  https://w3id.org/osdu#lastFireBoatDrillDate
osdu:lastFireBoatDrillDate rdf:type owl:DatatypeProperty ;
	rdfs:comment "Last fire or life boat drill. " ;
	rdfs:domain osdu:HealthSafetyEnvironment ;
	rdfs:range time:DateTimeDescription ;
.

###  https://w3id.org/osdu#lastRigInspectionDate
osdu:lastRigInspectionDate rdf:type owl:DatatypeProperty ;
	rdfs:comment "Last rig inspection/check. " ;
	rdfs:domain osdu:HealthSafetyEnvironment ;
	rdfs:range time:DateTimeDescription ;
.

###  https://w3id.org/osdu#lastSafetyInspectionDate
osdu:lastSafetyInspectionDate rdf:type owl:DatatypeProperty ;
	rdfs:comment "Last safety inspection. " ;
	rdfs:domain osdu:HealthSafetyEnvironment ;
	rdfs:range time:DateTimeDescription ;
.

###  https://w3id.org/osdu#lastSafetyMeetingDate
osdu:lastSafetyMeetingDate rdf:type owl:DatatypeProperty ;
	rdfs:comment "Last safety meeting. " ;
	rdfs:domain osdu:HealthSafetyEnvironment ;
	rdfs:range time:DateTimeDescription ;
.

###  https://w3id.org/osdu#lastShotPoint
osdu:lastShotPoint rdf:type owl:DatatypeProperty ;
	rdfs:comment "The last shotpoint represented by the data " ;
	rdfs:domain osdu:SeismicTraceData ;
	rdfs:range xsd:decimal ;
.

###  https://w3id.org/osdu#lastStationLabel
osdu:lastStationLabel rdf:type owl:DatatypeProperty ;
	rdfs:comment "Station label (such as shot point name) corresponding to LastCMP " ;
	rdfs:domain osdu:SeismicLineGeometry ;
	rdfs:range xsd:string ;
.

###  https://w3id.org/osdu#lastSuccessfulRunDateUTC
osdu:lastSuccessfulRunDateUTC rdf:type owl:DatatypeProperty ;
	rdfs:comment "The last successful run date of the job (UTC) " ;
	rdfs:domain osdu:ConnectedSourceDataJob ;
	rdfs:range time:DateTimeDescription ;
.

###  https://w3id.org/osdu#lastTripDrillDate
osdu:lastTripDrillDate rdf:type owl:DatatypeProperty ;
	rdfs:comment "Last trip drill. " ;
	rdfs:domain osdu:HealthSafetyEnvironment ;
	rdfs:range time:DateTimeDescription ;
.

###  https://w3id.org/osdu#lcm
osdu:lcm rdf:type owl:DatatypeProperty ;
	rdfs:comment "Lost circulation material. " ;
	rdfs:domain osdu:Fluid ;
	rdfs:range xsd:decimal ;
.

###  https://w3id.org/osdu#leakOffPressure
osdu:leakOffPressure rdf:type owl:DatatypeProperty ;
	rdfs:comment "The pressure observed from the LeakOff " ;
	rdfs:domain osdu:FormationIntegrityEvaluation ;
	rdfs:range xsd:decimal ;
.

###  https://w3id.org/osdu#legalTags
osdu:legalTags rdf:type owl:DatatypeProperty ;
	rdfs:comment "The list of legal tags, which resolve to legal properties (like country of origin, export classification code, etc.) and rules with the help of the Compliance Service. " ;
	rdfs:domain osdu:AbstractLegalTags ;
	rdfs:range xsd:string ;
.

###  https://w3id.org/osdu#length
osdu:length rdf:type owl:DatatypeProperty ;
	rdfs:comment "The measured length of a target along the shortest side " ;
	rdfs:domain [
		rdf:type owl:Class ;
		owl:unionOf (
			osdu:Core
			osdu:Geometry
			osdu:SingleCellAquifer
		) ;
	] ;
	rdfs:range xsd:decimal ;
.

###  https://w3id.org/osdu#lengthRadius
osdu:lengthRadius rdf:type owl:DatatypeProperty ;
	rdfs:comment "Length of straight line section or radius of arc for continuous curve section. " ;
	rdfs:domain osdu:GeometrySection ;
	rdfs:range xsd:decimal ;
.

###  https://w3id.org/osdu#licenceName
osdu:licenceName rdf:type owl:DatatypeProperty ;
	rdfs:comment "Legal name of the well as described within the Licence " ;
	rdfs:domain osdu:WellPlanningWell ;
	rdfs:range xsd:string ;
.

###  https://w3id.org/osdu#licenceNumber
osdu:licenceNumber rdf:type owl:DatatypeProperty ;
	rdfs:comment "License number of the well " ;
	rdfs:domain osdu:WellPlanningWell ;
	rdfs:range xsd:string ;
.

###  https://w3id.org/osdu#lifecyclePhaseID
osdu:lifecyclePhaseID rdf:type owl:DatatypeProperty ;
	rdfs:comment "The Lifecycle Phase [Facility State Type] permitted in this summary category. " ;
	rdfs:domain osdu:WellStatusSummary ;
	xsd:pattern "^[\\\\w\\\\-\\\\.]+:reference-data\\\\-\\\\-FacilityStateType:[\\\\w\\\\-\\\\.\\\\:\\\\%]+:[0-9]*$" ;
	rdfs:range xsd:string ;
.

###  https://w3id.org/osdu#lime
osdu:lime rdf:type owl:DatatypeProperty ;
	rdfs:comment "Lime content. " ;
	rdfs:domain osdu:Fluid ;
	rdfs:range xsd:decimal ;
.

###  https://w3id.org/osdu#limitRecords
osdu:limitRecords rdf:type owl:DatatypeProperty ;
	rdfs:comment "The maximum number of records to be processed in this job. " ;
	rdfs:domain osdu:ConnectedSourceDataJob ;
	rdfs:range xsd:integer ;
.

###  https://w3id.org/osdu#lineNames
osdu:lineNames rdf:type owl:DatatypeProperty ;
	rdfs:comment "Segment names and aliases for the Line. " ;
	rdfs:domain osdu:NotionalSeismicLine ;
	rdfs:range xsd:string ;
.

###  https://w3id.org/osdu#lineageRelationshipType
osdu:lineageRelationshipType rdf:type owl:DatatypeProperty ;
	rdfs:comment "Used by LineageAssertion to describe the nature of the line of descent of a work  from a prior Resource, such as DIRECT, INDIRECT, REFERENCE.  It is not for proximity (number of nodes away), it is not to cover all the relationships in a full ontology or graph, and it is not to describe the type of activity that created the asserting WPC.  LineageAssertion does not encompass a full provenance, process history, or activity model. " ;
	rdfs:domain osdu:LineageAssertion ;
	xsd:pattern "^[\\\\w\\\\-\\\\.]+:reference-data\\\\-\\\\-LineageRelationshipType:[\\\\w\\\\-\\\\.\\\\:\\\\%]+:[0-9]*$" ;
	rdfs:range xsd:string ;
.

###  https://w3id.org/osdu#linerInnerDiameter
osdu:linerInnerDiameter rdf:type owl:DatatypeProperty ;
	rdfs:comment "Liner inside diameter. " ;
	rdfs:domain osdu:PumpOperations ;
	rdfs:range xsd:decimal ;
.

###  https://w3id.org/osdu#linerTypeID
osdu:linerTypeID rdf:type owl:DatatypeProperty ;
	rdfs:comment "This reference table describes the type of liner used in the borehole. For example, slotted, gravel packed or pre-perforated etc. " ;
	rdfs:domain osdu:TubularAssembly ;
	xsd:pattern "^[\\\\w\\\\-\\\\.]+:reference-data\\\\-\\\\-LinerType:[\\\\w\\\\-\\\\.\\\\:\\\\%]+:[0-9]*$" ;
	rdfs:range xsd:string ;
.

###  https://w3id.org/osdu#lithology
osdu:lithology rdf:type owl:DatatypeProperty ;
	rdfs:comment "Description of the lithology for the interval. " ;
	rdfs:domain osdu:OperationsReport ;
	rdfs:range xsd:string ;
.

###  https://w3id.org/osdu#lithologyTypeID
osdu:lithologyTypeID rdf:type owl:DatatypeProperty ;
	rdfs:comment "The ID for a LithologyType" ;
	rdfs:domain [
		rdf:type owl:Class ;
		owl:unionOf (
			osdu:AbstractGeologicUnitInterpretation
			osdu:GeologyInterval
		) ;
	] ;
	xsd:pattern "^[\\\\w\\\\-\\\\.]+:reference-data\\\\-\\\\-LithologyType:[\\\\w\\\\-\\\\.\\\\:\\\\%]+:[0-9]*$" ;
	rdfs:range xsd:string ;
.

###  https://w3id.org/osdu#lithostratigraphicID
osdu:lithostratigraphicID rdf:type owl:DatatypeProperty ;
	rdfs:comment "Name of lithostratigraphy, regionally dependent. " ;
	rdfs:domain osdu:GeologyInterval ;
	xsd:pattern "^[\\\\w\\\\-\\\\.]+:reference-data\\\\-\\\\-LithoStratigraphy:[\\\\w\\\\-\\\\.\\\\:\\\\%]+:[0-9]*$" ;
	rdfs:range xsd:string ;
.

###  https://w3id.org/osdu#localModelCompoundCrsID
osdu:localModelCompoundCrsID rdf:type owl:DatatypeProperty ;
	rdfs:comment "Allow to link a local CRS with this representation " ;
	rdfs:domain osdu:AbstractRepresentation ;
	xsd:pattern "^[\\\\w\\\\-\\\\.]+:work-product-component\\\\-\\\\-LocalModelCompoundCrs:[\\\\w\\\\-\\\\.\\\\:\\\\%]+:[0-9]*$" ;
	rdfs:range xsd:string ;
.

###  https://w3id.org/osdu#locationDescription
osdu:locationDescription rdf:type owl:DatatypeProperty ;
	rdfs:comment "Location description. " ;
	rdfs:domain osdu:Incident ;
	rdfs:range xsd:string ;
.

###  https://w3id.org/osdu#logActivity
osdu:logActivity rdf:type owl:DatatypeProperty ;
	rdfs:comment "Log Activity, used to describe the type of pass such as Calibration Pass - Main Pass - Repeated Pass " ;
	rdfs:domain osdu:WellLog ;
	rdfs:range xsd:string ;
.

###  https://w3id.org/osdu#logCurveBusinessValueID
osdu:logCurveBusinessValueID rdf:type owl:DatatypeProperty ;
	rdfs:comment "The related record id of the Log Curve Business Value Type. " ;
	rdfs:domain osdu:Curves ;
	xsd:pattern "^[\\\\w\\\\-\\\\.]+:reference-data\\\\-\\\\-LogCurveBusinessValue:[\\\\w\\\\-\\\\.\\\\:\\\\%]+:[0-9]*$" ;
	rdfs:range xsd:string ;
.

###  https://w3id.org/osdu#logCurveFamilyID
osdu:logCurveFamilyID rdf:type owl:DatatypeProperty ;
	rdfs:comment "The related record id of the Log Curve Family - which is the detailed Geological Physical Quantity Measured - such as neutron porosity " ;
	rdfs:domain osdu:Curves ;
	xsd:pattern "^[\\\\w\\\\-\\\\.]+:reference-data\\\\-\\\\-LogCurveFamily:[\\\\w\\\\-\\\\.\\\\:\\\\%]+:[0-9]*$" ;
	rdfs:range xsd:string ;
.

###  https://w3id.org/osdu#logCurveMainFamilyID
osdu:logCurveMainFamilyID rdf:type owl:DatatypeProperty ;
	rdfs:comment "The related record id of the Log Curve Main Family Type - which is the Geological Physical Quantity measured - such as porosity. " ;
	rdfs:domain osdu:Curves ;
	xsd:pattern "^[\\\\w\\\\-\\\\.]+:reference-data\\\\-\\\\-LogCurveMainFamily:[\\\\w\\\\-\\\\.\\\\:\\\\%]+:[0-9]*$" ;
	rdfs:range xsd:string ;
.

###  https://w3id.org/osdu#logCurveTypeID
osdu:logCurveTypeID rdf:type owl:DatatypeProperty ;
	rdfs:comment "The related record id of the Log Curve Type - which is the standard mnemonic chosen by the company - OSDU provides an initial list " ;
	rdfs:domain osdu:Curves ;
	xsd:pattern "^[\\\\w\\\\-\\\\.]+:reference-data\\\\-\\\\-LogCurveType:[\\\\w\\\\-\\\\.\\\\:\\\\%]+:[0-9]*$" ;
	rdfs:range xsd:string ;
.

###  https://w3id.org/osdu#logRemark
osdu:logRemark rdf:type owl:DatatypeProperty ;
	rdfs:comment "Log remark provides contextual information during the actual log object acquisition. Explains how the measurement in the wellbore is taken on a point in time or depth. Additional information may be included such as bad weather, tool failure, etc. Usually a part of the log header, log remark contains info specific for an acquisition run, specific for a given logging tool (multiple measurements) and/or a specific interval. In essence, log remark represents the external factors and operational environment, directly or indirectly affecting the measurement quality/uncertainty (dynamically over time/depth) - adding both noise and bias to the measurements. " ;
	rdfs:domain osdu:WellLog ;
	rdfs:range xsd:string ;
.

###  https://w3id.org/osdu#logRun
osdu:logRun rdf:type owl:DatatypeProperty ;
	rdfs:comment "Log Run - describe the run of the log - can be a number, but may be also a alphanumeric description such as a version name " ;
	rdfs:domain osdu:WellLog ;
	rdfs:range xsd:string ;
.

###  https://w3id.org/osdu#logSource
osdu:logSource rdf:type owl:DatatypeProperty ;
	rdfs:comment "OSDU Native Log Source - will be updated for later releases - not to be used yet " ;
	rdfs:domain osdu:WellLog ;
	rdfs:range xsd:string ;
.

###  https://w3id.org/osdu#logVersion
osdu:logVersion rdf:type owl:DatatypeProperty ;
	rdfs:comment "Log Version " ;
	rdfs:domain osdu:WellLog ;
	rdfs:range xsd:string ;
.

###  https://w3id.org/osdu#loggingDirection
osdu:loggingDirection rdf:type owl:DatatypeProperty ;
	rdfs:comment "Specifies whether curves were collected downward or upward " ;
	rdfs:domain osdu:WellLog ;
	rdfs:range xsd:string ;
.

###  https://w3id.org/osdu#loggingService
osdu:loggingService rdf:type owl:DatatypeProperty ;
	rdfs:comment "Logging Service - mainly a short concatenation of the names of the tools " ;
	rdfs:domain osdu:WellLog ;
	rdfs:range xsd:string ;
.

###  https://w3id.org/osdu#lossyCompressionIndicator
osdu:lossyCompressionIndicator rdf:type owl:DatatypeProperty ;
	rdfs:comment "Boolean that warns that an imperfect compression algorithm has been applied to the bulk binary data.  Details of the compression method need to be discovered from the format properties and file access methods. " ;
	rdfs:domain osdu:AbstractCompressionInfo ;
	rdfs:range xsd:boolean ;
.

###  https://w3id.org/osdu#lowShearYieldPoint
osdu:lowShearYieldPoint rdf:type owl:DatatypeProperty ;
	rdfs:comment "Shearing capacity of mud at low velocity " ;
	rdfs:domain osdu:Fluid ;
	rdfs:range xsd:decimal ;
.

###  https://w3id.org/osdu#lowerI
osdu:lowerI rdf:type owl:DatatypeProperty ;
	rdfs:comment "The lower included I index of the box of the grid in connection " ;
	rdfs:domain osdu:AbstractIjkGridFlowSimulationBoundaryConnection ;
	rdfs:range xsd:integer ;
.

###  https://w3id.org/osdu#lowerJ
osdu:lowerJ rdf:type owl:DatatypeProperty ;
	rdfs:comment "The lower included J index of the box of the grid in connection " ;
	rdfs:domain osdu:AbstractIjkGridFlowSimulationBoundaryConnection ;
	rdfs:range xsd:integer ;
.

###  https://w3id.org/osdu#lowerK
osdu:lowerK rdf:type owl:DatatypeProperty ;
	rdfs:comment "The lower included K index of the box of the grid in connection " ;
	rdfs:domain osdu:AbstractIjkGridFlowSimulationBoundaryConnection ;
	rdfs:range xsd:integer ;
.

###  https://w3id.org/osdu#maasp
osdu:maasp rdf:type owl:DatatypeProperty ;
	rdfs:comment "Maximum allowable shut-in casing pressure. " ;
	rdfs:domain [
		rdf:type owl:Class ;
		owl:unionOf (
			osdu:Phase
			osdu:DrillingReportStatusInfo
		) ;
	] ;
	rdfs:range xsd:decimal ;
.

###  https://w3id.org/osdu#mppPressure
osdu:mppPressure rdf:type owl:DatatypeProperty ;
	rdfs:comment "Mid point perf pressure " ;
	rdfs:domain osdu:PerforationInterval ;
	rdfs:range xsd:decimal ;
.

###  https://w3id.org/osdu#magnesium
osdu:magnesium rdf:type owl:DatatypeProperty ;
	rdfs:comment "Magnesium content. " ;
	rdfs:domain osdu:Fluid ;
	rdfs:range xsd:decimal ;
.

###  https://w3id.org/osdu#majorAxis
osdu:majorAxis rdf:type owl:DatatypeProperty ;
	rdfs:comment "Measured length of the target along Target Ref Azimuth " ;
	rdfs:domain osdu:Geometry ;
	rdfs:range xsd:decimal ;
.

###  https://w3id.org/osdu#manufacturer
osdu:manufacturer rdf:type owl:DatatypeProperty ;
	rdfs:comment "Manufacturer / supplier of the item. " ;
	rdfs:domain osdu:BitRecord ;
	rdfs:range xsd:string ;
.

###  https://w3id.org/osdu#manufacturerID
osdu:manufacturerID rdf:type owl:DatatypeProperty ;
	rdfs:comment "Unique identifier for the manufacturer of this equipment. " ;
	rdfs:domain osdu:TubularComponent ;
	xsd:pattern "^[\\\\w\\\\-\\\\.]+:master-data\\\\-\\\\-Organisation:[\\\\w\\\\-\\\\.\\\\:\\\\%]+:[0-9]*$" ;
	rdfs:range xsd:string ;
.

###  https://w3id.org/osdu#mapStateID
osdu:mapStateID rdf:type owl:DatatypeProperty ;
	rdfs:comment "The mapping status declaring whether the mapping is straight forward, direct (identical) or whether special treatment is required (corrected). Items, which are known not to be mappable are declared as unsupported." ;
	rdfs:domain [
		rdf:type owl:Class ;
		owl:unionOf (
			osdu:ExternalUnitOfMeasure
			osdu:ExternalUnitQuantity
		) ;
	] ;
	xsd:pattern "^[\\\\w\\\\-\\\\.]+:reference-data\\\\-\\\\-CatalogMapStateType:[\\\\w\\\\-\\\\.\\\\:\\\\%]+:[0-9]*$" ;
	rdfs:range xsd:string ;
.

###  https://w3id.org/osdu#markerDate
osdu:markerDate rdf:type owl:DatatypeProperty ;
	rdfs:comment "Timestamp of the date and time when the when the Marker was interpreted. " ;
	rdfs:domain osdu:Markers ;
	rdfs:range time:DateTimeDescription ;
.

###  https://w3id.org/osdu#markerID
osdu:markerID rdf:type owl:DatatypeProperty ;
	rdfs:comment "A unique identifier of the marker in the list of data.Markers[], ideally a UUID. If unpopulated, the string-converted element index number is used. The first index is 0. " ;
	rdfs:domain osdu:Markers ;
	rdfs:range xsd:string ;
.

###  https://w3id.org/osdu#markerInterpreter
osdu:markerInterpreter rdf:type owl:DatatypeProperty ;
	rdfs:comment "The name of the Marker interpreter (could be a person or vendor). " ;
	rdfs:domain osdu:Markers ;
	rdfs:range xsd:string ;
.

###  https://w3id.org/osdu#markerMeasuredDepth
osdu:markerMeasuredDepth rdf:type owl:DatatypeProperty ;
	rdfs:comment "The depth at which the Marker was noted. " ;
	rdfs:domain osdu:Markers ;
	rdfs:range xsd:decimal ;
.

###  https://w3id.org/osdu#markerName
osdu:markerName rdf:type owl:DatatypeProperty ;
	rdfs:comment "Name of the Marker " ;
	rdfs:domain osdu:Markers ;
	rdfs:range xsd:string ;
.

###  https://w3id.org/osdu#markerObservationNumber
osdu:markerObservationNumber rdf:type owl:DatatypeProperty ;
	rdfs:comment "Any observation number that distinguishes a Marker observation from others with same Marker name, date. " ;
	rdfs:domain osdu:Markers ;
	rdfs:range xsd:decimal ;
.

###  https://w3id.org/osdu#markerPropertyTypeID
osdu:markerPropertyTypeID rdf:type owl:DatatypeProperty ;
	rdfs:comment "The reference to a marker property type - or if interpreted as CSV columns, the 'well-known column type. It is a relationship to a reference-data--MarkerPropertyType record id. " ;
	rdfs:domain osdu:MarkerProperty ;
	xsd:pattern "^[\\\\w\\\\-\\\\.]+:reference-data\\\\-\\\\-MarkerPropertyType:[\\\\w\\\\-\\\\.\\\\:\\\\%]+:[0-9]*$" ;
	rdfs:range xsd:string ;
.

###  https://w3id.org/osdu#markerPropertyUnitID
osdu:markerPropertyUnitID rdf:type owl:DatatypeProperty ;
	rdfs:comment "Unit of Measure for the marker properties of type MarkerPropertyType. " ;
	rdfs:domain osdu:MarkerProperty ;
	xsd:pattern "^[\\\\w\\\\-\\\\.]+:reference-data\\\\-\\\\-UnitOfMeasure:[\\\\w\\\\-\\\\.\\\\:\\\\%]+:[0-9]*$" ;
	rdfs:range xsd:string ;
.

###  https://w3id.org/osdu#markerSetCollectionID
osdu:markerSetCollectionID rdf:type owl:DatatypeProperty ;
	rdfs:comment "List of marker set where horizon, fault and geo-boundary markers from different wellbores (potentially the result of a query) are used as input for the structural model. " ;
	rdfs:domain osdu:UnsealedSurfaceFramework ;
	xsd:pattern "^[\\\\w\\\\-\\\\.]+:work-product-component\\\\-\\\\-PersistedCollection:[\\\\w\\\\-\\\\.\\\\:\\\\%]+:[0-9]*$" ;
	rdfs:range xsd:string ;
.

###  https://w3id.org/osdu#markerSubSeaVerticalDepth
osdu:markerSubSeaVerticalDepth rdf:type owl:DatatypeProperty ;
	rdfs:comment "The Marker's TVD converted to a Sub-Sea Vertical depth, i.e., below Mean Sea Level. Note that TVD values above MSL are negative. This is the same as true vertical depth referenced to the vertical CRS “MSL depth”. " ;
	rdfs:domain osdu:Markers ;
	rdfs:range xsd:decimal ;
.

###  https://w3id.org/osdu#markerTypeID
osdu:markerTypeID rdf:type owl:DatatypeProperty ;
	rdfs:comment "Marker Type Reference Type. Possible values - Biostratigraphy, Lithostratigraphy, seismic, depth of well, sequence, flow unit " ;
	rdfs:domain osdu:Markers ;
	xsd:pattern "^[\\\\w\\\\-\\\\.]+:reference-data\\\\-\\\\-MarkerType:[\\\\w\\\\-\\\\.\\\\:\\\\%]+:[0-9]*$" ;
	rdfs:range xsd:string ;
.

###  https://w3id.org/osdu#maxAllowedAbsoluteDecline
osdu:maxAllowedAbsoluteDecline rdf:type owl:DatatypeProperty ;
	rdfs:comment "the maximum allowable pressure loss for a pressure decline test (expressed as an absolute value) " ;
	rdfs:domain osdu:PressureCriteria ;
	rdfs:range xsd:decimal ;
.

###  https://w3id.org/osdu#maxAllowedPercentageDecline
osdu:maxAllowedPercentageDecline rdf:type owl:DatatypeProperty ;
	rdfs:comment "the maximum allowable pressure loss for a pressure decline test (expressed as a percentage of test pressure) " ;
	rdfs:domain osdu:PressureCriteria ;
	rdfs:range xsd:decimal ;
.

###  https://w3id.org/osdu#maxAllowedRateOfChange
osdu:maxAllowedRateOfChange rdf:type owl:DatatypeProperty ;
	rdfs:comment "Criteria pressure rate of change for a flat-line test. Averaged over the duration of  the Validation Duration " ;
	rdfs:domain osdu:PressureCriteria ;
	rdfs:range xsd:decimal ;
.

###  https://w3id.org/osdu#maxOccurs
osdu:maxOccurs rdf:type owl:DatatypeProperty ;
	rdfs:comment "Maximum number of parameters of this type allowed in the activity. If the maximum number of parameters is infinite, use -1 value. " ;
	rdfs:domain osdu:ParameterTemplate ;
	rdfs:range xsd:integer ;
.

###  https://w3id.org/osdu#maxOffsetDistance
osdu:maxOffsetDistance rdf:type owl:DatatypeProperty ;
	rdfs:comment "Horizontal distance between source and last receiver. " ;
	rdfs:domain osdu:SeismicAcquisitionSurvey ;
	rdfs:range xsd:decimal ;
.

###  https://w3id.org/osdu#maxPower
osdu:maxPower rdf:type owl:DatatypeProperty ;
	rdfs:comment "Maximum power defined by the manufacturer. " ;
	rdfs:domain osdu:MudPump ;
	rdfs:range xsd:decimal ;
.

###  https://w3id.org/osdu#maxPumpFlowrate
osdu:maxPumpFlowrate rdf:type owl:DatatypeProperty ;
	rdfs:comment "Maximum required/delivered flowrate from/by the pump " ;
	rdfs:domain osdu:MudPump ;
	rdfs:range xsd:decimal ;
.

###  https://w3id.org/osdu#maxPumpPressure
osdu:maxPumpPressure rdf:type owl:DatatypeProperty ;
	rdfs:comment "Maximum required/delivered pressure from/by the pump " ;
	rdfs:domain osdu:MudPump ;
	rdfs:range xsd:decimal ;
.

###  https://w3id.org/osdu#maxTestPressureAtSurface
osdu:maxTestPressureAtSurface rdf:type owl:DatatypeProperty ;
	rdfs:comment "The maximum pressure observed at the surface during the test. " ;
	rdfs:domain osdu:FormationIntegrityEvaluation ;
	rdfs:range xsd:decimal ;
.

###  https://w3id.org/osdu#maxValue
osdu:maxValue rdf:type owl:DatatypeProperty ;
	rdfs:comment "Maximum value of the Property " ;
	rdfs:domain osdu:GenericProperty ;
	rdfs:range xsd:decimal ;
.

###  https://w3id.org/osdu#maxWaterDepth
osdu:maxWaterDepth rdf:type owl:DatatypeProperty ;
	rdfs:comment "Required maximum workable water depth for the rig. " ;
	rdfs:domain osdu:RigUtilization ;
	rdfs:range xsd:decimal ;
.

###  https://w3id.org/osdu#maximum
osdu:maximum rdf:type owl:DatatypeProperty ;
	rdfs:comment "The maximum value. " ;
	rdfs:domain [
		rdf:type owl:Class ;
		owl:unionOf (
			osdu:AngleRange
			osdu:LengthRange
		) ;
	] ;
	rdfs:range xsd:decimal ;
.

###  https://w3id.org/osdu#maximumAge
osdu:maximumAge rdf:type owl:DatatypeProperty ;
	rdfs:comment "Time interval Maximum age the fault throw was active - if the link to horizon is defined, we can derive the link to horizons through geologic age " ;
	rdfs:domain osdu:FaultThrowDescriptions ;
	rdfs:range time:TemporalDuration ;
.

###  https://w3id.org/osdu#maximumBitFlowrate
osdu:maximumBitFlowrate rdf:type owl:DatatypeProperty ;
	rdfs:comment "The maximum flowrate at the bit during the run " ;
	rdfs:domain osdu:DrillingParameters ;
	rdfs:range xsd:decimal ;
.

###  https://w3id.org/osdu#maximumDepthTestStart
osdu:maximumDepthTestStart rdf:type owl:DatatypeProperty ;
	rdfs:comment "The maximum start depth for the drillstem test. Depth relative to Planned wellbore ZDP. Navigate via WellboreID to the side-car WellPlanningWellbore, which holds the depth reference in data.VerticalMeasurement. " ;
	rdfs:domain osdu:DSTRun ;
	rdfs:range xsd:decimal ;
.

###  https://w3id.org/osdu#maximumDogleg
osdu:maximumDogleg rdf:type owl:DatatypeProperty ;
	rdfs:comment "Dogleg severity - Maximum. " ;
	rdfs:domain osdu:BHARun ;
	rdfs:range xsd:decimal ;
.

###  https://w3id.org/osdu#maximumFaultThrowValue
osdu:maximumFaultThrowValue rdf:type owl:DatatypeProperty ;
	rdfs:comment "Indicates the maximum current fault throw value " ;
	rdfs:domain osdu:FaultInterpretation ;
	rdfs:range xsd:decimal ;
.

###  https://w3id.org/osdu#maximumFlowratePump
osdu:maximumFlowratePump rdf:type owl:DatatypeProperty ;
	rdfs:comment "Maximum mud pump flow rate. " ;
	rdfs:domain osdu:DrillingParameters ;
	rdfs:range xsd:decimal ;
.

###  https://w3id.org/osdu#maximumInclination
osdu:maximumInclination rdf:type owl:DatatypeProperty ;
	rdfs:comment "Maximum inclination. " ;
	rdfs:domain osdu:DrillingParameters ;
	rdfs:range xsd:decimal ;
.

###  https://w3id.org/osdu#maximumMudTemperatureDownhole
osdu:maximumMudTemperatureDownhole rdf:type owl:DatatypeProperty ;
	rdfs:comment "Maximum mud temperature downhole during run. " ;
	rdfs:domain osdu:DrillingParameters ;
	rdfs:range xsd:decimal ;
.

###  https://w3id.org/osdu#maximumOuterDiameter
osdu:maximumOuterDiameter rdf:type owl:DatatypeProperty ;
	rdfs:comment "This is the maximum outer diameter of the component. " ;
	rdfs:domain osdu:TubularComponent ;
	rdfs:range xsd:decimal ;
.

###  https://w3id.org/osdu#maximumPumpPressure
osdu:maximumPumpPressure rdf:type owl:DatatypeProperty ;
	rdfs:comment "The maximum pump pressure used during the run " ;
	rdfs:domain osdu:DrillingParameters ;
	rdfs:range xsd:decimal ;
.

###  https://w3id.org/osdu#maximumROP
osdu:maximumROP rdf:type owl:DatatypeProperty ;
	rdfs:comment "Maximum rate of penetration through Interval. " ;
	rdfs:domain osdu:DrillingParameters ;
	rdfs:range xsd:decimal ;
.

###  https://w3id.org/osdu#maximumRpm
osdu:maximumRpm rdf:type owl:DatatypeProperty ;
	rdfs:comment "Maximum turn rate (commonly in rpm). " ;
	rdfs:domain osdu:DrillingParameters ;
	rdfs:range xsd:decimal ;
.

###  https://w3id.org/osdu#maximumThickness
osdu:maximumThickness rdf:type owl:DatatypeProperty ;
	rdfs:comment "The maximum thickness of the StratigraphicUnitInterpretation. " ;
	rdfs:domain osdu:StratigraphicUnitInterpretation ;
	rdfs:range xsd:decimal ;
.

###  https://w3id.org/osdu#maximumTorqueOnBottom
osdu:maximumTorqueOnBottom rdf:type owl:DatatypeProperty ;
	rdfs:comment "Maximum torque: on bottom. " ;
	rdfs:domain osdu:DrillingParameters ;
	rdfs:range xsd:decimal ;
.

###  https://w3id.org/osdu#maximumVolume
osdu:maximumVolume rdf:type owl:DatatypeProperty ;
	rdfs:comment "Maximum expected volume pumped at specified pressure " ;
	rdfs:domain osdu:ExpectedVolume ;
	rdfs:range xsd:decimal ;
.

###  https://w3id.org/osdu#maximumWOB
osdu:maximumWOB rdf:type owl:DatatypeProperty ;
	rdfs:comment "Weight on bit - maximum. " ;
	rdfs:domain osdu:DrillingParameters ;
	rdfs:range xsd:decimal ;
.

###  https://w3id.org/osdu#mbt
osdu:mbt rdf:type owl:DatatypeProperty ;
	rdfs:comment "Cation exchange capacity (CEC) of the mud sample as measured by methylene blue titration (MBT).  NOTE: This is temporarily set to be a GenericMeasure with no unit validation, pending addition of CEC units to the Energistics UoM spec. " ;
	rdfs:domain osdu:Fluid ;
	rdfs:range xsd:decimal ;
.

###  https://w3id.org/osdu#mdPlanned
osdu:mdPlanned rdf:type owl:DatatypeProperty ;
	rdfs:comment "The measured depth planned to be reached. " ;
	rdfs:domain osdu:DrillingReportStatusInfo ;
	rdfs:range xsd:decimal ;
.

###  https://w3id.org/osdu#meanPressure
osdu:meanPressure rdf:type owl:DatatypeProperty ;
	rdfs:comment "The average pressure in which the gas permeability has been measured. " ;
	rdfs:domain osdu:Conditions ;
	rdfs:range xsd:decimal ;
.

###  https://w3id.org/osdu#meanValue
osdu:meanValue rdf:type owl:DatatypeProperty ;
	rdfs:comment "Mean value of the Property " ;
	rdfs:domain osdu:GenericProperty ;
	rdfs:range xsd:decimal ;
.

###  https://w3id.org/osdu#measurePointDensity
osdu:measurePointDensity rdf:type owl:DatatypeProperty ;
	rdfs:comment "Density of measured points in unit of measure. Must be the same unit as the Image Area. Interdependent with image area and number of measured points " ;
	rdfs:domain osdu:ProcessedInSAR ;
	rdfs:range xsd:decimal ;
.

###  https://w3id.org/osdu#measuredDepth
osdu:measuredDepth rdf:type owl:DatatypeProperty ;
	rdfs:comment "The measured depth to the activity/object. " ;
	rdfs:domain [
		rdf:type owl:Class ;
		owl:unionOf (
			osdu:Fluid
			osdu:DrillingActivity
		) ;
	] ;
	rdfs:range xsd:decimal ;
.

###  https://w3id.org/osdu#measuredDepthBase
osdu:measuredDepthBase rdf:type owl:DatatypeProperty ;
	rdfs:comment "The measured depth at the base object " ;
	rdfs:domain [
		rdf:type owl:Class ;
		owl:unionOf (
			osdu:Core
			osdu:InstalledTubular
			osdu:HoleSection
			osdu:PlannedLithology
		) ;
	] ;
	rdfs:range xsd:decimal ;
.

###  https://w3id.org/osdu#measuredDepthBit
osdu:measuredDepthBit rdf:type owl:DatatypeProperty ;
	rdfs:comment "Along-hole measured depth of the measurement from the drill datum. " ;
	rdfs:domain osdu:PumpOperations ;
	rdfs:range xsd:decimal ;
.

###  https://w3id.org/osdu#measuredDepthCasingShoe
osdu:measuredDepthCasingShoe rdf:type owl:DatatypeProperty ;
	rdfs:comment "The measured depth of the Casing Shoe during this evaluation. Depth relative to Planned wellbore ZDP. Navigate via WellboreID to the side-car WellPlanningWellbore, which holds the depth reference in data.VerticalMeasurement. " ;
	rdfs:domain osdu:FormationIntegrityEvaluation ;
	rdfs:range xsd:decimal ;
.

###  https://w3id.org/osdu#measuredDepthErrorBase
osdu:measuredDepthErrorBase rdf:type owl:DatatypeProperty ;
	rdfs:comment "The  error associated with the measured depth at the base of the tubular " ;
	rdfs:domain osdu:InstalledTubular ;
	rdfs:range xsd:decimal ;
.

###  https://w3id.org/osdu#measuredDepthErrorTop
osdu:measuredDepthErrorTop rdf:type owl:DatatypeProperty ;
	rdfs:comment "The error associated with the measured depth at the top of the tubular " ;
	rdfs:domain osdu:InstalledTubular ;
	rdfs:range xsd:decimal ;
.

###  https://w3id.org/osdu#measuredDepthRunStart
osdu:measuredDepthRunStart rdf:type owl:DatatypeProperty ;
	rdfs:comment "Measured depth at run start. Depth relative to Planned wellbore ZDP. Navigate via WellboreID to the side-car WellPlanningWellbore, which holds the depth reference in data.VerticalMeasurement. " ;
	rdfs:domain osdu:BHARun ;
	rdfs:range xsd:decimal ;
.

###  https://w3id.org/osdu#measuredDepthRunStop
osdu:measuredDepthRunStop rdf:type owl:DatatypeProperty ;
	rdfs:comment "Measured depth at run stop. Depth relative to Planned wellbore ZDP. Navigate via WellboreID to the side-car WellPlanningWellbore, which holds the depth reference in data.VerticalMeasurement. " ;
	rdfs:domain osdu:BHARun ;
	rdfs:range xsd:decimal ;
.

###  https://w3id.org/osdu#measuredDepthTop
osdu:measuredDepthTop rdf:type owl:DatatypeProperty ;
	rdfs:comment "The measured depth at the top" ;
	rdfs:domain [
		rdf:type owl:Class ;
		owl:unionOf (
			osdu:Core
			osdu:InstalledTubular
			osdu:HoleSection
			osdu:PlannedLithology
		) ;
	] ;
	rdfs:range xsd:decimal ;
.

###  https://w3id.org/osdu#measuredPoints
osdu:measuredPoints rdf:type owl:DatatypeProperty ;
	rdfs:comment "Number of measured points in an Image Area. Interdependent with Image Area and Measure Point density. " ;
	rdfs:domain osdu:ProcessedInSAR ;
	rdfs:range xsd:integer ;
.

###  https://w3id.org/osdu#measuredPropertyID
osdu:measuredPropertyID rdf:type owl:DatatypeProperty ;
	rdfs:comment "The unique identifier of the fluid property (density or temperature measurement,….) " ;
	rdfs:domain osdu:FluidFacet ;
	xsd:pattern "^[\\\\w\\\\-\\\\.]+:reference-data\\\\-\\\\-UnitQuantity:[\\\\w\\\\-\\\\.\\\\:\\\\%]+:[0-9]*$" ;
	rdfs:range xsd:string ;
.

###  https://w3id.org/osdu#memberIDs
osdu:memberIDs rdf:type owl:DatatypeProperty ;
	rdfs:comment "List of objects which are part of a collection, defined as an array of the member IDs " ;
	rdfs:domain [
		rdf:type owl:Class ;
		owl:unionOf (
			osdu:RockFluidOrganizationInterpretation
			osdu:VoidageGroupInterpretation
			osdu:PersistedCollection
		) ;
	] ;
	xsd:pattern "^[\\\\w\\\\-\\\\.]+:work-product-component\\\\-\\\\-RockFluidUnitInterpretation:[\\\\w\\\\-\\\\.\\\\:\\\\%]+:[0-9]*$" ;
	xsd:pattern "^[\\\\w\\\\-\\\\.]+:work-product-component\\\\-\\\\-ReservoirCompartmentInterpretation:[\\\\w\\\\-\\\\.\\\\:\\\\%]+:[0-9]*$" ;
	xsd:pattern "^[\\\\w\\\\-\\\\.]+:(master-data\\\\-\\\\-[\\\\w\\\\-\\\\.]+|reference-data\\\\-\\\\-[\\\\w\\\\-\\\\.]+|work-product-component\\\\-\\\\-[\\\\w\\\\-\\\\.]+|work-product\\\\-\\\\-[\\\\w\\\\-\\\\.]+):[\\\\w\\\\-\\\\.\\\\:\\\\%]+:[0-9]*$" ;
	rdfs:range xsd:string ;
.

###  https://w3id.org/osdu#memberUnits
osdu:memberUnits rdf:type owl:DatatypeProperty ;
	rdfs:comment "Specifies the symbol of a unit of which is a member of this class. Membership indicates that a value of that class can be converted to any other member unit of that class without loss of semantics. This because the conversion formula represents a unitless factor of one. " ;
	rdfs:domain [
		rdf:type owl:Class ;
		owl:unionOf (
			osdu:UnitQuantity
			osdu:ExternalUnitQuantity
		) ;
	] ;
	rdfs:range xsd:string ;
.

###  https://w3id.org/osdu#metadataAdditionalPropertiesTrue
osdu:metadataAdditionalPropertiesTrue rdf:type owl:DatatypeProperty ;
	rdfs:comment "The count of total number of additional properties that are not populated. " ;
	rdfs:domain osdu:AbstractQualityMetric ;
	rdfs:range xsd:decimal ;
.

###  https://w3id.org/osdu#metadataCountAdditionalProperty
osdu:metadataCountAdditionalProperty rdf:type owl:DatatypeProperty ;
	rdfs:comment "Total number of additional properties. " ;
	rdfs:domain osdu:AbstractQualityMetric ;
	rdfs:range xsd:decimal ;
.

###  https://w3id.org/osdu#metadataCountFormat
osdu:metadataCountFormat rdf:type owl:DatatypeProperty ;
	rdfs:comment "Total number of attributes defined in reference value lists. " ;
	rdfs:domain osdu:AbstractQualityMetric ;
	rdfs:range xsd:decimal ;
.

###  https://w3id.org/osdu#metadataCountPattern
osdu:metadataCountPattern rdf:type owl:DatatypeProperty ;
	rdfs:comment "Total number of attributes with a pattern. " ;
	rdfs:domain osdu:AbstractQualityMetric ;
	rdfs:range xsd:decimal ;
.

###  https://w3id.org/osdu#metadataCountRequired
osdu:metadataCountRequired rdf:type owl:DatatypeProperty ;
	rdfs:comment "Total number required attributes. " ;
	rdfs:domain osdu:AbstractQualityMetric ;
	rdfs:range xsd:decimal ;
.

###  https://w3id.org/osdu#metadataCountRequiredTrue
osdu:metadataCountRequiredTrue rdf:type owl:DatatypeProperty ;
	rdfs:comment "The count of required metadata that are not populated. " ;
	rdfs:domain osdu:AbstractQualityMetric ;
	rdfs:range xsd:decimal ;
.

###  https://w3id.org/osdu#metadataCountTotal
osdu:metadataCountTotal rdf:type owl:DatatypeProperty ;
	rdfs:comment "Total number of metadata attributes for object in scope. " ;
	rdfs:domain osdu:AbstractQualityMetric ;
	rdfs:range xsd:decimal ;
.

###  https://w3id.org/osdu#metadataFormat
osdu:metadataFormat rdf:type owl:DatatypeProperty ;
	rdfs:comment "The count of total number where attribute follows the defined reference value lists. " ;
	rdfs:domain osdu:AbstractQualityMetric ;
	rdfs:range xsd:decimal ;
.

###  https://w3id.org/osdu#metadataNull
osdu:metadataNull rdf:type owl:DatatypeProperty ;
	rdfs:comment "The count of total number where metadata is not populated. " ;
	rdfs:domain osdu:AbstractQualityMetric ;
	rdfs:range xsd:decimal ;
.

###  https://w3id.org/osdu#metadataPattern
osdu:metadataPattern rdf:type owl:DatatypeProperty ;
	rdfs:comment "The count of total number of attributes that follow pattern. " ;
	rdfs:domain osdu:AbstractQualityMetric ;
	rdfs:range xsd:decimal ;
.

###  https://w3id.org/osdu#metadataScore
osdu:metadataScore rdf:type owl:DatatypeProperty ;
	rdfs:comment "The score in % for the evaluated record. " ;
	rdfs:domain osdu:AbstractQualityMetric ;
	rdfs:range xsd:decimal ;
.

###  https://w3id.org/osdu#metalRecovered
osdu:metalRecovered rdf:type owl:DatatypeProperty ;
	rdfs:comment "Metal recovered from the wellbore. " ;
	rdfs:domain osdu:Fluid ;
	rdfs:range xsd:decimal ;
.

###  https://w3id.org/osdu#methane
osdu:methane rdf:type owl:DatatypeProperty ;
	rdfs:comment "Methane (C1) concentration " ;
	rdfs:domain osdu:GasReading ;
	rdfs:range xsd:decimal ;
.

###  https://w3id.org/osdu#methodID
osdu:methodID rdf:type owl:DatatypeProperty ;
	rdfs:comment "Perforation job method, often the brand name of the service offered by the contractor " ;
	rdfs:domain osdu:PerforationJob ;
	xsd:pattern "^[\\\\w\\\\-\\\\.]+:reference-data\\\\-\\\\-PerforationIntervalType:[\\\\w\\\\-\\\\.\\\\:\\\\%]+:[0-9]*$" ;
	rdfs:range xsd:string ;
.

###  https://w3id.org/osdu#mf
osdu:mf rdf:type owl:DatatypeProperty ;
	rdfs:comment "Methyl orange alkalinity of filtrate. " ;
	rdfs:domain osdu:Fluid ;
	rdfs:range xsd:decimal ;
.

###  https://w3id.org/osdu#mfgCode
osdu:mfgCode rdf:type owl:DatatypeProperty ;
	rdfs:comment "The manufacturers code for the bit. " ;
	rdfs:domain osdu:BitRecord ;
	rdfs:range xsd:string ;
.

###  https://w3id.org/osdu#minOccurs
osdu:minOccurs rdf:type owl:DatatypeProperty ;
	rdfs:comment "Minimum number of parameter of this type required by the activity. If the minimum number of parameters is infinite, use -1 value. " ;
	rdfs:domain osdu:ParameterTemplate ;
	rdfs:range xsd:integer ;
.

###  https://w3id.org/osdu#minOffsetDistance
osdu:minOffsetDistance rdf:type owl:DatatypeProperty ;
	rdfs:comment "Horizontal distance between source and first receiver. " ;
	rdfs:domain osdu:SeismicAcquisitionSurvey ;
	rdfs:range xsd:decimal ;
.

###  https://w3id.org/osdu#minValue
osdu:minValue rdf:type owl:DatatypeProperty ;
	rdfs:comment "Minimum value of the Property " ;
	rdfs:domain osdu:GenericProperty ;
	rdfs:range xsd:decimal ;
.

###  https://w3id.org/osdu#minimum
osdu:minimum rdf:type owl:DatatypeProperty ;
	rdfs:comment "The minimum value. " ;
	rdfs:domain [
		rdf:type owl:Class ;
		owl:unionOf (
			osdu:AngleRange
			osdu:LengthRange
		) ;
	] ;
	rdfs:range xsd:decimal ;
.

###  https://w3id.org/osdu#minimumAge
osdu:minimumAge rdf:type owl:DatatypeProperty ;
	rdfs:comment "Time interval Minimum age the fault throw was active - if the link to horizon is defined, we can derive the link to horizons through geologic age " ;
	rdfs:domain osdu:FaultThrowDescriptions ;
	rdfs:range time:TemporalDuration ;
.

###  https://w3id.org/osdu#minimumBitFlowrate
osdu:minimumBitFlowrate rdf:type owl:DatatypeProperty ;
	rdfs:comment "The minimum flowrate at the bit during the run " ;
	rdfs:domain osdu:DrillingParameters ;
	rdfs:range xsd:decimal ;
.

###  https://w3id.org/osdu#minimumDepthTestStart
osdu:minimumDepthTestStart rdf:type owl:DatatypeProperty ;
	rdfs:comment "The minimum start depth for the drillstem test. Depth relative to Planned wellbore ZDP. Navigate via WellboreID to the side-car WellPlanningWellbore, which holds the depth reference in data.VerticalMeasurement. " ;
	rdfs:domain osdu:DSTRun ;
	rdfs:range xsd:decimal ;
.

###  https://w3id.org/osdu#minimumFlowratePump
osdu:minimumFlowratePump rdf:type owl:DatatypeProperty ;
	rdfs:comment "Minimum mud pump flow rate. " ;
	rdfs:domain osdu:DrillingParameters ;
	rdfs:range xsd:decimal ;
.

###  https://w3id.org/osdu#minimumInclination
osdu:minimumInclination rdf:type owl:DatatypeProperty ;
	rdfs:comment "Minimum inclination. " ;
	rdfs:domain osdu:DrillingParameters ;
	rdfs:range xsd:decimal ;
.

###  https://w3id.org/osdu#minimumInnerDiameter
osdu:minimumInnerDiameter rdf:type owl:DatatypeProperty ;
	rdfs:comment "This is the minimum inner diameter of the whole assembly. " ;
	rdfs:domain osdu:TubularAssembly ;
	rdfs:range xsd:decimal ;
.

###  https://w3id.org/osdu#minimumPumpPressure
osdu:minimumPumpPressure rdf:type owl:DatatypeProperty ;
	rdfs:comment "The minimum pump pressure used during the run " ;
	rdfs:domain osdu:DrillingParameters ;
	rdfs:range xsd:decimal ;
.

###  https://w3id.org/osdu#minimumROP
osdu:minimumROP rdf:type owl:DatatypeProperty ;
	rdfs:comment "Minimum rate of penetration through Interval. " ;
	rdfs:domain osdu:DrillingParameters ;
	rdfs:range xsd:decimal ;
.

###  https://w3id.org/osdu#minimumRpm
osdu:minimumRpm rdf:type owl:DatatypeProperty ;
	rdfs:comment "Minimum turn rate (commonly in rpm). " ;
	rdfs:domain osdu:DrillingParameters ;
	rdfs:range xsd:decimal ;
.

###  https://w3id.org/osdu#minimumThickness
osdu:minimumThickness rdf:type owl:DatatypeProperty ;
	rdfs:comment "The minimum thickness of the StratigraphicUnitInterpretation. " ;
	rdfs:domain osdu:StratigraphicUnitInterpretation ;
	rdfs:range xsd:decimal ;
.

###  https://w3id.org/osdu#minimumTorqueOnBottom
osdu:minimumTorqueOnBottom rdf:type owl:DatatypeProperty ;
	rdfs:comment "Minimum torque: on bottom. " ;
	rdfs:domain osdu:DrillingParameters ;
	rdfs:range xsd:decimal ;
.

###  https://w3id.org/osdu#minimumVolume
osdu:minimumVolume rdf:type owl:DatatypeProperty ;
	rdfs:comment "Minimum expected  volume pumped at specified pressure " ;
	rdfs:domain osdu:ExpectedVolume ;
	rdfs:range xsd:decimal ;
.

###  https://w3id.org/osdu#minimumWOB
osdu:minimumWOB rdf:type owl:DatatypeProperty ;
	rdfs:comment "Weight on bit - minimum. " ;
	rdfs:domain osdu:DrillingParameters ;
	rdfs:range xsd:decimal ;
.

###  https://w3id.org/osdu#minorAxis
osdu:minorAxis rdf:type owl:DatatypeProperty ;
	rdfs:comment "Measured length of the target perpendicular to Target Ref Azimuth, assumed to be on target dip, strike, rotation plane. " ;
	rdfs:domain osdu:Geometry ;
	rdfs:range xsd:decimal ;
.

###  https://w3id.org/osdu#misfires
osdu:misfires rdf:type owl:DatatypeProperty ;
	rdfs:comment "Total number of gun / charge misfires " ;
	rdfs:domain osdu:PerforationInterval ;
	rdfs:range xsd:integer ;
.

###  https://w3id.org/osdu#missing
osdu:missing rdf:type owl:DatatypeProperty ;
	rdfs:domain osdu:Markers ;
	rdfs:range xsd:string ;
.

###  https://w3id.org/osdu#mixedStringIndicator
osdu:mixedStringIndicator rdf:type owl:DatatypeProperty ;
	rdfs:comment "A YES or NO flag indicating the assembly is a mixed string. The length of the assembly may be made up of joints with different tensile strengths, or collapse resistance and yield strengths. " ;
	rdfs:domain osdu:TubularAssembly ;
	xsd:pattern "^YES|NO$" ;
	rdfs:range xsd:string ;
.

###  https://w3id.org/osdu#mnemonic
osdu:mnemonic rdf:type owl:DatatypeProperty ;
	rdfs:comment "The Mnemonic of the Log Curve is the value as received either from Raw Providers or from Internal Processing team " ;
	rdfs:domain osdu:Curves ;
	rdfs:range xsd:string ;
.

###  https://w3id.org/osdu#model
osdu:model rdf:type owl:DatatypeProperty ;
	rdfs:comment "Name of the component Model as defined per the operating company " ;
	rdfs:domain osdu:TubularComponent ;
	rdfs:range xsd:string ;
.

###  https://w3id.org/osdu#modelFeatureID
osdu:modelFeatureID rdf:type owl:DatatypeProperty ;
	rdfs:comment "The scope of this local model feature can be extended by this relationship to a master-data ModelFeature with wider or global scope. " ;
	rdfs:domain osdu:LocalModelFeature ;
	xsd:pattern "^[\\\\w\\\\-\\\\.]+:master-data\\\\-\\\\-ModelFeature:[\\\\w\\\\-\\\\.\\\\:\\\\%]+:[0-9]*$" ;
	rdfs:range xsd:string ;
.

###  https://w3id.org/osdu#modifyTime
osdu:modifyTime rdf:type owl:DatatypeProperty ;
	rdfs:comment "Timestamp of the time at which this version of the OSDU resource object was created. Set by the System. The value is a combined date-time string in ISO-8601 given in UTC. " ;
	rdfs:domain osdu:System ;
	rdfs:range time:DateTimeDescription ;
.

###  https://w3id.org/osdu#modifyUser
osdu:modifyUser rdf:type owl:DatatypeProperty ;
	rdfs:comment "The user reference, which created this version of this resource object. Set by the System. " ;
	rdfs:domain osdu:System ;
	rdfs:range acl:AuthenticatedAgent ;
.

###  https://w3id.org/osdu#mudClass
osdu:mudClass rdf:type owl:DatatypeProperty ;
	rdfs:comment "The class of the drilling fluid. " ;
	rdfs:domain [
		rdf:type owl:Class ;
		owl:unionOf (
			osdu:Fluid
			osdu:DrillingParameters
		) ;
	] ;
	xsd:pattern "^[\\\\w\\\\-\\\\.]+:reference-data\\\\-\\\\-MudClass:[\\\\w\\\\-\\\\.\\\\:\\\\%]+:[0-9]*$" ;
	rdfs:range xsd:string ;
.

###  https://w3id.org/osdu#mudEngineer
osdu:mudEngineer rdf:type owl:DatatypeProperty ;
	rdfs:comment "The name of the Mud Engineer " ;
	rdfs:domain osdu:Fluid ;
	rdfs:range xsd:string ;
.

###  https://w3id.org/osdu#mudLostVolumeAbandonDownhole
osdu:mudLostVolumeAbandonDownhole rdf:type owl:DatatypeProperty ;
	rdfs:comment "Mud volume lost downhole during abandonment. " ;
	rdfs:domain osdu:MudLosses ;
	rdfs:range xsd:decimal ;
.

###  https://w3id.org/osdu#mudLostVolumeBehindCasingDownhole
osdu:mudLostVolumeBehindCasingDownhole rdf:type owl:DatatypeProperty ;
	rdfs:comment "Mud volume lost downhole behind casing. " ;
	rdfs:domain osdu:MudLosses ;
	rdfs:range xsd:decimal ;
.

###  https://w3id.org/osdu#mudLostVolumeCasingHole
osdu:mudLostVolumeCasingHole rdf:type owl:DatatypeProperty ;
	rdfs:comment "Mud volume lost at the time of the report. Captures volumes of mud lost for specific activities or onsite locations and total volumes for surface and down hole. " ;
	rdfs:domain osdu:MudLosses ;
	rdfs:range xsd:decimal ;
.

###  https://w3id.org/osdu#mudLostVolumeCementingDownhole
osdu:mudLostVolumeCementingDownhole rdf:type owl:DatatypeProperty ;
	rdfs:comment "Mud volume lost downhole while cementing. " ;
	rdfs:domain osdu:MudLosses ;
	rdfs:range xsd:decimal ;
.

###  https://w3id.org/osdu#mudLostVolumeCirculatingDownhole
osdu:mudLostVolumeCirculatingDownhole rdf:type owl:DatatypeProperty ;
	rdfs:comment "Mud volume lost downhole while circulating. " ;
	rdfs:domain osdu:MudLosses ;
	rdfs:range xsd:decimal ;
.

###  https://w3id.org/osdu#mudLostVolumeMeasureDepthBase
osdu:mudLostVolumeMeasureDepthBase rdf:type owl:DatatypeProperty ;
	rdfs:comment "Bottom measured depth for which the mud loss reading was occurred " ;
	rdfs:domain osdu:MudLosses ;
	rdfs:range xsd:decimal ;
.

###  https://w3id.org/osdu#mudLostVolumeMeasureDepthTop
osdu:mudLostVolumeMeasureDepthTop rdf:type owl:DatatypeProperty ;
	rdfs:comment "Top measured depth for which the mud loss reading was occurred " ;
	rdfs:domain osdu:MudLosses ;
	rdfs:range xsd:decimal ;
.

###  https://w3id.org/osdu#mudLostVolumeMudCleanerSurface
osdu:mudLostVolumeMudCleanerSurface rdf:type owl:DatatypeProperty ;
	rdfs:comment "Volume of mud lost in mud cleaning equipment (at surface). " ;
	rdfs:domain osdu:MudLosses ;
	rdfs:range xsd:decimal ;
.

###  https://w3id.org/osdu#mudLostVolumeOtherLocationDownhole
osdu:mudLostVolumeOtherLocationDownhole rdf:type owl:DatatypeProperty ;
	rdfs:comment "Mud volume lost downhole from other location. " ;
	rdfs:domain osdu:MudLosses ;
	rdfs:range xsd:decimal ;
.

###  https://w3id.org/osdu#mudLostVolumeOtherLocationSurface
osdu:mudLostVolumeOtherLocationSurface rdf:type owl:DatatypeProperty ;
	rdfs:comment "Surface volume lost other location. " ;
	rdfs:domain osdu:MudLosses ;
	rdfs:range xsd:decimal ;
.

###  https://w3id.org/osdu#mudLostVolumePitsSurface
osdu:mudLostVolumePitsSurface rdf:type owl:DatatypeProperty ;
	rdfs:comment "Volume of mud lost in pit room (at surface). " ;
	rdfs:domain osdu:MudLosses ;
	rdfs:range xsd:decimal ;
.

###  https://w3id.org/osdu#mudLostVolumeShakerSurface
osdu:mudLostVolumeShakerSurface rdf:type owl:DatatypeProperty ;
	rdfs:comment "Volume of mud lost at shakers (at surface). " ;
	rdfs:domain osdu:MudLosses ;
	rdfs:range xsd:decimal ;
.

###  https://w3id.org/osdu#mudLostVolumeTrippingSurface
osdu:mudLostVolumeTrippingSurface rdf:type owl:DatatypeProperty ;
	rdfs:comment "Volume of mud lost while tripping (at surface). " ;
	rdfs:domain osdu:MudLosses ;
	rdfs:range xsd:decimal ;
.

###  https://w3id.org/osdu#mudLostVolumeTvdBase
osdu:mudLostVolumeTvdBase rdf:type owl:DatatypeProperty ;
	rdfs:comment "Bottom true vertical depth interval over which the mud loss reading was occurred " ;
	rdfs:domain osdu:MudLosses ;
	rdfs:range xsd:decimal ;
.

###  https://w3id.org/osdu#mudLostVolumeTvdTop
osdu:mudLostVolumeTvdTop rdf:type owl:DatatypeProperty ;
	rdfs:comment "Top  true vertical depth interval over which the mud loss reading was occurred " ;
	rdfs:domain osdu:MudLosses ;
	rdfs:range xsd:decimal ;
.

###  https://w3id.org/osdu#mudPh
osdu:mudPh rdf:type owl:DatatypeProperty ;
	rdfs:comment "Mud pH. " ;
	rdfs:domain osdu:Fluid ;
	rdfs:range xsd:decimal ;
.

###  https://w3id.org/osdu#mudTempPh
osdu:mudTempPh rdf:type owl:DatatypeProperty ;
	rdfs:comment "Mud pH measurement temperature. " ;
	rdfs:domain osdu:Fluid ;
	rdfs:range xsd:decimal ;
.

###  https://w3id.org/osdu#mudVolumeBuilt
osdu:mudVolumeBuilt rdf:type owl:DatatypeProperty ;
	rdfs:comment "Volume of mud built. " ;
	rdfs:domain osdu:MudVolume ;
	rdfs:range xsd:string ;
.

###  https://w3id.org/osdu#mudVolumeCasing
osdu:mudVolumeCasing rdf:type owl:DatatypeProperty ;
	rdfs:comment "Volume of mud contained in casing annulus. " ;
	rdfs:domain osdu:MudVolume ;
	rdfs:range xsd:decimal ;
.

###  https://w3id.org/osdu#mudVolumeDumped
osdu:mudVolumeDumped rdf:type owl:DatatypeProperty ;
	rdfs:comment "Volume of mud dumped. " ;
	rdfs:domain osdu:MudVolume ;
	rdfs:range xsd:decimal ;
.

###  https://w3id.org/osdu#mudVolumeEnd
osdu:mudVolumeEnd rdf:type owl:DatatypeProperty ;
	rdfs:comment "Volume of mud at the end of the report interval (including pits and hole). " ;
	rdfs:domain osdu:MudVolume ;
	rdfs:range xsd:decimal ;
.

###  https://w3id.org/osdu#mudVolumeHole
osdu:mudVolumeHole rdf:type owl:DatatypeProperty ;
	rdfs:comment "Volume of mud contained in the openhole annulus. " ;
	rdfs:domain osdu:MudVolume ;
	rdfs:range xsd:decimal ;
.

###  https://w3id.org/osdu#mudVolumeMeasureDepthBase
osdu:mudVolumeMeasureDepthBase rdf:type owl:DatatypeProperty ;
	rdfs:comment "Bottom measured depth for which the mud volume reading was conducted " ;
	rdfs:domain osdu:MudVolume ;
	rdfs:range xsd:decimal ;
.

###  https://w3id.org/osdu#mudVolumeMeasureDepthTop
osdu:mudVolumeMeasureDepthTop rdf:type owl:DatatypeProperty ;
	rdfs:comment "Top measured depth for which the mud volume reading was conducted " ;
	rdfs:domain osdu:MudVolume ;
	rdfs:range xsd:decimal ;
.

###  https://w3id.org/osdu#mudVolumeReceived
osdu:mudVolumeReceived rdf:type owl:DatatypeProperty ;
	rdfs:comment "Volume of mud received from mud warehouse. " ;
	rdfs:domain osdu:MudVolume ;
	rdfs:range xsd:decimal ;
.

###  https://w3id.org/osdu#mudVolumeReturned
osdu:mudVolumeReturned rdf:type owl:DatatypeProperty ;
	rdfs:comment "Volume of mud returned to mud warehouse. " ;
	rdfs:domain osdu:MudVolume ;
	rdfs:range xsd:decimal ;
.

###  https://w3id.org/osdu#mudVolumeRiser
osdu:mudVolumeRiser rdf:type owl:DatatypeProperty ;
	rdfs:comment "Volume of mud contained in riser section annulus. " ;
	rdfs:domain osdu:MudVolume ;
	rdfs:range xsd:decimal ;
.

###  https://w3id.org/osdu#mudVolumeStart
osdu:mudVolumeStart rdf:type owl:DatatypeProperty ;
	rdfs:comment "Volume of mud at start of report interval (including pits and hole). " ;
	rdfs:domain osdu:MudVolume ;
	rdfs:range xsd:decimal ;
.

###  https://w3id.org/osdu#mudVolumeString
osdu:mudVolumeString rdf:type owl:DatatypeProperty ;
	rdfs:comment "Volume of mud contained within active string. " ;
	rdfs:domain osdu:MudVolume ;
	rdfs:range xsd:decimal ;
.

###  https://w3id.org/osdu#mudVolumeTvdBase
osdu:mudVolumeTvdBase rdf:type owl:DatatypeProperty ;
	rdfs:comment "Bottom true vertical depth interval over which the mud volume reading was conducted. " ;
	rdfs:domain osdu:MudVolume ;
	rdfs:range xsd:decimal ;
.

###  https://w3id.org/osdu#mudVolumeTvdTop
osdu:mudVolumeTvdTop rdf:type owl:DatatypeProperty ;
	rdfs:comment "Top  true vertical depth interval over which the mud volume reading was conducted. " ;
	rdfs:domain osdu:MudVolume ;
	rdfs:range xsd:decimal ;
.

###  https://w3id.org/osdu#n
osdu:n rdf:type owl:DatatypeProperty ;
	rdfs:comment "Power Law index (Power Law and HB). " ;
	rdfs:domain osdu:CementingFluid ;
	rdfs:range xsd:decimal ;
.

###  https://w3id.org/osdu#name
osdu:name rdf:type owl:DatatypeProperty ;
	rdfs:comment "The name of the object. " ;
	rdfs:domain [
		rdf:type owl:Class ;
		owl:unionOf (
			osdu:FrameOfReferenceUOM
			osdu:FrameOfReferenceCRS
			osdu:FrameOfReferenceDateTime
			osdu:FrameOfReferenceAzimuthReference
			osdu:AbstractContact
			osdu:AbstractDataset
			osdu:AbstractFileSourceInfo
			osdu:AbstractWorkProductComponent
			osdu:AbstractReferenceType
			osdu:AbstractPropertyType
			osdu:DataCollection
			osdu:FluidsProgram
			osdu:ModelFeature
			osdu:WellPlanningWellbore
			osdu:FluidsReport
			osdu:RockSample
			osdu:RiskResponse
			osdu:Risk
			osdu:WellPlanningWell
			osdu:Target
			osdu:GeometricTargetSet
			osdu:RockVolumeFeature
			osdu:ReferenceLevel
			osdu:SurveySection
			osdu:ActivityTemplateArc
			osdu:WellboreArchitecture
			osdu:ActivityTemplate
			osdu:CasingDesign
			osdu:OperationsReport
			osdu:BHARun
			osdu:PointsSource
			osdu:PerforationJob
			osdu:WellPlanningActivity
			osdu:ActivityPlan
			osdu:MudPump
			osdu:PerforationInterval
			osdu:BoundaryFeature
			osdu:Coring
			osdu:HoleSection
			osdu:PlannedCementJob
			osdu:ConnectedSourceRegistryEntry
			osdu:SecurityScheme
			osdu:ConnectedSourceDataJob
			osdu:WorkflowParameter
			osdu:Type
			osdu:MarkerProperty
			osdu:Curve
			osdu:QualityDataRuleSet
			osdu:Method
			osdu:ConcatenatedTransformation
			osdu:SourceCRS
			osdu:TargetCRS
			osdu:Usage
			osdu:Extent
			osdu:Scope
			osdu:PreferredUsage
			osdu:HorizontalCRS
			osdu:VerticalCRS
			osdu:Transformation
			osdu:Datum
			osdu:DatumEnsemble
			osdu:Projection
			osdu:BaseCRS
			osdu:CoordinateSystem
			osdu:Configuration
			osdu:WorkProduct
		) ;
	] ;
	rdfs:range xsd:string ;
	owl:sameAs foaf:name ;
.

###  https://w3id.org/osdu#nameCementedString
osdu:nameCementedString rdf:type owl:DatatypeProperty ;
	rdfs:comment "Name for the cemented string " ;
	rdfs:domain osdu:PlannedCementJob ;
	rdfs:range xsd:string ;
.

###  https://w3id.org/osdu#namespaceID
osdu:namespaceID rdf:type owl:DatatypeProperty ;
	rdfs:comment "A namespace reference grouping a list of records with the goal of providing unique look-ups by Name/Code. It is strongly recommended to make the NamespaceID's code part of the system property id. " ;
	rdfs:domain [
		rdf:type owl:Class ;
		owl:unionOf (
			osdu:ExternalUnitOfMeasure
			osdu:ExternalUnitQuantity
		) ;
	] ;
	xsd:pattern "^[\\\\w\\\\-\\\\.]+:reference-data\\\\-\\\\-ExternalCatalogNamespace:[\\\\w\\\\-\\\\.\\\\:\\\\%]+:[0-9]*$" ;
	rdfs:range xsd:string ;
.

###  https://w3id.org/osdu#naturalKeys
osdu:naturalKeys rdf:type owl:DatatypeProperty ;
	rdfs:comment "Identifies the natural keys if declared. The keys are identified via the dot notation; example: assume the ProjectName is the natural key for a SeismicAcquisitionSurvey then the natural key reference would be [data.ProjectName]. " ;
	rdfs:domain osdu:Type ;
	rdfs:range xsd:string ;
.

###  https://w3id.org/osdu#negativeVerticalDelta
osdu:negativeVerticalDelta rdf:type owl:DatatypeProperty ;
	rdfs:comment "The distance vertically below the Marker position that marks the limit of the high confidence range for the Marker pick. " ;
	rdfs:domain osdu:Markers ;
	rdfs:range xsd:decimal ;
.

###  https://w3id.org/osdu#nestedIndexableElementID
osdu:nestedIndexableElementID rdf:type owl:DatatypeProperty ;
	rdfs:comment "The topological element kind nested inside the first given indexable element kind  which are selected. For example, it allows to select all top front left corner of all cells of an IJK grid " ;
	rdfs:domain osdu:SubRepresentation ;
	xsd:pattern "^[\\\\w\\\\-\\\\.]+:reference-data\\\\-\\\\-IndexableElement:[\\\\w\\\\-\\\\.\\\\:\\\\%]+:[0-9]*$" ;
	rdfs:range xsd:string ;
.
